

\subsection*{c)}

\begin{equation*}
\Delta S = \sum_{i} \frac{\dot{Q}_i}{T_i} + \dot{S}_{\text{erz}} \quad \Rightarrow \quad \dot{S}_{\text{erz}} = - \frac{\dot{Q}_{\text{aus}}}{T_{\text{UF}}} = \frac{62.182 \text{kW}}{293.12 \text{K}} = 212.139 \frac{\text{W}}{\text{K}}
\end{equation*}

``````latex

1. 
\[
\frac{DE}{QE} = \sum_i^j m_i(t) h_i(t) + \sum_i^j q_e:(t) + \sum_i^j c_i(t) - \sum_i^j w_i(t)
\]

\[
\Delta E = m_2 u_2 - m_1 u_1 = \sum_i^j Q_i = Q_{aus2} = 35MJ
\]

\[
m_2 = m_1 + \Delta m \quad m_2 = 5755kg \quad m_{AB} = x \cdot m_1 \quad m_{NB} = m_1 (1 - x) \quad m_2 = \Delta m
\]

\[
u_{1f} [EOC] = 250.65 \frac{u}{kg}
\]

\[
u_{1pf} [200^\circ C] = 42.94 \frac{u}{kg}
\]

\[
u_{2pf} [200^\circ C] = 292.95 \frac{u}{kg}
\]

\[
u_{3f} [200^\circ C] = 87.95 \frac{u}{kg}
\]

\[
\Delta t = m_3 \cdot u_3 + m_2 u_2 - m_1 u_1 = 35MJ = \Delta m u_3 + m_2 u_2 + \Delta m u_2 - m_1 u_1
\]

\[
\frac{m_1 u_1 - m_1 u_2}{u_3 + u_2} = \frac{m_{A1} u_{A1} + m_{A1} u_{A1} - m_1 u_{2pf} + 35MJ}{u_{3f} + u_{2f}}
\]

\[
= \frac{0.005 + 5755kg \cdot 250.65 \frac{u}{kg} + 5755kg \cdot (1 - 0.005) \cdot 42.94 \frac{u}{kg} - 5755kg \cdot 292.95 \frac{u}{kg}}{87.95 \frac{u}{kg} + 292.95 \frac{u}{kg}}
\]

\[
\Delta m_2 = 2.176.02kg
\]