

\subsection*{a)}

\begin{equation*}
\frac{\partial E}{\partial t} = \sum_{i} \dot{m}_i(t) \left[ h_i(t) + \frac{c_i^2(t)}{2} + g z_i(t) \right] - \sum_{e} \dot{m}_e(t) \left[ h_e(t) + \frac{c_e^2(t)}{2} + g z_e(t) \right] + \sum_{i} \dot{Q}_i(t) - \sum_{e} \dot{Q}_e(t) - \dot{m}(t)
\end{equation*}

\begin{equation*}
0 = \dot{m} (h_e - h_a) + \dot{Q}_{\text{aus}} - \dot{Q}_{\text{aus}} \quad \Rightarrow \quad \dot{Q}_{\text{aus}} = \dot{m} (h_e - h_a) + \dot{Q}_R
\end{equation*}

\begin{equation*}
h_e [\text{20°C+1 bar}] = 292.98 \frac{\text{kJ}}{\text{kg}} \quad \text{Aus TAB A-2}
\end{equation*}

\begin{equation*}
h_u [\text{200°C+1 bar}] = 419.94 \frac{\text{kJ}}{\text{kg}} \quad \text{Aus TAB A-2}
\end{equation*}

\begin{equation*}
\dot{Q}_{\text{aus}} = 0.3 \frac{\text{kg}}{\text{s}} \left[ (292.98 \frac{\text{kJ}}{\text{kg}}) - (419.94 \frac{\text{kJ}}{\text{kg}}) \right] + 100 \text{kW} = 62.182 \text{kW}
\end{equation*}