c)

\[
\dot{m} (\cancel{h_a} - h_o - T_o (s_{1} - s_{6}) + \Delta k)_{12}
\]

\[
T_o = 243,15 K
\]

\[
\Delta e_{x,str} = \dot{m} (h_e - h_s)
\]

\[
\dot{m} \left( h_e + h_o - T_o (s_6 - s_o) + k_e \right) - \dot{m} \left( h_s - h_o - T_o (s_5 - s_o) + k_{e5} \right) =
\]

\[
= \dot{m} \left( h_e - h_s - T_o (s_6 - s_5) + \frac{w_{e}^{2} - w_{s}^{2}}{2} \right)
\]

\[
h_e - h_s = \int_{T_o}^{T_o} c_p dT = 1,006 \left( 328,07 + 243,15 \right) = 243,15 \frac{kJ}{kg}
\]

\[
s_6 - s_5 = \int_{T_o}^{T_o} \frac{c_p}{T} dT - R \ln \left( \frac{p_o}{p_o} \right) =
\]

\[
= 1,006 \ln \left( \frac{328,07}{243,15} \right) - 1,725 \cancel{\frac{kJ}{kgK}} \left( \ln \left( \frac{4}{1} \right) \right)
\]

\[
= 0,301 \frac{kJ}{kgK}
\]

\[
\Delta E_{x,str} = \dot{m}_{ges} \left( 85,43 \frac{kJ}{kg} - 243,15 \frac{kJ}{kg} \cdot 0,301 \frac{kJ}{kgK} \right)
\]

\[
= \dot{m}_{ges} \left( 24659,122 \frac{kJ}{kg} \right) \quad e_x = 24659,122 \frac{kJ}{kg}
\]