b) 
\[
\bar{T}_{\text{KF}} = \frac{\int_{s_a}^{s_e} T ds}{s_e - s_a}
\]

\[
s_e - s_a = \int_{T_a}^{T_e} c \frac{1}{T} dT = c \ln \left( \frac{T_e}{T_a} \right)
\]

\[
\int_{s_a}^{s_e} T ds = \Delta H = h_e - h_a = \int_{T_a}^{T_e} c dT + v^3 \left( p_e - p_a \right)
\]

\[
\Rightarrow \frac{c \left( T_e - T_a \right)}{c \ln \left( \frac{T_e}{T_a} \right)} \Rightarrow \bar{T}_{\text{KF}} \quad | : c
\]

\[
\bar{T}_{\text{KF}} = \frac{T_e - T_a}{\ln \left( \frac{T_e}{T_a} \right)}
\]

\[
T_{\text{kein}} = 298.15 \\
T_{\text{kaus}} = 298.15
\]

\[
\frac{298.15 - 298.15}{\ln \left( \frac{298.15}{298.15} \right)} = 293.12\,K = \bar{T}_{\text{KF}}
\]