

\subsection*{c)}

\[
e_{x,str,c} - e_{x,str,0} = h_6 - h_0 - T_0 (S_6 - S_0) + \frac{w_6^2}{2} - \frac{w_0^2}{2}
\]

\[
\Rightarrow w_0 = 200 \frac{m}{s}, \quad w_6 = 510 \frac{m}{s}, \quad h_6 - h_0 = c_p (T_6 - T_0) = 1.006 \frac{kJ}{kgK} (340 K - 243.15 K) = 97.43 \frac{kJ}{kg}
\]

\[
S_6 - S_0 = c_p \ln \left( \frac{T_6}{T_0} \right) - R \ln \left( \frac{P_6}{P_0} \right) = 1.006 \frac{kJ}{kgK} \ln \left( \frac{340 K}{243.15 K} \right) = 0.337 \frac{kJ}{kgK}
\]

\[
e_{x,str,c} - e_{x,str,0} = 97.43 - 243.15 K (0.337 \frac{kJ}{kgK}) + \frac{510 \frac{m}{s}^2}{2} - \frac{200 \frac{m}{s}^2}{2} =
\]

\[
\Delta e_{x,str} = 125.47 \frac{kJ}{kg}
\]

``````latex


\section*{Solution}

\begin{itemize}