d) \\
\[
M_2 h_2 - M_1 h_1 = \Delta M_{12} h_{ein} + Q_{Rm}
\]
\[
\Rightarrow M_2 h_2 = M_1 + \Delta M_{12} = Q_{Rm} = M_1 (h_2 - h_1) + \Delta M_{12} (h_2 - h_{12,ein})
\]
\[
\Rightarrow \Delta M_{12} = \frac{Q_{R,12} - M_1 (h_2 - h_1)}{h_{12,ein} - h_{ein}} = \frac{U_2 - U_{ein}}{7_{TAB-A2}} = U_2 = U_f (20^\circ C) = 292.95 \frac{kJ}{kg}
\]
\[
U_f = U_f (100^\circ C) + x_0 (U_g (100^\circ C) - U_f (100^\circ C)) = 419.34 \frac{kJ}{kg} + 0.005 (2506.5 - 419.34) \frac{kJ}{kg} = 429.37 \frac{kJ}{kg}
\]
\[
h_g = 429.37 \frac{kJ}{kg} \quad h_{ein} = h_f (20^\circ C) 7_{TAB-A2} = 83.96 \frac{kJ}{kg}
\]
\[
\Delta U_{12} = \frac{35.000 \frac{kJ}{s} - 5.755 \frac{kg}{s} (292.95 - 429.37) \frac{kJ}{kg}}{83.96 \frac{kJ}{kg}} = 392.4 \frac{kg}{s}
\]