c) Zunahme der Str√∂mungsenergie:

\[
e_{x,stro} - e_{r,stro} = v_r (s_{r} - s_{6}) + \Delta e_{ke} \quad \Rightarrow \quad e_{x,stro} - e_{r,stro} = \left[ h_6 - h_0 - T_0 (s_6 - s_0) + \frac{w_6^2}{2} - \frac{w_0^2}{2} \right]
\]

\[
s_6 - s_0 = \int_{T_0}^{T} \frac{c_p}{T} dT = R \ln \left( \frac{p_6}{p_0} \right) \quad \Rightarrow \quad s_6 - s_0 = \int_{T_0}^{T_0} \frac{c_p}{T} dT = c_p \ln \left( \frac{T_0}{T_0} \right) = 0.30 \, \frac{kJ}{kg}
\]

\[
s_0 - s_6 = c_p \ln \left( \frac{T_0}{T_6} \right) = -0.30 \, \frac{kJ}{kg}
\]

\[
\frac{w_6^2}{2} - \frac{w_0^2}{2} = \frac{w_6^2}{2} - \frac{w_0^2}{2} = 10.8 \cdot 10^3 \, \frac{kJ}{kg}
\]

\[
h_0 - h_6 = c_p (T_0 - T_6) = -95.43 \, \frac{kJ}{kg} \quad \Rightarrow \quad h_6 - h_0 = 95.43 \, \frac{kJ}{kg}
\]

\[
\text{total:} \quad e_{x,stro} - e_{r,stro} = 95.43 \, \frac{kJ}{kg} - 243.15 \left( 0.30 \right) - 10.8 \cdot 653 = -96.41 \, \frac{kJ}{kg}
\]

``````latex