\section*{1 b)}
\begin{equation}
0 = \dot{m} (h_{\text{ein}} - h_{\text{aus}}) + \dot{Q}_{\text{aus}}
\end{equation}
\begin{equation}
0 = \dot{m} (h_{\text{ein}} - h_{\text{aus}}) - \dot{Q} + \dot{Q}_R
\end{equation}
\begin{equation}
\dot{Q}_{\text{aus}} = \dot{m} (h_{\text{ein}} - h_{\text{aus}}) + \dot{Q}_R
\end{equation}

\subsection*{T-Az}
\begin{align*}
h_{\text{ein}} @ 70^\circ C &= 292.98 \, \frac{\text{kJ}}{\text{kg}} \\
h_{\text{aus}} @ 100^\circ C &= 418.04 \, \frac{\text{kJ}}{\text{kg}}
\end{align*}

\subsection*{FAZ}
\begin{align*}
h_{\text{ein}} \cdot \dot{m} @ 70^\circ C / x = 0.005 &= 364.64 \, \frac{\text{kJ}}{\text{kg}} \\
h_{\text{aus}} = h @ 100^\circ C / x = 0.005 &= 421.1 \, \frac{\text{kJ}}{\text{kg}}
\end{align*}

\begin{equation}
\dot{Q}_{\text{aus}} = 66.24 \, \text{kW}
\end{equation}
\begin{equation}
\dot{Q}_{\text{aus}} = 65.05 \, \text{kW}
\end{equation}

``````latex



\section*{b)}

\[
\overline{T} = \frac{\Delta h}{\Delta S}, \quad \text{da ideale Fl√ºssigkeil}
\]

\[
\overline{T} = \frac{T_2 - T_1}{\ln \left( \frac{T_2}{T_1} \right)} = \boxed{203.12 \, \text{K} = \overline{T}}
\]