

\section*{d)}

\[
\Delta m_2 u_2 - m_1 u_1 = \Delta m_2 (h_2) + \dot{q} - \dot{W}
\]

\[
(m_1 + \Delta m_2) u_2 - m_1 u_1 = \Delta m_2 (h_2 - h_1) + \dot{q}
\]

\[
= \Delta m_2 c_p (T_2 - T_1) + \dot{q}
\]

\[
(m_1 + \Delta m_2) u_2 - m_1 u_1
\]

\[
m_1 (h_2 - u_1) - \dot{Q} = \Delta m_2 (c_p (T_2 - T_1) + m_1 u_2
\]

\[
m_1 c_v (T_2 - T_1)
\]

``````latex

\section*{1.d}

\begin{align*}
(m_1 + \Delta m_{12}) u_2 - m_1 u_1 &= \Delta m_{12} c_p (T_2 - T_1) + Q \\
m_1 (u_2 - u_1) + Q &= \Delta m_{12} \left[ c_p (T_2 - T_1) + u_2 \right] \\
m_1 c_v (T_2 - T_1) + Q &= \Delta m_{12} \\
c_p (T_2 - T_1) + u_2 &= \Delta m_{12}
\end{align*}