

\section*{c)}

\[
0 = \dot{m} (s_{\text{ein}} - s_{\text{aus}}) + \frac{Q}{\overline{T}} + \dot{S}_{\text{Erz}}
\]

\[
-\dot{S}_{\text{Erz}} = -\dot{m} (s_{\text{ein}} - s_{\text{aus}}) - \frac{Q_{\text{aw}}}{T_{\text{R}}} - \frac{Q_{\text{aus}}}{T_{\text{KF}}} - \frac{Q_{\text{R}}}{373.15}
\]

\[
T - T_{\text{A2}}
\]

\[
s_{\text{ein}} - s_f @ 70^\circ \text{C} = 0.93479
\]

\[
s_{\text{aus}} - s_f @ 100^\circ \text{C} = 1.3069
\]

\[
= 0.06 \, \frac{\text{kJ}}{\text{kg} \cdot \text{K}}
\]

\[
\dot{S}_{\text{Erz}} = 0 = \dot{m} (s_{\text{ein}} - s_{\text{aus}}) + \frac{Q}{\overline{T}} + \dot{S}_{\text{Erz}}
\]

\[
\dot{S}_{\text{Erz}} = \left( \dot{m} (s_{\text{ein}} - s_{\text{aus}}) - \frac{Q_{\text{aus}}}{T_{\text{R}}} + \frac{Q_{\text{aw}}}{\overline{T}} \right)
\]

\[
= 0.057 \, \frac{\text{kJ}}{\text{kg} \cdot \text{K}}
\]