

\section*{d)}
\begin{align*}
Q &= \sum ex_{str} + \sum ex_q - \sum W - \frac{av}{P_0 a_0} - ex_{verl} \\
0 &= \dot{m}(s_0 - s_a) + \frac{\dot{Q}}{T} + S_{elvz} \\
S_{elvz} &= S_6 - S_0 \quad \text{da ideales gas} \\
&= S^0(T_6) - S^0(T_0) - R \ln \left( \frac{P_6}{P_0} \right) \\
&\quad \text{, da } P_6 = P_0 \\
\dot{e}_{ex,verl} &= T_0 \cdot S_{elvz}
\end{align*}

``````latex

2.

d)

\[
s(T_1) = s^0(T_1)
\]

\[
\begin{aligned}
s^0(1240 \, \text{K}) & \quad \text{interpolieren auf} \quad s^0(1243.15 \, \text{K}) = 243.17 \, \frac{\text{kJ}}{\text{kg} \cdot \text{K}} \\
s^0(1250 \, \text{K}) & \\
\\
s^0(325 \, \text{K}) & \quad \text{interpolieren auf} \quad s^0(328.71 \, \text{K}) = 328.39 \, \frac{\text{kJ}}{\text{kg} \cdot \text{K}} \\
s^0(330 \, \text{K}) & \\
\end{aligned}
\]

\[
\dot{s}_{erz} = 85.22 \, \frac{\text{kJ}}{\text{kg} \cdot \text{K}}
\]

\[
\Rightarrow \, ex_{ver1} = T_0 \cdot \dot{s}_{erz} = 20.723 \, \frac{\text{MJ}}{\text{kg}}
\]

``````latex