

\subsection*{a)}

\begin{equation*}
0 = \dot{m} \left[ h_{in} - h_{out} \right] + \dot{Q}_R - \dot{Q}_{out}
\end{equation*}

\begin{equation*}
\dot{Q}_{out} = \dot{m} \left[ h_{out} - h_{in} \right] + \dot{Q}_R
\end{equation*}

\begin{equation*}
h_{in} = h_{A} (e \ 70^\circ C \rightarrow A-2) = 292.98 \ \frac{kJ}{kg}
\end{equation*}

\begin{equation*}
h_{out} = h_{A} (e \ 100^\circ C \rightarrow A-2) = 479.04 \ \frac{kJ}{kg}
\end{equation*}

\begin{equation*}
\Rightarrow \dot{Q}_{out} = \text{(scratched out)} \ 62.182 \ kW
\end{equation*}