

\section*{1d}
\Delta U = \dot{m} (h_{\text{ein,1z}}) + 35 \text{MJ} \\
\Delta Q = \dot{m}_{\text{gr}} (u_2 - u_1) , \quad Q_2 = x_D u_g + (1 - x_D) u_f \\
u_2 \Rightarrow \text{TAB1: } 203.82 \frac{\text{kJ}}{\text{kg}} \\
u_1 \Rightarrow \text{TAB1: } 929.88 \frac{\text{kJ}}{\text{kg}} \\
-693.8 \text{MJ} = \Delta m h_{\text{ein,1z}} + 35 \text{MJ} \\
h_{\text{ein,1z}} \Rightarrow \text{TAB1: } 29.57 \frac{\text{kJ}}{\text{kg}} \\
\left[ -728.8 \text{MJ} \right] = 1 \text{m} \cdot 29.57 \frac{\text{kJ}}{\text{kg}} = 1 \text{m} \cdot 29.57 \frac{\text{MJ}}{\text{kg}} \\
1 \text{MJ}_{\text{1z}} = 296.99 \text{kg}
``````latex