

\subsection*{2b}

\[
\text{ges: } \omega_6, T_6
\]

\[
\text{isentrope Schubd√ºse, } U_s, p_s, T_s \text{ bekannt}
\]

\[
Q = \dot{m} \left( h_s - h_6 + \frac{\omega_s^2 - \omega_6^2}{2} \right) \quad \text{(crossed out)}
\]

\[
\dot{m} = \dot{m}_{\text{ges}}
\]

\[
\text{Exergiebilanz:}
\]

\[
Q = \dot{m}_{\text{ges}} \left( h_s - h_6 + \frac{\Delta k}{e} \right), \quad \Delta k = \frac{\omega_s^2 - \omega_6^2}{2}
\]

\[
h_s \Rightarrow \text{TAB A2: } h_s (930K) + \frac{h(990K) - h(952K)}{10K} \cdot 1.9K
\]

``````latex


\begin{align*}
&h_5 = 953.26 \frac{\text{kJ}}{\text{kg}} \\
&\text{Isentrop } 5 \rightarrow 6 \text{ and:} \\
&T_6 = T_5 \left( \frac{p_6}{p_5} \right)^{\frac{n-1}{n}} \\
&T_6 = 328.075K \\
&h_6 = h(328K) + \frac{h(333K) - h(328K)}{5K} \cdot (3.075K) \\
&h_6 = 333.93 \frac{\text{kJ}}{\text{kg}} \\
&0 = \dot{m}_{\text{ges}} (h_5 - h_6) + \frac{\omega_5^2 - \omega_6^2}{2} \\
&\dot{m}_{\text{ges}}^2 (h_6 - h_5) = \dot{m}_{\text{ges}} \frac{\omega_5^2 - \omega_6^2}{2} - \omega_6^2 = 2(h_6 - h_5) - \omega_5^2 \\
&\omega_6^2 = 2(h_5 - h_6) + \omega_5^2, \quad \omega_6 = 998.26 \frac{\text{m}}{\text{s}} \\
&\text{ex}_{\text{str}6} - \text{ex}_{\text{str}0} = \dot{m}_{\text{ges}} (h_6 - h_0 - T_0 (s_6 - s_0) + \Delta \text{ke}) \\
&h_6 = 333.93 \frac{\text{kJ}}{\text{kg}}, \quad h_0 = h(265.15K) \\
&s_6 = s(T_6), \quad s_0 = s(T_0), \quad \Delta \text{ke} = \frac{\omega_6^2 - \omega_0^2}{2} \\
&s(T_6) \approx 1.79 \frac{\text{kJ}}{\text{kgK}}, \quad s_0 \approx 1.86 \frac{\text{kJ}}{\text{kgK}} \\
&h_0 \approx 263 \frac{\text{kJ}}{\text{kg}} \\
&\Delta \text{ex}_{\text{str}} = \frac{\text{ex}_{\text{str}}}{\dot{m}_{\text{ges}}} = \frac{109.19 \frac{\text{kJ}}{\text{kg}}}{119.09 \frac{\text{kJ}}{\text{kg}}}
\end{align*}

``````latex