d)

\begin{equation*}
\dot{Q}_{out} = \sum \dot{E}_{x,str,i} + \sum \dot{E}_{x,Q,i} - \sum \dot{W}_n - \dot{E}_{x,ver,l}
\end{equation*}

\begin{equation*}
0 = \sum \dot{E}_{x,str,i} + \dot{E}_{x,Q,i} - \dot{E}_{x,ver,l}
\end{equation*}

\begin{equation*}
\dot{e}_{x,ver,l} = h_0 - h_0 - T_0(s_0 - s_0) + ke + \left(1 - \frac{T_0}{T_B}\right)q_B
\end{equation*}

\begin{equation*}
\dot{e}_{x,ver,l} = \Delta e_{x,str} + \left(1 - \frac{T_0}{T_B}\right)q_B
\end{equation*}

\begin{equation*}
\dot{e}_{x,ver,l} = 100 \frac{kJ}{kg} + \left(1 - \frac{273,15 - 30}{1285}\right)1195 = \underline{1069,58 \, kJ}
\end{equation*}

``````latex