

\subsection*{a)}

\[
\frac{d}{dt} = \dot{m} \left[ h_i + \frac{c^2}{2} + \xi \frac{Q_i}{\dot{m}} \right] - \sum \frac{W_i}{\dot{m}}
\]

\[
\dot{Q}_{\text{aus}} = \dot{m} \left[ h_{\text{ein}} - h_{\text{aus}} \right] + \dot{Q}_{\text{aus}} + \dot{Q}_R
\]

\[
\dot{Q}_{\text{aus}} = \dot{m} (h_{\text{ein}} - h_{\text{aus}}) + \dot{Q}_R
\]

\[
h_{\text{ein}} = h_f(70^\circ C) + x \left( h_g(70^\circ C) - h_f(70^\circ C) \right) \quad \text{aus TAB A-2}
\]

\[
= 301,65 \frac{\text{kJ}}{\text{kg}}
\]

\[
h_{\text{aus}} = h_f(100^\circ C) + x \left( h_g(100^\circ C) - h_f(100^\circ C) \right) \quad \text{aus TAB A-2}
\]

\[
= 430,33 \frac{\text{kJ}}{\text{kg}}
\]

\[
\dot{Q}_{\text{aus}} = 62,296 \text{kW}
\]