\subsection*{a) perfekte Gas}

\begin{align*}
p_1 &= p_{\text{amb}} + 32 \frac{kg}{s} \cdot \frac{\dot{V}}{A} + \frac{\dot{m}}{A} \cdot \frac{\dot{m}}{2} \cdot \frac{1}{\rho} + \frac{\dot{m}}{A} \cdot \frac{\dot{m}}{A} \\
&= 1,40059 \, \text{bar}
\end{align*}

\textit{ideale Gasgleichung:}
\begin{align*}
m_{\text{g2}} &= \frac{p_2 \cdot V_1}{R \cdot T_1} \\
R &= \frac{\bar{R}}{M_{\text{g}}} = 166,28 \, \frac{\text{kJ}}{\text{kg} \cdot \text{K}}
\end{align*}

\begin{align*}
m_{\text{g2}} &= \frac{1,40059 \cdot 3,75 \cdot 10^{-2}}{166,28 \cdot (500 + 273,15)} \\
&= 3,434 \, \text{g}
\end{align*}



\section*{a)}

Die Widerlager werden vorerst komplett \( u = u_{2} - u_{n} \) angenommen.

\[
m_E \cdot (u_2 - u_n) = Q_{12}
\]

\[
u_2 - u_n = \frac{Q_{12}}{m_E} \Rightarrow u_2 = \frac{Q_{12}}{m_E} + u_n
\]

\[
\frac{148}{1} \text{ links}
\]

mit \( u_n \left(0 + l\right) = x_{E,2} \cdot u_{FE} + (1 - x_{E,2}) \cdot u_{FE} \)

\[
= -200 \frac{1}{l}
\]

da \( T \) sich nicht verändert, da \( \text{provo.} \) daher

\[
\text{d.h.} \text{ gilt für } u_2 = x_{E,2} \cdot u_{FE} + (1 - x_{E,2}) \cdot u_{FE}
\]

\[
u_2 = \frac{2500 \cdot kg}{6 \cdot m} + u_n = \text{anpassen} - 128,3 \frac{1}{l}
\]

\[
x_{E,2} = \frac{(u_2 - u_{FE})}{u_{FE} - u_{FE}} = 0,555
\]

``````latex