

\section*{c)}

\begin{align*}
\Delta s_{tot} &= s_2 - s_0 - \frac{Q}{T_0}(s_3 - s_0) + \rho(v_2 - v_0) \\
\frac{u_2}{c_p} - \frac{u_0}{c_p} &= c_v \ln \left( \frac{T}{T_0} \right) = \\
&= c_v \left( T_0 \left( \frac{T_2}{T_0} \right) - T_0 \ln \left( \frac{T_2}{T_0} \right) \right)
\end{align*}

\textbf{T0-Break:}

\begin{align*}
\Delta s_{tot} &= u_2 - u_0 - T_0(s_2 - s_0) + k \cdot m \\
&= c_p \left( T_2 - T_0 \right) - T_0 \cdot c_p \left( \frac{T_2}{T_0} \right) + \frac{v_0^2 - v_0^2}{2} \\
&= -m \left( \frac{Q}{T_0} \right) \ln \left( \frac{T_2}{T_0} \right)
\end{align*}