

\section*{c)}

\[
Q_{12} = m_g \cdot C_p \cdot \Delta T = 3.42 \text{g} \cdot 0.80 \frac{\text{J}}{\text{g K}} \cdot (500^\circ \text{C} - 0.003^\circ \text{C}) = 1367.46 \text{J}
\]

``````latex


\section*{Student Solution}

\begin{equation}
d l \quad T_{EW,2} = T_{g,2} = 0,005^\circ C
\end{equation}

\begin{equation}
\frac{m_{EW}}{m_{EW}} = 0,6 \quad \Rightarrow \quad m_{Ci} = 0,6 - 0,6 \cdot 0,1_{kg} = 0,06 \, kg
\end{equation}

\begin{equation}
u_{n} = u_{k} + x \left( u_{tot} - u_{k} \right)_{k_{tot}} \quad \Rightarrow \quad \text{(crossed out text)}
\end{equation}

\begin{equation}
\text{Tab(0,0)}
\end{equation}

\begin{equation}
u_{n} = -333,485 \, \frac{kJ}{kg} + 0,6 \left[ -0,045 \, \frac{kJ}{kg} + 333,485 \, \frac{kJ}{kg} \right] = -733,47 \, J
\end{equation}

\begin{equation}
\text{EB gleichsetzen System:} \quad \Delta E = Q_{n2} \quad \Rightarrow \quad \Delta U = Q_{n2} = (u_{2} - u_{n}) = Q_{n2}
\end{equation}

\begin{equation}
u_{2} = Q_{n2} + u_{n} = 1,500 \cdot 10^{3} - 733,47 \, J = 733,588 \, J
\end{equation}

\begin{equation}
x_{2} = \frac{u_{2} - u_{k,1} (0,005^\circ)}{u_{tot}(0,005^\circ) - u_{k,1} (0,005^\circ)} = 0,5
\end{equation}

``````latex