

\subsection*{b)}

\begin{equation*}
\frac{dE}{dt} = 0 = \dot{m} (h_0 - h_6) + \left( \frac{w_0^2 - w_6^2}{2} \right) + \frac{q_{13}}{\dot{m}_K} + \dot{W}
\end{equation*}

\begin{equation*}
0 = \dot{m} c_p (T_0 - T_6) + \left( \frac{w_0^2 - w_6^2}{2} \right) = - \frac{q_{13}}{\dot{m}_K}
\end{equation*}

\begin{equation*}
5.273 \cdot \dot{m}_K = \dot{m} = \dot{m} - \dot{m}_K
\end{equation*}

\begin{equation*}
\dot{m}_K = \frac{\dot{m}}{6.273}
\end{equation*}



\subsection*{b)}

\[
\frac{dE}{dt} = 0 = \dot{m} \left( h_0 - h_6 + \frac{w_0^2 - w_6^2}{2} \right) + q_{B} - \dot{W}
\]

\[
0 = h_0 - h_6 + \frac{w_0^2 - w_6^2}{2} + q_{B}
\]

\[
w_6 = \sqrt{2 \left( h_0 - h_6 + q_{B} \right) + w_0^2}
\]

\[
= \sqrt{2 \left[ c_p (T_0 - T_6) + q_{B} \right] + w_0^2}
\]

\[
q_{B} = 1195 \frac{kJ}{kg}
\]

\[
T_0 = 243.15 \, K
\]

\[
T_6 = \ldots
\]

\[
w_0 = 200 \frac{m}{s}
\]