

\subsection*{d)}

\begin{equation*}
T_{\text{KF}} = 70^\circ C \quad \Delta m_{12} \quad T_{\text{pin, 12}} = 200^\circ C
\end{equation*}

\begin{equation*}
z1 \rightarrow z2 \quad \Delta m_{12} > 0
\end{equation*}

\begin{equation*}
m_{2} u_{2} - m_{1} u_{1} - \Delta m_{12} h_{e} = Q
\end{equation*}

\begin{equation*}
(m_{1} + m_{2}) u_{2} - m_{1} u_{1} - \Delta m_{12} h_{e} = Q
\end{equation*}

\begin{equation*```latex


\section*{A1}

d) 
\begin{equation}
m_1 u_2 + m_e (u_2 - h_e) - m_1 u_1 = Q
\end{equation}

\begin{equation}
m_e = \frac{Q + m_1 (h_1 - u_2)}{u_2 - h_e}
\end{equation}

\begin{equation}
Q = -35 \, \text{MJ}
\end{equation}

\begin{equation}
m_1 = 5.755 \, \text{kg}
\end{equation}

\begin{equation}
T_1 = 100^\circ \text{C}
\end{equation}

\begin{equation}
T_2 = 70^\circ \text{C}
\end{equation}

\begin{equation}
T_e = 200^\circ \text{C}
\end{equation}

\begin{equation}
u_1 (100^\circ \text{C}, 5. \text{F})
\end{equation}

\begin{equation}
u_2 (70^\circ \text{C}, 5. \text{F})
\end{equation}

\begin{equation}
u_e (200^\circ \text{C}, 5. \text{F})
\end{equation}

\begin{equation}
h_e (200^\circ \text{C}, 5. \text{F})
\end{equation}

\begin{equation}
4.13 \cdot 10^2
\end{equation}

\begin{equation}
4.29, 38 \frac{\text{kJ}}{\text{kg}} + 4.18, 94 + 0.005 (205.045)
\end{equation}