e)

\begin{align*}
\Delta S &= \cancel{S_2} M_2 S_2 - M_1 S_1 \\
S_1 &= x \cdot S_g + (1-x) S_f = \frac{1.33714 \, \text{kJ}}{\text{kg}} \\
x &= 0.905 \\
S_g &= 7.3549 \, \frac{\text{kJ}}{\text{kgK}} \text{ aus A-2} \\
S_f &= 1.3069 \, \frac{\text{kJ}}{\text{kgK}} \\
S_2 &= x \cdot S_f (-7.0^\circ \text{C}) \\
x_2 &= 0 \\
S_f (7.0^\circ \text{C}) &= 0.9549 \, \frac{\text{kJ}}{\text{kgK}} \text{ aus A-2} \\
m_1 &= 5755 \, \text{kg} + 3600 \, \text{kg} = \underline{9355 \, \text{kg}}
\end{align*}

\[
\Delta S = \underline{1235.83 \, \text{kJ}}
\]

``````latex