\section*{1. d)}

\begin{enumerate}
    \item 
    \begin{align*}
        T_{R1} &= 100^\circ C \\
        x_D &= 0.005 \\
        m_1 &= 5755 \text{ kg}
    \end{align*}
    
    \item 
    \begin{align*}
        T_{R2} &= 70^\circ C \\
        x_2 &= 0 \\
        m_2 &= m_1 + \Delta m_{12}
    \end{align*}
\end{enumerate}

\noindent
\text{=D halboffenes System}

\begin{align*}
    \Delta E &= m_2 u_2 - m_1 u_1 = \Delta m_{12} (h_{ein}) + Q \\
    (m_1 + \Delta m_{12}) u_2 - m_1 u_1 &= \Delta m_{12} (h_e) + Q_{R12} \\
    m_1 u_2 - Q_{R12} - m_1 u_1 &= \Delta m_{12} (h_e) - \Delta m_{12} u_2 \\
    m_1 u_2 - Q_{R12} - m_1 u_1 &= \Delta m_{12} (h_e - u_2)
\end{align*}

\noindent
\text{h_{ein}:}
\begin{align*}
    T_{ein} &= 20^\circ C \\
    x &= 0 \\
    p_{ein} &= 0.02339 \\
    h_{ein} = h_f &= 83.96 \frac{\text{kJ}}{\text{kg}} \quad \text{(aus A-2)}
\end{align*}

\noindent
\text{U_2:}
\begin{align*}
    x_1 &= 0.005 \\
    U_2 = U_f (70^\circ C) &= 292.95 \quad \text{(aus A-2)}
\end{align*}

\noindent
\text{U_A:}
\begin{align*}
    U_A &= x_1 u_g (100^\circ C) + (1 - x_1) u_f (100^\circ C) \\
    &= x_1 \left( 2506.5 \frac{\text{kJ}}{\text{kg}} \right) + (1 - x_1) \left( 419.89 \frac{\text{kJ}}{\text{kg}} \right) \\
    &= 429.37 \frac{\text{kJ}}{\text{kg}}
\end{align*}

\noindent
\text{aus A-2}
\begin{align*}
    \Delta m_{12} &= \frac{m_1 u_2 + Q_{R12} - m_1 u_1}{h_e - u_2} \\
    &= 3589.37 \text{ kg}
\end{align*}

``````latex