a)

\text{Stat. Flie√üprozess mit 1 Massenstrom}

\[
0 = \dot{m} (h_e - h_a) + \dot{Q} - \dot{Q}_{\text{Aus}}
\]

\[
0 = \dot{m} (h_{\text{ein}} - h_{\text{aus}}) + \dot{Q}_R - \dot{Q}_{\text{Aus}}
\]

\[
\dot{Q}_{\text{Aus}} = \dot{m} (h_{\text{ein}} - h_{\text{aus}}) + \dot{Q}_R
\]

\[
\dot{Q}_{\text{Aus}} = 0.3 (h_{\text{ein}} - h_{\text{aus}}) + 100 \frac{\text{kJ}}{\text{s}} = 67.182 \text{kW}
\]

\underline{hein:}

\[
T = 70^\circ C
\]

\[
x = 0
\]

\[
p = 0.3119 \text{ bar aus A-2}
\]

\[
h_{\text{ein}} = h_f = 252.98 \frac{\text{kJ}}{\text{kg}} \text{ aus A-2}
\]

\underline{hinaus:}

\[
T_{\text{aus}} = 100^\circ C
\]

\[
x = 0
\]

\[
p = 1.013 \text{ bar aus A-2}
\]

\[
h_{\text{aus}} = h_f = 419.04 \frac{\text{kJ}}{\text{kg}} \text{ aus A-2}
\]