

\subsection*{c)}
\begin{align*}
0 &= \dot{m} (S_e - S_a) + \frac{\dot{Q}_\text{um}}{T_\text{irr}} + \dot{S}_\text{erz} \\
S_\text{erz} &= \dot{m} (S_a - S_e) - \frac{\dot{Q}_\text{um}}{T_\text{irr}} = \dot{m} (S_a - S_e) + \frac{\dot{Q}_\text{um}}{T_\text{irr}} \\
\text{Werte:} \\
S_e &= S_f (70^\circ \text{C}) = 0,3564 \frac{\text{kJ}}{\text{kg K}} \\
S_a &= S_f (100^\circ \text{C}) = 1,3069 \frac{\text{kJ}}{\text{kg K}} \\
\Rightarrow S_\text{erz} &= 0,3178 \frac{\text{kJ}}{\text{K}}
\end{align*}

``````latex