

\subsection*{b)}
\begin{align*}
Q_{\text{aus rein}} &\rightarrow \text{reversibel} \rightarrow S_{\text{tot}} = 0 \\
Q &= \dot{m} (s_1 - s_2) + \frac{Q_{\text{aus}}}{T} \rightarrow \overline{T} = \dot{m} (s_2 - s_1) + \dot{Q}_{\text{aus}} \\
Q &= \dot{m} (u_{EF1} - u_{EF2}) + Q_{\text{aus}} \\
\frac{Q_{\text{aus}}}{u_{EF1} - u_{EF2}} &= \dot{m} \cdot \overline{T} \\
\frac{Q_{\text{aus}}}{e^{\frac{(T_1 - T_2)}{T_1}}} &= \dot{m} \cdot e^{\frac{(T_1 - T_2)}{T_1}} \\
\overline{T} &= \frac{1}{\frac{Q_{\text{aus}}}{e^{\frac{(T_2}{T_1}}}}} = \frac{Q_{\text{aus}}}{e^{\frac{(T_1 - T_2)}{T_1}}} = \frac{(T_1 - T_2)}{\ln \left( \frac{T_2}{T_1} \right)} \rightarrow 293.12 \text{K}
\end{align*}