

\subsection*{b)}

\[
0 = \dot{m} \left[ h_e - h_a + \frac{w_e^2 - w_a^2}{2} + g \frac{z_e - z_a}{2} \right] + \dot{Q} - \sum \dot{W}
\]

For $5-6$, isentropic:

\[
0 = \dot{m} \left[ h_5 - h_6 + \frac{w_5^2 - w_6^2}{2} \right] + 0 - 0
\]

\[
= \dot{m}_{\text{ges}} \left[ h_5 - h_6 + \frac{220^2 - w_6^2}{2} \right]
\]

\[
\text{suche } h_5 - h_6
\]

\[
\text{Luft ist } ZG \text{ mit } C_p \approx 1.006 \frac{\text{kJ}}{\text{kg K}}, \quad 5-6 \text{ isentrope, } n = k = 1.4,
\]

\[
h(T_5) - h(T_6) = C_p (T_5 - T_6)
\]

\[
= 1.006 \frac{\text{kJ}}{\text{kg K}} (431.9 \text{K} - T_6)
\]

\[
\text{suche für } w_6
\]

\[
\text{Für gesamte System } 0-6,
\]

\[
0 = \dot{m} \left[ h_e - h_a```latex


\section*{Solution}

\subsection*{1.}

\[
h_6 - h_5 = \frac{220^2 - w_6^2}{2}
\]

\[
h_6 - h_5 = h_6 - h_5 = \frac{220^2 - w_6^2}{2}
\]

\[
h_5 + h_6 = \frac{220^2 - w_6^2}{2}
\]

\[
5 - 6 \text{ isentropic}
\]

\[
\frac{T_5}{T_6} = \left( \frac{P_5}{P_6} \right)^{\frac{n-1}{n}}
\]

\[
\frac{T_5}{T_6} = \left( \frac{0.5}{P_6} \right)^{\frac{k-1}{k}}
\]

\[
T_6 = 431.8K
\]

\[
\frac{T_6}{T_5} = \left( \frac{P_6}{P_5} \right)^{\frac{k-1}{k}} = \left( \frac{0.111}{0.5} \right)^{\frac{0.4}{1.4}} = 0.759608
\]

\[
T_6 = 0.759608 \cdot 431.8K
\]

\[
T_6 = 328.0747K
\]

\[
V_{on(1)}: 0 = 1.006(431.8K - 328.0747K) + \frac{220^2 - w_6^2}{2}
\]

\[
= 104.4882 + 24200 - \frac{w_6^2}{2}
\]

\[
\frac{w_6^2}{2} = 24304
\]

\[
w_6^2 = 48608 \quad w_6 = 220.472 \frac{m}{s}
\]

\subsection*{2.}

\subsection*{2C.}

\[
\Delta e_{exter} = e_{x6} - e_{x40}
\]

\[
= h - h_0 - T_0(S - S_0) + ke + pe
\]

\[
= h_6 - h_0 - T_0(S_6 - S_0) + ke \frac{w_6^2 - w_0^2}{2}
\]

\[
P_0 - P_0 \text{ isobar, adiabat: } 6 - 1 \text{ isentropic.}
\]

\[
S: S_6 - S_0 = Cp \ln \left( \frac{T_6}{T_0} \right) - R \ln \left( \frac{P_6}{P_0} \right)
\]

\[
= 1.006 \ln \left( \frac{340}{243.15} \right) - R \ln \left( 1 \right)^0 = 0.337278 \frac{kJ}{kg \cdot K}
\]

\[
h_6 - h_0 = Cp(T_6 - T_0) = 1.006 \times (340 - 243.15) = 97.4311 \frac{kJ}{kg}
\]

\[
\Delta e_{exter} = 97.4311 \frac{kJ}{kg} - (243.15K) (0.337278) \frac{kJ}{kg \cdot K}
\]

\[
= 100.05 \frac{kJ}{kg} + \frac{510^2 - 200^2}{2 \cdot 1000}
\]

\[
= 100.05 + 15.42 = 125.47 \frac{kJ}{kg}
\]

``````latex