

\subsection*{b)}
\begin{align*}
0 &= \dot{m} \left[ h_e - h_a \right] + \dot{m} e + g z_e - z_a \right] + \dot{Q} - \sum \dot{W}_{ein} \\
  &= \dot{m}_{\text{K}} \left[ h_1 - h_2 \right] + \left( -\dot{Q}_{ab} \right) + Q_k + 28 W \\
0 &= \dot{m} \left[ h_1 - h_2 \right] + Q_k \\
Q_k &= \dot{m}_{\text{K}} \left[ h_2 - h_1 \right]
\end{align*}

\subsection*{2-3:}
\begin{align*}
0 &= \dot{m}_{\text{K}} \left[ h_2 - h_3 \right] + Q_k + 28 W \\
  &= \dot{m} \left[ \int_{T_1}^{T_2} c_{if}(T) dT + v \left( p_2 - p_1 \right) + \dot{Q}_k + 28 W \right]
\end{align*}
\begin{align*}
h_2 &= \text{ges√§ttigt dampf} \\
h_2 &= 
\end{align*}