

\subsection*{d)}
\begin{align*}
0 &= \dot{m} \left[ h_e - h_a \left( \frac{v_e^2 - v_a^2}{2} \right) + g (z_e - z_a) \right] + \sum \dot{Q} - \sum \dot{W} \\
\text{Zustand 1:} & \quad T_1 = 100^\circ \text{C} \\
\text{Zustand 2:} & \quad T_2 = 70^\circ \text{C} \\
\text{Tein} &= 20^\circ \text{C} \\
\text{hei√ües System:} & \quad \Delta E = m_2 u_2 - m_1 u_1 = \sum m_i \left[ h_i + \frac{v_i^2}{2}```latex


1(c). \(\Delta S = m_2 S_2 - m_1 S_1 = \sum dm_i S_i + \sum \frac{Q_i}{T_i} + S_{env}\)

\[
m_{02}(m_1 + m_{412}) S_2 - m_1 S_1 = dm_{12} S_{12} + \frac{Q_{412}}{T} + S_{env}
\]

``````latex