

\subsection*{a)}

\begin{align*}
0 &= \dot{m}_{\text{ein}} h_{\text{ein}} - \dot{m}_{\text{aus}} h_{\text{aus}} - \dot{Q}_{\text{aus}} + \dot{Q}_R \\
\dot{Q}_{\text{aus}} &= \dot{m}_{\text{ein}} h_{\text{ein}} - \dot{m}_{\text{aus}} h_{\text{aus}} + \dot{Q}_R \\
\dot{Q}_{\text{aus}} &= \dot{m}_{\text{ein}} (h_{\text{ein}} - h_{\text{aus}}) + \dot{Q}_R \\
h_{\text{ein}} &= h_f(750) = 292,38 \, \frac{\text{kJ}}{\text{kg}} \\
h_{\text{aus}} &= 413,04 \quad \text{(TABELLE 2)} \\
\dot{Q}_{\text{aus}} &= 0,3 \left( 292,38 - 413,04 \right) + 100 = 62,182 \, \text{kW}
\end{align*}