

\subsection*{c)}

\[
e_{k, \text{ist,0}} = e_{k, \text{ist,0}} + \frac{u_{c, \text{ist}}^2}{2} = \frac{u_{c, \text{ist}}^2}{2}
\]

\[
h_c - h_0 = c_p (T_6 - T_0) = 1.006 \, \frac{\text{kJ}}{\text{kg K}} (382.07 \, \text{K} - 243.15 \, \text{K}) = 85.43 \, \frac{\text{kJ}}{\text{kg}}
\]

\[
s_6 - s_0 = c_p \ln \left( \frac{T_6}{T_0} \right) - R \ln \left( \frac{p_6}{p_0} \right) = 1.006 \, \frac{\text{kJ}}{\text{kg K}} \ln \left( \frac{382.07}{243.15} \right) - 0.30 \, \frac{\text{kJ}}{\text{kg K}}
\]

\[
\Delta e_{k, \text{ist}} = \frac{u_{c, \text{ist}}^2}{2}
\]

\[
\Delta e_{k, \text{ist}} = 85.43 \, \frac{\text{kJ}}{\text{kg}} - 243.15 \cdot 15 \, \text{K} (0.3 \, \frac{\text{kJ}}{\text{kg K}}) + \frac{(498.80 \, \frac{\text{m}}{\text{s}})^2 - (200 \, \frac{\text{m}}{\text{s}})^2}{2}
\]

\[
= 116.63 \, \frac{\text{kJ}}{\text{kg}}
\]