

\subsection*{d)}
7.45:

\[
0 = m_2 u_2 - m_1 u_1 - \dot{m} \left[ h_{\text{ein}} \right] - Q_{\text{R12}}
\]

\[
h_{\text{ein}} = h_f (200^\circ) = 83.96 \, \frac{\text{kJ}}{\text{kg}}
\]

\[
Q_{\text{R12}} = 35 \times 10^6 \, \text{J}
\]

\[
m_2 = \dot{m} + m_{\text{ges},1}
\]

\[
m_1 = m_{\text{ges},1}
\]

\[
0 = \dot{m} u_2 + m_{\text{ges},1} u_2 - \dot{m} u_{\text{ein}} - Q_{\text{R12}}
\]

\[
\dot{m} (u_2 - h_{\text{ein}}) = m_{\text{ges}} (u_1 - u_2) - Q_{\text{R12}}
\]

\[
\dot{m} = \frac{m_{\text{ges}} (u_1 - u_2) - Q_{\text{R12}}}{u_2 - h_{\text{ein}}} = 330 \, \frac{\text{kg}}{\text{s}}
\]

\[
u_2 = u_f (70^\circ) = 292.35 \, \frac{\text{kJ}}{\text{kg}}
\]

\[
u_1 = u_f (100^\circ) = 418.9 \, \frac{\text{kJ}}{\text{kg}}
\]