

\subsection*{a)}

\textit{Annahme KF:}

\[
0 = \dot{m}_{KF} \left[ h_{ein} - h_{aus} \right] + Q_{aus}
\]

\[
Q_{aus} = \dot{m}_{KF} \left[ h_{aus} - h_{ein} \right]
\]

\[
Q_{zu} = \dot{m}_{KF} \cdot c \left( T_{aus} - T_{ein} \right)
\]

\[
0 = \dot{m}_{ein} \left[ h_{ein} - h_{aus} \right] + Q_{e} - Q_{aus}
\]

\[
Q_{zu} = m_{ein} \left[ h_{e} - h_{aus} \right] + Q_{R}
\]

\[
h_{aus} = h_{f} \left( 100^\circ C \right) = 419.04
\]

\[
h_{e} = h_{f} \left( 70^\circ C \right) + x \cdot \left( h_{g} \left( 70^\circ \right) - h_{f} \left( 70^\circ \right) \right) =
\]