\section*{Problem c}

\[
e_{x, \text{ser}, s} = h_6 - h_0 - T_0 (s_6 - s_0) + \frac{1}{2} v_6^2
\]

\[
h_6 - h_0 = c_p (T_6 - T_0) = 97.9 \frac{\text{kJ}}{\text{kg}}
\]

\[
s_6 - s_0 = c_p \ln \left( \frac{T_6}{T_0} \right) = 0.3373 \frac{\text{kJ}}{\text{kg K}}
\]

\[
c_p (340 \text{K} - 293.15 \text{K}) = 97.9 \frac{\text{kJ}}{\text{kg}}
\]

\[
e_{x, \text{ser}, s} = 97.9 \frac{\text{kJ}}{\text{kg}} - 293.15 \text{K} \cdot 0.3373 \frac{\text{kJ}}{\text{kg K}} + \frac{1}{2} \cdot 5 \frac{\text{m}^2}{\text{s}^2}
\]

\[
= 130 \frac{\text{kJ}}{\text{kg}}
\]

\[
e_{x, \text{ser}, 0} = \cancel{0} + \frac{1}{2} \cdot 200 \frac{\text{m}^2}{\text{s}^2} = 20 \frac{\text{kJ}}{\text{kg}}
\]

\[
\Delta e_{x, \text{ser}} = 130 \frac{\text{kJ}}{\text{kg}} - 20 \frac{\text{kJ}}{\text{kg}} = 110 \frac{\text{kJ}}{\text{kg}}
\]