c) \quad \Delta e_{x,str} = e_{x,str,6} - e_{x,str,0}

\[
= h_6 - h_0 - T_0 (s_6 - s_0) + ke_6 - \left( h_0 - h_0 - T_0 \left( s_6 - s_0 \right) + ke_0 \right)
\]

\[
h_c = h_0 = \int_{T_0}^{T_c} c_{p,luft} (T) \, dT = c_{p,luft} (T_c - T_0)
\]

\[
= 1.006 \, \frac{kJ}{kgK} \left( 325.0 \, K - 243.15 \, K \right) = 85.43 \, \frac{kJ}{kg}
\]

Aus TAB A-22:

\[
s^0 (T_c) = \left( 1.79813 + 1.798249 \right) \frac{kJ}{kgK} \left( \frac{325.0 \, K + 325 \, K}{330 - 325} \right) = 1.798249 \, \frac{kJ}{kgK}
\]

\[
s^0 (T_c) = 1.79819 \, \frac{kJ}{kgK}
\]

\[
s^0 (T_0) = \left( 1.49819 + 1.49824 \right) \frac{kJ}{kgK} \left( \frac{243.15 \, K - 240 \, K}{250 - 240} \right) = 1.49824 \, \frac{kJ}{kgK}
\]

\[
s^0 (T_0) = 1.49811 \, \frac{kJ}{kgK}
\]

\[
\rightarrow \Delta e_{x,str} = h_c - h_0 - T_0 (s_6 - s_0) + ke_6 + ke_0
\]

\[
ke_6 = \frac{v_6^2}{2} \quad ke_0 = \frac{1}{2} v_{luft}^2 = 20000 \, \frac{m^2}{s^2}
\]

\[
= 128654.23 \, \frac{m^2}{s^2}
\]

\[
\rightarrow \Delta e_{x,str} = 85.43 \, \frac{kJ}{kg} - 243.15 \, K \left( 1.79819 \, \frac{kJ}{kgK} - 1.49811 \, \frac{kJ}{kgK} \right)
\]

\[
+ \left( 128654.23 - 20000 \right) \frac{m^2}{s^2}
\]

\[
\Delta e_{x,str} = 1280.94 \, \frac{kJ}{kg}
\]