

\section*{d)}
\text{ges.} \quad e_{3, \text{verl}}

\text{Exergiebilanz:} \quad \text{(1)} \rightarrow \text{(2)} \quad \text{da adiabatisch}

\[
\frac{dE_X}{dt} = \sum \dot{m} e_{\text{str}} + \sum \dot{E}_X - \sum \dot{W} - \rho_0 \frac{dV}{dt} - E_{3, \text{verl}} \quad \Bigg| \dot{m}
\]

\[
\Leftrightarrow C = e_{\text{str}} - W - e_{3, \text{verl}}
\]

\[
e_{3, \text{verl}} = e_{\text{str}} - W
\]

\text{Energiegleichung:} \quad \text{(1)} \rightarrow \text{(2)}

\[
0 = \dot{m} (ri + kei + pei) + \sum \dot{Q} - \sum \dot{W}
\]

``````latex