

\section*{c)}
\text{Annahme:} \quad \dot{m}_0 = 350 \, \frac{\text{kg}}{\text{h}}

\text{ges.} \quad \Delta e_{\text{str}} \quad \text{zwischen} \quad 0 - 6 \quad \Rightarrow \text{Exergiebilanz einer Str√∂mung}

\[
\Delta e_{\text{str}} = h_6 - h_0 - T_0 (s_6 - s_0) + \frac{v_6^2}{2} - \frac{v_0^2}{2}
\]

\[
= c_p^0 (T_6 - T_0) - T_0 \left( c_p^0 \ln \left( \frac{T_6}{T_0} \right) - R \ln \left( \frac{p_6}{p_0} \right) \right) + \frac{v_6^2}{2} - \frac{v_0^2}{2}
\]

\[
= c_p^0 (T_6 - T_0) - T_0 c_p^0 \ln \left( \frac{T_6}{T_0} \right) + T_0 R \ln \left( \frac{p_6}{p_0} \right) + \frac{v_6^2}{2} - \frac{v_0^2}{2}
\]

\text{mit} \quad c_p^0 = 1.006 \, \frac{\text{kJ}}{\text{kgK}}, \quad T_0 = 30^\circ \text{C}, \quad T_6 = 293.7 \, \text{K}

\[
\Rightarrow \Delta e_{\text{str}} = 540.57 \, \frac{\text{kJ}}{\text{kg}} - 46.37 \, \frac{\text{kJ}}{\text{kg}} + 110.05 \, \frac{\text{kJ}}{\text{kg}}
\]

\[
\Rightarrow \Delta e_{\text{str}} = 603.7 \, \frac{\text{kJ}}{\text{kg}}
\]