

\subsection*{c)}

\[
\Delta e_{x, \text{str}} = e_{x, \text{str}, a} - e_{x, \text{str}, e} =
\]

\[
= h_a - h_e - T_0 (s_a - s_e) + \Delta ke
\]

\[
\Rightarrow \Delta ke = \frac{w_5^2}{2} - \frac{w_6^2}{2} = 108.651 \, J = 108.651 \, \frac{kJ}{kg}
\]

\[
\Rightarrow h_a - h_e = c_p^* (T_6 - T_0) = 85.430 \, \frac{kJ}{kg}
\]

\[
\Rightarrow s_a - s_e = c_p^* \ln \left( \frac{T_6}{T_0} \right) - R \ln \left( \frac{p_6}{p_0} \right) = 0.301 \, \frac{kJ}{kg \cdot K}
\]

\[
\Rightarrow q = c_p^* T_0 - c_p^* T_0 \ln \left( \frac{T_6}{T_0} \right) = 0.2874 \, \frac{kJ}{kg}
\]

\[
\Rightarrow \Delta e_{x, \text{str}} = 120.89 \, \frac{kJ}{kg}
\]

``````latex


\begin{itemize}