

\section*{c)}

\[
Q = \dot{m} (s_2 - s_1) + \frac{\dot{Q}}{T_0} + s_1
\]

\[
\text{Serie: } - \dot{m} (s_1 - s_c)
\]

\[
T_s = 0,7056 - \frac{Q_{u,s}}{T_0} = 0,7056 + \frac{61,182}{273}
\]

\[
= 0,3764161 \frac{kJ}{kgK}
\]

\[
= 376,39 \frac{J}{kgK}
\]



\subsection*{c)}
\[
\frac{\overline{T}}{T} = \frac{\int_{s_1}^{s_2} T \, ds}{s_1 - s_2} = \frac{\int_{T_e}^{T_a} c \, dT}{\int_{T_e}^{T_a} \frac{c}{T} \, dT} = \frac{Q}{c \ln \left( \frac{T_a}{T_e} \right)} = \frac{\epsilon (T_a - T_e)}{c \ln \left( \frac{T_a}{T_e} \right)} = \frac{T_a - T_e}{\ln \left( \frac{T_a}{T_e} \right)} = 
\]

``````latex