

\subsection*{b)}
\[
T = \int_{s_a}^{s_e} T \, ds = \frac{q_{\text{rev}}}{s_i - s_e} = \frac{h_{\text{aus}} - h_{\text{ein}}}{s_{\text{aus}} - s_{\text{ein}}} = \frac{f (T_{\text{aus}} - T_{\text{ein}}) + v_i^2 (p_{\text{aus}} - p_{\text{ein}})}{s_i \ln \left( \frac{T_{\text{aus}}}{T_{\text{ein}}} \right)}
\]
\[
= \frac{T_{\text{aus}} - T_{\text{ein}}}{\ln \left( \frac{T_{\text{aus}}}{T_{\text{ein}}} \right)} = \frac{298.15 \, \text{K} - 288.15 \, \text{K}}{\ln \left( \frac{298.15 \, \text{K}}{288.15 \, \text{K}} \right)}
\]
\[
= 293.12 \, \text{K}
\]