

\section*{d)}

\begin{equation*}
\frac{dE}{dt} = \sum_i \dot{m}_i \left[ h_i + \frac{c_i^2}{2} + \frac{g z_i}{2} \right] - \dot{Q} - \dot{W}^o
\end{equation*}

\begin{equation*}
\Delta U = \Delta m_{12} h_{ein} + \dot{Q}
\end{equation*}

\begin{equation*}
m_2 u_2 - m_1 u_1 = \Delta m_{12} h_{ein} + \dot{Q} \quad \text{with} \quad m_2 = m_1 + \Delta m_{12}
\end{equation*}

\begin{equation*}
(m_1 + \Delta m_{12}) u_2 - m_1 u_1 = \Delta m_{12} h_{ein} + \dot{Q}
\end{equation*}

\begin{equation*}
- \dot{Q} + m_1 u_2 - m_1 u_1 = \Delta m_{12} h_{ein} - m_1 u_2 - \Delta m_{12} u_2
\end{equation*}

\begin{equation*}
- \dot{Q} + m_1 (u_2 - u_1) = \Delta m_{12} h_{ein} - \Delta m_{12} u_2
\end{equation*}

\begin{equation*}
- \dot{Q} + m_1 (u_2 - u_1) = \Delta m_{12} (h_{ein} - u_2)
\end{equation*}

\begin{equation*}
\Rightarrow \Delta m_{12} = \frac{m_1 (u_2 - u_1) - \dot{Q}}{h_{ein} - u_2}
\end{equation*}

\subsection*{siedende Fl√ºssigkeit: $\lambda = 0.5$}

\begin{equation*}
h_{ein} = 83.96 + 0.5 (2538.1 - 83.96) = 1311.03 \frac{kJ}{kg} \quad \text{(TAB-A-2)}
\end{equation*}

\begin{equation*}
u_1 = 418.94 + 0.005 (2506.5 - 418.94) = 429.3778 \frac{kJ}{kg} \quad \text{(TAB-A-2)}
\end{equation*}

\begin{equation*}
u_2 = 292.35 + 0.5 (2463.6 - 292.35) = 1381.275 \frac{kJ}{kg} \quad \text{(TAB-A-2)}
\end{equation*}

\begin{equation*}
\Delta m_{12} = \frac{5755 kg (1381.275 \frac{kJ}{kg} - 429.3778 \frac{kJ}{kg}) + 35 \frac{kJ}{s}}{1311.03 \frac{kJ}{kg} - 1381.275 \frac{kJ}{kg}}
\end{equation*}

``````latex


\section*{Problem 2}