d) 1. HS um Eis:
\begin{equation}
\frac{dE}{dt} = \sum_i \dot{m}_i (h_i + \frac{p_i}{\rho_i} + \frac{v_i^2}{2}) + \dot{Q} - \dot{V}
\end{equation}

\begin{equation}
\Delta U = Q_{12}
\end{equation}

\begin{equation}
m_{ew} (u_2 - u_1) = Q_{12}
\end{equation}

\begin{equation}
u_2 - u_1 = \frac{Q_{12}}{m_{ew}} \Rightarrow u_2 = u_1 + \frac{Q_{12}}{m_{ew}}
\end{equation}

\begin{equation}
u_1 = u_{rest} + x_{eis,1} (u_{schliss} - u_{rest})
\end{equation}

\begin{equation}
= (-333.485 + 0.6 (-0.045 \cdot 333.485)) \, \frac{\text{kJ}}{\text{kg}}
\end{equation}

\begin{equation}
= -133.421 \, \frac{\text{kJ}}{\text{kg}}
\end{equation}

\begin{equation}
u_2 = -133.421 \, \frac{\text{kJ}}{\text{kg}} + \frac{1.5 \, \text{kJ}}{0.1 \, \text{kg}} = -118.421 \, \frac{\text{kJ}}{\text{kg}}
\end{equation}

\begin{equation}
T_{eis,2} = T_{eis,1} + 0.003 \, ^\circ \text{C}
\end{equation}

\begin{equation}
x_{eis,2} = \frac{u_2 - u_{rest}}{u_{schliss} - u_{rest}} = \frac{-118.421 + 333.442}{-0.033 + 333.442} = 0.64
\end{equation}

``````latex