c) \text{miges.}

\[
\Delta_{ex,st} = e_{x,st,6} - e_{x,st,0}
\]

\[
\Delta_{ex,st} = (h_6 - h_0 - T_0 (s_6 - s_0) + \Delta ke)
\]

\[
\Delta ke = \frac{\omega_6^2}{2} - \frac{\omega_2^2}{2} = \frac{3200 \frac{m^2}{s^2}}{2} - \frac{200 \frac{m^2}{s^2}}{2}
\]

\[
= \frac{(10 \frac{m}{s})^2}{2} - \frac{(200 \frac{m}{s})^2}{2}
\]

\[
h_6 - h_0 = C_p (T_6 - T_5) = 110050 \frac{J}{kg} = 110.1 \frac{kJ}{kg}
\]

\[
\Delta s_T = e_{1000} (300K - (27.2 + 15 - 30)K)
\]

\[
= 97 \frac{kJ}{kg}
\]

\[
\Delta e = T_0 (s_6 - s_0) = 243.15 \frac{kJ}{kg} \cdot C_p \ln \left( \frac{T_6}{T_0} \right) - R \ln \left( \frac{P_6}{P_0} \right)
\]

\[
= 82.0 \frac{kJ}{kg}
\]

\[
\Delta_{ex,st} = (97 - 82.0 + 110.1) \frac{kJ}{kg} = 125.09 \frac{kJ}{kg}
\]