c)
\[
W_G = 520 \frac{\text{kJ}}{\text{kg}}
\]
\[
T_6 = 340 \text{K}
\]
\[
\Delta e_{\text{ex,istr}} = e_{\text{ex,istr6}} - e_{\text{ex,istr0}}
\]
\[
e_{\text{ex,istr6}} = h_6 - h_0 - T_0 (s_6 - s_0) + \frac{w_6^2}{2}
\]
\[
e_{\text{ex,istr0}} = h_0 - h_0 - T_0 (s_0 - s_0) + \frac{w_0^2}{2}
\]
\[
\Delta e_{\text{ex,istr}} = h_6 - h_0 - T_0 (s_6 - s_0) + \frac{w_6^2 - w_0^2}{2}
\]
\[
T_{u0} = T_0 = 243.15 \text{K}
\]
\[
h_6 - h_0 = c_p \cdot (T_6 - T_0) \quad \text{(stabiles IG)}
\]
\[
s_6 - s_0 = c_p \cdot \ln \left( \frac{T_6}{T_0} \right) - R \ln \left( \frac{p_6}{p_0} \right) \quad \text{(IG)}
\]
\[
\Delta e_{\text{ex,istr}} = c_p \cdot \left[ (T_6 - T_0) - T_0 \ln \left( \frac{T_6}{T_0} \right) \right] + \frac{w_6^2 - w_0^2}{2}
\]
\[
\Delta e_{\text{ex,istr}} = 1.006 \frac{\text{kJ}}{\text{kg} \cdot \text{K}} \left[ (340 - 243.15) - 243.15 \cdot \ln \left( \frac{340}{243.15} \right) \right] + \frac{520^2 - 200^2}{2}
\]
\[
\Delta e_{\text{ex,istr}} = 125.42 \frac{\text{kJ}}{\text{kg}}
\]