c) \(\dot{S}_{\text{erz}}\):
\[
0 = \dot{m} [s_e - s_a] + \frac{\dot{Q}}{T} + \dot{S}_{\text{erz}}
\]
\[
\Rightarrow \dot{S}_{\text{erz}} = \dot{m} C [s_a - s_e] - \frac{\dot{Q}}{T}
\]
\[
= 0.3 (1.3374 - 0.9889) - \frac{-65 \, \text{kW}}{295 \, \text{K}}
\]

\[
s_a = 1.3065 + 0.005 (7.3549 - 1.3065) \quad \text{at} \quad 100^\circ
\]
\[
= 1.3374
\]

\[
s_e = s_{e2} \quad \text{at} \quad 0.9549 + 0.005 (7.7553 - 0.6491)
\]
\[
= 0.9889
\]

\[
\dot{S}_{\text{erz}} = 0.3 (1.3374 - 0.9889) - \frac{65 \, \text{kW}}{295 \, \text{K}} = -220.23 \, \frac{\text{kJ}}{\text{K}}
\]

``````latex