

\subsection*{c)}

\[
\Delta s_{1-6} = \dot{m} \left( h_0 - h_6 - T_0 \left( s_6 - s_0 \right) + \frac{v_6^2}{2} \right)
\]

\[
\Delta s_{1-6} = \dot{m} \left( h_6 - h_0 - T_0 \left( s_6 - s_0 \right) + \frac{v_6^2}{2} \right)
\]

\[
\Delta s_{1-6} = \dot{m} \left( h_6 - h_0 - T_0 \left( s_6 - s_0 \right) + \frac{v_6^2}{2} \right)
\]

\[
\Delta s_{1-6} = \dot{m} \left( h_6 - h_0 - T_0 \left( s_6 - s_0 \right) + \frac{v_6^2}{2} \right)
\]

\[
\Delta s_{1-6} = \dot{m} \left( h_6 - h_0 - T_0 \left( s_6 - s_0 \right) + \frac{v_6^2}{2} \right)
\]

\[
\Delta s_{1-6} = \dot{m} \left( h_6 - h_0 - T_0 \left( s_6 - s_0 \right) + \frac{v_6^2}{2} \right)
\]

\```latex