

\subsection*{e)}

\begin{align*}
    m_2 s_2 - m_1 s_1 &= \Delta m_2 s_{\text{ein}} + \frac{Q}{T} = S_{12}
\end{align*}

\begin{align*}
    \Delta S_{12} &= m_2 s_2 - m_1 s_1 - \Delta m_2 s_{\text{ein}}
\end{align*}

\begin{align*}
    s_2 &= s_l(70^\circ) = 0.3548 \, \frac{\text{kJ}}{\text{kg K}} \\
    s_1 &= s_l(100^\circ) + x_1 \left( s_{lg}(100^\circ) - s_l(100^\circ) \right) = 1.357416 \, \frac{\text{kJ}}{\text{kg K}} \\
    s_{\text{ein}} &= s_l(20^\circ) = 0.2966 \, \frac{\text{kJ}}{\text{kg K}}
\end{align*}

\begin{align*}
    \Delta S_{12} &= 162.8 \, \frac{\text{kJ}}{\text{K}}
\end{align*}

\begin{align*}
    m_2 &= m_1 + \Delta m_2 = 93.4 \, \text{kg} \\
    m_1 &= 57.55 \, \text{kg}
\end{align*}

``````latex