

\subsection*{d)}

\begin{align*}
    m_1 &= 57.55 \, \text{kg} \\
    x_1 &= 0.005 \\
    T_1 &= 100^\circ \text{C}
\end{align*}

\begin{align*}
    h_2 &= h_1(100^\circ) + x_1 \left( h_{lg}(100^\circ) - h_l(100^\circ) \right) = 430.3253 \, \frac{\text{kJ}}{\text{kg}} \\
    u_2 &= u_1(100^\circ) + x_1 \left( u_{lg}(100^\circ) - u_l(100^\circ) \right) = 423.3778 \, \frac{\text{kJ}}{\text{kg}}
\end{align*}

\begin{align*}
    \text{hinzu} \quad m_h \Delta m_2 \quad T_{\text{ein}} = 20^\circ \text{C} \quad x_{\text{ein}} = 0 \quad u_{\text{ein}} = u_l(20^\circ \text{C}) = 83.85 \, \frac{\text{kJ}}{\text{kg}} \quad \Delta t
\end{align*}

\text{Energieerhaltung:}

\begin{align*}
    \frac{dE}{dt} &= \text{Eintritt} - \text{Austritt} + \sum Q - \sum W = 0 \\
    \Delta U &= Q \quad Q = 55 \, \text{MJ}
\end{align*}

\subsection*{2:}

\begin{align*}
    T_2 &= 70^\circ \text{C} \\
    x_2 &= 0
\end{align*}

\begin{align*}
    h_2: \quad u_2 &= u_l(70^\circ) = 292.35 \, \frac{\text{kJ}}{\text{kg}}
\end{align*}

\begin{align*}
    (m_1 + \Delta m_2) u_2 - m_1 u_1 - \Delta m_2 u_{\text{ein}} &= Q \\
    \Delta m_2 u_2 - \Delta m_2 u_{\text{ein}} &= Q - m_1 u_1 + m_1 u_2 \\
    \Delta m_2 &= \frac{Q - m_1 u_1 + m_1 u_2}{u_2 - u_{\text{ein}}} = 35.83 \, \text{kg}
\end{align*}