

\subsection*{c)}

\begin{equation*}
Q_{12} = m (u_{2} - u_{1})
\end{equation*}

\begin{equation*}
Q_{12} = m \cdot 0.653 \frac{\text{kJ}}{\text{kg K}} (T_{2} - T_{1})
\end{equation*}

\begin{equation*}
Q_{12} = -1 \, 082.183
\end{equation*}

``````latex


\section*{Student Solution}

\begin{itemize}
    \item Zustand 2 $Q = 0$
    \item $m_6 (u_2 - u_1) = m_{EL} (u_2 - u_1)$
    \item $m \cdot c_v (T_2 - T_1) = m \cdot c_w (u_2 - u_1)$
    \item $1,139,89$
    \item $-11,353,03 \cdot \frac{D}{\eta_{12}} (u_2 - u_1)$
    \item $u_1 = -133,91$
    \item $u_1 = -146 \frac{12}{19}$
    \item Interpolation bei $p_2 = 0,003 = \frac{x - u_f}{u_g - u_f}$
    \item $x = \frac{-146 - u_f}{u_g - u_f}$
    \item $x = 560,568$
\end{itemize}

``````latex