

\section*{c)}

\[
\Delta e_{x, \text{ist}} = (h_6 - h_0 - T_0 (s_6 - s_0) + \frac{1}{2} \dot{m} w_6^2 - \frac{1}{2} \dot{m} w_0^2)
\]

\[
m_{05} = 
\]

\[
\dot{m} k = 5.293
\]

\[
\dot{m}_{05} = 5.293 \dot{m}
\]

\[
\Delta e_{x, \text{st}} = (cp (T_6 - T_0) - T_0 \left( cp \left( \ln \left( \frac{T_6}{T_0} \right) - R \ln \left( \frac{P_0}{P_0} \right) \right) \right) + \frac{w_6^2 - w_0^2}{2})
\]

\[
T_6, w_6 \text{ von}
\]

\textbf{LÃ¶sung:}

\[
s_{ext} = 14.413 \frac{kJ}{kg} + 110.050 \frac{kJ}{kg} = 264.18 \frac{kJ}{kg}
\]