

\subsection*{d)}
\[
\epsilon_k = \frac{\dot{Q}_{\text{zu}}}{\dot{Q}_{\text{ab}} - \dot{Q}_{\text{zu}}} = \frac{\dot{Q}_k}{\dot{W}_k} = 2,0836 = \epsilon_k
\]

\[
\dot{Q}_k = \dot{m} (h_2 - h_1)
\]

\[
= \frac{1,9667 \cdot 10^{-4} \frac{\text{kg}}{\text{s}}}{2,6068 \cdot 10^{-4} \frac{\text{kg}}{\text{s}}} \cdot (249,53 \frac{\text{kJ}}{\text{kg}} - 93,42 \frac{\text{kJ}}{\text{kg}}) = 0,029765 \frac{\text{kJ}}{\text{s}} = \dot{Q}_k
\]

\[
\dot{Q}_k = 41,6718 \frac{\text{J}}{\text{s}}
\]

\[
= 0,0416718 \frac{\text{kJ}}{\text{s}} = \dot{Q}_k
\]

```