

\subsection*{c)}
\[ x_1 \]

\[
0 = \dot{m} (h_4 - h_1) \quad \text{-- da } \dot{W} = 0 \quad \dot{Q} = 0
\]

\[
h_4 = h_1
\]

\[
h_4 = h_f (8 \text{bar}) \quad \text{TAB A-11}
\]

\[
h_4 = 93,42 \frac{\text{kJ}}{\text{kg}} = h_1
\]

\[
h_1 = h_f + x (h_g - h_f)
\]

\[
p_1 - p_2 \quad \text{TAB A-10}
\]

\[
p_2 (4^\circ \text{C}) = 3,3765 \text{bar} \quad \text{TAB A-11}
\]

\[
h_f (3,3765 \text{bar}) = \frac{h_f (3,6 \text{bar}) - h_f (3,2 \text{bar})}{3,6 - 3,2} \cdot (3,3765 - 3,2) + h_f (3,2 \text{bar})
\]

\[
h_f = 55,3 \frac{\text{kJ}}{\text{kg}}
\]

\[
h_g (3,3765 \text{bar}) = \frac{h_g (3,6 \text{bar}) - h_g (3,2 \text{bar})}{3,6 - 3,2} \cdot (3,3765 - 3,2) + h_g (3,2 \text{bar})
\]

\[
h_g = 249,5072
\]

\[
x = \frac{h_1 - h_f}{h_g - h_f} = 0,1963 = x_1
\]