\subsection*{a) Q\textsubscript{aus}}

\subsubsection*{1. Hauptsatz der Thermodynamik}
\[
\dot{Q}_E = \sum_i \dot{m}_i (h_i)_{\text{ein}} - \sum_j \dot{m}_j (h_j)_{\text{aus}} + \sum_i \dot{Q}_i (i) - \sum_j \dot{W}_j (j)
\]
\[
\dot{Q}_E = \dot{m}_{\text{ein}} (h_{\text{ein}} + h_{\text{aus}}) + \dot{Q}_R + \dot{Q}_{\text{aus}}
\]

\subsubsection*{Zustandsgrößen}
\[
h_{\text{ein}} - h_{\text{aus}}
\]

\subsubsection*{Zustand 1}
\[
\text{Ein: } 70^\circ \text{C}
\]
\[
\text{aus Tabelle A-2}
\]
\[
\text{und } q_2: q_1 + (q_2 - q_1)
\]

\subsubsection*{Zustand 2}
\[
\text{Ein: } 100^\circ \text{C}
\]
\[
\text{aus Tabelle A-2}
\]
\[
\text{und } q_2: q_1 + (q_2 - q_1)
\]

\[
h_{\text{ein}} = 297,35 + 0,005 \cdot 0,025 \cdot (297,35 - 253,15) \frac{\text{kJ}}{\text{kg}} = 304,643 \frac{\text{kJ}}{\text{kg}}
\]

\[
h_{\text{aus}} = 473,04 + 0,005 \cdot 0,10 \cdot 5 \cdot 297,6 \cdot (473,04 - 253,15) \frac{\text{kJ}}{\text{kg}} = 430,325 \frac{\text{kJ}}{\text{kg}}
\]

\[
\dot{Q}_{\text{aus}} = 0,3 \frac{\text{kg}}{\text{s}} \cdot (304,643 \frac{\text{kJ}}{\text{kg}} - 430,325 \frac{\text{kJ}}{\text{kg}}) + 100 \frac{\text{kW}}{\text{kg}} - \dot{Q}_{\text{aus}}
\]

\[
\Rightarrow \dot{Q}_{\text{aus}} = 62,29 \text{kJ}
\]