c) 

\[ m (U_{2a} - U_{1a}) + Q_{12} = 0 \]

\[
\begin{array}{|c|c|}
\hline
\text{Gas} & \text{EW} \\
\hline
\end{array}
\]

\[ m_g (c_v (T_{a2} - T_{a1})) \neq Q_{12} \]

\[ c_v = 0.633 \, \frac{\text{kJ}}{\text{kg} \cdot \text{K}} \]

\[ m_g c_v \Delta T = Q_{12} \]

\[ 0.0277 \, \text{kg} \cdot 0.633 \, \frac{1}{\text{kg} \cdot \text{K}} \left( -499.997 \, \text{K} \right) = Q_{12} \]

\[ -7.21 \, \text{kJ} = Q_{12} \]

\[ \Rightarrow 7.21 \, \text{kJ} \]

WÃ¤rme von Gas zu EW

``````latex


d \quad \cancel{d} \quad AGW

\[
\Rightarrow \quad \cancel{\cancel{d}} \quad U_{zg} - U_{zew} = 0
\]

\[
Mg U_{zg} - MEW U_{zew} = 0
\]

``````latex


36

\[
\text{EW}
\]

\[
\text{A} \quad \dot{Q}_{zu} \ln \left( \frac{U_2 - U_1}{U_1} \right) = Q_{zu}
\]

\[