

\subsection*{c)}

\[
-\Delta \dot{E}_{xstr} = \dot{E}_{xstr,0} - \dot{E}_{xstr,e}
\]

\[
\dot{m} (h_0 - h_e - T_0 (s_0 - s_e) + \Delta ke)
\]

\[
-\dot{e}_{xstr} = h_0 - h_e - T_0 (s_0 - s_e)
\]

\[
= C_p (T_0 - T_e) - T_0 \left( \ln \frac{T_0}{T_e} - R \left( \ln \frac{p_0}{p_e} \right) \right) + \frac{W_0^2 - W_e^2}{2}
\]

\[
= -1.006 \frac{kJ}{kg} \left( 297.15k - 328.1k \right) - 293.15k \left( \ln \left( \frac{297.15k}{328.1k} \right) \right) - 0.287 \frac{kJ}{kg} \left( \ln (1) \right)
\]

\[
+ \frac{200^2 \frac{m^2}{s^2}}{2} - \frac{329 \frac{m^2}{s^2}}{2}
\]

\[
\underline{\hspace{5cm}}
\]

\[
\dot{e}_{xstr} = 119.5 \frac{kJ}{kg}
\]