

\subsection*{c)}

\[
\text{ex}_{\text{str,6}} = h_6 - h_0 - T_0 (s_6 - s_0) + \frac{1}{2} \omega_6^2
\]

\[
\text{ex}_{\text{str,0}} = h_0 - h_0 - T_0 (s_0 - s_0) + \frac{1}{2} \omega_0^2
\]

\[
\Delta \text{ex}_{\text{str,06}} = \text{ex}_{\text{str,6}} - \text{ex}_{\text{str,0}} = h_6 - h_0 - T_0 s_6 + T_0 s_0 + \frac{1}{2} \omega_6^2 - \frac{1}{2} \omega_0^2
\]

\[
= c_p (T_6 - T_0) = -T_0 (s_6 - s_0)
\]

\[
\Delta \text{ex}_{\text{str,06}} = c_p (T_6 - T_0) - T_0 \left( c_p \ln \left( \frac{T_6}{T_0} \right) + \frac{\omega_6^2 - \omega_0^2}{2} \right) - R_u \left( \frac{\dot{V}_{\text{es}}}{\dot{m}_p} \right)
\]

\[
= 120.8 \, \frac{\text{kJ}}{\text{kg}}
\]

``````latex

\section*{Aufg. 2}