

\section*{c)}

\begin{align*}
    \dot{m}_{ges} \frac{c_2^2}{2} &= \Delta e_{ex,str} \\
    \Delta e_{ex,str} &= \dot{m}_{ges} \left( h_6 - h_0 - T_0 (s_6 - s_0) + \frac{c_6^2}{2} - \frac{c_0^2}{2} \right)
\end{align*}

\begin{align*}
    h_6 - h_0 &= c_p (T_6 - T_0) \\
    s_6 - s_0 &= c_p \ln \left( \frac{T_6}{T_0} \right) - R \ln \left( \frac{p_6}{p_0} \right) = c_p \ln \left( \frac{T_6}{T_0} \right)
\end{align*}

\begin{align*}
    \Delta e_{ex,str} &= \dot{m}_{ges} \left( h_6 - h_0 - T_0 \left( c_p \ln \left( \frac{T_6}{T_0} \right) \right) + \frac{c_6^2}{2} - \frac{c_0^```latex