b) \\
x_{\text{eis,2}} > 0 \\
T_{g1,2} = ? \\
p_g = ? \\

\begin{align*}
p_{g2} &= p_{g1} = 1.2885 \, \text{bar} \\
pV &= RT_A \\
\left[ V_A = \frac{RT_A}{p_g} = \frac{0.16628 \, \frac{\text{kJ}}{\text{kg} \cdot \text{K}} \cdot (500 + 273.15)}{1.2885 \cdot 10^2 \, \frac{\text{kN}}{\text{m}^2}} = 0.997745 \, \frac{\text{m}^3}{\text{kg}} \right]
\end{align*}

\begin{align*}
p_A V_A &= ? \\
\frac{pV}{R} &= \frac{mRT}{R} \\
R &= \frac{pV_A}{T_{0^\circ \text{C}} \cdot m_{\text{eis}}} \\
\frac{pV_0}{R_0} &= \frac{p```latex



\section*{3b)}
$x_{eis,2} = ?$

\[
\Delta Q = Q - W
\]

\[
E = U + \frac{pV}{m} = 0
\]

\[
\Delta U = Q - W
\]

\[
\Delta U = Q_{12} = 1.500 J
\]

\[
U = U
\]

\[
U_1 = U
\]

\[
T = 0^\circ C \quad x = 0.6
\]

\[
\text{Tabelle 1}
\]

\[
u_{fest} = -333.4158 \frac{kJ}{kg}
\]

\[
u_{fl端ssig} = -0.045 \frac{kJ}{kg}
\]

\[
u_1 = u_{fest} + x (u_{fl端ssig} - u_{fest})
\]

\[
= -333.4158 + 0.6 (-0.045 + 333.4158) \frac{kJ}{kg} = -133.6532 \frac{kJ}{kg} = u_1
\]

\[
u_2 = u_{fest} + x_2 (u_{fl端ssig} - u_{fest})
\]

\[
= -333.442 + x_2 (-0.033 + 333.442) \frac{kJ}{kg}
\]

\[
m = 0.1 kg
\]

\[
m \cdot c (u_1 - u_2) = Q_{12}
\]

\[
c \cdot m (u_1 - u_2) = \frac{Q_{12}}{m}
\]

\[
u_2 = u_1 - \frac{Q_{12}}{m}
\]

\[
x_2 = \frac{u_1 - \frac{Q_{12}}{m} - u_{fest}}{u_{fl端ssig} - u_{fest}}
\]

\[
x_2 = \frac{-133.6532 \frac{kJ}{kg} - 1.500 \frac{kJ}{0.1 kg} + 333.442 \frac{kJ}{kg}}{-0.033 + 333.442 \frac{kJ}{kg}}
\]

\[
x_2 = 0.5542
\]

``````latex