

\subsection*{b)}

\[
T_{KF} = \frac{\int_{T_e}^{T} T \, dS}{S_{max} - S_{min}} \quad \text{(Siedelnde Fl√ºssigkeit)}
\]

\[
= \frac{1}{c^{ii}} \left( \frac{T_{aus}^3}{T_{ein}^3} \right)
\]

\[
= \frac{S_e - T \, dS}{\int_{T_e}^{T} \frac{c^{ii}}{T} \, dT}
\]

\[
= \frac{T_e \int_{T_e}^{T} e^{\frac{S - S_e}{c^{ii}}} \, dS}{c^{ii} \ln \left( \frac{T_{max}}{T_{min}} \right)}
\]

\[
= \frac{T_e e^{\frac{S_e}{c^{ii}}} \left[ e^{\frac{S}{c^{ii}}} - e^{\frac{S_e}{c^{ii}}} \right]}{c^{ii} \ln \left( \frac{T_{max}}{T_{min}} \right)}
\]

\[
S - S_e = c^{ii} \ln \left( \frac{T}{T_e} \right) \Rightarrow T = T_e e^{\frac{S - S_e}{c^{ii}}}
\]

\[
= \underline{\hspace{2cm}}
\]

``````latex