

\section*{d)}

\[ e_{x,vel} = T_{0} (s_{6} - s_{0}) = \cancel{\dot{m}_{in} \left( T_{0} (s_{6} - s_{0}) + \frac{1}{2} (w_{2}^{2} - w_{0}^{2}) \right)} \]

\[ \dot{Q}_{B,5A} = \frac{\dot{Q}_{B}}{\dot{m}_{in}} = \frac{\dot{Q}_{B}}{\dot{m}_{ges}} = 6.233 \Rightarrow \frac{\dot{Q}_{B}}{\dot{m}_{ges}} = 6.233 \, \dot{Q}_{B} = \dot{Q}_{B,5A} \]

\[ \Rightarrow e_{x,vel} = T_{0} (s_{6} - s_{0}) - \cancel{\dot{m}_{in} \left( \frac{1}{2} (w_{2}^{2} - w_{0}^{2}) \right)} \]

\[ s_{6} - s_{0} = c_{p} \ln \left( \frac{T_{6}}{T_{0}} \right) \]

``````latex