

\subsection*{b)}

\[
\dot{E}_{\text{kf}} = \frac{\int_a^e T \, ds}{s_a - s_e} \quad \text{ex. umben.} \quad \frac{T_{\text{aus}} - T_{\text{ein}}}{\ln \left( \frac{T_{\text{aus}}}{T_{\text{ein}}} \right)} = 293.12 \, \text{K}
\]

\[
s_a - s_e = c_{l} \ln \left( \frac{T_{\text{aus}}}{T_{\text{ein}}} \right) \quad (\text{ideale Fl√ºssigkeit}) \quad (\text{isobar})
\]

\[
\int_a^e T \, ds = q_{\text{zu}} = h_{\text{aus}} - h_{\text{ein}} \quad (\text{1. HS})
\]

\[
= c_{l} \left[ T_{\text{aus}} - T_{\text{ein}} \right] \quad (\text{ideale Fl.}) \quad (\text{isobar})
\]

\[
T_{\text{aus}} = 298.15 \, \text{K}
\]

\[
T_{\text{ein}} = 288.15 \, \text{K}
\]

``````latex