a) \(\dot{Q}_{\text{aus}}^* = -\dot{m} (h_e - h_a)\)

\[
\begin{aligned}
    T_{K,\text{ein}} &= 288.15 \, \text{K} \\
    T_{K,\text{aus}} &= 298.15 \, \text{K}
\end{aligned}
\]

\[
\begin{aligned}
    T_{\text{ein}} &= 70^\circ \text{C} \\
    T_{\text{aus}} &= 100^\circ \text{C} \quad \text{(reines Wasser)}
\end{aligned}
\]

\[
\begin{aligned}
    h_e &= h_f(70^\circ \text{C}) \quad \text{/TAB. A-2} \\
    &= 292.98 \, \frac{\text{kJ}}{\text{kg}}
\end{aligned}
\]

\[
\begin{aligned}
    h_{ea} &= h_f(100^\circ \text{C}) + x_D \cdot (h_g(100^\circ \text{C}) - h_f(100^\circ \text{C})) \\
    &= 419.04 + 0.005 \cdot (2676.1 - 419.04) \, \left[\frac{\text{kJ}}{\text{kg}}\right] \\
    &= 430.33 \, \left[\frac{\text{kJ}}{\text{kg}}\right]
\end{aligned}
\]

\[
\begin{aligned}
    \dot{Q}_{\text{aus}}^* &= -0.3 \, \frac{\text{kg}}{\text{s}} \left[ 292.98 \, \frac{\text{kJ}}{\text{kg}} - 430.33 \, \frac{\text{kJ}}{\text{kg}} \right] \\
    &= 41.2 \, \text{kW} \quad \rightarrow \quad \dot{Q}_R = \dot{Q}_{\text{aus}}^* - \dot{Q}_{\text{aus}} \\
    \dot{Q}_{\text{aus}} &= 58.8 \, \text{kW}
\end{aligned}
\]