d)

\[
\dot{m}_2 u_2 - m_1 u_1 = \sum_i \dot{m}_i [h_i] \iff Q_{\text{aus,72}}
\]

\[
\Delta m \cdot h_{\text{ein}} = m_2 \cdot u_2 - m_1 \cdot u_1 + Q_{\text{aus,72}}
\]

\[
\Delta m (h_{\text{ein}} - u_2) = m_1 (u_2 - u_1) + Q_{\text{aus,72}}
\]

\[
\Delta m = \frac{1}{h_{\text{ein}} - u_2} (m_1 (u_2 - u_1)) + Q_{\text{aus,72}}
\]

\[
\Delta m = \dots = 3307.3 \text{kg}
\]

2)

\[
\Delta S = m_2 s_2 - m_1 s_1
\]

\[
= (5755 \text{kg} + 3302 \text{kg}) 0.2594 \frac{\text{kJ}}{\text{kg K}}
\]

\[
- 5755 \text{kg} \cdot 7.306 \frac{\text{kJ}}{\text{kg K}} = 7768 \frac{\text{kJ}}{\text{kg}}
\]

\[
s_1 = 7000 \frac{\text{kJ}}{\text{kg}} = 7.306 \frac{\text{kJ}}{\text{kg K}}
\]

\[
s_2 = 7000 \frac{\text{kJ}}{\text{kg}} = 0.2594 \frac{\text{kJ}}{\text{kg K}}
\]

\[
m_2 = m_1 + \Delta m
\]

``````latex