d) 
\[
u_n = x \cdot u_{fl√ºssig} + (x - x) \cdot u_{fest} = 0.6 \cdot (-0.045 \frac{kJ}{kg}) + (0.4) \cdot (-333.485 \frac{kJ}{kg})
\]
\[
= -733.9702 \frac{kJ}{kg}
\]

``````latex

3d

\[
u_1 = -733.4702 \frac{\text{kJ}}{\text{kg}}
\]

\[
U_2 = m_{w} u_1 + Q_{12} = m_{w} u_2
\]

\[
\Rightarrow u_2 = u_1 + \frac{Q_{12}}{m_{w}} = -733.4702 \frac{\text{kJ}}{\text{kg}} + \frac{77.35 \text{kJ}}{0.7 \text{kg}}
\]

\[
= -733.4702 \frac{\text{kJ}}{\text{kg}} + 110.5 \frac{\text{kJ}}{\text{kg}}
\]

\[
= -79.97 \frac{\text{kJ}}{\text{kg}}
\]

\[
x_2 (u_{FI} - u_{FE}) = U_2 - U_{FE}
\]

\[
x = \frac{U_2 - U_{FE}}{u_{FI} - u_{FE}} = \frac{-79.97 \frac{\text{kJ}}{\text{kg}} + 333.958 \frac{\text{kJ}}{\text{kg}}}{-0.085 \frac{\text{kJ}}{\text{kg}} + 333.958 \frac{\text{kJ}}{\text{kg}}} \approx 0.990
\]

``````latex