d) 1. HS.

\[
\Delta E = \Delta m_{12}(h) + \dot{Q}
\]

\[
m_2 u_2 - m_1 u_1 = \Delta m_{12} h + \dot{Q}
\]

\[
\Delta m_{12} = \frac{1}{h} (m_2 u_2 - m_1 u_1 - \dot{Q})
\]

\[
h = h_f(20^\circ) = \cancel{88} \ 83.96 \left[\frac{kJ}{kg}\right], \quad A2 \ (\text{illegible text})
\]

\[
\dot{Q} = -35 \text{MJ}
\]

\[
m_2 u_2 - m_1 u_1:
\]

\[
T_1 = 100^\circ C \quad T_2 = 70^\circ C
\]

\[
m_1 = 5755 \text{kg}
\]

\[
m_2 = m_1 + \Delta m
\]

\[
u_2 = u_f(T_2) = 232.15 \left[\frac{kJ}{kg}\right], \quad A2
\]

\[
u_1 = u_f(T_1) = 418.94 \left[\frac{kJ}{kg}\right], \quad A2
\]

\[
\Rightarrow \Delta m_{12} = \frac{1}{h} m_2 u_2 + \frac{1}{h} \Delta m u_2 - m_1 u_1 \frac{1}{h} - \dot{Q} \frac{1}{h}
\]

\[
\Delta m \left(1 - \frac{u_2}{h}\right) = \frac{1}{h} (m_2 u_2 - m_1 u_1 - \frac{\dot{Q}}{h})
\]

\[
\Delta m = \frac{1}{83.96} (5755 \cdot 232.15 - 5755 \cdot 418.94 - \frac{-35 \cdot 10^3}{83.96})
\]

\[
= \cancel{3888} \ 3965.9 \text{kg}
\]