a)

\[
0 = \dot{m}_{\text{aus}} \left[ h_{\text{em}} - h_{\text{aus}} \right] + \dot{Q}_{\text{aus}}
\]

\[
\dot{Q} = \dot{m}_{\text{aus}} \left[ h_{\text{aus}} + h_{\text{em}} \right]
\]

\[
\dot{Q} = Q_{\text{1}} \left( 449,04 + 292,88 \right)
\]

\[
= 371,87 \, \text{J}
\]

\begin{itemize}
    \item On the right side of the page, there are two notes:
    \begin{itemize}
        \item $h_{\text{em}} = 292,88 \, \frac{\text{kJ}}{\text{kg}}$
        \item $h_{\text{aus}} = 449,04 \, \frac{\text{kJ}}{\text{kg}}$
    \end{itemize}
\end{itemize}

a)

\[
0E = m_2 u_2 - m_1 u_1 = 0 m_2 \left[ h_1 \right] + Q_{aus}
\]

\[
\Delta m_2 = m_2 u_2 - m_1 u_1 - Q_{aus}
\]