a) 

\underline{ref 1} \quad P_g = P_{amb} + \frac{4 \cdot m_u \cdot g}{D^2 \pi} + \frac{4 \cdot m_{ew} \cdot g}{D^2 \pi} \quad \left| A = \frac{D^2}{4 \pi} \right.

\[
= 1 \text{bar} + \frac{4 \cdot g}{D^2 \pi} (m_u + m_{ew})
\]

\[
= 1 \text{bar} + \frac{4 \cdot 9.81}{(0.7 \text{m})^2 \pi} \left(32 \text{kg} + 0.7 \text{kg}\right)
\]

\[
P_g = \boxed{1.4 \text{bar}}
\]

\[
m_g = \frac{P_g V_{1,1} M}{R \cdot T_{1,1}} = \frac{1.4 \text{bar} \cdot 3.74 \text{L} \cdot 50 \frac{\text{g}}{\text{mol}}}{8.314 \frac{\text{J}}{\text{mol K}} \cdot 77.75 \text{K}}
\]

\[
m_g = \boxed{3.43 \text{g}}
\]