c)

\begin{align*}
e_{xst} &= \left[ h_6 - h_0 - T_0 (s_6 - s_0) + \frac{\omega_2^2}{2} - \frac{\omega_0^2}{2} \right] \\
&= c_p (T_6 - T_0) - T_0 (s_6 - s_0) + \frac{\omega_2^2}{2} - \frac{\omega_0^2}{2} \\
&= c_p (T_6 - T_0) - T_0 \left( c_p \ln \left( \frac{T_6}{T_0} \right) \right) - R \left( \frac{p_6}{p_0} \right) + \frac{\omega_2^2}{2} - \frac{\omega_0^2}{2} \\
&= 0.7006 (328.0 + 46 - 243.75 \cdot \ln 7.006) - 243.75 \left( \ln 7.006 \right) \\
&\quad + s \cdot \ln \left( \frac{378.07}{243.75} \right) + \frac{2002 - 325^2}{2} \\
&= \frac{\omega_2}{\omega_0} - 77.295 \frac{\text{kJ}}{\text{kg}}
\end{align*}

``````latex