d)

\begin{align*}
u_{1\text{ges}} &= u_{\text{f,est}} + (r-x_1) (u_{\text{f,flüssig}} - u_{\text{f,est}}) \\
&= -333,485 + 0,6 \alpha \left( (1-0,6) (-0,005 + 333,458) \right) \\
&= -200,1768 \frac{\text{kJ}}{\text{kg}}
\end{align*}

\[
\boxed{-200,1768 \frac{\text{kJ}}{\text{kg}}}
\]

\begin{align*}
\Delta E &= E_2 - E_1 = Q_{12} \\
Q_{12} &= m_{\text{ew}} (u_{\text{ew}} - u_{\text{ew}}) \\
&= 0 \, \text{m}_{\text{ew}} \left( u_{\text{f,est}} + (r-x_2) (u_{\text{f,flüssig}} - u_{\text{f,est}}) - a_1 \right)
\end{align*}

``````latex


3.

(d) continued

\begin{equation*}
\frac{Q_{12}}{m_{ew}} = u_{f_{est}} + (1 - x_{2_{eis}})(u_{f_1} - u_{f_{est}}) - u_1
\end{equation*}

\begin{equation*}
\frac{1}{(u_{f_1} - u_{f_{est}})} \left( \frac{Q_{12}}{m_{ew}} - u_{f_{est}} + u_1 \right) = 1 - x_{2_{eis}}
\end{equation*}

\begin{equation*}
1 - \frac{1}{(u_{f_1} - u_{f_{est}})} \left( \frac{Q_{12}}{m_{ew}} - u_{f_{est}} + u_1 \right) = x_{2_{eis}}
\end{equation*}

\begin{equation*}
x_{2_{eis}} = 1 - \frac{1}{(-q_{aus} + 333,485)} \left( \frac{4,0856 \, q}{0,7 \, kg} - 333,458 + 200,000 \right)
\end{equation*}

\begin{equation*}
x_{2_{eis}} = \boxed{0,6828} \quad \boxed{1,567}
\end{equation*}

``````latex