

\subsection*{d)}
\begin{align*}
    \Delta U &= \Delta m (h_1 - h_2) + Q_{12} - Q_{12} \\
    \Delta U &= \Delta m (h_1 - h_2) \\
    \text{mit} \\
    (m_1 + \Delta m) T_2 c_e - m_1 T_a c_p &= \Delta m (h_1 - h_2) \\
    m_1 T_2 c_p - m_1 T_a c &= \Delta m (h_1 - h_2) - T_2 c \\
    \Delta m &= \frac{m_1 T_2 - m_1 T_a c}{(h_1 - h_2) - T_2 c} \\
    h_1, h_2 \quad T_{AB} A-2 \\
    \text{verkleben und } \Delta m \text{ gel√∂st}
\end{align*}

``````latex


\begin{itemize}



\item[d)]
\end{itemize}

\begin{itemize}