

\subsection*{a)}
\begin{align*}
    \dot{Q}_{\text{aus}}: \\
    \dot{Q}_{\text{aus}} &= \dot{Q}_r - \dot{Q}_w \\
    \dot{Q}_w &\rightarrow 0 = \dot{m} (h_e - h_a) + \dot{Q}_w \\
    &\rightarrow \dot{Q}_w = \dot{m} (h_a - h_e) \\
    h_e &= 292,98 + 0,005 (2626,5 - 292,98) = 304,65 \frac{\text{kJ}}{\text{kg}} \\
    h_a &= 419,01 + 0,005 (2676,1 - 419,01) = 430,33 \frac{\text{kJ}}{\text{kg}} \\
    T_{AB} A-2 &\quad T_{AB} A-2 \quad \dot{Q}_w = G_B (430,33 - 304,65) = 37,7 \text{kJ} \\
    L = 100 \text{kg} - 37,7 \text{kg} = 62,30 \text{kJ} = \dot{Q}_{\text{aus}}
\end{align*}