c) \quad \dot{E}_{x, \text{ist,er}} = \dot{e}_{x, \text{ist,er}} - \dot{e}_{x, \text{ist,to}}

\[
\dot{e}_{x, \text{ist,er}} = \dot{m} \left[ h_a - h_c - T_0 (s_a - s_c) + \frac{\Delta w_e}{\dot{m}} \right] = 87.829 \, \frac{\text{kJ}}{\text{kg}}
\]

\[
h_a - h_c = c_p (T_c - T_0) = 85.321 \, \frac{\text{kJ}}{\text{kg}}
\]

\[
T_0 = 243.15 \, \text{K}
\]

\[
s_a - s_c = c_p \ln \left( \frac{T_c}{T_0} \right) - R \ln \left( \frac{p_c}{p_0} \right) = 0.30136 \, \frac{\text{kJ}}{\text{kg K}}
\]

\[
\Delta w_e = \frac{w_e^2}{2} - \frac{w_0^2}{2} = 75.0 + 0.193 = 75.193 \, \frac{\text{kJ}}{\text{kg}}
\]