

\subsection*{c)}

\[
\Delta e_{x,str} = e_{x,str,6} - e_{x,str,0}
\]

\[
= (h_6 - h_0 - T_0 (s_6 - s_0) + \frac{w_6^2}{2} - \frac{w_0^2}{2})
\]

\[
= c_p (T_6 - T_0) - T_0 (c_p \ln \left( \frac{T_6}{T_0} \right) - R \ln \left( \frac{p_6}{p_0} \right)) + \frac{w_6^2}{2} - \frac{w_0^2}{2}
\]

\[
T_6 = \overline{T_6} = 328.07 \, \text{K} \quad T_0 = 283.75 \, \text{K}
\]

\[
c_p = 1.006 \quad w_6 = 502.2 \, \text{m/s} \quad w_0 = 200 \, \text{m/s}
\]

\[
\Delta e_{x,str} = 120.8 \, \frac{\text{kJ}}{\text{kg}}
\]