

\subsection*{b)}

\begin{equation*}
    1. \, \text{HS}
\end{equation*}

\begin{equation*}
    \dot{m} (h_2 - h_3) = \omega
\end{equation*}

\begin{equation*}
    \dot{m} = \frac{\omega}{h_2 - h_3}
\end{equation*}

\begin{equation*}
    T_1 = -20^\circ \text{C} = T_2
\end{equation*}

\begin{equation*}
    h_{2f} = 29.26 \, \frac{\text{kJ}}{\text{kg}}
\end{equation*}

\begin{equation*}
    T_3 = T_2 \left( \frac{P_3}{P_2} \right)
\end{equation*}

\begin{equation*}
    \text{mit} \quad T_3 \quad \text{und} \quad P_3 = 4 \text{bar}
\end{equation*}

\begin{equation*}
    \text{in Tabelle} \quad h_3 = h_{2f}
\end{equation*}

``````latex