

\subsection*{b)}

\begin{itemize}
    \item $1 \, \text{HS}$ \quad \text{Schreibweise}
    \item \text{station√§r:} \quad $Q = 0 \quad \omega = 0$
\end{itemize}

\[
0 = \dot{m} (h_5 - h_6 + \frac{\omega_5^2 - \omega_6^2}{2})
\]

\[
= \dot{m} c_p (T_5 - T_6) + y_5 \frac{\omega_5^2}{2} - y_6 \frac{\omega_6^2}{2}
\]

\[
\omega_6 = \sqrt{\omega_5^2 + 2 c_p (T_5 - T_6)}
\]

\begin{itemize}
    \item \text{AS Gleichung:}
\end{itemize}

\[
0 = \dot{m} (h_2 - h_3) + Q
\]

\begin{itemize}
    \item \text{adiabat + reversibel = isentrop}
\end{itemize}

\[
T_6 - T_5 = \left( \frac{P_6}{P_5} \right)^{\frac{k-1}{k}} = 831.94 \left( \frac{0.459 \, \text{bar}}{0.5 \, \text{bar}} \right)^{\frac{0.4}{1.4}} = 328.07 \, K
\]

\[
\omega_0 = \sqrt{(270 \, \frac{m}{s})^2 + 1.006 \frac{kJ}{kgK} (831.94 - 328.07 \, K)} = 507.25 \, \frac{m}{s}
\]

``````latex