

\subsection*{a)}

\begin{align*}
\text{1HS} & \quad \text{Reaktion} \\
0 &= \dot{m}_{\text{ein}} (h_e - h_a) + \dot{Q}_{\text{ab}} \\
\dot{Q}_{\text{ab}} &= \dot{m} (h_a - h_e) \\
&= 0.3 \frac{\text{kg}}{\text{s}} (1407.6 \frac{\text{kJ}}{\text{kg}} - 1265.4 \frac{\text{kJ}}{\text{kg}}) \\
&= 42.18 \text{ kW}
\end{align*}

\begin{align*}
\dot{Q}_{\text{aus}} &= \dot{Q}_R - \dot{Q}_{\text{ab}} \\
&= 100.6 \text{ kW} - 42.78 \text{ kW} \\
&= 57.82 \text{ kW}
\end{align*}

\section*{Aufgabe a)}

\[
Q_{\text{aus}} = 35000 \, \text{kJ}
\]

\[
x = 0.065
\]

\[
m_1 = 5755 \, \text{kg}
\]

\[
T_1 = 273.15 \, \text{K}
\]

\text{tabellierte gesetztes System} \( T_1 \)

\[
\dot{m} = \dot{m}_2 - \dot{m}_1
\]

\[
\dot{m}_2 = \dot{m}_1 + \dot{m}_\text{aus}
\]

\text{Siedend mit} \( T_2 = 273.15 \, \text{K} \)

\[
\frac{dE}{dt} = \dot{m}_2 u_2 - \dot{m}_1 u_1 = \dot{m} (h_\text{ein}) + \dot{Q}
\]

\[
-\dot{m} u_2 - \dot{m} h_\text{ein} = \dot{m} u_1 - \dot{m}_2 + \dot{Q}
\]

\[
\dot{m} = \frac{\dot{m}_1 u_1 - \dot{m}_2 + \dot{Q}}{u_2 - u_1}
\]

\[
= 2755.13 \, \text{kg}
\]

\text{alles ersetzen}

\[
\text{TAD 1 \& 2}
\]

\[
\left\{
\begin{aligned}
u_2 (20^\circ C) &= 83.56 \, \frac{\text{kJ}}{\text{kg}} \\
u_2 (70^\circ C) &= 293.15 \, \frac{\text{kJ}}{\text{kg}}
\end{aligned}
\right.
\]

\[
m_1 = 5755 \, \text{kg}
\]

\[
Q = 25000 \, \text{kJ}
\]

\[
h_\text{ein} (20^\circ C) = 83.56 \, \frac{\text{kJ}}{\text{kg}}
\]