\subsection*{b) Energiegleichung}

\begin{equation}
0 = \dot{m} \left( h_e - h_a - \frac{w_e^2 - w_a^2}{2} + g(z_e - z_a) \right) + \dot{Q} - \frac{V_f}{t}
\end{equation}

\begin{equation}
q_{13} = \frac{\dot{Q}_{13}}{\dot{m}_k}
\end{equation}

\begin{equation}
q_{B} = \frac{\dot{Q}_{13}}{\dot{m}_k} = q_{13}
\end{equation}

\begin{equation}
\frac{\dot{m}_m}{\dot{m}_k} = \frac{5.293}{7} = 7 \cdot \dot{m}_k = \left( \frac{5.293}{7} \right) \cdot \dot{m}_m
\end{equation}

b)

\[
T_0 : \quad p v = R T \quad \rightarrow \frac{p}{R} = \text{const} = \frac{T}{v}
\]

\[
T_0 = T_s, \quad \text{da adiabater Prozess}
\]

\[
\frac{T_1}{v_1} = \frac{T_0}{v_0}
\]