

\subsection*{d)}

\begin{equation*}
    \eta_{K} = \frac{\dot{Q}_{zu}}{\dot{W}_{t}} = \frac{[\dot{Q}_{ab} - \dot{Q}_{zu}]}{[\dot{Q}_{ab}]} = \left( \frac{\dot{Q}_K}{\dot{W}_K} \right)
\end{equation*}

\begin{equation*}
    \dot{Q}_K = \text{"Energie√ºbergang"}
\end{equation*}

\begin{equation*}
    \dot{Q}_K = \dot{m} (h_e - h_a + \frac{v_e^2 - v_a^2}{2} + g(z_e - z_a)) \dot{Q}_K - Q_e
\end{equation*}

\begin{equation*}
    \frac{dE}{dt} = \sum_i Q_i - \sum W_n
\end{equation*}

\begin{equation*}
    E = U - KE - PE \rightarrow \Delta E = \Delta U
\end{equation*}

\begin{equation*}
    \Delta V = \dot{Q}_K
\end{equation*}