\section*{1a) $\dot{Q}_{\text{aus}}$}

\[
0 = \dot{m}_{\text{ein}} \left( h_{\text{ein}} - h_{\text{aus}} \right) + \dot{Q}_R - \dot{q}_{\text{aus}}
\]

\[
\dot{Q}_{\text{aus}} = \dot{m}_{\text{ein}} \left( h_{\text{ein}} - h_{\text{aus}} \right) + \dot{Q}_R
\]

\[
h_{\text{ein}} = h_f(70^\circ C) = 292.98 \frac{\text{kJ}}{\text{kg}} \quad \text{A2}
\]

\[
h_{\text{aus}} = h_f(100^\circ C) = 419.04 \frac{\text{kJ}}{\text{kg}} \quad \text{A2}
\]

\[
\dot{Q}_{\text{aus}} = \underline{62.182 \text{ kW}}
\]