

\section*{2b)}

\begin{align*}
w_6, \, T_6 \\
T_6 &= T_5 \left( \frac{P_0}{P_5} \right)^{\frac{n-1}{n}} = \underline{328 \, K} \\
n &= 1.4 \\
0 &= \dot{m}_{\text{gas}} \left( h_5 - h_6 + \frac{w_5^2}{2} - \frac{w_6^2}{2} \right) \\
0 &= h_5 - h_6 + \frac{w_5^2}{2} - \frac{w_6^2}{2} \\
w_6 &= \sqrt{2 \cdot \left( h_5 - h_6 + \frac{w_5^2}{2} \right)} \\
w_6 &= \sqrt{2 \cdot \left( c_p (T_5 - T_6) + \frac{w_5^2}{2} \right)} = \underline{507.4 \, \frac{m}{s}}
\end{align*}

``````latex

2C)
\[
\dot{D}_{e_{x_{str}}} = e_{x_{str6}} - e_{x_{str0}}
\]

\[
\dot{e}_{x_{str}} = \dot{m} (h - h_0 - T_0 (s - s_0)) + p_0 \left( \frac{v}{\nu} V_0 \right)
\]

\[
\Delta e_{x_{str}} = \dot{m} (h_6 - h_0 - T_0 (\frac{s_6}{\nu_6} - s_0)) + p_0 \left( \frac{V_6}{\nu} - V_0 \right)
\]

\[
h_6 - h_0 = C_p (T_6 - T_0)
\]

\[
s_6 - s_0 = C_p \ln \left( \frac{T_6}{T_0} \right)
\]

\[
\Delta e_{x_{str}} = \dot{m} \left( C_p (T_6 - T_0) - T_6 \left( C_p \ln \left( \frac{T_6}{T_0} \right) \right) \right) + p_0 (V_6 - V_0)
\]

``````latex