c) \quad \dot{m}_{\text{gen}}

\[
\Delta e_{\text{xs}} = e_{\text{xs, in}} - e_{\text{xs, out}} = 
\]

\[
\Delta e_{\text{xs, in}} = h - h_0 - T_0 (s - s_0) + k.e + p.e
\]

\[
e_{\text{xs, in}} = \Delta h - T_0 \Delta s + k.e
\]

\[
= 36.91 \frac{\text{kJ}}{\text{kg}} - 243.15 \frac{\text{kJ}}{\text{kg}} \cdot 0.335 + 48.05 \frac{\text{kJ}}{\text{kg}} - 63.5 \frac{\text{kJ}}{\text{kg}}
\]

\[
\Delta h = c_p^{\text{ig}} (T_e - T_0) = 1.006 \frac{\text{kJ}}{\text{kg K}} (340 \text{K} - 243.15 \text{K})
\]

\[
= 36.91 \frac{\text{kJ}}{\text{kg}}
\]

\[
\Delta s = c_p^{\text{ig}} \ln \left( \frac{T_e}{T_0} \right) - R \ln \left( \frac{p_e}{p_0} \right)
\]

\[
= 1.006 \frac{\text{kJ}}{\text{kg K}} \ln \left( \frac{340 \text{K}}{243 \text{K}} \right) - 0.287 \ln (1) = 0.335
\]

\[
c_v^{\text{ig}} = \frac{c_p^{\text{ig}}}{k} = \frac{1.006}{1.4} = 0.719
\]

\[
R = 0.287
\]

\[
k.e = \frac{1}{2} (v_e^2 - v_0^2) = \frac{1}{2} (510 \frac{\text{m}}{\text{s}} - 200 \frac{\text{m}}{\text{s}})^2
\]

\[
= 48,050 \frac{\text{J}}{\text{kg}} = 48.05 \frac{\text{kJ}}{\text{kg}}
\]