c)
\begin{align*}
e_{x, \text{ist}} &= h_1 - h_2 - T_0 (s_1 - s_2) + \frac{\omega_2^2 - \omega_1^2}{2} \\
&= h_1 - h_2 - T_0 \left( \frac{q_2}{T_2} - \frac{q_1}{T_1} \right) + \frac{\omega_2^2 - \omega_1^2}{2}
\end{align*}

\[
T_0 = 273.15 \, K
\]

\[
q_1 - q_0 = \int_{T_0}^{T_1} c_p \, dT = c_p (T_1 - T_0)
\]

\[
q_2 - q_0 = \int_{T_0}^{T_2} c_p \, dT = c_p (T_2 - T_0)
\]

\[
q_2 - q_0 = \int_{T_0}^{T_2} \frac{c_p}{T} \, dT - R \ln \left( \frac{p_2}{p_0} \right) = 0 \degree T_2 - 0 \degree T_1 - 0
\]

\[
e_{x, \text{ist}} = 133.6 \frac{kJ}{kg}
\]

\[
\omega_2 = 50 \cdot 2.25 \frac{m}{s}
\]

\[
\omega_0 = 200 \frac{m}{s}
\]

\[
T_0 = 273.15 \, K
\]

\[
s_2 (325.07 \, K) = s_2 (T_2) + \int_{T_0}^{T_2} \frac{c_p}{T} \, dT
\]

\[
= s_2 (T_0) + \frac{c_p}{T} \, dT
\]

\[
= 2.703 \frac{kJ}{kg \cdot K}
\]

\[
s_0 = 273.15 \, K
\]

\[
s_0 (325.07 \, K) = s_0 (T_2) + \frac{c_p}{T} \, dT
\]

\[
= 2.703 \frac{kJ}{kg \cdot K}
\]

\[
= 2.654 \frac{kJ}{kg \cdot K}
\]