

\subsection*{a)}

1. HS:
\[
\frac{d\dot{E}}{dt} = \sum \dot{m}_i \left( h_i + \frac{c_i^2}{2} + g z_i \right) - \sum \dot{m}_e \left( h_e + \frac{c_e^2}{2} + g z_e \right) + \sum \dot{Q} - \sum \dot{W}_{\text{in}}
\]

\[
0 = \dot{m} (\dot{h}_{\text{ein}} - \dot{h}_{\text{aus}}) + \dot{Q}_e - \dot{Q}_{\text{aus}}
\]

\[
\Rightarrow \dot{Q}_{\text{aus}} = \dot{m} (\dot{h}_{\text{ein}} - \dot{h}_{\text{aus}}) + \dot{Q}_e
\]

\[
\dot{h}_{\text{ein}} \text{ aus TAB A-2: } \dot{h}_{\text{ein}} = 292.98 \frac{\text{kJ}}{\text{kg}}
\]

\[
\dot{h}_{\text{aus}} \text{ aus TAB A-2: } \dot{h}_{\text{aus}} = 419.04 \frac{\text{kJ}}{\text{kg}}
\]

\[
\Rightarrow \dot{Q}_{\text{aus}} = 0.3 \frac{\text{kg}}{\text{s}} \left( 292.98 - 419.04 \right) \frac{\text{kJ}}{\text{kg}} + 100 \text{kJ}
\]

\[
= 62.182 \text{kJ}
\]

a) \text{Werte:} \quad h_{\text{ein}} \text{ aus TAB A2:} \quad h_{\text{ein}} = 83.896 \frac{\text{kJ}}{\text{kg}}

\[
\Rightarrow m_{\text{ges,1}} (u_2 - u_1) + c_{\text{sm,2}} u_2 = c_{\text{sm,2}} h_{\text{ein}} + Q_R
\]

\[
\Rightarrow c_{\text{sm,2}} = \frac{m_{\text{ges,1}} (u_2 - u_1) - Q_R}{h_{\text{ein}} - u_2}
\]

\[
= \frac{3928.8}{3923.45 \text{ kg}}
\]