d) \quad t_{\text{ein},2} = t_{\text{ein},2} = 0.003^\circ C

\[
\Rightarrow \Delta E = E_2 - E_1 = Q_{12} = 1500 J
\]

\[
\Delta u_{12} = \frac{1500 J}{m} = m \cdot (u_2 - u_1) = m \cdot \left( \frac{(x_2 \cdot u_{2,\text{fest}} + (1 - x_2) \cdot u_{2,\text{flüssig}})}{(x_1 \cdot u_{1,\text{fest}} + (1 - x_1) \cdot u_{1,\text{flüssig}})} \right)
\]

\[
\Rightarrow \frac{\Delta u_{12}}{m} + (x_1 \cdot u_{1,\text{fest}} + (1 - x_1) \cdot u_{1,\text{flüssig}}) = x_2 \cdot u_{2,\text{fest}} + (1 - x_2) \cdot u_{2,\text{flüssig}}
\]

\[
\Rightarrow x_2 = \frac{\left( \frac{\Delta u_{12}}{m} + (x_1 \cdot u_{1,\text{fest}} + (1 - x_1) \cdot u_{1,\text{flüssig}}) - u_{2,\text{flüssig}} \right)}{u_{2,\text{fest}} - u_{2,\text{flüssig}}}
\]

\[
x_2 = 0.555
\]

``````latex