d)

\[
m_2 h_2 - m_1 h_1 = \Delta m_2 [h_2] + \sum_i Q_i
\]

\[
\Rightarrow \dot{m} (h_2 - h_1) - \dot{Q}_R = \Delta \dot{m}_2 h_2
\]

\[
\Delta \dot{m}_2 = \frac{\dot{m} (h_2 - h_1) - \dot{Q}_R}{h_2}
\]

\[
h_{A-2} = 2538.1 \, \frac{\text{kJ}}{\text{kg}}, \quad h_2 = 2626.8 \, \frac{\text{kJ}}{\text{kg}}, \quad U_1 = h_{A,f} + x_0 \cdot h_{fg,1}
\]

\[
= 419.04 \, \frac{\text{kJ}}{\text{kg}} + 0.005 \cdot 2257 \, \frac{\text{kJ}}{\text{kg}}
\]

\[
= 430.325 \, \frac{\text{kJ}}{\text{kg}}
\]

``````latex


\[
\Delta W_{n2} = \frac{57556_y \left( 2626.8 \frac{L^2_0}{t^2_0} - 430.325 \frac{L^2_1}{t^2_1} \right) - 35 \text{t000ts}}{2538.4 \frac{L^2_1}{t^2_1}} = 4966.59 \frac{L^2_y}{t^2_y}
\]

\begin{itemize}
    \item[2)] $\Delta S_{n2} = ?$
\end{itemize}

\[
\Delta S_{n2} = u(S_2 - S_1) \Rightarrow S_2 = 7.7553 \frac{L^3_1}{t^2_1}
\]

\[
S_n = S_f + x_b (S_f - S_t) = 1.306 \frac{L^3_k}{t^2_k} - 0.005 \left( 7.3145 - 1.3061 \right) \frac{L^3_k}{t^2_k} = 1.33214 \frac{L^3_k}{t^2_k}
\]

\[
\Rightarrow \Delta S_{n2} = \left( 57556_y + 36006_y \right) \cdot 7.7553 \frac{L^3_y}{t^2_y} - 57556_y \cdot 1.33214 \frac{L^3_y}{t^2_y} = 64658.42 \frac{L^3_y}{t^2_y}
\]

``````latex