a) $\dot{Q}_{\text{ums}} = ?$

\[
0 = \dot{m} [h_e - h_c] + \sum_i \dot{Q}_i
\]

\[
\Rightarrow \dot{m} [h_a - h_e] - \dot{Q}_i = \dot{Q}_{\text{ums}} = 0.3 \dot{m} [h_2 - h_1] - 100 \, \text{kW}
\]

\[
h_{A-2} = 2626.8 \, \frac{\text{kJ}}{\text{kg}}, \quad h_{A-2g} = 2676.4 \, \frac{\text{kJ}}{\text{kg}}, \quad h_{A,f} = 252.9 \, \frac{\text{kJ}}{\text{kg}}, \quad h_{2,f} = 419.04 \, \frac{\text{kJ}}{\text{kg}}
\]

\[
h = h_f + x (h_{fg})
\]

\[
h_1 = 304.65 \, \frac{\text{kJ}}{\text{kg}}, \quad h_2 = 436.33 \, \frac{\text{kJ}}{\text{kg}}
\]

\[
\dot{Q}_{\text{ums}} = -62.3 \, \text{kW}
\]