

\item[(c)] 
    \begin{equation*}
        0 = \dot{m} (s_{e} - s_{a}) - \frac{\dot{Q}_{\text{aus}}}{T_{KF}} + S_{\text{erz}}
    \end{equation*}
    \begin{equation*}
        S_{\text{erz}} = \dot{m} (s_{a} - s_{e}) + \frac{\dot{Q}_{\text{aus}}}{T_{KF}}
    \end{equation*}
    \begin{equation*}
        0 = \dot{m} (h_{e} - h_{a}) + \dot{Q}_{\text{aus}}
    \end{equation*}
    \begin{equation*}
        \dot{m} = \frac{\dot{Q}_{\text{aus}}}{h_{a} - h_{e}} = \frac{62,182 \, \text{kJ}}{h_{a} - h_{e}}
    \end{equation*}
\end{itemize}

``````latex