

\subsection*{c)}

\begin{equation*}
e_{x,st,s} = h_6 - h_0 - T_0 \cdot (s_6 - s_0) + ke_6 + pe_6
\end{equation*}

\begin{equation*}
e_{x,st,0} = h_s - h_0 - T_0 \cdot (s_s - s_0) + ke_s + pe_s
\end{equation*}

\begin{equation*}
\Delta e_{x,st} = h_6 - h_s - T_0 \cdot (s_6 - s_s) + ke_6 - ke_s
\end{equation*}

\begin{equation*}
= C_p \cdot (T_6 - T_0) - T_0 \cdot (C_p \cdot \ln \left( \frac{T_6}{T_0} \right) - R \cdot \ln \left( \frac{p_6}{p_0} \right)) + \frac{w_6^2}{2} - \frac{w_s^2}{2}
\end{equation*}

\begin{equation*}
= 1,006 \frac{kJ}{kgK} \cdot (328,07K - 243,15K) - 243,15K \cdot 1,006 \frac{kJ}{kgK} \cdot \ln \left( \frac{328,07K}{243,15K} \right)
\end{equation*}

\begin{equation*}
+ \frac{(50,25 \frac{m}{s})^2}{2} - \frac{(200 \frac{m}{s})^2}{2}
\end{equation*}

\begin{equation*}
= 120,808 \frac{kJ}{kg}
\end{equation*}