e) \quad m_2 s_2 - m_1 s_1 = S_m s_{ein} + \frac{Q}{T} + 1 s_{ez}

\quad s_{ez} = m_2 s_2 - m_1 s_1 - S_m s_{ein} - \frac{Q}{T}

\text{mit Zwischenergebnis} \quad m_D = 28.775 \, \text{kg}

\quad m_2 = 5755 \, \text{kg} + 3600 \, \text{kg} = 9355 \, \text{kg}

\quad m_1 = 5755 \, \text{kg}

\quad s_2 = 

\text{Tabelle A-2}

\quad s_2 = 0.954 \, \frac{\text{kJ}}{\text{kg} \cdot \text{K}} + \frac{28.775 \, \text{kg}}{9355 \, \text{kg}} \quad (7.7553 - 0.954 \, \frac{\text{kJ}}{\text{kg} \cdot \text{K}})

\quad = 0.976 \, \frac{\text{kJ}}{\text{kg} \cdot \text{K}}

\text{Tabelle A-2}

\quad s_1 = 1.306 \, \frac{\text{kJ}}{\text{kg} \cdot \text{K}} + \frac{28.775 \, \text{kg}}{5755 \, \text{kg}} \quad (7.3549 - 1.306 \, \frac{\text{kJ}}{\text{kg} \cdot \text{K}})

\quad = 1.337 \, \frac{\text{kJ}}{\text{kg} \cdot \text{K}}

\quad S_m s_{ein} = \text{Tabelle A-2}

\quad s_t(200^\circ \text{C}) = 0.2966 \, \frac{\text{kJ}}{\text{kg} \cdot \text{K}}

\quad s_{ez} = 9355 \cdot 0.976 - 5755 \cdot 1.337 - 3600 \cdot 0.2966

\quad + \frac{35000 \, \text{kJ}}{293.12 \, \text{K}} = 487.69 \, \frac{\text{kg} \cdot \text{kJ}}{\text{kg} \cdot \text{K}}
``````latex