

\section*{1a)}
\begin{equation*}
0 = \dot{m}_{ein} \left( h_1 - h_2 \right) - \dot{Q}_{aus} + Q_n
\end{equation*}
\begin{equation*}
\dot{Q}_{aus} = \dot{m}_{ein} \left( h_1 - h_2 \right) + Q_R
\end{equation*}
\begin{equation*}
= 62.18 \, \text{kW}
\end{equation*}
\begin{equation*}
h_1 = 232.58 \, \frac{\text{kJ}}{\text{kg}}
\end{equation*}
\begin{equation*}
h_2 = 479.04 \, \frac{\text{kJ}}{\text{kg}}
\end{equation*}



\section*{a)}
\begin{equation*}
\Delta E = m_{ges} \left( u_2 - u_1 \right)
\end{equation*}
\begin{equation*}
= \left( m_{ges,1} + \Delta m_x \right) u_2 - \left( m_{ges,1} \right) u_1 = \Delta m_2 \, h_{wasser@20^\circ C} + Q_{zu}^0
\end{equation*}
\begin{equation*}
h_{wasser@20^\circ C} = 83.86 \, \frac{\text{kJ}}{\text{kg}}, \quad u_2 = 292.85 \, \frac{\text{kJ}}{\text{kg}}
\end{equation*}
\begin{equation*}
u_1 = 0.395 \, u_f + 0.005 \, u_g
\end{equation*}
\begin{equation*}
h_2 = 423.30 \, \frac{\text{kJ}}{\text{kg}}
\end{equation*}

``````latex