c) \quad \Delta e_{x,str} = e_{x,str,e} - e_{x,str,0}

\[
\begin{aligned}
    \Delta e_{x,str} &= h - h_0 - T_0 (s - s_0) + \frac{c u^2}{2} \\
    &= h_6 - h_0 - T_0 (s_6 - s_0) + \frac{c u^2}{2} \\
    &= C_p (T_6 - T_0) - T_0 (s_6 - s_0) + \frac{c u^2}{2}
\end{aligned}
\]

\[
\begin{aligned}
    T_0 &= 293 \, \text{K} \\
    T_6 &= 328.07 \, \text{K}
\end{aligned}
\]

\[
s_6 - s_0 = \int_{T_1}^{T_2} \frac{C_p}{T} \, dT - R \ln \left( \frac{p_6}{p_0} \right)
\]

\[
\begin{aligned}
    \frac{p_6}{p_0} &= 1, \quad \ln(1) = 0 \\
    s_6 - s_0 &= C_p \ln \left( \frac{T_6}{T_0} \right) - R \ln \left( \frac{p_6}{p_0} \right)
\end{aligned}
\]

\[
R = C_p - C_v = C_p - \frac{C_p}{\kappa} = 0.2874
\]

\[
C_v = \frac{C_p}{\kappa}
\]

\[
\Rightarrow s_6 - s_0 = C_p \ln \left( \frac{328.07}{293} \right) - 293 \cdot 0.2874 + \frac{c u^2}{2} = 2.6974 \, \text{J/gK}
\]