

\subsection*{c)}

\[
d\hat{H} = Tds + Vdp \quad (\text{da sich } \dot{v} \text{ nicht Ã¤ndert})
\]

\[
\dot{H} = \dot{m} \int s \, ds
\]

\[
\dot{T} = \frac{\dot{Q}_{aus}}{s_{aus} - s_{ein}} = \frac{\dot{Q}_{aus}}{\dot{m} \left( s_{aus} - s_{ein} \right)} = \frac{\dot{Q}_{aus}}{\dot{m} \left( \int_{T_{ein}}^{T_{aus}} \frac{c_p}{T} \, dT \right)} = \frac{\dot{Q}_{aus}}{\dot{m} \left( c_p \ln \left( \frac{T_{aus}}{T_{ein}} \right) \right)} = \frac{T_{aus} - T_{ein}}{c_p \ln \left( \frac{T_{aus}}{T_{ein}} \right)} = 293.42
\]