a)

\[
QE = m_2 u_2 - m_1 u_1 = Q m_{12} h_{12} + Q_{\text{aus} + 2}
\]

\[
\Delta m (u_2 - u_1) = Q m_{12} h_{12} + Q_{\text{aus} + 2}
\]

\[
u_2 (x = 0, T = 70^\circ C)
\]

\[
u_2 (x = x_0)
\]

\[
u_f (100^\circ C) = 419.94 \frac{\text{kJ}}{\text{kg}} \quad \text{Tabelle A2}
\]

\[
u_g (100^\circ C) = 2506.5 \frac{\text{kJ}}{\text{kg}} \quad \text{Tabelle A2}
\]

\[
u_{m x} = u_f + x_m (u_g - u_f) = 429.3378 \frac{\text{kJ}}{\text{kg}}
\]

\[
u_2 (T = 70^\circ C)
\]

\[
\text{isochor} \quad u_1 = u_2 \quad V_1 = V_2
\]