a) 

\[
\dot{m}_w = 0.3 \, \frac{\text{kg}}{\text{s}}
\]

\[
m_{ges} = 5755 \, \text{kg}
\]

\[
0 = \dot{m}_w (h_{ein} - h_{aus}) + \dot{Q}_e + \dot{Q}_{aus} - \cancel{0}
\]

\[
\dot{Q}_{aus} = -\dot{Q}_e + \dot{m}_w (h_{aus} - h_{ein})
\]

\[
h_{ein} = h_f (70^\circ \text{C}) + 0.005 \left( h_{fg} (70^\circ \text{C}) - h_f (70^\circ \text{C}) \right) = 304.65 \, \frac{\text{kJ}}{\text{kg}}
\]

\[
h_{aus} = h_f (100^\circ \text{C}) + 0.005 \left( h_{fg} (100^\circ \text{C}) \right) = 430.825 \, \frac{\text{kJ}}{\text{kg}}
\]

\[
\Rightarrow \dot{Q}_{aus} = -62.2972 \, \frac{\text{kJ}}{\text{s}} = -62.3 \, \text{kW}
\]