

\section*{d)}

\[
\Delta E = m_2 u_2 - m_1 u_1 = \Delta m_{12} h_{12} + Q_{e,12} - \cancel{W}
\]

\[
m_2 = m_1 + \Delta m_{12}
\]

\[
u_2 = u_f (70^\circ C) = 292.95 \frac{\text{kJ}}{\text{kg}}
\]

\[
u_1 = u_f (100^\circ C) = 418.97 \frac{\text{kJ}}{\text{kg}}
\]

\[
m_1 = 5755 \text{ kg}
\]

\[
m_2 = 5755 \text{ kg} + \Delta m_{12}
\]

\[
h_{12} = 83.96 \frac{\text{kJ}}{\text{kg}}
\]

\[
\Rightarrow m_1 u_2 + \Delta m_{12} u_2 - m_1 u_1 = \Delta m_{12} h_{12} + Q_{e,12}
\]

\[
\Delta m_{12} (u_2 - h_{12}) = Q_{e,12} + m_1 u_1 - m_1 u_2
\]

\[
\Delta m_{12} \approx 3500 \text{ kg}
\]