d) \quad \text{aus} \quad \dot{Q} = \Delta m_{12} \\
T = 70^\circ C = 343.15 \, K \\
\Delta E = Q - \cancel{W} \quad \cancel{W} = 0 \\
35 \, \text{MJ} = m \left( u_2 - u_1 \right) \\
35 \, 000 \, 000 \, \text{J} = m \left( 418.5 \, \frac{\text{kJ}}{\text{kg}} - 83.55 \, \frac{\text{kJ}}{\text{kg}} \right) \\
35 \, 000 \, 000 \, \text{J} = m \left( 418.5 \, \frac{\text{kJ}}{\text{kg}} - 83.55 \, \frac{\text{kJ}}{\text{kg}} \right) \\
35 \, 000 \, 000 \, \text{J} = m \left( 418.5 \, \frac{\text{kJ}}{\text{kg}} - 83.55 \, \frac{\text{kJ}}{\text{kg}} \right) \\
35 \, 000 \, 000 \, \text{J} = m \left( 418.5 \, \frac{\text{kJ}}{\text{kg}} - 83.55 \, \frac{\text{kJ}}{\text{kg}} \right) \\
35 \, 000 \, 000 \, \text{J} = m \left( 418.5 \, \frac{\text{kJ}}{\text{kg}} - 83.55 \, \frac{\text{kJ}}{\text{kg}} \right) \\
35 \, 000 \, 000 \, \text{J} = m \left( 418.5 \, \frac{\text{kJ}}{\text{kg}} - 83.55 \, \frac{\text{kJ}}{\text{kg}} \right) \\
35 \, 000 \, 000 \, \text{J} = m \left( 418.5 \, \frac{\text{kJ}}{\text{kg}} - 83.55 \, \frac{\text{kJ}}{\text{kg}} \right) \\
35 \, 000 \, 000 \, \text{J} = m \left( 418.5 \, \frac{\text{kJ}}{\text{kg}} - 83.55 \, \frac{\text{kJ}}{\text{kg}} \right) \\
35 \, 000 \, 000 \, \text{J} = m \left( 418.5 \, \frac{\text{kJ}}{\text{kg}} - 83.55 \, \frac{\text{kJ}}{\text{kg}} \right) \\
35 \, 000 \, 000 \, \text{J} = m \left( 418.5 \, \frac{\text{kJ}}{\text{kg}} - 83.55 \, \frac{\text{kJ}}{\text{kg}} \right) \\
35 \, 000 \, 000 \, \text{J} = m \left( 418.5 \, \frac{\text{kJ}}{\text{kg}} - 83.55 \, \frac{\text{kJ}}{\text{kg}} \right) \\
35 \, 000 \, 000 \, \text{J} = m \left( 418.5 \, \frac{\text{kJ}}{\text{kg}} - 83.55 \, \frac{\text{kJ}}{\text{kg}} \right) \\
35 \, 000 \, 000 \, \text{J} = m \left( 418.5 \, \frac{\text{kJ}}{\text{kg}} - 83.55 \, \frac{\text{kJ}}{\text{kg}} \right) \\
35 \, 000 \, 000 \, \text{J} = m \left```latex