

\subsection*{b)}

\[
0 = \dot{m}(h_1) + \frac{\dot{V}^2}{2} \bigg|_{\text{isobar}}
\]

\[
0 = -\dot{m}(h_0 - h_6) + \frac{\omega_1^2}{2} - \frac{\omega_6^2}{2} \Rightarrow -\dot{m}(C_p^g(T_0 - T_6) + \frac{\omega_0^2}{2} - \frac{\omega_2^2}{2})
\]

\[
\frac{\omega_1^2}{2} - \frac{\omega_2^2}{2} = -C_p^g(T_0 - T_6)
\]

\[
\omega_1 = \sqrt{\omega_0^2 - 2C_p(T_0 - T_6)}
\]

\[
\omega_1 = 200.48 \, \text{m/s}
\]

\[
mRT = P \cdot V
\]

\[
\dot{m}RT_1 = \frac{mR T_2}{V_2} \bigg|_{\text{isobar}} \quad P_0 \frac{V_1}{T_0}
\]

\[
\frac{T_6}{T_0} = \left( \frac{P_6}{P_0} \right)^{\frac{n-1}{n}} T_0 = T_6 = 340
\]

\section*{Problem b}

\[
\frac{T_6}{T_5} = \left( \frac{p_6^0}{p_5^0} \right)^{\frac{n-1}{n}} \implies T_6 = T_5 \left( \frac{p_6^0}{p_5^0} \right)^{\frac{n-1}{n}} = 328.07 \, \text{K}
\]

\[
0 = \dot{m}(h_6) + \dot{e}_{xq}^0 - W
\]

\[
W^0 = \dot{m} \left( h_5 - h_6 + \frac{\omega_5^2}{2} - \frac{\omega_6^2}{2} \right)
\]

\[
c_p (T_5 - T_6) = \frac{\omega_6^2}{2} - \frac{\omega_5^2}{2} \implies \omega_6 = \sqrt{2 c_p (T_5 - T_6) + \frac{\omega_5^2}{2}} = 220.47 \, \frac{\text{m}}{\text{s}}
\]

\[
\text{adiabat \& reversibel : isentrop} \implies s_6 = s_5
\]

\[
0 = \int_{T_5}^{T_6} \ln \left( \frac{T_6}{T_5} \right) c_p - R \ln \left( \frac{p_6^0}{p_5^0} \right)
\]

\[
\implies T_5 = T_6
\]