d) 1. HS GS $\Delta U = Q + \dot{m} \frac{v^2}{2}$

\[
Q = \Delta U = m u_{1} - m u_{a1}
\]

\[
u_{1} \equiv u_{F1} + x (u_{F2} - u_{F1}) = -200,1168 \frac{\text{kJ}}{\text{kg}}
\]

\[
\text{L} \Rightarrow m u_{2} = m u_{1} + Q
\]

\[
= 1,200 \frac{\text{kJ}}{\text{kg}} + 0,1 \left[ \frac{\text{kg}}{\text{kg}} \cdot (-200,1168 \frac{\text{kJ}}{\text{kg}}) \right]
\]

\[
= 1,200 \frac{\text{kJ}}{\text{kg}} - 28,58 \frac{\text{kJ}}{\text{kg}}
\]

``````latex


\[
u_2 = \frac{-28.518 \, \text{kg} \cdot \frac{\text{m}}{\text{s}} - (-140.1168 \, \text{kg} \cdot \frac{\text{m}}{\text{s}})}{0.115 \, \text{kg}}
\]

\[
x_{Eis,2} = \frac{u_2 - u_{Eis,0.005^\circ C}}{u_{Eis,49.005^\circ C} - u_{Eis,0.005^\circ C}}
\]

\[
= \frac{u_2 - u_{Eis,0.005^\circ C}}{u_{Eis,49.005^\circ C} - u_{Eis,0.005^\circ C}}
\]

\[
= \frac{u_2 - u_{Eis,0.005^\circ C}}{u_{Eis,49.005^\circ C} - u_{Eis,0.005^\circ C}}
\]

\[
= \frac{u_2 - u_{Eis,0.005^\circ C}}{u_{Eis,49.005^\circ C} - u_{Eis,0.005^\circ C}}
\]

\[
= 0.1570 \quad \text{57\%}
\]

``````latex