

\subsection*{a)}
\begin{align*}
\text{SFP 1.HS} \\
0 &= \dot{m} (h_e - h_a) + \dot{Q} - \frac{\dot{m}^2}{2} \cdot 0 \\
&= \dot{m} (h_e - h_a) + \dot{Q}_R + \dot{Q}_{\text{Aus}} \\
Q_{\text{Aus}} &= \dot{m} (h_u - h_e) - \dot{Q}_R \\
h_a &= h_2 = h_f (100^\circ C) = 419.04 \frac{\text{kJ}}{\text{kg}} \quad \text{A2} \\
h_e &= h_a = h_f (70^\circ C) = 292.97 \frac{\text{kJ}}{\text{kg}} \quad \text{A2} \\
Q_{\text{Aus}} &= \dot{m} (h_2 - h_1) - 10 \text{kW} = -62.182 \text{kW} \\
\text{da } Q_{\text{Aus}} \text{ als}
\end{align*}