

\subsection*{b)}

\textit{reversible adiabatic = isentrop}

1. HS.

\[
0 = \dot{m} \left( h_e + \frac{w_{e2}}{2} - h_a - \frac{w_{a2}}{2} \right) + \sum \dot{Q} = 0
\]

\[
\Rightarrow h_e + \frac{w_{e2}}{2} = h_a + \frac{w_{a2}}{2}
\]

\textit{isentrop} \( n = 1.4 = \kappa \)

\[
\frac{T_2}{T_1} = \left( \frac{P_2}{P_1} \right)^{\frac{\kappa - 1}{\kappa}}
\]

\[
\Rightarrow T_2 = T_1 \left( \frac{P_2}{P_1} \right)^{\frac{\kappa - 1}{\kappa}}
\]

\[
T_6 = T_5 \left( \frac{P_0}{P_5} \right)^{\frac{\kappa - 1}{\kappa}} = 328.07 \, \text{K}
\]

\[
h_e - h_a = w_a \quad \Rightarrow \quad h_e - h_a + \frac{w_{e2}}{2} = \frac{w_{a2}}{2}
\]

\[
w_a = \sqrt{2 (h_e - h_a) + w_{e2}^2}
\]

\[
h_e - h_a = h_5 - h_6 = c_p^{\infty} (T_4 - T_2) = 1.005 \frac{kJ}{kgK} (431.9K - 328.07K)
\]

\[
w_a =
\]