

\section*{c)}

\[
+\Delta e_{x1, \text{str}} = h_0 - h_6 - T_0 (s_6 - s_0) + \Delta ke
\]
\[
= (h_0 - h_6 - T_c (s_6^0 - s_0)) + \frac{w_2^2 - w_6^2}{2}
\]
\[
\text{gegeben aus Aufgabe 2}
\]
\[
h_0 - h_6 = c_p (T_0 - T_6) = 1.006 \frac{\text{kJ}}{\text{kgK}} (243.15 \text{K} - 340 \text{K})
\]
\[
T_c = -30 + 273.15 = 243.15 \text{K}
\]
\[
h_0 - h_6 \approx -97.43 \frac{\text{kJ}}{\text{kg}}
\]
\[
s_0 - s_6 = 0, \text{ da adiabatic \& reversibel}
\]
\[
\Rightarrow \Delta e_{x1, \text{str}} = (h_0 - h_6 + \frac{w_2^2 - w_6^2}{2})
\]
\[
= (-97.43 \frac{\text{kJ}}{\text{kg}} + \frac{200 \frac{\text{m}^2}{\text{s}^2} - 5 \frac{\text{m}^2}{\text{s}^2}}{2})
\]
\[
= (-97.43 \frac{\text{kJ}}{\text{kg}} + \frac{200^2 \frac{\text{m}^2}{\text{s}^2} - 5 \cdot 10^2 \frac{\text{m}^2}{\text{s}^2}}{2})
\]
\[
\approx +207.48 \frac{\text{kJ}}{\text{kg}}
\]