

\subsection*{b)}

\begin{equation*}
0 = \dot{m}_{\text{el}} \left( h_2 - h_3 \right) - \dot{W}_K
\end{equation*}

\begin{equation*}
\dot{m}_{\text{el}} = \frac{\dot{W}_K}{h_2 - h_3}
\end{equation*}

\begin{equation*}
h_2 = h_f + x \left( h_g - h_f \right) = h_f + h_{fg}
\end{equation*}

\begin{equation*}
\text{TABELLE A-12: } h_3 \left( p_3 = 8 \text{ bar} \right) = 
\end{equation*}

\begin{equation*}
T_3 = ?
\end{equation*}

\begin{equation*}
\frac{h_2 \left( T = -22^\circ C \right)}{h_f}
\end{equation*}

\begin{equation*}
\text{TABELLE A-10: } h_2 \left( T_2 = -22^\circ C \right) = 21.77 + 212.32 = 234.09 \frac{\text{kJ}}{\text{kg}}
\end{equation*}

``````latex


\begin{itemize}