

\section*{d)}

\[
\sum \dot{m} \left( \frac{-T_c}{T} \dot{Q} + \sum \dot{W}_{\text{in}} - \dot{e}_{x, \text{verl}} \right)
\]
\[
\dot{e}_{x, \text{verl}} = T_0 \dot{S}_{\text{verl}}
\]
\[
\dot{S}_{\text{verl}} = -\dot{e}_{x, \text{str}} \frac{1}{T} \text{ da } 7 \frac{\text{kJ}}{\text{kg}}
\]
\[
C = -\Delta e_{x, \text{str}} + \sum \left( \frac{1 - \frac{T_c}{T}}{T} \dot{Q} \right) = \sum \frac{\dot{Q}_{\text{in}}}{T} - \dot{e}_{x, \text{verl}}
\]
\[
\dot{e}_{x, \text{verl}} = -\Delta e_{x, \text{str}}
\]
\[
= -207.48 \frac{\text{kJ}}{\text{kg}}
\]

``````latex