

\subsection*{c)}
\begin{align*}
    \Delta e_{x,str} &= e_{x,str,b} - e_{x,str,0} \\
    e_{x,str,0} &= \left[ h_0 - h_0 - T_0 (s - s_0) + \frac{v^2}{2} \right] \\
    &= c_p \left( T_6 - T_0 \right) - T_0 (s_6 - s_0) + \frac{v^2}{2} \\
    &= 1.006 \, \frac{kJ}{kg K} (340 \, K - 431.9 \, K) - 243.15 \, \frac{kJ}{kg} \left( 4.006 \, \frac{kJ}{kg K} \frac{340}{243} \right) + \frac{1}{2} \left( 510 \, \frac{m}{s} \right)^2 \\
    e_{x,str,b} &= 220 \, \frac{m}{s} \\
    &= 65.04 \, \frac{kJ}{kg}
\end{align*}

``````latex

\section*{A2}

\subsection*{c) Fortsetzung}

\begin{align*}
    e_{x, str, 0} &= \left[ c_p \cdot \dot{s}(T_0) - \dot{s}(s_0) + \dot{u} \right] \\
    e_{x, str, 0} &= -1.006 \frac{\text{kJ}}{\text{kgK}} (743.15 \text{K}) - 243.15 \frac{\text{kJ}}{\text{kg}} (0) + \frac{1}{2} \left( \frac{200 \text{m}}{\text{s}} \right)^2 \\
    e_{x, str, 0} &= -19.755 \frac{\text{kJ}}{\text{kg}} \\
    e_{x, str, 0} - e_{x, str, 0} &= 85 \frac{\text{kJ}}{\text{kg}} \\
    \Delta e_{x, str} &= 85 \frac{\text{kJ}}{\text{kg}}
\end{align*}

``````latex