

\subsection*{c)}

\begin{equation*}
    \dot{e} = \frac{\dot{E}}{\dot{m}} = \left[ h_0 - h_6 - T_0 (s_0 - s_6) + \frac{1}{2} (\omega_0^2 - \omega_6^2) \right]
\end{equation*}

\begin{equation*}
    \left[ h_0 - h_6 \right] = - \left[ h_c - h_0 \right] = \exp \left\{ T_0 - T_6 \right\} = 1.1006 \frac{J}{kg} \left[ 293.15 K - 328.07 K \right]
\end{equation*}

\begin{equation*}
    = -85.359 \frac{J}{kg} \quad \text{da } P_6 = P_0
\end{equation*}

\begin{equation*}
    s_6 - s_0 = \int_{T_1}^{T_2} \frac{c_p(T)}{T} dT - R \ln \left( \frac{P_6}{P_0} \right)
\end{equation*}

\begin{equation*}
    = \ln \left( \frac{T_0}{T_0} \right) \cdot c_p = 0.3013 \frac{J}{kgK}
\end{equation*}

\begin{equation*}
    s_0 - s_6 = - (s_6 - s_0) = -0.3013 \frac{J}{kgK}
\end{equation*}

\begin{equation*}
    \dot{e} = -85.359 \frac{J}{kg} \cdot 243 \dot{m} \left( -0.3013 \frac{J}{kgK} + \frac{1}{2} \left( (200 \frac{m}{s})^2 - (510 \frac{m}{s})^2 \right) \right)
\end{equation*}

\begin{equation*}
    = 2.167 \cdot 10^7 \frac{J}{kg}
\end{equation*}

``````latex