

\subsection*{b)}

\[
0 = \dot{m} (h_2 - h_a) + \dot{Q} - \dot{W}_k
\]

\[
0 = \dot{m} (h_2 - h_3) - \dot{W}_k
\]

\[
\frac{\dot{W}_k}{h_2 - h_3} = \dot{m}
\]

\[
h_2 = h_g \left( T_2 \text{ bei } p_{k2} \right) = 259,60 \frac{\text{kJ}}{\text{kg}}
\]

\[
h_3 = h_f \left( 8 \text{ bar} \right) = 93,42 \frac{\text{kJ}}{\text{kg}}
\]

\[
h_g (220^\circ \text{C}) = \frac{266,45 - 258,36}{261 - 20} (22 - 20) + 258,36 = 259,40 \frac{\text{kJ}}{\text{kg}}
\]

\[
p_1 = p_2
\]

\[
p_3 = 8 \text{ bar}
\]

\[
x_2 = 1
\]

\[
T_2 = T_1 - 6K = -22^\circ \text{C}
\]