b) \quad w_6, \; i_6

\text{Gleichung:}
\[
\frac{d}{dt} \left( \dot{m} \left[ h_5 + \frac{v_5^2}{2} \right] \right) = \dot{m} \left[ h_6 + \frac{v_6^2}{2} \right]
\]

\text{(ggf. Ideales Gas)}
\[
c_p \left[ T_5 + T_6 \right] = \frac{1}{2} \left[ v_5^2 - w_6^2 \right]
\]

\[
\frac{T_6}{T_5} = \left( \frac{p_6}{p_5} \right)^{\frac{n-1}{n}}
\]

\[
\Rightarrow \quad T_6 = T_5 \left( \frac{p_6}{p_5} \right)^{\frac{n-1}{n}}
\]

\[
\Rightarrow \quad T_6 = 493.15 \cdot \left( \frac{0.184}{0.5} \right)^{\frac{1.4-1}{1.4}}
\]

\[
= 328.1 \, \text{K}
\]

\[
w_6 = \sqrt{2 \, c_p \left[ T_5 - T_6 \right] + v_5^2}
\]

\[
w_6 = \sqrt{2 \cdot 1.006 \left( 493.15 - 328.1 \right) + v_5^2}
\]

\[
= 507.2 \, \frac{m}{s}
\]

``````latex

\subsection*{E_b}

\begin{equation*}
e_{k, str} = \tilde{h}_1 - h_0 - \tilde{r}_0 (s_i - s_0) tke
\end{equation*}

\begin{equation*}
= c_p (\tilde{T}_1 - \tilde{T}_0) - \tilde{r}_0 c_p \ln \left( \frac{\tilde{T}_1}{\tilde{T}_0} \right) - R \ln \left( \frac{\tilde{p}_1}{p_0} \right) + \frac{1}{2} \tilde{v}^2
\end{equation*}

``````latex