

\section*{d)}

\begin{align*}
\text{1. Hauptsatz} \, \text{an} \, \text{EV} \\
E_2 - E_1 = + Q_{12} \\
m(h_2 - h_1) = Q_{12} \\
h_2 = \frac{Q_{12}}{m} + h_1 = -7082.24 \, \frac{\text{J}}{\text{s}} \\
Q_{12} = -7082.24 \, \frac{\text{J}}{\text{s}} \\
m = 0.01 \, \text{kg} \\
h_2 = \text{Uplisting} \, f_x \, (h_{\text{res}} - h_{\text{fin}}) = -200.0928 \, \frac{\text{kJ}}{\text{kg}} \\
h_{f1} = -0.048 \, \frac{\text{kJ}}{\text{kg}} \\
h_{\text{res}} = -333.988 \, \frac{\text{kJ}}{\text{kg}}
\end{align*}

``````latex