

\section*{d)}
\begin{align*}
s_{m12} \\
m_2 u_2 - m_1 u_1 &= \Delta m_{12} (h_m) + Q_{m12} \\
m_2 &= (m_1 + \Delta m_{12})
\end{align*}

``````latex


\[
m_1 u_1 + m_2 u_2 - \Delta m_2 h_1 = Q_{aus} + t_1 m_1
\]

\[
\Delta m_2 (h_2 - h_1) = Q_{aus} + t_1 m_1 - t_1 m_2
\]

\[
\Delta m_2 = \frac{Q_{aus} + t_1 m_1 - t_1 m_2}{(h_2 - h_1)} = 3982.82 \frac{kg}{s}
\]

\[
m_1 = 5755 \, kg
\]

\[
m_2 = m_f + t_0 (m_3 - m_f) = 4373.75 \frac{kg}{s}
\]

\[
m_f = 848.15
\]

\[
m_3 = 2006.5
\]

\[
u_2 = 252.55 \frac{kg}{s}
\]

\[
h_1 = 8.96 \frac{kg}{s}
\]

\[
\text{e)}
\]

\[
\Delta s_{12}
\]

\[
\Delta s_{12} = m_{s2} - m_{s1} = 1603 \frac{kg}{s}
\]

\[
m_2 = \Delta m_2 + m_1 = 9737.82 \, kg
\]

\[
m_1 = 5755 \, kg
\]

\[
s_2 = 0.5549 \frac{kg}{sK}
\]

\[
s_1 = s_p + k(s_3 - s_t) = 1.33714 \frac{kg}{sK}
\]

\[
s_c = 1.3663 \frac{kg}{sK}
\]

\[
s_3 = 7.3585 \frac{kg}{sK}
\]

\[
k = 0.005
\]

``````latex