\subsection*{a) Energiebilanz}

\[
Q = \dot{m} [h_1 - h_2] - \dot{Q}_{\text{Aus}} + \dot{Q}_R
\]

\[
\dot{Q}_{\text{Aus}} = \dot{m} [h_1 - h_2] + \dot{Q}_R
\]

\[
h_1 = h_f \text{ at } 70^\circ \text{C} \rightarrow \text{aus A-2}
\]

\[
h_1 = 292,58 \, \text{c}^\circ
\]

\[
h_2 = h_f \text{ at } 130^\circ \text{C} \rightarrow \text{aus A-2}
\]

\[
h_2 = 419,04 \, \text{c}^\circ
\]

\[
\rightarrow \dot{Q}_{\text{Aus}} = 0.3 [292,58 - 419,04] + 100
\]

\[
\dot{Q}_{\text{Aus}} = 62,182 \, \text{kW}
\]