

\section*{d)}

\textbf{Energieblanz}
\begin{equation*}
m_2 u_2 - m_1 u_1 = \Delta m h_{\text{ein}} + \sum Q
\end{equation*}

\begin{equation*}
(1m - \Delta m) u_2 - m_1 u_1 - \Delta m h_{\text{ein}} = Q_{\text{umluft}}
\end{equation*}

\begin{equation*}
u_2 = u_4 + \cancel{u_3} \quad 70^\circ \rightarrow \text{Aus A2}
\end{equation*}

\begin{equation*}
= \cancel{u_3} \quad 252,55
\end{equation*}

\begin{equation*}
u_1 = u_4 + x (u_5 - u_4) \quad \text{at } 120^\circ \rightarrow \text{Aus A2}
\end{equation*}

\begin{equation*}
= 425,377
\end{equation*}

\begin{equation*}
h_{\text{ein}} = h_f \quad \text{at } 70^\circ = 83,58 \rightarrow \text{Aus A2}
\end{equation*}

\begin{equation*}
m_1 (u_2 - \Delta m u_2 - m_1 u_1 - \Delta m h_{\text{ein}} - Q
\end{equation*}

\begin{equation*}
- \Delta m (u_2 + h_{\text{ein}}) + m_1 u_2 - m_1 u_1 = Q
\end{equation*}

\begin{equation*}
\Delta m = \frac{Q + m_1 u_1 - m_1 u_2}{u_2 + h_{\text{ein}}} = 2.883 \, \text{J} \, 54 \, \text{kg}
\end{equation*}