

\subsection*{d)}

\begin{align*}
1.083 \, \text{kJ} & \quad \text{abgegeben} \\
m (u_2 - u_{A1}) &= Q \\
\Rightarrow u_2 &= \frac{Q}{m} + u_A = \frac{1.083 \cdot 10^3}{0.1} + (-200.093 \cdot 10^3) \\
&= -188.26 \, \frac{\text{kJ}}{\text{kg}}
\end{align*}

\begin{align*}
u_A &: \quad u_A = -0.045 \cdot 10^3 + 0.6 \left( -333.458 \cdot 10^3 - (-0.045 \cdot 10^3) \right) \\
&= -200.093 \, \frac{\text{kJ}}{\text{kg}}
\end{align*}

\begin{align*}
\Rightarrow u_2 &= u_{A1} + x \left( u_{E1} - u_{A1} \right) \\
\Rightarrow \frac{u_2 - u_{A1}}{u_{E1} - u_{A1}} &= x = \frac{-188.26 \cdot 10^3 + 0.045 \cdot 10^3}{-333.458 \cdot 10^3 + 0.045 \cdot 10^3} \\
&= 0.568 \\
&= ( = 56.8 \, \%)
\end{align*}

``````latex