

\subsection*{c)}
\begin{align*}
0 &= \dot{m} (s_e - s_a) + \frac{\dot{Q}_e}{T_e} - \frac{\dot{Q}_\text{aus}}{295 \text{K}} + \dot{s}_\text{erz} \\
\Rightarrow \dot{s}_\text{erz} &= \dot{m} (s_a - s_e) + \frac{\dot{Q}_R}{100^\circ C} + \frac{\dot{Q}_\text{aus}}{295 \text{K}} \\
                               &= 0.3 (s_a - s_e) - \frac{Q \cdot 10^3}{(100 + 273.15)} + \frac{-62.182 \cdot 10^3}{295 \text{K}}
\end{align*}

\begin{align*}
s_a - s_e: & \quad s_w @ 100^\circ C: \quad 1.30669 \cdot 10^3 \frac{\text{J}}{\text{kg K}} \\
s_e @ 70^\circ C: & \quad 0.9549 \cdot 10^3 \frac{\text{J}}{\text{kg K}}
\end{align*}

\begin{align*}
\Rightarrow &= -0.373 \frac{\text{kJ}}{\text{kg K}}
\end{align*}

``````latex