

\subsection*{a)}
\begin{align*}
0 &= \dot{m} (h_e - h_a) + \sum \dot{Q} - \sum \dot{Q}_\text{aus} \\
  &= \dot{m} (h_e - h_a) + \dot{Q}_R - \dot{Q}_\text{aus} \\
\Rightarrow \dot{Q}_\text{aus} &= \dot{m} (h_e - h_a) + \dot{Q}_R
\end{align*}

$h_e - h_a$: Weil siedende, spezifische Fl√ºssigkeit bei $70^\circ C$ und $100^\circ C$

\begin{align*}
h_e: & \quad \underline{\text{TAB A2}} \quad 70^\circ C \quad 292.98 \frac{\text{kJ}}{\text{kg}} \\
h_a: & \quad \underline{\text{TAB}} \quad 100^\circ C \quad 419.04 \frac{\text{kJ}}{\text{kg}}
\end{align*}

\begin{align*}
h_e - h_a &\Rightarrow \dot{Q}_\text{aus} = 0.3 \left( 292.98 \cdot 10^3 - 419.04 \cdot 10^3 \right) + 100 \cdot 10^3 \\
          &= -62.182 \text{ kW}
\end{align*}

(Muss negativ sein aus Sicht ohne Mantel $\Rightarrow \dot{Q}_\text{aus} = -62.182 \text{ kW}$)