

\subsection*{c)}

\begin{equation*}
\dot{m}
\end{equation*}

\begin{equation*}
\dot{E}_{x, \text{in}} = \dot{E}_{x, \text{stro}} - \dot{E}_{x, \text{stro}}
\end{equation*}

\textit{Exergieinlanz}

\begin{equation*}
\dot{E}_{x, \text{str}} = \dot{m} \left( h_2 - h_0 - T_0 (s_6 - s_0) + \frac{w_{\text{out}}^2 - w_6^2}{2} \right)
\end{equation*}

\begin{equation*}
\dot{E}_{x, \text{str}} = h_2 - h_0 - T_0 (s_6 - s_0) + \frac{w_{\text{out}}^2 - w_6^2}{2}
\end{equation*}

\begin{equation*}
= 79.9 - 243.15 (s_6 - s_0) + \frac{200^2 - 5.8^2}{2}
\end{equation*}

\begin{equation*}
= 968.56 + \frac{200^2 - 5.8^2}{2}
\end{equation*}

\begin{equation*}
s_6 - s_0 = s^0 (T_0) - s^0 (T_0) - R \ln \left( \frac{p_6}{p_0} \right)
\end{equation*}

\begin{equation*}
= c_p \ln \left( \frac{T_6}{T_0} \right) - R \ln \left( \frac{p_6}{p_0} \right)
\end{equation*}

\begin{equation*}
= 1.0889 \cdot \ln \left( \frac{314.95}{243.1} \right) = 0.362 \frac{kJ}{kgK}
\end{equation*}

\begin{equation*}
s_6 - s_0
\end{equation*}

\begin{equation*}
\frac{c_p}{c_v} = n \Rightarrow c_p = 1.4 \cdot c_v = 1.4 \cdot 0.688 = 1.4084
\end{equation*}