\subsection*{a) weiter}

\[
\dot{Q}_{\text{aus}} = \dot{m} (h_1 - h_2) + \dot{Q}_R
\]

\[
= 0.3 \left( -125.67 \frac{\text{kJ}}{\text{kg}} \right) + 100 \frac{\text{kJ}}{\text{s}} \Rightarrow \boxed{\dot{Q}_{\text{aus}} = 62.29 \frac{\text{kJ}}{\text{s}}}
\]

(a)
\]

\[
(s_2 - s_4) = s^i (T_2) - s^i (T_3) - \frac{E_{1P}}{T_P}
\]

\[
(s_2 - s_3) = s^i (T_4) - s^i (T_3)
\]

\[
\frac{1}{\overline{T}} = c \cdot \ln \left( \frac{T_2}{T_3} \right)
\]

\[
\dot{S}_{\text{EZ}} = \frac{\dot{Q}_{\text{ab}}}{T_{\text{ab}}} - \frac{T_2 - T_{\text{KL}}}{T_{\text{KL}}} = 62.29 \text{ kW} \cdot \frac{373.15 - 293.12}{373.15 \cdot 293.12} = 48.94 \frac{\text{W}}{\text{K}}
\]