

\subsection*{d)}

\[
\Delta m_{12} \left( h_{12} + \dot{Q}_{\text{aus}} \cdot \frac{1}{2} + m_{\text{out}} (h_{\text{inside}}) \right) = \Delta E = \Delta m_{12} (h_1) + \dot{Q}_{\text{aus}} \cdot \frac{1}{2} + m_{\text{out}} (h_{\text{inside}}) - m_{\text{out}} (h_{\text{inside}}) 
\]

\[
h_{\text{in}} = h (200^\circ C) + 83.96 \frac{\text{kJ}}{\text{kg}}
\]

\[
h_{\text{inside}} = 3.632 \frac{\text{kJ}}{\text{kg}} \left( \text{aus } (a), 100^\circ C \right) (\text{inkl. } x_2)
\]

\[
\Delta m_{12} = \left( -\dot{Q}_{\text{aus}} + m_{\text{out}} (h_{\text{inside}}) \right) \left( \frac{h_{\text{```latex