d)

\begin{equation*}
m_2 u_2 - m_1 u_1 = \Delta m \cdot h_{zu}
\end{equation*}

\begin{equation*}
\text{Tabelle A2} \\
u_2, u_{1f}, u_{1g} \\
h_{zu}
\end{equation*}

\begin{align*}
m_2 &= 5755 \, \text{kg} \\
u_2 &= 292.85 \, \frac{\text{kJ}}{\text{kg}} \\
m_0 &= 5755 \cdot 0.005 \, \text{kg} = 28.775 \, \text{kg} \\
u_{1g} &= 2506.5 \, \frac{\text{kJ}}{\text{kg}} \\
m_f &= 5755 \cdot (1 - 0.005) \, \text{kg} = 5726.23 \, \text{kg} \\
u_{1f} &= 418.94 \, \frac{\text{kJ}}{\text{kg}} \\
h_{zu} &= 83.96 \, \frac{\text{kJ}}{\text{kg}}
\end{align*}

\begin{equation*}
m_2 u_2 - m_0 u_{1g} - m_f u_{1f} = \Delta m \cdot h_{zu}
\end{equation*}

\begin{equation*}
\Delta m = \frac{m_2 u_2 - m_0 u_{1g} - m_f u_{1f}}{h_{zu}}
\end{equation*}

\begin{equation*}
= \frac{5755 \, \text{kg} \cdot 292.85 \, \frac{\text{kJ}}{\text{kg}} - 28.775 \, \text{kg} \cdot 2506.5 \, \frac{\text{kJ}}{\text{kg}} - 5726.23 \, \text{kg} \cdot 418.94 \, \frac{\text{kJ}}{\text{kg}}}{83.96 \, \frac{\text{kJ}}{\text{kg}}}
\end{equation*}

\begin{equation*}
= -9351.40 \, \text{kg}
\end{equation*}