d)

\begin{align*}
p_1 &= 1.4 \, \text{bar} \\
m_{\text{ev}} &= 0.1 \, \text{kg} \\
m_{\text{eis}} &= 0.06 \, \text{kg} \\
m_{\text{los}} &= 0.04 \, \text{kg}
\end{align*}

\underline{u_1}

\begin{align*}
u_1 &= u_{\text{fest}} \cdot m_{\text{fest}} + u_{\text{flüss}} \cdot m_{\text{los}} \\
&= -333.638 \, \frac{\text{kJ}}{\text{kg}} \cdot 0.06 \, \text{kg} + (-0.045 \, \frac{\text{kJ}}{\text{kg}}) \cdot 0.04 \, \text{kg} \\
&= -20.01 \, \text{kJ}
\end{align*}

\underline{u_2}

\begin{align*}
u_2 &= u_1 + \dot{Q}_{12} \\
&= -20.01 \, \text{kJ} + 1.082 \, \text{kJ} \\
&= -18.927 \, \text{kJ}
\end{align*}

\begin{align*}
u_{25} &= -18.927 \, \text{kJ} \\
&= -189.273 \, \frac{\text{kJ}}{\text{kg}}
\end{align*}

\begin{align*}
x &= \frac{u_{25} - u_{\text{eis}} + 0.003R}{u_{\text{flüssig}} + 0.003R - u_{\text{fest}}} = \frac{\text{something}}{\text{something}} = 4.32 \cdot 10^{-1}
\end{align*}

``````latex