

\subsection*{a)}
Energiebilanz am Reaktionsgemisch:
\[
\frac{d}{dt} \left( \sum_i \dot{m}_i h_i + \sum_j \dot{n}_j e_j \right) = \sum_i \dot{m}_i \dot{h}_i
\]
\[
\Rightarrow 0 = \dot{m}_{ein} h_{ein} - \dot{m}_{aus} h_{aus} + \dot{Q}_R - \dot{Q}_{aus}
\]
\[
\dot{m}_{ein} = \dot{m}_{aus}
\]
\[
\Rightarrow \dot{Q}_{aus} = \dot{m}_{ein} (h_{ein} - h_{aus}) + \dot{Q}_R
\]
\[
h_{ein} = h_C (70^\circ C) - h_{aus} = 292,88 \frac{kJ}{kg} \quad \Rightarrow \text{TAB-A2 @ 70}^\circ C
\]
\[
h_{aus} = h_E (100^\circ C) - h_{aus} = 415,04 \frac{kJ}{kg} \quad \Rightarrow \text{TAB-A2 @ 110}^\circ C
\]
\[
\Rightarrow \dot{Q}_{aus} = 62,192 \, \text{kW}
\]

\subsection*{a) Energiebilanz am Reaktionsgemisch}

\begin{align*}
\Delta E &= \Delta m_{12} \cdot (u_2 - u_1) = m_{ges,1} \cdot h_1 + \dot{Q}_R - \dot{Q}_{aus} \\
&\Rightarrow \Delta u_{m,12} = \frac{m_{ges,1} \cdot h_1 + \dot{Q}_R - \dot{Q}_{aus}}{u_2 - u_1} \quad \text{mit} \quad \dot{Q}_R = \dot{Q}_{aus}
\end{align*}

\subsubsection*{h\textsubscript{m1}:}
\begin{align*}
h_{m1} &= h_{f}(100^\circ C) + x_p \cdot \left( h_{g}(100^\circ C) - h_{f}(100^\circ C) \right) \\
&= 419,04 + 0,005 \left( 2654,1 - 419,04 \right) = 430,325 \, \text{kJ/kg}
\end{align*}

\subsubsection*{u\textsubscript{m1}:}
\begin{align*}
u_{m1} &= u_{f}(100^\circ C) + x_p \cdot \left( u_{g}(100^\circ C) - u_{f}(100^\circ C) \right) \\
&= 418,921 + 0,005 \left( 2506,5 - 418,9 \right) = 429,377 \, \text{kJ/kg}
\end{align*}

\subsubsection*{u\textsubscript{2}:}
\begin{align*}
T_2 = 70^\circ C
\end{align*}