

\item[c)] \text{ich nehme} \quad \dot{m} = 4 \frac{\text{kg}}{\text{h}} \quad \text{for safety} = \frac{4}{3600} \frac{\text{kg}}{\text{s}}
\end{itemize}

\begin{align*}
0 &= \dot{m}(h_1 - h_2) + \dot{Q}_K \\
-\frac{\dot{Q}_K}{\dot{m}} + h_2 &= h_1
\end{align*}

\begin{align*}
h_3 &= 271.3 \frac{\text{kJ}}{\text{kg}}
\end{align*}

\text{3} \rightarrow \text{4} \quad \text{ischor} \quad 2 \nu: \quad 8 \text{bar} \quad x = 0 \quad h_4 = h_f(8 \text{bar})

\begin{align*}
h_4 &= 93.42 \frac{\text{kJ}}{\text{kg}}
\end{align*}

\begin{align*}
\dot{m}(h_3 - h_4) + \dot{Q} &= 0 \\
Q &= 0.198 \text{kW}
\end{align*}

\text{Aufgrund Kreisprozess:} \quad W + \dot{E}_{\text{ab}} = 0

``````latex

4c)

\begin{align*}
-28W + (-197.6W) + \dot{Q}_c &= 0 \\
\dot{Q}_c &= 225.6W
\end{align*}

\begin{align*}
\dot{m}(h_1 - h_2) + \dot{Q} &= 0 \\
h_1 &= -\frac{\dot{Q}}{m} + h_2
\end{align*}

```