\section*{A1e)}

\[
\Delta S = (m_1 + \Delta m) S_2 - m_1 S_1
\]

\[
S_1: \quad 100^\circ C \quad x = 0.005
\]

\[
\Rightarrow A2 \quad S_1 = S_f (100) + x (S_g (100) - S_f (100)) \quad S_f (100) = 1.3064 \quad S_g (100) = 7.3543
\]

\[
\underline{S_1 = 1.33714 \, \frac{kJ}{kg \cdot K}}
\]

\[
S_2: \quad 70^\circ C \quad x = 0.005 \quad \Rightarrow A2
\]

\[
S_2 = S_f (70) + x (S_g (70) - S_f (70)) \quad S_f (70) = 0.9549 \quad S_g (70) = 7.7553
\]

\[
S_2 = 0.9888 \, \frac{kJ}{kg \cdot K}
\]

\[
\Delta S = (m_1 + \Delta m) S_2 - m_1 S_1 = \underline{1439.2 \, \frac{kJ}{K} = \Delta S}
\]

``````latex