\section*{A2) c)}

\begin{align*}
    e_{x,sito}^\# - e_{x,sito} &= h_6 - h_0 - T_0 s_6 + T_0 s_0 + ke_6 - ke_0 \\
    h_6 - h_0 &= C_p (T_6 - T_0) \\
    s_0 - s_6 &= C_p \ln \left( \frac{T_0}{T_6} \right) - R \ln \left( \frac{p_0}{p_6} \right) \\
    ke_6 - ke_0 &= \frac{1}{2} (w_6^2 - w_0^2)
\end{align*}

\begin{align*}
    s_e &= C_p (T_6 - T_0) + T_0 \left( C_p \ln \left( \frac{T_0}{T_6} \right) \right) + \frac{1}{2} (w_6^2 - w_0^2)
\end{align*}

\begin{align*}
    C_p &= 1.006 \\
    T_6 &= 328.1 \quad T_0 = 293.15 = T_4 \\
    W_6 &= 507.2 \\
    W_0 &= 200
\end{align*}

\begin{align*}
    s_{ex,tr} &= 120.8 \frac{kJ}{kg}
\end{align*}