c)

\[
Q = \dot{m} \left( S_{\text{ein}} - S_{\text{out}} \right) + \frac{\dot{Q}_{\text{aus}}}{\overline{T}_{\text{Utk}}} = m \cdot \dot{S}_{\text{ez}}
\]

\[
\dot{S}_{\text{ez}} = \dot{m} \left( S_{\text{aus}} - S_{\text{ein}} \right) + \frac{\dot{Q}_{\text{aus}}}{\overline{T}_{\text{Utk}}}
\]

\[
\dot{S}_{\text{ez}} = \dot{m} \left( S_{\text{aus}} - S_{\text{ein}} \right) + \frac{\dot{Q}_{\text{aus}}}{\overline{T}_{\text{Utk}}}
\]

\[
S_{\text{out}} = S_f (70^\circ \text{C}) = 0.85 \, \frac{\text{kJ}}{\text{kgK}}
\]

\[
S_{\text{ein}} = S_f (100^\circ \text{C}) = 1.306 \, \frac{\text{kJ}}{\text{kgK}}
\]

\[
\dot{m} = 0.3 \, \frac{\text{kg}}{\text{s}} \left( 1.306 \, \frac{\text{kJ}}{\text{kgK}} - 0.85 \, \frac{\text{kJ}}{\text{kgK}} \right) + \frac{62.182 \, \frac{\text{kJ}}{\text{s}}}{295 \, \text{K}}
\]

\[
= 0.316 \, \frac{\text{kJ}}{\text{K}}
\]

``````latex