c)

\[
R = c_{p} - c_{v}
\]

\[
R = \frac{c_{p}}{c_{v}} - \frac{c_{p}}{n}
\]

\[
= 1.006 \frac{kJ}{kg \cdot K} - \frac{1.006 \frac{kJ}{kg \cdot K}}{1.4}
\]

\[
= 722.85 \frac{kJ}{kg \cdot K}
\]

``````latex


\[
-e_{x,sirr,0} = -e_{x,sirr,0}
\]

\[
e_{x,sirr,0} = (h_2 - h_0 - T_0 (s_2 - s_0) - \Delta \text{kcl})
\]

\[
= c_{p,mix} (T_0 - T_0) - T_0 \left( c_{p,mix} \ln \left( \frac{T_0}{T_0} \right) - R \ln \left( \frac{p_0}{p_0} \right) \right) + \left( \frac{w_2^2 - w_0^2}{2} \right)
\]

\[
= c_{p,mix} (T_0 - T_0) - T_0 \left( c_{p,mix} \ln \left( \frac{T_0}{T_0} \right) - R \ln \left( \frac{p_0}{p_0} \right) \right) + \left( \frac{w_2^2 - w_0^2}{2} \right)
\]

\[
= \dot{m}_{ges} \left( 1,006 \frac{\text{kJ}}{\text{kgK}} (328,0 K - 293,15 K) - 2,493,75 \frac{\text{kJ}}{\text{kg}} \ln \left( \frac{1}{1} \right) + \frac{1,006 \frac{\text{kJ}}{\text{kgK}}}{2,493,75 \frac{\text{kJ}}{\text{kg}}} \right)
\]

\[
= -722,88 \frac{\text{kJ}}{\text{kg}} \ln \left( \frac{1}{1} \right) + \left( \frac{502,78 \frac{\text{kJ}}{\text{kg}}}{2,493,75 \frac{\text{kJ}}{\text{kg}}} \right)
\]

\[
= 120,8 \frac{\text{kJ}}{\text{kg}}
\]

\[