d)
\]

\[
0 = - (e_{x,sirr,0} - e_{x,sirr,0})
\]

\[
= - (e_{x,sirr,0} - e_{x,sirr,0}) + \left( 1 - \frac{T_0}{T} \right) \cdot \left( \frac{2,493,75 \frac{\text{kJ}}{\text{kg}}}{2,493,75 \frac{\text{kJ}}{\text{kg}}} \right)
\]

\[
= -120,8 \frac{\text{kJ}}{\text{kg}} + \left( 1 - \frac{2,493,75 \frac{\text{kJ}}{\text{kg}}}{2,493,75 \frac{\text{kJ}}{\text{kg}}} \right) \cdot 1,295 \frac{\text{kJ}}{\text{kg}}
\]

\[
= 845,38 \frac{\text{kJ}}{\text{kg}} \quad (= e_{x,verl})
\]

\[
\text{alles kein "e"}
\]

\[
= e_{x,1,0,3}
\]

``````latex