b)

\[
T_6 = T_5 \left( \frac{p_6}{p_5} \right)^{\frac{n-1}{n}}
\]

\[
= 437.9 K \left( \frac{0.1019 \cdot 10^5 \frac{N}{m^2}}{0.5 \cdot 10^5 \frac{N}{m^2}} \right)^{\frac{1.4-1}{1.4}}
\]

\[
= 328.07 K
\]

\[
0 = m \left( h_e - h_a - \frac{w_e^2 - w_a^2}{2} \right)
\]

\[
h_a - h_e = \frac{w_e^2 - w_a^2}{2} \quad (1)
\]

\[
c_{p} (T_6 - T_5) = \frac{w_0^2 - w_6^2}{2}
\]

\[
\sqrt{2 c_{p} (T_6 - T_5) + w_5^2} = w_6
\]

\[
w_6 = \sqrt{2 \cdot 1.006 \frac{kJ}{kg \cdot K} (328.07 K - 437.9 K) + (220 \frac{m}{s})^2}
\]

\[
= 507.25 \frac{m}{s}
\]