

\item[a)]
    \begin{align*}
        \dot{m} (h_e - h_a) - \dot{m} (h_{e,u} + \dot{Q} - \dot{W}) &= 0 \\
        \dot{Q} &= \dot{m} (h_e - h_a) + \dot{Q} - \dot{W} \\
        \dot{Q} &= \dot{m} (h_e - h_a) \\
        h_e &= h_e (70^\circ C) \quad \text{(Tabelle A-2)} \\
        &= 292.98 \frac{\text{kJ}}{\text{kg}} \\
        h_a &= h_a (70^\circ C) \quad \text{(Tab. A-2)} \\
        &= 419.04 \frac{\text{kJ}}{\text{kg}} \\
        \dot{Q} &= \dot{m} (h_a - h_e) \\
        &= 0.3 \frac{\text{kg}}{\text{s}} (419.04 \frac{\text{kJ}}{\text{kg}} - 292.98 \frac{\text{kJ}}{\text{kg}}) \\
        &= 37.818 \text{kW} \\
        -\dot{Q}_{\text{aus}} &= \dot{Q} - \dot{Q}_R \\
        &= 37.818 \text{kW} - 100 \text{kW} \\
        &= -62.182 \text{kW} \\
        \dot{Q}_{\text{aus}} &= 62.182 \text{kW}
    \end{align*}