c)

\[
\Delta E = \sum Q - \sum EW
\]

\[
\Delta E = Q_{12} - W_v
\]

\[
\Delta E = \Delta U = Q_{12} - W_v
\]

\[
\Delta U = m \cdot c_v (T_2 - T_1)
\]

\[
= 3.479 \, \text{g} \cdot 0.653 \, \frac{\text{kJ}}{\text{kgK}} (0 - 500 \, \text{K})
\]

\[
= -1082 \, \text{J}
\]

\[
W_v = \int_{V_1}^{V_2} p_{1,2} \, dv = p_{8,7} (V_2 - V_1)
\]

\[
V_2 = \frac{mRT_2}{p_2} = 0.0071 \, \text{m}^3 = 1.1 \, \text{L}
\]

\[
W_v = -285.6 \, \text{J}
\]

\[
\Delta U + W_v = Q_{12} = -796.4 \, \text{J}
\]

\[
Q_{12} = -796.4 \, \text{J}
\]

\[
\Delta U + W_v = Q_{12} = -1367.6 \, \text{J}
\]

\[
Q_{12} = -1367.6 \, \text{J}
\]