

\subsection*{a)}
\begin{align*}
    h_e &= h_f(T = 70^\circ C) = 292.98 \frac{kJ}{kg} \\
    h_a &= h_f(T = 100^\circ C) = 479.04 \frac{kJ}{kg} \\
    0 &= \dot{m}(h_e - h_a) + \sum \dot{Q} \\
    &= \dot{m}(h_e - h_a) + \dot{Q}_R - \dot{Q}_{\text{aus}} \\
    \dot{Q}_{\text{aus}} &= 0.3 \frac{kg}{s} (292.98 \frac{kJ}{kg} - 479.04 \frac{kJ}{kg}) + 100 kW \\
    &= \boxed{62.182 \, kW}
\end{align*}



\item[(a)] 
    \begin{align*}
        h_1 &= x_D h_g + (1 - x_D) h_f \\
        &= \boxed{930.32 \frac{kJ}{kg}}
    \end{align*}
    
    h_2 = h_f (T = 70^\circ C) = \boxed{292.49 \frac{kJ}{kg}}
    
    \text{halboffenes System}
    
    m_2 u_2 - m_1 u_1 &= \Delta m \left[ h_e - h_2 \right] + Q \\
    u_2 &= u_f (T = 20^\circ C) = \boxed{292.95 \frac{kJ}{kg}} \\
    u_1 &= x_D u_g (T = 100^\circ C) + (1 - x_D) u_f (T = 20^\circ C) \\
    &= \boxed{929.378 \frac{kJ}{kg}}
    
    (m_1 + \Delta m) u_2 - m_1 u_1 &= \Delta m h_{em} + \cancel{Q} \\
    0 &= m_1 u_2 - m_1 u_1 + Q \\
    &= \frac{h_{em} - u_2}{u_1 - u_2}
    
    h_{em} = h_f (T = 20^\circ C) = \boxed{83.96 \frac{kJ}{kg}}
    
    m_1 = \boxed{5755 kg}
    
    Q = \boxed{35000 kJ}
    
    \Delta m = \boxed{3589.37 kg}
\end{itemize}

``````latex


1.