

\subsection*{a)}

\begin{align*}
    p_{g1} &= p_{amb} + (m_k + m_{EW}) g \frac{1}{A} \\
    A &= \frac{D^2}{4} \pi = 0.00785 \, \text{m}^2 \\
    p_{g1} &= 1 \, \text{bar} + (32 \, \text{kg} + 0.76 \, \text{kg}) \cdot g \cdot \frac{1}{0.00785 \, \text{m}^2} \\
    &= 10^5 \, \text{Pa} + 40 \, 771.78 \, \text{Pa} \\
    &= \boxed{7.4 \, \text{bar}}
\end{align*}

\begin{align*}
    m_g &= \frac{p_{g1} V_1}{R T_0} m \\
    V_1 &= 3.794 \cdot 10^{-3} \, \text{m}^3 \\
    R &= \frac{\overline{R}}{50 \, \frac{g}{mol}} = \boxed{0.7663 \, \frac{\text{kJ}}{\text{kg K}}}
\end{align*}

\[
    m_g = \boxed{3.919 \, \text{g}}
\]