

\section*{3a)}
\begin{equation*}
    p_{g1} = \frac{F}{A} + p_{amb}
\end{equation*}
\begin{equation*}
    A = \pi \left( \frac{d}{2} \right)^2 = 0.00785 \, \text{m}^2
\end{equation*}
\begin{equation*}
    F = F_{G,1} + F_{G,EW} = (m_t + m_{EW}) \cdot g = (32 \, \text{kg} + 0.7 \, \text{kg}) \cdot 9.81 = 319.901
\end{equation*}
\begin{equation*}
    p_{g1} = \frac{319.901}{0.00785} + 1.013 \cdot 10^5 = 140148 \, \frac{\text{N}}{\text{m}^2}
\end{equation*}

\section*{4)}
\begin{equation*}
    p \cdot V = n \cdot R \cdot T \Rightarrow n = \frac{p \cdot V}{R \cdot T} = 3.42 \, \text{g}
\end{equation*}
\begin{equation*}
    T = 500^\circ \text{C} = 773.15 \, \text{K}
\end{equation*}
\begin{equation*}
    p = 146148 \, \text{Pa}
\end{equation*}
\begin{equation*}
    V = 0.00314 \, \text{m}^3
\end{equation*}
\begin{equation*}
    n = \frac{m}{M}
\end{equation*}
\begin{equation*}
    R = \frac{R}{M} = \frac{8.314}{50} = 0.16628 \, \frac{\text{J}}{\text{mol} \cdot \text{K}} = 0.16628 \, \frac{\text{J}}{\text{g} \cdot \text{K}}
\end{equation*}

\section*{6)}
\begin{equation*}
    T_{2g} = T_{2w} \quad \text{sonst fließt noch Wärme}
\end{equation*}
\begin{equation*}
    p_{S2} = p_{g1} \quad \text{Da Masse von } \Sigma W \text{ gleich bleibt}
\end{equation*}
\begin{equation*}
    p \cdot V = m \cdot R \cdot T
\end{equation*}
\begin{equation*}
    \Delta T_{EW} = c_{p,EW} \cdot m_{EW} \cdot \Delta T_G \cdot c_{p,G} \cdot m_G
\end{equation*}
\begin{equation*}
    c_p = R + c_V = 0.633 + 0.16628 = 0.799 \, \frac{\text{J}}{\text{g} \cdot \text{K}}
\end{equation*}
\begin{equation*}
    \Delta T_{EW} = T_{EW} \cdot T
\end{equation*}
\begin{equation*}
    \Delta T_G = T_G \cdot T
\end{equation*}
\begin{equation*}
    T \left( c_{p,EW} \cdot m_{EW} + c_{p,G} \cdot m_G \right) = T_{EW} \cdot c_{p,EW} \cdot m_{EW} - T_G \cdot c_{p,G} \cdot m_G
\end{equation*}
\begin{equation*}
    T \left( c_{p,EW} \cdot m_{EW} + c_{p,G} \cdot m_G \right) = T_{EW} \cdot c_{p,EW} \cdot m_{EW} - T_G \cdot c_{p,G} \cdot m_G
\end{```latex


\[
T_{ew} = 0^\circ C \quad \text{da sonst kein Eis übrig ist bei Gleichgewicht}
\]
\[
\text{also} \quad T_{gr} = 0^\circ C
\]

\begin{itemize}