\subsection*{a) halboffenes System}

\begin{align*}
    m(u_2 - u_1) &= \dot{m} (h_{ein} - h_{aus}) + \dot{Q}_{aus} - \dot{W} \\
    \dot{Q}_{aus} &= m(u_2 - u_1) - \dot{m} (h_{ein} - h_{aus}) \\
    \dot{Q}_{aus} &= m(u_2 - u_1) - \dot{m} (h_{ein} - h_{aus}) \quad \text{(kein $\dot{W}$, da $u_{ein} = u_{aus}$)}
\end{align*}



\subsection*{a)}
\begin{align*}
    Q_{\text{aus}} &= -\dot{m}_{\text{ein}} (h_{\text{ein}} - h_{\text{aus}}) \\
    \dot{Q}_{\text{aus}} &= 293.6 \frac{\text{kJ}}{\text{kg}} \\
    Q_{\text{aus}} &= 37.818 \text{ kW}
\end{align*}



\subsection*{a)}
1.1.1 Halboffenes System:

\[
\Delta E = m_2 u_2 - m_1 u_1 = \dot{m} \cdot (h_{\text{ein}} - h_{\text{aus}}) + Q - \dot{m} \cdot \frac{v^2}{2}
\]

\[
-Q + \dot{m} \cdot (u_{\text{innen}} - u_{\text{au√üen}}) = m \cdot u_2 = \dot{m} \cdot h_{\text{ein}} - h_{\text{aus}}
\]

\[
-Q + \dot{m} (u_2 - u_1) = \dot{m} \cdot (h_{\text{ein}} - h_{\text{aus}})
\]

\[
\dot{m} = \frac{-Q + \dot{m} (u_2 - u_1)}{h_{\text{ein}} - h_{\text{aus}}}
\]

\[
\dot{m} = \frac{-Q + \dot{m} (u_2 - u_1)}{h_{\text{ein}} - h_{\text{aus}}}
\]