

\subsection*{d)}
\[
T_2 = T_{2,1G} = 0.003^\circ C = 273.15K
\]

1. HS:

\[
\Delta E = m(u_2 - u_1) = Q_{12} - W_{v,12}
\]

\[
u_2 - u_1 = \frac{Q_{12}}{m}
\]

\[
u_2 = u_1 + \frac{Q_{12}}{m}
\]

\[
u_2 = u_1 + Q_{12} \rightarrow Q_{12} = 1500J
\]

\[
Q_{12} = -1.5u
\]

\[
u_2 \text{ kann aus Tab.1 ermittelt werden}
\]

\[
u_2 \text{ bei } 0^\circ C = -333.05 \frac{kJ}{kg}
\]

\[
u_2 \text{ bei } 0^\circ C = -0.045 \frac{kJ}{kg}
\]

``````latex

\section*{A3}

\begin{equation*}
u_1 = (1 - x_1) u_{\text{flüssig}} + x_1 u_{\text{fest}}
\end{equation*}

\begin{equation*}
u_1 = -200.0528 \frac{\text{kJ}}{\text{kg}}
\end{equation*}

\begin{equation*}
u_2 = u_1 + \frac{Q_{12}}{m_{\text{Wasser}}} \quad \rightarrow \quad Q_{12} = 1.5 \text{kJ}
\end{equation*}

\begin{equation*}
u_2 = -145.0528 \frac{\text{kJ}}{\text{kg}}
\end{equation*}

\begin{equation*}
T_{2, \text{is}} = 0.003^\circ \text{C} \quad \rightarrow \quad u_{\text{fest}} (0.003^\circ \text{C}) = -333.442 \frac{\text{kJ}}{\text{kg}}
\end{equation*}

\begin{equation*}
u_{\text{flüssig}} (0.003^\circ \text{C}) = -0.033 \frac{\text{kJ}}{\text{kg}}
\end{equation*}

\begin{equation*}
u_2 = (1 - x_2) u_{\text{flüssig}} + x_2 u_{\text{fest}}
\end{equation*}

\begin{equation*}
u_2 - u_{\text{flüssig}} = x_2 (u_{\text{fest}} - u_{\text{flüssig}})
\end{equation*}

\begin{equation*}
x_2 = \frac{u_2 - u_{\text{flüssig}}}{u_{\text{fest}} - u_{\text{flüssig}}}
\end{equation*}

\begin{equation*}
x_2 = 0.555
\end{equation*}

``````latex