\section*{2. c)}

\begin{align*}
\Delta e_{x,str} &= e_{x,str6} - e_{x,h0} \\
e_{x,str6} &= h_6 - h_0 - T_0 (s_6 - s_0) \\
e_{x,str6} - e_{x,h0} &= h_6 - h_0 - T_0 (s_6 - s_0) = \Delta \dot{e}_{x,str}
\end{align*}

\[
\frac{h_6}{h_0} = \frac{(h_6 - h_0)}{c_p (T_6 - T_0)}
\]

\[
s_6 - s_0 = c_p \ln \left( \frac{T_6}{T_0} \right) - R \ln \left( \frac{p_6}{p_0} \right) \quad \text{, } p_6 = p_0
\]

\[
\Rightarrow \Delta \dot{e}_{x,str} = c_p \left( T_6 - T_0 - T_0 \ln \left( \frac{T_6}{T_0} \right) \right)
\]

\[
= 1.006 \cdot \left( 340 \text{K} - 243.15 \text{K} - 243.15 \text{K} \cdot \ln \left( \frac{340 \text{K}}{243.15 \text{K}} \right) \right) \frac{\text{kJ}}{\text{kg K}}
\]

\[
= \underline{115.42 \frac{\text{kJ}}{\text{kg}}}
\]