

\subsection*{b)}

\begin{equation*}
\overline{T} = \frac{\int_{S_a}^{S_e} T dS}{\int_{S_a}^{S_e} dS} = T_{dS} = \text{ideale Gastheorie} \quad \Rightarrow \quad C \ln \left( \frac{T_{K, \text{aus}}}{T_{K, \text{ein}}} \right) = \text{isobar} = h_{K, \text{aus}} - h_{K, \text{ein}}
\end{equation*}

\begin{equation*}
= \frac{T_{\text{aus}} - T_{\text{ein}}}{\ln \left( \frac{T_{\text{aus}}}{T_{\text{ein}}} \right)} = \frac{298,15 \text{K} - 288,15 \text{K}}{\ln \left( \frac{298,15 \text{K}}{288,15 \text{K}} \right)} \approx 293,1 \text{K}
\end{equation*}