

\subsection*{a)}

\begin{equation*}
\begin{array}{c}
\text{1} \quad \xrightarrow{Q_{\text{ab}}} \quad \text{2} \\
T_1 = 70^\circ C \quad \quad T_2 = 100^\circ C
\end{array}
\end{equation*}

\begin{equation*}
0 = \dot{m}(h_1 - h_2) + \dot{Q}_{\text{ab}} \quad \Rightarrow \quad \dot{Q}_{\text{ab}} = \dot{m}(h_2 - h_1) = \dot{Q}_{\text{aus}} + \dot{Q}_R
\end{equation*}

\begin{equation*}
h_2 = \text{nur der fl√ºssige Anteil geht raus:}
\end{equation*}

\begin{equation*}
h_2(T = 100^\circ C) = 419,04 \frac{\text{kJ}}{\text{kg}}
\end{equation*}

\begin{equation*}
h_1:
\end{equation*}

\begin{equation*}
h_1(T = 70^\circ C) = 292,88 \frac{\text{kJ}}{\text{kg}}
\end{equation*}

\begin{equation*}
\Rightarrow \quad \dot{Q}_{\text{ab}} = \dot{m}(h_2 - h_1) \quad \Rightarrow \quad \dot{Q}_R = 0.3 \frac{\text{kg}}{\text{s}} (419,04 - 292,88) \frac{\text{kJ}}{\text{kg}} = 107,818 \text{kW}
\end{equation*}

a)

\[
\frac{dE}{dt} = + \dot{Q} \implies \Delta V_{12} = Q_{\text{aus,12}}
\]

\[
\Delta m_{12} \left( u_{2,E} U_{k4} \right) + m_{\text{ges}} \left( u_{2,\text{gas}} - u_{A,\text{gas}} \right) = -35 \text{MJ}
\]

\[
\Delta m_{12} C \left( T_2 - T_{\text{ein,12}} \right) + m_{\text{ges}} C \left( T_2 - T_{\text{Reaktor,1}} \right) = -35 \text{MJ}
\]

\[
\Delta m_{12} C \left( T_2 - T_{\text{ein,12}} \right) = -35 \text{MJ} - m_{\text{ges}} C \left( T_2 - T_{\text{Reaktor,1}} \right)
\]

\[
\Delta m_{12} = -\frac{35 \text{MJ}}{C} - \frac{m_{\text{ges}} \left( T_2 - T_{\text{Reaktor,1}} \right)}{T_2 - T_{\text{ein,12}}}
\]

\[
1 = \frac{1}{1 - 35 \text{MJ}} - \frac{m_{\text{ges}} \left( u_{2,\text{gas}} - u_{\text{gas}} \right)}{u_{2,k} - u_{k4}}
\]

\[
u_{\text{Reaktor,1}} = 418,94 \frac{\text{kJ}}{\text{kg}} + 0,005 \left( 2506,5 - 418,94 \right) \frac{\text{kJ}}{\text{kg}} = 423,38 \frac{\text{kJ}}{\text{kg}}
\]

\[
u_{K,1} = 83,55 \frac{\text{kJ}}{\text{kg}}
\]

\[
u_2 =
\]

``````latex