a) Energiebilanz:}

\begin{equation*}
\dot{m} (h_e - h_a) + \dot{Q}_R - \dot{Q}_{\text{aus}} = 0 \quad \text{station√§r}
\end{equation*}

\begin{equation*}
\dot{Q}_{\text{aus}} = \dot{m} (h_e - h_a) + \dot{Q}_R
\end{equation*}

\begin{equation*}
h_e = h_f (90^\circ C) = 232.98 \frac{\text{kJ}}{\text{kg}}
\end{equation*}

\begin{equation*}
h_a = h_f (100^\circ C) = 419.04 \frac{\text{kJ}}{\text{kg}}
\end{equation*}

\begin{equation*}
\Rightarrow \dot{Q}_{\text{aus}} = 0.3 \left( \frac{h_e - h_a}{\cancel{h_e - h_a}} \right) + 100 \text{kW} = 62.182 \text{kW}
\end{equation*}

\noindent
\text{Vorzeichen nach Skizze,}