

\subsection*{c)}

\[
e_{x,\text{sir},6} = h_6 - h_0 - T_0 (s_6 - s_0) + \text{Ke} + \text{pe}
\]

\[
h_6 = \cancel{h_6} \, (s_0, c, 1.91 \, \text{bar})
\]

\[
T_6 = 340 \, K
\]

\[
R = c_p - c_v = c_p - \frac{c_p}{k}
\]

\[
= c_p^{\text{ig}} \, (T_6 - T_0) - T_0 \left( c_p \ln \left( \frac{T_6}{T_0} \right) - R \ln \left( \frac{p_0}{p_0} \right) \right) + \text{Ke}
\]

\[
= 97.43 \, \frac{kJ}{kg} - 82.01 \, \frac{kJ}{kg} + \frac{w_6^2}{2} - \frac{w_0^2}{2} \cdot \frac{1}{\cancel{kg}}
\]

\[
= 125.47 \, \frac{kJ}{kg}
\]

\[
e_{x,\text{sir},0} = h_0 - h_0 - T_0 (s_0 - s_0) + \text{Ke} + \text{pe}
\]

\[
= \text{Ke}
\]

\[
= \frac{w_0^2}{2}
\]

\[
= 0 \, \frac{kJ}{kg}
\]

\[
\Delta e_{x,\text{sir}} = 105.47 \, \frac{kJ}{kg}
\]