

\subsection*{c)}
\begin{equation*}
    T_{G,2} = \frac{Q_{EW} + k Q_{G,1}}{m \, c_m}
\end{equation*}

\begin{equation*}
    T_{G,2} = \frac{Q_{EW,1} + k Q_{G,1}}{m \, c_m}
\end{equation*}

\begin{equation*}
    T_{G,2} = \frac{Q_{EW,2} + k Q_{G,2}}{m \, c_m}
\end{equation*}

\begin{equation*}
    T_{G,2} = \frac{Q_{EW,2} + k Q_{G,2}}{m \, c_m}
\end{equation*}

\begin{equation*}
    T_{G,2} = \frac{Q_{EW,2} + k Q_{G,2}}{m \, c_m}
\end{equation*}

\begin{equation*}
    T_{G,2} = \frac{Q_{EW,2} + k Q_{G,2}}{m \, c_m}
\end{equation*}

\begin{equation*}
    T_{G,2} = \frac{Q_{EW,2} + k Q_{G,2}}{m \, c_m}
\end{equation*}

\begin{equation*}
    T_{G,2} = \frac{Q_{EW,2} + k Q_{G,2}}{m \, c_m}
\end{equation*}

\begin{equation*}
    T_{G,2} = \frac{Q_{EW,2} + k Q_{G,2}}{m \, c_m}
\end{equation*}

\begin{equation*}
    T_{G,2} = \frac{Q_{EW,2} + k Q_{G,2}}{m \, c_m}
\end{equation*}

\begin{equation*}
    T_{G,2} = \frac{Q_{EW,2} + k Q_{G,2}}{m \, c_m}
\end{equation*}

\begin{equation*}
    T_{G,2} = \frac{Q_{EW,2} + k Q_{G,2}}{m \, c_m}
\end{equation*}

\begin{equation*}
    T_{G,2} = \frac{Q_{EW,2} + k Q_{G,2}}{m \, c_m}```latex

\begin{itemize}



\item[c)] 
    \begin{align*}
        Q_{1,2} &= m_g \cdot C_p \left( T_{g,2} - T_{g,1} \right) \\
        C_p &= k \cdot C_v = 0.80 \frac{kJ}{kg \cdot K} \\
        Q_{1,2} &= 3.6g \cdot 0.8 \frac{kJ}{kg \cdot K} \left( 0.003^\circ C - 500^\circ C \right) \\
        &= -1.44 \, kJ
    \end{align*}