

\subsection*{b)}

\begin{align*}
&\dot{Q} = \dot{m} \left( h_e - h_a + \frac{w_e^2 - w_a^2}{2} \right) \\
&\dot{Q} = 0 \\
&w_a^2 = h_e - h_a + \frac{w_e^2}{2} \\
&w_a = \sqrt{h_e - h_a + \frac{w_e^2}{2}} \\
&w_a = \sqrt{c_p (T_5 - T_6) + \frac{w_e^2}{2}} \\
&\frac{T_0}{T_5} = \left( \frac{p_0}{p_5} \right)^{\frac{n-1}{n \cdot T_5}} = \left( \frac{p_0}{p_5} \right)^{\frac{k-1}{k \cdot T_5}} = \left( \frac{0,191}{0,5} \right)^{\frac{0,4}{1,4}} \cdot 431,9 \, \text{K} \\
&= 328,07 \, \text{K} \\
&w_a = \sqrt{1,006 \frac{kJ}{kg \cdot K} (431,9 - 328,07) + \frac{220 \frac{m^2}{s^2}}{2}} = 682,79 \, \frac{m}{s}
\end{align*}

``````latex