

\section*{c)}
\[
\Delta_{ex,s}
\]
\[
0 = \dot{m} \left( h_e - h_a - T_0 (s_e - s_a) \right) + \frac{w_e^2}{2} - \frac{w_a^2}{2} = -\Delta E_{x,st}
\]
\[
T_0 = 243.15 \, K, \quad T_0 = 340 \, K
\]
\[
h_0 - h_e = cp \left( T_0 - T_e \right) = 1.006 \, \frac{kJ}{kgK} \cdot 96.85 \, K = 97.43 \, \frac{kJ}{kg}
\]
\[
s_e - s_d = cp \cdot \ln \left( \frac{T_0}{T_e} \right) - R \ln \left( \frac{p_0}{p_0} \right)
\]
\[
= cp \cdot \ln \left( \frac{T_0}{T_0} \right) = 1.006 \, \frac{kJ}{kgK} \cdot \ln \left( \frac{243.15 \, K}{240 \, K} \right) = -0.033
\]
\[
\Delta_{ex,st} = -\dot{m} \left( cp (h_0 - h_e) - T_0 \left( cp \ln \left( \frac{T_0}{T_e} \right) + \frac{w_e^2}{2} - \frac{w_a^2}{2} \right) \right)
\]