c)
\begin{align*}
e_{x,st,c} &= h_c - h_0 - T_c(s_6 - s_c) + \frac{\omega_c^2}{2} \\
e_{x,st,c} &= \cancel{h_c} - \cancel{h_0} - T_c(\cancel{s_6} - \cancel{s_c}) + \cancel{\frac{\omega_c^2}{2}} \\
\Delta e_{x,st} &= \cancel{h_c} - \cancel{h_0} - T_c(\cancel{s_6} - \cancel{s_c}) + \cancel{\frac{\omega_c^2}{2}} \\
R &= c_p - c_v \\
&= c_p - \frac{c_p}{\kappa} = 0.2874 \frac{\text{kJ}}{\text{kg K}} \\
e_{x,st,0} &= \frac{1}{2} \omega_0^2 \\
\Delta e_{x,st} &= h_6 - h_0 - T_c(s_6 - s_0) + \frac{\omega_6^2}{2} - \frac{\omega_0^2}{2} \\
&= c_{p,luft}(T_6 - T_0) - T_0 \left( c_{p,luft} \ln \left( \frac{T_6}{T_0} \right) - R \ln \left( \frac{p_6}{p_0} \right) \right) + \frac{\omega_6^2}{2} - \frac{\omega_0^2}{2} \\
&= 85.43 \frac{\text{kJ}}{\text{kg}} - 73.276 \frac{\text{kJ}}{\text{kg}} + 108.65 \frac{\text{kJ}}{\text{kg}} \\
&= 120.81 \frac{\text{kJ}}{\text{kg}}
\end{align*}