

\section*{e)}

\begin{equation*}
\Delta S = m_{\text{ges},1} + \Delta m_{12} - m_{\text{ges},1} s_1
\end{equation*}

\begin{equation*}
- \Delta \dot{m}_{12} s_1 = 1,5069 + 0,005 (7,355 \cdot 9 - 1,5069) = 1,33714 \frac{\text{kJ}}{\text{kg} \cdot \text{K}}
\end{equation*}

\begin{equation*}
s_2 = s(70^\circ C, x=1) = 7,7553
\end{equation*}

\begin{equation*}
\rightarrow \Delta S = 5755 + 3600 (7,7553) - 5755 (1,33714) = 66'230,38 \frac{\text{kJ}}{\text{kg} \cdot \text{K}}
\end{equation*}

``````latex