

\item[c)] 
    \[
    0 = \dot{m} \left( h_{\text{ein}}^{w} - h_{\text{aus}}^{w} \right) - \frac{\dot{Q}_{\text{zu}}}{T_{\text{KF}}}
    \]
    \[
    \dot{S}_{\text{zu}} = \frac{\dot{Q}_{\text{zu}}}{T_{\text{KF}}} \rightarrow \dot{S}_{\text{zu}} = \boxed{0.326 \, \frac{\text{kW}}{\text{K}}}
    \]



\subsection*{c)}

\begin{equation*}
\Delta S_{12} = \left( m_{ges} + \Delta m_{12} \right) S_2 - m_{ges} S_1 = 1237.8488 \frac{kJ}{K}
\end{equation*}

\begin{equation*}
S_2 = f \left( T \right) = 0.95249 \frac{kJ}{kgK}
\end{equation*}

\begin{equation*}
S_1 = S_f + x \left( S_g - S_f \right) = 1.23744 \frac{kJ}{kgK}
\end{equation*}