

\item[d)] 
    \[
    \Delta U = \dot{m} \left( h_{\text{ein}}^{w} - h_{\text{aus}}^{w} \right) + \dot{Q}_{\text{zu}} - \dot{Q}_{\text{aus}} = 0
    \]
    \[
    h_{\text{ein}}^{w} = h_{2} (20^\circ \text{C}) = 83.96 \, \frac{\text{kJ}}{\text{kg}} \quad \text{(A2)}
    \]
    \[
    \Delta U = \dot{m}_{\text{ges}} \left( u_{1} \left( \text{ges} + \Delta m_{12} \right) u_{2} \right)
    \]
    \[
    u_{f} = u_{f} (40^\circ \text{C}) + (u_{c} - u_{f}) = 429.3778 \, \frac{\text{kJ}}{\text{kg}}
    \]
    \[
    u_{2} = u_{f} (70^\circ \text{C}) = \boxed{292.5 \, \frac{\text{kJ}}{\text{kg}}}
    \]
\end{itemize}

``````latex


\section*{Solution}



\subsection*{d)}

\begin{equation*}
m_{ges} \left( u_1 - u_2 \right) - \Delta m_{12} u_2 = \Delta m_{12} h_{e,n}^{''}
\end{equation*}

\begin{equation*}
\Delta m_{12} = \frac{m_{ges} \left( u_1 - u_2 \right)}{h_{e,n}^{''} + u_2} = 6.408 \, T
\end{equation*}

``````latex