

\subsection*{d)}

\begin{align*}
e_k &= \frac{\dot{Q}_k}{\left| \dot{Q}_{20} \right| - \left| \dot{Q}_{k20} \right|}
\end{align*}

\begin{align*}
\Theta &= \dot{m}_2 (h_4 - h_3) - \dot{Q}_{20} \quad \Rightarrow \quad \dot{Q}_{20} = 0.1892 \, \text{kW} \\
h_4 &= 0.342 \, \frac{\text{kJ}}{\text{kg}} \\
h_3 &= h_g (8 \, \text{bar}) = 260.15 \, \frac{\text{kJ}}{\text{kg}} \\
\dot{Q}_k &= \dot{m} (h_2 - h_1)
\end{align*}

``````latex


\section*{Solution}

\begin{equation*}
Q = m_f (h_{f2} - h_{f1})
\end{equation*}

adiabat $\rightarrow h_1 = h_f \quad (8 \text{bar}) = 934.2 \frac{kJ}{kg} \quad \text{AM} \quad (AM \text{ is circled})

\begin{equation*}
h_{f1} = x_f (h_g - h_f)
\end{equation*}

\begin{equation*}
p_1 = p_2 \quad -22^\circ C = h_f \quad (-22^\circ C) = 233.08 \frac{kJ}{kg} \quad \text{(circled: AM)}
\end{equation*}

\begin{equation*}
1.2192 \frac{kg}{kg} \quad \text{(circled: 410)}
\end{equation*}

\begin{equation*}
h_f = \frac{25.77 - 9.32}{1.4 - 1.2} = \frac{(1.2192 - 1.2) + 21.32}{1.4 - 1.2} = 21.2472 \frac{kJ}{kg}
\end{equation*}

\begin{equation*}
h_g = \frac{236.04 - 233.86}{1.4 - 1.2} = \frac{(1.2192 - 1.2) + 233.86}{1.4 - 1.2} = 233.069 \frac{kJ}{kg}
\end{equation*}

\begin{equation*}
x_f = 0.358
\end{equation*}