

\section*{d)}

\[
u = u_f + x(u_s - u_f)
\]

\[
\frac{u - u_f}{u_s - u_f} = x_2
\]

\[
u_s = -333{,}442 \frac{\text{kJ}}{\text{kg}}
\]

\[
u_f = -0{,}033 \frac{\text{kJ}}{\text{kg}}
\]

\[
(Q x_1 = \Delta U \Rightarrow \Delta U = m \cdot (u_2 - u_1)) \quad (u_2 = u_1)
\]

\[
u_1 = u(0^\circ \text{C})
\]

\[
\frac{Q}{m} + u_1 = u_2
\]

\[
u_1 = u_f + x_1 (u_s - u_f)
\]

\[
u_1 = -0{,}045 + 0{,}6 \cdot (-333{,}458 + 0{,}045)
\]

\[
u_1 = -200{,}0828 \frac{\text{kJ}}{\text{kg}}
\]

\[
\frac{1{,}5 \text{kJ}}{0{,}1 \text{kg}} - 200{,}0828 \frac{\text{kJ}}{\text{kg}}
\]

\[
= -185{,}0828 \frac{\text{kJ}}{\text{kg}}
\]

\[
x_2 = \frac{-185{,}0828 \frac{\text{kJ}}{\text{kg}} + 0{,}033 \frac{\text{kJ}}{\text{kg}}}{-333{,}442 \frac{\text{kJ}}{\text{kg}} + 0{,}033 \frac{\text{kJ}}{\text{kg}}} = 0{,}555
\]

``````latex