d)

\begin{align*}
\varphi &= \varphi_f + x_2 (\varphi_g - \varphi_f) \\
u_2 &= u_{2f} + x_2 (u_{2g} - u_{2f}) \\
\end{align*}

\[
\Theta_2 = \Theta_{EW}
\]

\[
T_{EW2} = 0,0^\circ
\]

\[
x_2 = \frac{u_2 - u_{2f}}{u_{2g} - u_{2f}}
\]

\[
x_2 = \frac{-3047,093 - (-0,045)}{-333,458 - (-0,045)}
\]

\[
x_2 = 0,913
\]

\[
u_2
\]

\[
T_{EW2}
\]

\[
T_{EW2} = 0^\circ
\]

\[
u_g = u_{\text{fest.}}
\]

\[
m_{ew}(u_2 - u_1) = Q_{12}
\]

\[
u_1 = u_{1f} + x_1 (u_{1g} - u_{1f})
\]

\[
= -0,045 + 0,6 (-333,458 - (-0,045))
\]

\[
= -200,093
\]

\[
u_2 = \frac{Q_{12}}{m_{ew}} + u_1 = \frac{-2847}{0,1} + (-200,093)
\]

\[
= -3047,093 \frac{kJ}{kg}
\]

``````latex