\section*{d) Energiebilanz halboffenes System:}

\[
\Delta E = m_2 \cdot u_2 - m_1 \cdot u_1 = \Delta m_{12} \cdot h_{12} + \cancel{Q_{R12}} - \cancel{Q_{aus}} - \cancel{W}
\]

\[
m_2 = m_{\text{ges},1} + \Delta m_{12} \quad \text{und} \quad m_1 = m_{\text{ges},1}
\]

\[
\text{TAB A2:} \quad u_2 = u_f (70^\circ \text{C}) = 292.95 \, \frac{\text{kJ}}{\text{kg}}
\]

\[
u_f (100^\circ \text{C}) = 418.94 \, \frac{\text{kJ}}{\text{kg}} \quad \text{und} \quad u_g (100^\circ \text{C}) = 2506.5 \, \frac{\text{kJ}}{\text{kg}}
\]

\[
h_{12} = h_f (20^\circ \text{C}) = 83.96 \, \frac{\text{kJ}}{\text{kg}}
\]

\[
u_1 = u_f + x_0 (u_g - u_f) = 429.36 \, \frac{\text{kJ}}{\text{kg}}
\]

\[
\Rightarrow (m_1 + \Delta m_{12}) \cdot u_2 - m_1 \cdot u_1 = \Delta m_{12} \cdot h_{12}
\]

\[
\Delta m_{12} \cdot (u_2 - h_{12}) = m_1 u_1 - m_1 u_2
\]

\[
\Delta m_{12} = \frac{m_1 u_1 - m_1 u_2}{u_2 - h_{12}}
\]

\[
\Delta m_{12} = 3756.43 \, \text{kg}
\]