

\section*{e)}

\[
\Delta S = m_2 s_2 - m_1 s_1
\]

\[
= (m_1 + \Delta m_{12}) \cdot s_2 - m_1 \cdot s_1
\]

\[
\Delta S_{12} = 1387.22 \, \frac{\text{kJ}}{\text{K}}
\]

\[
\text{TAB A2:}
\]

\[
s_2 = s_f (70^\circ \text{C}) = 0.9549 \, \frac{\text{kJ}}{\text{kg} \cdot \text{K}}
\]

\[
s_1 = s_f (100^\circ \text{C}) + x_0 (s_g (100^\circ \text{C}) - s_f (100^\circ \text{C}))
\]

\[
s_f (100^\circ \text{C}) = 1.306 \, \frac{\text{kJ}}{\text{kg} \cdot \text{K}} \quad \text{und} \quad s_g (100^\circ \text{C}) = 7.3549 \, \frac{\text{kJ}}{\text{kg} \cdot \text{K}}
\]

\[
s_1 = 1.33714 \, \frac{\text{kJ}}{\text{kg} \cdot \text{K}}
\]

``````latex