d)

\[
\Delta U_{12} = Q_{12}
\]

\[
m_{EW} (U_2 - U_1) = Q_{12}
\]

\[
\begin{array}{c}
\text{TAB-1 (Prüfung):} \\
U_{1, flüssig} = -0,045 \frac{kJ}{kg} \quad U_{1, fest} = -333,758 \frac{kJ}{kg}
\end{array}
\]

\[
U_1 = U_{1, flüssig} + 0,6 \left( U_{1, fest} - U_{1, flüssig} \right) = -200,1 \frac{kJ}{kg}
\]

\[
U_2 = \frac{Q_{12}}{m_{EW}} + U_1 = -188,7 \frac{kJ}{kg}
\]

\[
p_2 = \frac{m \cdot k}{\left( \frac{d}{2} \right)^2} = 2,256 \text{ bar}
\]

\[
\begin{array}{c}
\text{TAB:} \\
U_{2, fest} (2 \text{ bar}) = -333,495 \frac{kJ}{kg} \quad U_{2, fest} (10 \text{ bar}) = -333,812 \frac{kJ}{kg}
\end{array}
\]

\[
U_{2, fest} (2,256 \text{ bar}) = U_{2, fest} (2 \text{ bar}) + \frac{2,256 \text{ bar} - 2 \text{ bar}}{10 \text{ bar} - 2 \text{ bar}} \left( U_{2, fest} (10 \text{ bar}) - U_{2, fest} (2 \text{ bar}) \right)
\]

\[
= -333,51 \frac{kJ}{kg}
\]

\[
\begin{array}{c}
\text{TAB:} \\
U_{2, flüssig} (2 \text{ bar}) = -0,07 \frac{kJ}{kg} \quad U_{2, flüssig} (10 \text{ bar}) = -0,332 \frac{kJ}{kg}
\end{array}
\]

\[
U_{2, flüssig} (2,256 \text{ bar}) = U_{2, flüssig} (2 \text{ bar}) + \frac{2,256 \text{ bar} - 2 \text{ bar}}{10 \text{ bar} - 2 \text{ bar}} \left( U_{2, flüssig} (10 \text{ bar}) - U_{2, flüssig} (2 \text{ bar}) \right)
\]

``````latex


\section*{Aufgabe 3}

d)

\[
u_{\text{flüssig}} (2,25 \text{ bar}) = -0{,}0871 \frac{\text{kJ}}{\text{kg}}
\]

\[
x = \frac{u_2 - u_{\text{flüssig}}}{u_{\text{fest}} - u_{\text{flüssig}}} = 0{,}566
\]

``````latex