

\section*{c)}

\subsection*{TAD-411:}

\begin{equation*}
h_f = h_f (8 \text{ bar}) = 93,42 \frac{kJ}{kg}
\end{equation*}

\begin{equation*}
h_f = h_1 = 93,42 \frac{kJ}{kg}
\end{equation*}

\begin{equation*}
T_{4} = 37,33^\circ C = T_{1}
\end{equation*}

\begin{equation*}
h_{1,f} (T_1) = h_f (30^\circ C) + \frac{37,33 - 30}{32 - 30} (h_{f} [32^\circ C] - h_f [30^\circ C]) =
\end{equation*}

\begin{equation*}
h_{1,g} (T_1) = h_g (30^\circ C) + \frac{37,33 - 30}{32 - 30} (h_{g} [32^\circ C] - h_g [30^\circ C]) =
\end{equation*}

\subsection*{TAB-A10:}

\begin{equation*}
h_f (30^\circ C) = 91,43
\end{equation*}

\begin{equation*}
h_f (32^\circ C) = 94,39
\end{equation*}

```