

\subsection*{b)}

\begin{align*}
    T_2 &= T_i - 6K = 257.15K = -16^\circ C \\
    \text{TAB - 10:} \\
    h_{2} &= h_{fg}(T_2) = 238.74 \frac{kJ}{kg} \\
    s_{2} &= s_{g}(T_2) = 0.9298 \frac{kJ}{kgK} = s_{3} \\
    h_{3} &= h_{8bar, s_3} = h_{f}(8bar, 0.9066 \frac{kJ}{kgK}) + \frac{s_3 - 0.9066 \frac{kJ}{kgK}}{0.9374 - 0.9066 \frac{kJ}{kgK}} \left( h_{fg}(8bar, 0.9374 \frac{kJ}{kgK}) \right) \\
    h_{f}(8bar, 0.9066 \frac{kJ}{kgK}) &= 271.31 \frac{kJ}{kg} \\
    \text{TAB - A 12:} \\
    h_{fg}(8bar, 0.9066 \frac{kJ}{kgK}) &= 284.15 \frac{kJ}{kg} \\
    h_{fg}(8bar, 0.9374 \frac{kJ}{kgK}) &= 273.66 \frac{kJ}{kg}
\end{align*}

``````latex


\section*{Energiebilanz Kompressor}

\begin{equation*}
\frac{dE}{dt} = \sum \dot{m}_i \left( h_i + \frac{v^2}{2} + g z \right) + \sum \dot{Q}_j - \sum \dot{W}_n
\end{equation*}

adiabat

\begin{equation*}
0 = \dot{m} (h_2 - h_3) - \dot{W}_{23}
\end{equation*}

\begin{equation*}
\dot{W}_{23} = -\dot{W}_K
\end{equation*}

\begin{equation*}
\dot{m} = \frac{-\dot{W}_K}{h_2 - h_3} = 2,89 \frac{kg}{h}
\end{equation*}