\section*{c) Exergie einer Str√∂mung}

\[
\dot{E}_{x,st} = \dot{m} \left[ h - h_0 - T_0 (s - s_0) + \frac{ke}{2} + \frac{pe}{2} \right]
\]

\subsection*{Zustand 0:}
\[
\dot{E}_{x,0} = \dot{m} g \left[ h_0 - h_0 - T_0 (s_0 - s_0) + ke \right]
\]
\[
= \dot{m} g \left[ ke \right] = \dot{m} g e_0
\]
\[
e_{x,0} = \frac{w_0^2}{2} = 20000 \frac{m^2}{s^2}
\]

\subsection*{Zustand 6:}
\[
\dot{E}_{x,6} = \dot{m} \left[ h_6 - h_0 - T_0 (s_6 - s_0) + \frac{w_6^2}{2} \right]
\]
\[
h_6 - h_0 = c_p (T_6 - T_0) = 97,431 \frac{kJ}{kg}
\]
\[
s_6 - s_0 = c_p \ln \left( \frac{T_6}{T_0} \right) - R \ln \left( \frac{p_6}{p_0} \right)
\]
\[
R_L = \frac{R}{M} = \frac{R}{28,97 \frac{kJ}{kmol \cdot K}} = 0,287 \frac{kJ}{kg \cdot K}
\]
\[
e_{x,6} = 97,431 \frac{kJ}{kg} - R \left( \frac{p_6}{p_0} \right)
\]
\[
s_6 - s_0 = \int_{T_0}^{T_6} \frac{c_p}{T} dT = \left[ c_p \ln (T) \right]_{T_0}^{T_6} = c_p \left( \ln (T_6) - \ln (T_0) \right)
\]
\[
s_6 - s_0 = 0,337 \frac{kJ}{kg \cdot K}
\]
\[
e_{x,6} = 97,431 \frac{kJ}{kg} - 243,15 K \cdot 0,337 \frac{kJ}{kg \cdot K} + \frac{510 \frac{m^2}{s^2}}{2}
\]
\[
= 130065,5 \frac{kJ}{kg}
\]

``````latex


\section*{Problem 2}



\subsection*{c)}

\[
\Delta e_x = e_{x6} - e_{x0} = 110065.5 \frac{\text{kJ}}{\text{kg}}
\]