d)

\[
m_{\text{gas}} (u_{2,\text{eis}} - u_{1,\text{gas}}) = -Q
\]

\[
u_{1,\text{gas}} = u_{\text{flüssig}} (1 \text{ bar}) + x_{\text{eis}} (u_{\text{fest}} (1 \text{ bar}) - u_{\text{flüssig}} (1 \text{ bar}))
\]

\[
u_{\text{flüssig}} (1 \text{ bar}) = -0.045 \frac{\text{kJ}}{\text{kg}}
\]

\[
u_{\text{fest}} (1 \text{ bar}) = 333.458 \frac{\text{kJ}}{\text{kg}}
\]

\[
u_1 = -200.0928 \frac{\text{kJ}}{\text{kg}}
\]

\[
m_{\text{gas}} \cdot u_{2,\text{eis}} = Q \cdot m_{\text{gas}} = -18.875 \text{ kJ}
\]

\[
u_{2,\text{eis}} = -18.875 \frac{\text{kJ}}{\text{kg}}
\]

\[
x_{2,\text{eis}} = \frac{u_{2,\text{eis}} - u_{\text{flüssig}} (1 \text{ bar})}{u_{\text{fest}} (1 \text{ bar}) - u_{\text{flüssig}} (1 \text{ bar})} = 0.566
\]

``````latex