e)
\begin{align*}
s_1 &= s_1 \left( x = 0,005, 100^\circ \text{C} \right) = s_f (100^\circ \text{C}) + x \left( s_g (100^\circ \text{C}) - s_f (100^\circ \text{C}) \right) \\
&\quad \boxed{\text{TAB A-2}} \quad A1 = 1,33714 \, \frac{\text{kg}}{\text{kg} \cdot \text{K}} \\
s_2 &= s_2 \left( x = 0,70^\circ \text{C} \right) = 0,9548 \, \frac{\text{kg}}{\text{kg} \cdot \text{K}} \\
\Delta s_{12} &= m_2 s_2 - m_1' s_1 \\
&= (\Delta m_{12} + m_1) \cdot s_2 - m_1' s_1 = 13947,198 \, \frac{\text{kg}}{\text{K}}
\end{align*}

``````latex