\section*{Problem c)}

\begin{align*}
    \omega_6 &= 510 \frac{\text{m}}{\text{s}}
\end{align*}

\text{Given:}

\begin{align*}
    \Delta e_{x,st} &= e_{x,st,6} - e_{x,st,0} \\
    &= h_6 - h_0 - T_0 (s_6 - s_0) + \Delta k e
\end{align*}

\begin{align*}
    h_0 (T = 280 \text{K}) &= 240.02 \frac{\text{kJ}}{\text{kg}} + \left( 50.05 - 240.2 \frac{\text{kJ}}{\text{kg}} \right) \left( \frac{250 - 280 \text{K}}{243.15 - 240.2 \frac{\text{kJ}}{\text{kg}}} \right) \\
    &= 242.906 \frac{\text{kJ}}{\text{kg}}
\end{align*}

\begin{align*}
    h_6 (T = 328.162 \text{K}) &= 325.31 \frac{\text{kJ}}{\text{kg}} + \left( \frac{330.34 - 325.31 \frac{\text{kJ}}{\text{kg}}}{330 - 325 \text{K}} \right) (328.62 - 325 \text{K}) \\
    &= 328.957 \frac{\text{kJ}}{\text{kg}}
\end{align*}

``````latex


\[
\Delta_{ex,st} = \dot{m} \left( h_0 - h - T_0 \left( s^0(T_6) - s^0(T_0) \right) + \frac{1}{2} \left( w_0^2 - w^2 \right) \right)
\]

\[
s_6 - s_0 = s^0(T_6) - s^0(T_0)
\]

\[
s^0(T_6) = 2.106977 \frac{\text{kJ}}{\text{kg K}}
\]

\[
s^0(T_0) = 1.47814 + \frac{1.51917 - 1.17824}{250 - 240} (243.15 - 240)
\]

\[
= 1.4911 \frac{\text{kJ}}{\text{kg K}}
\]

\[
T_{A,B} = A - 22
\]

\[
\Delta_{ex,st} = 109.995 \frac{\text{kJ}}{\text{kg}}
\]

\[
\dot{E}_{x,vel} = T_0 \cdot \frac{\dot{S}_{ex}}{\dot{m}}
\]

\[
\dot{S}_{ex} = s_6 - s_0 + \frac{\dot{Q}}{\dot{m} T_0}
\]

\[
= s^0_6 - s^0_0 = 0.157867 \frac{\text{kJ}}{\text{kg K}}
\]

\[
\dot{E}_{x,vel} = 1 + (0.1704) \frac{\text{kJ}}{\text{kg}}
\]

``````latex