b) 

\[
\frac{\dot{T}_f}{\dot{T}_f} = \frac{T_2 - T_A}{S_2 - S_1} = \frac{T_{\text{aus}} - T_{\text{ein}}}{S_2 - S_1} = 8,5227^\circ C
\]

\[
S_{\text{aus}} = S_2 (x = 0, 100^\circ C) = S_f = 1,3069 \frac{\text{kJ}}{\text{kg} \cdot \text{K}}
\]

\[
S_{\text{ein}} = S_1 (x = 0, 70^\circ C) = S_f = 0,9549 \frac{\text{kJ}}{\text{kg} \cdot \text{K}}
\]

b)

\[
T_{KF} = \frac{T_{KF, \text{aus}} - T_{KF, \text{ein}}}{S_{\text{aus}} - S_{\text{ein}}} = \frac{T_{KF, \text{aus}} - T_{KF, \text{ein}}}{\ln \left( \frac{T_2}{T_1} \right)}
\]

\[
S_{\text{aus}} - S_{\text{ein}} = \ln \left( \frac{T_2}{T_1} \right) = 293.12 \, K
\]

``````latex