

\section*{1d)}

\begin{align*}
\text{Zustand 1:} & \quad 100^\circ C \\
\text{Zustand 2:} & \quad 70^\circ C \quad \Rightarrow \quad 0 \text{MJ} + Q_{\text{rein}} = Q_{\text{aus}} + W
\end{align*}

\begin{align*}
Q_{\text{zu}} &= 2 \text{MJ} \\
Q_{\text{aus}} &= 35 \text{MJ}
\end{align*}

\text{Energiegleichung:}
\begin{align*}
Q_{\text{zu}} &= Q_{\text{zu}} + Q_{\text{rein}} + Q_{\text{aus}} - Q_{\text{aus}} + W
\end{align*}

\begin{align*}
\Delta U &= m_2 u_2 - m_1 u_1 \\
Q_{\text{zu}} &= m_2 - m_1
\end{align*}

\begin{align*}
u_2 &= u_f(70^\circ C) = 202,95 \frac{\text{kJ}}{\text{kg}} \\
u_1 &= u_f(100^\circ C, 0,005) = u_f(100^\circ C) + 0,005 (u_g(100^\circ C) - u_f(100^\circ C)) = 423,4 \frac{\text{kJ}}{\text{kg}}
\end{align*}

\begin{align*}
h_{\text{ein}} &= h_f(70^\circ C) = 83,06 \frac{\text{kJ}}{\text{kg}}
\end{align*}

\begin{align*}
m_1 &= 5755 \text{kg}
\end{align*}

\begin{align*}
\Rightarrow m_2 &= m_1 + Q_{\text{zu}} \\
\Rightarrow (m_1 + Q_{\text{zu}}) u_2 - m_1 u_1 &= Q_{\text{zu}} m_{\text{ein}} \\
\Rightarrow m_1 (u_2 - u_1) &= Q_{\text{zu}} (m_{\text{ein}} - u_1) \\
\Rightarrow Q_{\text{zu}} &= \frac{m_1 (u_2 - u_1)}{m_{\text{ein}} - u_2} = 3757,45 \text{kg}
\end{align*}