b)

\[
0 = \dot{m} (h_5 - h_6 + \frac{v_5^2 - v_6^2}{2}) + \dot{Q} - \dot{V}_0
\]

\[
\dot{V}_0 = \frac{R}{M} (\dot{T}_6 - \dot{T}_5) = \frac{R}{M} \frac{(\dot{T}_6 - \dot{T}_5)}{7 - n}
\]

\[
\dot{V}_0 = \frac{R}{M} \frac{(\dot{T}_6 - \dot{T}_5)}{7 - n} = \frac{2 \dot{q} (273.15 - 30 + 4.5741)}{7 - 7.4} = (47.875 \frac{\dot{q}}{s})
\]

\[
\dot{Q} = \dot{m} \frac{R}{M} = 8.314 \frac{J}{mol \cdot K} \cdot 2000 \frac{mol}{s} = 2 \dot{q}
\]

\[
\dot{V}_0 = \dot{m} (h_1 - h_0) = \dot{m} (\frac{v_1^2 - v_0^2}{2})
\]

\[
V_0 = \sqrt{v_2^2 + 2 (\dot{V}_0 - \dot{m} (h_5 - h_6))}
\]

\[
h_5 - h_6 = c_p (T_5 - T_6)
\]