\section*{Problem c}

\begin{align*}
e_{x,st6} &= e_{x,st4} - \left( h_6 - h_0 - T_0 (s_6 - s_0) + \frac{\omega_6^2}{2} \right) - \left( h_5 - h_0 - T_0 (s_5 - s_0) + \frac{\omega_5^2}{2} \right) \\
&= \left( h_6 - h_5 \right) - T_0 (s_6 - s_5) + \frac{\omega_6^2 - \omega_5^2}{2} \\
&= \int c_p dT - T_0 \left( \int \frac{c_p}{T} dT - \ln \left( \frac{P_6}{P_5} \right) \right) + \frac{\omega_6^2 - \omega_5^2}{2}
\end{align*}

\begin{align*}
R &= c_p - c_v = \frac{c_p}{c_p - c_v} = 0.28742 \frac{\text{kJ}}{\text{kg K}} \\
T_0 &= 293.15 \text{ K}
\end{align*}

\begin{align*}
\Delta e_{x,st4} &= c_p \left( T_6 - T_5 \right) - T_0 c_p \ln \left( \frac{T_6}{T_5} \right) - T_0 \ln \left( \frac{P_6}{P_5} \right) + \frac{\omega_6^2 - \omega_5^2}{2} \\
&= -109.95 - 67.26 - 67.255 + 1 + 74.437 \\
&= -167.97 \frac{\text{kJ}}{\text{kg}}
\end{align*}