\subsection*{a) stationär}

\[
0 = \dot{m} (h_{\text{ein}} - h_{\text{aus}}) + \dot{Q}_K + \dot{Q}_{\text{aus}}
\]

\[
\Rightarrow \dot{Q}_{\text{aus}} = \dot{m} (h_{\text{aus}} - h_{\text{ein}}) - \dot{Q}_K
\]

\text{Tab A2:} 
\[
h_{\text{ein}} = h_f (70^\circ C) = 292,38 \frac{\text{kJ}}{\text{kg}}
\]
\[
h_{\text{aus}} = h_f (100^\circ C) = 419,04 \frac{\text{kJ}}{\text{kg}}
\]

\[
\Rightarrow \dot{Q}_{\text{aus}} = 37,384 \text{ kW} - 100 \text{ kW} = -62,182 \text{ kW}
\]
\text{(mit } \dot{Q}_K \text{ = norm wärme austausch)}