d) 
\begin{align*}
0 &= \Delta e_{ex,str} + \sum \left( 1 - \frac{T_c}{T_0} \right) \dot{m} \left( \frac{e_{ex,in}}{\dot{m}} - \frac{e_{ex,out}}{\dot{m}} \right) - \dot{W}_{t,in} - \dot{e}_{x,vol} \\
-e_{ex,vol} &= \Delta e_{ex,str} - \dot{W}_{t,in} \\
e_{x,vol} &= T_0 \dot{S}_{ex} = T_0 \left( s_{e2} - s_{a} \right) = T_0 \left( s_{a} - s_{e} \right) = T_0 \left( s_{e2} - s_{a} \right) \\
&= T_0 \left( cp \ln \left( \frac{T_e}{T_0} \right) - R \ln \left( \frac{p_0}{p_c} \right) \right) = 15'471.75 \frac{J}{kg} = 15.622 \frac{kJ}{kg}
\end{align*}

``````latex