\subsection*{a) 1. HS um Reaktor ohne KÃ¼hlmantel}

\begin{align*}
\dot{m} (h_{\text{ein}} - h_{\text{aus}}) + \dot{Q}_R - \dot{Q}_{\text{aus}} &= 0 \\
\dot{Q}_{\text{aus}} &= \dot{m} (h_{\text{ein}} - h_{\text{aus}}) + \dot{Q}_R
\end{align*}

\begin{align*}
h_{\text{ein}} &= h(70^\circ C, x = \infty) = 292{,}98 \frac{\text{kJ}}{\text{kg}} \quad \text{(Tab A-2)} \\
h_{\text{aus}} &= h(100^\circ C, x = 0) = 419{,}04 \frac{\text{kJ}}{\text{kg}} \quad \text{(Tab A-2)}
\end{align*}

\[
\Rightarrow \dot{Q}_{\text{aus}} = 62{,}182 \, \text{RW}
\]