

\subsection*{a)}

\[
\text{Energiebilanz:} \quad \dot{m} (\hat{h}_{ein} - \hat{h}_{aus}) + \dot{Q} = \dot{Q}_{aus} = 0
\]

\[
\dot{Q}_{aus} = \dot{Q} + \dot{m} (\hat{h}_{ein} - \hat{h}_{aus})
\]

\[
\hat{h}_{ein} = 209.95 \, \frac{\text{kJ}}{\text{kg}} \quad \text{(TAB A-2)}
\]

\[
\hat{h}_{aus} = 419.04 \, \frac{\text{kJ}}{\text{kg}} \quad \text{(TAB A-2)}
\]

\[
\dot{Q}_{aus} = 100 \, \text{kW} + 0.2 \, \frac{\text{kg}}{\text{s}} (209.95 - 419.04) \, \frac{\text{kJ}}{\text{kg}} = 62.193 \, \text{kW}
\]