

\subsection*{d)}

\[
u_2 = u_2^e + x_D (u_2^g - u_2^e) = 429.38 \, \frac{\text{kJ}}{\text{kg}}
\]

\[
u_2^e = 419.94 \, \frac{\text{kJ}}{\text{kg}} \quad \text{(TAB A-2)}
\]

\[
u_2^g = 250.6 \, \frac{\text{kJ}}{\text{kg}} \quad \text{(TAB A-2)}
\]

\[
\text{Energiebilanz:}
\]

\[
(m_1 + \Delta m_2) u_2 - m_1 u_1 = \Delta m_2 h - Q_{aus}
\]

\[
(m_2 + \Delta m_2) u_2^g + m_2 g u_2^g - m_1 u_1 = \Delta m_2 h - Q_{aus}
\]

\[
\Rightarrow \Delta m_2 =```latex

\section*{Aufgabe 1.d)}

\begin{align*}
u_{R2} &= 232.95 \, \frac{\text{kJ}}{\text{kg}} \quad \text{TAR A-2} \\
u_{g2} &= 2469.6 \, \frac{\text{kJ}}{\text{kg}} \quad \text{TAB A-2} \\
m_{g}^{f} &= m_{g2}(1 - x_{D}) = 5726.225 \, \text{kg} \quad m_{g}^{g} = m_{ges} x_{D} = 28.775 \, \text{kg} \\
\Delta m_{1} &= 3288.73 \, \text{kg}
\end{align*}