

\subsection*{c)}

\[
e_{x,stc} = e_{x,stc,0} = e_{x,stc,6} = (h_{01} - h_0 - T_0 (s_{01} - s_0) + p_0 (v_{01} - v_0))
\]

\[
- (h_6 - h_0 - T_0 (s_6 - s_0) + p_0 (v_6 - v_0))
\]

\[
= h_{01} + T_0 (s_0 - s_{01} + s_6 - s_0) - h_6
\]

\[
e_{x,stc} = h_{01} - h_6 + T_0 (s_6 - s_{01})
\]

\[
-30^\circ \text{C} = (273.15 - 30) \, \text{K} = 243.15 \, \text{K}
\]

\textbf{Tabelle A-22:}

\[
h_{01} = 250.65 - 240.02 \left( \frac{24 \times 3.75 - 240}{250 - 240} \right) + 240.42
\]

\[
= 244.7 \, \frac{\text{kJ}}{\text{kg}}
\]

\[
h_0 \, \text{kennen wir}
\]

``````latex


\section*{Aufgabe 2.3}

\[
R = \frac{\bar{R}}{M_{\text{Luft}}}
\]

\[
S_6 - S_0 = S_6^\circ (6) - S_6^\circ (0) - R \ln \left( \frac{P_2}{P_1} \right)
\]

\text{Interpolation:}

\[
S_6^\circ = 1.54191 - 1.47624 \left( \frac{243.75 - 240}{250 - 240} \right) + 1.47624
\]

\[
= 1.4911 \, \text{(result)}
\]

\[
c = 1.49113
\]

``````latex