

\subsection*{b)}

\begin{align*}
    &\text{1HS} \quad h_s - h_6 \\
    &0 = \dot{m} \left[ h_s - h_6 + \frac{\omega_s^2 - \omega_6^2}{2} + g(z_e - z_a) \right] + \dot{Q} - \dot{W}_s \\
    &\frac{\dot{m} \omega_s^2}{2} + \frac{\dot{m} \omega_6^2}{2} \\
    &\frac{\dot{m} \omega_s^2}{2} h_s = \frac{\dot{m} \omega_6^2}{2} h_6 \\
    &\omega_s^2 h_s = \omega_6^2 h_6 \implies \omega_s \frac{h_s}{h_6} = \omega_6 \\
    &\text{Aus Tabelle A-22} \\
    &h_s = \frac{431.63 - 421.26}{431.9 - 430} (431.9 - 430) + 421.26 = 49 + 421.4356 \\
    &h_s = 421.44 \frac{kJ}{kg} \\
    &\text{uns ist } h_6? \\
    &\text{wir ben√∂tigen } T_6 \\
    &T_6 = T_s \left( \frac{P_6}{P_s} \right)^{\frac{n-1}{n}} \quad n = k - \frac{C_p}{C_v} = \frac{1.006 \frac{kJ}{kgK}}{C_p - R} \\
    &\text{gegeben } n = 1.4
\end{align*}

``````latex


\section*{Aufgabe 2 weiter, 2}



\subsection*{b)}

\[
T_6 = 431.4 \left( \frac{191,100 \, \text{Pa}}{50,000 \, \text{Pa}} \right)^{\frac{1.4 - 1}{1.4}}
\]

\[
= 328.67464 \, \text{K}
\]

\[
= \underline{328.1 \, \text{K}}
\]

\textbf{Interpolation:}

\[
h_6 = 328.4051 \, \frac{\text{kJ}}{\text{kg}}
\]

\[
= 328.40 \, \frac{\text{kJ}}{\text{kg}}
\]

\[
w_0 = w_s
\]

\[
w_0 = \sqrt{\frac{h_s}{k h_6}} = \sqrt{\frac{328.4031}{421.48366}} = 220 \, \text{m} \, \text{s}^{-1}
\]

\[
= 194.2051 \, \text{m} \, \text{s}^{-1}
\]

\[
\underline{w_6 = 194.2 \, \text{m} \, \text{s}^{-1}}
\]