

\item[b)] 
    \begin{align*}
        S - 3.1: \quad & \dot{S}_{\text{ein}} - \dot{S}_{\text{aus}} \\
        \dot{S}_{\text{ein}} &= \frac{\dot{Q}_{\text{aus}}}{T_{\text{RF}}} + \dot{m} \hat{s}_{\text{ein}} \\
        \dot{S}_{\text{aus}} &= \dot{m} \hat{s}_{\text{aus}} \\
        \hat{s}_{\text{ein}} &= \hat{s}_f (70^\circ C) \frac{\Delta^2}{\text{kg}} = 293.72 \frac{\text{kJ}}{\text{kg}} \\
        \hat{s}_{\text{aus}} &= \hat{s}_f (20^\circ C) \frac{\Delta^2}{\text{kg}} = 0 \\
        \dot{S}_{\text{aus}} &= \dot{m} \hat{s}_{\text{aus}} + \dot{Q}_{\text{aus}} \left( \frac{1}{T_{\text{RF}}} - \frac{1}{T_{\text{ein}}} \right)
    \end{align*}