d) \quad x_{1,2} = 2

\[
|Q_{21}| = \Delta E
\]
\[
= E_2 - E_1
\]
\[
= m_2 \cdot u_2 - m_1 \cdot u_1
\]

\[
u_2 = u_{F, ext} + \left( u_{F, ext} - u_{F, ext} \right)
\]
\[
= -333,442 + 0,1 \cdot (-0,333 - (-333,442))
\]
\[
= -333,442 + 133,397
\]

\[
Q_{21} = m_2 \cdot u_2 - m_1 \cdot u_1
\]

\[
m_2 \cdot u_2 = Q_{21} + m_1 \cdot u_1
\]

\[
u_2 = \frac{Q_{21} + m_1 \cdot u_1}{m_2}
\]

\[
u_{F, ext} + x_2 \left( u_{F, ext} - u_{F, ext} \right) = \frac{Q_{21} + m_1 \cdot u_1}{m_2}
\]

\[
x_2 = \frac{\frac{Q_{21} + m_1 \cdot u_1}{m_2} - u_{F, ext}}{u_{F, ext} - u_{F, ext}}
\]

\[
= \frac{133,410 \frac{1}{kg} - (-333,442 \frac{1}{kg})}{0,1 \frac{1}{kg} (333,442 \frac{1}{kg})}
\]

\[
= \frac{133,410 + 333,442}{0,1 \cdot 333,442}
\]

\[
= 4,555
\]

\[
u_{F, ext} - u_{F, ext} = -0,89 + 333,442 \frac{1}{kg}
\]

\[
= 333,442 \frac{1}{kg}
\]

``````latex


\[
U_1 = U_{\text{fest}} + X_1 \left( U_{\text{gesam}} - U_{\text{fest}} \right)
\]

\[
= -333,458 + 0,6 \left( -32,045 - (-333,458) \right) \frac{\text{kJ}}{\text{kg}}
\]

\[
= -333,610 \frac{\text{kJ}}{\text{kg}}
\]

``````latex