\subsection*{b) $w_0, T_6$}

\begin{equation*}
    \frac{T_6}{T_5} = \left( \frac{p_6}{p_5} \right)^{\frac{n-1}{n}}
\end{equation*}

\begin{equation*}
    T_6 = T_5 \left( \frac{p_0}{p_5} \right)^{\frac{n-1}{n}}
\end{equation*}

\begin{equation*}
    = 328.07 \, K
\end{equation*}

\begin{equation*}
    c_v = \frac{c_p}{k} = 0.718 \, c
\end{equation*}

\begin{equation*}
    s-6 \text{ reversibel adiabat}
\end{equation*}

\begin{equation*}
    \frac{dE}{dt} = \sum \dot{m}_i (h_i + \frac{c_i^2}{2}) + \dot{Q} - \dot{W}
\end{equation*}

\begin{equation*}
    m \dot{g} (u_6 - u_0) = \dot{m} \left( \frac{w_0^2}{2} - \frac{w_6^2}{2} \right)
\end{equation*}

\begin{equation*}
    2 c_v (T_6 - T_0) = \frac{w_0^2}{2} - \frac{w_6^2}{2}
\end{equation*}

\begin{equation*}
    w_6^2 = w_0^2 + 2 c_v (T_0 - T_6)
\end{equation*}

\begin{equation*}
    w_6 = 199.85 \, m/s
\end{equation*}



\subsection*{b)}

\begin{align*}
    &\Delta E = m c v_2 - m u_1 + \Delta K + \Delta P E \\
    &m \dot{s} (u_2 - u_1) = \frac{w_{c2}^2}{2} - \frac{w_{o2}^2}{2} \\
    &w_{c2}^2 = 2 \dot{m} g s (u_2) \\
    &0 = \dot{m} (h_2 - h_1 + \frac{w_{o2}^2}{2} - \frac{w_{c2}^2}{2}) + t_2 (\dot{Q} - \dot{W}) \\
    &Q_B = \dot{m} (h_0 - h_0 + \frac{w_{c2}^2}{2} - \frac{w_{o2}^2}{2}) \\
    &w_{c2}^2 = \frac{2 \dot{Q}}{m} + h_0 - h_0 + \frac{w_{o2}^2}{2} \\
    &w_{c2}^2 = \frac{2 \dot{Q}}{m} + 2 (h_0 - h_6) + \frac{w_{o2}^2}{2} \\
    &= 2 \frac{\dot{Q}}{m} + 2 cp (T_0 - T_6) + \frac{w_{o2}^2}{2}
\end{align*}

``````latex