

\section*{d)}

\[
\Delta E = (m_1 + \Delta m) u_2 - m_1 u_1 = \Delta m \left( h_f \left( 200^\circ \right) \right)
\]

\[
h_f \left( 200^\circ \right) = 83.86 \frac{\text{kJ}}{\text{kg}} \quad \text{Tafel A-Z}
\]

\[
u_2 = u_f \left( 70^\circ \right) = 292.95 \frac{\text{kJ}}{\text{kg}}
\]

\[
u_1 = x_D \left( u_f \left( 1000^\circ \right) \right) + (1 - x_D) u_f \left( 1000^\circ \right) = 429.38 \frac{\text{kJ}}{\text{kg}}
\]

\[
m_1 = 5755 \text{ kg}
\]

\[
m_1 u_2 - m_1 u_1 = \Delta m \left( h_f \left( 200^\circ \right) - u_2 \right)
\]

\[
\frac{m_1 (u_2 - u_1)}{h_f \left( 200^\circ \right) - u_2} = \Delta m = 3756.9 \text{ kg}
\]