

\subsection*{b)}
\[
\frac{d\dot{E}}{dt} = \dot{m} (h_e - h_a) \dot{Q}_{\text{aus}} \Rightarrow \dot{m} (h_a - h_e) = -\dot{Q}_{\text{aus}} = c^{it} \Delta T \dot{m}
\]
\[
c^{it} \dot{m} = -\frac{\dot{Q}_{\text{aus}}}{\Delta T} = 6,2182 \frac{\text{kJ}}{\text{sK}}
\]
\[
\frac{d\dot{E}}{dt} = \dot{m} (s_e - s_a) \dot{Q}_{\text{aus}} + s_{\text{rev}}
\]
\[
\frac{\dot{Q}_{\text{aus}}}{\dot{m} (s_e - s_a)} = \frac{\dot{Q}_{\text{aus}}}{\dot{m} c^{it} \ln \left( \frac{T_2}{T_1} \right)} = \bar{T}_h = 293,72 \text{K}
\]