

\section*{d)}

\begin{align*}
T_{EW,12} &= T_{g12} = 0^\circ \text{C} \\
\Delta E_{EW,12} &= \Delta U_{12} = Q_{12} \\
m_{EW} (u_2 - u_1) &= m_g c_v (T_{g2} - T_{g1}) = Q_{12}
\end{align*}

\begin{align*}
Q_{12} &= m_{EW} \left( u_{F,st} (1.400 \, \text{kJ}) \cdot x_{2,EW} + (1 - x_{2,EW}) u_{F,sw} (1.400 \, \text{kJ}) - u_{F,st} (1.400 \, \text{kJ}) x_{1,EW} + (1 - x) u_{F,sw} \right) \\
\frac{Q_{12}}{m_{EW}} &= \left( x_{2,EW} (u_{F,st} - u_{F,sw}) + u_{F,sw} \right) - (u_{F,sw}) + x_{2,EW} (u_{F,st} - u_{F,sw})
\end{align*}

\begin{align*}
x_{2,EW} &= \frac{1}{u_{F,st} - u_{F,sw}} \left( \frac{Q_{12}}{m_{EW}} + x_{1,EW} u_{F,st} - u_{F,sw} \right) \\
&= \frac{1}{-333.458 + 0.0458} \left( \frac{-1366.5}{0.1 \, \text{kg}} \right) \cdot 0.6 \\
x_{2,EW} &= 0.559
\end{align*}

``````latex