

\subsection*{d)}

\begin{equation*}
m_2 \, u_2 - m_1 \, u_1 = \Delta m_2 \, h_{\text{ein}}
\end{equation*}

\textbf{Tabelle A-2} f√ºr $u_{1f}$, $u_{1g}$, $u_f (70^\circ C)$, $h_{\text{ein}}$

\begin{equation*}
u_{1f} = 418{,}94 \frac{\text{kJ}}{\text{kg}}, \quad u_{1g} = 2506{,}4 \frac{\text{kJ}}{\text{kg}}
\end{equation*}

\begin{equation*}
u_1 = u_{1f} + x_0 (u_{1g} - u_{1f}) = 429{,}8 \frac{\text{kJ}}{\text{kg}}
\end{equation*}

\begin{equation*}
u_2 = u_f (70^\circ C) = 292{,}95 \frac{\text{kJ}}{\text{kg}}
\end{equation*}

\begin{equation*}
h_{\text{ein}} = 83{,}96 \frac{\text{kJ}}{\text{kg}}
\end{equation*}

\begin{equation*}
m_2 = \Delta m_2 + m_1
\end{equation*}

\begin{equation*}
\Delta m_2 \, u_2 + m_1 (u_2 - u_1) = \Delta m_2 \, h_{\text{ein}}
\end{equation*}

\begin{equation*}
\frac{m_1 (u_2 - u_1)}{h_{\text{ein}} - u_2} = \Delta m_2
\end{equation*}

\begin{equation*}
\Delta m_2 = 3756{,}9 \, \text{kg}
\end{equation*}

``````latex


\section*{Aufgabe 1:}