

\subsection*{a)}

\[
\dot{m} = 0{,}3 \, \frac{\text{kg}}{\text{s}}
\]

\[
\dot{Q}_{\text{aus}} = \dot{m} \left( h_{\text{aus}} - h_{\text{ein}} \right) - \dot{Q}_{a}
\]

\subsubsection*{Tabelle A2:}

\[
h_{\text{ein}} = h_f \left( 70^\circ \text{C} \right) = 292{,}88 \, \frac{\text{kJ}}{\text{kg}}
\]

\[
h_{\text{aus}} = h_f \left( 100^\circ \text{C} \right) = 419{,}04 \, \frac{\text{kJ}}{\text{kg}}
\]

\[
\dot{Q}_{\text{aus}} = -62{,}187 \, \text{kW}
\]



\subsection*{a)}

\begin{align*}
\Delta s_{12} &= s_2 - s_1
\end{align*}

\subsection*{Tabelle A-2:}

\begin{align*}
s(100^\circ C)_f &= 1{,}306 \frac{kJ}{kg \cdot K} & s(100^\circ C)_g &= 7{,}358 \frac{kJ}{kg \cdot K} \\
s(90^\circ C)_f &= 0{,}955 \frac{kJ}{kg \cdot K}
\end{align*}

\begin{align*}
s_1 &= s_f + x_0 (s_g - s_f) = 1{,}337 \frac{kJ}{kg \cdot K} \\
s_2 &= 0{,}955 \frac{kJ}{kg \cdot K}
\end{align*}

\begin{align*}
\Delta s_{12} &= s_2 - s_1 = -0{,}382 \frac{kJ}{kg \cdot K}
\end{align*}

``````latex