

\subsection*{d)}

\begin{equation*}
m_2 u_2 - m_1 u_1 = \Delta m_{12} u_{12} + Q_R
\end{equation*}

\begin{align*}
m_1 &= 5755 \, \text{kg} \\
m_2 &= 5755 + \Delta m
\end{align*}

\begin{equation*}
u_2 = u_f + x (u_g - u_f)
\end{equation*}

\begin{equation*}
u_2 (1000 \, \text{C}) = 478.94 + 0.005 \left( 2506.5 - 478.94 \right)
\end{equation*}

\begin{equation*}
= 429.3778 \frac{kJ}{kg}
\end{equation*}

\begin{equation*}
u_2 = u_f + x u_f (70 \, \text{C}) = 292.95 \frac{kJ}{kg}
\end{equation*}

\begin{equation*}
h_{12} = h (20 \, \text{C}, x = 0) = 83.95
\end{equation*}

\begin{equation*}
\Rightarrow (m_1 + \Delta m) u_2 - m_1 u_1 = \Delta m u_{12} + Q_R
\end{equation*}

\begin{equation*}
\Delta m (u_{12} - u_2) = -m_1 u_1 + m_1 u_2 - Q_R
\end{equation*}

\begin{equation*}
\Delta m = \frac{-m_1 u_1 + m_1 u_2 - Q_R}{u_{12} - u_2}
\end{equation*}

``````latex

\section*{1d) weiter:}

\[
\Delta m = - \frac{5775 (429,377) + 5775 (292,95) - 35 \cdot 10^3}{83,95 - 292,95}
\]

\[
= 3937 \, \text{kg}
\]