a) E-Bilanz um Reaktor (stationär)

\[
0 = \dot{Q}_R - \dot{Q}_{\text{aus}} + \dot{m}_{\text{ein}} (h_e - h_a)
\]

\[
\Rightarrow \dot{Q}_{\text{aus}} = \dot{Q}_R + \dot{m}_{\text{ein}} (h_e - h_a)
\]

\[
h_e = h_f (20^\circ C) + x_D (h_g (70^\circ C) - h_f (70^\circ C))
\]

\[
\text{Tabelle A-2} \Rightarrow 292.98 \frac{\text{kJ}}{\text{kg}} + 0.005 (2626.8 \frac{\text{kJ}}{\text{kg}} - 292.98 \frac{\text{kJ}}{\text{kg}})
\]

\[
\Rightarrow h_e = 304.65 \frac{\text{kJ}}{\text{kg}}
\]

analog gilt für $h_a$

\[
h_a = h_f (100^\circ C) + x_D (h_g (100^\circ C) - h_f (100^\circ C))
\]

\[
\text{Tab A-2} \Rightarrow 419.04 + 0.005 (2676.1 - 419.04) \frac{\text{kJ}}{\text{kg}}
\]

\[
\Rightarrow h_a = 430.325 \frac{\text{kJ}}{\text{kg}}
\]

``````latex


\section*{Aufgabe 1}



\subsection*{a)}
\begin{align*}
&\rightarrow \text{einsetzen in} \quad \dot{Q}_{\text{aus}} = \dot{Q}_R + \dot{m} (h_e - h_a) \\
&= 100 \frac{\text{kJ}}{\text{s}} + 0.3 \frac{\text{kg}}{\text{s}} \left( 304.65 - 930.325 \right) \frac{\text{kJ}}{\text{kg}} \\
&= 62.3 \frac{\text{kJ}}{\text{s}} = \dot{Q}_{\text{aus}}
\end{align*}