d) $\Delta E = \Delta U = \dot{m} (u_1 - u_2)$

\[
u_1 = u_{fg} \cdot (x \cdot u_{fg}(70,0^\circ C) + (1-x) \cdot u_1(100^\circ C))
\]

\[
u_2 = u_f(70^\circ C)
\]

\[
\Rightarrow u_1 = 0,005 \cdot 2506,5 + 0,995 \cdot 48,91 \left( \frac{4}{4,5} \right) = 429,38 \frac{kJ}{kg}
\]

\[
u_2 = 292,55 \frac{kJ}{kg}
\]

\[
\Rightarrow \Delta E = 5755 \cdot (429,38 - 292,55) = 7841,83245 = 785,0 \, MJ
\]

\[
\Delta E = \Delta m \cdot c_{wasser} \cdot \Delta T
\]

\[
\Delta E = (\dot{m}_{\text{neu}} - \dot{m}) \cdot c_w \cdot \Delta T
\]

\[
\dot{m}_{\text{neu}} = \frac{\Delta E}{c_w \cdot \Delta T} + \dot{m}, \quad c_w = 4,22
\]

\[
\dot{m}_{\text{neu}} = \frac{785000 \, kJ}{4,22 \frac{kJ}{kg \cdot K} \cdot 30} + 5755 = 11455 \, kg = 9475 \, kg
\]

\[
\Rightarrow \Delta m = 9475 - 5755 = 3720 \, kg
\]

``````latex

\begin{itemize}