c) $(m_1 \cdot v_1 = 510 \frac{J}{kg}, \quad T_0 = 340K)$

\text{Exergie einer Str√∂mung}

\[
e_{\text{ex, str}} = \dot{m} \left( h_1 - h_0 - T_0 (s_1 - s_0) + \frac{ke}{pe} \right)
\]

\[
\Rightarrow e_{\text{ex, str}} = h_1 - h_0 - T_0 (s_1 - s_0) + ke
\]

\[
ke = \frac{1}{2} \frac{510 \frac{J}{kg} \cdot 2}{2 \cdot 200^2} = 110050 \frac{J}{kg} = 110 \frac{kJ}{kg}
\]

\[
h_1 - h_0 = \int_{T_0}^{T_1} c_p(T) dT
\]

\[
\Rightarrow h_1 - h_0 = 1.006 \frac{kJ}{kg \cdot K} \cdot 340K - 1.006 \frac{kJ}{kg \cdot K} \cdot 243.15K = 97 \frac{kJ}{kg}
\]

\[
s_1 - s_0 = c_p \cdot \int_{T_0}^{T_1} \frac{dT}{T} - R \ln \left( \frac{p_1}{p_0} \right)
\]

\[
\Rightarrow s_1 - s_0 = 1.006 \frac{kJ}{kg \cdot K} \ln \left( \frac{340K}{243.15K} \right) - 8.314 \frac{kJ}{kg \cdot K} \left( \frac{1}{0} \right)
\]

\[
\Rightarrow s_1 - s_0 = 0.3372 \frac{kJ}{kg \cdot K}
\]

\[
\Rightarrow e_{\text{ex, str}} = \frac{97 \frac{kJ}{kg}}{kg} + 243.15
\]

\[
e_{\text{ex, str}} = 97 \frac{kJ}{kg} + 243.15 \frac{kJ}{kg} + 0.3372 \frac{kJ}{kg \cdot K} + 110 \frac{kJ}{kg}
\]

\[
e_{\text{ex, str}} = 125.06 \frac{kJ}{kg}
\]