

\subsection*{a)}
\begin{equation*}
0 = \dot{m}_{\text{ein}} (h_{\text{ein}} - h_{\text{aus}}) + \dot{Q}_R - \dot{W}_R^0 + \dot{Q}_{\text{aus}}
\end{equation*}

\begin{equation*}
h(70^\circ C) = h_{\text{ein}} = 292.98 \frac{\text{kJ}}{\text{kg}} \quad \text{TAB. A-2}
\end{equation*}

\begin{equation*}
h(100^\circ C) = h_{\text{aus}} = 419.04 \frac{\text{kJ}}{\text{kg}} \quad \text{TAB. A-2}
\end{equation*}

\begin{equation*}
\dot{Q}_{\text{aus}} = \dot{m}_{\text{ein}} (h_{\text{aus}} - h_{\text{ein}}) - \dot{Q}_R = 0.3 \cdot (419.04 - 292.98) - 400 = -62.18 \, \text{kW}
\end{equation*}