d)
\]

\[
T_{\text{Eis},1} = T_{\text{Eis},2} \quad \text{weil} \quad x_2 > 0
\]

\[
\Delta u_{12,\text{Eis}} = 0 - Q_{12}
\]

\[
m_{\text{Eis}} \cdot (u_{1,2,\text{Eis}} - u_{1,1,\text{Eis}}) = -Q_{12}
\]

\[
u_{1,1,\text{Eis},\text{flüssig}} = -0,045 \, \frac{\text{kJ}}{\text{kg}} \quad \text{Tab. 1}
\]

\[
u_{1,1,\text{Eis},\text{fest}} = -333,458 \, \frac{\text{kJ}}{\text{kg}}
\]

\[
u_{1,2,\text{Eis}} = u_{1,1,\text{Eis},F} + (1 - x_{\text{Eis},1}) \left( u_{1,\text{Eis},\text{flüssig}} - u_{1,1,\text{Eis},F} \right) =
\]

\[
= -333,458 + (1 - 0,6) \left( -0,045 + 333,458 \right) = -200,093 \, \frac{\text{kJ}}{\text{kg}}
\]

\[
u_{2,1,\text{Eis}} = \frac{-Q_{12}}{m_{\text{Eis}}} + u_{1,1,\text{Eis}} = \frac{0,8046}{0,1} \quad \text{bzw.} \quad -200,093 =
\]

\[
= -192,05 \, \frac{\text{kJ}}{\text{kg}}
\]

\[
x_{1,2,\text{Eis}} = \frac{u_{2,1,\text{Eis}} - u_{2,1,\text{Eis},F}}{u_{2,1,\text{Eis},\text{flüssig}} - u_{2,1,\text{Eis},F}} + 1 = \frac{-192,05 + 333,458}{-0,045 + 333,458} + 1 = 0,5759
\]

``````latex