

\subsection*{b)}

\[
\dot{Q}_{\text{aus}} = 65 \text{kW}
\]

\[
\frac{1}{I_{kS}} = \frac{s_{\text{ein}} - s_{\text{aus}}}{s_{\text{aus}} - s_{\text{ein}}}
\]

\[
T \cdot ds = dU - p \cdot dV = dH
\]

\[
dH = \dot{U} + p dV
\]

\[
\frac{1}{I_{kS}} = \frac{\int_{s_{\text{ein}}}^{s_{\text{aus}}} dH}{s_{\text{aus}} - s_{\text{ein}}} = \frac{h_{\text{aus}} - h_{\text{ein}}}{s_{\text{aus}} - s_{\text{ein}}} = C \cdot \frac{(T_{\text{aus}} - T_{\text{ein}})}{s_{\text{aus}} - s_{\text{ein}}}
\]

\[
\frac{1}{I_{kS}} = \frac{(T_{\text{aus}} - T_{\text{ein}})}{\mu \cdot \ln \left( \frac{T_2}{T_1} \right)} = \frac{T_{\text{aus}} - T_{\text{ein}}}{\ln \left( \frac{T_{\text{aus}}}{T_{\text{ein}}} \right)} = 293,1226 \text{K}
\]

``````latex