

\subsection*{d)}
\[
\left| Q_{12} \right| = 1500 \, \text{J} \quad \text{zugef√ºhrt}
\]

\[
\Delta E = E_2 - E_1 = m_{eq} MEW (u_2 - u_1) = \cancel{Q_{12} - W}^0 \quad \text{EW dehnt sich nicht aus}
\]

\[
u_{12} \quad u_2 - u_1 = \frac{Q_{12}}{m_{EW}} = \frac{1.5 \, \text{kJ}}{0.1 \, \text{kg}} = 15 \, \frac{\text{kJ}}{\text{kg}}
\]

\[
u_2 @ 0^\circ C \quad x_{es1} = 0.6 \quad P_{es1} = \frac{M k g}{A} + P_{amb} = \frac{g}{D^2} \frac{mk}{4} + P_{amb}
\]

\[
u_{fes} + 13.997 = -333.224 + 333.812 \quad \left( \frac{13.997 - 10}{20 - 10} - 333.812 \right) = 13.997 \, \text{Pa} = 3.997 \, \text{bar}
\]

\[
u_{fes3} = -333.224 - 333.812 \quad \text{Tafel 1}
\]

\[
u_{fes} = -333.97 \, \frac{\text{kJ}}{\text{kg}}
\]

\[
u_{fes13.997} = -0.663 - 0.322 \quad \left( \frac{13.997 - 10}{20 - 10} - 0.322 \right) = -0.450 \, \frac{\text{kJ}}{\text{kg}}
\]

\[
u_1 = u_f + x(u_{fg} - u_f) = -16.721 \, \frac{\text{kJ}}{\text{kg}}
\]

\[
u_2 = u_1 + \frac{15 \, \text{kJ}}{\text{kg}} \quad u_2 = -1.721 \, \frac{\text{kJ}}{\text{kg}}
\]

``````latex

3(d)

\[
u_2 = -152,2 \frac{kJ}{kg}
\]

\[
u_2 = u_{4L} + x_2 (u_{4E} - u_{4L})
\]

\[
\frac{u_2 - u_{4L}}{u_{4E} - u_{4L}} = x_{2eis} = \frac{-152,2 - 0,450}{-333,97 - 0,450} = 0,455 = x_{2eis}
\]

``````latex