

\section*{3d)}

\begin{equation*}
    X_{EIS} = \frac{\Theta - \Theta_f}{\Theta_g - \Theta_f}
\end{equation*}

\begin{equation*}
    = \frac{u_2 - u_f}{u_g - u_f} = \frac{-185.090 \frac{kJ}{kg} + 335.458 \frac{kJ}{kg}}{u_g - u_f}
\end{equation*}

\textbf{Zustand 1}

\begin{equation*}
    0.06 \, kg \, Eis
\end{equation*}

\begin{equation*}
    0.09 \, kg \, Wasser
\end{equation*}

\begin{equation*}
    u_1 = -335.458 \frac{kJ}{kg} \cdot 0.06 \, kg - 0.045 \frac{kJ}{kg} \cdot 0.09 \, kg = -20.009 \, kJ
\end{equation*}

\begin{equation*}
    Q_m = \Delta U = u_2 - u_1
\end{equation*}

\begin{equation*}
    u_2 = Q_m + u_1 = -185.097 - 20.0097 = -185.097 \, kJ
\end{equation*}

\begin{equation*}
    u_2 = \frac{u_m}{m} = \frac{-185.090 \, kJ}{kg}
\end{equation*}

``````latex