

\item[a)] \textbf{Energiebilanz: (station√§r)}
    \begin{align*}
        0 &= \dot{m} (h_{\text{ein}} - h_{\text{aus}}) + \dot{Q}_{\text{aus}} \\
        \Rightarrow \dot{Q}_{\text{aus}} &= \dot{m} (h_{\text{ein}} - h_{\text{aus}})
    \end{align*}
    \begin{align*}
        h_{\text{ein}} &= h_f (70^\circ C) = 252.58 \frac{\text{kJ}}{\text{kg}} \\
        h_{\text{aus}} &= h_f (40^\circ C) = 418.09 \frac{\text{kJ}}{\text{kg}} \\
        \dot{Q}_{\text{aus}} &= -\dot{m} (h_{\text{ein}} - h_{\text{aus}}) = 37.82 \text{kW}
    \end{align*}