

\subsection*{d)}

\begin{align*}
    \Delta m_{x2}, \text{ sodass } T_{R,2} = 70^\circ C \text{ erreicht wird.} \\
    T_{ein, x2} = 20^\circ C \\
    Q_{R, x2} = 35 \text{ MJ}
\end{align*}

Energiegleichung geschlossenes System:

\begin{align*}
    \Delta E &= m_2 u_2 - m_1 u_1 = \Delta m_{x2} \cdot h_{ein} + Q_{R, x2} - Q_{a, x1} \\
    &\quad \text{(kein } Q_{a, x1} = 0) \\
    m_2 &= m_1 + \Delta m_{x2}, \quad u_2 = u(70^\circ C, \text{sied. FL}) \\
    m_1 &= m_{ges}, 1, \quad u_1 = u(100^\circ C, \text{sied. FL}) \\
    h_{ein} &= h(20^\circ C, \text{sied. FL})
\end{align*}

\begin{align*}
    (m_1 + \Delta m_{x2}) u_2 - m_1 u_1 &= \Delta m_{x2} \cdot h_{ein} + Q_{R, x2} \\
    m_1 u_2 + \Delta m_{x2} u_2 - m_1 u_1 &= \Delta m_{x2} \cdot h_{ein} + Q_{R, x2} \\
    \Delta m_{x2} (u_2 - h_{ein}) &= m_1 (u_1 - u_2) + Q_{R, x2}
\end{align*}

\begin{align*}
    \Delta m_{x2} &= \frac{m_1 (u_1 - u_2) + Q_{R, x2}}{u_2 - h_{ein}} \\
    &= \frac{5755 \text{ kg} \left( 418.54 \frac{\text{kJ}}{\text{kg}} - 252.57 \frac{\text{kJ}}{\text{kg}} \right) + 35000 \text{ kJ}}{252.57 \frac{\text{kJ}}{\text{kg}} - 83.96 \frac{\text{kJ}}{\text{kg}}} \\
    &= \frac{5755 \text{ kg} \cdot 165.97 \frac{\text{kJ}}{\text{kg}} + 35000 \text{ kJ}}{168.61 \frac{\text{kJ}}{\text{kg}}} \\
    &= \frac{955.36 \text{ kJ} + 35000 \text{ kJ}}{168.61 \frac{\text{kJ}}{\text{kg}}} \\
    &= 3465.4 \text{ kg} + 167.4 \text{ kg} = 3636.8 \text{ kg} = \Delta m_{x2}
\end{align*}