d)

\begin{align*}
    m_2 u_2 - m_1 u_1 &= \Delta m_{12} (h_2 - h_1) \\
    m_2 u_2 - m_1 u_1 &= \Delta m_{12} (h_2 - h_1) \quad \text{weil} \\
    &\quad \text{Q = 0} \\
    m_1 &= 5755 \, \text{kg} \\
    m_2 &= x m_1 + \Delta m_{12} \\
    u_2 &= x u_g + (1 - x) u_f \quad \text{aus A-2} \\
    u_g &= 2506.5 \, \frac{\text{kJ}}{\text{kg}} \\
    u_f &= 428.94 \, \frac{\text{kJ}}{\text{kg}} \\
    x &= 0.005 \\
    u_2 &= h_{fg} (70^\circ \text{C}) = 2333.8 \, \frac{\text{kJ}}{\text{kg}} \quad \text{aus A-2} \\
    &\quad \text{weil Volum√§nderung} \\
    h_1 &= h_{fg} (20^\circ \text{C}) = 2454.1 \, \frac{\text{kJ}}{\text{kg}} \quad \text{aus A-2} \\
    h_2 &= h_{fg} (70^\circ \text{C}) = 2333.8 \, \frac{\text{kJ}}{\text{kg}} \quad \text{aus A-2} \\
    (m_1 + \Delta m_{12}) u_2 - m_1 u_1 &= \Delta m_{12} (h_2 - h_1) \\
    \Delta m_{12} (u_2 - h_2 + h_1) &= m_1 u_1 - u_2 m_1 \\
    \Delta m_{12} &= \frac{-m_1 u_1 + m_1 u_2}{u_2 - h_2 + h_1} = \frac{m_1 (u_2 - u_1)}{h_1} \\
    \Delta m_{12} &= 4468.31 \, \text{kg}
\end{align*}

``````latex


\section*{Aufgabe 1}