

\subsection*{c)}

\begin{align*}
\frac{(u_{g,2} - u_{g,1})}{m_g} &= q_{12} - w_v \\
w_v &= \int_{1}^{2} p \, dv \rightarrow \text{isobar} \\
w_v &= mp(v_2 - v_1) \\
v_2 &= \frac{RT_2}{p_{g,2}} = 0.324 \, \frac{\text{m}^3}{\text{kg}} \\
v_2 &= 0.9182 \, \frac{\text{m}^3}{\text{kg}} \\
p_{g,2} &= 1.4 \, \text{bar} \\
m_g &= 3.42 \, \text{g} \\
w_v &= -284.42 \, \text{J} \\
u_{g,2} - u_{g,1} &= c_v p_{g,2} (T_2 - T_1) = -376.5 \, \frac{\text{kJ}}{\text{kg}} \\
q_{12} &= m_g (u_{g,2} - u_{g,1}) + w_v \\
q_{12} &= -1.3688 \, \text{kJ}
\end{align*}

\begin{align*}
|q_{12}| &= 1.3688 \, \text{kJ}
\end{align*}

``````latex