

\section*{b)}

\[
\dot{Q}_{\text{aus}} = 65 \text{kW}
\]

\[
\overline{T}_{\text{MF}} = \frac{\int_{s_{\text{ein}}}^{s_{\text{aus}}} T ds}{s_{\text{aus}} - s_{\text{ein}}} = \frac{q_{\text{kV}}}{s_{\text{aus}} - s_{\text{ein}}}
\]

\[
\text{aus Energiebilanz:} \quad q_{\text{kV}} = h_{\text{aus}} - h_{\text{ein}} = c \dot{m} (T_{\text{aus}} - T_{\text{ein}})
\]

\[
s_{\text{aus}} - s_{\text{ein}} = \int_{T_{\text{ein}}}^{T_{\text{aus}}} \frac{c \dot{m}}{T} dT = c \dot{m} \ln \left( \frac{T_{\text{aus}}}{T_{\text{ein}}} \right)
\]

\[
\Rightarrow \overline{T}_{\text{MF}} = \frac{T_{\text{aus}} - T_{\text{ein}}}{\ln \left( \frac{T_{\text{aus}}}{T_{\text{ein}}} \right)} = 293.123 \text{K}
\]