

\subsection*{b)}

\[
\frac{\overline{T}_{\text{KF}}}{\overline{T}_{\text{KF}}} = \frac{\int_{s_a}^{s_e} T dS}{s_a - s_e}
\]

\[
\Rightarrow \dot{Q} = \dot{m}_{\text{KF}} (S_{\text{KF ein}} - S_{\text{KF aus}}) + \frac{\dot{Q}_{\text{aus}}}{\overline{T}}
\]

\[
\frac{\dot{Q}_{\text{aus}}}{\overline{T}} = \frac{S_{\text{UF ein}} - S_{\text{UF aus}}}{\overline{T}}
\]

\[
\Rightarrow \overline{T} = \frac{T_{\text{aus}} - T_{\text{ein}}}{\ln \left( \frac{T_{\text{aus}}}{T_{\text{ein}}} \right)} = 357.84 \, \text{K}
\]