(d) \( m_{EW} \left( U_{EW,2} - U_{EW,1} \right) = Q_{12} \quad \text{(Arbeit 0, da isochor)} \)

\[
\Delta E = \Delta U = \cancel{\Delta p_{EW}}
\]

\[
U_{EW,1} = U_{flüssig} \left( 0^\circ C, 1.4 \text{bar} \right) + X_{Eis,1} \cdot \left( U_{fest} \left( 0^\circ C, 1.4 \text{bar} \right) - U_{flüssig} \left( 0^\circ C, 1.4 \text{bar} \right) \right)
\]

\[
= -200.117 \, \frac{kJ}{kg}
\]

\[
U_{EW,2} = U_{flüssig} \left( 0^\circ C, 1.4 \text{bar} \right) + X_{Eis,2} \cdot \left( U_{fest} \left( 0^\circ C, 1.4 \text{bar} \right) - U_{flüssig} \left( 0^\circ C, 1.4 \text{bar} \right) \right)
\]

\[
m_{EW} \left( U_{EW,2} - U_{EW,1} \right) = m_{EW} \left( X_{Eis,2} \cdot \left( U_{fest} \left( 0^\circ C, 1.4 \text{bar} \right) - U_{flüssig} \left( 0^\circ C, 1.4 \text{bar} \right) \right) - X_{Eis,1} \cdot \left( U_{fest} \left( 0^\circ C, 1.4 \text{bar} \right) - U_{flüssig} \left( 0^\circ C, 1.4 \text{bar} \right) \right) \right) = Q_{12}
\]

``````latex


Fortsetzung 3.d.:

\[
X_{\text{Eis,2}} = \frac{\frac{Q_{12}}{m_{\text{EN}}} + X_{\text{Eis,1}} \left( U_{\text{Eis}} (0^\circ C, 1.46 \text{bar}) - U_{\text{flüssig}} (0^\circ C, 1.46 \text{bar}) \right)}{U_{\text{Eis}} (0^\circ C, 1.46 \text{bar}) - U_{\text{flüssig}} (0^\circ C, 1.46 \text{bar})}
\]

\[
= 0.559
\]

``````latex