

\subsection*{(e)}

\begin{align*}
\Delta S &= m_2 S_2 - m_1 S_1 = (m_2 + \Delta m_{12}) S_2 - m_1 S_1
\end{align*}

\begin{align*}
S_1 &= s(100^\circ C, \, x=0.005) = s_f(100^\circ C) + x \cdot (s_g(100^\circ C) - s_f(100^\circ C)) \\
&= 1.337 \, \frac{\text{kJ}}{\text{kg} \cdot \text{K}} \quad \text{(A-2)}
\end{align*}

\begin{align*}
S_2 &= s(70^\circ C, \, x=0) = s_f(70^\circ C) = 0.3549 \, \frac{\text{kJ}}{\text{kg} \cdot \text{K}} \quad \text{(A-2)}
\end{align*}

\begin{align*}
\Delta S &= 1227.7 \, \frac{\text{kJ}}{\text{K}}
\end{align*}

``````latex