(a) Stationärer Fließprozess:

\[
0 = \dot{m}_{\text{ein}} (h_{\text{ein}} - h_{\text{aus}}) + \dot{Q}_R - \dot{Q}_{\text{aus}}
\]

\[
\dot{Q}_{\text{aus}} = \dot{m}_{\text{ein}} (h_{\text{ein}} - h_{\text{aus}}) + \dot{Q}_R
\]

\[
h_{\text{ein}} - h(70^\circ C, x=0) = h_f(70^\circ C) = 292.98 \frac{\text{kJ}}{\text{kg}} \quad \text{(A-2)}
\]

\[
h_{\text{aus}} = h(100^\circ C, x=0) = h_f(100^\circ C) = 419.04 \frac{\text{kJ}}{\text{kg}} \quad \text{(A-2)}
\]

\[
\dot{Q}_{\text{aus}} = 0.3 \frac{\text{kg}}{\text{s}} \left( 292.98 \frac{\text{kJ}}{\text{kg}} - 419.04 \frac{\text{kJ}}{\text{kg}} \right) + 100 \text{kW}
\]

\[
= 62.18 \text{kW}
\]