(d) 

\[
\Delta E = \cancel{\Delta U} = m_2 u_2 - m_1 u_1 = \Delta m_{12} h_{\text{ein,12}} - \dot{Q}_{\text{aus,12}}
\]

\[
\Delta m_{12} = \frac{m_2 u_2 - m_1 u_1 + \dot{Q}_{\text{aus,12}}}{h_{\text{ein,12}}} =
\]

``````latex


\section*{Fortsetzung 1.d:}

\begin{align*}
(m_1 + \Delta m_{12}) U_2 - m_1 U_1 &= \Delta m_{12} \cdot h_{\text{ein},12} - Q_{\text{aus},12} \\
\Delta m_{12} (U_2 - h_{\text{ein},12}) &= m_1 U_1 - m_1 U_2 - Q_{\text{aus},12} \\
\Delta m_{12} &= \frac{m_1 U_1 - m_1 U_2 - Q_{\text{aus},12}}{U_2 - h_{\text{ein},12}}, \quad m_1 = m_{\text{gas},1} = 3755 \, \text{kg}
\end{align*}

\begin{align*}
h_{\text{ein},12} &= h(20^\circ C, \, x=0) = h_f(20^\circ C) = 83.36 \, \frac{\text{kJ}}{\text{kg}} \quad \text{(A-2)} \\
U_1 &= U(100^\circ C, \, x=0) = U_f(100^\circ C) = 418.94 \, \frac{\text{kJ}}{\text{kg}} \quad \text{(A-2)} \\
U_2 &= U(70^\circ C, \, x=0) = U_f(70^\circ C) = 292.95 \, \frac{\text{kJ}}{\text{kg}} \quad \text{(A-2)}
\end{align*}

\begin{align*}
\Delta h_{12} &= U_1 = U(100^\circ C, \, x=0.005) - U_f(100^\circ C) + x \cdot (U_g(100^\circ C) - U_f(100^\circ C)) \\
&= 429.38 \, \frac{\text{kJ}}{\text{kg}} \quad \text{(A-2)}
\end{align*}

\begin{align*}
\Delta m_{12} &= 3588.4 \, \text{kg}
\end{align*}