

\subsection*{d)}
\begin{align*}
    m_{ew} (u_2 - u_1) &= l Q_{12} \quad \text{mit vorgegebenem } l \text{ (gilt unter anderem)} \\
    u_1 &= 0,6 \cdot (-333,455 \frac{\text{J}}{\text{kg}}) + 0,4 \cdot (-0,65 \frac{\text{J}}{\text{kg}}) = -200,933 \frac{\text{J}}{\text{kg}} \\
    u_2 &= x_{Eis2} \cdot (-333,455 \frac{\text{J}}{\text{kg}}) + (1 - x_{Eis2}) \cdot (-0,65 \frac{\text{J}}{\text{kg}}) \\
    Q_{12} &= 15 \frac{\text{J}}{\text{kg}} \\
    u_2 &= 15 \frac{\text{J}}{\text{kg}} = 200,933 \frac{\text{J}}{\text{kg}} - 185,693 \frac{\text{J}}{\text{kg}} \\
    -185,693 \frac{\text{J}}{\text{kg}} &= x_{Eis2} \cdot (-333,455 \frac{\text{J}}{\text{kg}}) \\
    x_{Eis2} &= 0,555
\end{align*}

``````latex