

\subsection*{c}

\begin{align*}
0 &= \dot{m} \left[ S_e - S_a \right] + \frac{\dot{Q}_{aus}}{T} + \dot{S} \\
-\dot{S} &= 0,3 \, \frac{\text{kg}}{\text{s}} \left[ 0,9549 \, \frac{\text{kJ}}{\text{kgK}} + 1,308 \, \frac{\text{kJ}}{\text{kgK}} \right] \\
&+ \frac{62,18 \, \text{kW}}{293,12 \, \text{K}} \\
&\Rightarrow \dot{S} = 0,1 \, \frac{\text{kJ}}{\text{kgK}}
\end{align*}

\begin{align*}
S_{ex} - S_{0} &= S_{e} - S_{a} = c \ln \left( \frac{T_a}{T_{ein}} \right) \\
S_e &= 0,9549 \, \frac{\text{kJ}}{\text{kgK}} \\
S_a &= 1,308 \, \frac{\text{kJ}}{\text{kgK}}
\end{align*}