\section*{Problem d)}

\begin{equation*}
    dE = 0 \quad \text{(O, Wasser macht keine W)}
\end{equation*}

\begin{equation*}
    dE = \sum \dot{m} \left( h + \frac{c^2}{2} + gz \right) + \sum \dot{Q} - \sum \dot{W}
\end{equation*}

\begin{equation*}
    m (u_2 - u_1) = \dot{Q}
\end{equation*}

\begin{equation*}
    p_{EW,2} = p_0 + \rho g + \frac{c^2}{2}
\end{equation*}

\begin{equation*}
    = 1.4 \text{ bars}
\end{equation*}

\begin{equation*}
    m \left( x_{Eis,2} \left( u_{Eis,2} \right) + (1 - x_{Eis,2}) u_{Wasser,2} \right) = \dot{Q}
\end{equation*}

\begin{equation*}
    m \left( x_{Eis,2} \left( u_{Eis,2} \right) + (1 - x_{Eis,2}) u_{Wasser,2} \right) = \dot{Q}
\end{equation*}

\begin{equation*}
    m \left( x_{Eis,2} \left( u_{Eis,2} \right) + (1 - x_{Eis,2}) u_{Wasser,2} \right) = \dot{Q}
\end{equation*}

\begin{equation*}
    m \left( x_{Eis,2} \left( u_{Eis,2} \right) + (1 - x_{Eis,2}) u_{Wasser,2} \right) = \dot{Q}
\end{equation*}

\begin{equation*}
    m \left( x_{Eis,2} \left( u_{Eis,2} \right) + (1 - x_{Eis,2}) u_{Wasser,2} \right) = \dot{Q}
\end{equation*}

\begin{equation*}
    m \left( x_{Eis,2} \left( u_{Eis,2} \right) + (1 - x_{Eis,2}) u_{Wasser,2} \right) = \dot{Q}
\end{equation*}

\begin{equation*}
    m \left( x_{Eis,2} \left( u_{Eis,2} \right) + (1 - x_{Eis,2}) u_{Wasser,2} \right) = \dot{Q}
\end{equation*}

\begin{equation*}
    m \left( x_{Eis,2} \left( u_{Eis,2} \right) + (1 - x_{Eis,2}) u_{Wasser,2} \right) = \dot{Q}
\end{equation*}

\begin{equation*}
    m \left( x_{Eis,2} \left( u_{Eis,2} \right) + (1 - x_{Eis,2}) u_{Wasser,2} \right) = \dot{Q}
\end{equation*}

\begin{equation*}
    m \left( x_{Eis,2} \left( u_{Eis,2} \right) + (1 - x_{Eis,2}) u_{Wasser,2} \right) = \dot{Q}
\end{equation*}

\begin{equation*}
    m \left( x_{Eis,2} \left( u_{Eis,2} \right) + (1 - x_{Eis,2}) u_{Wasser,2} \right) = \dot{Q}
\end{equation*}

\begin{equation*}
    m \left( x_{Eis,2} \left( u_{Eis,2} \right) + (1 - x_{Eis,2}) u_{Wasser,```latex