

\subsection*{c)}

\[
\Delta e_{ex,Stk} = (h_6 - h_0 - T_0 (s_6 - s_0) + ke_6 - ke_0)
\]

\[
= c_p (T_6 - T_0) - T_0 \left( c_p \ln \left( \frac{T_6}{T_0} \right) - R \ln \left( \frac{p_6^0}{p_0} \right) \right) + \frac{1}{2} w_6^2 - \frac{1}{2} w_0^2
\]

\[
= 85.432425 \, \frac{kJ}{kg} - 73.275 \, \frac{kJ}{kg} + \frac{1}{2} w_6^2 - \frac{1}{2} w_0^2 + 40.55.55.7.45
\]

\[
= 16.254 \, \frac{kJ}{kg}
\]

``````latex

\[
\frac{d}{d t} \left( \dot{m} e_x \right) = \sum \dot{m} e_{x, \text{ein}} + \sum \dot{m} e_{x, \text{aus}} - \sum \left( \dot{m} \frac{p^0}{\rho^0} \frac{d \rho^0}{d t} \right) - \dot{E}_{x, \text{verl}}
\]

\[
0 = \Delta \dot{E}_{x, \text{sonst}} - \dot{E}_{x, \text{verl}}
\]

\[
\dot{E}_{x, \text{verl}} = \Delta \dot{E}_{x, \text{sonst}}
\]

\[
\dot{E}_{x, \text{verl}} = \Delta e_{x, \text{sonst}}
\]

\[
\dot{m} = 16.254 \, \text{kJ}
\]

``````latex