

\section*{d)}

\begin{equation*}
\frac{dE^{\text{ab}}}{dt} = \sum \dot{m}_i \cdot i - \sum \dot{Q} - \sum \dot{\omega}^{\text{ab}}
\end{equation*}

\begin{equation*}
\Delta U = \dot{m} (h_{\text{ein},12} - h_{\text{aus},12}) - \dot{Q}_{R,12}
\end{equation*}

\begin{equation*}
m_{\text{tot},12} - m_{u,12} = \dot{m} \cdot t_{\text{ein},12} - \dot{Q}_{R,12}
\end{equation*}

\begin{equation*}
(\dot{m} \cdot u_2 - m_{u,12}) = \dot{m} \cdot h_{\text{ein},12} - \dot{Q}_{R,12}
\end{equation*}

\begin{equation*}
\dot{m} \cdot u_2 - \dot{m} \cdot h_{\text{ein},12} = - \dot{Q}_{R,12} + m_{u,12} \cdot u_2 - m_{u,12}
\end{equation*}

\begin{equation*}
\dot{m} (u_2 - h_{\text{ein},12}) = \dot{Q}_{R,12} + m_{u,12} \cdot u_2 - m_{u,12}
\end{equation*}

\begin{equation*}
\boxed{\dot{m} = 3301.94 \, \text{kg}}
\end{equation*}