

\subsection*{b)}

\begin{equation*}
    \frac{T_6}{T_5} = \left( \frac{P_6}{P_5} \right)^{\frac{n-1}{n}}
\end{equation*}

\begin{equation*}
    T_6 = T_5 \left( \frac{P_0}{P_5} \right)^{\frac{n-1}{n}} = 439.9 \text{K} \left( \frac{0.994 \text{ bar}}{0.5 \text{ bar}} \right)^{0.4/1.4} = \underline{328.1 \text{ K}}
\end{equation*}

\textbf{Energiegleich:}

\begin{equation*}
    0 = \dot{m} \left[ h_5 - h_6 + \frac{(w_5^2 - w_0^2)}{2} \right]
\end{equation*}

\begin{equation*}
    h_5 - h_6 = c_p \left( T_5 - T_6 \right) = 1.006 \frac{\text{kJ}}{\text{kg} \cdot \text{K}} (439.9 - 328.1) = 112.4 \frac{\text{kJ}}{\text{kg}}
\end{equation*}

\begin{equation*}
    w_0^2 = 2 (h_5 - h_6) + w_5^2 = 2 (112.4) + 220^2 \frac{\text{m}^2}{\text{s}^2} = 224.8 + 48400 = 48624.8 \frac{\text{m}^2}{\text{s}^2}
\end{equation*}

\begin{equation*}
    w_0 = \sqrt{48624.8 \frac{\text{m}^2}{\text{s}^2}} = \underline{220.5 \frac{\text{m}}{\text{s}}}
\end{equation*}

``````latex