c)
\begin{align*}
\Delta e_{x,str} &= (h_{aus} - h_{ein} - T_0 (s_{aus} - s_{ein}) + \frac{v_{aus}^2 - v_{ein}^2}{2} \\
h_{aus} - h_{ein} &= h_2 - h_0 = c_p^{15} (T_2 - T_0) = 1006 \frac{kJ}{kgK} \\
&= 1.006 \frac{kJ}{kgK} (328.16 - 243.15 K) \\
&= 85.4597 \frac{kJ}{kg} \\
T_0 (s_{aus} - s_{ein}) &\approx T_0 (s_2 - s_0) = T_0 \left( c_p^{15} \ln \left( \frac{T_2}{T_0} \right) - R \ln \left( \frac{p_0}{p_0} \right) \right) \quad \text{(p_0 = p_2)} \\
&= 243.15 K / 1.006 \frac{kJ}{kgK} \left( \ln \left( \frac{328.1}{243.15} \right) \right) = 73.2946 \frac{kJ}{kg} \\
\frac{v_{aus}^2 - v_{ein}^2}{2} &= \frac{v_2^2 - v_0^2}{2} = \frac{507.1 \frac{m^2}{s^2} - 200 \frac{m^2}{s^2}}{2} = 108620.85 \frac{J}{kg} \\
&= 108.621 \frac{kJ}{kg} \\
\Delta e_{x,str} &= 85.4597 \frac{kJ}{kg} - 73.2946 \frac{kJ}{kg} + 108.621 \frac{kJ}{kg} \\
&= 120.786 \frac{kJ}{kg}
\end{align*}