

\subsection*{b)}

\begin{align*}
    w_0 \quad \text{und} \quad T_6 \quad \text{am Austritt} \\
    \rightarrow \text{Energie Gleich für stationären Fließprozess} \\
    0 &= h \left[ h_5 - h_6 - \frac{w_2^2 - w_1^2}{2} \right] + \sum \frac{\dot{Q}_j}{\dot{m}} - \sum \frac{\dot{W}_k}{\dot{m}} \\
    \rightarrow 2 (h_6 - h_5) + w_5^2 - w_6^2 \\
    w_6 &= \sqrt{2 \cdot (h_5 - h_6) + w_5^2} \\
    h_6 - h_5 &= \int_{T_5}^{T_6} c_p dT = c_p (T_6 - T_5) \\
    \rightarrow T_5 - T_6 \quad \text{adiabat - reversibel} \rightarrow \text{isentrop} \\
    \rightarrow \text{polytrope Temperaturverhältnis mit} \quad n = k = 1.4 \\
    \frac{T_6}{T_5} &= \left( \frac{p_6}{p_5} \right)^{\frac{n-1}{n}} \rightarrow T_6 = T_5 \left( \frac{p_6}{p_5} \right)^{\frac{n-1}{n}} \\
    \rightarrow T_6 &= 431.9 \, K \quad \left( 0.193 \frac{bar}{0.1 \, bar} \right)^{\frac{0.4}{1.4}} \\
    &= 326.07 \, K \\
    \rightarrow h_6 - h_5 &= c_p (T_6 - T_5) \\
    &= 1.006 \frac{kJ}{kgK} (326.07 K - 431.9 K) \\
    &= -106.45 \frac{kJ}{kg} \\
    \rightarrow w_6 &= \sqrt{2 (h_5 - h_6) + w_5^2} \\
    &= \sqrt{2 \cdot 106.45 \frac{kJ}{kg}} \\
    &= 243.54 \frac{m}{s}
\end{align*}