

\subsection*{c)}

\begin{itemize}
    \item \textbf{Stationäre 1HS um Schaufelröhre:}
    \[
    0 = \dot{m} \left( h_5 - h_6 \right) + \frac{w_{s5}^2 - w_{s6}^2}{2}
    \]
    \item \textbf{reversible adiabate Schaufelröhre:}
    \[
    \frac{T_6}{T_5} = \left( \frac{P_6}{P_5} \right)^{\frac{n-1}{n}}
    \]
    \item \( n = 1.4 \)
    \item \( h_5 - h_6 = c_p (T_5 - T_6) \)
    \[
    = 1.006 (431.5 - 320)
    \]
    \[
    = 104 \frac{kJ}{kg}
    \]
    \item \( T_6 = T_5 \left( \frac{P_6}{P_5} \right)^{\frac{n-1}{n}} = 320 K \)
\end{itemize}

``````latex



\section*{c)}

\begin{align*}
\dot{Q}_{str} &= \dot{m} \left[ h_0 - h_6 - T_0(s_0 - s_6) + \Delta k_e \right] \\
\dot{Q}_{str} &= \\
h_0 - h_6 &= c_p (T_0 - T_6) = 85.36 \, \frac{kJ}{kg} \\
s_6 - s_6 &= c_p \ln \left( \frac{T_0}{T_6} \right) - R \ln \left( \frac{p_0}{p_6} \right) = -0.3 - 286.99 \left( \frac{p_0}{p_6} \right) \\
R &= \frac{R}{M} = \frac{8314}{28.97} = 286.99 \\
\Delta k_e &= \left( \frac{200^2 - 481.67^2}{2} \right) \\
\dot{Q}_{str} &= \dot{m} \left[ 85.36 - 243.25 (-0.3) - \Delta k_e \right]
\end{align*}

``````latex