d) 
\[
n_2 u_2 - m_1 u_1 = \Delta m_2 h_2 + 35 MJ - 35 MJ
\]
\[
u_1 = h_1 - x_1 2506.5 + (1 - x_1) \cdot 418.04 \quad \text{TAB A-2}
\]
\[
= 429.38 \frac{kJ}{kg}
\]
\[
u_2 = 202.95 \frac{kJ}{kg} \quad \text{TAB A-2}
\]
\[
m_2 = 5755 kg
\]
\[
n_2 = m_1 + \Delta m_2
\]
\[
h_2 = 83.06 \frac{kJ}{kg} \quad \text{TAB A-2}
\]
\[
(m_1 + \Delta m_2) u_2 - m_1 u_1 = \Delta m_2 h_2
\]

``````latex

\begin{itemize}



\item[d)] 
    \begin{align*}
        m_1 h_2 + \Delta m_{12} h_2 - m_1 h_1 &= \Delta m_{12} h_2 \\
        \Delta m_{12} (h_2 - h_2) &= m_1 h_1 - m_1 h_2 \\
        \Delta m_{12} &= 3756.9 \, \text{kg}
    \end{align*}