d) Halboffenes System:

\begin{align*}
\Delta E &= m_2 U_2 - m_1 U_1 = \dot{m}_e h_e + \sum \dot{Q} - \sum \dot{E}_W \\
&\downarrow \\
&= 575 \frac{kg}{s} \quad \text{(TBA 4-2)} \quad p_T = 100^\circ C \quad x = 0.005 \\
&\dot{m}_e = \dot{m}_2 \\
&\text{hor. gerade siedende Flüssigkeit} \\
&\dot{m}_e = \frac{A_{TBA}}{A_{TBA 2}} \quad \frac{U_A}{U_A} = \frac{h_f(T_{in}) + x \cdot (h_{fg}(T_{in}) - h_f(T_{in}))}{h_f(T_{in})} \\
&\text{(crossed out)} \quad = 425.38 \\
&\text{TBA 2} \\
&\text{T}_{\text{ein}} = 20^\circ C \quad h_f(T_{\text{ein}}) = 83.96 \frac{kJ}{kg} \\
&U_2 = UF(T_2) = 252.55 \frac{kJ}{kg} \\
&\text{siedende Flüssigkeit bei } T_2 = 70^\circ C \\
&\text{(m_1 + \dot{m}_e t) U_2 - m_1 U_1 = \dot{m}_e h_e + \dot{Q}} \\
&\dot{m}_e U_2 - \dot{m}_e h_e = \dot{Q} + m_1 U_1 - m_1 U_2 \\
&\dot{m}_e (U_2 - h_e) = \dot{Q} + m_1 (U_1 - U_2) \quad \text{1: U_2 - h_e} \\
&\dot{m}_e = \frac{\dot{Q} + m_1 (U_1 - U_2)}{(U_2 - h_e)} = 3589.4 \frac{kg}{s}
\end{align*}

``````latex