c)
\begin{align*}
    e_{x,str}^m &= \left[ h_0 - h_0 - T_0 (s - s_0) + \frac{v_0^2}{2} \right] \\
    e_{x,str,6} &= \left[ h_6 - h_0 - T_0 (s_6 - s_0) + \frac{v_6^2}{2} \right] \\
    e_{x,str,0} &= \left[ h_0 - h_0 - T_0 (s_0 - s_0) + \frac{v_0^2}{2} \right] \\
    &= \frac{v_0^2}{2} = 20000 \frac{m^2}{s^2}
\end{align*}

``````latex

\section*{2. a1}

\begin{align*}
    \dot{E}_{x,\text{verL}} &= \dot{m} \left[ h_e - h_a - T_0 (s_e - s_a) + s \Delta e \right] + \sum_i \left( \eta_i \frac{T_0}{T_i} \right) \dot{Q}_i = e_{x,\text{verL in}} \\
    0 &= \dot{m} \left[ h_e - h_a + s \Delta e \right] + \sum_j \dot{Q}_j \\
    \Rightarrow \\
    \dot{E}_{x,\text{verL}} &= \dot{m} \left[ - T_0 (s_e - s_a) \right] + \sum_i \left( \eta_i - \frac{T_0}{T_i} \right) \dot{Q}_i - \sum_j \dot{Q}_j \\
    &= e_{x,\text{verL in}} \\
    e_{x,\text{verL}} &= - T_0 (s_e - s_a) + \frac{1}{\dot{m}} \sum_i \left( \eta_i - \frac{T_0}{T_i} \right) \dot{Q}_i - \frac{1}{\dot{m}} \sum_j \dot{Q}_j
\end{align*}

``````latex