d)

\[
\Delta E = \cancel{\Delta m_{12} (h_2 - h_1)} = 0
\]

\[
\Delta E = \Delta m_{12} \left[ h_2 - h_1 \right] - Q_{aus, 12} + \dot{Q}_{R, 12}
\]

\[
= m_2 u_2 - m_1 u_1 = (m_1 + \Delta m_{12}) u_2 - (m_1) u_1
\]

\[
\text{Values:}
\]

\[
h_1 = h_f (20^\circ C) = 83.96 \frac{KJ}{kg}
\]

\[
h_2 = h_f (70^\circ C) = 419.04 \frac{KJ}{kg}
\]

\[
u_1 = u_f (20^\circ C) = 83.95 \frac{KJ}{kg}
\]

\[
u_2 = u_f (70^\circ C) = 292.95 \frac{KJ}{kg}
\]

\[
m_1 = 5755 \, kg
\]

\[
\Delta m_{12} \ast [h_2 - h_1] = m_1 u_2 + \Delta m_{12} u_2 - m_1 u_1
\]

\[
\Delta m_{12} = \frac{m_1 u_2 - m_1 u_1}{h_2 - h_1 - u_2}
\]

\[
= 28549 \, kg
\]

``````latex


1.