\section*{Problem c}

\begin{align*}
e_{x,5\rightarrow 6} - e_{x,5\rightarrow 0} &= \dot{m} \left( h_6 - h_0 - T_0 (s_6 - s_0) + \frac{ke}{\dot{m}} \right) \\
h_6 - h_0 &= c_p (T_6 - T_0) = 1.006 \frac{kJ}{kgK} (328.07 - 30) \\
&= 83.43 \frac{kJ}{kg} \\
T_0 (s_6 - s_0) &= 293.15 K \left( c_p \ln \left( \frac{T_6}{T_0} \right) - R \ln \left( \frac{v_1}{v_0} \right) \right) \\
&= 293.15 \left( 1.006 \ln \left( \frac{328.07}{293.15} \right) \right) = 73.27 \frac{kJ}{kg} \\
\Delta e_x &= \dot{m} (85.43) \\
ke &= \frac{\omega_6^2 r^2}{2} = \frac{50^2 \cdot 2.5^2}{2} = 128857.3 \, W \\
\text{Total } \Delta E_{x,1\rightarrow 6} &= -85.139 + 73.27 + 128.65 \, (kW) \\
&= 140.82 \, kW = \Delta E_x
\end{align*}