a)

\[
\frac{d\dot{E}}{dt} = \sum \dot{m} h + \sum \dot{Q} - \sum \dot{W}
\]

\[
0 = \dot{m} (h_{\text{ein}} - h_{\text{aus}}) + \dot{Q}_R - \dot{Q}_{\text{a,w}}
\]

\[
\dot{Q}_{\text{a,w}} = Q_{\text{a,w}} \cdot \dot{m}_{\text{a}} (h_{\text{ein}} - h_{\text{aus}})
\]

\[
h_{\text{ein}} = h(70^\circ C, \text{siedende Fl.}) = h(30^\circ C, 3,1482 \text{bar}) = 232,88 \frac{\text{kJ}}{\text{kg}}
\]

\[
h_{\text{aus}} = h(100^\circ C, \text{siedende Fl.}) \Rightarrow h(100^\circ C, 1,014 \text{bar}) = 419,04 \frac{\text{kJ}}{\text{kg}}
\]

\[
\Rightarrow \dot{Q}_{\text{a,w}} = 100 + 0,3 (232,88 - 419,04)
\]

\[
\approx 62,2 \text{kW}
\]

a) 
\[
h_{n_2} = h_1(100^\circ C, x = 0.005) = h_1(100^\circ) + x \left( h_{g_2}(100^\circ) - h_1(100^\circ) \right)
\]
\[
\approx 430.3 \, \frac{\text{kJ}}{\text{kg}} \quad \text{(A-2)}
\]

\[
h_2 = h(30^\circ C, x = 0) = h_f(30^\circ) = 292.88 \, \frac{\text{kJ}}{\text{kg}} \quad \text{(A-2)}
\]

\[
h_{en_{12}} = h(20^\circ C, x = 0) = h_f(20^\circ) = 83.96 \, \frac{\text{kJ}}{\text{kg}} \quad \text{(A-2)}
\]

\[
\Rightarrow \Delta h_{12} = \frac{535}{83.96} \left( 292.88 - 430.3 \right) \frac{1}{1 - 83.96}
\]

\[
\approx 109.5 \, \text{kJ}
\]