

\section*{d)}

\[
\frac{dE}{dt} = \sum \dot{m} \cdot h + \sum \dot{Q} - \sum \dot{V}
\]

\[
\Delta U = \Delta m_{12} \cdot h_{ein_{12}} + Q_{er} - Q_{aus}
\]

\[
\Delta U = \Delta m_{12} \cdot h_{ein_{12}}
\]

\[
\Delta m_{12} \cdot \frac{\Delta U}{h_{ein_{12}}} = \frac{(m_1 + \Delta m_{12}) h_2}{h_{ein_{12}}} - \frac{m_1 h_1}{h_{ein_{12}}}
\]

\[
\Delta m_{12} - \Delta m_{12} = \frac{m_1 h_2}{h_{ein_{12}}} - \frac{m_1 h_1}{h_{ein_{12}}}
\]

\[
\Delta m_{12} \left( 1 - \frac{1}{h_{ein_{12}}} \right) = \frac{m_1}{h_{ein_{12}}} (h_2 - h_1)
\]

\[
\Rightarrow \Delta m = \frac{m_1}{h_{ein_{12}}} (h_2 - h_1) \cdot \frac{1}{1 - h_{ein_{12}}}
\]

``````latex


1.