\section*{Problem c)}

\begin{align*}
    \Delta e_{x,s} &= E_{x,s,in} - E_{x,s,out} \\
    &= \dot{m}_{\text{ges}} \left( h_{0} - h_{0} - T_{0}(S_{e} - S_{0}) + \frac{w_{0}^2}{2} \right) - \dot{m}_{\text{ges}} \left( h_{0} - h_{0} - T_{0}(S_{0} - S_{0}) + \frac{w_{0}^2}{2} \right) \\
    &= \dot{m}_{\text{ges}} \left( h_{0} - h_{0} - T_{0}(S_{e} - S_{0}) + \frac{w_{0}^2}{2} - \frac{w_{0}^2}{2} \right)
\end{align*}

\begin{align*}
    \dot{m}_{\text{ges}} \cdot c_{p} \cdot T_{0} &= 350 \frac{\text{kJ}}{\text{kg}} \\
    h_{0} &= h_{0} - h_{0} = c_{p}(T_{0} - T_{0}) = 8.5 \text{V} \cdot 85.03 \frac{\text{kJ}}{\text{kg}}
\end{align*}

\begin{align*}
    T_{0} &= 293.15 \text{K} \\
    S_{e} - S_{0} &= c_{p} \ln \left( \frac{T_{0}}{T_{0}} \right) - R \left( \frac{P_{0}}{P_{0}} \right) \\
    &= c_{p} \ln \left( \frac{T_{0}}{T_{0}} \right) = 0.307 \frac{\text{kJ}}{\text{kg} \cdot \text{K}}
\end{align*}

\begin{align*}
    \Delta e_{x,s} &= \dot{m}_{\text{ges}} \left( c_{p}(T_{0} - T_{0}) - T_{0} \ln \left( \frac{T_{0}}{T_{0}} \right) + \frac{w_{0}^2}{2} - \frac{w_{0}^2}{2} \right)
\end{align*}

\begin{align*}
    \Delta e_{x,s} &= 56.25 \cdot \dot{m}_{\text{ges}} \frac{\text{kJ}}{\text{kg}}
\end{align*}

``````latex