c) $\Delta e_{x,str} = e_{x,str,6} - e_{x,str,0} = ?$

\[
\Delta e_{x,str,6} = \Delta h_{0G} - T_0 (s_6 - s_0) + \Delta \frac{\omega^2_6 - \omega^2_0}{2}
\]

\[
\Delta h_{0G} = \int_{T_0}^{T_6} c_p dT = c_p (T_6 - T_0) = 360 \frac{J}{kgK} (273,15 K - 288,15 K) = -5400 \frac{J}{kg}
\]

\[
\Delta s_{60} = \int_{T_0}^{T_6} \frac{c_p}{T} dT - R \ln \left( \frac{p_6}{p_0} \right) = c_p \left( \ln(T_6) - \ln(T_0) \right) - R \ln \left( \frac{p_6}{p_0} \right)
\]

\[
= 360 \frac{J}{kgK} \left( \ln(288,15 K) - \ln(273,15 K) \right) - 287 \frac{J}{kgK} \ln \left( \frac{1}{1} \right) = 6,30135 \frac{J}{kgK}
\]

\[
\Delta \frac{\omega^2_6 - \omega^2_0}{2} = \frac{\omega^2_6 - \omega^2_0}{2} = 102,648 \frac{J}{kg}
\]

\[
\Rightarrow \Delta e_{x,str} = \Delta h - T_0 \Delta s + \Delta \frac{\omega^2}{2} = 118,426 \frac{J}{kg}
\]

``````latex