a) $p_{g1,1} = p_{amb} + \frac{A_u \cdot m \cdot g}{A_u} = p_{amb} + \frac{m \cdot g}{A_u}$

\[
A_u = \pi \left(\frac{d}{2}\right)^2 = \pi \left(0.05 \, \text{m}\right)^2 = 0.0078 \, \text{m}^2
\]

\[
p = \frac{F}{A} \quad \Rightarrow \quad F = pA
\]

\[
p_{g1,1} = p_{amb} + \frac{m \cdot g}{A_u} = 1.05 \, \text{Pa} + \frac{32 \, \text{kg} \cdot 9.81 \, \frac{\text{m}}{\text{s}^2}}{0.0078 \, \text{m}^2} = 1.4 \, \text{bar}
\]

\[
p_{g1,1} = 1.3886 \, \text{bar} \approx 1.4 \, \text{bar}
\]

\[
pV = mRT \quad \Rightarrow \quad \frac{p_{g1,1} \cdot V_1}{R_g \cdot T_1} = \frac{p_{g1,2} \cdot V_1}{R_g \cdot T_2}
\]

\[
m_g = \frac{3 \, \text{mol}}{1 \, \text{mol}} = 3 \, \text{mol}
\]

\[
m_g = 3.42 \, \text{g}
\]