

\subsection*{d)}

\[
e_k = \frac{1}{\dot{Q}_{k1}} \left| \dot{Q}_{k2} - \dot{Q}_{k1} \right|
\]

\[
\text{Ãœbergang 1,4,3 \quad 3} \rightarrow 4:
\]

\[
Q = m_2 (h_{2,g} - h_{2,f}) + \dot{Q}_{ab}
\]

\[
\dot{Q}_{k2} = m_3 (h_{3,g} - h_{3,f})
\]

\[
h_{2,g} - h_{2,f} \left( 5 \text{ bar} \right) = (3.42 \frac{\text{kJ}}{\text{kg}})
\]

\[
T_{43}
\]

\[
4 \rightarrow 1
\]

\[
h_{2,g} = h_{2,f} + x_{2} (h_{2,g} - h_{2,f}) \quad (5 \text{ bar})
\]

\[
x_2 = \frac{s_2 - s_{2,f}}{s_{2,g} - s_{2,f}} \quad (5 \text{ bar})
\]

\[
s_{2,g} = s_{2,f}
\]

\[
h_{2,g} = h_{2,f} + x_{2} (h_{2,g} - h_{2,f}) \quad (5 \text{ bar})
\]

```