

\section*{d)}

\[
T_{x_2} = 90^\circ C
\]

\textbf{1HS:}
\[
\Delta U_{x_1 BW} = Q - W = (7,36c\dot{2} - 0,2852) \, kJ = 7,0748 \, kJ
\]

\[
\Delta U_{x_2} = m_{BW} (u_2 - u_1)
\]

\[
u_2 = \frac{1 - x_2}{v_f (0,0931 \, c)} + \frac{x_2}{v_f (0,201 \, c)}
\]

\[
u_1 = v_f (0^\circ C) (1 - x_1) + v_f (0^\circ C) x_1, \quad x_1 = 0,16
\]

\[
m_{BW} (u_2 - u_1) = x_2 (u_f (T_x) - u_f (T_1)) + u_f (T_1) - u_1 = \Delta u_{x_2}
\]

\[
x_2 = \frac{\Delta u_{x_2} + u_f (T_1) - u_f (T_x)}{u_f (T_x) - u_f (T_1)}
\]

\[
x = \frac{7,0748 \, kJ}{0,1 \, kg} = \frac{(-0,085 \, \frac{kJ}{kg}) \cdot 0,1 + (-333,652 \, \frac{kJ}{kg}) \cdot 0,6 - (-0,053 \, \frac{kJ}{kg})}{-333,652 \, \frac{kJ}{kg} - (-0,053 \, \frac{kJ}{kg})}
\]

\[
= 0,575
\]

``````latex