

\subsection*{b)}

\begin{align*}
    \text{Energiegleichung am Verdichter:} \quad & 0 = \dot{m} (h_{2} - h_{1}) - \dot{W}_{\text{K}} \\
    \dot{m} = \quad & \frac{\dot{W}_{\text{K}}}{h_{2} - h_{1}}
\end{align*}

\begin{itemize}
    \item $h_{2} + h_{2} = h_{g} (22^{\circ}C) \quad \text{no Interpolation}$
    \item $h_{2} = h_{g} = h_{g} (6 \text{bar}) = 261,15 \frac{\text{kJ}}{\text{kg}}$
    \item $h_{2} (22^{\circ}C) = h_{g} (0^{\circ}C) + \frac{h_{g} (2^{\circ}C) - h_{g} (0^{\circ}C)}{2 - 0}$
    \item $= 268,38 \frac{\text{kJ}}{\text{kg}} \quad h_{g} = 268,38 \quad \& \quad 269,23 \quad \& \quad 285,57 \frac{\text{kJ}}{\text{kg}}$
\end{itemize}

\begin{align*}
    \dot{m} = \quad & \frac{2,8 \frac{\text{kJ}}{\text{s}}}{(268,38 - 261,15) \frac{\text{kJ}}{\text{kg}}} \\
    = \quad & 1,2099 \cdot 10^{-3} \frac{\text{kJ}}{\text{kg}} \frac{\text{kg}}{\text{s}}
\end{align*}

``````latex


\begin{itemize}