

\section*{2c)}

\begin{align*}
    \omega_6 &= 510 \frac{m}{s} \\
    T_6 &= 370 \mu
\end{align*}

\begin{align*}
    h - h_0 - T_0 (s - s_0) + ke
\end{align*}

\begin{align*}
    h_6 - h_e - T_0 (s_6 - s_e) + \dot{m} ke
\end{align*}

\begin{align*}
    \Rightarrow \Delta e_{x,sth} &= h_6 - h_0 - T_0 (s_6 - s_0) + \frac{\omega_6^2 - \omega_0^2}{2}
\end{align*}

\begin{align*}
    h_6 - h_0 &= C_p (T_6 - T_0)
\end{align*}

\begin{align*}
    s_6 - s_0 &= C_p \ln \left( \frac{T_6}{T_0} \right) - R \ln \left( \frac{p_6}{p_0} \right)
\end{align*}

\begin{align*}
    \Delta e_{x,sth} &= C_p (T_6 - T_0) + T_0 C_p \ln \left( \frac{T_6}{T_0} \right) + \frac{\omega_6^2 - \omega_0^2}{2} = 
\end{align*}

``````latex