

\section*{c)}

\[
\Delta \dot{E}_{x,sis} = \Delta \dot{E}_{x,siro}
\]

\[
\Delta \dot{E}_{x,sir} = \dot{m}_{gs} \left( h_6 - h_0 - T_0 (s_6 - s_0) + \frac{\omega_6^2}{2} \right) - \dot{m}_{gs} \left( h_0 - h_0 - T_0 (s_5 - s_0) + \frac{\omega_5^2}{2} \right)
\]

\[
= \dot{m}_{gs} \left( h_6 - h_0 - T_0 (s_6 - s_0) + \frac{\omega_6^2}{2} - \frac{\omega_5^2}{2} \right) \quad \text{Stoffmeckell:}
\]

\[
h_6 - h_0 = c_p (T_6 - T_0) \quad s_6 - s_0 = c_p \ln \left( \frac{T_6}{T_0} \right) \quad \ln(1) = 0
\]

\[
\Delta \dot{e}_{x,sir} = \frac{\dot{E}_{x,sir}}{\dot{m}_{gs}} = c_p (T_6 - T_0) - T_0 \left( c_p \ln \left( \frac{T_6}{T_0} \right) - \frac{\omega_6^2 - \omega_5^2}{2} \right)
\]

\[
= 1,006 \frac{\text{kJ}}{\text{kgK}} (T_6 - T_0) - 1,006 \cdot 10^3 \frac{\text{J}}{\text{kg}} T_0 \ln \left( \frac{T_6}{T_0} \right) - \frac{\omega_6^2 - \omega_5^2}{2}
\]

\[
= 37,551,579 \frac{\text{J}}{\text{kg}} - 37,551 \frac{\text{kJ}}{\text{kg}} = 37,551 \frac{\text{kJ}}{\text{kg}} = \Delta \dot{e}_{x,sir}
\]