\section*{e) Halboffen}

\begin{align*}
    M_{S2} - M_{S1} &= \Delta M \cdot S_{\text{ein}} + \frac{Q_{\text{ein}}}{T} - S_{\text{ez}} \\
    S_{\text{ez}} &= M_{S2} - M_{S1} + \Delta M \cdot S_{\text{ein}} - \frac{Q_{\text{ein}}}{T}
\end{align*}

\begin{align*}
    S_{\text{ez}} &= 1012.428 \text{kJ}
\end{align*}

\begin{align*}
    M_2 &= m_1 + m_2 = 9355 \text{kg} \\
    \Delta M_2 &= 3600 \\
    M_2 &= M_1 + S_2 \\
    M_1 &= M_A \\
    S_2 &= S_p(70^\circ) = 0.9549 \frac{\text{kJ}}{\text{kg}} \\
    S_1 &= S_p(100^\circ) + x \left( S_f(100^\circ) - S_p(100^\circ) \right) \\
    \Delta 2 &= 1.3063 + x \left( 7.3540 - 1.3063 \right) \\
    S_2 &= 4.339 \frac{\text{kJ}}{\text{kg}} \\
    S_{\text{ein}} &= S_p(70^\circ) = 0.2966 \\
    Q &= 35 \cdot 10^3 \text{kJ} \\
    T &= 255 K
\end{align*}

``````latex