a) 
\begin{align*}
0 &= \dot{m} \cdot h_{\text{ein}} - \dot{m} \cdot h_{\text{aus}} + 100 \text{kW} - \dot{Q}_{\text{aus}} - \dot{W} \\
\dot{Q}_{\text{aus}} &= \dot{m} \cdot h_{\text{ein}} - \dot{m} \cdot h_{\text{aus}} + \dot{Q}_R
\end{align*}

\text{TAB A2}
\begin{align*}
h_{\text{ein}} &= h_f (70^\circ \text{C}) = 292,88 \frac{\text{kJ}}{\text{kg}} \\
h_{\text{aus}} &= h_f (100^\circ \text{C}) = 419,64 \frac{\text{kJ}}{\text{kg}} \\
\dot{m}_{\text{ein}} &= 0,3 \frac{\text{kg}}{\text{s}} \\
\dot{m}_{\text{aus}} &= 0,3 \frac{\text{kg}}{\text{s}} - \dot{m}_{\text{ein}}
\end{align*}

\begin{align*}
\Rightarrow \dot{Q}_{\text{aus}} &= \dot{m} (h_{\text{ein}} - h_{\text{aus}}) + 100 \text{kW} \\
\dot{Q}_{\text{aus}} &= 62,182 \text{kW}
\end{align*}

\section*{a) Halboffenes System}

\begin{align*}
    M_2 U_2 - M_1 U_1 &= \Delta M \cdot h_{\text{ein}} + Q - CW \\
    M_1 &= M_{\text{ges}} \\
    Q &= Q_{\text{aus}} = 835 \text{MJ} \\
    M_2 &= m_{\text{ges}} + m_B \\
    (m_g + m_B) U_2 - m_g U_1 &= \Delta M \cdot h_{\text{ein}} + (-Q_{\text{aus}}) \\
    m_g U_2 + m_B U_2 - m_g U_1 &= \Delta m h + (x) \\
    \Delta m \left( \frac{U_2 - h_{\text{ein}}}{U_2 - h_{\text{ein}}} \right) &= m_g U_1 + (x) \\
    \Delta m &= \frac{M_{\text{ges}} h_{\text{ein}} + Q}{U_2 - h_{\text{ein}}}
\end{align*}

\begin{align*}
    h_{\text{ein}} &= h_f(100^\circ) - h_f(20^\circ) \\
    h_{\text{ein}} &= h_f(20^\circ) = 83.36 \frac{\text{kJ}}{\text{kg}}
\end{align*}

\begin{align*}
    M_{\text{ges}} &= 5755 \text{kg}
\end{align*}

\begin{align*}
    \Delta m &= \frac{5755 \text{kg} \cdot 418.94 \frac{\text{kJ}}{\text{kg}} - 835 \cdot 10^3 \text{kJ}}{292.35 - 83.36}
\end{align*}

\begin{align*}
    \Delta m &= 11368.9 \text{kg}
\end{align*}