d) 
\[
\dot{e}_{x1} \frac{d \dot{E}_x}{dt} = \dot{E}_{x1,dir} + \dot{E}_{x1,Q} - \left[ \dot{V}_u \left( e_0 - \frac{\Delta U(t)}{dt} \right) \right] = \dot{E}_{x1,vel}
\]

\[
\Rightarrow \dot{e}_{x1,vel} = \dot{e}_{x1,dir} + \dot{e}_{x1,Q}
\]

\[
\dot{e}_{x1,Q} = \frac{\dot{E}_{x1,Q}}{\dot{m}} = \frac{1}{\dot{m}} \left( 1 - \frac{T_0}{T} \right) \cdot \dot{Q} = \left( 1 - \frac{T_0}{T} \right) q \cdot y
\]

\[
q = 1785 \frac{kJ}{kg} \quad T = 1725 K
\]

\[
\dot{e}_{x1,vel} = 116.60 \frac{kJ}{kg} + \left( 869.58 \cdot \frac{1}{6.293} \right) \frac{kJ}{kg}
\]

\[
= \underline{270.67 \frac{kJ}{kg}}
\]

\[
y \text{inges} = \dot{m}
\]

\[
\dot{m}_{inges} = \dot{m}_K + 5.253 \dot{m}_K
\]

\[
\dot{m}_K = \frac{\dot{m}}{6.293} \text{ inges}
\]

``````latex