

\subsection*{a)}

\begin{equation*}
O = \dot{m}_{ein} (h_{ein} - h_{aus}) + \dot{Q}_R - \dot{Q}_{aw} - \dot{W}^0
\end{equation*}

\begin{equation*}
\dot{m}_{ein} = \dot{m}_{aus} = \dot{m}
\end{equation*}

station√§rer Fallprozess

\begin{equation*}
\Rightarrow \dot{Q}_{aw} = \dot{m} (h_{ein} - h_{aus}) + \dot{Q}_R
\end{equation*}

\begin{equation*}
\dot{Q}_{aw} = 0,3 \frac{\text{kg}}{\text{s}} (293,88 \frac{\text{kJ}}{\text{kg}} - 930,12 \frac{\text{kJ}}{\text{kg}}) + 100 \text{kW} = \underline{58,86 \text{kW}}
\end{equation*}

\begin{equation*}
h_{ein} = h_f \left( 70^\circ \text{C} \right) = 292,88 \frac{\text{kJ}}{\text{kg}}
\end{equation*}

\begin{equation*}
X_D = \frac{h_{aus} - h_f}{h_g - h_f} \quad \text{bei} \quad T = 100^\circ \text{C}
\end{equation*}

\begin{equation*}
\Rightarrow h_{aus} = h_f + X_D (h_g - h_f) = 419,06 \frac{\text{kJ}}{\text{kg}} + 0,005 (2631,3 - 419,06) \frac{\text{kJ}}{\text{kg}} = 930,12 \frac{\text{kJ}}{\text{kg}}
\end{equation*}



\subsection*{a)}

\[
S_{\text{en}} = S_f(T=70^\circ C) = 0{,}9549 \frac{\text{kJ}}{\text{kg K}}
\]

\[
\dot{S}_{\text{ev}} = \frac{58{,}86 \text{kW}}{293{,}15 \text{K}} + 0{,}3 \frac{\text{kg}}{\text{s}} \left(1{,}3379 \frac{\text{kJ}}{\text{kg K}} - 0{,}9549 \frac{\text{kJ}}{\text{kg K}}\right) = \frac{100 \text{kW}}{371{,}15 \text{K}}
\]

\[
= 0{,}096 \frac{\text{kW}}{\text{K}}
\]