

\subsection*{c)}

\textbf{Entropiebilanz:}

\begin{equation*}
0 = \dot{m} (s_{ein} - s_{aus}) + \frac{\dot{Q}_R}{T_{Trenn,1}} - \frac{\dot{Q}_{aw}}{T_{KF}} + \dot{S}_{erz}
\end{equation*}

\begin{equation*}
\Rightarrow \dot{S}_{erz} = \frac{\dot{Q}_{aw}}{T_{KF}} + \dot{m} \left( s_{ein} - s_{aus,ein} \right) - \frac{\dot{Q}_R}{T_{Trenn,1}}
\end{equation*}

\begin{equation*}
s_{aus} = s_f + X_D (s_g - s_f) = 1,3069 \frac{\text{kJ}}{\text{kg} \cdot \text{K}} + 0,005 (7,3589 - 1,3069) \frac{\text{kJ}}{\text{kg} \cdot \text{K}} = 1,3374 \frac{\text{kJ}}{\text{kg} \cdot \text{K}}
\end{equation*}

``````latex


\section*{Student Solution}