

\subsection*{d)}

\begin{align*}
e_{x,\text{verl}} &= \frac{\dot{E}_{x,\text{verl}}}{\dot{m}_{ges}} = T_0 \dot{S}_{e, \text{verl}} \\
\end{align*}

\text{Entropiebilanz:} \quad 0 = \dot{m}_g s_0 - \dot{m}_k s_6 + \frac{\dot{Q}}{T_0} + \dot{S}_{e, \text{verl}}

\begin{align*}
\dot{S}_{e, \text{verl}} &= \frac{\dot{m}_g}{\dot{m}_{ges}} s_0 - s_0 \\
&= \\
\end{align*}

\text{Massenstrombilanz am Verdichter:} \quad \dot{m}_g (h_0 - h_{ns}) = \dot{m}_k (h_0 - h_1)

\begin{align*}
\Rightarrow \eta_{ns} &= \frac{h_0 - h_{ns}}{h_0 - h_1} = \frac{\dot{m}_g}{\dot{m}_k}
\end{align*}