

\item[d)] $m_2 u_2 - m_4 u_4 = \Delta m h_{ein} + Q_{2 \rightarrow 4} = 0$
    
    \[
    (m_1 + \Delta m) u_2 - m_1 u_1 = \Delta m h_{ein}
    \]
    
    \[
    u_2 = 292.35 \frac{\text{kJ}}{\text{kg}} \quad \text{(A-2)}
    \]
    
    \[
    u_1 = 918.99 \frac{\text{kJ}}{\text{kg}} \quad (2566.5 \frac{\text{kJ}}{\text{kg}} - 918.99 \frac{\text{kJ}}{\text{kg}}) = 929.3778 \frac{\text{kJ}}{\text{kg}}
    \]
    
    \[
    h_{ein} = 83.06 \frac{\text{kJ}}{\text{kg}} \quad \text{(A-2)}
    \]
    
    \[
    \Delta m_{ein} = \frac{m_4 u_4 - m_2 u_2}{u_2 - h_{ein}} = \cancel{\frac{0}{0}} = 3756.889 \, \text{kg}
    \]