c) 
\begin{align*}
\Delta e_{x,str} &= \left[ (h_6 - h_6 - T_0 (s_6 - s_6) + \frac{w_6^2 - w_0^2}{2} \right] \\
h_6 - h_6 &= c_p (T_0 - T_6) = -85.43 \frac{kJ}{kg} \\
s_6 - s_6 &= c_p \ln \left( \frac{T_0}{T_6} - R \left( \frac{p_0}{p_6} \right) \right) = -0.3013 \frac{kJ}{kgK} \\
\frac{w_6^2 - w_0^2}{2} &= -108.64 \frac{kJ}{kg} \\
\Delta e_{x,str} &= \underline{-96.187 \frac{kJ}{kg}}
\end{align*}

d1)
\begin{align*}
0 &= -\Delta e_{x,str} + \left( 1 - \frac{T_0}{T} \right) \frac{\dot{Q}}{\dot{m}_{ges}} - \frac{\dot{W}}{\dot{m}_{ges}} - e_{x,vel} \quad \text{(Aus Hinweis)} \\
\left( 1 - \frac{T_0}{T} \right) \frac{\dot{Q}}{\dot{m}_{ges}} &= 159.073 \frac{kJ}{kg} \\
\frac{\dot{Q}}{\dot{m}_{ges}} &= \frac{159.073}{1} = 159.073 \frac{kJ}{kg} \\
\dot{m}_{ges} &= 6.293 \\
\dot{m}_k &= \dot{m}_{ges} - \dot{m}_k = 5.293 \\
\dot{m}_k &= \dot{m}_{ges} \left( \frac{1}{5.293 + 1} \right) = \frac{\dot{m}_{ges}}{6.293}
\end{align*}

\begin{align*}
e_{x,vel} &= -\Delta e_{x,str} + \left( 1 - \frac{T_0}{T} \right) \frac{\dot{Q}}{\dot{m}_{ges}} = 250.286 \frac{kJ}{kg} \\
&= \underline{57.886 \frac{kJ}{kg}}
\end{align*}

``````latex