

\item[e)] $\Delta S = m_2 s_2 - m_1 s_1$
    
    \[
    s_1 = 1.3069 \frac{\text{kJ}}{\text{kg K}} + x_0 (7.3550 \frac{\text{kJ}}{\text{kg K}} - 1.3069 \frac{\text{kJ}}{\text{kg K}}) = 1.337 \frac{\text{kJ}}{\text{kg K}}
    \]
    
    \[
    s_2 = 0.359 \frac{\text{kJ}}{\text{kg K}} \quad \text{(A-2)}
    \]
    
    \[
    \Delta S = (m_1 + \Delta m_2) s_2 - m_1 s_1 = \cancel{\frac{0}{0}} = 1388.921 \frac{\text{kJ}}{\text{K}}
    \]
    
    \[
    \text{(Es könnte sein, dass die Lösung falsch ist.)}
    \]
    
\end{itemize}

``````latex