

\subsection*{b)}

\[
\dot{m}_{\text{Re}} = \dot{m}_{\text{Ra}}
\]

\[
0 = -\dot{s}_{\text{in}} - \dot{V}_0 + Q \geq 0
\]

\[
h_2 = \frac{h_1}{2}
\]

\[
h_4 = 52, \quad h_2 \quad \left( \frac{W}{s} \right)
\]

\[
h_4 = 32.75 \quad \left( \frac{W}{s} \right)
\]

\[
h_2 = h_2(-16^\circ C)
\]

\[
s_2 = s_2 - 0.0258 \frac{h_2}{s_k}
\]

\[
\frac{A}{10} = 237.7 \left( \frac{T}{s} \right)
\]

\[
(2.3)
\]

\[
p_2 = 1 \text{bar}
\]

\[
T_i = -10^\circ C
\]

\[
T_i = -10^\circ C
\]

``````latex


\[
A_{u}(s) = const
\]

\[
\begin{array}{ccc}
A_{12} & y_{sat} \\
1 & F_{sat}
\end{array}
\]

\[
\frac{S - S_{sat}(y_{b})}{S_{sat}(y_{a}) - S_{sat}(y_{b})} \cdot \left( h_{S}(s_{a}) - h_{u}(s) \right) - h_{u}(s)
\]

\[
t_{3} = 27,31
\]

\[
\dot{U}_{u} = \dot{m}_{E} (h_{2} - h_{3})
\]

\[
\dot{m}_{E} = \frac{\dot{m}_{u} - \dot{U}_{u}}{h_{2} - h_{3}} - 9.8 \frac{kg}{s}
\]