

\item[a)] 
    \begin{equation}
    \frac{dE}{dt} = \dot{m} (h_{\text{ein}} - h_{\text{aus}}) + \dot{Q} - \dot{W}^{\text{o}}
    \end{equation}
    \begin{equation}
    \dot{Q} = \dot{m} (h_{\text{aus}} - h_{\text{ein}})
    \end{equation}
    \begin{equation}
    = 0
    \end{equation}
    \begin{equation}
    h_{\text{aus}} = 449.09 \frac{\text{kJ}}{\text{kg}} \quad h_{\text{ein}} = 292.88 \frac{\text{kJ}}{\text{kg}}
    \end{equation}
    \begin{equation}
    T = 293.12 \text{K}
    \end{equation}