

\item[b)] \textbf{Energiebilanz um ganzes Triebwerk}
        \begin{align*}
            \frac{d\dot{E}}{dt} &= \dot{m} (\dot{h}_{\text{ein}} - \dot{h}_{\text{aus}} + \frac{1}{2} w_{0}^2 - \frac{1}{2} w_{6}^2) \\
            0 &= c_p (T_0 - T_6) + \frac{1}{2} w_{0}^2 - \frac{1}{2} w_{6}^2
        \end{align*}
        \begin{equation*}
            h_{\text{ein}} - h_{\text{aus}} = c_p (T_0 - T_6)
        \end{equation*}
        
        \textbf{Energiebilanz um Schubd√ºse}
        \begin{align*}
            0 &= c_p (T_5 - T_6) + \frac{1}{2} w_{6}^2 - \frac{1}{2} w_{6}^2 \\
            0 &= c_p (T_0 - T_6) + \frac{1}{2} w_{0}^2 = c_p (T_5 - T_6) + \frac{1}{2} w_{6}^2
        \end{align*}