

\section*{d)}

\textbf{7. HS im Reaktionsgemisch, halboffenen System}

\[
\Delta E = m_2 U_2 - m_1 U_1 + \cancel{ \Delta KE + \Delta PE } = \Delta m_{\text{ein}} h_{\text{ein}} + \cancel{Q_{\text{out}} - Q_{\text{in}}}
\]

\[
\Delta m_{\text{ein}} = m_2 - m_1 \quad \Rightarrow \quad m_2 = m_1 + \Delta m_{\text{ein}}
\]

\[
\Delta m_{\text{ein}} = \frac{( \Delta m + m_1 ) U_2 - m_1 U_1}{h_{\text{ein}} - U_2}
\]

\[
\Delta m_{\text{ein}} = \frac{m_2 U_2 - m_1 U_1}{h_{\text{ein}} - U_2} = m_1 \frac{U_2 - U_1}{h_{\text{ein}} - U_2}
\]

\[
\Delta m = 3 \, 469,69 \, \text{kg}
\]

\[
\begin{aligned}
    m_1 &= m_{\text{ges}} = 5755 \, \text{kg} \\
    \text{TAB A-2:} \\
    h_{\text{ein}} &= h_f (20^\circ \text{C}) = 83,96 \, \frac{\text{kJ}}{\text{kg}} \\
    U_2 &= U_f (70^\circ \text{C}) = 222,87 \, \frac{\text{kJ}}{\text{kg}} \\
    U_1 &= U_f (70^\circ \text{C}) = 418,94 \, \frac{\text{kJ}}{\text{kg}}
\end{aligned}
\]