\section*{c) Entropiebilanz am Reaktor}

\[
Q = \dot{m} (S_{e2} - S_{e1}) + \frac{\dot{Q}}{T} + S_{erz}
\]

\[
= \dot{m} (S_{ein} - S_{aus}) + \frac{\dot{Q}_{aus}}{T_{KW}} + S_{erz}
\]

\[
S_{erz} = \dot{m} (S_{aus} - S_{ein}) + \frac{Q_{aus}}{T_{KW}} = \underline{0.317 \, \text{kW}} = S_{erz}
\]

\[
S_{aus} = x_{aus} S_g + (1 - x_{aus}) S_f \quad \text{aus TAB A-2}
\]

\[
= 1.33714 \, \frac{\text{kJ}}{\text{kgK}}
\]

\[
S_{ein} = x_{ein} S_g + (1 - x_{ein}) S_f \quad \text{aus TAB A-2}
\]

\[
= 0.888902 \, \frac{\text{kJ}}{\text{kgK}}
\]