

\section*{d)}

\[
\Delta E = Q - \dot{W}
\]

\[
-m_{ges} U_1 + (m_{ges} + \Delta m_{12}) U_2 = Q_{aus, 12}
\]

\[
m_{ges} (U_2 - U_1) + \Delta m_{12} U_2 = Q_{aus, 12}
\]

\[
\Delta m_{12} = \frac{Q_{aus} + m_{ges} (U_1 - U_2)}{U_2} = \underline{2793.5971 \, \text{kg}}
\]

\[
U_1 = x_0 \cdot U_g + (1 - x_0) U_f \quad \text{aus TAB A-2}
\]

\[
= 428.3778 \, \frac{\text{kJ}}{\text{kg}}
\]

\[
U_2 = 282.55 \, \frac{\text{kJ}}{\text{kg}} \quad \text{aus TAB A-2}
\]

\[
x_{sieden} = 0
\]

``````latex