\subsection*{b) aus der Entropiebilanz}

\[
0 = \dot{m} (s_e - s_a) + \sum_j \frac{\dot{Q}_j}{T_j} + \dot{S}_{\text{erzeugt}}
\]

\subsubsection*{aus der Exergiebilanz}

\[
0 = \dot{m} (h_e - h_a) + \left( 1 - \frac{T_0}{T} \right) \dot{Q} = 0
\]

\[
\frac{T_0}{T} = \frac{\dot{m} (h_e - h_a)}{\dot{m} (s_e - s_a)} = \frac{C_v (T_{\text{ein}} - T_{\text{aus}})}{C_v \ln \left( \frac{T_{\text{ein}}}{T_{\text{aus}}} \right)}
\]

\[
= \frac{(288.15 - 298.15) \, \text{K}}{\ln \left( \frac{288.15 \, \text{K}}{298.15 \, \text{K}} \right)} = 293.12 \, \text{K}
\]

``````latex