c) \quad \dot{Q}_{\text{aus}} = 65 \, \text{kW}, \quad \overline{T}_{\text{KF}} = 298 \, \text{K}

\text{aus der Entropiebilanz:}
\[
0 = \dot{m} \, (s_e - s_a) + \sum_j \frac{\dot{Q}_j}{T_j} + \dot{S}_{\text{erz}}
\]

\[
\dot{S}_{\text{erz}} = \dot{m} \, (s_e - s_a) - \frac{\dot{Q}_j}{298 \, \text{K}}
\]

\text{aus der TAB A-2:}
\[
s_e = s_f (15^\circ \text{C}) = 62.99 \, \frac{\text{kJ}}{\text{kg} \cdot \text{K}}
\]
\[
s_a = s_f (250^\circ \text{C}) = 104.88 \, \frac{\text{kJ}}{\text{kg} \cdot \text{K}}
\]

\[
\dot{S}_{\text{erz}} = 0.3 \, \frac{\text{kg}}{\text{s}} \cdot (62.99 - 104.88) \, \frac{\text{kJ}}{\text{kg} \cdot \text{K}} - \frac{65 \, \text{kW}}{298 \, \text{K}}
\]
\[
= -12.79 \, \frac{\text{kW}}{\text{K}}
\]