b) \quad \dot{m}_s = \dot{m}_b \quad \text{stationär reversibel} \\
\Rightarrow s_s = s_b \Rightarrow \text{können polytropen Kompression} \\
\Rightarrow n = k = 1.4 \\

\frac{T_0}{T_s} = \left( \frac{p_0}{p_s} \right)^{\frac{n-1}{n}} \quad T_b = T_s \left( \frac{p_b}{p_s} \right)^{\frac{n-1}{n}} = 328.1 \, K \\

\text{für} \quad W_b \quad \text{und} \quad h_s \quad \text{ist} \quad s_b \\

0 = \dot{m} h_{es} \left[ h_s - h_{s_i} + \frac{v_s^2 - v_b^2}{2} \right] + \dot{Q} \quad \text{adiab} \quad 0-\text{weise} \\

h_s - h_{b} = \int_{T_b}^{T_s} c_p \, dT = c_p (T_s - T_b) \\

0 = h_s - h_b + \frac{v_s^2 - v_b^2}{2} = c_p (T_s - T_b) + \frac{v_s^2 - v_b^2}{2} \\

c_p (T_b - T_s) 2 = v_s^2 - v_b^2 \quad \Rightarrow \quad v_b = 390.93 \, \frac{m}{s} \\

\text{(d) C)} \quad e_{s + str} = [h_b - h_0 - \dot{p} (s - s_0)] \quad \text{KE} \\

e_{s + str_2} - e_{s + str_2} = h_b - h_0 - \dot{p} (s - s_0) \quad \text{KE} \\

\left( h_b - h_0 = \int_{T_0}^{T_b} c_p \, dT = c_v (T_b - T_0) = 41.08 \, \frac{kJ}{kg} \right) \quad \text{es geht} \\

n = k = \frac{c_p}{c_v} \quad \leftarrow c_v = \frac{c_p}{k} = 0.419 \, \frac{kJ}{kg \cdot K} \quad p_1 = p_0 \quad \text{ln(1)} = 0 \\

s_b - s_0 = \int_{T_0}^{T_b} \frac{c_p}{T} \, dT - R \ln \left( \frac{p_b}{p_0} \right) = c_p \ln \left( \frac{T_b}{T_0} \right) - R \ln \left( \frac{p_b}{p_0} \right) \\

\left( v_b - v_0 = \int_{T_0}^{T_b} \frac{c_p}{T} \, dT = c_v (T_b - T_0) = 41.08 \, \frac{kJ}{kg} \right) \quad \text{es geht} \\

v_b - v_0 \quad pv = RT \quad v = \frac{RT}{p} \quad R = \frac{R}{M} \quad c_p - c_v = 0.28 \, \frac{kJ}{kg \cdot K} \quad - 28 \, \frac{J}{kg \cdot K} \\

v_b - \frac{R T_b}{p_b} = 7.93 \, \frac{m^2}{kg}
``````latex


\section*{Handwritten Student Solution}

\subsection*{Aufgabe 2