

\section*{d)}
\begin{align*}
\Delta E &= \text{smash}_{\text{ein}} + Q_e - Q_{\text{aus}} - U_2^2 \\
m_2 v_2 - m_1 v_1 &= \text{smash}_{\text{ein}} \quad \text{mit} \quad m_2 = m_1 + \Delta m \\
(m_1 + \Delta m) v_2 - m_1 v_1 &= \text{smash}_{\text{ein}} \\
m_2 v_2 + \Delta m v_2 - m_1 v_1 &= \text{smash}_{\text{ein}} \\
\text{smash}_{\text{ein}} &= m_2 v_2 - m_1 v_1 = m_1 (v_2 - v_1) \\
\Delta m &= \frac{m_1 (v_2 - v_1)}{v_{\text{ein}} - v_2}
\end{align*}

\begin{align*}
\Delta m &= \frac{5755 \, \text{kg} \, (v_2 - v_1)}{v_{\text{ein}} - v_2} = 3469.9 \, \text{kg}
\end{align*}

\begin{align*}
\Delta m_{12} &= 3469.9 \, \text{kg}
\end{align*}

\subsection*{Tabelle:}
\begin{align*}
U_2 &= U_2 (70^\circ \text{C}) = 292.95 \, \frac{\text{kJ}}{\text{kg}} \\
U_1 &= U_1 (100^\circ \text{C}) = 418.94 \, \frac{\text{kJ}}{\text{kg}} \\
h_{\text{ein}} &= h_{\text{p}} (20^\circ \text{C}) = 83.96 \, \frac{\text{kJ}}{\text{kg}} \\
m_1 &= 5755 \, \text{kg}
\end{align*}