b) \\
\[
\dot{S} = \dot{m} \left( s_{\text{ein}} - s_{\text{aus}} \right) + \frac{\dot{Q}_{\text{aus}}}{T}
\]

\[
T = \frac{T_{\text{a,aus}} - T_{\text{e,aus}}}{s_{\text{a}} - s_{\text{e}}}
\]

\[
s_{\text{a}} - s_{\text{e}} = c_{\text{p,m}} \ln \left( \frac{T_{\text{a}}}{T_{\text{e}}} \right)
\]

\[
0 = \dot{m} (h_{\text{e}} - h_{\text{a}}) + \dot{Q}_{\text{aus}}
\]

\[
\dot{Q} = \dot{m} c_{\text{p,m}} \Delta T + \dot{Q}_{\text{aus}}
\]

\[
\Delta T \approx -10 \text{K}
\]

\[
\dot{S} = \int \frac{\dot{Q}}{T} ds
\]

\[
\dot{S} = \frac{\dot{Q}}{s_{\text{a}} - s_{\text{e}}}
\]