d)

\[
U_{E2A} = m_{E2A} (u_{E2} + x_{E2A} (u_{E1} - u_{E2})) = -13.399 \, \text{kJ}
\]

\[
\rightarrow u_{E2} = -333.4 \, \frac{\text{kJ}}{\text{kg}} \quad \left( T_{A2} = 1 \, \text{bar}, \, p_{sat} = 1.000 \, \text{bar} \right)
\]

\[
u_{E1} = -0.046 \, \frac{\text{kJ}}{\text{kg}} \quad \left( 15000 \, \text{J} \right)
\]

\[
\rightarrow U_{E2A} = U_{E2} + \dot{Q}_{E2} = -11.848 \, \text{kJ}
\]

\[
\rightarrow x_{E2A} = \frac{U_{E2A}/m_{E2A} - u_{E2}}{u_{E1} - u_{E2}} = \underline{0.645}
\]

```