

\subsection*{b}
\begin{equation*}
T_{wir} = \frac{\int_{s_1}^{s_2} T \cdot ds}{s_2 - s_1}
\end{equation*}

\begin{equation*}
T_{wir, am} = 15^\circ C
\end{equation*}

\begin{equation*}
T_{wir, aus} = 25^\circ C
\end{equation*}

\begin{equation*}
s_2 = s (285.15 K) \rightarrow AZ
\end{equation*}
\begin{equation*}
= s (15^\circ C)
\end{equation*}
\begin{equation*}
= 0.2245 \frac{kJ}{kgK}
\end{equation*}

\begin{equation*}
s_2 = s (298 K) \rightarrow AZ
\end{equation*}
\begin{equation*}
= s (25^\circ C)
\end{equation*}
\begin{equation*}
= 0.36494 \frac{kJ}{kgK}
\end{equation*}

``````latex


\section*{1.C}
\begin{equation*}
0 = \dot{m} (se - sa) + \sum_{j} \dot{Q}_j + \dot{S}_{gen}
\end{equation*}

\begin{equation*}
\dot{S}_{gen} = - \dot{m} (se - sa) - \frac{\dot{Q}_{oven}}{T_{ref}}
\end{equation*}