\subsection*{1.a}
\begin{equation*}
\frac{dE}{dt} = \sum_i \dot{m}_i (h_i(t) + \frac{v_i^2(t)}{2} + p_i v_i(t)) - \sum_j \dot{m}_j (h_j(t) + \frac{v_j^2(t)}{2} + p_j v_j(t)) + \sum_j \dot{Q}_j - \sum_n \dot{W}_n
\end{equation*}

\begin{equation*}
0 = \dot{m}_{in} (h_e - h_a) + \dot{G}_z - \dot{Q}_{aus}
\end{equation*}

\begin{equation*}
\dot{Q}_{aus} = \dot{m}_{in} (h_e - h_a) - \dot{G}_z
\end{equation*}

\begin{equation*}
h_e = h_i (70^\circ C) \rightarrow AZ
\end{equation*}
\begin{equation*}
= 292.88 \frac{kJ}{kg}
\end{equation*}

\begin{equation*}
h_a = h_i (0^\circ C) \rightarrow AZ
\end{equation*}
\begin{equation*}
= 41.5 \frac{kJ}{kg}
\end{equation*}

\begin{equation*}
\dot{Q}_{aus} = 0.3 \frac{kg}{s} \cdot (292.88 \frac{kJ}{kg} - 41.5 \frac{kJ}{kg}) + 100 kW
\end{equation*}

\begin{equation*}
\dot{Q}_{aus} = 62.182 kW
\end{equation*}