

\section*{d}
\begin{equation*}
(m_{gas} \cdot c_{m2}) \cdot (T_{outlet2}) = m_{gas} \cdot c_{m2} \cdot T_{outlet} + \dot{m}_{gas} \cdot T_{in}
\end{equation*}

\begin{equation*}
0 = m_{gas} \cdot c_{m2} \cdot (T_{outlet2} - T_{in}) = m_{gas} \cdot c_{m2} \cdot T_{outlet} - m_{gas} \cdot c_{m2} \cdot T_{outlet2}
\end{equation*}

\begin{equation*}
m_{gas} = \frac{\dot{m}_{gas} \cdot (T_{outlet2} - T_{outlet})}{T_{outlet} - T_{in}}
\end{equation*}

\begin{equation*}
= 57.55 \, \text{kg} \cdot \frac{400^\circ C - 70^\circ C}{80^\circ C - 20^\circ C}
\end{equation*}

\begin{equation*}
m_{gas} = 3453 \, \text{kg}
\end{equation*}