

\section*{b}

\begin{align*}
    \text{given:} \quad \omega_2 &= \omega_1 \quad \& \quad T_2 \\
    \frac{T}{T_s} &= \left( \frac{P}{P_s} \right)^{\frac{\gamma-1}{\gamma}} \\
    T_2 &= \left( \frac{P_2}{P_1} \right)^{\frac{\gamma-1}{\gamma}} \cdot T_1 \\
    &= \left( \frac{0.5 \text{bar}}{0.1 \text{bar}} \right)^{\frac{1.4-1}{1.4}} \cdot 431.5 \text{K} \\
    T_2 &= 328.075 \text{K}
\end{align*}

\begin{align*}
    \frac{dE}{dt} &= \sum_i \dot{m}_i \left( h_i - h_e + \frac{\omega_i^2 - \omega_e^2}{2} \right) + \sum_j \dot{Q}_j - \sum_u \dot{W}_u \\
    0 &= \dot{m}_a \left( h_e - h_a + \frac{\omega_e^2 - \omega_a^2}{2} \right) \\
    2(h_2 - h_e) &= \omega_e^2 - \omega_2^2 \\
    \Rightarrow \omega_2 &= \sqrt{2(h_2 - h_e) + \omega_2^2}
\end{align*}

\begin{align*}
    h_a &= h \left( 431.5 \text{K} \right) \quad \rightarrow \text{A2Z} \\
    h_a &= h(431.5) + 1.5 \left( \frac{h(440 \text{K}) - h(430 \text{K})}{10} \right) \\
    &= 431.43 \frac{\text{kJ}}{\text{kg}} + 1.5 \left( \frac{441.6 \frac{\text{kJ}}{\text{kg}} - 431.43 \frac{\text{kJ}}{\text{kg}}}{10} \right) \\
    &= 432.364 \frac{\text{kJ}}{\text{kg}}
\end{align*}

``````latex

\begin{align*}
h_2 - h(328.075K) & \\
= h(320K) + 8.075 \cdot \frac{h(350K) - h(320K)}{10} & \\
= 320.25 \frac{kJ}{kg} + 8.075 \cdot \frac{330.36 \frac{kJ}{kg} - 320.25 \frac{kJ}{kg}}{10} & \\
= 328.405 \frac{kJ}{kg} &
\end{align*}

\begin{align*}
\omega_1 = \omega_3 = 220 \frac{m}{s} &
\end{align*}

\begin{align*}
\omega_2 = \sqrt{2(h_1 - h_2) + \omega_1^2} & \\
= 220.47 \frac{m}{s} &
\end{align*}

``````latex


\section*{2.C}

\[
\dot{E}_{x,sir} = \dot{m} \cdot e_{x,sir} = \dot{m} (h_0 - h_y - T_0 (s_0 - s_y) + ke_0 + hpc)
\]

\[
0 = e_{x,sir,0} = e_{x,sir,e}
\]

\[
e_{x,sir} = (h_0 - h_y - T_0 (s_0 - s_y) + ke_0 + hpc) - (h_0 - h_y - T_0 (s_0 - s_y) + ke_0 + hpc)
\]

\[
= h_0 - h_y - T_0 (s_0 - s_y) + ke_0 - ke_0 = 0
\]

\[
h_0 = h(T_0) = h(328.075K) \quad \text{in b interpret}
\]

\[
328.405 \frac{kJ}{kg}
\]

\[
h_{ke} = h(T_0) = h(243K)
\]

\[
h_e = h(50^\circ C) = h(243K)
\]

\[
= h(240K) + 3.15 \cdot \frac{h(250K) - h(240K)}{10}
\]

\[
= 240.024 \frac{kJ}{kg} + 3.15 \cdot \frac{250.05 \frac{kJ}{kg} - 240.024 \frac{kJ}{kg}}{10}
\]

\[
= 243.129 \frac{kJ}{kg}
\]

\[
T_y = T_0 = 243.15K
\]

\[
s_0 = s(328.075K)
\]

\[
= s(320K) + 8.075 \cdot \frac{s(330K) - s(320K)}{10}
\]

\[
= 1.7665 \frac{kJ}{kgK} + 8.075 \cdot \frac{1.79783 \frac{kJ}{kgK} - 1.7665 \frac{kJ}{kgK}}{10}
\]

\[
= 1.752 \frac{kJ}{kgK}
\]

\[
s_e = s(243.15K)
\]

\[
= s(240K) + 3.15 \cdot \frac{s(250K) - s(240K)}{10}
\]

\[
= 1.47824 \frac{kJ}{kgK} + 3.15 \cdot \frac{1.5 \frac{kJ}{kgK} - 1.47824 \frac{kJ}{kgK}}{10}
\]

\[
= 1.493 \frac{kJ}{kgK}
\]

\[
ke_0 = \frac{1}{2} \cdot v_0^2
\]

\[
= \frac{1}{2} \cdot (510 \frac{m}{s})^2
\]

\[
= 130.050 \frac{m^2}{s^2}
\]

\[
h_{ke} = \frac{1}{2} \cdot v_e^2
\]

\[
= \frac{1}{2} \cdot (200 \frac{m}{s})^2
\]

\[
= 20.000 \frac{m^2}{s^2}
\]

``````latex


\[
\Delta e_{2, \text{out}} = h_e - h_c - T_0 (s_e - s_c) + h_{ze} - h_{zc}
\]

\[
= 325.405 \frac{\text{kJ}}{\text{kg}} - 243.479 \frac{\text{kJ}}{\text{kg}} - 243.15 \text{K} \left(1.752 \frac{\text{kJ}}{\text{kg K}} - 1.653 \frac{\text{kJ}}{\text{kg K}}\right)
\]

\[
+ 130 \frac{\text{m}^2}{\text{s}^2} - 20 \frac{\text{m}^2}{\text{s}^2}
\]

\[
\Delta e_{2, \text{out}} = \underline{122.150 \frac{\text{kJ}}{\text{kg}}}
\]

``````latex