\section*{2.d}

\begin{align*}
e_{x,ve1} &= T_0 \cdot s_{e2} \\
s_{e2} &= s_{e} - s_{e1} \\
s_{e0} &= s_{e}(1.3/15\text{K}) \\
&= s(250\text{K}) - s(250\text{K}) \\
&= s(2\text{C}) - s(1.5\text{C}) \\
&= s(250\text{K}) - s(250\text{K}) \\
&= \frac{s(250\text{K}) - s(250\text{K})}{\Delta C}
\end{align*}

\begin{align*}
s_{e0} &= 1.494 \frac{\text{kJ}}{\text{kgK}} \quad \rightarrow \text{in 2c berechnet/interpoliert} \\
s_{e} &= 1.752 \frac{\text{kJ}}{\text{kgK}} \quad \rightarrow \text{in 2c berechnet/interpoliert}
\end{align*}

\begin{align*}
e_{x,ve1} &= T_0 \cdot (s_{e} - s_{e1}) \\
&= 293.15\text{K} \cdot (1.494 \frac{\text{kJ}}{\text{kgK}} - 1.752 \frac{\text{kJ}}{\text{kgK}})
\end{align*}

\begin{align*}
e_{x,ve1} &= -73.126 \frac{\text{kJ}}{\text{kg}}
\end{align*}

``````latex