

\subsection*{a)}

\text{ges.:} \quad \dot{Q}_{aus}

\text{Stationärer Fließprozess:}
\[
0 = \dot{m} (h_e - h_a) + \frac{\omega_e^2 - \omega_a^2}{2} + g(z_e - z_a) + \sum \dot{Q}_j - \sum \dot{W}_k
\]

\[
\Rightarrow 0 = \dot{m} (h_e - h_a) + \sum \dot{Q}_j
\]

\[
0 = \dot{m} (h_e - h_a) + \dot{Q}_k - \dot{Q}_{aus}
\]

\[
\Rightarrow \dot{Q}_{aus} = \dot{m} (h_e - h_a) + \dot{Q}_k
\]

\[
= \dot{m} (22,98 \frac{\text{kJ}}{\text{kg}} - 419,04 \frac{\text{kJ}}{\text{kg}}) + \dot{Q}_k
\]

\[
= 0,3 \frac{\text{kg}}{\text{s}} (22,98 \frac{\text{kJ}}{\text{kg}} - 419,04 \frac{\text{kJ}}{\text{kg}}) + 100 \text{kW}
\]

\[
= 62,182 \frac{\text{kJ}}{\text{s}} = 62,182 \text{kW}
\]

\text{Werte für } h_e, h_a \text{ kommen aus Tabelle 42!}