

\subsection*{a)}
\[
\dot{Q}_{\text{aus}}
\]
\[
\frac{d}{dt} \left( \sum m_i h_i + \xi Q - \xi W \right) = 0
\]
\[
\dot{m}_{\text{ein}} = \dot{m}_{\text{aus}} = 0.3 \, \text{kg/s}
\]
\[
h_{\text{ein}} = h(80^\circ \text{C}) \quad h_{\text{aus}} = h(40^\circ \text{C})
\]
\[
h_1, \, h_2 + v(r_1 g - h f) \, @ \, 10 \, \text{kJ} = 252.38 + 0.005 (2626.8 - 292.88)
\]
\[
= 304.64 \quad \leftarrow \frac{1}{3}
\]
\[
h_2 = 448.04 + 0.005 (2676.1 - 448.04) = 430.32 \quad \leftarrow \frac{1}{3}
\]
\[
Q_{\text{zu}} = \dot{m} (h_1 - h_2) + \dot{Q}_{\text{zu}} - \dot{Q}_{\text{aus}}
\]
\[
\dot{Q}_{\text{aus}} = \dot{m} (h_1 - h_2) + \dot{Q}_{\text{zu}} = 0.3 (304.64 - 430.32) + 100 \, \text{kW}
\]
\[
= 62.286 \, \text{kW}
\]
\[
= 62.3 \, \text{kW}
\]