

\section*{d)}

\begin{itemize}
    \item $u_{PS} =$
    \item $u_{PS} (T_1) = u_{K}$
    \item $m_g (u_{PS} (T_2) - u_{PS} (T_1)) = -u_{Kaiser} (T_3) \cdot m_{M} - u_{Kaiser} (T_1) \cdot m_{g}$
    \item $= (X_{T_1,1} \cdot u_{Kaiser} + (1 - X_{T_1,1}) \cdot u_{perf})_{m_{PS,1}}$
    \item $+ (X_{T_1,2} \cdot u_{Kaiser} + (1 - X_{T_1,2}) \cdot u_{perf})_{m_{PS,2}}$
    \item $\Rightarrow$ \underline{Fazit:} $u_{PS} (T_2) - u_{PS} (T_1)$
\end{itemize}

``````latex

\section*{Aufgabe 3) d).}

\[
m_s \left( u_{ps}(t_2) - u_{ps}(t_1) \right) = \int_{T_{s1}}^{T_{s2}} c_v \, dT \cdot m_{es}
\]

\[
= c_v \cdot \Delta T \cdot m_{es}
\]

\[
= 0.633 \left( \frac{\text{kJ}}{\text{kgK}} \right) \cdot (-500 \degree \text{C})
\]

\[
= -7.092 \, \text{kJ}
\]

\section*{}

\[
x_{es1} \cdot u_{f1es} + m_{f1es} + (1 - x_{f2es}) \cdot u_{f2f} \cdot m_{f2f}
\]

\[
= 0.6 \cdot 0.1 \, \text{kg} - 0.01 \, \text{kg/kg} + 0.4 \cdot 0.1 \, \text{kg} - 133.418 \, \text{kJ/kg}
\]

```