d) \quad m_2 u_2 - m_1 u_1 = \Delta m_2 (h_{ein}) + \dot{Q}_{zu} \quad \text{Energie Austausch gleich}

\[
\Delta m_2 = m_2 u_2 - m_1 u_1 - \dot{Q}_{zu}
\]

\[
u_1 = u_f (100^\circ C) + x_D (u_g (100^\circ C) - u_f (100^\circ C)) = 429.38 \frac{kJ}{kg}
\]

\[
h_{ein} (20^\circ C) = u_f (20^\circ C) = 83.35 \frac{kJ}{kg}
\]

\[
u_2 (70^\circ C) = u_f (70^\circ C) = 232.35 \frac{kJ}{kg}
\]

\[
\Delta m_2 = m_2 - m_1
\]

\[
m_2 u_2 - m_1 u_1 = (m_2 - m_1) h_{ein} + \dot{Q}_{zu}
\]

\[
m_2 = \frac{m_1 u_1 - \dot{Q}_{zu}}{u_2 - h_{ein}}
\]

\[
m_2 = 5511.72 \, \text{kg}
\]

\[
\Delta m_2 = \frac{40.8 + 8.2}{2} = 3576.72 \, \text{kg}
\]