d) \quad m_{EV}(u_2 - u_1) + m_g(u_2 - u_1) = \dot{Q} - \dot{W} = 0

\[
\dot{Q} = \dot{W}
\]

\[
p_g = p_{EV}
\]

\[
u_{2, \text{new}} = u_g - 353.638 \frac{kJ}{kg} + x \left( -0.05 \frac{kJ}{kg} + 533.65 \frac{kJ}{kg} \right) = x = -133.64 \frac{kJ}{kg}
\]

\[
m_g(u_2 - u_1) = m_g c_v (T_2 - T_1) = -1.082 \, kJ
\]

\[
u_{2, EV} = u_4 + \frac{m_g (u_2 - u_1)}{m_{EV}} = -122.55 \frac{kJ}{kg}
\]

\[
p_{2, EV} = p_{1, EV} = 1.4 \, \text{bar}
\]

\[
T_{1, EV} = T_{2, EV}
\]

\[
x = \frac{u_{2, EV} + 353.638 \frac{kJ}{kg}}{-0.05 \frac{kJ}{kg} + 533.65 \frac{kJ}{kg}} = 0.632
\]

``````latex