

\subsection*{b)}

\begin{align*}
\text{ges: } \omega_0, T_6 \\
0 &= m_{gs} \left[ h_5 - h_6 + \frac{\left( \omega_5^2 - \omega_6^2 \right)}{2} \right] + \dot{Q}_{SG}^0 + \dot{W}_{S6} \\
0 &= m_{gs} \left[ h_4 - h_6 + \frac{\left( \omega_4^2 - \omega_6^2 \right)}{2} \right] + \dot{Q}_{SG}^0 - \dot{Q}_{20}^0 \\
h_4 - h_6 &= C_p \left( T_4 - T_6 \right) \\
\frac{T_1}{T_5} &= \left( \frac{p_c}{p_5} \right)^{\frac{\kappa - 1}{\kappa}} \Rightarrow T_6 = T_1 \left( \frac{p_0}{p_5} \right)^{\frac{\kappa - 1}{\kappa}} = 433.51K \left( \frac{0.15 \text{bar}}{0.5 \text{bar}} \right)^{\frac{0.4}{1.4}} = 325.07K = T_6 \\
\Rightarrow C_p \left( T_0 - T_6 \right) + \frac{\left( \omega_2^2 - \omega_6^2 \right)}{2} = 0 \\
\Rightarrow 2 C_p \left( T_0 - T_6 \right) - \omega_0^2 = - \omega_6^2 \\
\Rightarrow \sqrt{\omega_6^2 + 2 C_p \left( T_0 - T_6 \right)} = \omega_0 \\
\Rightarrow \omega_0 = \sqrt{200 \frac{kJ}{kgK} \cdot 2 \cdot 1.006 \frac{kJ}{kgK} \left( 243.15 - 325.07 \right) K} = 453.19 \frac{m}{s}
\end{align*}

``````latex

\section*{2)}



\subsection*{b)}

\[
0 = \dot{m}_{gs} \left[ \Delta e_{x,str} \right] - \dot{E}_{x,ver}
\]

\[
\Rightarrow 0 = \left[ \Delta e_{x,str} \right] - \dot{E}_{x,ver}
\]

\[
\Rightarrow e_{x,ver} = 122,21 \frac{kJ}{kg}
\]

``````latex