
``````latex


\section*{1.}

\subsection*{a) $\dot{Q}_{\text{aus}}$}

\textbf{E-Bilanz stat. Fließprozesses}

\[
0 = \dot{m} \left( h_e - h_a \right) + \sum \dot{Q} - \dot{W}^0 = \dot{m} (h_e - h_a) + \dot{Q} - \dot{Q}_{\text{aus}}
\]

\[
\dot{Q}_{\text{aus}} = \dot{m} (h_e - h_a) + \dot{Q}
\]

\[
h_e = h_f(200^\circ C) + x_0 \left( h_g(200^\circ C) - h_f(200^\circ C) \right) = 292.89 + 0.9 \cdot (3040.64 - 292.89) = 2704.65 \quad \text{(A-2)}
\]

\[
h_a = h_f(100^\circ C) + x_0 \left( h_g(100^\circ C) - h_f(100^\circ C) \right) = 419.04 + 0.1 \cdot (2675.4 - 419.04) = 643.34 \quad \text{(A-2)}
\]

\[
\dot{Q}_{\text{aus}} = 62.492 \, \text{kW} \quad \text{:= A}
\]

\textbf{Variablen}

\[
A := \dot{Q}_{\text{aus}}
\]

\subsection*{b) $\overline{T}_{\text{KF}}$}

\textbf{Entropiebilanz stat.}

\[
0 = \dot{m} \left( s_e - s_a \right) + \frac{\dot{Q}}{T} + s^0_{12}
\]

\textbf{keine Druckänderung, adiabatisch $\Leftrightarrow$ isentrop}

\[
\overline{T} = \frac{\dot{Q}}{\dot{m} (s_e - s_a)}
\]

\subsection*{c) $\dot{s}_{\text{erz}}$}

\[
\overline{T}_{\text{KF}} = 295 \, \text{K}
\]

\[
0 = \dot{m} \left( s_e - s_a \right) + \frac{\dot{Q}}{T} + \dot{s}_{\text{erz}}
\]

\[
\dot{s}_{\text{erz}} = \dot{m} \left( s_e - s_a \right) = \dot{m} c \ln \left( \frac{T_a}{T_e} \right) - \frac{\dot{Q}}{T}
\]

\textbf{Entropiebilanz am Wand}

\[
0 = \dot{m} s^0_{12} + \frac{\dot{Q}}{T} + \dot{s}_{\text{erz}}
\]

\[
\dot{s}_{\text{erz}} = -2 \left( \frac{\dot{Q}_{\text{aufb}}}{T_{\text{reaktor}}} \right) + \frac{\dot{Q}_{\text{aus}}}{\overline{T}_{\text{KF}}} = 0.0441 \, \frac{\text{kJ}}{\text{kg K}}
\]

\subsection*{d) $\Delta m_{12}$}

\textbf{E-Bilanz}

\[
\Delta E = m_2 u_2 - m_1 u_1 + \dot{m} \left( h_e - h_a \right) + \dot{Q} - \dot{W}^0
\]

\[
(m_2 + \Delta m_{12}) u_2 - m_1 u_1 = \Delta m_{12} h_e - Q_{\text{aus}} = \dot{m} (u_2 - u_1) + \Delta m_{12} h_e - Q_{\text{aus}}
\]

\[
h_e = h_f(200^\circ C) + x_0 \left( h_g(200^\circ C) - h_f(200^\circ C)```latex


1. e)
\[
\Delta s = m_2 s_2 - m_1 s_1 = m_1 (s_2 - s_1) + \Delta m \, s_2
\]
\[
s_2 = s_f(400^\circ \text{C}) + x_0 \left( s_g(400^\circ \text{C}) - s_f(100^\circ \text{C}) \right) \quad \text{(A-2)}
\]
\[
s_2 = s_f(400^\circ \text{C})
\]
\[
s_1 = 1.33714 \quad \text{= 1B}
\]
\[
s_2 = 0.9549
\]
\[
\Delta s = -4299.4 \, \frac{\text{kJ}}{\text{kg K}}
\]

\underline{\hspace{5cm}}

``````latex


