
``````latex


a) 
\begin{align*}
T_{\text{ein}} &= 70^\circ C \\
T_{\text{aus}} &= 100^\circ C \\
T_{\text{rout}} &= 100^\circ C \\
\end{align*}

\begin{align*}
T_{\text{kein}} &= 298.15\,K \\
T_{\text{kaus}} &= 286.15\,K \\
\end{align*}

\begin{align*}
m_{\text{ges}} &= 5755\,\mu g \\
x_D &= 0.005 = \frac{m_D}{m_{\text{ges}}} \\
\dot{Q}_R &= 10\,\text{kW} \\
\end{align*}

\begin{align*}
\dot{Q}_{\text{aus}} = ?
\end{align*}

\[
\left[ \text{stat.} \frac{2x}{m} \right]
\]

\[
0 = \dot{m}_{\text{ein}} (h_e - h_a) + \dot{m}_{\text{aus}} (h_e - h_a) + \dot{Q}_R + \dot{Q}_{\text{aus}} - \cancel{Z\dot{W}}
\]

\[
\dot{Q}_{\text{aus}} = 2\dot{m}_{\text{ein}} (h_e - h_a) + \dot{Q}_R
\]

\[
\dot{Q}_{\text{aus}} = 2 \cdot 0.3 \frac{kg}{s} (292.98 - 419.04) \frac{kJ}{kg} + 10\,\text{kW}
\]

\[
= 26.36\,\text{kW}
\]

b) 
\[
\bar{T}_{\text{KF}} = \frac{\int_{s_a}^{s_e} T ds}{s_e - s_a}
\]

\[
s_e - s_a = \int_{T_a}^{T_e} c \frac{1}{T} dT = c \ln \left( \frac{T_e}{T_a} \right)
\]

\[
\int_{s_a}^{s_e} T ds = \Delta H = h_e - h_a = \int_{T_a}^{T_e} c dT + v^3 \left( p_e - p_a \right)
\]

\[
\Rightarrow \frac{c \left( T_e - T_a \right)}{c \ln \left( \frac{T_e}{T_a} \right)} \Rightarrow \bar{T}_{\text{KF}} \quad | : c
\]

\[
\bar{T}_{\text{KF}} = \frac{T_e - T_a}{\ln \left( \frac{T_e}{T_a} \right)}
\]

\[
T_{\text{kein}} = 298.15 \\
T_{\text{kaus}} = 298.15
\]

\[
\frac{298.15 - 298.15}{\ln \left( \frac{298.15}{298.15} \right)} = 293.12\,K = \bar{T}_{\text{KF}}
\]

c) 
\[
\dot{S}_{\text{exz}} = ?
\]

\[
\left[ \text{stat.} \frac{2x}{m} \right]
\]

\[
0 = \dot{m}_{\text{ein}} (s_e - s_a) + \dot{m}_{\text{aus}} (s_e - s_a) + \frac{\dot{Q}_{\text{aus}}}{\bar{T}_{\text{KW}}} + \dot{S}_{\text{exz}}
\]

\[
\dot{S}_{\text{exz}} = 2\dot{m}_{\text{ein}} (s_e - s_a) - \frac{\dot{Q}_{\text{aus}}}{\bar{T}_{\text{KW}}}
\]

\[
= 2 \cdot 0.3 \frac{kg}{s} (0.36 \frac{kJ}{kgK} - 0.226 \frac{kJ}{kgK}) - \frac{```latex


\begin{enumerate}
    \item[d)] \( T \)
    \item[2] \( \dot{Q} \)
\end{enumerate}

\[
\Delta m_2
\]
\[
Q_{\text{aus}} = 35 \cdot 10^3 \, \text{J}
\]

\[
\text{Zulauf gestopft}
\]

\[
\frac{dE}{dt} = \dot{m}_2 (h_1 - h_2) + \sum \dot{Q} - \sum \dot{W} = 0
\]

\[
m_2 u_2 - m_2 u_1 = \dot{m}_2 (h_1 - h_2) + \frac{Q_{\text{aus}}}{t}
\]

\[
m_2
\]

\[
h_1 = h_2 (20^\circ \text{C}) = 83.96
\]
\[
h_2 = h_3 (70^\circ \text{C}) = 292.98
\]
\[
u_2 - u_3 (70^\circ \text{C}) = 1.0228 \cdot 10^{-3}
\]
\[
u_2 - u_2 (20^\circ \text{C}) = 1.018 \cdot 10^{-3}
\]

``````latex


