
``````latex


\section*{Aufgabe 4:}

\subsection*{a)}

\begin{itemize}
    \item The graph is a Pressure-Temperature ($P$-$T$) diagram.
    \item The $y$-axis is labeled $P$ with units in $[\text{bar}]$.
    \item The $x$-axis is labeled $T$ with units in $[\text{K}]$.
    \item The curve starts at the origin, rises to a peak, and then falls back down, forming a closed loop.
    \item There are three points marked on the curve:
        \begin{itemize}
            \item Point 1 is at the lower left part of the curve.
            \item Point 2 is at the lower right part of the curve.
            \item Point 3 is at the top of the curve.
        \end{itemize}
    \item There is a horizontal line connecting points 1 and 2, labeled $x$.
    \item There is a vertical line from point 3 to the horizontal line, labeled $y$.
    \item The region inside the loop is labeled "2-Phasen".
\end{itemize}

\subsection*{b)}

\[
0 = \dot{m} (h_e - h_a) + \dot{Q} - \dot{W}
\]

\begin{itemize}
    \item Wir schauen uns 2 $\rightarrow$ 3 an
    \item adabat, reversibel, $\rightarrow$ bentos
    \item $p_3 = 8 \text{ bar} \quad T_3 =$
    \item $s_3 = s_2$
\end{itemize}

``````latex


c)

\[
T_2 = -22^\circ C
\]

\[
\dot{m} = 4 \frac{kg}{h} = \frac{4}{3600} \frac{kg}{s}
\]

\text{ADIABATE PROZESS - ISENTHAP}

\[
h_4 = h_4
\]

\[
p_4 = 8 \text{ bar} \quad T_4 = 31.33^\circ C
\]

\[
h_4 = 93.12 \frac{kJ}{kg}
\]

\[
h_4 = 93.12 \frac{kJ}{kg}
\]

\[
p_{a2} = 1 \text{ bar} + \frac{0.45 \text{ bar}}{7.63^\circ C} (-22^\circ C - (-26.48))
\]

\[
= 1.23 \text{ bar}
\]

\[
p_1 = p_2 = 1.23 \text{ bar}
\]

\[
x = \frac{h_1 - h_f}{h_g - h_f}
\]

\[
h_f = 21.82 + \frac{4.15}{0.2} (1.23 - 1.2) = 21.6875 \frac{kJ}{kg} \quad \text{TAB A11}
\]

\[
h_g = 233.6 + \frac{2.18}{0.2} (1.23 - 1.2) = 234.187 \frac{kJ}{kg}
\]

\[
p = 1.23 \text{ bar}
\]

\[
T = -22^\circ C
\]

\[
x = \frac{93.12 \frac{kJ}{kg} - 21.6875 \frac{kJ}{kg}}{234.187 \frac{kJ}{kg} - 21.6875 \frac{kJ}{kg}} = 0.337
\]

``````latex


\section*{Aufgabe 9:}

\begin{equation*}
a) \quad E_k = \frac{\dot{Q}_{zu}}{(\dot{W}_t)} = \frac{\dot{Q}_{zu}}{\dot{Q}_{ab} - \dot{Q}_{zu}}
\end{equation*}

```