
``````latex


3)

a) 
\[
p_{g1} = p_{amb} + \frac{m_c \cdot g \cdot h}{A} + \frac{m_{eng} \cdot g \cdot h}{A}
\]

\[
A = \pi \frac{D^2}{4} = 7.85 \cdot 10^{-3} \, \text{m}^2
\]

\[
p_{g1} = 3.473 \, \text{bar} \quad \boxed{}
\]

\[
p_{gn} = 1.1 \, \text{bar} \quad \boxed{}
\]

\[
\frac{p_{g1} V_{g1}}{R T_{g1}} = 3.429 = mg \quad \underline{}
\]

\[
R = \frac{\bar{R}}{M_g} = 0.16628
\]

b) 
\[
\Delta E = Q - W
\]

\[
\Delta E = Q - W
\]

\[
\Delta E = 0
\]

\[
= mg (u_2 - u_1) \quad , \text{perfektes Gas}
\]

\[
= mg (c_v (T_2 - T_1))
\]

\[
p_{g2} = \frac{mg \bar{R} T_{g2}}{V_{g1}}
\]

\[
V_{g1} = V_{g2} \quad , \text{da isotherm perfektes Gas}
\]

``````latex


\begin{itemize}
    \item[(c)] 
    \begin{equation*}
        \frac{dE}{dt} = \dot{Q} - \sum \dot{W}^c
    \end{equation*}
    \begin{equation*}
        mg(u_2 - u_1) = \dot{Q}
    \end{equation*}
    \begin{equation*}
        mg(v(T_2 - T_1)) = \boxed{-1.07 \, \text{kW} = \dot{Q}}
    \end{equation*}
\end{itemize}

``````latex


