
``````latex


\section*{Aufgabe 1}

\subsection*{a)}

Energiebilanz:

\[
Q = \dot{m} (h_e - h_a) + \dot{Q}_R - \dot{Q}_{\text{aus}}
\]

\[
\dot{Q}_{\text{aus}} = \dot{m} (h_{\text{ein}} - h_{\text{aus}}) + \dot{Q}_{R}
\]

\[
h_{\text{ein}} = 292.98 \frac{\text{kJ}}{\text{kg}}
\]

\[
h_{\text{aus}} = 419.04 \frac{\text{kJ}}{\text{kg}}
\]

\[
\dot{Q}_{\text{aus}} = 0.3 \left( 292.98 - 419.04 \right) + 100
\]

\[
= 62.182 \, \text{kW}
\]

\subsection*{b)}

\[
\dot{Q}_{\text{aus}} = 65 \, \text{kW}
\]

\[
\overline{T}_{\text{kF}} = \frac{\int_{s_{\text{ein}}}^{s_{\text{aus}}} T \, ds}{s_{\text{aus}} - s_{\text{ein}}}
\]

``````latex

\section*{Aufgabe 1}

\subsection*{c)}
\[
T_{HF} = 298 \, \text{K}
\]
\[
0 = \dot{m} \left( s_e - s_a \right) + \sum \frac{\dot{Q}_j}{T} + \dot{S}_{erz}
\]
\[
\dot{S}_{erz} = -\dot{m} \left( s_e - s_a \right) - \sum \frac{\dot{Q}_j}{T}
\]

\subsection*{d)}
\[
\Delta m \left[ h \right] + Q - W + \cancel{W} = \Delta U + \cancel{\Delta KE} + \cancel{\Delta PE}
\]

\subsection*{e)}
\[
\Delta S = m_2 s_2 - m_1 s_1
\]
\[
m_2 = m_1 + \Delta m_{12}
\]

``````latex


