
``````latex


\section*{Aufgabe 3}

\subsection*{a)}

\begin{align*}
pV &= mRT \quad \text{(m\textsubscript{EW} + m\textsubscript{Eis} = 0.16 kg)} \\
\sum F &= 0 \\
p_{s1} \cdot A - 0.1 \cdot g - 32 \cdot g - p_{amb} \cdot A &= 0 \\
p_{s1} &= \frac{(0.1 + 32) \cdot g}{A} + p_{amb} \\
A &= \left(\frac{2}{2}\right)^2 \cdot \pi = \left(\frac{10 \cdot 10^{-3}}{2}\right)^2 \cdot \pi \\
&= 0.0078 \, \text{m}^3 \\
p_{s1} &= \frac{(0.1 + 32) \cdot 9.81}{0.0078} + 1.10^5 \\
&= 1.4 \, \text{bar} \\
R &= \frac{R}{M} = \frac{8314}{50} = 166.28 \\
m_{g,1} &= \frac{p_{s1} \cdot V_{g,1}}{R \cdot T_{g,1}} \\
&= \frac{1.4 \cdot 10^5 \cdot 3.14 \cdot 10^{-3}}{166.28 \cdot 773} \\
&= 0.0034 \, \text{kg} = 3.4 \, g
\end{align*}

\subsection*{b)}

\begin{align*}
h_{gas} &= h_{EW}
\end{align*}

``````latex


\section*{Aufgabe 3}

\subsection*{a)}

Energiebilanz

\[
Q - W = \Delta U + \Delta KE + \Delta PE
\]

\[
Q_{12} = W_{12} + \Delta U_{12}
\]

\[
\Delta U_{12} = U_2 - U_1 = m_g (u_2 - u_1) = m_g \left( c_v (T_{g,2} - T_{g,1}) \right)
\]

\[
= 3.6 \cdot 10^{-3} \cdot 0.633 \left( 0.003 - 500 \right)
\]

\[
= -1.14 \, \text{kJ}
\]

\subsection*{b)}

\[
T_{g,2} = T_{EW,2} = 0.003 \, ^\circ \text{C}
\]

\[
Q_{12} = \Delta U = m \Delta U = (m_{EW} + m_{eis}) \left( x_{eis} \cdot U_{fest} + (1 - x_{eis}) \cdot U_{flüssig} \right)
\]

\[
1500 \, \text{J} = 0.16 \, \text{kg} \left( x_{eis} (U_{fest} - U_{flüssig}) + U_{fest} \right)
\]

\[
x_{eis} = \frac{1500 \, \text{J}}{0.16} - \frac{V_{fest}}{U_{fest} - U_{flüssig}}
\]

\[
= \frac{1500}{0.16} + 333.4
\]

\[
= -333.4 + 0.033
\]

\[
Q_{12} = \Delta U = U_2 - U_1
\]

\[
U_2 = \frac{m_{eis}}{m_{tot}} x_{eis,2} U_{fest} + \frac{m_{eis}}{m_{tot}} (1 - x_{eis,2}) U_{flüssig}
\]

\[
U_1 = x_{eis,1} U_{fest} + (1 - x_{eis,1}) U_{flüssig}
\]

``````latex


