
``````latex


1. a)

\text{Stat. Flie√üprozess mit 1 Massenstrom}

\[
0 = \dot{m} (h_e - h_a) + \dot{Q} - \dot{Q}_{\text{Aus}}
\]

\[
0 = \dot{m} (h_{\text{ein}} - h_{\text{aus}}) + \dot{Q}_R - \dot{Q}_{\text{Aus}}
\]

\[
\dot{Q}_{\text{Aus}} = \dot{m} (h_{\text{ein}} - h_{\text{aus}}) + \dot{Q}_R
\]

\[
\dot{Q}_{\text{Aus}} = 0.3 (h_{\text{ein}} - h_{\text{aus}}) + 100 \frac{\text{kJ}}{\text{s}} = 67.182 \text{kW}
\]

\underline{hein:}

\[
T = 70^\circ C
\]

\[
x = 0
\]

\[
p = 0.3119 \text{ bar aus A-2}
\]

\[
h_{\text{ein}} = h_f = 252.98 \frac{\text{kJ}}{\text{kg}} \text{ aus A-2}
\]

\underline{hinaus:}

\[
T_{\text{aus}} = 100^\circ C
\]

\[
x = 0
\]

\[
p = 1.013 \text{ bar aus A-2}
\]

\[
h_{\text{aus}} = h_f = 419.04 \frac{\text{kJ}}{\text{kg}} \text{ aus A-2}
\]

b)

\[
\bar{T} = \frac{\int_{S_e}^{S_a} T dS}{S_a - S_e}
\]

\[
\int_{S_e}^{S_a} T dS = Q \text{ weil p const.}
\]

\[
S_{a}^* - S_e = \int_{T_{AE}}^{T_A} \frac{c_p (T)}{T} dT
\]

\[
= c_p (T) \left[ \ln(T) \right]_{T_{AE}}^{T_A}
\]

\[
=
\]

c)

\[
\bar{T} = 295.5 K \text{ aus Aufgabenstellung}
\]

\[
0 = \dot{m} (s_e - s_a) + \frac{\dot{Q}_{\text{aus}}}{\bar{T}} + \dot{s}_{\text{ext}}
\]

\[
- \dot{s}_{\text{ext}} =
\]

``````latex


\section*{1. d)}

\begin{enumerate}
    \item 
    \begin{align*}
        T_{R1} &= 100^\circ C \\
        x_D &= 0.005 \\
        m_1 &= 5755 \text{ kg}
    \end{align*}
    
    \item 
    \begin{align*}
        T_{R2} &= 70^\circ C \\
        x_2 &= 0 \\
        m_2 &= m_1 + \Delta m_{12}
    \end{align*}
\end{enumerate}

\noindent
\text{=D halboffenes System}

\begin{align*}
    \Delta E &= m_2 u_2 - m_1 u_1 = \Delta m_{12} (h_{ein}) + Q \\
    (m_1 + \Delta m_{12}) u_2 - m_1 u_1 &= \Delta m_{12} (h_e) + Q_{R12} \\
    m_1 u_2 - Q_{R12} - m_1 u_1 &= \Delta m_{12} (h_e) - \Delta m_{12} u_2 \\
    m_1 u_2 - Q_{R12} - m_1 u_1 &= \Delta m_{12} (h_e - u_2)
\end{align*}

\noindent
\text{h_{ein}:}
\begin{align*}
    T_{ein} &= 20^\circ C \\
    x &= 0 \\
    p_{ein} &= 0.02339 \\
    h_{ein} = h_f &= 83.96 \frac{\text{kJ}}{\text{kg}} \quad \text{(aus A-2)}
\end{align*}

\noindent
\text{U_2:}
\begin{align*}
    x_1 &= 0.005 \\
    U_2 = U_f (70^\circ C) &= 292.95 \quad \text{(aus A-2)}
\end{align*}

\noindent
\text{U_A:}
\begin{align*}
    U_A &= x_1 u_g (100^\circ C) + (1 - x_1) u_f (100^\circ C) \\
    &= x_1 \left( 2506.5 \frac{\text{kJ}}{\text{kg}} \right) + (1 - x_1) \left( 419.89 \frac{\text{kJ}}{\text{kg}} \right) \\
    &= 429.37 \frac{\text{kJ}}{\text{kg}}
\end{align*}

\noindent
\text{aus A-2}
\begin{align*}
    \Delta m_{12} &= \frac{m_1 u_2 + Q_{R12} - m_1 u_1}{h_e - u_2} \\
    &= 3589.37 \text{ kg}
\end{align*}

``````latex


e)

\begin{align*}
\Delta S &= \cancel{S_2} M_2 S_2 - M_1 S_1 \\
S_1 &= x \cdot S_g + (1-x) S_f = \frac{1.33714 \, \text{kJ}}{\text{kg}} \\
x &= 0.905 \\
S_g &= 7.3549 \, \frac{\text{kJ}}{\text{kgK}} \text{ aus A-2} \\
S_f &= 1.3069 \, \frac{\text{kJ}}{\text{kgK}} \\
S_2 &= x \cdot S_f (-7.0^\circ \text{C}) \\
x_2 &= 0 \\
S_f (7.0^\circ \text{C}) &= 0.9549 \, \frac{\text{kJ}}{\text{kgK}} \text{ aus A-2} \\
m_1 &= 5755 \, \text{kg} + 3600 \, \text{kg} = \underline{9355 \, \text{kg}}
\end{align*}

\[
\Delta S = \underline{1235.83 \, \text{kJ}}
\]

``````latex


