
``````latex


\section*{Aufgabe 1: Reaktor}

\subsection*{a)}
\begin{align*}
0 &= \dot{m} (\hat{h}_\text{ein} - \hat{h}_\text{aus}) + \dot{Q}_e + \dot{Q}_\text{um} + \dot{Q}_\text{v} \\
\hat{h}_\text{ein} &\Rightarrow \text{S\"{a}ttigungsfl\"{u}ssigkeit bei 70^\circ \text{C}} \quad \Rightarrow \hat{h}_\text{ein} = 293,98 \frac{\text{kJ}}{\text{kg}} \\
\hat{h}_\text{aus} &\Rightarrow \text{S\"{a}ttigungsdampf bei 100^\circ \text{C}} \quad \Rightarrow \hat{h}_\text{aus} = 2675,5 \frac{\text{kJ}}{\text{kg}} \\
\dot{Q}_\text{aus} &= \dot{m} (\hat{h}_\text{aus} - \hat{h}_\text{ein}) - \dot{Q}_\text{in} = -62,1824 \frac{\text{kW}}{}
\end{align*}

\subsection*{b)}
\begin{align*}
T_\text{irr} &= \int_{S_a}^{S_e} \frac{\delta e}{T} \quad ; \quad de = \frac{\delta Q}{T} \\
&= - \int_{S_a}^{S_e} \frac{dS}{S_a - S_e} = \frac{q_a - q_e}{S_a - S_e} = \frac{u_a - u_e}{S_a - S_e} \quad \text{(ideale Gase)} \\
&= c_p \left( \frac{T_a - T_e}{T_a - T_e} \right) = c_p \ln \left( \frac{T_a}{T_e} \right) \\
&= 293,12 \text{K}
\end{align*}

\subsection*{c)}
\begin{align*}
0 &= \dot{m} (S_e - S_a) + \frac{\dot{Q}_\text{um}}{T_\text{irr}} + \dot{S}_\text{erz} \\
S_\text{erz} &= \dot{m} (S_a - S_e) - \frac{\dot{Q}_\text{um}}{T_\text{irr}} = \dot{m} (S_a - S_e) + \frac{\dot{Q}_\text{um}}{T_\text{irr}} \\
\text{Werte:} \\
S_e &= S_f (70^\circ \text{C}) = 0,3564 \frac{\text{kJ}}{\text{kg K}} \\
S_a &= S_f (100^\circ \text{C}) = 1,3069 \frac{\text{kJ}}{\text{kg K}} \\
\Rightarrow S_\text{erz} &= 0,3178 \frac{\text{kJ}}{\text{K}}
\end{align*}

``````latex


\section*{d) Halboffenes System:}

\[
\Delta E = \dot{m}_{12} h_{12} + \dot{Q}_{12} + \dot{W}_{12} \rightarrow 0
\]

\[
m_{u2} - m_{u1} = \Delta m_{12} h_{12}
\]

\[
\Rightarrow \Delta m_{12} = \frac{m_{u2} - m_{u1}}{h_{12}} = 
\]

\[
u_1 = u_e(1000) + x_0 (u_g - u_f) = 429.37 \frac{kJ}{kg}
\]

\[
u_2 = u_e(20^\circ C) + x_0 (u_g - u_f) = 303.368 \frac{kJ}{kg}
\]

\[
m_{u2} = m_{u1} + \Delta m_{12}
\]

\[
h_{12} = h_{g12} = 126.06 \frac{kJ}{kg}
\]

\[
\Rightarrow \Delta m_{12} = \frac{(m_{u2} - m_{u1})}{h_{12}}
\]

\[
\Delta m_{12} + m_{u2} = m_{u2} - m_{u1} \leftarrow \Delta m_{12} \left(1 + \frac{1}{h_{12}}\right) = \frac{m_{u2} - m_{u1}}{h_{12}}
\]

\[
\Delta m_{12} = \frac{m_{u2} - m_{u1}}{h_{12} \left(1 + \frac{1}{h_{12}}\right)} = 5680 \mu g
\]

\section*{e)}

\[
\Delta S = S_2 - S_1 = \dot{m} (s_2 - s_1) = \frac{\dot{Q}}{T} - \frac{\dot{Q}_{loss}}{T_0} + S_{erz}
\]

\[
\Rightarrow \Delta S_{12} = S_{erz}
\]

``````latex


