
``````latex

1) a. Stationarer Flie√üprozess: 
\[ 0 = \dot{m} \left[ h_{\text{ein}} - h_{\text{aus}} \right] + \dot{Q}_{\text{aus}} \frac{\dot{m}_{\text{dampf}}}{\dot{m}_{\text{dampf}}} \]

\[ \dot{Q}_{\text{aus}} = \dot{m} \left[ h_{\text{aus}} - h_{\text{ein}} \right] - \dot{Q}_{\text{R}} \]

\[ h_{\text{ein}} (70^\circ C) = (1-x) h_c^{70^\circ C} + x h_g^{70^\circ C} = \]

\[ = (1-0.005) \cdot 292.98 \frac{\text{kJ}}{\text{kg}} + 0.005 \cdot 2333.8 \frac{\text{kJ}}{\text{kg}} \]

\[ = 292.68 \frac{\text{kJ}}{\text{kg}} \]

\[ h_{\text{aus}} (100^\circ C) = (1-x) h_c (100^\circ C) + x h_g (100^\circ C) = \]

\[ = 428.23 \frac{\text{kJ}}{\text{kg}} \]

\[ \dot{Q}_{\text{aus}} = 0.3 \left[ 428.23 - 292.68 \right] \frac{\text{kJ}}{\text{kg}} = 406 \text{kW} - 100 \text{kW} \]

b. 
\[ + 65 \text{kW} \]

\[ T_{\text{KF}} = 4 \frac{T_{\text{KF,aus}} - T_{\text{ein}}}{2} \]

c. 
\[ 0 = \dot{m} \left[ s_{\text{ein}} - s_{\text{aus}} \right] + \frac{\dot{Q}_{\text{aus}}}{T_{\text{KF}}} + \dot{S}_{\text{erz}} \]

d.

``````latex


