
``````latex


\section*{Aufgabe 1}

\subsection*{a)}
1 HS am Reaktor \\
\(\dot{Q}_{\text{statisch}}\)

\[
0 = \sum \dot{m} \left[ h_i + \frac{c^2}{2} + g z \right] - \dot{Q}_{\text{aus}} - \dot{W}
\]

\[
\dot{Q}_{\text{aus}} = \dot{m}_{\text{ein}} h_{\text{ein}} + \dot{m}_{\text{aus}} h_{\text{aus}}
\]

\[
\text{Tab A-2:} \quad h_{\text{ein}} (T_{\text{ein}} = 70^\circ C) = 292.58 \frac{\text{kJ}}{\text{kg}}
\]

\[
h_{\text{aus}} (T_{\text{aus}} = 100^\circ C) = 419.04 \frac{\text{kJ}}{\text{kg}}
\]

\[
\dot{Q}_{\text{aus}} = -0.3 \frac{\text{kg}}{\text{s}} \cdot 292.58 \frac{\text{kJ}}{\text{kg}} + 0.3 \frac{\text{kg}}{\text{s}} \cdot 419.04 \frac{\text{kJ}}{\text{kg}}
\]

\[
= 33.818 \frac{\text{kJ}}{\text{s}} = 33.818 \text{kW}
\]

\subsection*{b)}
\[
\overline{T}_{\text{KF}} = \frac{\int_{S_e}^{S_a} T \, ds}{S_a - S_e} = \frac{T_a - T_e}{S_a - S_e}
\]

\subsection*{c)}
\[
\dot{S}_{e2} = \dot{m} \left[ s_a - s_e \right] + \frac{\dot{Q}_E}{T_E}
\]

\[
\text{Tab A-2:} \quad s_a (T_a = 100^\circ C) = 1.3069 \frac{\text{kJ}}{\text{kgK}}
\]

\[
s_e (T_e = 70^\circ C) = 0.9549 \frac{\text{kJ}}{\text{kgK}}
\]

\[
\dot{S}_{e2} = 0.3 \frac{\text{kg}}{\text{s}} \left[ 1.3069 - 0.9549 \right] \frac{\text{kJ}}{\text{kgK}} + \frac{100 \text{kW}}{295 \text{K}} = 0.1056 \frac{\text{kJ}}{\text{K}} + 0.3390 \frac{\text{kJ}}{\text{K}} = 0.4446 \frac{\text{kJ}}{\text{K}}
\]

``````latex


\section*{Student Solution}

\subsection*{d)}

\[
\frac{dE}{dt} = \sum_i \dot{m}_i \left[ h_i + \frac{v_i^2}{2} + \cancel{pe_i} \right] + \sum_j Q_j - \sum_k \dot{m}_k \left[ h_k + \frac{v_k^2}{2} + \cancel{pe_k} \right]
\]

\subsection*{e)}

\[
\Delta S = S_2 - S_1 = m (s_2 - s_1) = \sum_i \frac{Q_i}{T_j} + S \cancel{e x z}
\]

\[
- S e x z \sum_i \dot{m}_i s_i + \frac{\sum_j Q_j}{T_j}
\]

``````latex


