
``````latex


\section*{Aufgabe 1}

\subsection*{a)}
\[
\dot{S} = 0 \Rightarrow 0 = \dot{m}_{ein} \cdot h_{ein} - \dot{m}_{aus} \cdot h_{aus} + \dot{Q} - \dot{Q}_{Aus}
\]
\[
\Rightarrow \dot{Q}_{Aus} = \dot{m} \cdot (h_e - h_{aus}) + \dot{Q}
\]
\[
\text{Gleiche Feuchtigkeit beide am Ein- und Ausgang}
\]
\[
\Rightarrow x_e = 0 \quad ; \quad x_f = 1 \quad \text{jeweils}
\]
\[
\text{aus TABELLE:} \quad h_e = h_f (p = 700 \, \text{kPa}) = 292,98 \, \frac{\text{kJ}}{\text{kg}}
\]
\[
h_{aus} = h_f (p = 1000 \, \text{kPa}) = 434,04 \, \frac{\text{kJ}}{\text{kg}}
\]
\[
\dot{Q}_{Aus} = \dot{m} \cdot \left(292,98 - 434,04\right) \, \frac{\text{kJ}}{\text{kg}} + 200 \, \frac{\text{kJ}}{\text{s}}
\]
\[
\dot{Q}_{Aus} = 0,3 \, \frac{\text{kg}}{\text{s}} \cdot \left(292,98 - 434,04\right) \, \frac{\text{kJ}}{\text{kg}} + 200 \, \frac{\text{kJ}}{\text{s}}
\]
\[
\dot{Q}_{Aus} = 62,438 \, \text{kW}
\]

\subsection*{b)}
\[
\bar{T} = \frac{\int_{s_a}^{s_e} T \, ds}{s_a - s_e} = 
\]

``````latex


