
``````latex


\section*{Aufgabe 1}

\subsection*{a)}
\[
Q = \dot{m}_{\text{w}} (h_{\text{ein}} - h_{\text{aus}}) + Q_{\text{aus}}
\]
\[
Q_{\text{aus}} = \dot{m}_{\text{w}} (h_{\text{aus}} - h_{\text{ein}})
\]
\[
= \dot{m}_{\text{w}} \left[ c (T_{\text{aus}} - T_{\text{ein}}) + v_i^2 (p_{\text{aus}} - p_{\text{ein}}) \right]
\]

\subsection*{b)}
\[
T = \int_{s_a}^{s_e} T \, ds = \frac{q_{\text{rev}}}{s_i - s_e} = \frac{h_{\text{aus}} - h_{\text{ein}}}{s_{\text{aus}} - s_{\text{ein}}} = \frac{f (T_{\text{aus}} - T_{\text{ein}}) + v_i^2 (p_{\text{aus}} - p_{\text{ein}})}{s_i \ln \left( \frac{T_{\text{aus}}}{T_{\text{ein}}} \right)}
\]
\[
= \frac{T_{\text{aus}} - T_{\text{ein}}}{\ln \left( \frac{T_{\text{aus}}}{T_{\text{ein}}} \right)} = \frac{298.15 \, \text{K} - 288.15 \, \text{K}}{\ln \left( \frac{298.15 \, \text{K}}{288.15 \, \text{K}} \right)}
\]
\[
= 293.12 \, \text{K}
\]

\subsection*{c)}
\textbf{Verbal description of the diagram:}

The diagram consists of a horizontal arrow pointing to the right, labeled "Energieblance". Above the arrow, there is a label "Q_{\text{aus}}". Below the arrow, there is a label "T_{\text{KF}}". To the right of the arrow, there is a circle labeled "Q_{\text{aus}}". From this circle, there are two arrows pointing to the right. The upper arrow is labeled "Serz" and the lower arrow is labeled "Q_{\text{aus}}". The upper arrow points to a label "T_{\text{Reaktor, a}}" and the lower arrow points to a label "T_{\text{Reaktor, n}}".

\[
Q = \dot{m}_{\text{w}} (h_{\text{ein}} - h_{\text{aus}}) + Q_{\text{aus}}
\]
\[
Q_{\text{aus}} = \dot{m}_{\text{w}} (h_{\text{aus}} - h_{\text{ein}})
\]
\[
= \dot{m}_{\text{w}} \left[ c (T_{\text{aus}} - T_{\text{ein}}) + v_i^2 (p_{\text{aus}} - p_{\text{ein}}) \right]
\]

\[
\text{Serz} = \frac{Q_{\text{aus}}}{T_{\text{KF}}} + \frac{Q_{\text{R}}}{T_{\text{Reaktor, a}}}
\]
\[
= \frac{Q_{\text{aus}}}{T_{\text{KF}}} + \frac{Q_{\text{R}}}{T_{\text{Reaktor, n}}}
\]
\[
= \frac{63 \, \text{kW}}{293 \, \text{K}} + \frac{100 \, \text{kW}}{373.15 \, \text{K}}
\]
\[
= 47.64 \, \frac{\text{W}}{\text{K}}
\]

``````latex


\section*{d)}

\begin{equation*}
\frac{dE}{dt} = \sum_i \dot{m}_i \left[ h_i + \frac{c_i^2}{2} + \frac{g z_i}{2} \right] - \dot{Q} - \dot{W}^o
\end{equation*}

\begin{equation*}
\Delta U = \Delta m_{12} h_{ein} + \dot{Q}
\end{equation*}

\begin{equation*}
m_2 u_2 - m_1 u_1 = \Delta m_{12} h_{ein} + \dot{Q} \quad \text{with} \quad m_2 = m_1 + \Delta m_{12}
\end{equation*}

\begin{equation*}
(m_1 + \Delta m_{12}) u_2 - m_1 u_1 = \Delta m_{12} h_{ein} + \dot{Q}
\end{equation*}

\begin{equation*}
- \dot{Q} + m_1 u_2 - m_1 u_1 = \Delta m_{12} h_{ein} - m_1 u_2 - \Delta m_{12} u_2
\end{equation*}

\begin{equation*}
- \dot{Q} + m_1 (u_2 - u_1) = \Delta m_{12} h_{ein} - \Delta m_{12} u_2
\end{equation*}

\begin{equation*}
- \dot{Q} + m_1 (u_2 - u_1) = \Delta m_{12} (h_{ein} - u_2)
\end{equation*}

\begin{equation*}
\Rightarrow \Delta m_{12} = \frac{m_1 (u_2 - u_1) - \dot{Q}}{h_{ein} - u_2}
\end{equation*}

\subsection*{siedende Fl√ºssigkeit: $\lambda = 0.5$}

\begin{equation*}
h_{ein} = 83.96 + 0.5 (2538.1 - 83.96) = 1311.03 \frac{kJ}{kg} \quad \text{(TAB-A-2)}
\end{equation*}

\begin{equation*}
u_1 = 418.94 + 0.005 (2506.5 - 418.94) = 429.3778 \frac{kJ}{kg} \quad \text{(TAB-A-2)}
\end{equation*}

\begin{equation*}
u_2 = 292.35 + 0.5 (2463.6 - 292.35) = 1381.275 \frac{kJ}{kg} \quad \text{(TAB-A-2)}
\end{equation*}

\begin{equation*}
\Delta m_{12} = \frac{5755 kg (1381.275 \frac{kJ}{kg} - 429.3778 \frac{kJ}{kg}) + 35 \frac{kJ}{s}}{1311.03 \frac{kJ}{kg} - 1381.275 \frac{kJ}{kg}}
\end{equation*}

``````latex


\section*{Problem 2}

\subsection*{e) Entropiebilanz}

\[
\frac{dS}{dt} = \dot{m}_{ein} s_{ein} - \frac{\dot{Q}_{zu}}{T_j} + S_{erz}(t)
\]

\[
\Delta S = m_2 s_2 - m_1 s_1
\]

\[
m_2 = m_1 + \dot{m}_{12} = 5755 \, \text{kg} + 3600 \, \text{kg} = 9355 \, \text{kg}
\]

\[
s_2 = 0.8549 + 0.5 (7.7553 - 0.8549) = 4.3551 \, \frac{\text{kJ}}{\text{kg K}}
\]

\[
s_1 = 1.3069 + 0.005 (7.3549 - 1.3069) = 1.33714 \, \frac{\text{kJ}}{\text{kg K}}
\]

\[
\Delta S_{12} = 9355 \, \text{kg} \cdot 4.3551 \, \frac{\text{kJ}}{\text{kg K}} - 5755 \, \text{kg} \cdot 1.33714 \, \frac{\text{kJ}}{\text{kg K}}
\]

\[
= 33046.7 \, \frac{\text{kJ}}{\text{K}} = 33.05 \, \frac{\text{MJ}}{\text{K}}
\]

``````latex


