
``````latex


\section*{A3) E1}

\subsection*{a) $p_{g,1}$, $m_g$ im Zylinder:}

\[
Cv = 0{,}623 \frac{J}{kgK}
\]

\[
p_{g,1} = p_{amb} + \left( \frac{m_g}{A_{Zyl}} \right) + \left( \frac{m_{W,1}g}{A_{Zyl}} \right)
\]

\[
= \Delta h^3 Pq \left( \frac{32{,}9}{0{,}00785 \, m^2} \right) + \left( \frac{0{,}1 \cdot 9{,}81}{0{,}00785} \right)
\]

\[
= 10^5 \, m + 39{,}983{,}8 \, Pa + 1{,}25 \, kPa
\]

\[
= 1{,}4 \, bars
\]

\[
A_{Zyl} = \left( \frac{D}{2} \right)^2 \cdot \pi
\]

\[
= (0{,}05 \, m)^2 \cdot \pi
\]

\[
=
\]

\[
m_g = p_{A,g} \cdot V_{g,1} = m_g \cdot R_g \cdot T_{g,1}
\]

\[
R_g = \frac{8{,}314}{50 \, \frac{kg}{mol}} = 166{,}28
\]

\[
\Rightarrow m_g = \frac{p_{A,g} \cdot V_{g,1}}{R_g \cdot T_{g,1}} = \frac{1{,}4 \, bar \cdot 3{,}14 \cdot 10^{-3} \, m^3}{166{,}28 \cdot 773 \, K} = 0{,}00342 \, kg
\]

\[
= 3{,}42 \, g
\]

\[
3{,}14 \, L = 3{,}14 \, dm^3
\]

\[
= 3{,}14 \cdot 10^{-3} \, m^3
\]

\[
500^\circ C = 773 \, K
\]

\subsection*{b) Thermodyn. Gleichung: $T_{g,2} = T_{B,w,2}$}

\[
\Delta h = Q = Cv \cdot m_g \cdot (T_{g,2} - T_{g,1})
\]

\[
T_{g,2} = \frac{T_{1,g}}{Cv \cdot m_g} = 273 \, K
\]

``````latex


\section*{Problem c)}

\begin{align*}
    T_{g,2} &= 0{,}003^\circ C \quad (\text{aus Tipp}) \\
    &= 273{,}153 \, K \\
    p_{2,g} \cdot v_{2,g} &= R_g \cdot T_{2,g} \\
    v_{1,g} &= \frac{V_2 \cdot g}{m_g} \\
    \Rightarrow T_{2,g} &= 0{,}003^\circ C = 273{,}153 \, K \\
    \Rightarrow \dot{Q} &= C_v \cdot m_g \cdot (T_{2,g} - T_{1,g}) \\
    &= 0{,}633 \, \frac{kJ}{kgK} \cdot 0{,}00842 \, kg \cdot (273{,}153 - 273) \\
    &= -1{,}08 \, kJ = |Q| = 1{,}08 \, kJ
\end{align*}

\section*{Problem d)}

$x_{\text{eis},2}$ berechnen:

Energiebilanz:
\begin{align*}
    m_{\text{ew}} (u_2 - u_1) &= \dot{Q}_{12} \\
    m_{\text{ew}} &= 0{,}1 \, kg
\end{align*}

Thermodyn. GGW:
\begin{align*}
    u_2 \, EN &= u_{2,g} \Rightarrow (u_2 - u_1)_{\text{EW}} = (u_{1,g} - u_{g}')
\end{align*}

\begin{align*}
    \int_{T_1}^{T_2} (u_{2,g} - u_{g}') &= \int_{T_1}^{T_2} C_v(T) \, dT = C_v (T_2 - T_1) \\
    &= Q_{12}
\end{align*}

\begin{align*}
    u_2 - u_1 &= \frac{\dot{Q}}{m_{\text{ew}}} \\
    u_2 &= \frac{\dot{Q}}{m_{\text{ew}}} + u_1
\end{align*}

``````latex


