
``````latex

\section*{1. Reaktor}

\subsection*{a)}
\begin{align*}
\text{ges.:} & \quad \dot{Q}_{\text{aus}} \\
\text{geg.:} & \quad \dot{m} = 0.3 \, \frac{\text{kg}}{\text{s}}, \quad T_{\text{ein}} = 70^\circ \text{C} \\
& \quad T_{\text{aus}} = 100^\circ \text{C} \\
& \quad m_{\text{ges}} = 5755 \, \text{kg}, \quad T_R = 100^\circ \text{C}, \quad \dot{Q}_R = 100 \, \text{kW} \\
& \quad \Delta T_{\text{KF}} = T_{\text{KF,aus}} - T_{\text{KF,ein}} = 10 \, \text{K} \\
\\
\dot{Q}_{\text{aus}} & = \dot{Q}_R \frac{T_{\text{ein}}}{T_{\text{aus}}} \\
& = 100 \, \text{kW} \frac{70^\circ \text{C}}{100^\circ \text{C}} \\
& = 70 \, \text{kW}
\end{align*}

\subsection*{b)}
\begin{align*}
\overline{T}_{\text{KF}} & = \frac{T_{\text{KF,aus}} + T_{\text{KF,ein}}}{2} \\
& = \frac{298.15 \, \text{K} + 288.15 \, \text{K}}{2} \\
& = 293.15 \, \text{K}
\end{align*}

\subsection*{c)}
\begin{align*}
\dot{S}_{\text{erzg}} & = -\dot{m} (s_2 - s_1) - \sum_j \frac{\dot{Q}_j}{T_j} \\
& = \frac{65 \, \text{kW}}{293 \, \text{K}} \\
& = 220.333 \, \frac{\text{kJ}}{\text{kg K}}
\end{align*}

\subsection*{d)}
\begin{align*}
\frac{dE}{dt} & = \sum_i \dot{m}_i (h_i(t) + k_{ei}(t) + p_{ei}(t)) + \sum_j \dot{Q}_j(t) - \sum_n \dot{W}_n(t)
\end{align*}

\subsection*{e)}
\begin{align*}
\Delta S_{1-2} & = S_2 - S_1
\end{align*}

``````latex


