
``````latex


\section*{Problem 9}

\subsection*{a)}
\[
Q_{\text{aus}} = ?
\]
\[
\text{E-Bil: } 0 = m_{\text{ein}} (h_e - h_a) + QR - Q_{\text{aus}}
\]
\[
h_e = 262.6 \, \frac{\text{kJ}}{\text{kg}} \quad \text{TAB A-2, } h_a = 269.6 \, \frac{\text{kJ}}{\text{kg}} \quad \text{TAB A-2}
\]
\[
Q_{\text{aus}} = m_{\text{ein}} (h_e - h_a) + QR = 85.24 \, \text{kJ}
\]

\subsection*{b)}
\[
\overline{T}_{\text{KF}} = ?
\]
\[
\overline{T} = \frac{\int_{s_a}^{s_e} T \, ds}{s_e - s_a}
\]
\[
\int_{T_1}^{T_2} \frac{c}{T} \, dT = c \cdot \ln \left( \frac{T_a}{T_e} \right)
\]
\[
T \, ds = q
\]
\[
\text{E-Bil: } 0 = m_{\text{KF}} (h_e - h_a) + Q_{\text{aus}}
\]
\[
q = \frac{Q_{\text{aus}}}{m_{\text{KF}}} = m_{\text{KF}} \cdot \frac{h_e - h_a}{c \cdot (T_a - T_e)} = \psi = c \cdot \theta (T_a - T_e)
\]
\[
\overline{T}_{\text{KF}} = \frac{q \cdot (T_a - T_e)}{q \cdot \ln \left( \frac{T_a}{T_e} \right)} = 293.12 \, \text{K}
\]

\subsection*{c)}
\[
S_{e2} = ?
\]
\[
\frac{Q_{\text{aus}}}{\overline{T}_{\text{KF}}} = S_{e2} = 0.29 \, \frac{\text{kJ}}{\text{K}}
\]

\subsection*{d)}
\[
\text{E-Bil: } \Delta U_{e2} = QR + Q_{e2}
\]
\[
\Delta U_{e2} = m_{e2} u_{e2} - m_{e1} u_{e1} \quad m_f = 5755 \, \text{kg}, \quad m_{e2} = m_{e1} + \Delta m_{e2}
\]
\[
u = 438.94 + x_0 (2506.5 - 438.94) = 429.38 \, \frac{\text{kJ}}{\text{kg}} \quad \text{TAB A-2}
\]
\[
u_{e2} = u_g (30^\circ \text{C}) = 246.6 \, \frac{\text{kJ}}{\text{kg}} \quad \text{TAB A-2}
\]
\[
m_{e1} u_{e1} + \Delta m_{e2} u_{e2} = QR + m_{e1} u_{e1} = 7 \Delta m_{e2} (Q_{\text{aus}} + m_{e1} u_{e1} - m_{e1} u_{e2}) \cdot \frac{1}{u_{e2}}
\]
\[
\Delta m_{e2} = 
\]

\subsection*{e)}
\[
\Delta m_{e2} = 3600 \, \text{kg} \quad \text{Annahme} \quad \Delta S_{m2} = ?
\]
\[
m_{e2} = m_{e1} + \Delta m_{e2} = 9355 \, \text{kg}
\]
\[
\text{S-Bil: } \Delta S_{m2} = \frac{Q_{\text{aus}}}{\overline{T}_{\text{KF}}} - S_{e2}```latex


