
``````latex


\section*{7) a) $\dot{Q}_{aus} = ?$}

\begin{equation*}
\frac{dE}{dt} = \sum \dot{m}_{ein} \cdot h_{ein} - \sum \dot{m}_{aus} \cdot h_{aus} + \sum \dot{Q} - \sum \dot{W}
\end{equation*}

\text{Stationär:}

\begin{equation*}
0 = \sum \dot{m}_{ein} \cdot h_{ein} + \sum \dot{Q}
\end{equation*}

\begin{equation*}
0 = \dot{m}_{ein} \cdot h_{ein} - \dot{m}_{aus} \cdot h_{aus} + \dot{Q}_{aus} + \dot{Q}_{12}
\end{equation*}

\begin{equation*}
\dot{m}_{ein} \cdot (h_{aus} - h_{ein}) = \dot{Q}_{aus} + \dot{Q}_{12} \text{(keine Wassers)}
\end{equation*}

\begin{equation*}
0.3 \cdot \dot{m}_{ein} \cdot \left[ \int_{T_2}^{T_1} c(T) dT + \dot{m}_{ein} \cdot (p_2 - p_1) \right] = \dot{Q}_{aus}
\end{equation*}

\text{Siedende Flüssigkeit (Wasser)}

\begin{equation*}
T_{ein} = 70^\circ C \rightarrow \text{TAB A-2} \rightarrow p_A = 0.3119 \frac{kg}{s}
\end{equation*}

\begin{equation*}
h_f = 292.98 \frac{kJ}{kg}
\end{equation*}

\begin{equation*}
h_g = 2626.8 \frac{kJ}{kg}
\end{equation*}

\begin{equation*}
T_{aus} = 100^\circ C \rightarrow \text{TAB A-2} \rightarrow p_A = 1.0149 \frac{kg}{s}
\end{equation*}

\begin{equation*}
h_f = 419.04 \frac{kJ}{kg}
\end{equation*}

\begin{equation*}
h_g = 2676.1 \frac{kJ}{kg}
\end{equation*}

\text{Das gesamte System}

\begin{equation*}
\frac{dE}{dt} = \sum \dot{m}_{ein} \cdot h_{ein} + \sum \dot{Q}
\end{equation*}

\begin{equation*}
0 = \dot{m}_{ein} \cdot (h_{ein} - h_{aus}) \text{im nur betracht.}
\end{equation*}

\begin{equation*}
\dot{m}_{ein} \cdot (h_{aus} - h_{ein}) = \dot{Q}_{12} = \dot{Q}_{aus}
\end{equation*}

\begin{equation*}
x = 0.005
\end{equation*}

\begin{equation*}
h_{ein} = h_f + x \cdot (h_g - h_f) = 292.98 \frac{kJ}{kg} + 0.005 \cdot (2626.8 \frac{kJ}{kg} - 292.98 \frac{kJ}{kg})
\end{equation*}

\begin{equation*}
h_{ein} = 304.645 \frac{kJ}{kg}
\end{equation*}

\begin{equation*}
h_{aus} = h_{f100^\circ C} + x \cdot (h_{g100^\circ C} - h_{f100^\circ C}) = 419.04 \frac{kJ}{kg} + 0.005 \cdot (2676.1 \frac{kJ}{kg} - 419.04 \frac{kJ}{kg})
\end{equation*}

\begin{equation*}
h_{aus} = 430.325 \frac{kJ}{kg}
\end{equation*}

\begin{```latex

\begin{itemize}
    \item[b)] 
    \[
    \text{TRF} = \frac{\int_{s_a}^{s_e} T ds}{s_a - s_e}
    \]
    \[
    0 = \dot{m} \left[ s_e - s_a \right] + \sum \frac{\dot{Q}_j}{T_j} + \dot{s}_{\text{rez}}
    \]
    \text{Lorenzgleichung}
    \[
    s_a - s_e = \int_{T_1}^{T_2} \frac{c_{if}(T)}{T} dT \quad \text{p const} = n = \dot{Q}?
    \]
    \[
    \rightarrow \text{TRF} = 295 K
    \]
    
    \item[c)] 
    \[
    \dot{S}_{\text{rez}} = ?
    \]
    \[
    \frac{dS}{dt} = 0 = \dot{m} \left[ s_e - s_a \right] T + \sum \frac{\dot{Q}_j}{T_j} + \dot{s}_{\text{rez}}
    \]
\end{itemize}

``````latex


