
``````latex


1)

a) \(\dot{Q}_{\text{aus}}^* = -\dot{m} (h_e - h_a)\)

\[
\begin{aligned}
    T_{K,\text{ein}} &= 288.15 \, \text{K} \\
    T_{K,\text{aus}} &= 298.15 \, \text{K}
\end{aligned}
\]

\[
\begin{aligned}
    T_{\text{ein}} &= 70^\circ \text{C} \\
    T_{\text{aus}} &= 100^\circ \text{C} \quad \text{(reines Wasser)}
\end{aligned}
\]

\[
\begin{aligned}
    h_e &= h_f(70^\circ \text{C}) \quad \text{/TAB. A-2} \\
    &= 292.98 \, \frac{\text{kJ}}{\text{kg}}
\end{aligned}
\]

\[
\begin{aligned}
    h_{ea} &= h_f(100^\circ \text{C}) + x_D \cdot (h_g(100^\circ \text{C}) - h_f(100^\circ \text{C})) \\
    &= 419.04 + 0.005 \cdot (2676.1 - 419.04) \, \left[\frac{\text{kJ}}{\text{kg}}\right] \\
    &= 430.33 \, \left[\frac{\text{kJ}}{\text{kg}}\right]
\end{aligned}
\]

\[
\begin{aligned}
    \dot{Q}_{\text{aus}}^* &= -0.3 \, \frac{\text{kg}}{\text{s}} \left[ 292.98 \, \frac{\text{kJ}}{\text{kg}} - 430.33 \, \frac{\text{kJ}}{\text{kg}} \right] \\
    &= 41.2 \, \text{kW} \quad \rightarrow \quad \dot{Q}_R = \dot{Q}_{\text{aus}}^* - \dot{Q}_{\text{aus}} \\
    \dot{Q}_{\text{aus}} &= 58.8 \, \text{kW}
\end{aligned}
\]

b)

\[
\begin{aligned}
    \overline{T} &= \frac{\int_{s_e}^{s_a} T \, ds}{s_a - s_e} = \frac{298.15 \, \text{K} - 288.15 \, \text{K}}{s_a - s_e}
\end{aligned}
\]

\[
\begin{aligned}
    s_a &= s_f + x_D (s_g - s_f) \quad \text{(A-2)} \\
    &= 1.337
\end{aligned}
\]

\[
\begin{aligned}
    \overline{T} &= \frac{298.15 - 288.15 \, \text{K}}{0.1549 - 1.337 \, \left[\frac{\text{kJ}}{\text{kgK}}\right]} = -26.17 \, \text{K}
\end{aligned}
\]

``````latex

\section*{c)}
\begin{equation*}
\dot{S}_{gen} = -\dot{m}(s_e - s_a) + \sum \frac{\dot{Q}}{T}
\end{equation*}
\begin{equation*}
\dot{m} = 0.3 \frac{kg}{s}, \quad s_e = 0.254 \frac{kJ}{kgK}, \quad s_a = 1.377 \frac{kJ}{kgK}
\end{equation*}
\begin{equation*}
\dot{Q} = \dot{Q}_R - \dot{Q}_{\text{aus}}
\end{equation*}

\section*{d)}
\begin{equation*}
0 = \dot{m}(h_e - h_a) + \dot{Q}_R + \dot{Q}_{\text{aus}}
\end{equation*}
\begin{equation*}
\dot{m} = -\frac{\dot{Q}_R + \dot{Q}_{\text{aus}}}{(h_e - h_a)}
\end{equation*}

\section*{e)}
\begin{equation*}
\Delta S = m(s_2 - s_1)
\end{equation*}
\begin{equation*}
m = 5755 \, kg
\end{equation*}

``````latex


