
``````latex


\section*{3) a) Ges: $P_{1g}$, $m_g$}

\begin{itemize}
    \item A diagram is drawn showing a vertical cylinder with a piston inside. The piston is labeled with $P_{eis}$ on top and $P_{gas}$ on the bottom. The top of the cylinder is labeled $P_1$ and the bottom is labeled $P_3$. An arrow pointing downwards is labeled $mg$.
\end{itemize}

\[
P_{eis} = P_{gas} \text{ da gleichgewicht}
\]

\[
P_a + \frac{m \cdot g}{A} = P_{eis}
\]

\[
1.10^5 + 32 \cdot 9.81 - P_{eis} = 1.399369 \text{ bar}
\]

\[
P_{1g} = 1.4 \text{ bar}
\]

\[
m_g = \frac{P_1 \cdot V_1}{R \cdot T_1}
\]

\[
R = \frac{R}{M} = \frac{8344}{50} = 166.28
\]

\[
m_g = \frac{1.4 \cdot 10^5 \cdot 3.14 \cdot 0.001}{166.28 \cdot (500 + 273.15)} - 0.003418 \text{ kg} = 3.4189
\]

\section*{b)}

Da keine zus채tzliche Kraft dazukommt ist der Prozess im Zylinder isobar und daher $P_{23} = P_{1g} = 1.4 \text{ bar}$.

Da wir immer noch im Eis Wasser gebildet sind, im Zustand 2 ist $T_{2w} = T_{1w} = 0^\circ C$ und es stellt sich im thermischen Gleichgewicht. Deshalb $T_{2w} = T_{2g} = 0^\circ C$.

\section*{c) Ges: $Q_{12}$}

1 HS am Gas. F체r Volum

\[
\Delta U = Q - W \quad \text{da Potentielle energien vernachl채ssigen}
\]

\[
\Delta U = \dot{m} \cdot c_v \cdot (T_2 - T_1) = Q_{12}
\]

\[
3.4189 \cdot 0.633 \cdot 10^5 \cdot (0 - 500^\circ C) = -1.08755 \text{ kJ}
\]

\[
= -1077154 J
\]

``````latex


3d) \(r_{\text{eis}} = ?\)

\[
x_{\text{eis}_1} = 0,6
\]

\[
m_{\text{eis}} = 0,06 \, \text{kg}
\]
\[
m_{\text{wasser}} = 0,04 \, \text{kg}
\]

1HS am Eis:

\[
\Delta U = Q - \dot{W}^0
\]

\[
v_1 = m_{\text{eis}} \cdot V
\]

Station채r geschlossen

\[
\Delta U = Q - \dot{W}^0 = m_{\text{ew}} \cdot x_2 \cdot u_{\text{de}_2} + m_{\text{ew}} \cdot (1 - x_2) \cdot u_{fE_2}
\]
\[
- m_{\text{ew}} \cdot x_1 \cdot u_{\text{d}1} - m_{\text{ew}} \cdot (1 - x_1) \cdot u_{fE_1}
\]

\[
u_{df12} = u_{df1} = -0,0415 \, \text{kJ/kg} = u_d
\]
\[
u_{dfE1} = u_{df2} = -333,458 \, \text{kJ/kg} = u_f
\]

\[
Q = m_{\text{ew}} \left( x_2 \cdot u_d + (1 - x_2) \cdot u_f - x_1 \cdot u_d \cdot (1 - x_1) \cdot u_f \right)
\]

\[
\frac{Q}{m_{\text{ew}}} + x_1 \cdot u_d + (1 - x_1) \cdot u_f = x_2 \cdot u_d + u_f - x_2 \cdot u_f
\]

\[
\frac{Q}{m_{\text{ew}}} + x_1 \cdot u_d + (1 - x_1) \cdot u_f - u_f = x_2
\]

\[
u_d - u_f
\]

\[
-1,0735 \, \text{kJ} + 6,6 - 0,0415 + (0,4) - 333,458 - 0,0415
\]

\[
-333,417 + 0,045
\]

\[
= 0,14325
\]

``````latex


