
``````latex


1) \quad KE = PE = 0

\textbf{Prozess: stationärer Fließprozess mit Massenstrom}

\[
0 = \dot{m} \left( h_{\text{ein}} - h_{\text{aus}} \right) + \dot{Q}_R - \dot{W}_t
\]

\[
h_{\text{ein}} \text{ mit } (T=70^\circ \text{ gesättigt}) \quad \text{Tab}
\]

\[
h_{\text{aus}} = h_f + x_D \left( h_g - h_f \right)
\]

\[
h_f = \text{Tab A-2 (T=100^\circ \text{C})} = 419.04 \, \frac{\text{kJ}}{\text{kg}}
\]

\[
h_g = \text{Tab A-2 (T=100^\circ \text{C})} = 2676.1 \, \frac{\text{kJ}}{\text{kg}}
\]

\[
h_{\text{aus}} = 430.33 \, \frac{\text{kJ}}{\text{kg}}
\]

\[
h_{\text{ein}} = \text{Tab A-2 (T=70^\circ \text{C})} \left\{
\begin{array}{l}
h_f = 293.38 \, \frac{\text{kJ}}{\text{kg}} \\
h_g = 2626.8 \, \frac{\text{kJ}}{\text{kg}}
\end{array}
\right.
\]

a) \quad \text{WF}

\textbf{ideale Flüssigkeit}

\[
c_p^{\text{if}} = c_v^{\text{if}} = c^{\text{if}}(T) = f
\]

\[
\Delta T = 10 \, \text{K}
\]

\[
h_{\text{ein}} = h_f + x_D \left( h_g - h_f \right) = 3041.6491 \, \frac{\text{kJ}}{\text{kg}}
\]

\[
\dot{m} = 0.3 \, \frac{\text{kg}}{\text{s}}
\]

\[
0 = \dot{m} \left( h_{\text{ein}} - h_{\text{aus}} \right) + \dot{Q}_R - \dot{Q}_{\text{aus}}
\]

\[
\dot{Q}_{\text{aus}} = \dot{m} \left( h_{\text{ein}} - h_{\text{aus}} \right) + \dot{Q}_R = \underline{62.256 \, \mu \text{W}}
\]

``````latex

\begin{itemize}
    \item[(b)] 
    \[
    \overline{T} = \frac{\int_{s_e}^{s_a} T \, ds}{s_a - s_e}
    \]
    \[
    s_a - s_e = \int_{T_1}^{T_2} \frac{cif(T)}{T} \, dT = 0.73376 \, \frac{\text{kJ}}{\text{kgK}}
    \]
    \[
    = cif \cdot \ln \left( \frac{T_2}{T_1} \right)
    \]
    \[
    cif = \dot{m} \cdot \Delta t = 21.66 \, \frac{\text{kJ}}{\text{kgK}}
    \]
    \[
    \overline{T} = \frac{\int_{s_e}^{s_a} T \, ds}{s_a - s_e} \left( \frac{T_2 - T_1}{s_a - s_e} \right) + T_1 = 254.514 \, K
    \]
    
    \item[(c)]
    \[
    0 = \dot{m} (s_e - s_a) + \sum \frac{\dot{Q}}{T} + S_{erz}
    \]
    \[
    S_{erz} = \dot{m} (s_a - s_e) - \sum \frac{\dot{Q}}{T}
    \]
    \[
    = \dot{m} (s_a - s_e) + \frac{\dot{Q}_{aus}}{T}
    \]
    \[
    S_{erz} = 0.44209 \, \frac{\text{kW}}{\text{h}}
    \]
\end{itemize}

``````latex


\section*{Problem 1}

\subsection*{(a)}

\[
T
\]

1. \(100^\circ C\)

2. \(70^\circ C\)

\[
T_{\text{ein}} = 20^\circ C
\]

\[
Q_{R,12} = Q_{\text{aus},12} = 35 \, \text{MJ}
\]

\text{halb offen}

\[
\Delta E = m_2 u_2 - m_1 u_1 = \Delta m_{12} (h_e) + \cancel{\sum Q} - \cancel{\sum W}
\]

\[
h_e = \text{Tab A-2} \left( T = 20^\circ C, h_f \right) = 83.16 \, \frac{\text{W}}{\text{kg}}
\]

\[
m_2 = m_1 + \Delta m_{12}
\]

\[
m_2 = 5755 \, \text{kg}
\]

\[
u_f = \text{Tab A-2} \left( T = 100^\circ C, u_f \right) = 426.94 \, \frac{\text{W}}{\text{kg}}
\]

\[
u_2 = \text{Tab A-2} \left( T = 100^\circ C, u_f \right) = 292.55 \, \frac{\text{W}}{\text{kg}}
\]

\[
m_1 u_2 + \Delta m_{12} u_2 - m_1 u_1 = \Delta m_{12} h_e
\]

\[
m_1 (u_2 - u_1) = \Delta m_{12} (h_e - u_2)
\]

\[
m_1 \frac{u_2 - u_1}{h_e - u_2} = \Delta m_{12} = 3486.41 \, \text{kg}
\]

``````latex

e) \quad \Delta S = m_2 s_2 - m_1 s_1

\[
= m_1 (s_2 - s_1) + \Delta \dot{m} s_2
\]

\[
s_1 = \text{Tab A-2} \left( T = 100^\circ, s_f \right) = 1.306 \frac{\text{kJ}}{\text{kg K}}
\]

\[
s_2 = \text{Tab A-2} \left( T = 20^\circ, s_f \right) = 0.958 \frac{\text{kJ}}{\text{kg K}}
\]

\[
\Delta S = 1411.88 \frac{\text{kJ}}{\text{K}}
\]

``````latex


