
``````latex


\section*{Aufgabe 1}

\subsection*{a)}
1. HS \underline{Kontinuierlicher} Reaktor:

\[
0 = \dot{m}(h_e - h_a) + \dot{Q}
\]

\[
\dot{Q} = \dot{m}(h_a - h_e) = \dot{m} \cdot c_p \cdot (T_a - T_e)
\]

\[
h_a(T_1) = h_{a,f}(T_1) = 252.18 \frac{\text{kJ}}{\text{kg}}, \quad A = 2
\]

\[
h_e(T_2) = h_{e,f}(T_2) = 449.01 \frac{\text{kJ}}{\text{kg}}, \quad A = 2
\]

\[
\dot{Q} = C \cdot 3 \frac{\text{kg}}{\text{s}} \cdot (252.18 - 449.01) = -37.8 \frac{\text{kJ}}{\text{s}}
\]

\subsection*{b)}
Isobar: aus Vorlesung

\[
\frac{h_2 - h_1}{s_2 - s_1} = \frac{c_p \cdot (T_2 - T_1)}{c_p \cdot \ln \left( \frac{T_2}{T_1} \right)}
\]

\[
\frac{2.88 \cdot 15 - 252.18}{\ln \left( \frac{298.15}{258.15} \right)} = 293.12 \text{K} = \overline{T}
\]

\subsection*{c)}
2. HS aus Vorlesung:

\[
S_{\text{erzeugt}} = \left| \frac{\dot{Q}}{\overline{T}} \left( \frac{1}{T_{\text{hei√ü}}} - \frac{1}{T_{\text{kalt}}} \right) \right| = 37.8 \frac{\text{kJ}}{293.12 \text{K}} \left( \frac{1}{293.12} - \frac{1}{293.15} \right)
\]

\[
= 0.062 \frac{\text{kJ}}{\text{K}}
\]

``````latex


d) 1. HS.

\[
\Delta E = \Delta m_{12}(h) + \dot{Q}
\]

\[
m_2 u_2 - m_1 u_1 = \Delta m_{12} h + \dot{Q}
\]

\[
\Delta m_{12} = \frac{1}{h} (m_2 u_2 - m_1 u_1 - \dot{Q})
\]

\[
h = h_f(20^\circ) = \cancel{88} \ 83.96 \left[\frac{kJ}{kg}\right], \quad A2 \ (\text{illegible text})
\]

\[
\dot{Q} = -35 \text{MJ}
\]

\[
m_2 u_2 - m_1 u_1:
\]

\[
T_1 = 100^\circ C \quad T_2 = 70^\circ C
\]

\[
m_1 = 5755 \text{kg}
\]

\[
m_2 = m_1 + \Delta m
\]

\[
u_2 = u_f(T_2) = 232.15 \left[\frac{kJ}{kg}\right], \quad A2
\]

\[
u_1 = u_f(T_1) = 418.94 \left[\frac{kJ}{kg}\right], \quad A2
\]

\[
\Rightarrow \Delta m_{12} = \frac{1}{h} m_2 u_2 + \frac{1}{h} \Delta m u_2 - m_1 u_1 \frac{1}{h} - \dot{Q} \frac{1}{h}
\]

\[
\Delta m \left(1 - \frac{u_2}{h}\right) = \frac{1}{h} (m_2 u_2 - m_1 u_1 - \frac{\dot{Q}}{h})
\]

\[
\Delta m = \frac{1}{83.96} (5755 \cdot 232.15 - 5755 \cdot 418.94 - \frac{-35 \cdot 10^3}{83.96})
\]

\[
= \cancel{3888} \ 3965.9 \text{kg}
\]

e)

\[
\Delta S = S_2 - S_1 = \cancel{\text{illegible text}}
\]

\[
m_2 s_2 - m_1 s_1
\]

\[
s_2 = s_f(T_2) = 0.9509 \left[\frac{kJ}{kg \cdot K}\right]
\]

\[
s_1 = s_f(T_1) = 1.3069 \left[\frac{kJ}{kg \cdot K}\right]
\]

\[
\Rightarrow (5755 \text{kg} + 3965.9 \text{kg}) \cdot 0.9509 - 5755 \text{kg} \cdot 1.3069 = \cancel{10287.8} \ (\text{illegible text})
\]

``````latex


