
``````latex


3) 

a) 

\underline{ref 1} \quad P_g = P_{amb} + \frac{4 \cdot m_u \cdot g}{D^2 \pi} + \frac{4 \cdot m_{ew} \cdot g}{D^2 \pi} \quad \left| A = \frac{D^2}{4 \pi} \right.

\[
= 1 \text{bar} + \frac{4 \cdot g}{D^2 \pi} (m_u + m_{ew})
\]

\[
= 1 \text{bar} + \frac{4 \cdot 9.81}{(0.7 \text{m})^2 \pi} \left(32 \text{kg} + 0.7 \text{kg}\right)
\]

\[
P_g = \boxed{1.4 \text{bar}}
\]

\[
m_g = \frac{P_g V_{1,1} M}{R \cdot T_{1,1}} = \frac{1.4 \text{bar} \cdot 3.74 \text{L} \cdot 50 \frac{\text{g}}{\text{mol}}}{8.314 \frac{\text{J}}{\text{mol K}} \cdot 77.75 \text{K}}
\]

\[
m_g = \boxed{3.43 \text{g}}
\]

b) 

\[
P_{1,g} = P_{2,g} \quad \text{da sich gleichung ref 1 nicht ver채ndert}
\]

\[
T_2 = T_1 \left( \frac{P_2}{P_1} \right)^{\frac{n-1}{n}} \quad n = \frac{c_p}{c_v} = \frac{R + c_v}{c_v} = \frac{R}{c_v} + 1
\]

\[
= \frac{8.314}{50} + 0.633 = 1.2667
\]

\[
T_2 = 500 \left( \frac{4}{1} \right)^{\frac{0.2667}{1.2667}} \rightarrow 7
\]

\[
T_2 = T_1 \quad \text{da sich der druck nicht 채ndert bleibt T konstant}
\]

``````latex

c)

\begin{align*}
\Delta E &= E_2 - E_1 = Q_{12} \\
&= m_2 u_2 - m_1 u_1 = Q_{12} \\
&= m_2 c_v (T_{g2} - T_{g1})
\end{align*}

\begin{align*}
Q_{12} &= 3,423 \, \text{g} \cdot 0,653 \frac{\text{kJ}}{\text{kgK}} (5000 \degree \text{C} + 0,003 \degree \text{C})
\end{align*}

\[
Q_{12} = 1,0856 \, \text{kJ}
\]

d)

\begin{align*}
u_{1\text{ges}} &= u_{\text{f,est}} + (r-x_1) (u_{\text{f,fl체ssig}} - u_{\text{f,est}}) \\
&= -333,485 + 0,6 \alpha \left( (1-0,6) (-0,005 + 333,458) \right) \\
&= -200,1768 \frac{\text{kJ}}{\text{kg}}
\end{align*}

\[
\boxed{-200,1768 \frac{\text{kJ}}{\text{kg}}}
\]

\begin{align*}
\Delta E &= E_2 - E_1 = Q_{12} \\
Q_{12} &= m_{\text{ew}} (u_{\text{ew}} - u_{\text{ew}}) \\
&= 0 \, \text{m}_{\text{ew}} \left( u_{\text{f,est}} + (r-x_2) (u_{\text{f,fl체ssig}} - u_{\text{f,est}}) - a_1 \right)
\end{align*}

``````latex


3. (d) continued

\begin{equation*}
\frac{Q_{12}}{m_{ew}} = u_{f_{est}} + (1 - x_{2_{eis}})(u_{f_1} - u_{f_{est}}) - u_1
\end{equation*}

\begin{equation*}
\frac{1}{(u_{f_1} - u_{f_{est}})} \left( \frac{Q_{12}}{m_{ew}} - u_{f_{est}} + u_1 \right) = 1 - x_{2_{eis}}
\end{equation*}

\begin{equation*}
1 - \frac{1}{(u_{f_1} - u_{f_{est}})} \left( \frac{Q_{12}}{m_{ew}} - u_{f_{est}} + u_1 \right) = x_{2_{eis}}
\end{equation*}

\begin{equation*}
x_{2_{eis}} = 1 - \frac{1}{(-q_{aus} + 333,485)} \left( \frac{4,0856 \, q}{0,7 \, kg} - 333,458 + 200,000 \right)
\end{equation*}

\begin{equation*}
x_{2_{eis}} = \boxed{0,6828} \quad \boxed{1,567}
\end{equation*}

``````latex


