
``````latex


\section*{1.}
\subsection*{a)}
\begin{align*}
    \dot{Q}_{\text{aus}}: \\
    \dot{Q}_{\text{aus}} &= \dot{Q}_r - \dot{Q}_w \\
    \dot{Q}_w &\rightarrow 0 = \dot{m} (h_e - h_a) + \dot{Q}_w \\
    &\rightarrow \dot{Q}_w = \dot{m} (h_a - h_e) \\
    h_e &= 292,98 + 0,005 (2626,5 - 292,98) = 304,65 \frac{\text{kJ}}{\text{kg}} \\
    h_a &= 419,01 + 0,005 (2676,1 - 419,01) = 430,33 \frac{\text{kJ}}{\text{kg}} \\
    T_{AB} A-2 &\quad T_{AB} A-2 \quad \dot{Q}_w = G_B (430,33 - 304,65) = 37,7 \text{kJ} \\
    L = 100 \text{kg} - 37,7 \text{kg} = 62,30 \text{kJ} = \dot{Q}_{\text{aus}}
\end{align*}

\subsection*{b)}
\begin{align*}
    \frac{T}{T_{KF}} \sqrt{\frac{T}{S_a S_e}} &= \frac{T_a - T_e}{S_a - S_e} = \frac{T_a - T_e}{c \ln \left( \frac{T_a}{T_e} \right)} \quad c \text{ unbekannt} \\
    S_a - S_e &= c \ln \left( \frac{T_e}{T_1} \right) \rightarrow 298 \text{K} \\
    &\Longleftarrow \frac{T_{KF}}{T_{KF}} = \frac{T_1 + T_2}{2} = 293,15 \text{K}
\end{align*}

\subsection*{c)}
\begin{align*}
    \text{mit } T &= 298 \text{K} \\
    0 &= \dot{m} [S_e - S_a] + \frac{\dot{Q}_r}{T} + \dot{S}_{S_e} \\
    \text{für } S_{a+} &= \dot{m} [S_a - S_e] - \frac{\dot{Q}_r}{T} \rightarrow S_{a+} - \frac{\dot{Q}_r}{T} - \frac{37,7}{298 \text{K}} = 127,8 \frac{\text{J}}{\text{K}} \\
    \dot{Q}_r &= 37,7 \frac{\text{kJ}}{\text{kg}} \\
    S_a &=
\end{align*}

\subsection*{d)}
\begin{align*}
    \Delta U &= \Delta m (h_1 - h_2) + Q_{12} - Q_{12} \\
    \Delta U &= \Delta m (h_1 - h_2) \\
    \text{mit} \\
    (m_1 + \Delta m) T_2 c_e - m_1 T_a c_p &= \Delta m (h_1 - h_2) \\
    m_1 T_2 c_p - m_1 T_a c &= \Delta m (h_1 - h_2) - T_2 c \\
    \Delta m &= \frac{m_1 T_2 - m_1 T_a c}{(h_1 - h_2) - T_2 c} \\
    h_1, h_2 \quad T_{AB} A-2 \\
    \text{verkleben und } \Delta m \text{ gelöst}
\end{align*}

``````latex


\begin{itemize}
    \item[d)]
\end{itemize}

\begin{itemize}
    \item[e)] \(\Delta S = \Delta m \Delta s\)
\end{itemize}

``````latex


