
``````latex


\section*{1a) $\dot{Q}_{\text{aus}}$}

\[
0 = \dot{m}_{\text{ein}} \left( h_{\text{ein}} - h_{\text{aus}} \right) + \dot{Q}_R - \dot{q}_{\text{aus}}
\]

\[
\dot{Q}_{\text{aus}} = \dot{m}_{\text{ein}} \left( h_{\text{ein}} - h_{\text{aus}} \right) + \dot{Q}_R
\]

\[
h_{\text{ein}} = h_f(70^\circ C) = 292.98 \frac{\text{kJ}}{\text{kg}} \quad \text{A2}
\]

\[
h_{\text{aus}} = h_f(100^\circ C) = 419.04 \frac{\text{kJ}}{\text{kg}} \quad \text{A2}
\]

\[
\dot{Q}_{\text{aus}} = \underline{62.182 \text{ kW}}
\]

\section*{1b)}

\[
\overline{T}_{k\#} = \frac{\int_{s_2}^{s_1} T \, ds}{s_a - s_e} = \frac{T_{\text{KF ein}} - T_{\text{KF aus}}}{s_{\text{aus}} - s_{\text{ein}}}
\]

\[
s_{\text{aus}} = s_f(15^\circ C) = 0.2245 \frac{\text{kJ}}{\text{kg K}} \quad \text{A2}
\]

\[
s_{\text{ein}} = s_f(25^\circ C) = 0.3674 \frac{\text{kJ}}{\text{kg K}} \quad \text{A2}
\]

\[
T_{k\#} = \frac{T_{\text{KF ein}} - T_{\text{KF aus}}}{s_{\text{aus}} - s_{\text{ein}}} = \underline{70^\circ C}
\]

``````latex


1.c)
\[
0 = \dot{m}_{\text{ein}} (s_e - s_a) + \frac{\dot{Q}_{\text{aus}}}{T_{kf}} + \dot{S}_{erz}
\]
\[
\dot{S}_{erz} = \dot{m}_{\text{ein}} (s_a - s_e) - \frac{\dot{Q}_{\text{aus}}}{T_{kf}}
\]
\[
s_a = s_f (100^\circ C) = 1.3069 \frac{\text{kJ}}{\text{kg K}}
\]
\[
s_e = s_f (70^\circ C) = 0.9549 \frac{\text{kJ}}{\text{kg K}}
\]
\[
\dot{S}_{erz} = -0.105 \frac{\text{kJ}}{\text{K}}
\]

1.d)
\[
\Delta m_{12}
\]
\[
\Delta m_{12} (u_2 - u_1) = \Delta m_{12} (h_1 - h_2) - Q_{\text{aus}}
\]
\[
\Delta m_{12} \left( u_2 - u_1 + h_2 - h_1 \right) = -Q_{\text{aus}}
\]
\[
\Delta m_{12} = \frac{-Q_{\text{aus}}}{u_2 - u_1 + h_2 - h_1} = \frac{83.7 \, \text{kg}}{0.465 \, \frac{\text{kJ}}{\text{kg}}}
\]

\[
u_1 = h_f (20^\circ C) = 83.98 \frac{\text{kJ}}{\text{kg}} \quad \text{A2}
\]
\[
h_2 = h_f (70^\circ C) = 232.98 \frac{\text{kJ}}{\text{kg}} \quad \text{A2}
\]
\[
u_1 = u_f (20^\circ C) = 83.86 \frac{\text{kJ}}{\text{kg}} \quad \text{A2}
\]
\[
u_2 = u_f (70^\circ C) = 232.95 \frac{\text{kJ}}{\text{kg}} \quad \text{A2}
\]

``````latex

1e) \(\Delta S_{12} = \cancel{\cancel{S_2 - S_1}}\)

\[
\Delta S_{12} = \Delta m_{12}(s_2 - s_1) + \frac{Q_{aus,12}}{\overline{T}}
\]

\[
s_1 = s_f(20^\circ C) = 0.2966 \frac{kJ}{kg \cdot K} \quad A2
\]

\[
s_2 = s_f(700^\circ C) = 0.9545 \frac{kJ}{kg \cdot K} \quad A2
\]

\[
\overline{T} = 285 K
\]

\[
\Delta S_{12} = 2.5 \frac{MJ}{kg \cdot K}
\]

``````latex


