
``````latex


3) a) $p_{G,1}, \quad m_g$

\[
p_{G,1} = p_0 + \frac{F_{mech}}{A} = p_0 + \frac{F_{mech}}{A} = p_0 + \left( \frac{32 \, \text{kg} \cdot 9.81 \, \frac{\text{m}}{\text{s}^2} + 0.1 \, \text{kg} \cdot 5.81 \, \frac{\text{m}}{\text{s}^2}}{A} \right)
\]

\[
p_{G,1} = 1.1 \, \text{bar} \Rightarrow \Delta p = 1.4 \, \text{bar}
\]

\[
pV = mRT \Rightarrow m_g = \frac{p_{G,1} V_{G,1}}{R T_{G,1}} = \frac{1.4 \, \text{bar} \cdot 3.14 \cdot 10^{-3} \, \text{m}^3}{8.314 \, \frac{\text{J}}{\text{mol} \cdot \text{K}} \cdot 773.15 \, \text{K}}
\]

\[
m_g = 0.00342 \, \text{kg} = 3.42 \, \text{g}
\]

b) $X > 0$

\[
\Delta E_Q = \Delta E_{EW} \Rightarrow \Delta E_Q - \Delta E_{EW} = 0
\]

\[
\Delta E_Q - \Delta U = m_g c_V (T_2 - T_1)
\]

\[
\Delta E_{EW} = \Delta \dot{m} = \dot{m}_{EW} (T_{2,EW} - T_{1,EW}) = m_{EW} (u_2 - u_1)
\]

c) $\Delta E = E_2 - E_1 = Q_{12}$

\[
\Rightarrow Q_{12} = \Delta U = -m_g c_V (T_{2,G} - T_{1,G}) = -(0.00342 \, \text{kg} \cdot 0.633 \, \frac{\text{kJ}}{\text{kg} \cdot \text{K}} (773.15 \, \text{K} - 293.15 \, \text{K}))
\]

\[
= -1.052 \, \text{kJ}
\]

``````latex

d) \quad t_{\text{ein},2} = t_{\text{ein},2} = 0.003^\circ C

\[
\Rightarrow \Delta E = E_2 - E_1 = Q_{12} = 1500 J
\]

\[
\Delta u_{12} = \frac{1500 J}{m} = m \cdot (u_2 - u_1) = m \cdot \left( \frac{(x_2 \cdot u_{2,\text{fest}} + (1 - x_2) \cdot u_{2,\text{flüssig}})}{(x_1 \cdot u_{1,\text{fest}} + (1 - x_1) \cdot u_{1,\text{flüssig}})} \right)
\]

\[
\Rightarrow \frac{\Delta u_{12}}{m} + (x_1 \cdot u_{1,\text{fest}} + (1 - x_1) \cdot u_{1,\text{flüssig}}) = x_2 \cdot u_{2,\text{fest}} + (1 - x_2) \cdot u_{2,\text{flüssig}}
\]

\[
\Rightarrow x_2 = \frac{\left( \frac{\Delta u_{12}}{m} + (x_1 \cdot u_{1,\text{fest}} + (1 - x_1) \cdot u_{1,\text{flüssig}}) - u_{2,\text{flüssig}} \right)}{u_{2,\text{fest}} - u_{2,\text{flüssig}}}
\]

\[
x_2 = 0.555
\]

``````latex


