
``````latex


\section*{1a)}
\begin{equation*}
0 = \dot{m}_{ein} \left( h_1 - h_2 \right) - \dot{Q}_{aus} + Q_n
\end{equation*}
\begin{equation*}
\dot{Q}_{aus} = \dot{m}_{ein} \left( h_1 - h_2 \right) + Q_R
\end{equation*}
\begin{equation*}
= 62.18 \, \text{kW}
\end{equation*}
\begin{equation*}
h_1 = 232.58 \, \frac{\text{kJ}}{\text{kg}}
\end{equation*}
\begin{equation*}
h_2 = 479.04 \, \frac{\text{kJ}}{\text{kg}}
\end{equation*}

\section*{1b)}
\begin{equation*}
\overline{T} = \frac{\int_{s_e}^{s_2} T \, ds}{s_2 - s_e} = \frac{T_2 s_2 - T_e s_e}{s_2 - s_e}
\end{equation*}
\begin{equation*}
s_2 = 
\end{equation*}
\begin{equation*}
s_e = 
\end{equation*}

\section*{1c)}
\begin{equation*}
0 = \frac{\dot{Q}_{aus}}{\overline{T}} + \dot{S}_{er \, s}
\end{equation*}
\begin{equation*}
\dot{S}_{er \, s} = - \frac{\dot{Q}_{zu}}{\overline{T}}
\end{equation*}

\section*{a)}
\begin{equation*}
\Delta E = m_{ges} \left( u_2 - u_1 \right)
\end{equation*}
\begin{equation*}
= \left( m_{ges,1} + \Delta m_x \right) u_2 - \left( m_{ges,1} \right) u_1 = \Delta m_2 \, h_{wasser@20^\circ C} + Q_{zu}^0
\end{equation*}
\begin{equation*}
h_{wasser@20^\circ C} = 83.86 \, \frac{\text{kJ}}{\text{kg}}, \quad u_2 = 292.85 \, \frac{\text{kJ}}{\text{kg}}
\end{equation*}
\begin{equation*}
u_1 = 0.395 \, u_f + 0.005 \, u_g
\end{equation*}
\begin{equation*}
h_2 = 423.30 \, \frac{\text{kJ}}{\text{kg}}
\end{equation*}

``````latex

\subsection*{1d (continued)}

\begin{equation*}
m_{g0s,1} (u_2 - u_1) + \Delta m_{12} (u_2 - h_{w@20^\circ C}) = 0
\end{equation*}

\begin{equation*}
\Delta m_{12} = -m_{g0s,1} \frac{(u_2 - u_1)}{u_2 - h_{w@20^\circ C}} = 3756.84 \frac{J}{g}
\end{equation*}

\subsection*{e)}

\begin{equation*}
\Delta S_{12} \left( m_{g0s,1} + \Delta m_{12} \right) s_2 - r_{g0s,1} s_1
\end{equation*}

\begin{equation*}
S_1 = 0.995 s_c + 0.005 s_j
\end{equation*}

\begin{equation*}
A^{-2} = 1.337 \frac{J}{kg \cdot K}
\end{equation*}

\begin{equation*}
S_2 = 0.9549 \frac{J}{kg \cdot K}
\end{equation*}

\begin{equation*}
= 1388.42 \frac{J}{K}
\end{equation*}

``````latex


