
``````latex


\section*{A1}

\subsection*{a)}

\begin{align*}
\dot{Q}_{\text{zu}} 
\end{align*}

\begin{align*}
\Delta E = m_2 u_2 - m_1 u_1
\end{align*}

\begin{align*}
\dot{Q}_{\text{zu}} = \dot{m} (u_2 - u_1)
\end{align*}

\begin{align*}
\Delta E = \Delta U
\end{align*}

\begin{align*}
T_1 &= 343.15 \, \text{K} \\
T_2 &= 373.15 \, \text{K}
\end{align*}

\begin{align*}
p_1 &= 1 \, \text{bar} \\
p_2 &= 5 \, \text{bar}
\end{align*}

\begin{align*}
\dot{Q}_{\text{zu}} &= 37 \, \frac{\text{kJ}}{\text{s}}
\end{align*}

\begin{align*}
u_1 &= 288.15 \, \text{K} \\
u_2 &= 258.15 \, \text{K}
\end{align*}

\begin{align*}
\dot{Q}_{\text{zu}} &= 6.288 \, \frac{\text{kJ}}{\text{s}}
\end{align*}

\subsection*{b)}

\begin{align*}
T_{\text{m}} = \frac{\int_{s_a}^{s_e} T \, ds}{s_e - s_a}
\end{align*}

\begin{align*}
s_e &= 288.15 \, \text{K} \\
s_a &= 258.15 \, \text{K}
\end{align*}

\begin{align*}
T_{\text{m}} &= \frac{2.8545 \, \frac{\text{kJ}}{\text{kg} \cdot \text{K}}}{1.3 \, \frac{\text{kJ}}{\text{kg} \cdot \text{K}}}
\end{align*}

\begin{align*}
s_e &= 288.15 \, \text{K} \\
s_a &= 258.15 \, \text{K}
\end{align*}

``````latex

c) \quad \dot{Q}_{\text{ges}} \quad \dot{q} \frac{dS}{dt} = \sum ms + \frac{\dot{Q}}{T} + \dot{S}

d) \quad \text{aus} \quad \dot{Q} = \Delta m_{12} \\
T = 70^\circ C = 343.15 \, K \\
\Delta E = Q - \cancel{W} \quad \cancel{W} = 0 \\
35 \, \text{MJ} = m \left( u_2 - u_1 \right) \\
35 \, 000 \, 000 \, \text{J} = m \left( 418.5 \, \frac{\text{kJ}}{\text{kg}} - 83.55 \, \frac{\text{kJ}}{\text{kg}} \right) \\
35 \, 000 \, 000 \, \text{J} = m \left( 418.5 \, \frac{\text{kJ}}{\text{kg}} - 83.55 \, \frac{\text{kJ}}{\text{kg}} \right) \\
35 \, 000 \, 000 \, \text{J} = m \left( 418.5 \, \frac{\text{kJ}}{\text{kg}} - 83.55 \, \frac{\text{kJ}}{\text{kg}} \right) \\
35 \, 000 \, 000 \, \text{J} = m \left( 418.5 \, \frac{\text{kJ}}{\text{kg}} - 83.55 \, \frac{\text{kJ}}{\text{kg}} \right) \\
35 \, 000 \, 000 \, \text{J} = m \left( 418.5 \, \frac{\text{kJ}}{\text{kg}} - 83.55 \, \frac{\text{kJ}}{\text{kg}} \right) \\
35 \, 000 \, 000 \, \text{J} = m \left( 418.5 \, \frac{\text{kJ}}{\text{kg}} - 83.55 \, \frac{\text{kJ}}{\text{kg}} \right) \\
35 \, 000 \, 000 \, \text{J} = m \left( 418.5 \, \frac{\text{kJ}}{\text{kg}} - 83.55 \, \frac{\text{kJ}}{\text{kg}} \right) \\
35 \, 000 \, 000 \, \text{J} = m \left( 418.5 \, \frac{\text{kJ}}{\text{kg}} - 83.55 \, \frac{\text{kJ}}{\text{kg}} \right) \\
35 \, 000 \, 000 \, \text{J} = m \left( 418.5 \, \frac{\text{kJ}}{\text{kg}} - 83.55 \, \frac{\text{kJ}}{\text{kg}} \right) \\
35 \, 000 \, 000 \, \text{J} = m \left( 418.5 \, \frac{\text{kJ}}{\text{kg}} - 83.55 \, \frac{\text{kJ}}{\text{kg}} \right) \\
35 \, 000 \, 000 \, \text{J} = m \left( 418.5 \, \frac{\text{kJ}}{\text{kg}} - 83.55 \, \frac{\text{kJ}}{\text{kg}} \right) \\
35 \, 000 \, 000 \, \text{J} = m \left( 418.5 \, \frac{\text{kJ}}{\text{kg}} - 83.55 \, \frac{\text{kJ}}{\text{kg}} \right) \\
35 \, 000 \, 000 \, \text{J} = m \left( 418.5 \, \frac{\text{kJ}}{\text{kg}} - 83.55 \, \frac{\text{kJ}}{\text{kg}} \right) \\
35 \, 000 \, 000 \, \text{J} = m \left```latex


