
``````latex


\section*{Problem 1}

\subsection*{a)}

\begin{itemize}
    \item The graph is a plot with the x-axis labeled as "1" and the y-axis labeled as "1".
    \item There are three curves on the graph:
        \begin{itemize}
            \item The first curve is labeled "isotherm" and is a concave curve starting from the origin and increasing.
            \item The second curve is labeled "adiabatic" and is a straight line starting from the origin and increasing at a steeper angle than the isotherm.
            \item The third curve is labeled "polytropic" and is a curve that lies between the isotherm and adiabatic curves.
        \end{itemize}
    \item Points on the graph are labeled as follows:
        \begin{itemize}
            \item Point "1" is at the intersection of the isotherm and polytropic curves.
            \item Point "2" is at the intersection of the polytropic and adiabatic curves.
            \item Point "P" is at the intersection of the isotherm and adiabatic curves.
        \end{itemize}
\end{itemize}

\subsection*{b)}

\[
p_2 = 3.32 \text{ bar}
\]

\[
T_1 = -16^\circ \text{C} \quad p_1 = 1.5 \text{ bar}
\]

\[
\pi = \frac{p_2}{p_1} = \frac{3.32}{1.5} = 2.21
\]

\[
T_2 = -16^\circ \text{C}
\]

\[
\text{OFP} \quad \dot{m}(h_e - h_a) = \dot{Q} - \dot{W}
\]

\[
\text{SFP} \quad \dot{m}(h_e - h_a) = \dot{Q} - \dot{W}
\]

\[
h_e = h_{g}(\text{kur}) = 2641.5 \frac{\text{kJ}}{\text{kg}}
\]

\[
h_e = h_{g}(-16^\circ \text{C}) = 2537.74 \frac{\text{kJ}}{\text{kg}}
\]

\[
\dot{W} = \dot{m}(h_1 - h_e)
\]

\[
\dot{m} = \frac{\dot{W}}{h_1 - h_e} = \frac{0.028 \text{ kW}}{1.0002 \cdot 10^5 \frac{\text{kg}}{\text{h}}}
\]

\subsection*{c)}

\[
1.\text{HS} \quad \dot{m}(h_e - h_a) = \dot{W}
\]

\[
\dot{m} \cdot 1.1(h_e - h_a) = \dot{m}(h_e - h_a) + \dot{Q} - \dot{W}
\]

\[
h_e = h_a
\]

\[
h_{g}(\text{Staur}) = h_a = 43.42 \frac{\text{kJ}}{\text{kg}}
\]

\[
h_a = h_{g}(-16^\circ \text{C})
\]

\[
X_1 = \frac{m_{g}(-16^\circ \text{C})}{m_{g}(-16^\circ \text{C})} = \frac{1.3076}{30.76\%}
\]

\subsection*{d)}

\[
1.\text{HS} \quad \dot{m}(h_e - h_a) + \dot{Q} - \dot{W} = 0
\]

\[
\epsilon_k = \frac{\dot{Q}_{zu}}{\dot{Q}_{ab} - \dot{Q}_{zu}}
\]

\[
\dot{Q}_{zu} = \dot{Q}_k = \dot{m}(h_a - h_e)
\]

\[
= \dot{m}(h_{g}(-16^\circ \text{C})) = 4 \frac{\text{kg}}{\text{h}} \cdot h_{g}(-16^\circ \text{C}) = 833.8 \