
``````latex


1. a)

\[
\dot{Q}_{\text{out}}
\]

\[
\dot{m}(h_2 - h_1) + \dot{Q}_{\text{out}} = 0
\]

\[
\dot{Q}_{\text{out}} = \text{min} \left( \frac{h_{\text{out}} - h_{\text{in}}}{h_{\text{out}} - h_{\text{in}}} \right)
\]

\[
\dot{Q}_{\text{out}} A = 2
\]

\[
h_{\text{out}} = h(T = 190^\circ C, \dot{m} = 0.005) = + h_p + (2-1) h_p = 430.325 \frac{\text{kJ}}{\text{kg}}
\]

\[
h_{\text{in}} = h_{\text{analog}} = 302.649 \frac{\text{kJ}}{\text{kg}}
\]

\[
\dot{Q}_{\text{out}} = 37.702774 \text{W}
\]

b)

\[
\bar{T} = \frac{\int T \, dt}{e}
\]

\[
s_2 - s_1 = \int \frac{\dot{Q}}{T} = 733.792 \frac{\text{kJ}}{\text{kg}} - 7.72 \frac{\text{kJ}}{\text{kg}} = -6.354 \frac{\text{kJ}}{\text{kg}}
\]

\[
= \beta T - s_2 s_1
\]

\[
s_2 - s_1 = \int \frac{e^{\frac{a}{T}}}{T} \, dt = e^{\frac{a}{T}} \ln \left( \frac{T_2}{T_1} \right)
\]

``````latex


\section*{Problem c)}

\begin{equation*}
Q = \dot{m}
\end{equation*}

\begin{equation*}
\dot{S}_{gen,2} = \dot{m} (s_{2} - s_{1}) - \frac{Q_{j}}{T_{j}}
\end{equation*}

\begin{equation*}
= \dot{m} (7.33 \frac{kJ}{kgK} - 7.71 \frac{kJ}{kgK}) - 6.384 \frac{kJ}{kgK}
\end{equation*}

\begin{equation*}
Q_{j} = 384.6 \frac{kJ}{s} = 37.7027 kW
\end{equation*}

\begin{equation*}
T_{j} = 100^\circ C
\end{equation*}

\begin{equation*}
\Rightarrow -2.016231 \frac{kJ}{kgK}
\end{equation*}

\begin{equation*}
\dot{S}_{total} = \dot{S}_{gen,2} = \dot{m} \left( s_{2} - s_{1} \right) - \frac{Q_{j}}{T}
\end{equation*}

\section*{Problem d)}

\begin{equation*}
Q = \dot{m} (h_{1} - h_{2}) + Q_{s}
\end{equation*}

\begin{equation*}
\Rightarrow \dot{m}_{Reactor} h_{f} (T = 200) = \dot{m}_{2} h (T = 20) - (m_{gen} \dot{m}_{2} h (T = 70))
\end{equation*}

\begin{equation*}
= \dot{m}_{gen} h_{f} (T = 20) - \dot{m}_{gen} h (T = 70) = \dot{m}_{gen} h (T = 70) - m_{gen} h (T = 70)
\end{equation*}

\begin{equation*}
= \dot{m}_{2} = \dot{m}_{gen} \frac{h (T = 70) - h (T = 70)}{h (T = 20) - h (T = 70)} = 2765.08 kg
\end{equation*}

``````latex


7.e)

\begin{align*}
\Delta S &= \frac{m_{12} \cdot s_{12}(100)}{m_{12} \cdot (s_{12}-s_{12})} + \\
\Delta S &= \sum_{i=1}^{2} \sum_{j=1}^{0} \frac{Q_{ij}}{T_{ij}} - S_{12} \\
&= (m_{12} - m_{12}) \frac{s_{12}(70^\circ C)}{T} - (m_{12} \cdot m_{12}) \frac{(200^\circ C)}{T} - m_{12} \Delta m_{12} \frac{(150^\circ C)}{T} \\
&= 263.07 \, \text{kg}
\end{align*}

\[
\Delta t = -600.6647 \times S_{12}
\]

``````latex


