
``````latex


\section*{Aufgabe 3}

\subsection*{a)}

\begin{align*}
p_{g,1} &= p_{amb} + (m_k + m_{ew}) \cdot g \cdot \frac{1}{A} \\
&= 1.10^5 \, \text{Pa} + \frac{(m_k + m_{ew}) \cdot g}{A} \\
A &= \pi \cdot d^2 \left[ \frac{\text{m}}{4} \right] = 0.052 \pi \approx 0.0079 \, \text{m}^2 \\
p_{g,1} &= 1.10^5 \, \text{Pa} + \frac{(32 \, \text{kg} + 0.1 \, \text{kg}) \cdot 9.81 \, \frac{\text{m}}{\text{s}^2}}{0.0079 \, \text{m}^2} \\
p_{g,1} &\approx 140094 \, \text{Pa} \\
&\approx 1.4 \, \text{bar}
\end{align*}

\begin{align*}
m_{g,1} \\
pV &= mRT \\
\Rightarrow m_{g,1} &= \frac{RT_{g,1}}{p_{g,1} V_{g,1}} \\
R &= \frac{R}{M_{g,1}} = \frac{8.314 \, \frac{\text{kJ}}{\text{kmol K}}}{50 \, \frac{\text{kg}}{\text{kmol}}} \approx 0.166 \, \frac{\text{kJ}}{\text{kg K}} \\
m_{g,1} &= \frac{1.4 \cdot 10^5 \, \text{Pa} \cdot 3.14 \cdot 10^{-3} \, \text{m}^3}{0.166 \, \frac{\text{kJ}}{\text{kg K}} \cdot (50 + 273.15) \, \text{K}} \\
&\approx 2.92 \, \text{g}
\end{align*}

\subsection*{b)}

\begin{align*}
V_{g,12} &= V_{g,1} \\
p_{g,12} &= \frac{V_{g,1} mRT_{g,2}}{V_{g,1}} \\
p_{amb} \\
p_{g,12} &= p_{g,1} = 1.4 \, \text{bar}
\end{align*}

``````latex


\section*{c)}

\begin{align*}
\Delta U &= Q_{12} - W_{12} \\
U_{A2} &= Q_{A2} - W_{A2,v} \\
&= Q_{A2} = U_{A2} + W_{12,v} \\
U_{A2} &= mc_V (T_2 - T_1) = m \cdot 0.633 \frac{\text{kJ}}{\text{kgK}} \left( 273.15 \text{K} - 773.15 \text{K} \right) \\
&= -3.16 \cdot 4.98 \frac{\text{kJ}}{\text{kg}} \cdot 2.29 \frac{\text{kg}}{m_{g,1}} = -92.496 \text{J} \\
W_{12,v} &= m \int p \, dv = m \frac{R (T_2 - T_1)}{1 - n} \\
n &= \frac{c_p}{c_v} \approx 1.263 \quad , \quad c_p = R + c_v = \frac{R}{M} + c_v = 0.166 \frac{\text{kJ}}{\text{kgK}} + 0.633 \frac{\text{kJ}}{\text{kgK}} \\
&\approx 0.799 \frac{\text{kJ}}{\text{kgK}} \\
W_{12,v} &= 0.00292 \text{kg} \cdot \frac{0.166 (273.15 \text{K} - 773.15 \text{K})}{1 - 1.263} \\
&= 92.496 \text{J} \\
\Rightarrow Q_{12} &= -92.496 \text{J} + 92.496 \text{J} = 0 \text{J}
\end{align*}

\section*{d)}

\begin{align*}
X_{\text{Eis},2} &= \frac{m_{\text{Eis},2}}{m_{\text{EW},2}} = \frac{m_{\text{Eis},2}}{m_{\text{EW},2}} \\
&= \frac{m_{\text{Eis},2}}{0.1 \text{kg}}
\end{align*}

\begin{align*}
m_{\text{Eis},2}
\end{align*}

\begin{align*}
m_{\text{EW}} = m_{\text{W2}}
\end{align*}

``````latex


