
``````latex


\section*{Aufgabe 1}

\subsection*{a) Energiebilanz stationär:}

\[
\dot{Q}_{zu} = \dot{Q}_{ab}
\]

\[
0 = \dot{m}_{ein} h_{ein} - \dot{m}_{aus} h_{aus} + \dot{Q}_{aus}
\]

\[
\Rightarrow \dot{Q}_{aus} = \dot{m}_{aus} h_{aus} - \dot{m}_{ein} h_{ein} \quad | \quad \dot{m}_{ein} = \dot{m}_{aus}
\]

\[
\dot{m} (h_{aus} - h_{ein}) = \int_{T_1}^{T_2} c_{if} dT + v_{if} (p_2 - p_1)
\]

\[
0, da \, isobar
\]

\subsection*{b)}

\[
\overline{T}_{kf} = \frac{\int_{s_a}^{s_e} T \, ds}{s_a - s_e}
\]

\[
= \frac{288.15 + 298.15 \, K}{2} \approx \underline{293.15 \, K}
\]

\subsection*{c) Entropiebilanz stationär:}

\[
0 = \dot{m} (s_e - s_a) + \frac{\dot{Q}_{aus}}{T_{kf}} + \dot{S}_{erzeugt}
\]

\[
\dot{S}_{erzeugt} = \dot{m} (s_a - s_e) + \frac{\dot{Q}_{aus}}{T_{kf}} - \frac{\dot{Q}_{R}}{T_{aus}}
\]

\[
s_a - s_e = \int_{T_a}^{T_2} c \frac{1}{T} dT = c \ln \left( \frac{T_2}{T_a} \right)
\]

\[
= c \ln \left( \frac{298.15}{288.15} \right)
\]

``````latex

\section*{Problem d)}

\begin{equation*}
\frac{dE}{dt} = \dot{m}(h_1 - h_2) + \sum \dot{Q} - \sum \dot{W}
\end{equation*}

\begin{equation*}
\Delta E = \Delta m_{12} (h_1 - h_2)
\end{equation*}

\begin{equation*}
\Delta E = \Delta U = U_2 - U_1
\end{equation*}

\begin{equation*}
\Rightarrow \Delta m_{12} = \frac{u_2 - u_1}{h_1 - h_2} = \frac{c(T_2 - T_1)}{c(T_1 - T_2)} = \infty
\end{equation*}

\section*{Problem e)}

\begin{equation*}
\frac{dS}{dt} = \dot{m}(s_1 - s_2) + \sum \frac{\dot{Q}}{T} + \dot{s}_{erz}
\end{equation*}

\begin{equation*}
\Delta S_{12} = \Delta m_{12} (s_1 - s_2) + \frac{\dot{Q}}{T} + \dot{s}_{erz}
\end{equation*}

\begin{equation*}
= \Delta m_{12} (s_1 - s_2)
\end{equation*}

\begin{equation*}
s_1 - s_2 = \int_{T_2}^{T_1} \frac{c}{T} dT = c \ln \left( \frac{T_1}{T_2} \right)
\end{equation*}

``````latex


