
``````latex


\section*{Aufgabe 1}

\subsection*{a) Energiebilanz}

\[
Q = \dot{m} [h_1 - h_2] - \dot{Q}_{\text{Aus}} + \dot{Q}_R
\]

\[
\dot{Q}_{\text{Aus}} = \dot{m} [h_1 - h_2] + \dot{Q}_R
\]

\[
h_1 = h_f \text{ at } 70^\circ \text{C} \rightarrow \text{aus A-2}
\]

\[
h_1 = 292,58 \, \text{c}^\circ
\]

\[
h_2 = h_f \text{ at } 130^\circ \text{C} \rightarrow \text{aus A-2}
\]

\[
h_2 = 419,04 \, \text{c}^\circ
\]

\[
\rightarrow \dot{Q}_{\text{Aus}} = 0.3 [292,58 - 419,04] + 100
\]

\[
\dot{Q}_{\text{Aus}} = 62,182 \, \text{kW}
\]

\subsection*{b)}

\[
\overline{T} = \frac{\int_{a}^{b} T \, dS}{S_a - S_e}
\]

\[
\overline{T} = \frac{h_a - h_e}{S_a - S_e}
\]

\[
\overline{T} = 293,214
\]

\[
S_a \rightarrow \text{aus A-2} = 0,3674
\]

\[
S_e \rightarrow \text{aus A-2} = 0,2445
\]

\[
h_e \rightarrow \text{aus A-2} = 62,55
\]

\[
h_a \rightarrow \text{aus A-2} = 124,85
\]

\subsection*{c) Entropie-Bilanz}

\[
Q = \dot{m} [S_e - S_a] + \frac{\dot{Q}}{T} + S_{e2}
\]

\[
S_{e2} = \dot{m} [S_a - S_e] = \frac{\dot{Q}_R}{T_R} + \frac{\dot{Q}_{\text{Aus}}}{\overline{T}}
\]

\[
= 458,7 \, \text{J/K}
\]

``````latex


\section*{d)}

\textbf{Energieblanz}
\begin{equation*}
m_2 u_2 - m_1 u_1 = \Delta m h_{\text{ein}} + \sum Q
\end{equation*}

\begin{equation*}
(1m - \Delta m) u_2 - m_1 u_1 - \Delta m h_{\text{ein}} = Q_{\text{umluft}}
\end{equation*}

\begin{equation*}
u_2 = u_4 + \cancel{u_3} \quad 70^\circ \rightarrow \text{Aus A2}
\end{equation*}

\begin{equation*}
= \cancel{u_3} \quad 252,55
\end{equation*}

\begin{equation*}
u_1 = u_4 + x (u_5 - u_4) \quad \text{at } 120^\circ \rightarrow \text{Aus A2}
\end{equation*}

\begin{equation*}
= 425,377
\end{equation*}

\begin{equation*}
h_{\text{ein}} = h_f \quad \text{at } 70^\circ = 83,58 \rightarrow \text{Aus A2}
\end{equation*}

\begin{equation*}
m_1 (u_2 - \Delta m u_2 - m_1 u_1 - \Delta m h_{\text{ein}} - Q
\end{equation*}

\begin{equation*}
- \Delta m (u_2 + h_{\text{ein}}) + m_1 u_2 - m_1 u_1 = Q
\end{equation*}

\begin{equation*}
\Delta m = \frac{Q + m_1 u_1 - m_1 u_2}{u_2 + h_{\text{ein}}} = 2.883 \, \text{J} \, 54 \, \text{kg}
\end{equation*}

\section*{e)}

\begin{equation*}
\Delta S = \sum \frac{\Delta Q}{T} = \sum m_2 s_2 - m_1 s_1
\end{equation*}

\begin{equation*}
\Delta S = m_2 s_2 - m_1 s_1 = S
\end{equation*}

\begin{equation*}
m_2 = 9355 \quad (\Delta m = 3600)
\end{equation*}

\begin{equation*}
s_1 = s_f + x (s_g - s_f) = 1,337
\end{equation*}

\begin{equation*}
s_2 = 9.9548
\end{equation*}

\begin{equation*}
\rightarrow \Delta S = 1238,6 \, \text{kg}
\end{equation*}

``````latex


