
``````latex


\section*{Aufgabe 1}

\subsection*{a)}

\begin{align*}
Q &= \dot{m}_{ein} (h_{ein} - h_{aus}) + \dot{C}_{aus} \dot{W} + Q_R \\
\dot{C}_{aus} &= \dot{m}_{ein} (h_{aus} - h_{ein}) \\
h_{ein} &= h_f (70^\circ C) = 292,98 \frac{kJ}{kg} \quad \text{TAB A2} \\
h_{aus} &= h_f (100^\circ C) = 419,04 \frac{kJ}{kg} \quad \text{TAB A2} \\
\dot{C}_{aus} &= 0.3 \frac{kg}{s} (419,04 \frac{kJ}{kg} - 292,98 \frac{kJ}{kg}) - 100 \frac{kJ}{s} \\
&= -67,182 \frac{kJ}{s}
\end{align*}

\begin{quote}
Vorzeichen nach Vorzeichenkonvention wie auf Zusammenfassung
\end{quote}

\subsection*{b)}

\begin{align*}
\overline{T}_{kF} &= \frac{\int_{e}^{a} T \cdot dS}{S_a - S_e} \\
S_a - S_e &= -C_p \\
\overline{T}_{kF} &= \frac{2 \cdot 258,15 K + 293,15 K}{2} \\
&= 293,15 K
\end{align*}

``````latex

\[
\overline{T}_{\text{Utk}} = 295 \, \text{K}
\]

c)

\[
Q = \dot{m} \left( S_{\text{ein}} - S_{\text{out}} \right) + \frac{\dot{Q}_{\text{aus}}}{\overline{T}_{\text{Utk}}} = m \cdot \dot{S}_{\text{ez}}
\]

\[
\dot{S}_{\text{ez}} = \dot{m} \left( S_{\text{aus}} - S_{\text{ein}} \right) + \frac{\dot{Q}_{\text{aus}}}{\overline{T}_{\text{Utk}}}
\]

\[
\dot{S}_{\text{ez}} = \dot{m} \left( S_{\text{aus}} - S_{\text{ein}} \right) + \frac{\dot{Q}_{\text{aus}}}{\overline{T}_{\text{Utk}}}
\]

\[
S_{\text{out}} = S_f (70^\circ \text{C}) = 0.85 \, \frac{\text{kJ}}{\text{kgK}}
\]

\[
S_{\text{ein}} = S_f (100^\circ \text{C}) = 1.306 \, \frac{\text{kJ}}{\text{kgK}}
\]

\[
\dot{m} = 0.3 \, \frac{\text{kg}}{\text{s}} \left( 1.306 \, \frac{\text{kJ}}{\text{kgK}} - 0.85 \, \frac{\text{kJ}}{\text{kgK}} \right) + \frac{62.182 \, \frac{\text{kJ}}{\text{s}}}{295 \, \text{K}}
\]

\[
= 0.316 \, \frac{\text{kJ}}{\text{K}}
\]

``````latex


\section*{Fortsetzung Aufgabe d)}

\subsection*{d) $\Delta m_{12}$}

\begin{align*}
m_2 u_2 - m_1 u_1 &= \Delta m_{12} h_{12} + Q_{k12} \\
m_1 &= 5755 \, \text{kg} \\
m_2 &= 5755 \, \text{kg} + \Delta m_{12} \\
u_2 &= u_{2f} (30^\circ \text{C}) = 292,95 \, \frac{\text{kJ}}{\text{kg}} \quad \text{TAB A2} \\
u_n &= u_f + x_D (u_g - u_f) \\
&= (418,94 + 0.005 (2506,5 - 418,94)) \, \frac{\text{kJ}}{\text{kg}} \quad \text{Werte aus TAB A2 bei 100Â°C} \\
&= 429,3378 \, \frac{\text{kJ}}{\text{kg}} \\
h_{12} &= h_f (20^\circ \text{C}) = 83,96 \, \frac{\text{kJ}}{\text{kg}} \quad \text{TAB A2}
\end{align*}

\begin{align*}
(m_1 + \Delta m_{12}) u_2 - m_1 u_1 &= \Delta m_{12} h_{12} + Q_{k12} \\
\Delta m_{12} &= \frac{m_1 u_2 - m_1 u_1 - Q_{k12}}{h_{12} - u_2} \\
&= 3538,57 \, \text{kg}
\end{align*}

``````latex


\section*{e)}

\begin{align*}
\Delta S_{12} &= m_2 S_2 - m_1 S_1 + \Delta m_{12} S_{12}
\end{align*}

\begin{align*}
S_2 &= S_f (30^\circ C) = 0,95 \frac{kg}{kg} \quad \text{TAB A2}
\end{align*}

\begin{align*}
S_2 &= S_f + x_0 (S_g - S_f) \\
&= 1.3337 \frac{kg}{kg} \quad \text{werte aus TAB A2 bei 100^\circ C}
\end{align*}

\begin{align*}
S_{12} &= S_f (20^\circ C) = 0,2966 \frac{kg}{kg} \quad \text{TAB A2}
\end{align*}

\begin{align*}
\Delta S_{12} &= 130,455 \frac{kg}{kg}
\end{align*}

``````latex


