
``````latex


2

a)

\[
\begin{array}{c}
\text{Graph with the following details:} \\
\text{Y-axis labeled as } T [K] \\
\text{X-axis labeled as } s \left[ \frac{kJ}{kg \cdot K} \right] \\
\text{The graph contains a closed loop with points labeled 1, 2, 3, 4, 5, and 6.} \\
\text{Point 1 is connected to point 2 with a curve.} \\
\text{Point 2 is connected to point 3 with a straight line.} \\
\text{Point 3 is connected to point 4 with a curve.} \\
\text{Point 4 is connected to point 5 with a straight line.} \\
\text{Point 5 is connected to point 6 with a curve.} \\
\text{Point 6 is connected back to point 1 with a curve.} \\
\text{Points 1, 2, 3, 4, 5, and 6 are labeled as follows:} \\
\text{Point 1: } p_1 \\
\text{Point 2: } p_r \\
\text{Point 3: } p_2 \\
\text{Point 4: } p_3 \\
\text{Point 5: } p_4 \\
\text{Point 6: } p_0 \\
\end{array}
\]

b)

\[
T_6 = T_5 \left( \frac{p_6}{p_5} \right)^{\frac{n-1}{n}}
\]

\[
= 437.9 K \left( \frac{0.1019 \cdot 10^5 \frac{N}{m^2}}{0.5 \cdot 10^5 \frac{N}{m^2}} \right)^{\frac{1.4-1}{1.4}}
\]

\[
= 328.07 K
\]

\[
0 = m \left( h_e - h_a - \frac{w_e^2 - w_a^2}{2} \right)
\]

\[
h_a - h_e = \frac{w_e^2 - w_a^2}{2} \quad (1)
\]

\[
c_{p} (T_6 - T_5) = \frac{w_0^2 - w_6^2}{2}
\]

\[
\sqrt{2 c_{p} (T_6 - T_5) + w_5^2} = w_6
\]

\[
w_6 = \sqrt{2 \cdot 1.006 \frac{kJ}{kg \cdot K} (328.07 K - 437.9 K) + (220 \frac{m}{s})^2}
\]

\[
= 507.25 \frac{m}{s}
\]

c)

\[
R = c_{p} - c_{v}
\]

\[
R = \frac{c_{p}}{c_{v}} - \frac{c_{p}}{n}
\]

\[
= 1.006 \frac{kJ}{kg \cdot K} - \frac{1.006 \frac{kJ}{kg \cdot K}}{1.4}
\]

\[
= 722.85 \frac{kJ}{kg \cdot K}
\]

``````latex


\[
-e_{x,sirr,0} = -e_{x,sirr,0}
\]

\[
e_{x,sirr,0} = (h_2 - h_0 - T_0 (s_2 - s_0) - \Delta \text{kcl})
\]

\[
= c_{p,mix} (T_0 - T_0) - T_0 \left( c_{p,mix} \ln \left( \frac{T_0}{T_0} \right) - R \ln \left( \frac{p_0}{p_0} \right) \right) + \left( \frac{w_2^2 - w_0^2}{2} \right)
\]

\[
= c_{p,mix} (T_0 - T_0) - T_0 \left( c_{p,mix} \ln \left( \frac{T_0}{T_0} \right) - R \ln \left( \frac{p_0}{p_0} \right) \right) + \left( \frac{w_2^2 - w_0^2}{2} \right)
\]

\[
= \dot{m}_{ges} \left( 1,006 \frac{\text{kJ}}{\text{kgK}} (328,0 K - 293,15 K) - 2,493,75 \frac{\text{kJ}}{\text{kg}} \ln \left( \frac{1}{1} \right) + \frac{1,006 \frac{\text{kJ}}{\text{kgK}}}{2,493,75 \frac{\text{kJ}}{\text{kg}}} \right)
\]

\[
= -722,88 \frac{\text{kJ}}{\text{kg}} \ln \left( \frac{1}{1} \right) + \left( \frac{502,78 \frac{\text{kJ}}{\text{kg}}}{2,493,75 \frac{\text{kJ}}{\text{kg}}} \right)
\]

\[
= 120,8 \frac{\text{kJ}}{\text{kg}}
\]

\[
d)
\]

\[
0 = - (e_{x,sirr,0} - e_{x,sirr,0})
\]

\[
= - (e_{x,sirr,0} - e_{x,sirr,0}) + \left( 1 - \frac{T_0}{T} \right) \cdot \left( \frac{2,493,75 \frac{\text{kJ}}{\text{kg}}}{2,493,75 \frac{\text{kJ}}{\text{kg}}} \right)
\]

\[
= -120,8 \frac{\text{kJ}}{\text{kg}} + \left( 1 - \frac{2,493,75 \frac{\text{kJ}}{\text{kg}}}{2,493,75 \frac{\text{kJ}}{\text{kg}}} \right) \cdot 1,295 \frac{\text{kJ}}{\text{kg}}
\]

\[
= 845,38 \frac{\text{kJ}}{\text{kg}} \quad (= e_{x,verl})
\]

\[
\text{alles kein "e"}
\]

\[
= e_{x,1,0,3}
\]

``````latex


