
``````latex


\section*{Aufgabe 1}

\subsection*{a)}
\begin{align*}
    h_e &= h_f(T = 70^\circ C) = 292.98 \frac{kJ}{kg} \\
    h_a &= h_f(T = 100^\circ C) = 479.04 \frac{kJ}{kg} \\
    0 &= \dot{m}(h_e - h_a) + \sum \dot{Q} \\
    &= \dot{m}(h_e - h_a) + \dot{Q}_R - \dot{Q}_{\text{aus}} \\
    \dot{Q}_{\text{aus}} &= 0.3 \frac{kg}{s} (292.98 \frac{kJ}{kg} - 479.04 \frac{kJ}{kg}) + 100 kW \\
    &= \boxed{62.182 \, kW}
\end{align*}

\subsection*{b)}
da isobar
\[
\overline{T} = \frac{T_2 - T_1}{\ln(\frac{T_2}{T_1})}
\]
\[
= \boxed{293.72 \, K}
\]

\subsection*{c)}
\[
\overline{T}_2 = 293.72 \, K
\]
Graphical description: There is a horizontal line with an upward arrow labeled $\dot{Q}_{\text{aus}}$ pointing upwards from the line. Below this line, there is another horizontal line with an upward arrow labeled $\dot{Q}_{\text{aus}}$ pointing upwards from the line. To the right of these lines, there is a handwritten note: $\dot{S}_{\text{erzeugt}} = \frac{\dot{Q}_{\text{aus}}}{293.72}$.

\[
T_1 = 70^\circ C = 373.15 \, K
\]
\[
0 = \dot{m}(h_e - h_a) + \frac{\dot{Q}_{\text{aus}}}{T_2} - \frac{\dot{Q}_{\text{aus}}}{T_1} = \dot{S}_{\text{erzeugt}}
\]
\[
\dot{S}_{\text{erzeugt}} = \dot{Q}_{\text{aus}} \left( \frac{1}{T_2} - \frac{1}{T_1} \right)
\]
\[
= 62.182 \frac{kW}{K} = \boxed{45.497 \, \frac{W}{K}}
\]

``````latex


T = 70^\circ C

\begin{itemize}
    \item[(a)] 
    \begin{align*}
        h_1 &= x_D h_g + (1 - x_D) h_f \\
        &= \boxed{930.32 \frac{kJ}{kg}}
    \end{align*}
    
    h_2 = h_f (T = 70^\circ C) = \boxed{292.49 \frac{kJ}{kg}}
    
    \text{halboffenes System}
    
    m_2 u_2 - m_1 u_1 &= \Delta m \left[ h_e - h_2 \right] + Q \\
    u_2 &= u_f (T = 20^\circ C) = \boxed{292.95 \frac{kJ}{kg}} \\
    u_1 &= x_D u_g (T = 100^\circ C) + (1 - x_D) u_f (T = 20^\circ C) \\
    &= \boxed{929.378 \frac{kJ}{kg}}
    
    (m_1 + \Delta m) u_2 - m_1 u_1 &= \Delta m h_{em} + \cancel{Q} \\
    0 &= m_1 u_2 - m_1 u_1 + Q \\
    &= \frac{h_{em} - u_2}{u_1 - u_2}
    
    h_{em} = h_f (T = 20^\circ C) = \boxed{83.96 \frac{kJ}{kg}}
    
    m_1 = \boxed{5755 kg}
    
    Q = \boxed{35000 kJ}
    
    \Delta m = \boxed{3589.37 kg}
\end{itemize}

``````latex


1. e)

\begin{align*}
\Delta S_{12} &= \Delta S_{12} = m_2 s_2 - m_1 s_1 \\
\Delta S_{12} &= m_2 s_2 - m_1 s_1 \\
m_2 &= 0m + m_1 = 9349.37 \, \text{kg} \\
s_2 &= s_f (700^\circ \text{C}) = 0.9549 \, \frac{kJ}{kgK} \\
s_1 &= x \cdot s_g + (1 - x) s_f = 1.3377 \, \frac{kJ}{kgK} \quad \text{at} \quad 700^\circ \text{C} \\
\Delta S_{12} &= 7227.93 \, \frac{kJ}{K}
\end{align*}

``````latex


