
``````latex


\section*{Aufgabe 1}

\subsection*{a)}

\begin{equation*}
\begin{array}{c}
\text{1} \quad \xrightarrow{Q_{\text{ab}}} \quad \text{2} \\
T_1 = 70^\circ C \quad \quad T_2 = 100^\circ C
\end{array}
\end{equation*}

\begin{equation*}
0 = \dot{m}(h_1 - h_2) + \dot{Q}_{\text{ab}} \quad \Rightarrow \quad \dot{Q}_{\text{ab}} = \dot{m}(h_2 - h_1) = \dot{Q}_{\text{aus}} + \dot{Q}_R
\end{equation*}

\begin{equation*}
h_2 = \text{nur der fl√ºssige Anteil geht raus:}
\end{equation*}

\begin{equation*}
h_2(T = 100^\circ C) = 419,04 \frac{\text{kJ}}{\text{kg}}
\end{equation*}

\begin{equation*}
h_1:
\end{equation*}

\begin{equation*}
h_1(T = 70^\circ C) = 292,88 \frac{\text{kJ}}{\text{kg}}
\end{equation*}

\begin{equation*}
\Rightarrow \quad \dot{Q}_{\text{ab}} = \dot{m}(h_2 - h_1) \quad \Rightarrow \quad \dot{Q}_R = 0.3 \frac{\text{kg}}{\text{s}} (419,04 - 292,88) \frac{\text{kJ}}{\text{kg}} = 107,818 \text{kW}
\end{equation*}

\subsection*{b)}

\begin{equation*}
\overline{T} = \frac{\int_{S_a}^{S_e} T dS}{\int_{S_a}^{S_e} dS} = T_{dS} = \text{ideale Gastheorie} \quad \Rightarrow \quad C \ln \left( \frac{T_{K, \text{aus}}}{T_{K, \text{ein}}} \right) = \text{isobar} = h_{K, \text{aus}} - h_{K, \text{ein}}
\end{equation*}

\begin{equation*}
= \frac{T_{\text{aus}} - T_{\text{ein}}}{\ln \left( \frac{T_{\text{aus}}}{T_{\text{ein}}} \right)} = \frac{298,15 \text{K} - 288,15 \text{K}}{\ln \left( \frac{298,15 \text{K}}{288,15 \text{K}} \right)} \approx 293,1 \text{K}
\end{equation*}

\subsection*{c)}

\begin{equation*}
\text{System um die Wand:}
\end{equation*}

\begin{equation*}
0 = \frac{\dot{Q}_{\text{aus}}}{T_{\text{Reaktor}}} - \frac{\dot{Q}_{\text{aus}}}{T_{KF}} + \dot{S}_{\text{erz}}
\end{equation*}

\begin{equation*}
\Rightarrow \quad \dot{S}_{\text{erz}} = \frac{\dot{Q}_{\text{aus}}}{T_{KF}} - \frac{\dot{Q}_{\text{aus}}}{T_{\text{Reaktor}}}
\end{equation*}

\begin{equation*}
= \frac{65 \text{kW}}{293,1 \text{K}} - \frac{65 \text{kW}}{373,15 \text{K}} \approx -16,21 \frac{\text{kW}}{\text{K}}
\end{equation*}

\begin{equation*}
\text{(T_{\text{Reaktor}} = 100^\circ C = 373,15 \text{K})}
\end{equation*}

\subsubsection*{Description of the diagram in part (c):}

The diagram```latex


a)

\[
\frac{dE}{dt} = + \dot{Q} \implies \Delta V_{12} = Q_{\text{aus,12}}
\]

\[
\Delta m_{12} \left( u_{2,E} U_{k4} \right) + m_{\text{ges}} \left( u_{2,\text{gas}} - u_{A,\text{gas}} \right) = -35 \text{MJ}
\]

\[
\Delta m_{12} C \left( T_2 - T_{\text{ein,12}} \right) + m_{\text{ges}} C \left( T_2 - T_{\text{Reaktor,1}} \right) = -35 \text{MJ}
\]

\[
\Delta m_{12} C \left( T_2 - T_{\text{ein,12}} \right) = -35 \text{MJ} - m_{\text{ges}} C \left( T_2 - T_{\text{Reaktor,1}} \right)
\]

\[
\Delta m_{12} = -\frac{35 \text{MJ}}{C} - \frac{m_{\text{ges}} \left( T_2 - T_{\text{Reaktor,1}} \right)}{T_2 - T_{\text{ein,12}}}
\]

\[
1 = \frac{1}{1 - 35 \text{MJ}} - \frac{m_{\text{ges}} \left( u_{2,\text{gas}} - u_{\text{gas}} \right)}{u_{2,k} - u_{k4}}
\]

\[
u_{\text{Reaktor,1}} = 418,94 \frac{\text{kJ}}{\text{kg}} + 0,005 \left( 2506,5 - 418,94 \right) \frac{\text{kJ}}{\text{kg}} = 423,38 \frac{\text{kJ}}{\text{kg}}
\]

\[
u_{K,1} = 83,55 \frac{\text{kJ}}{\text{kg}}
\]

\[
u_2 =
\]

``````latex


