
``````latex

1) a) $\dot{Q}_{\text{aus}} \quad \text{gr}$

\[
0 = \dot{m}_k \left[ h_2 - h_a \right] + \dot{Q}_R - \dot{Q}_{\text{aus}}
\]

\[
h_e = h(70^\circ)
\]

\[
h_a = h(100^\circ)
\]

b) \quad $0 = \dot{m} \left[ s_e - s_a \right] + \dot{Q}''_{\text{aus}}$

c) \quad $\dot{S}_{\text{rez}} = \dot{m} \left[ s_e - s_e \right] - \frac{\dot{Q}''_{\text{aus}}}{T_j} = \frac{\dot{Q}}{T_k}$

\[
\begin{array}{c}
\begin{array}{c}
\begin{array}{c}
\begin{array}{c}
\begin{array}{c}
\begin{array}{c}
\begin{array}{c}
\begin{array}{c}
\begin{array}{c}
\begin{array}{c}
\begin{array}{c}
\begin{array}{c}
\begin{array}{c}
\begin{array}{c}
\begin{array}{c}
\begin{array}{c}
\begin{array}{c}
\begin{array}{c}
\begin{array}{c}
\begin{array}{c}
\begin{array}{c}
\begin{array}{c}
\begin{array}{c}
\begin{array}{c}
\begin{array}{c}
\begin{array}{c}
\begin{array}{c}
\begin{array}{c}
\begin{array}{c}
\begin{array}{c}
\begin{array}{c}
\begin{array}{c}
\begin{array}{c}
\begin{array}{c}
\begin{array}{c}
\begin{array}{c}
\begin{array}{c}
\begin{array}{c}
\begin{array}{c}
\begin{array}{c}
\begin{array}{c}
\begin{array}{c}
\begin{array}{c}
\begin{array}{c}
\begin{array}{c}
\begin{array}{c}
\begin{array}{c}
\begin{array}{c}
\begin{array}{c}
\begin{array}{c}
\begin{array}{c}
\begin{array}{c}
\begin{array}{c}
\begin{array}{c}
\begin{array}{c}
\begin{array}{c}
\begin{array}{c}
\begin{array}{c}
\begin{array}{c}
\begin{array}{c}
\begin{array}{c}
\begin{array}{c}
\begin{array}{c}
\begin{array}{c}
\begin{array}{c}
\begin{array}{c}
\begin{array}{c}
\begin{array}{c}
\begin{array}{c}
\begin{array}{c}
\begin{array}{c}
\begin{array}{c}
\begin{array}{c}
\begin{array}{c}
\begin{array}{c}
\begin{array}{c}
\begin{array}{c}
\begin{array}{c}
\begin{array}{c}
\begin{array}{c}
\begin{array}{c}
\begin{array}{c}
\begin{array}{c}
\begin{array}{c}
\begin{array}{c}
\begin{array}{c}
\begin{array}{c}
\begin{array}{c}
\begin{array}{c}
\begin{array}{c}
\begin{array}{c}
\begin{array}{c}
\begin{array}{c}
\begin{array}{c}
\begin{array}{c}
\begin{array}{c}
\begin{array}{c}
\begin{array}{c}
\begin{array}{c}
\begin{array}{c}
\begin{array}{c}
\begin{array}{c}
\begin{array}{c}
\begin{array}{c}
\begin{array}{c}
\begin{array}{c}
\begin{array}{c}
\begin{array}{c}
\begin{array}{c}
\begin{array}{c}
\begin{array}{c}
\begin{array}{c}
\begin{array}{```latex


c)

\[
\Delta E = \Delta U = Q - W \quad \Rightarrow \Delta Q = \Delta U + W = -1229.183 \, J
\]

\[
\Delta U = mc_V (T_2 - T_1) = -1139.393 \, \text{J}
\]

\[
W = \frac{R(T_2 - T_1)}{1.4 - 1} \cdot m = -89.789 \, \text{J}
\]

d)

\[
x_{Eis,2 \, \text{ges}} = \frac{m_{Rest}}{m_{Rest} + m_{FlÃ¼ssig}}
\]

\[
u_2 - u_1 = c_V \left( \frac{T_2 - T_1}{T_1} \right) \quad \Rightarrow \Delta u_2 = -200.091 \, \text{kJ/kg}
\]

\[
x \cdot u_{Eis,0^\circ} + (1 - x) \cdot u_{Fl,0^\circ} = -200.093 \, \text{kJ/kg}
\]

\[
u_2 = x \cdot u_{Eis,0.03^\circ} + (1 - x) \cdot u_{Fl,0.03^\circ}
\]

\[
\Rightarrow x = 0.600
\]

``````latex


