
``````latex


\section*{Aufgabe 1}

\subsection*{a) Q aus}
\textit{Verbrennung flüssiggas}

\[
0 = \dot{m} \int (h_e - h_a + ke + pe) + \sum_j (\dot{G}_j) - \sum_n (\dot{V}_n h_n)
\]

\[
= \dot{m}_{ein} (h_e - h_a) + \dot{Q}_R - Q_{aus}
\]

\[
Q_{aus} = \dot{m}_{ein} (h_e - h_a) + \dot{Q}_R
\]

\[
= 61,972 \, kW
\]

\subsection*{b)}

\[
\overline{T}_{kF} = \frac{\int_{a}^{e} T ds}{s_e - s_a} = \frac{\Delta h}{s_e - s_a} = \frac{h_a - h_e}{s_e - s_a} = 360,11 \, K
\]

\subsection*{c)}

\[
\dot{S}_{erf} = \sum_j \frac{\dot{Q}_j}{T_j} \quad \text{durch Umwandlung}
\]

\subsection*{d)}

\[
\overline{T}_{kF} = \frac{\int_{a}^{e} T ds}{s_e - s_a} = \frac{\Delta h}{s_e - s_a} = \frac{h_a - h_e}{s_e - s_a}
\]

\[
= 293,72 \, K
\]

\subsection*{Tabelle 2}

\begin{align*}
h_e (70^\circ C, x=0) &= 297,28 \, \frac{kJ}{kg} \\
s_e (70^\circ C, x=0) &= 1,3069 \, \frac{kJ}{kg \cdot K} \\
h_a (90^\circ C, x=0) &= 419,94 \, \frac{kJ}{kg} \\
s_a (90^\circ C, x=0) &= 0,941 \, \frac{kJ}{kg \cdot K} \\
h_{af} (70^\circ C) &= 89,34 \\
h_e (70^\circ C) &= 48,70 \\
s_e (70^\circ C) &= 0,185 \\
s_a (70^\circ C) &= 0,3703 \\
h_a (25^\circ C) &= 104,81 \\
h_e (25^\circ C) &= 62,91 \\
s_e (25^\circ C) &= 0,2445 \\
s_a (25^\circ C) &= 0,3674 \\
\end{align*}

``````latex


\section*{c)}
\begin{equation*}
    \dot{S}_{\text{ers}} = \frac{\dot{Q}}{T_j}
\end{equation*}
\begin{equation*}
    = \frac{\dot{Q}_{\text{aus}}}{T} = 0.711 \frac{\text{kW}}{\text{K}}
\end{equation*}

\section*{d)}
\textbf{Treadstor auf 70°C} \\
\begin{equation*}
    x = 0
\end{equation*}
\text{4 mm-Zylinder Reaktor} \\
\text{Treadstor = 100°C} \\
\text{T}_{\text{ein}} = 20°C \\
\text{Q}_{\text{aus}} = 3.5 \frac{\text{kJ}}{\text{K}} \\

\textbf{halboffenes System} \\
\begin{equation*}
    \Delta E = m_1 u_2 - m_1 u_1 = \Delta m_{12} \left( h_{20°C} \right) + Q - W
\end{equation*}
\begin{equation*}
    \Delta m_{12} = \frac{m_1 u_2 - m_1 u_1 - Q}{h_{20°C}}
\end{equation*}
\begin{equation*}
    = \frac{(m_1 + \Delta m_{12}) u_2 - m_1 u_1 = \Delta m_{12} h + Q}{h - u}
\end{equation*}
\begin{equation*}
    \Delta m_{12} h - \Delta m_{12} u = m_1 u_2 - m_1 u_1 - Q
\end{equation*}
\begin{equation*}
    \Delta m_{12} = \frac{m_1 u_2 - m_1 u_1 - Q}{h - u}
\end{equation*}
\begin{equation*}
    \Delta m_{12} = 574.41 \text{ kg}
\end{equation*}

\begin{align*}
    m_1 &= 5757 \text{ kg} \\
    m_2 &= m_1 + \Delta m_{12} \\
    Q &= 35000 \text{ kJ}
\end{align*}

\begin{align*}
    u_2 \left( 70°C, x = 0 \right) &= 202.945 \frac{\text{kJ}}{\text{kg}} \\
    u_1 \left( 20°C, x = 0 \right) &= 418.94 \frac{\text{kJ}}{\text{kg}} \\
    h \left( 20°C, x = 0 \right) &= 83.96 \frac{\text{kJ}}{\text{kg}}
\end{align*}

``````latex


\section*{Aufgabe 1}

\subsection*{e)}

\[
\Delta S_{12} = m_2 S_2 - 4151
\]
\[
= 2886,24 \frac{kJ}{K}
\]

\[
m_2 = m_1 + \Delta m_2 = 10000 \, \text{kg}
\]

\[
S_2 \left( 700 \frac{kJ}{kg}, x=0 \right) = 0,9519
\]

\[
S_1 \left( 1000 \frac{kJ}{kg}, x=0 \right) = 1,3069
\]

``````latex


