
``````latex

\title{Thermo I 2024}
\date{}


\maketitle

\section*{Aufgabe 1}

\subsection*{a) Qaus?}

1. HS:
\[
0 = \dot{m}(h_e - h_a) + \Sigma \dot{Q} - \dot{W}
\]

\[
Q_{\text{aus}} = \dot{m}(h_a - h_e) \quad \dot{Q}_2
\]

\[
\dot{m} = \text{size: 0.3 kg/s}
\]

\[
h_e = h_f(10^\circ C, x=0) = 252,38 \, \text{kJ/kg} \quad \text{[Tab. A-2]}
\]

\[
h_a = h_f(100^\circ C, x=0) = 419,04 \, \text{kJ/kg}
\]

\[
Q_{\text{aus}} = 0.3 \, \text{kg/s} \left( 419,64 - 252,38 \right) \frac{\text{kJ}}{\text{kg}} - 100 \, \frac{\text{kJ}}{\text{s}}
\]

\[
= -62,18 \, \frac{\text{kJ}}{\text{s}} \, (\text{kW})
\]

\subsection*{b)}

\[
\overline{T}_{\text{KF}} = \frac{\int_{s_a}^{s_e} T \, ds}{s_a - s_e}
\]

\[
\int_{s_a}^{s_e} T \, ds = h_a - h_e \quad (\text{1. HS})
\]

\[
= \frac{h_a - h_e}{s_a - s_e} \quad \text{KF = ideale Flüssigkeit}
\]

\[
h_a - h_e = c_{\text{KF}} (T_2 - T_1)
\]

\[
s_a - s_e = c_{\text{KF}} \ln \left( \frac{T_2}{T_1} \right)
\]

\[
\overline{T}_{\text{KF}} = \frac{c_{\text{KF}} (T_2 - T_1)}{c_{\text{KF}} \ln \left( \frac{T_2}{T_1} \right)} = \frac{(289,15 \, \text{K} - 288,15 \, \text{K})}{\ln \left( \frac{289,15}{288,15} \right)}
\]

\[
= 293,12 \, \text{K}
\]

``````latex


\section*{Student Solution}

\begin{itemize}
    \item \(\sum \dot{Q}\)
    \item \(0\) Wärmeübertragung über Kühlwand?
    \item \(\dot{Q}_{\text{aus}}\) \(\dot{Q}_{\text{ein}}\)
    \item Adiabat
\end{itemize}

\[
\begin{array}{c}
\begin{array}{c}
\begin{array}{c}
\begin{array}{c}
\begin{array}{c}
\begin{array}{c}
\begin{array}{c}
\begin{array}{c}
\begin{array}{c}
\begin{array}{c}
\begin{array}{c}
\begin{array}{c}
\begin{array}{c}
\begin{array}{c}
\begin{array}{c}
\begin{array}{c}
\begin{array}{c}
\begin{array}{c}
\begin{array}{c}
\begin{array}{c}
\begin{array}{c}
\begin{array}{c}
\begin{array}{c}
\begin{array}{c}
\begin{array}{c}
\begin{array}{c}
\begin{array}{c}
\begin{array}{c}
\begin{array}{c}
\begin{array}{c}
\begin{array}{c}
\begin{array}{c}
\begin{array}{c}
\begin{array}{c}
\begin{array}{c}
\begin{array}{c}
\begin{array}{c}
\begin{array}{c}
\begin{array}{c}
\begin{array}{c}
\begin{array}{c}
\begin{array}{c}
\begin{array}{c}
\begin{array}{c}
\begin{array}{c}
\begin{array}{c}
\begin{array}{c}
\begin{array}{c}
\begin{array}{c}
\begin{array}{c}
\begin{array}{c}
\begin{array}{c}
\begin{array}{c}
\begin{array}{c}
\begin{array}{c}
\begin{array}{c}
\begin{array}{c}
\begin{array}{c}
\begin{array}{c}
\begin{array}{c}
\begin{array}{c}
\begin{array}{c}
\begin{array}{c}
\begin{array}{c}
\begin{array}{c}
\begin{array}{c}
\begin{array}{c}
\begin{array}{c}
\begin{array}{c}
\begin{array}{c}
\begin{array}{c}
\begin{array}{c}
\begin{array}{c}
\begin{array}{c}
\begin{array}{c}
\begin{array}{c}
\begin{array}{c}
\begin{array}{c}
\begin{array}{c}
\begin{array}{c}
\begin{array}{c}
\begin{array}{c}
\begin{array}{c}
\begin{array}{c}
\begin{array}{c}
\begin{array}{c}
\begin{array}{c}
\begin{array}{c}
\begin{array}{c}
\begin{array}{c}
\begin{array}{c}
\begin{array}{c}
\begin{array}{c}
\begin{array}{c}
\begin{array}{c}
\begin{array}{c}
\begin{array}{c}
\begin{array}{c}
\begin{array}{c}
\begin{array}{c}
\begin{array}{c}
\begin{array}{c}
\begin{array}{c}
\begin{array}{c}
\begin{array}{c}
\begin{array}{c}
\begin{array}{c}
\begin{array}{c}
\begin{array}{c}
\begin{array}{c}
\begin{array}{c}
\begin{array}{c}
\begin{array}{c}
\begin{array}{c}
\begin{array}{c}
\begin{array}{c}
\begin{array}{c}
\begin{array}{c}
\begin{array}{c}
\begin{array}{c}
\begin{array}{c}
\begin{array}{c}
\begin{array}{c}
\begin{array}{c}
\begin{array}{c}
\begin{array}{c```latex


\section*{d Continuous}

\begin{align*}
(m_1 + \Delta m) h_2 - \Delta m h_i &= m_1 h_1 \\
m_1 h_2 + \Delta m h_2 - \Delta m h_i &= m_1 h_1 \\
\Delta m &= \frac{m_1 h_1 - m_1 h_2}{h_2 - h_i} \\
&= \frac{5755 \, \text{kg} \, (429.37 \frac{\text{kJ}}{\text{kg}} - 292.95 \frac{\text{kJ}}{\text{kg}})}{292.95 \frac{\text{kJ}}{\text{kg}} - 83.96 \frac{\text{kJ}}{\text{kg}}} \\
&= 3765.11 \, \text{kg}
\end{align*}

\section*{e\textsubscript{2} includes other $\Delta S$}

\begin{align*}
\Delta S_{s2} &= m_2 S_2 - m_1 S_1 - \Delta m_2 \cdot 3600 \, \text{kg} \\
m_2 &= 9355 \, \text{kg} \\
m_1 &= 5755 \, \text{kg} \\
S_2 &= S(20^\circ C, x=0) = 0.19549 \frac{\text{kJ}}{\text{kg} \cdot \text{K}} \\
S_1 &= S(100^\circ C, x=0.005) = sf + x (sg - sf) \\
&= 1.30649 \frac{\text{kJ}}{\text{kg} \cdot \text{K}} + 0.005 (7.35549 - 1.30649) \\
&= 1.337 \frac{\text{kJ}}{\text{kg} \cdot \text{K}}
\end{align*}

\begin{align*}
\Delta S_{s2} &= 9355 \, \text{kg} \cdot 0.19549 \frac{\text{kJ}}{\text{kg} \cdot \text{K}} - 5755 \, \text{kg} \cdot 1.337 \frac{\text{kJ}}{\text{kg} \cdot \text{K}} \\
&= -293.47 \, \text{kJ/K} \\
&= -1236.65 \, \text{kJ/K}
\end{align*}

``````latex


