
``````latex


1. \underline{1. HS Reaktor}

a) 
\[
0 = \dot{m}_{\text{ein}} (h_{\text{ein}} - h_{\text{aus}}) + \dot{Q}_R + \dot{Q}_{\text{aus}}
\]
\[
\begin{cases}
h_{\text{ein}} = h_f(70^\circ C, x=0) = 252.80 \frac{\text{kJ}}{\text{kg}} & \text{A2} \\
h_{\text{aus}} = h_f(100^\circ C) = 419.04 \frac{\text{kJ}}{\text{kg}} & \text{A2}
\end{cases}
\]
\[
\dot{Q}_{\text{aus}} = \dot{m}_{\text{ein}} (h_{\text{aus}} - h_{\text{ein}}) - \dot{Q}_R
\]
\[
= -62.182 \text{ kW}
\]
\textcolor{orange}{\text{f negativ, von Reaktor abgeführt!}}

\textcolor{orange}{\text{1. HS/0 = (h2-h1) + qrev}}

b)
\[
T_{\text{uK}} = \frac{\int_{s_a}^{s_e} T \, ds}{s_a - s_e} = \frac{q_{\text{rev}}}{s_a - s_e} = \frac{c_p (T_{\text{uK aus}} - T_{\text{uK ein}})}{c_p \ln \left( \frac{T_{\text{uK aus}}}{T_{\text{uK ein}}} \right)}
\]
\[
= 233.12 \text{ K}
\]

c) \underline{2. HS Reaktor}
\[
0 = \dot{m}_{\text{ein}} (s_e - s_a) + \frac{\dot{Q}_{\text{aus}}}{T_{\text{uK}}} = \frac{\dot{Q}_R}{T_{\text{Reaktor}}} + \dot{S}_{\text{ez}}
\]
\[
\text{2. HS \text{unterstrichen} }
\]
\[
0 = \dot{m}_{\text{ein}} (
\]

``````latex


1. a)

\begin{tabular}{cccc}
 & 1 & 2 & $\Delta 12$ \\
T & 100°C & 70°C & 20°C \\
m & 5755 \, \text{kg} & & \Delta m_{12} \\
x & 0.005 & 0 & \\
\end{tabular}

\[
Q = 0 \quad W = 0
\]

1. HS:

\[
-m_2 u_2 - m_{12} u_{12} = \Delta m_{12} h_{ein}
\]

\[
u_1 = u_f + x \left( u_s - u_f \right) = 418.84 + 0.005 \left( 2506.5 - 418.84 \right) \frac{\text{kJ}}{\text{kg}}
\]

\[
= 428.38 \frac{\text{kJ}}{\text{kg}}
\]

\[
u_2 = u_f (70°C) = 252.35 \frac{\text{kJ}}{\text{kg}} \quad \text{A2}
\]

\[
h_{ein} = h_f (20°C) = 83.36 \frac{\text{kJ}}{\text{kg}} \quad \text{A2}
\]

\[
M_2 = m_1 + \Delta m_{12}
\]

\[
\Delta m_{12} h_{ein} - (m_1 + \Delta m_{12}) u_2 = m_1 u_1
\]

\[
\Rightarrow -\Delta m_{12} (h_{ein} - u_2) = m_1 u_2 - m_1 u_1
\]

\[
\Rightarrow \Delta m_{12} = \frac{m_1 u_2 - m_1 u_1}{(h_{ein} - u_2)} = \frac{1178 \, \text{kg}}{}
\]

e)

\[
\Delta S_{12} = m_2 S_2 - m_1 S_1 = \Delta m_{12} s_{ein} + S_{s2}
\]

``````latex


