
``````latex


\section*{1}
\textit{Es werden drei Werte aus den Aufgaben genommen. Z.B. \(Q_{\text{zu}} = 65 \, \text{kJ}\) (WÃœB)}

\begin{itemize}
    \item[a)] 
    \[
    0 = \dot{m} \left( h_{\text{ein}}^{w} - h_{\text{aus}}^{w} \right) + \dot{Q}_{\text{zu}}
    \]
    \[
    h_{\text{ein}}^{w} = h_{2} (70^\circ \text{C}) = 292.92 \, \frac{\text{kJ}}{\text{kg}} \quad \text{(A2)}
    \]
    \[
    h_{\text{aus}}^{w} = h_{f} (40^\circ \text{C}) = 419.04 \, \frac{\text{kJ}}{\text{kg}} \quad \text{(A2)}
    \]
    \[
    \dot{Q}_{\text{zu}} = \boxed{62.482 \, \text{kW}}
    \]

    \item[b)] 
    \[
    s_{f}^{\text{KF}} = \int_{s_{0}}^{s_{e}} \frac{T \, ds}{s}
    \]
    \[
    s_{f}^{\text{KF}} = \frac{h_{f}^{\text{KF}} - h_{\text{ein}}^{\text{KF}}}{T_{\text{ein}}^{\text{KF}}} = \frac{h_{f}^{\text{KF}} - h_{\text{ein}}^{\text{KF}}}{T_{\text{ein}}^{\text{KF}}} \ln \left( \frac{T_{\text{aus}}^{\text{KF}}}{T_{\text{ein}}^{\text{KF}}} \right)
    \]
    \[
    = \boxed{293.122 \, \text{K}}
    \]

    \item[c)] 
    \[
    0 = \dot{m} \left( h_{\text{ein}}^{w} - h_{\text{aus}}^{w} \right) - \frac{\dot{Q}_{\text{zu}}}{T_{\text{KF}}}
    \]
    \[
    \dot{S}_{\text{zu}} = \frac{\dot{Q}_{\text{zu}}}{T_{\text{KF}}} \rightarrow \dot{S}_{\text{zu}} = \boxed{0.326 \, \frac{\text{kW}}{\text{K}}}
    \]

    \item[d)] 
    \[
    \Delta U = \dot{m} \left( h_{\text{ein}}^{w} - h_{\text{aus}}^{w} \right) + \dot{Q}_{\text{zu}} - \dot{Q}_{\text{aus}} = 0
    \]
    \[
    h_{\text{ein}}^{w} = h_{2} (20^\circ \text{C}) = 83.96 \, \frac{\text{kJ}}{\text{kg}} \quad \text{(A2)}
    \]
    \[
    \Delta U = \dot{m}_{\text{ges}} \left( u_{1} \left( \text{ges} + \Delta m_{12} \right) u_{2} \right)
    \]
    \[
    u_{f} = u_{f} (40^\circ \text{C}) + (u_{c} - u_{f}) = 429.3778 \, \frac{\text{kJ}}{\text{kg}}
    \]
    \[
    u_{2} = u_{f} (70^\circ \text{C}) = \boxed{292.5 \, \frac{\text{kJ}}{\text{kg}}}
    \]
\end{itemize}

``````latex


\section*{Solution}

\subsection*{c)}

\begin{equation*}
\Delta S_{12} = \left( m_{ges} + \Delta m_{12} \right) S_2 - m_{ges} S_1 = 1237.8488 \frac{kJ}{K}
\end{equation*}

\begin{equation*}
S_2 = f \left( T \right) = 0.95249 \frac{kJ}{kgK}
\end{equation*}

\begin{equation*}
S_1 = S_f + x \left( S_g - S_f \right) = 1.23744 \frac{kJ}{kgK}
\end{equation*}

\subsection*{d)}

\begin{equation*}
m_{ges} \left( u_1 - u_2 \right) - \Delta m_{12} u_2 = \Delta m_{12} h_{e,n}^{''}
\end{equation*}

\begin{equation*}
\Delta m_{12} = \frac{m_{ges} \left( u_1 - u_2 \right)}{h_{e,n}^{''} + u_2} = 6.408 \, T
\end{equation*}

``````latex


