
``````latex


\section*{Problem 3}

\subsection*{a)}

\[
A = \pi \frac{D^2}{4} = 0.007854 \, \text{m}^3
\]

\[
p_{e2} = \frac{m_{e1} v_{e1}}{A} + \frac{m_{e2} g}{A} + p_{0m} = 1.4 \, \text{bar}
\]

\[
p_{e1} V_{e1} = G_1 \frac{R}{T_{e1}} \quad \text{and} \quad p_{e2} V_{e2} = G_2 \frac{R}{T_{e2}}
\]

\[
\frac{V_{e1}}{m_{e1}} = \frac{V_{e2}}{m_{e2}}
\]

\[
m_{e2} = \frac{p_{e1} V_{e1}}{\frac{R}{T_{e1}}} = 0.109 \, \text{kg}
\]

\subsection*{b)}

\[
V_{e2} = \frac{V_{e1}}{m_{e1}} m_{e2}
\]

\[
p_{e2} = p_{e1} = 1.4 \, \text{bar}, \quad \text{da sich} \, m_{e1}, m_{e2} \, \text{und} \, p_0 \, \text{nicht ver√§ndert}
\]

\[
m_{e1} \left( \frac{v_{e2}^2 - v_{e1}^2}{2} \right) = \dot{Q}
\]

\[
\rho = \frac{R}{A_{e2} T_{e2}}
\]

\[
\frac{V_{e2}}{m_{e2}} = \frac{p_{e2} V_{e2}}{m_{e2} \frac{R}{T_{e2}}}
\]

\subsection*{c)}

\[
m_{e1} (u_{e1} - u_{e2}) = \dot{Q} = -1.139 \, \text{kJ}
\]

\[
c_v (T_1 - T_2)
\]

\subsection*{d)}

\[
m_{e1} \left( \frac{v_{e2}^2}{2} - \frac{v_{e1}^2}{2} \right) = \dot{Q}
\]

\[
\frac{u_{e2}}{m_{e2}} = \frac{\dot{Q}}{m_{e1}} + u_{e1} = u_{e1} + x_2 (u_{e2} - u_{e1})
\]

\[
u_{e1} = u_{e1} + x_2 (u_{e2} - u_{e1})
\]

\[
u_{e1} = 200 \, \text{kJ/kg}
\]

\[
-333.485 \, \text{kJ/kg}
\]

\[
-0.045 \, \text{kJ/kg}
\]

\[
p_{e2} = p_0 + \frac{m_{e1} k_{e1}}{A} + \frac{m_{e2} g}{A}
\]

\[
p_{e2} = 2.9 \, \text{bar}
\]

\[
\frac{u_{e2}}{m_{e2}} = \frac{u_{e1}}{m_{e1}} + x_2 (u_{e2} - u_{e1})
\]

\[
\dot{Q} = \frac{m_{e2} (u_{e2} - u_{e1})}{m_{e1}} + \frac{u_{e1}}{m_{e1}} - \frac{u_{e2}}{m_{e2}}
\]

\[
\dot{Q} = -0.106 \, \text{kJ/kg}
\]

``````latex

\[
U_{\text{Fe2}} = \frac{-333.812 + 333.488}{4.9 - 2} = \frac{(2.9 - 2) \cdot 333.488}{4.9 - 2} = 333.533 \frac{\text{KJ}}{\text{Kg}}
\]

``````latex


