
``````latex


\section*{Aufgabe 1}

\subsection*{a)}

\begin{equation*}
\frac{d\dot{E}_t^0}{dt} = \sum \dot{m}_i \left[ h_i + \frac{v_i^2}{2} + g z_i \right]^0 + \dot{Q} - \dot{W}
\end{equation*}

\begin{equation*}
Q = \dot{m} (h_e - h_a) + \dot{Q}_{aus} + 100 \, \text{kW}
\end{equation*}

\begin{equation*}
\dot{Q}_{aus} = \dot{m} (h_a - h_e) - 100 \, \text{kW}
\end{equation*}

\begin{equation*}
h_a: \text{TAB AZ @ } T = 100^\circ C \quad \Rightarrow \quad 419.04 \, \frac{\text{kJ}}{\text{kg}}
\end{equation*}

\begin{equation*}
h_e: \text{TAB AZ @ } T = 70^\circ C \quad \Rightarrow \quad 292.98 \, \frac{\text{kJ}}{\text{kg}}
\end{equation*}

\begin{equation*}
\Rightarrow \dot{Q}_{aus} = 0.3 \, \frac{\text{kg}}{\text{s}} \cdot (419.04 \, \frac{\text{kJ}}{\text{kg}} - 292.98 \, \frac{\text{kJ}}{\text{kg}}) - 100 \, \text{kW}
\end{equation*}

\begin{equation*}
= 37.818 \, \frac{\text{kJ}}{\text{s}} - 100 \, \text{kW} = 37.818 \, \text{kW} - 100 \, \text{kW}
\end{equation*}

\begin{equation*}
\dot{Q}_{aus} = -62.182 \, \text{kW} \quad \text{(gegeben raus - negativ macht Sinn)}
\end{equation*}

\subsection*{b)}

\begin{equation*}
\bar{T}_{LT} = \frac{\int_{s_a}^{s_e} T ds}{s_a - s_e} = T
\end{equation*}

\subsection*{c)}

\begin{equation*}
\frac{d\dot{S}_e}{dt} = \frac{Q}{T} + \dot{S}_{erzeugt} \quad \Rightarrow \quad \dot{S}_{erzeugt} = \frac{Q}{T} = \frac{62.182 \, \text{kW}}{295 \, \text{K}}
\end{equation*}

\begin{equation*}
\dot{S}_{erzeugt} = -210.786 \, \frac{\text{J}}{\text{s} \cdot \text{K}}
\end{equation*}

``````latex


a)
\[
\frac{dE}{dt} = \sum m_i \left( h_i + \frac{v_i^2}{2} + gz_i \right) + \dot{Q} - \dot{W}
\]
\[
\Rightarrow 0 = \dot{E} - m_2 u_2 - m_1 u_1 = \Delta m + \dot{Q} - \dot{W} \quad \text{(he-hw)}
\]

e)
\[
0 = m_2 s_2 - m_1 s_1
\]

``````latex


