
``````latex


\section*{Aufgabe 1}

\subsection*{a)}
station√§r ohne ke$\delta$pe
\begin{align*}
0 &= \dot{m} (h_{\text{ein}} - h_{\text{aus}}) + \dot{Q}_R + \dot{Q}_{\text{aus}} \\
\dot{Q}_{\text{aus}} &= \dot{m} (h_{\text{aus}} - h_{\text{ein}}) - \dot{Q}_R \\
\dot{Q}_{\text{aus}} &= 2.69 \, \text{kW} - 123.04 \, \text{kW}
\end{align*}

\subsection*{b)}
\begin{align*}
\dot{S}_{\text{erz}} + \dot{m} (s_e - s_a) + \sum \frac{\dot{Q}}{T} \\
\dot{S}_{\text{erz}} = 0
\end{align*}

\begin{align*}
\dot{Q}_{\text{aus}} &= \dot{m} (s_e - s_a) \\
\frac{\dot{Q}_{\text{aus}}}{\dot{Q}_{\text{aus}}} &= -\frac{1}{T} \\
T &= \frac{c (T_2 - T_1) = (\dot{Q}_{\text{aus}})}{c (\ln (\frac{T_2}{T_1}))} = 7.12 \, \text{K}
\end{align*}

\subsection*{c)}
\begin{align*}
\dot{S}_{\text{erz}} = \dot{m} \left( \frac{h_{\text{aus}} - h_{\text{ein}}}{s} \right) + \frac{\dot{Q}}{T}
\end{align*}

\begin{align*}
s_{\text{aus}} &= \frac{(7.393 - 1.306) \, \frac{\text{kJ}}{\text{kgK}} \cdot 2257.0 + 1.306 \, \frac{\text{kJ}}{\text{kgK}}}{2576.1 - 499.04} \, \frac{\text{kJ}}{\text{kgK}} = 7.3547 \, \frac{\text{kJ}}{\text{kgK}}
\end{align*}

\begin{align*}
s_{\text{ein}} &= \frac{0.856 (7.393 - 0.856) \, \frac{\text{kJ}}{\text{kgK}}}{26.26 - 252.38} \, \frac{\text{kJ}}{\text{kgK}} = 2333.8 + 0.856 \, \frac{\text{kJ}}{\text{kgK}} = 7.7852 \, \frac{\text{kJ}}{\text{kgK}}
\end{align*}

\begin{align*}
\dot{S}_{\text{erz}} = 0.70268 \, \frac{\text{kJ}}{\text{kg}}
\end{align*}

26.6 \, \frac{\text{kJ}}{\text{kg}}

``````latex

\section*{Problem 1}

\[
\Delta U = \dot{Q}_{in12} + \dot{m}_{12} U
\]

\[
\dot{m}_{12} = \frac{\dot{Q}_{in12}}{U_{12}} = \frac{\dot{m}(U_2 - U_1)}{U_{12}}
\]

\[
U_1 = U_f - \omega \times (U_g - U_f) \quad 100^8 = 40R.15 \frac{kJ}{kg}
\]

\[
A-2 = 
\]

\[
U_{12} = \frac{(2333.33 \frac{kJ}{kg})}{\text{(crossed out part)}}
\]

\[
U_{12} = U_f + x(U_g - U_f) = 2333.33 \frac{kJ}{kg}
\]

\[
A-2 = \frac{\text{(crossed out part)}}{-h_f + h_g}
\]

\[
x_{12} = 0.03
\]

\[
\Delta S_{12} = \dot{m}(
\]

``````latex


