
``````latex


\section*{Problem a)}

\begin{center}
\textbf{Graphical Description:}
\end{center}

The graph is a Temperature-Entropy ($T$-$s$) diagram. The vertical axis is labeled $T [\text{K}]$ and the horizontal axis is labeled $s [\frac{kJ}{kgK}]$. There are three isobars drawn in red, labeled $P_2 = P_3$, $P_1 = P_4 = P_5$, and $P_6 = P_0$. 

There are six points labeled 1 through 6. The points are connected by various lines:
- Point 1 to Point 2 is a vertical line.
- Point 2 to Point 3 is a curved line.
- Point 3 to Point 4 is a vertical line.
- Point 4 to Point 5 is a curved line.
- Point 5 to Point 6 is a vertical line.
- Point 6 to Point 1 is a curved line.

The lines connecting Points 1 to 2, 3 to 4, and 5 to 6 are in black, while the lines connecting Points 2 to 3, 4 to 5, and 6 to 1 are in blue. The points are marked with small circles, and the lines are annotated with $m_H$ and $m_K$.

\section*{Problem b)}

\begin{align*}
&\begin{array}{c|c|c|c|c|c|c}
0 & 1 & 2 & 3 & 4 & 5 & 6 \\
\hline
0.5 & 0.151 & & & & & 0.151 \\
431.3K & & & & & & 213.15 \\
220 & & & & & & \\
\end{array}
\end{align*}

\begin{align*}
R &= c_p - c_v = 2.87943 \frac{kJ}{kgK} = 2.87943 \frac{J}{kgK} \\
c_{vL} &= \frac{c_{pL}}{k} = 0.78057 \frac{kJ}{kgK} \\
5 \rightarrow 6 &\text{ Adiabatic reversible: Isentropic: } s_5 = s_6 \\
s(T_5) &= 2.66533 \frac{kJ}{kgK} \\
T_6 &= T_5 \left(\frac{P_6}{P_5}\right)^{\frac{R}{c_{vL}}} = 2.66533 \frac{kJ}{kgK} \\
T_6 &= 328.097 K \\
\Delta s_{42} &= c_p \ln \left(\frac{T_4}{T_2}\right) = c_p \ln \left(\frac{T_4}{T_2}\right) \\
1. \text{HS (5-6)} &\text{ : } 0 = m_H (h_6 - h_5) + \left(\frac{w_{6-5}}{2}\right) \\
&= m_H (T_6 - T_5) + w_{6-5} = 236.755 \frac{m}{s} \\
&= \sqrt{2k(h_6 + h_5)} = w_{6-5}^2
\end{align*}

``````latex


c) 
\begin{align*}
\Delta e_{cx,str} &= \left( h_e - h_{c4} - T_0(s_{e2} - s_{c4}) + \Delta ke \right) \\
&= \left( h_e - h_{c4} - T_0(s_{e2} - s_{c4}) + \Delta ke \right) \\
&= \left( cp \left( \frac{T_e}{T_0} - 1 \right) - T_0 \left( cp \ln \left( \frac{T_e}{T_0} \right) - R \ln \left( \frac{p_e}{p_0} \right) + \frac{v_e^2}{2} - \frac{w_{c4}^2}{2} \right) \right) \\
&= 125'471.75 \frac{J}{kg} = 125.47 \frac{kJ}{kg}
\end{align*}

d) 
\begin{align*}
0 &= \Delta e_{ex,str} + \sum \left( 1 - \frac{T_c}{T_0} \right) \dot{m} \left( \frac{e_{ex,in}}{\dot{m}} - \frac{e_{ex,out}}{\dot{m}} \right) - \dot{W}_{t,in} - \dot{e}_{x,vol} \\
-e_{ex,vol} &= \Delta e_{ex,str} - \dot{W}_{t,in} \\
e_{x,vol} &= T_0 \dot{S}_{ex} = T_0 \left( s_{e2} - s_{a} \right) = T_0 \left( s_{a} - s_{e} \right) = T_0 \left( s_{e2} - s_{a} \right) \\
&= T_0 \left( cp \ln \left( \frac{T_e}{T_0} \right) - R \ln \left( \frac{p_0}{p_c} \right) \right) = 15'471.75 \frac{J}{kg} = 15.622 \frac{kJ}{kg}
\end{align*}

``````latex


