
``````latex

\section*{Aufgabe 1}

\subsection*{a) 1. HS um Reaktor ohne Kühlmantel}

\begin{align*}
\dot{m} (h_{\text{ein}} - h_{\text{aus}}) + \dot{Q}_R - \dot{Q}_{\text{aus}} &= 0 \\
\dot{Q}_{\text{aus}} &= \dot{m} (h_{\text{ein}} - h_{\text{aus}}) + \dot{Q}_R
\end{align*}

\begin{align*}
h_{\text{ein}} &= h(70^\circ C, x = \infty) = 292{,}98 \frac{\text{kJ}}{\text{kg}} \quad \text{(Tab A-2)} \\
h_{\text{aus}} &= h(100^\circ C, x = 0) = 419{,}04 \frac{\text{kJ}}{\text{kg}} \quad \text{(Tab A-2)}
\end{align*}

\[
\Rightarrow \dot{Q}_{\text{aus}} = 62{,}182 \, \text{RW}
\]

\subsection*{b)}

\[
\overline{T} = \frac{\dot{Q}_{\text{aus}}}{S_{KF,\text{aus}} - S_{KF,\text{ein}}}
\]

\[
= \frac{\dot{Q}_{\text{aus}}}{\dot{m}_{KF} c_{KF} \ln \left( \frac{T_{KF,\text{aus}}}{T_{KF,\text{ein}}} \right)}
\]

\subsection*{1. HS am Kühlmantel}

\[
\dot{Q}_{\text{aus}} = \dot{m}_{KF} c_{KF} (T_{KF,\text{aus}} - T_{KF,\text{ein}})
\]

\[
\Rightarrow \frac{\dot{Q}_{\text{aus}}}{\dot{m}_{KF} c_{KF}} = T_{\text{ein}} - T_{\text{aus}} = 61{,}5 \frac{\text{RJ}}{\text{kg K}}
\]

\[
\dot{Q}_{\text{aus}} = \dot{m}_{KF} (h_{KF,\text{ein}} - h_{KF,\text{aus}}) = \dot{m}_{KF} c_{KF} (T_{\text{ein}} - T_{\text{aus}})
\]

\[
\Rightarrow \dot{Q}_{\text{aus}} = \dot{m}_{KF} c_{KF} (T_{\text{ein}} - T_{\text{aus}})
\]

``````latex


\[
\Rightarrow \overline{T} = \frac{(T_{\text{ein}} - T_{\text{aus}})}{\ln \left( \frac{T_{\text{aus}}}{T_{\text{ein}}} \right)}
\]

\[
\approx 293.12 \, \text{K}
\]

\[
\boxed{\text{A1, Seite 2}}
\]

\[
\text{c)} \quad \dot{S}_{\text{erz}} = \frac{\dot{Q}_{\text{aus}}}{T_{\text{rechter}}} - \frac{\dot{Q}_{\text{aus}}}{\overline{T}}
\]

aus Entropiebilanz am Reaktorwand

\[
\text{d)} \quad m_2 u_2 - m_1 u_1 = \Delta m h(x=0, 20^\circ \text{C}) - Q_{\text{aus}, 12}
\]

\[
\Rightarrow m_1 (u_2 - u_1) + \Delta m u(x=0, 20^\circ \text{C}) = \Delta m h(x=0, 20^\circ \text{C}) - Q_{\text{aus}, 12}
\]

\[
\Rightarrow \Delta m = \frac{m_1 \left( u_2 (x=0, 70^\circ \text{C}) - u_1 (x=0, 100^\circ \text{C}) \right) + Q_{\text{aus}, 12}}{h(x=0, 20^\circ \text{C}) - u(x=0, 20^\circ \text{C})}
\]

\[
\text{e)} \quad \Delta S_{12} = m_2 s_2 - m_1 s_1
\]

``````latex


