
``````latex


\section*{Aufgabe 2}

\subsection*{a)}

\[
\begin{array}{c}
\begin{array}{c|c}
\text{Graph:} & \text{Description:} \\
\hline
\begin{array}{c}
\text{A graph with the x-axis labeled as } S \left[\frac{J}{K}\right] \text{ and the y-axis labeled as } T[K]. \\
\text{There are three curves labeled as } p = p_1, p = 0.5 \text{ bar, and } p_0 = 0.99 \text{ bar.} \\
\text{There are six points labeled 1 to 6 connected by lines.} \\
\text{Point 1 is on the curve } p = p_1, \text{ point 2 is on the curve } p = 0.5 \text{ bar,} \\
\text{point 3 is on the curve } p = p_1, \text{ point 4 is on the curve } p = 0.5 \text{ bar,} \\
\text{point 5 is on the curve } p = 0.99 \text{ bar, and point 6 is on the curve } p = 0.5 \text{ bar.} \\
\text{The points are connected in the following order: 1 to 2, 2 to 3, 3 to 4, 4 to 5, 5 to 6.} \\
\text{There is a horizontal line from point 1 to point 6.} \\
\text{There is a vertical line from point 1 to point 2, from point 3 to point 4, and from point 5 to point 6.} \\
\text{There is a diagonal line from point 2 to point 3 and from point 4 to point 5.} \\
\text{There is a label } T_0 = 273.15 - 30 = 243.15 \text{ K.}
\end{array}
\end{array}
\end{array}
\]

\subsection*{b)}

\[
T_6 = T_S \left( \frac{p_6}{p_S} \right)^{\frac{k-1}{k}} = 431.9 \text{ K} \left( \frac{0.191}{0.7} \right)^{\frac{0.4}{1.4}} = 327.29 \text{ K}
\]

\subsection*{c)}

\[
\text{Energiebilanz:}
\]

\[
\begin{array}{c}
\begin{array}{c|c}
\text{Diagram:} & \text{Description:} \\
\hline
\begin{array}{c}
\text{A diagram of a control volume with an inlet labeled 5 and an outlet labeled 6.} \\
\text{There is an arrow pointing into the control volume at 5 and an arrow pointing out of the control volume at 6.}
\end{array}
\end{array}
\end{array}
\]

\[
0 = \dot{m} \left( h_5 - h_6 + \frac{1}{2} (w_5^2 - w_6^2) \right)
\]

\[
w_6 = \sqrt{w_5^2 - 2 (h_6 - h_5)} = \sqrt{w_5^2 - 2 c_p (T_6 - T_5)}
\]

\[
w_6 = 508.6 \frac{m}{s}
\]

\subsection*{d)}

\[
\Delta e_{x,str} = e_{x,str,c} - e_{x,str,0} = h_6 - h_0 - T_0 (s_6 - s_0) + \frac{1}{2} (w_6^2 - w_0^2)
\]

\[
= c_p (T_6 - T_0) - T_0 (c_p \ln \left( \frac{T_6}{T_0} \right) - R \ln \left( \frac{p_6}{p_0} \right)) + \frac{1}{2} (w_6```latex


