
``````latex


\section*{Aufgabe 1}

a)

\[
0 = \dot{m} [h_e - h_a] + 2 \dot{Q}_j - \dot{W}_{b,in}^0
\]

\[
2 \dot{Q}_j = 6 \dot{Q}_{a,us}
\]

\[
\dot{Q}_R = \dot{Q}_{a,us}
\]

\[
\dot{Q}_{a,us} = \dot{m} [h_e - h_a]
\]

\[
h_e = 419.04 + 0.005 (2676.1 - 419.04) = 430.33 \frac{kJ}{kg}
\]

\[
h_a = 292.98 + 0.005 (2626.8 - 292.98) = 304.65 \frac{kJ}{kg}
\]

\[
\dot{Q}_{a,us} = 0.3 \left[ 304.65 - 430.33 \right] + 100 \frac{kJ}{kg} = +62.30 kW
\]

``````latex


\section*{Aufgabe 1}

\subsection*{b)}

\[
\bar{T} = \frac{\int_{S_a}^{S_e} T \, ds}{S_a - S_e} = \frac{\int_{S_a}^{S_e} T \, ds}{\int_{t_{ac}}^{t_{en}} \frac{c}{\dot{T}} \, dt}
\]

``````latex


\section*{Aufgabe 1}

\subsection*{c)}

\begin{align*}
\dot{Q}_{\text{acc}} &= 65 \, \text{kW} \quad \bar{T}_{\text{KF}} = 293 \, \text{K} \\
0 &= \dot{m} [S_e - S_a] + \frac{\dot{Q}}{\bar{T}} + \dot{S}_{\text{erz}} \\
&\quad \text{- Bilanz im Reaktor} \\
\dot{S}_{\text{erz}} &= \dot{m} [S_a - S_e] - \frac{\dot{Q}_{\text{acc}}}{\bar{T}_{\text{Reaktor}}} \\
\bar{T}_{\text{Reaktor}} &= 100^\circ \text{C} = 373.15 \, \text{K} \\
S_a &= 1.3 \cancel{69} + 0.005 (7.35 \cancel{69} - 1.3069) = 1.34 \, \frac{\text{kJ}}{\text{kg} \cdot \text{K}} \\
S_e &= 0.95 \cancel{69} + 0.005 (7.75 \cancel{53} - 0.95 \cancel{69}) = 0.9 \, \frac{\text{kJ}}{\text{kg} \cdot \text{K}} \\
\dot{S}_{\text{erz}} &= 0.3 [1.34 - 0.9] - \frac{65 \, \text{kW}}{373.15 \, \text{K}} = 0. \cancel{2} 29 \, \frac{\text{kW}}{\text{kg} \cdot \text{K}}
\end{align*}

``````latex


\section*{Aufgabe 1}

\subsection*{d)}

\[
\Delta F = \sum m_i [h_i] + \frac{1}{2} Q_i = m_2 d_2 - m_1 d_1 = (m_1 + \Delta m_{12}) d_2 - m_1 d_1
\]

\[
m_2 d_2 + \Delta m_{12} d_2 - m_1 d_1 = \Delta m_{12} [h_{12}] + Q_{R_{12}}
\]

\[
\Delta m_{12} = m_2 d_2 - m_1 d_1 - Q_{E_{12}} \frac{1}{h_{12}}
\]

\[
u_1 = 418.94 + 0.005 (2566.5 \frac{kJ}{kg} - 418.94) = 429.38 \frac{kJ}{kg}
\]

\[
a_2 = u(T_{20°C}) = 292.95 \frac{kJ}{kg}
\]

\[
h_{12} = h_p (20°C) = 83.96 \frac{kJ}{kg}
\]

\[
\Delta m_{12} = m_1 \frac{5735 kg \cdot 292.95 \frac{kJ}{kg} - 5735 kg \cdot 429.38 \frac{kJ}{kg} - 35 \cdot 10^6 kJ}{83.96 \frac{kJ}{kg} - 292.95 \frac{kJ}{kg}}
\]

\[
= 33.46 kg
\]

\subsection*{e)}

\[
\Delta S = m_2 s_2 - m_1 s_1
\]

\[
\Delta m_{12} = 3600 kg
\]

\[
s_1 = 1.3069 + 0.005 (4.3549 - 1.3069) = 1.34 \frac{kJ}{kg \cdot K}
\]

\[
s_2 = s(T_{20°C}) - 1.0955 \frac{kJ}{kg \cdot K}
\]

\[
\Delta S = (5735 kg + 3600 kg) 1.02 \frac{kJ}{kg \cdot K} - 5735 kg \cdot 1.34 \frac{kJ}{kg \cdot K} = 4830.4 \frac{kJ}{kg \cdot K}
\]

``````latex


