
``````latex


\section*{Aufgabe 1}

\subsection*{(a)}

\[
\dot{Q}_{\text{aus}} = ?
\]

\textbf{Kühlflüssigkeit}

\textbf{Energiebilanz:}

\textit{stationär:}

\[
\frac{dE}{dt} = \sum \dot{m} \left[ h_i + \frac{v^2}{2} + gz \right] + \sum \dot{Q} - \sum \dot{W}
\]

\[
0 = \dot{m} \left[ h_{\text{ein}} - h_{\text{aus}} \right] + \dot{Q}_R - \dot{Q}_{\text{aus}}
\]

\[
\dot{Q}_{\text{aus}} = \dot{m} \left[ h_{\text{ein}} - h_{\text{aus}} \right] + \dot{Q}_R =
\]

\textbf{TAB A-2:}

\textit{reines Wasser, siedende Flüssigkeit} $\rightarrow h_f$

\[
h_f (70^\circ C) = 292,98 \frac{\text{kJ}}{\text{kg}}
\]

\[
h_f (100^\circ C) = 419,04 \frac{\text{kJ}}{\text{kg}}
\]

\[
\dot{Q}_R = 100 \text{kW}
\]

\[
\dot{Q}_{\text{aus}} = 0.3 \frac{\text{kg}}{\text{s}} \left[ h_f (70) - h_f (100) \right] + \dot{Q}_R
\]

\[
\dot{Q}_{\text{aus}} = 62,182 \text{kW} \quad \boxed{}
\]

``````latex


(b)
\[
\overline{T}_{KF} = \frac{\int_{S_a}^{S_e} T dS}{S_a - S_e}
\]
\[
dH = T dS + V dp \quad \text{isobar}
\]
\[
dH = h_a - h_e
\]
\[
\overline{T}_{KF} = \frac{h_a - h_e}{S_a - S_e}
\]
\[
\overline{T}_{KF} = \frac{h_{aus} - h_{ein}}{S_{aus} - S_{ein}}
\]
\text{Ideale Flüssigkeit:}
\[
S_{if} = S_p(T)
\]
\[
S_{aus} - S_{ein} = S_p(T_{aus}) - S_p(T_{ein})
\]
\[
h_{aus} - h_{ein} = \int_{T_{ein}}^{T_{aus}} c_{if}(T) dT + v \cdot if(p_{aus} - p_{ein})
\]
\[
= c_{if}(T) \cdot (T_{aus} - T_{ein})
\]
\[
h_0 \quad S_{aus} - S_{ein} = \int_{T_{ein}}^{T_{aus}} \frac{c_{if}(T)}{T} dT = c_{if}(T) \left[ \ln \left( \frac{T_{aus}}{T_{ein}} \right) \right]
\]
\[
\Rightarrow \overline{T}_{KF} = \frac{c_{if} \cdot T_{aus} - T_{ein}}{c_{if} \ln \left( \frac{T_{aus}}{T_{ein}} \right)} = 293,12 K
\]
\[
T_{aus} = 298,15 K
\]
\[
T_{ein} = 288,15 K
\]

``````latex


\section*{Aufgabe 1}
(C)

\[
\frac{dS}{dt} = \dot{E} \frac{Q}{T} + \dot{S}_{er}
\]

\[
\dot{S}_{aus} - \dot{S}_{ein} = \frac{\dot{Q}_{aus}}{T} + \dot{S}_{er}
\]

\[
\dot{S}_{er} = \dot{S}_{aus} - \dot{S}_{ein} + \frac{\dot{Q}_{aus}}{T}
\]

\[
\frac{dS}{dt} = \dot{E} \frac{Q}{T} + \dot{S}_{er}
\]

\[
\dot{S}_{aus} - \dot{S}_{ein} = \frac{\dot{Q}_{aus}}{T} + \dot{S}_{er}
\]

stationär $\rightarrow \dot{S}_{er} = \dot{S}_{aus} - \dot{S}_{ein}$

\[
0 = \dot{m} \left( s_{ein} - s_{aus} \right) + \dot{E} \frac{Q}{T} + \dot{S}_{er}
\]

\[
\dot{S}_{er} = \dot{m} \left( s_{aus} - s_{ein} \right) - \left( \frac{\dot{Q}_{aus}}{T_R} + \frac{Q_{aus}}{T_{KF}} \right)
\]

\[
\dot{m} = 0.3
\]

TAB A-2

\[
s(70) = s_f(70) = 0.3579 \frac{kJ}{kgK}
\]

\[
s(100) = s_f(100) = 1.3669 \frac{kJ}{kgK}
\]

\[
\dot{S}_{er} = 0.1056 \frac{kJ}{K \cdot s} - \left( \frac{100}{(100+273.15)} \right) + \frac{Q_{aus}}{T_{KF}}
\]

\[
\dot{S}_{er} = 49.75 \frac{W}{K}
\]

``````latex


\section*{(d)}

\begin{align*}
T_R &= 70^\circ \\
\Delta m_{12} \\
T_{ein,12} &= 20^\circ C \\
Q_{R,12} &= 35 \, \text{MJ} \\
m_2 &= 
\end{align*}

\subsection*{Energieblanz:}

\subsubsection*{Halboffenes System:}
\begin{align*}
ke + pe &= 0 \\
\Delta E &= m_2 U_2 - m_2 U_1 = m_i h_i + \mathbb{E} Q - \mathbb{E} W^0 \\
m_2 U_2 - m_1 U_1 &= \Delta m_{12} h_i (20^\circ C) + Q_{aus} \\
m_2 &= 5255 \, \text{kg} \\
(m_2 - m_1) h_i (20^\circ C) + Q_{aus}
\end{align*}

\subsection*{TABA-Z:}
\begin{align*}
h_i (20^\circ C) &= h_{pf} (20^\circ C) = 83.96 \, \frac{\text{kJ}}{\text{kg}}
\end{align*}

\subsection*{TABA-Z:}
\begin{align*}
u_2 &= u_f + x (u_g - u_f) \\
u_f (100^\circ C) &= 418.92 \\
u_g (100^\circ C) &= 2506.5 \\
u_2 &= 429.3778 \, \frac{\text{kJ}}{\text{kg}} \\
U_2 &= U_f (70^\circ C) = 292.95 \, \frac{\text{kJ}}{\text{kg}}
\end{align*}

\begin{align*}
m_2 U_2 - m_1 U_1 &= m_2 h_i (20^\circ) - m_1 h_i + Q_{aus} \\
m_2 (u_2 - h_i) &= m_1 U_1 - m_1 h_i + Q_{aus} \\
m_2 &= \frac{m_2 U_1 - m_1 h_i + Q_{aus}}{(u_2 - h_i)} = 9,679.31 \, \text{kg} \\
\Delta m_{21} &= m_2 - m_1 = 3,921.31 \, \text{kg}
\end{align*}

``````latex


\section*{Problem 1 (e)}

\begin{equation*}
    \delta S_{12}
\end{equation*}

\begin{equation*}
    m_2 \cdot S_2 - m_1 \cdot S_1 =
\end{equation*}

\begin{equation*}
    \Delta S_{12} = 15475 \frac{kJ}{K}
\end{equation*}

\subsection*{TAB A-Z:}

\begin{equation*}
    S_1 = S_f + x (S_g - S_f)
\end{equation*}

\begin{equation*}
    S_f (100^\circ C) = 1.3069
\end{equation*}

\begin{equation*}
    S_g (100^\circ C) = 7.3595
\end{equation*}

\begin{equation*}
    x = 0.005
\end{equation*}

\begin{equation*}
    S_1 = 1.33717
\end{equation*}

\begin{equation*}
    S_2 = S_f (700^\circ C) = \text{TAB A-Z} = 0.9549
\end{equation*}

\subsection*{aus (d)}

\begin{equation*}
    M_2 = 9675.31
\end{equation*}

\begin{equation*}
    M_1 = 5755
\end{equation*}

``````latex


