
``````latex


\section*{2}
\subsection*{a)}
\begin{align*}
0 &= \dot{m} (h_{\text{ein}} - h_{\text{aus}}) + \dot{Q}_R - Q_{AB} \\
Q_{AB} &= \dot{Q}_R + \dot{m} (h_{\text{ein}} - h_{\text{aus}}) = 100 \text{kW} + 0.3 \frac{\text{kg}}{\text{s}} (292.98 \frac{\text{kJ}}{\text{kg}} - 419.04 \frac{\text{kJ}}{\text{kg}}) = \underline{62.18 \text{kW}}
\end{align*}
\begin{align*}
h_{\text{ein}} &= h(70^\circ C) = 292.98 \frac{\text{kJ}}{\text{kg}} \\
h_{\text{aus}} &= h(120^\circ C) = 419.04 \frac{\text{kJ}}{\text{kg}}
\end{align*}

\subsection*{b)}
\[
\overline{T}_{Fx} = \frac{\int_{s_e}^{s_a} T ds}{s_a - s_e} = \boxed{}
\]

\subsection*{c)}
``````latex


