
``````latex


\section*{Aufgabe 1:}

\subsection*{a)}

\[
\dot{m} = 0{,}3 \, \frac{\text{kg}}{\text{s}}
\]

\[
\dot{Q}_{\text{aus}} = \dot{m} \left( h_{\text{aus}} - h_{\text{ein}} \right) - \dot{Q}_{a}
\]

\subsubsection*{Tabelle A2:}

\[
h_{\text{ein}} = h_f \left( 70^\circ \text{C} \right) = 292{,}88 \, \frac{\text{kJ}}{\text{kg}}
\]

\[
h_{\text{aus}} = h_f \left( 100^\circ \text{C} \right) = 419{,}04 \, \frac{\text{kJ}}{\text{kg}}
\]

\[
\dot{Q}_{\text{aus}} = -62{,}187 \, \text{kW}
\]

\subsection*{b)}

\[
\overline{T} = \frac{\int_{s_e}^{s_a} T \, ds}{s_a - s_e} = \frac{c_p \left( T_a - T_e \right)}{c_p \ln \left( \frac{T_a}{T_e} \right)} = 293{,}12 \, \text{K}
\]

\[
T_a = T_{\text{K,aus}} = 288{,}15 \, \text{K}
\]

\[
T_e = T_{\text{K,ein}} = 288{,}15 \, \text{K}
\]

``````latex


\section*{Aufgabe 1:}

\subsection*{c)}

\begin{equation*}
0 = \dot{m}_{\text{ein}} (s_e - s_a) + \frac{\dot{Q}_{\text{aus}}}{T_{\text{KF}}} + \frac{\dot{Q}_R}{T_R} + S_{\text{erz}}
\end{equation*}

\begin{equation*}
S_{\text{erz}} = \dot{m}_{\text{ein}} (s_a - s_e) + \frac{\dot{Q}_{\text{aus}}}{T_{\text{KF}}} = \frac{\dot{Q}_R}{T_R}
\end{equation*}

\begin{equation*}
S_{\text{erz}} = - \frac{\dot{Q}_{\text{aus}}}{T_{\text{KF}}} = 0{,}212 \frac{\text{kJ}}{\text{kg K}}
\end{equation*}

\subsection*{d)}

\begin{equation*}
m_2 \, u_2 - m_1 \, u_1 = \Delta m_2 \, h_{\text{ein}}
\end{equation*}

\textbf{Tabelle A-2} f√ºr $u_{1f}$, $u_{1g}$, $u_f (70^\circ C)$, $h_{\text{ein}}$

\begin{equation*}
u_{1f} = 418{,}94 \frac{\text{kJ}}{\text{kg}}, \quad u_{1g} = 2506{,}4 \frac{\text{kJ}}{\text{kg}}
\end{equation*}

\begin{equation*}
u_1 = u_{1f} + x_0 (u_{1g} - u_{1f}) = 429{,}8 \frac{\text{kJ}}{\text{kg}}
\end{equation*}

\begin{equation*}
u_2 = u_f (70^\circ C) = 292{,}95 \frac{\text{kJ}}{\text{kg}}
\end{equation*}

\begin{equation*}
h_{\text{ein}} = 83{,}96 \frac{\text{kJ}}{\text{kg}}
\end{equation*}

\begin{equation*}
m_2 = \Delta m_2 + m_1
\end{equation*}

\begin{equation*}
\Delta m_2 \, u_2 + m_1 (u_2 - u_1) = \Delta m_2 \, h_{\text{ein}}
\end{equation*}

\begin{equation*}
\frac{m_1 (u_2 - u_1)}{h_{\text{ein}} - u_2} = \Delta m_2
\end{equation*}

\begin{equation*}
\Delta m_2 = 3756{,}9 \, \text{kg}
\end{equation*}

``````latex


\section*{Aufgabe 1:}

\subsection*{a)}

\begin{align*}
\Delta s_{12} &= s_2 - s_1
\end{align*}

\subsection*{Tabelle A-2:}

\begin{align*}
s(100^\circ C)_f &= 1{,}306 \frac{kJ}{kg \cdot K} & s(100^\circ C)_g &= 7{,}358 \frac{kJ}{kg \cdot K} \\
s(90^\circ C)_f &= 0{,}955 \frac{kJ}{kg \cdot K}
\end{align*}

\begin{align*}
s_1 &= s_f + x_0 (s_g - s_f) = 1{,}337 \frac{kJ}{kg \cdot K} \\
s_2 &= 0{,}955 \frac{kJ}{kg \cdot K}
\end{align*}

\begin{align*}
\Delta s_{12} &= s_2 - s_1 = -0{,}382 \frac{kJ}{kg \cdot K}
\end{align*}

``````latex


