
``````latex


\section*{4}

\subsection*{a)}

\begin{description}
    \item[Graph:] The graph is a pressure-temperature ($p$-$T$) diagram. The $y$-axis is labeled $p$ (pressure) and the $x$-axis is labeled $T [^\circ C]$ (temperature in degrees Celsius). There is a closed loop with four points labeled 1, 2, 3, and 4. The loop starts at point 1, goes to point 2, then to point 3, then to point 4, and back to point 1. The loop is roughly elliptical in shape, with point 1 at the top right, point 2 at the bottom right, point 3 at the bottom left, and point 4 at the top left.
\end{description}

\subsection*{b)}

\textbf{Energiebilanz}

\[
\dot{m}_{R134a} (h_2 - h_1) + \dot{Q}_K = 0
\]

\[
\Rightarrow \dot{m}_{R134a} = - \frac{\dot{Q}_K}{h_2 - h_1}
\]

\textbf{Energiebilanz}

\[
\dot{m}_{R134a} (h_3 - h_2) + \dot{W}_K = 0
\]

\[
\dot{m}_{R134a} = - \frac{\dot{W}_K}{h_2 - h_3}
\]

\textbf{Gegeben:}

\[
h_2 (8 \text{bar}, x=1) = 255.05 \frac{\text{kJ}}{\text{kg}}
\]

(TAB A8)

\[
T_{H2} = 15.45^\circ C
\]

\[
\Delta T \text{ von 2} \rightarrow 1 = 6^\circ C \Rightarrow T_1 = 9.45^\circ C
\]

``````latex

\section*{Aufgabe 1}

Energiebilanz

\[
\dot{m} \left( h_3 - h_2 \right) + W_u = 0
\]

\[
\dot{m} = \frac{W_u}{h_2 - h_3}
\]

4 $\rightarrow$ 1 \quad $s = \text{const}$

\[
s_4 (x = 0, s'_{3, \text{ev}}) = 0,2419
\]

\[
s_{4u} = s_3 = s_{3, \text{F}} + x \left( s_{3, \text{g}} - s_{3, \text{F}} \right)
\]

\[
x = \frac{s_4 - s_{3, \text{F}}}{s_{3, \text{g}} - s_{3, \text{F}}}
\]

\[
h_3 = h_{3, \text{F}} + x \left( h_{3, \text{g}} - h_{3, \text{F}} \right)
\]

\[
= h_{3, \text{F}} + \left( \frac{s_4 - s_{3, \text{F}}}{s_{3, \text{g}} - s_{3, \text{F}}} \right) \left( h_{3, \text{g}} - h_{3, \text{F}} \right)
\]

``````latex


\section*{Problem 4}

\subsection*{c)}

\[
\Delta x \text{ von } 2 \rightarrow 1 = 6^\circ \text{C}
\]

\[
\text{Bei } 8.8 \text{ bar}, x = 1 \quad h_2 = 255.05, \tau = 15.45
\]

\[
\therefore \quad T_1 = 15.45^\circ \text{C}
\]

\[
P_u = P_1 = P(53)
\]

\subsection*{d)}

\[
\mathcal{E}_u = \frac{|Q_{zu}|}{|Q_{ab}| - |Q_{zu}|} = \frac{| \dot{Q}_{zu} |}{| \dot{W}_u |} \quad \text{aus } 0 = \dot{m}(h_2 - h_1) + \dot{Q}_u
\]

\[
= \frac{\dot{Q}_u}{\dot{W}_u} = \frac{\dot{m}_{RT12} (h_1 - h_2)}{\dot{W}_u}
\]

```