
``````latex


\section*{1}
\subsection*{a)}
Energiebilanz:

\[
0 = \dot{m} (h_{\text{ein}} - h_{\text{aus}}) - \dot{Q}_{\text{aus}} + \dot{Q}_R
\]

\[
\dot{Q}_{\text{aus}} = \dot{m} (h_{\text{ein}} - h_{\text{aus}}) + \dot{Q}_R
\]

\[
h_{\text{ein}} (70^\circ C, x=0) : 292{,}98 \frac{kJ}{kg}
\]

\[
h_{\text{aus}} (100^\circ C, x=0) : 419{,}04 \frac{kJ}{kg}
\]

\[
\Rightarrow \dot{Q}_{\text{aus}} = 0{,}3 (292{,}98 - 419{,}04) + 700
\]

\[
= 62{,}18 kW
\]

\subsection*{b)}
\[
\eta = \frac{\int_{s_e}^{s_a} T ds}{s_a - s_e} = \frac{\Delta u}{\Delta s}
\]

\[
s_{\text{ein}} (70^\circ C, x=0) : 0{,}9549
\]

\[
s_{\text{aus}} (100^\circ C, x=0) : 1{,}7069
\]

\[
\eta = \frac{419{,}04 - 292{,}98}{1{,}7069 - 0{,}9549} = 358{,}125 K
\]

``````latex


\section*{Student Solution}

\subsection*{c)}

\begin{equation*}
0 = \dot{m} (s_{ein} - s_{out}) + \frac{\dot{Q}_R}{T} - \frac{\dot{Q}_{out}}{T} + \dot{s}_{ev.2}
\end{equation*}

\begin{equation*}
\dot{s}_{ev.2} = \dot{m} (s_{out} - s_{ein}) + \frac{\dot{Q}_{out}}{T} - \frac{\dot{Q}_R}{T}
\end{equation*}

$s_{ein}, s_{out}$ aus Teil b;

\begin{equation*}
\dot{s}_{ev.2} = 0.3 (1.3069 - 0.9544) + \frac{65}{295} - \frac{100}{295}
\end{equation*}

\begin{equation*}
= -0.0473 \frac{kJ}{K}
\end{equation*}

\subsection*{d)}

\begin{equation*}
m_2 u_2 - m_1 u_1 = \Delta m_{12} u_{12} + Q_R
\end{equation*}

\begin{align*}
m_1 &= 5755 \, \text{kg} \\
m_2 &= 5755 + \Delta m
\end{align*}

\begin{equation*}
u_2 = u_f + x (u_g - u_f)
\end{equation*}

\begin{equation*}
u_2 (1000 \, \text{C}) = 478.94 + 0.005 \left( 2506.5 - 478.94 \right)
\end{equation*}

\begin{equation*}
= 429.3778 \frac{kJ}{kg}
\end{equation*}

\begin{equation*}
u_2 = u_f + x u_f (70 \, \text{C}) = 292.95 \frac{kJ}{kg}
\end{equation*}

\begin{equation*}
h_{12} = h (20 \, \text{C}, x = 0) = 83.95
\end{equation*}

\begin{equation*}
\Rightarrow (m_1 + \Delta m) u_2 - m_1 u_1 = \Delta m u_{12} + Q_R
\end{equation*}

\begin{equation*}
\Delta m (u_{12} - u_2) = -m_1 u_1 + m_1 u_2 - Q_R
\end{equation*}

\begin{equation*}
\Delta m = \frac{-m_1 u_1 + m_1 u_2 - Q_R}{u_{12} - u_2}
\end{equation*}

``````latex


\section*{1d) weiter:}

\[
\Delta m = - \frac{5775 (429,377) + 5775 (292,95) - 35 \cdot 10^3}{83,95 - 292,95}
\]

\[
= 3937 \, \text{kg}
\]

\section*{e)}

\[
s_1 (400^\circ \text{C}) \text{daz} = 1,3069 \frac{\text{kJ}}{\text{kg}}
\]

\[
S_u = 1,3069 \cdot 5775 = 7547,3 \frac{\text{kJ}}{\text{kg}}
\]

\[
s_2 (40^\circ \text{C}) = 0,9549
\]

\[
S_x = 0,9549 (5775 + 3600) = 8952,2 \frac{\text{kJ}}{\text{kg}}
\]

\[
S_{\text{erz}} = \left( \frac{35 \cdot 10^3}{40 - 20} \right) = S_{\text{erz}} = 1400 \frac{\text{kJ}}{\text{kg}} = \frac{Q_{\text{B,itz}}}{T}
\]

\[
\Delta S = -S_1 + (S_x + S_{\text{erz}})
\]

\[
= -7547,3 + (8952,2 + 1400)
\]

\[
= 2804,9 \frac{\text{kJ}}{\text{kg}}
\]

``````latex


