
``````latex


\section*{Aufgabe 1}

a) E-Bilanz um Reaktor (stationär)

\[
0 = \dot{Q}_R - \dot{Q}_{\text{aus}} + \dot{m}_{\text{ein}} (h_e - h_a)
\]

\[
\Rightarrow \dot{Q}_{\text{aus}} = \dot{Q}_R + \dot{m}_{\text{ein}} (h_e - h_a)
\]

\[
h_e = h_f (20^\circ C) + x_D (h_g (70^\circ C) - h_f (70^\circ C))
\]

\[
\text{Tabelle A-2} \Rightarrow 292.98 \frac{\text{kJ}}{\text{kg}} + 0.005 (2626.8 \frac{\text{kJ}}{\text{kg}} - 292.98 \frac{\text{kJ}}{\text{kg}})
\]

\[
\Rightarrow h_e = 304.65 \frac{\text{kJ}}{\text{kg}}
\]

analog gilt für $h_a$

\[
h_a = h_f (100^\circ C) + x_D (h_g (100^\circ C) - h_f (100^\circ C))
\]

\[
\text{Tab A-2} \Rightarrow 419.04 + 0.005 (2676.1 - 419.04) \frac{\text{kJ}}{\text{kg}}
\]

\[
\Rightarrow h_a = 430.325 \frac{\text{kJ}}{\text{kg}}
\]

``````latex


\section*{Aufgabe 1}

\subsection*{a)}
\begin{align*}
&\rightarrow \text{einsetzen in} \quad \dot{Q}_{\text{aus}} = \dot{Q}_R + \dot{m} (h_e - h_a) \\
&= 100 \frac{\text{kJ}}{\text{s}} + 0.3 \frac{\text{kg}}{\text{s}} \left( 304.65 - 930.325 \right) \frac{\text{kJ}}{\text{kg}} \\
&= 62.3 \frac{\text{kJ}}{\text{s}} = \dot{Q}_{\text{aus}}
\end{align*}

\subsection*{b)}
\begin{align*}
\overline{T}_{\text{KF}} &= \frac{\int_{\text{ein}}^{\text{aus}} T \, ds}{s_{\text{aus}} - s_{\text{ein}}} = \frac{h_a - h_e}{T_a - T_e}
\end{align*}

\subsection*{c)}
Entropiebilanz um Kühlwand

\begin{center}
\begin{tabular}{c}
\begin{minipage}{0.8\textwidth}
\centering
\begin{picture}(200,50)
\put(0,20){\line(1,0){200}}
\put(0,30){\line(1,0){200}}
\put(100,30){\vector(0,-1){10}}
\put(100,20){\vector(0,1){10}}
\put(105,25){$\dot{Q}_{\text{aus}}$}
\put(95,5){$\dot{Q}_{\text{aus}}$}
\end{picture}
\end{minipage}
\end{tabular}
\end{center}

\begin{align*}
0 &= \frac{\dot{Q}_{\text{aus}}}{T_{\text{Reaktor}}} = \frac{\dot{Q}_{\text{aus}}}{T_{\text{KF}}} + \dot{S}_{\text{erzeugt}}
\end{align*}

``````latex


\section*{Aufgabe 1}

\subsection*{c)}
\begin{equation*}
    \dot{S}_{\text{erz}} = \frac{\dot{Q}_{\text{aus}}}{T_{\text{KF}}} - \frac{\dot{Q}_{\text{acs}}}{T_{\text{Reaktor}}} = 62.3 \frac{\text{kJ}}{\text{s}} \left( \frac{1}{293 \text{K}} - \frac{1}{373.15 \text{K}} \right)
\end{equation*}
\begin{equation*}
    = 44.3 \frac{1}{\text{K} \cdot \text{s}} = \dot{S}_{\text{erz}}
\end{equation*}

\subsection*{d)}
\textbf{E-Bilanz}
\begin{equation*}
    U_2 - U_1 = + Q_{R,12} - Q_{\text{aus}} + \Delta m_{12} \cdot h_{(200)}
\end{equation*}

``````latex


