
``````latex


\section*{Aufgabe 1}

\subsection*{a)}

\[
\dot{Q}_{\text{aus}} = \dot{m} (h_e - h_a) + \dot{Q}_R
\]

\[
h_e = h \left( T_{\text{e}} \right) + h_{fg} \left( T = 700^\circ \text{C} \right) - h_e
\]

\[
h_{ea} = h \left( T_{\text{e}} \right) + h_{fg} \left( T = 700^\circ \text{C} \right) = h_a
\]

aus Tabelle A2

\[
h_e = 2333,845 \frac{\text{kJ}}{\text{kg}}
\]

\[
h_a = 2252 \frac{\text{kJ}}{\text{kg}}
\]

\[
\Rightarrow \dot{Q}_{\text{aus}} = 0,3 \left( 2252 - 2333,8 \right) + 700 \text{ kW} = 70,36 \text{ kW}
\]

\subsection*{b)}

(weiter mit \(\dot{Q}_{\text{aus}} = 65 \text{ kW}\))

\[
\Delta S = S_e - S_a = \frac{\dot{Q}}{T}
\]

\[
T_i = \int_{S_i}^{S_e} T dS = \frac{S_e \cdot T_i - S_e \cdot T_a}{S_i - S_e}
\]

\[
S_e - S_a = S_i \left( \Delta S \right)
\]

\[
S_e - S_a = \int_{T_a}^{T_e} \frac{c}{T} dT = c \ln \left( T_e \right) - c \ln \left( T_a \right)
\]

``````latex


C) (weiter mit $T_K = 285K$)

\[
Q = \dot{m}(s_2 - s_1) = \sum \dot{Q}_i + \dot{S}_{evz}
\]

\[
- \dot{S}_{evz} = 0,3 \frac{kg}{s} \cdot (s_1(100^\circ C) - s_2(70^\circ C)) = \frac{6533}{285K} - \frac{100kJ}{285K}
\]

\[
\dot{S}_{evz} = \Delta u \cdot T \cdot A \cdot 2
\]

\[
s_1(100^\circ C) = 1,3063
\]

\[
s_1(70^\circ C) = 0,9349
\]

\[
\Rightarrow \dot{S}_{evz} = 0,258 \frac{kJ}{s}
\]

d) $\Delta E = \Delta U = \dot{m} (u_1 - u_2)$

\[
u_1 = u_{fg} \cdot (x \cdot u_{fg}(70,0^\circ C) + (1-x) \cdot u_1(100^\circ C))
\]

\[
u_2 = u_f(70^\circ C)
\]

\[
\Rightarrow u_1 = 0,005 \cdot 2506,5 + 0,995 \cdot 48,91 \left( \frac{4}{4,5} \right) = 429,38 \frac{kJ}{kg}
\]

\[
u_2 = 292,55 \frac{kJ}{kg}
\]

\[
\Rightarrow \Delta E = 5755 \cdot (429,38 - 292,55) = 7841,83245 = 785,0 \, MJ
\]

\[
\Delta E = \Delta m \cdot c_{wasser} \cdot \Delta T
\]

\[
\Delta E = (\dot{m}_{\text{neu}} - \dot{m}) \cdot c_w \cdot \Delta T
\]

\[
\dot{m}_{\text{neu}} = \frac{\Delta E}{c_w \cdot \Delta T} + \dot{m}, \quad c_w = 4,22
\]

\[
\dot{m}_{\text{neu}} = \frac{785000 \, kJ}{4,22 \frac{kJ}{kg \cdot K} \cdot 30} + 5755 = 11455 \, kg = 9475 \, kg
\]

\[
\Rightarrow \Delta m = 9475 - 5755 = 3720 \, kg
\]

``````latex

\begin{itemize}
    \item[(e)] \(\Delta S = m_2 s_2 - m_1 s_1\)
    
    \[
    s_1 = 0{,}005 - s_f(100^\circ C) + 0{,}935 \cdot s_f(100^\circ C)
    \]
    
    \[
    s_2 = s_f(70^\circ C) = 6{,}9543 \frac{kJ}{kgK}
    \]
    
    \[
    s_1 = 1{,}337 \frac{kJ}{kgK}
    \]
    
    \[
    \Rightarrow \Delta S = 8{,}475 \cdot 1{,}337 - 5{,}255 \cdot 0{,}8548 = 7172{,}6 \frac{kJ}{K}
    \]
    
    There is a small arrow pointing to the right next to the final result.
\end{itemize}

``````latex


