
``````latex


\section*{2.}
\textbf{a)} isobare Einheiten $p_0 = p_0$

\begin{description}
    \item[Graph Description:] The graph is a Temperature-Entropy ($T$-$s$) diagram. The x-axis is labeled $s \left[ \frac{k}{kg \cdot K} \right]$ and the y-axis is labeled $T [K]$. The graph consists of several lines and points:
    \begin{itemize}
        \item Point 1 is at the bottom left.
        \item A line from point 1 to point 2 is labeled "adiabat rev".
        \item A vertical line from point 2 to point 3 is labeled "isobar".
        \item A line from point 3 to point 4 is labeled "adiabat rev".
        \item A vertical line from point 4 to point 5 is labeled "isobar".
        \item A line from point 5 to point 6 is labeled "adiabat rev".
        \item A line from point 6 back to point 1 is labeled "adiabat rev".
        \item Points 2 and 3 are connected by a dashed line labeled "isotrop".
        \item Points 4 and 5 are connected by a dashed line labeled "isotrop".
        \item The line from point 5 to point 6 is labeled $P_5 = P_4 = p_1$.
        \item The line from point 6 to point 1 is labeled $P_6 = p_0$.
        \item The region between points 1, 2, 3, and 4 is labeled "Mischkammer isobar".
    \end{itemize}
\end{description}

\textbf{b)} $w_6 \rightarrow w_6 \& T_6$

$5 \rightarrow 6$ rev adiabat isentrop $n = k = 1.5$

\[
0 = \text{images} \left[ h_5 - h_6 + \frac{w_6^2 - w_5^2}{2} \right] + \dot{Q} \rightarrow \dot{0}
\]

\[
\frac{T_6}{T_5} = \left( \frac{P_6}{P_5} \right)^{\frac{k-1}{k}} \quad T_6 = T_5 \left( \frac{P_6}{P_5} \right)^{\frac{k-1}{k}} = 383.36 \, K \quad 328.07 \, K
\]

\[
w_6^2 = 2 \text{images} \left[ h_5 - h_6 \right] = 2 \text{images} c_v (T_5 - T_6)
\]

\[
w_6 = \sqrt{2 \text{images} c_p \cdot k (T_5 - T_6)}
\]

\[
w_6 = 564.08 \, \frac{m}{s}
\]

\[
k = \frac{c_p}{c_v} \rightarrow c_v = c_p \cdot k
\]

``````latex

\section*{c)}

\[
\Delta e_{x,str} = e_{x,str6} - e_{x,str0}
\]

\[
\Delta e_{x,str} = \left[ h_a - h_e - T_0(s_a - s_e) + \Delta ke + \Delta pe \right]
\]

\[
= h_s - h_0 - T_0(s_0 - s_0) + \frac{\omega_2^2 - \omega_0^2}{2}
\]

\[
= c_p k(T_0 - T_0) - T_0 \left[ c_p \ln \left( \frac{T_0}{T_0} \right) - R \ln \left( \frac{p_0}{p_0} \right) \right] + \frac{\omega_2^2 - \omega_0^2}{2}
\]

\[
\Delta e_{x,str} = -26019.4 \frac{kJ}{kg}
\]

\section*{d)}

\[
\dot{e}_{x,verl} \text{ ges } \Phi = 0
\]

\[
0 = -\Delta \dot{e}_{str} + \dot{e}_{x,Q} - \dot{e}_{x,t} - \dot{e}_{x,verl}
\]

\[
\dot{e}_{x,verl} = -\Delta \dot{e}_{str} + \left( 1 - \frac{T_0}{T_B} \right) \dot{Q}_B
\]

\[
= 86958 \frac{kJ}{kg s}
\]

\[
= -26
\]

\[
= -100 \frac{kJ}{kg} \left( 1 - \frac{298.15 K}{1289 K} \right)
\]

``````latex


