
``````latex


1. \\
a) \\
\begin{equation*}
\dot{Q}_{\text{ein}} = \dot{Q}_{\text{aus}} + \dot{Q}_{\text{Verlust}}
\end{equation*}

\begin{equation*}
0 = \dot{m}_{\text{ein}} (h_{\text{ein}} - h_{\text{aus}}) + \dot{Q}_{\text{aus}} - \dot{Q}_{\text{Verlust}}
\end{equation*}

\begin{equation*}
\dot{Q}_{\text{aus}} = \dot{Q}_{\text{Verlust}} + \dot{m}_{\text{ein}} (h_{\text{aus}} - h_{\text{ein}})
\end{equation*}

\begin{equation*}
\dot{m}_{\text{ein}} = \dot{m}_{\text{aus}}
\end{equation*}

\begin{equation*}
0 = \dot{Q}_{\text{Verlust}}
\end{equation*}

a) \\
\begin{equation*}
\dot{Q}_{\text{ein}} \rightarrow \dot{Q}_{\text{aus}} \text{ isobar}
\end{equation*}

\begin{equation*}
0 = \dot{m}_{\text{ein}} (h_{\text{ein}} - h_{\text{aus}}) + \dot{Q}_{\text{aus}} + \dot{Q}_{\text{Verlust}}
\end{equation*}

\begin{equation*}
\dot{Q}_{\text{aus}} = \dot{Q}_{\text{Verlust}} + \dot{m}_{\text{ein}} (h_{\text{aus}} - h_{\text{ein}})
\end{equation*}

\begin{equation*}
h_{\text{aus}} = 419.06 \frac{\text{kJ}}{\text{kg}}
\end{equation*}

\begin{equation*}
h_{\text{ein}} = 292.98 \frac{\text{kJ}}{\text{kg}}
\end{equation*}

\begin{equation*}
\dot{Q}_{\text{aus}} = 62.182 \frac{\text{kJ}}{\text{s}}
\end{equation*}

c)

``````latex


