
``````latex


\section*{Aufgabe 1:}

\subsection*{a)}
1. HS; stat. $\Rightarrow \dot{Q}_{\text{aus}} = \dot{m} (h_{\text{aus}} - h_{\text{ein}}) - Q_R$

\[
h_{\text{aus}} (200^\circ C, x=0) = 919.09 \frac{\text{kJ}}{\text{kg}} \quad \text{aus A-2}
\]

\[
h_{\text{ein}} (70^\circ C, x=0) = 292.98 \frac{\text{kJ}}{\text{kg}} \quad \text{aus A-2}
\]

\[
\dot{Q}_{\text{aus}} = 0.3 \frac{\text{kg}}{\text{s}} (919.09 - 292.98) = 3.78 \text{ kW} \quad \text{durchgestrichen} \quad -62.182 \text{ kW}
\]

\subsection*{b)}
\[
\overline{T}_{\text{RF}} = \frac{\int_{s_a}^{s_e} T ds}{s_a - s_e} = \frac{\int_{s_a}^{s_e} dH}{s_a - s_e} = c_p f \left( \frac{T_{\text{ausKF}} - T_{\text{einKF}}}{\ln \left( \frac{T_{\text{ausKF}}}{T_{\text{einKF}}} \right)} \right)
\]

\[
\frac{298.15 - 288.15}{\ln \left( \frac{298.15}{288.15} \right)} = 293.12 \text{ K}
\]

\subsection*{c)}
2. HS: $S_{\text{erz}} = \dot{m} (s_a - s_e) - \frac{\dot{Q}_{\text{aus}}}{T_{\text{Reaktor}}} - \frac{\dot{Q}_{\text{aus}}}{T_{\text{KF}}} \quad \text{am Wand!}$

\[
\Rightarrow S_{\text{erz}} = \frac{65 \text{ kW}}{293.15 \text{ K}} + \frac{65 \text{ kW}}{293.12 \text{ K}} = 0.4476 \frac{\text{kW}}{\text{K}} = 0.4476 \frac{\text{kW}}{\text{K}} = 0.4476 \frac{\text{kW}}{\text{K}} = 0.4476 \frac{\text{kW}}{\text{K}} = 0.4476 \frac{\text{kW}}{\text{K}} = 0.4476 \frac{\text{kW}}{\text{K}} = 0.4476 \frac{\text{kW}}{\text{K}} = 0.4476 \frac{\text{kW}}{\text{K}} = 0.4476 \frac{\text{kW}}{\text{K}} = 0.4476 \frac{\text{kW}}{\text{K}} = 0.4476 \frac{\text{kW}}{\text{K}} = 0.4476 \frac{\text{kW}}{\text{K}} = 0.4476 \frac{\text{kW}}{\text{K}} = 0.4476 \frac{\text{kW}}{\text{K}} = 0.4476 \frac{\text{kW}}{\text{K}} = 0.4476 \frac{\text{kW}}{\text{K}} = 0.4476 \frac{\text{kW}}{\text{K}} = 0.4476 \frac{\text{kW}}{\text{K}} = 0.4476 \frac{\text{kW}}{\text{K}} = 0.4476 \frac{\text{kW}}{\text{K}} = 0.4476 \frac{\text{kW}}{\text{K}} = 0.4476 \frac{\text{kW}}{\text{K}} = 0.4476 \frac{\text{kW}}{\text{K}} = 0.4476 \frac{\text{kW}}{\text{K}} = 0.4476 \```latex


\[
E_2 - E_1 = (m_{gs} + \Delta m) u_2 - m_{gs} u_1
\]

\[
u_1 (100^\circ C, x = 0.005) = u_f + x (u_g - u_f) = 929.378 \frac{kJ}{kg} \quad \text{aus A-2}
\]

\[
u_2 (70^\circ C, x = 0) = 292.95 \frac{kJ}{kg} \quad \text{aus A-2}
\]

\[
\Rightarrow (m_{gs} + \Delta m) u_2 - m_{gs} u_1 = \Delta m h_{12} + Q_{aus}
\]

\[
\Delta m (u_2 - h_{12}) = Q_{aus} + m_{gs} u_1 - m_{gs} u_2
\]

\[
\Delta m = \frac{Q_{aus} + m_{gs} (u_1 - u_2)}{u_2 - h_{12}} = \frac{-35 MJ + 5755 kg (929.378 - 292.95)}{292.95 - 83.96}
\]

\[
= 358932 kg
\]

\[
\Delta S = \Delta m_{gs} (s_{gs} + \Delta m) s_2 - m_{gs} s_1
\]

\[
s_1 (100^\circ C, (x = 0.005)) = s_f + x (s_g - s_f) = 1.337 \frac{kJ}{kg \cdot K} \quad \text{aus A-2}
\]

\[
s_2 (70^\circ C, x = 0) = 0.9599 \frac{kJ}{kg \cdot K} \quad \text{aus A-2}
\]

\[
\Rightarrow \Delta S = 929.37 kg \cdot 0.9599 - 5755 \cdot 1.337 = 1228.5 \frac{kJ}{K}
\]

``````latex


