
``````latex

\section*{Aufgabe 1:}

\subsection*{a) Energiebilanz:}

\begin{align*}
0 &= \dot{m} \left( h_{\text{ein}} - h_{\text{aus}} \right) + \dot{Q}_{\text{aus}} + \cancel{\dot{W}}^0 \\
\dot{Q}_{\text{aus}} &= \dot{m} \left( h_{\text{aus}} - h_{\text{ein}} \right) = \dot{m} \int_{T_{\text{ein}}}^{T_{\text{aus}}} c^f dT + \cancel{v^f (p_{\text{aus}} - p_{\text{ein}})}^0 \\
&= \dot{m} \, c^f \left( T_{\text{aus}} - T_{\text{ein}} \right)
\end{align*}

``````latex

\section*{b)}

\[
\dot{Q}_{\text{aus}} = 65 \text{kW}
\]

\[
\overline{T}_{\text{MF}} = \frac{\int_{s_{\text{ein}}}^{s_{\text{aus}}} T ds}{s_{\text{aus}} - s_{\text{ein}}} = \frac{q_{\text{kV}}}{s_{\text{aus}} - s_{\text{ein}}}
\]

\[
\text{aus Energiebilanz:} \quad q_{\text{kV}} = h_{\text{aus}} - h_{\text{ein}} = c \dot{m} (T_{\text{aus}} - T_{\text{ein}})
\]

\[
s_{\text{aus}} - s_{\text{ein}} = \int_{T_{\text{ein}}}^{T_{\text{aus}}} \frac{c \dot{m}}{T} dT = c \dot{m} \ln \left( \frac{T_{\text{aus}}}{T_{\text{ein}}} \right)
\]

\[
\Rightarrow \overline{T}_{\text{MF}} = \frac{T_{\text{aus}} - T_{\text{ein}}}{\ln \left( \frac{T_{\text{aus}}}{T_{\text{ein}}} \right)} = 293.123 \text{K}
\]

\section*{c) Entropiebilanz:}

\[
0 = \dot{m}_k \left( s_{\text{ein}} - s_{\text{aus}} \right) + \frac{\dot{Q}_{\text{aus}}}{\overline{T}_{\text{MF}}} + \dot{S}_{\text{erz}}
\]

\[
\Rightarrow \dot{S}_{\text{erz}} = \dot{m}_k \left( s_{\text{aus}} - s_{\text{ein}} \right) - \frac{\dot{Q}_{\text{aus}}}{\overline{T}_{\text{MF}}}
\]

\[
= \dot{m}_k c \ln \left( \frac{T_{\text{aus}}}{T_{\text{ein}}} \right) - \frac{\dot{Q}_{\text{aus}}}{\overline{T}_{\text{MF}}}
\]

``````latex


d) Energiebilanz - HÃ¼lloffenes System

\[
\Delta E = m_2 u_2 - m_1 u_1 = \Delta m_{12} h_{f12} + Q_{R,12} - Q_{aus,12}
\]

\begin{itemize}
    \item $m_1 = m_{ges,1} = 5755 \, \text{kg}$
    \item $m_2 = m_1 + \Delta m_{12}$
    \item $T_1 = 100^\circ \text{C}$
    \item $T_2 = 70^\circ \text{C}$
\end{itemize}

\[
-u_1 = u_f (100^\circ \text{C}) = (\text{TAB-A2}) = 418.44 \, \frac{\text{kJ}}{\text{kg}}
\]

\[
-u_2 = u_f (70^\circ \text{C}) = (\text{TAB-A2}) = 232.95 \, \frac{\text{kJ}}{\text{kg}}
\]

\[
h_{f12} = h_f (20^\circ \text{C}) = (\text{TAB-A2}) = 83.96 \, \frac{\text{kJ}}{\text{kg}}
\]

\[
(m_1 + \Delta m_{12}) u_2 - m_1 u_1 = \Delta m_{12} h_{12}
\]

\[
m_1 u_2 - m_1 u_1 = \Delta m_{12} (h_{12} - u_2)
\]

\[
\Delta m_{12} = m_1 \frac{u_2 - u_1}{h_{12} - u_2} = 3459.48 \, \text{kg} \quad \underline{3761.52 \, \text{kg}}
\]

\[
u_1 = u_f (100^\circ \text{C}) + x_0 (u_g (100^\circ \text{C}) - u_f (100^\circ \text{C})) = 429.58 \, \frac{\text{kJ}}{\text{kg}}
\]

``````latex


e) \quad \Delta m_{12} = 3600 \, \text{kg}

\textbf{Entropiebilanz:}

\[
\Delta S = m_2 \, s_2 - m_1 \, s_1
\]

\[
s_1 = (TAB - A - Z) = s_f(100^\circ C) + x_0 \left( s_g(100^\circ C) - s_f(100^\circ C) \right) = 1.33 + 14 \, \frac{\text{kJ}}{\text{kg K}}
\]

\[
s_2 = (TAB - A - Z) = s_f(70^\circ C) = 0.9549 \, \frac{\text{kJ}}{\text{kg K}}
\]

\[
\Rightarrow \Delta s = \left( m_1 + \Delta m_{12} \right) s_2 - m_1 \, s_1 = 1237.85 \, \frac{\text{kJ}}{\text{kg K}}
\]

``````latex


