
``````latex


1. (a) Stationärer Fließprozess:

\[
0 = \dot{m}_{\text{ein}} (h_{\text{ein}} - h_{\text{aus}}) + \dot{Q}_R - \dot{Q}_{\text{aus}}
\]

\[
\dot{Q}_{\text{aus}} = \dot{m}_{\text{ein}} (h_{\text{ein}} - h_{\text{aus}}) + \dot{Q}_R
\]

\[
h_{\text{ein}} - h(70^\circ C, x=0) = h_f(70^\circ C) = 292.98 \frac{\text{kJ}}{\text{kg}} \quad \text{(A-2)}
\]

\[
h_{\text{aus}} = h(100^\circ C, x=0) = h_f(100^\circ C) = 419.04 \frac{\text{kJ}}{\text{kg}} \quad \text{(A-2)}
\]

\[
\dot{Q}_{\text{aus}} = 0.3 \frac{\text{kg}}{\text{s}} \left( 292.98 \frac{\text{kJ}}{\text{kg}} - 419.04 \frac{\text{kJ}}{\text{kg}} \right) + 100 \text{kW}
\]

\[
= 62.18 \text{kW}
\]

(b) 

\[
\overline{T}_{\text{KF}} = \frac{\int_{s_{\text{aus}}}^{s_{\text{ein}}} T \, ds}{s_{\text{aus}} - s_{\text{ein}}}
\]

\[
\frac{h_{\text{aus}} - h_{\text{ein}}}{s_{\text{aus}} - s_{\text{ein}}} \quad \text{ideale Flüssigkeit}
\]

\[
dH = T \, ds + V \, dP \quad \overset{O, \text{isobar}}{\rightarrow}
\]

\[
= c_{p, \text{KF}} (T_{\text{aus}} - T_{\text{ein}}) + V \left( P_{\text{aus}} - P_{\text{ein}} \right)
\]

\[
= c_{p, \text{KF}} \ln \left( \frac{T_{\text{aus}}}{T_{\text{ein}}} \right)
\]

\[
\frac{T_{\text{aus}} - T_{\text{ein}}}{\ln \left( \frac{T_{\text{aus}}}{T_{\text{ein}}} \right)} = \frac{298.15 \text{K} - 288.15 \text{K}}{\ln \left( \frac{298.15 \text{K}}{288.15 \text{K}} \right)} = 293.12 \text{K}
\]

(c) 

\[
0 = \frac{\dot{Q}_{\text{aus}}}{T_{\text{KF}}} - \frac{\dot{Q}_{\text{aus}}}{T_{\text{Reaktor,1}}} + \dot{S}_{\text{erz}}
\]

\[
\dot{S}_{\text{erz}} = \frac{\dot{Q}_{\text{aus}}}{T_{\text{KF}}} - \frac{\dot{Q}_{\text{aus}}}{T_{\text{Reaktor,1}}} = 0.0455 \frac{\text{kJ}}{\text{K}} \text{kW}
\]

(d) 

\[
\Delta E = \cancel{\Delta U} = m_2 u_2 - m_1 u_1 = \Delta m_{12} h_{\text{ein,12}} - \dot{Q}_{\text{aus,12}}
\]

\[
\Delta m_{12} = \frac{m_2 u_2 - m_1 u_1 + \dot{Q}_{\text{aus,12}}}{h_{\text{ein,12}}} =
\]

``````latex


\section*{Fortsetzung 1.d:}

\begin{align*}
(m_1 + \Delta m_{12}) U_2 - m_1 U_1 &= \Delta m_{12} \cdot h_{\text{ein},12} - Q_{\text{aus},12} \\
\Delta m_{12} (U_2 - h_{\text{ein},12}) &= m_1 U_1 - m_1 U_2 - Q_{\text{aus},12} \\
\Delta m_{12} &= \frac{m_1 U_1 - m_1 U_2 - Q_{\text{aus},12}}{U_2 - h_{\text{ein},12}}, \quad m_1 = m_{\text{gas},1} = 3755 \, \text{kg}
\end{align*}

\begin{align*}
h_{\text{ein},12} &= h(20^\circ C, \, x=0) = h_f(20^\circ C) = 83.36 \, \frac{\text{kJ}}{\text{kg}} \quad \text{(A-2)} \\
U_1 &= U(100^\circ C, \, x=0) = U_f(100^\circ C) = 418.94 \, \frac{\text{kJ}}{\text{kg}} \quad \text{(A-2)} \\
U_2 &= U(70^\circ C, \, x=0) = U_f(70^\circ C) = 292.95 \, \frac{\text{kJ}}{\text{kg}} \quad \text{(A-2)}
\end{align*}

\begin{align*}
\Delta h_{12} &= U_1 = U(100^\circ C, \, x=0.005) - U_f(100^\circ C) + x \cdot (U_g(100^\circ C) - U_f(100^\circ C)) \\
&= 429.38 \, \frac{\text{kJ}}{\text{kg}} \quad \text{(A-2)}
\end{align*}

\begin{align*}
\Delta m_{12} &= 3588.4 \, \text{kg}
\end{align*}

\subsection*{(e)}

\begin{align*}
\Delta S &= m_2 S_2 - m_1 S_1 = (m_2 + \Delta m_{12}) S_2 - m_1 S_1
\end{align*}

\begin{align*}
S_1 &= s(100^\circ C, \, x=0.005) = s_f(100^\circ C) + x \cdot (s_g(100^\circ C) - s_f(100^\circ C)) \\
&= 1.337 \, \frac{\text{kJ}}{\text{kg} \cdot \text{K}} \quad \text{(A-2)}
\end{align*}

\begin{align*}
S_2 &= s(70^\circ C, \, x=0) = s_f(70^\circ C) = 0.3549 \, \frac{\text{kJ}}{\text{kg} \cdot \text{K}} \quad \text{(A-2)}
\end{align*}

\begin{align*}
\Delta S &= 1227.7 \, \frac{\text{kJ}}{\text{K}}
\end{align*}

``````latex


