
``````latex


\section*{1a}

\begin{align*}
&\dot{m}(h_e - h_a) + \dot{Q} = 0 \\
&\dot{m}(h_e - h_a) + \dot{Q}_R = \dot{Q}_{aus} = 62,18 \, \text{kW}
\end{align*}

\begin{align*}
h_e &= 292,98 \, \frac{\text{kJ}}{\text{kg}} \\
h_a &= 419,09 \, \frac{\text{kJ}}{\text{kg}}
\end{align*}

\subsection*{b}

\begin{align*}
T &= \frac{\int_{S_e}^{S_a} T \, ds}{S_a - S_e} = \frac{\int_{T_1}^{T_2} T \, ds}{\ln \left( \frac{T_a}{T_e} \right)} \\
&= \frac{e \left( T_a - T_e \right)}{\ln \left( \frac{T_a}{T_e} \right)} = \frac{T_a - T_e}{\ln \left( \frac{T_a}{T_e} \right)} = 293,12 \, \text{K}
\end{align*}

\subsection*{c}

\begin{align*}
0 &= \dot{m} \left[ S_e - S_a \right] + \frac{\dot{Q}_{aus}}{T} + \dot{S} \\
-\dot{S} &= 0,3 \, \frac{\text{kg}}{\text{s}} \left[ 0,9549 \, \frac{\text{kJ}}{\text{kgK}} + 1,308 \, \frac{\text{kJ}}{\text{kgK}} \right] \\
&+ \frac{62,18 \, \text{kW}}{293,12 \, \text{K}} \\
&\Rightarrow \dot{S} = 0,1 \, \frac{\text{kJ}}{\text{kgK}}
\end{align*}

\begin{align*}
S_{ex} - S_{0} &= S_{e} - S_{a} = c \ln \left( \frac{T_a}{T_{ein}} \right) \\
S_e &= 0,9549 \, \frac{\text{kJ}}{\text{kgK}} \\
S_a &= 1,308 \, \frac{\text{kJ}}{\text{kgK}}
\end{align*}

\subsection*{d}

\begin{align*}
Q_{aus12} &= 35 \, \text{MJ} \\
m_2 h_2 - m_1 u_1 &= m_1 h_1 \\
\text{Energie Wasser in Kessel Zustand 1} \\
x &= m_{g0} h_g + (1 - x) m_{g0} h_f = \Rightarrow 2706898,75 \, \frac{\text{kJ}}{\text{K}} = H_{gas}^1
\end{align*}

\begin{align*}
h_g &= 2676,1 \, \frac{\text{kJ}}{\text{kg}} \\
h_f &= 479,0 \, \frac{\text{kJ}}{\text{kg}}
\end{align*}

``````latex


