
``````latex


\section*{1.}

\[
\dot{m} = 0.3 \frac{\text{kg}}{\text{s}}
\]

\[
T_{\text{ein}} = 70^\circ \text{C} \quad T_{\text{aus}} = 100^\circ \text{C}
\]

\[
\text{siedend} \quad \text{siedend}
\]

\[
\text{mittlere konst. mass} = 573.5 \frac{\text{kg}}{\text{s}}
\]

\[
x_0 = 0.005
\]

\[
T = 100^\circ \text{C}
\]

\[
\text{Siedende Flüssigkeit } x = 1
\]

\subsection*{a)}

\[
Q_{\text{aus}}: \text{stationärer Fließprozess im Rechten}
\]

\[
0 = \dot{m} (h_{\text{ein}} - h_{\text{aus}}) + Q_{\text{aus}}
\]

\[
Q_{\text{aus}} = \dot{m} (h_{\text{aus}} - h_{\text{ein}})
\]

\[
Q_{\text{aus}} = 0.3 \frac{\text{kg}}{\text{s}} (2676.1 - 2626.8)
\]

\[
Q_{\text{aus}} = 0.3 \frac{\text{kg}}{\text{s}} \cdot 49.3 \frac{\text{kJ}}{\text{kg}} = 14.75 \text{kW}
\]

\[
h_{\text{ein}} = h_f (70^\circ \text{C})
\]

\[
h_{\text{aus}} = h_g (100^\circ \text{C})
\]

\subsection*{b)}

\[
T = \frac{\int_{s_e}^{s_a} T \, ds}{s_e - s_a}
\]

\[
T = \frac{q_{\text{zu}}}{s_a - s_e}
\]

``````latex


\section*{1. a) Hebbares System:}

\begin{align*}
    m_2 u_2 - m_1 u_1 &= \Delta m (h_{\text{ein}}) + Q_{R,12} \\
    m_1 &= 5755 \, \text{kg} \\
    u_1(T = 100^\circ C, x = 0.005) &= u_f + x (u_g - u_f) = 640.09 + 0.005 \cdot 422.7 \, \frac{\text{kJ}}{\text{kg}} \\
    m_2 &= m_1 + \Delta m \\
    u_2 (T = 70^\circ C) - u_f &= 292.35 \, \frac{\text{kJ}}{\text{kg}} \\
    h_{\text{ein}} (x = 1, 20^\circ) &= 2538.1 \, \frac{\text{kJ}}{\text{kg}} \\
    (m_1 + \Delta m) u_2 - m_1 u_1 &= \Delta m (h_{\text{ein}} + Q_{R,12}) \\
    \Delta m &= \frac{Q_{R,12} + m_1 u_1 - m_2 u_2}{u_2 - h_{\text{ein}}} \\
    \Delta m &= \frac{35000 \, \text{kJ} + 5755 \cdot 640.9 - 5755 \cdot 292.35}{292.35 - 2538.1} \\
    \Delta m &= 363 \, \text{kg}
\end{align*}

\section*{e)}

\begin{align*}
    \Delta s_{12} &= m_2 s_2 - m_1 s_1 \\
    \text{Austauschfaktor} \\
    m_2 &= m_1 + \Delta m = 5755 \, \text{kg} \\
    s_2 (T = 70^\circ, x = 1) &= 0.854 \, \frac{\text{kJ}}{\text{kg K}} \\
    s_1 (T = 100, x = 0.005)
\end{align*}

``````latex


