
``````latex


\section*{Aufgabe 1}

\subsection*{a) ges $\dot{Q}_{\text{aus}}$}

\[
\dot{Q}_{\text{aus}} = \dot{m}_{\text{ein}}
\]

\[
\dot{Q}_{\text{aus}} \quad \longleftarrow \quad \dot{m}_{\text{aus}}
\]

\[
Q_R = 100 \text{kW}
\]

\[
O = \dot{m} (h_{\text{ein}} - h_{\text{aus}}) + Q
\]

\[
h_{\text{ein}} (70^\circ \text{C})
\]

\[
h_{\text{ein}} - h_{\text{aus}} = c_{if} (T_{\text{ein}} - T_{\text{aus}}) + v_{if} (p_{\text{ein}} - p_{\text{aus}})
\]

\[
h_{\text{ein}} - h_{\text{aus}} = c_{if} (288.15 \text{K} - 293.15 \text{K})
\]

\subsection*{b)}

\[
T = \frac{\int_{s_a}^{s_e} T dS}{s_a - s_e} = h
\]

\subsection*{b)}

\[
T = \frac{\int_{s_a}^{s_e} T dS}{s_a - s_e} = \frac{h_a - h_e}{s_a - s_e}
\]

\textit{da reversibler station√§rer Prozess}

\[
h_{\text{ein}} - h_{\text{aus}} = c_{if} (T_{\text{ein}} - T_{\text{aus}}) + v_{if} (p_{\text{ein}} - p_{\text{aus}})
\]

\subsection*{c)}

\[
O = \dot{m}_{\text{ein}} (s_{\text{ein}} - s_{\text{aus}}) + \sum \frac{\dot{Q}_i}{T_i} + S_{\text{erz}}
\]

\subsection*{d)}

\[
\frac{dE}{dt} = \dot{m}_w (h_{\text{ein}} - h_{\text{aus}}) + \sum \dot{Q} - W
\]

\subsection*{e)}

\[
\Delta s_{12} = m_2 s_2 - m_1 s_1 = \sum \frac{\dot{Q}_i}{T_i} + S_{\text{erz}}
\]

``````latex


