
``````latex


\section*{Aufgabe 1}

\subsection*{1.a) stationarer Flie√üprozess}

\begin{align*}
0 &= \dot{m}_{ein} \left( h_e - h_a \right) - \dot{Q}_{aus} + \dot{Q}_R \\
h_e &= h_f \left( 70^\circ C \right) = 292,98 \frac{kJ}{kg} \\
h_a &= h_f \left( 100^\circ C \right) = 419,04 \frac{kJ}{kg} \\
\dot{Q}_{aus} &= \dot{m}_{ein} \left( h_e - h_a \right) + \dot{Q}_R \\
&= 62,182 \, kW
\end{align*}

``````latex

1. b)
\[
\overline{T}_{AF} = \frac{\int_{s_a}^{s_e} T \, ds}{s_a - s_e} = \frac{\frac{T_{aFau} + T_{aEin}}{2} (s_e - s_a)}{s_e - s_a}
\]
\[
= \frac{T_{aFau} + T_{aEin}}{2} = 293,15 \, K
\]

``````latex


1. c)

\[
0 = \dot{m}_{ein} (s_e - s_a)_{m} - \frac{\dot{Q}_{aus}}{T_{KF}} + \dot{S}_{ez}
\]

\[
s_e = s_f (70^\circ C) = 0.9549 \frac{kJ}{kg \cdot K}
\]

\[
s_a = s_f (100^\circ C) = 1.3069 \frac{kJ}{kg \cdot K}
\]

\[
\dot{S}_{ez} = -\dot{m}_{ein} (s_e - s_a) + \frac{\dot{Q}_{aus}}{T_{KF}}
\]

\[
= 0.3177 \frac{kJ}{K \cdot s}
\]

``````latex

1. d)

\[
\Delta E = \cancel{\Delta m_{12} (h_2 - h_1)} = 0
\]

\[
\Delta E = \Delta m_{12} \left[ h_2 - h_1 \right] - Q_{aus, 12} + \dot{Q}_{R, 12}
\]

\[
= m_2 u_2 - m_1 u_1 = (m_1 + \Delta m_{12}) u_2 - (m_1) u_1
\]

\[
\text{Values:}
\]

\[
h_1 = h_f (20^\circ C) = 83.96 \frac{KJ}{kg}
\]

\[
h_2 = h_f (70^\circ C) = 419.04 \frac{KJ}{kg}
\]

\[
u_1 = u_f (20^\circ C) = 83.95 \frac{KJ}{kg}
\]

\[
u_2 = u_f (70^\circ C) = 292.95 \frac{KJ}{kg}
\]

\[
m_1 = 5755 \, kg
\]

\[
\Delta m_{12} \ast [h_2 - h_1] = m_1 u_2 + \Delta m_{12} u_2 - m_1 u_1
\]

\[
\Delta m_{12} = \frac{m_1 u_2 - m_1 u_1}{h_2 - h_1 - u_2}
\]

\[
= 28549 \, kg
\]

``````latex


1. e) \(\Delta S = m_2 s_2 - m_1 s_1 = \sum_i dn_i s_i + \sum_j \frac{Q_j}{T_j} + \int e_z\)

``````latex


