
``````latex

1. a)

\[
\frac{d\dot{E}}{dt} = \sum \dot{m} h + \sum \dot{Q} - \sum \dot{W}
\]

\[
0 = \dot{m} (h_{\text{ein}} - h_{\text{aus}}) + \dot{Q}_R - \dot{Q}_{\text{a,w}}
\]

\[
\dot{Q}_{\text{a,w}} = Q_{\text{a,w}} \cdot \dot{m}_{\text{a}} (h_{\text{ein}} - h_{\text{aus}})
\]

\[
h_{\text{ein}} = h(70^\circ C, \text{siedende Fl.}) = h(30^\circ C, 3,1482 \text{bar}) = 232,88 \frac{\text{kJ}}{\text{kg}}
\]

\[
h_{\text{aus}} = h(100^\circ C, \text{siedende Fl.}) \Rightarrow h(100^\circ C, 1,014 \text{bar}) = 419,04 \frac{\text{kJ}}{\text{kg}}
\]

\[
\Rightarrow \dot{Q}_{\text{a,w}} = 100 + 0,3 (232,88 - 419,04)
\]

\[
\approx 62,2 \text{kW}
\]

b)

\[
\frac{T_2 - T_1}{\ln \left( \frac{T_2}{T_1} \right)} = \frac{238,15 - 286,15}{\ln \left( \frac{258,15}{291,15} \right)} \approx 293,1 \text{K}
\]

c)

\[
\frac{d\dot{S}}{dt} = \sum \dot{m} s + \sum \frac{\dot{Q}}{T} + \dot{S}_{\text{erz}}
\]

\[
0 = \dot{m} (s_{\text{KF,ein}} - s_{\text{KF,aus}}) + \frac{\dot{Q}_{\text{aus}}}{T_{\text{KF}}} + \dot{S}_{\text{erz}}
\]

\[
\dot{S}_{\text{erz}} = \dot{m}_{\text{KF}} (s_{\text{KF,aus}} - s_{\text{KF,ein}}) - \frac{Q_{\text{aus}}}{T_{\text{KF}}}
\]

\[
\text{ideales Fluid}
\]

\[
\Rightarrow s_{\text{aus}} - s_{\text{ein}} = \int_{T_{\text{ein}}}^{T_{\text{aus}}} \frac{c}{T} dT
\]

``````latex


\section*{Entropiebilanz um Reaktor}

\[
\dot{S} = \sum \dot{m} s + \frac{\dot{Q}}{T} + \dot{S}_{er}
\]

\[
0 = \dot{m} (s_{ein} - s_{aus}) + \frac{\dot{Q}_{erw}}{T_{HF}} + \dot{S}_{er}
\]

\[
\dot{S}_{er} = \frac{\dot{Q}_{erw}}{T_{HF}} + \dot{m} (s_{aus} - s_{ein})
\]

\[
s_{aus} = s(100^\circ \text{C}, \text{reduz. Fl.}) = s(100^\circ \text{C}, 0.04 \text{ bar}) = 1.3062 \frac{\text{kJ}}{\text{kg K}}
\]

\[
s_{ein} = s(30^\circ \text{C}, \text{reduz. Fl.}) = s(30^\circ \text{C}, 0.315 \text{ bar}) = 0.2549 \frac{\text{kJ}}{\text{kg K}}
\]

\[
\Rightarrow \dot{S}_{er} \times 22.4 \frac{\text{kJ}}{\text{K}}
\]

\section*{d)}

\[
\frac{dE}{dt} = \sum \dot{m} \cdot h + \sum \dot{Q} - \sum \dot{V}
\]

\[
\Delta U = \Delta m_{12} \cdot h_{ein_{12}} + Q_{er} - Q_{aus}
\]

\[
\Delta U = \Delta m_{12} \cdot h_{ein_{12}}
\]

\[
\Delta m_{12} \cdot \frac{\Delta U}{h_{ein_{12}}} = \frac{(m_1 + \Delta m_{12}) h_2}{h_{ein_{12}}} - \frac{m_1 h_1}{h_{ein_{12}}}
\]

\[
\Delta m_{12} - \Delta m_{12} = \frac{m_1 h_2}{h_{ein_{12}}} - \frac{m_1 h_1}{h_{ein_{12}}}
\]

\[
\Delta m_{12} \left( 1 - \frac{1}{h_{ein_{12}}} \right) = \frac{m_1}{h_{ein_{12}}} (h_2 - h_1)
\]

\[
\Rightarrow \Delta m = \frac{m_1}{h_{ein_{12}}} (h_2 - h_1) \cdot \frac{1}{1 - h_{ein_{12}}}
\]

``````latex


1. a) 
\[
h_{n_2} = h_1(100^\circ C, x = 0.005) = h_1(100^\circ) + x \left( h_{g_2}(100^\circ) - h_1(100^\circ) \right)
\]
\[
\approx 430.3 \, \frac{\text{kJ}}{\text{kg}} \quad \text{(A-2)}
\]

\[
h_2 = h(30^\circ C, x = 0) = h_f(30^\circ) = 292.88 \, \frac{\text{kJ}}{\text{kg}} \quad \text{(A-2)}
\]

\[
h_{en_{12}} = h(20^\circ C, x = 0) = h_f(20^\circ) = 83.96 \, \frac{\text{kJ}}{\text{kg}} \quad \text{(A-2)}
\]

\[
\Rightarrow \Delta h_{12} = \frac{535}{83.96} \left( 292.88 - 430.3 \right) \frac{1}{1 - 83.96}
\]

\[
\approx 109.5 \, \text{kJ}
\]

b) 
\[
\Delta S = S_2 - S_1 = m_2 S_2 - m_1 S_1
\]

\[
S_2 = S_f(30^\circ, \text{siehe F}) = 0.8542 \, \frac{\text{kJ}}{\text{kg K}} \quad \text{(A-2)}
\]

\[
S_1 = S_f(100^\circ) + x \left( S_g(100^\circ) - S_f(100^\circ) \right) \approx 1.337 \, \frac{\text{kJ}}{\text{kg K}}
\]

\[
\Delta S = (535 + 109) \cdot 0.8542 - 535 \cdot 1.337
\]

\[
\approx \underline{209.5 \, \frac{\text{kJ}}{\text{K}}}
\]

``````latex


