
``````latex


\section*{Aufgabe 1}

\subsection*{a)}

\begin{align*}
&\text{sst. Flie√üprozess} \quad ke = pe = 0 \\
&O = \dot{m} [h_e - h_a] + \dot{Q}_R = \dot{Q}_{aus} - W \quad W = 0 \\
&0 = \dot{m} [h_e - h_a] + \dot{Q}_R = 0.3 \left( 292.98 - 448.04 \right) + 100 \, \text{kW} = 62.782 \, \text{kW}
\end{align*}

\begin{align*}
\dot{m} = 0.3 \, \text{kg/s} \\
h_e = h_e (70^\circ \text{C}) \\
h_a = h_e (100^\circ \text{C}) = 292.98 \, \frac{\text{kJ}}{\text{kg}} \quad = 448.04 \, \frac{\text{kJ}}{\text{kg}}
\end{align*}

\subsection*{b)}

\begin{align*}
\int_{T_1}^{T_2} c_p \frac{dT}{T} &= \int_{T_1}^{T_2} \frac{Q}{T} \\
c_p \ln \left( \frac{T_2}{T_1} \right) &= \frac{10}{\ln \left( \frac{298.15}{288.15} \right)} = 288.12 \, \text{K}
\end{align*}

\subsection*{d)}

\begin{align*}
&\text{halb offenes} \\
&\text{geschlossenes System} \\
&\Delta E = Q_e - Q_{aus} - \dot{m}_2 [h_e] \\
&\dot{m}_2 = \dot{m}_1 + \Delta m_2 \\
&\dot{m}_2 u_2 - \dot{m}_1 u_1 = (\dot{m}_1 + \dot{m}_2) u_2 - \dot{m}_1 u_1 \\
&\Delta m_2 = m_2 \\
&\Delta m_2 (h_e - u_e) = m (u_2 - u_1) \\
&\Delta m_2 = \frac{SIS (292.98 - 448.04)}{83.96 - 292.98} = \frac{SIS (292.98 - 448.04)}{83.96 - 292.98} = 37.63 \, \text{kg}
\end{align*}

\begin{align*}
h_e = h_e (200^\circ \text{C}) = 83.96 \, \frac{\text{kJ}}{\text{kg}} \\
u_2 = u_e (70^\circ \text{C}) = 292.98 \, \frac{\text{kJ}}{\text{kg}} \quad \text{TAB A-2} \\
u_1 = u_e (100^\circ \text{C}) = 448.04 \, \frac{\text{kJ}}{\text{kg}}
\end{align*}

``````latex

\begin{equation}
\Delta S = m_{2} s_{2} - m_{1} s_{1} = Q \left( \frac{1}{T_{e}} - \frac{1}{T_{s}} \right)
\end{equation}

\begin{equation}
= (5755 \cdot 3.49 \frac{kJ}{kg} \cdot 0.95849 - 5755 \cdot 1.306 \frac{kJ}{kg} = 1287.18 \frac{kJ}{K}
\end{equation}

\textbf{TAB A-2}

\begin{equation}
s_{2} = s_{g}(70^{\circ}C) = 0.95849
\end{equation}

\begin{equation}
s_{1} = s_{f}(40^{\circ}C) = 1.306
\end{equation}

\textbf{c)}

\begin{equation}
\frac{dS}{dt} = \frac{Q}{T_{1}} + \frac{Q}{T_{2}}
\end{equation}

\begin{equation}
\frac{dS}{dt} = Q \left( \frac{1}{T_{1}} + \frac{1}{T_{2}} \right) + S_{cre}
\end{equation}

``````latex


