
``````latex


\section*{ex1}

\subsection*{a)}
\begin{align*}
1. HS: \quad 0 &= \dot{m}_{ein} (h_1 - h_2) + \dot{Q}_{zu} - \dot{Q}_{ab} \\
\dot{Q}_{ab, aus} &= \dot{m}_{ein} (h_1 - h_2) + \dot{Q}_{zu} \\
h_1 &= h_{1,f} \quad (70^\circ C) = 283.29298 \frac{kJ}{kg} \quad \text{Tabelle A-2} \\
h_2 &= h_{2,f} \quad (100^\circ C) = 419.04 \frac{kJ}{kg} \quad \text{Tabelle A-2} \\
\dot{Q}_{ab, aus} &= 0.3 \cdot (h_1 - h_2) + 100 = 62.182 \\
&= \boxed{62.182 \, \text{kW}}
\end{align*}

\subsection*{b)}
\begin{align*}
\bar{T} &= \frac{\int_{T_0}^{T_a} \frac{c_i}{T} dT}{\int_{T_0}^{T_a} c_i dT} \\
T_{a, aus} &= 25^\circ C \\
T_{e, ein} &= 15^\circ C \\
s_{a} - s_{e} &= \int_{T_0}^{T_a} \frac{c_i}{T} dT = c_i \ln \left( \frac{T_{a, aus}}{T_{e, ein}} \right)
\end{align*}

\subsection*{c)}
\begin{align*}
T_{ref} &= 295 K \\
\text{Entropiebilanz:} \quad 0 &= \dot{m}_{ein} (s_2 - s_1) + \frac{\dot{Q}_R}{T_R} + \frac{\dot{Q}_{zu}}{T_{zu}} - \frac{\dot{Q}_{ab}}{T_{ab}} + \dot{S}_{er, z} \\
\dot{S}_{er, z} &= \dot{m}_{ein} (s_2 - s_1) + \frac{\dot{Q}_R}{T_R} + \frac{\dot{Q}_{zu}}{T_{zu}} - \frac{\dot{Q}_{ab}}{T_{ab}} \\
s_2 &= s_{2,e} \quad (100^\circ C) = 1.306 \frac{kJ}{kgK} \quad \text{Tabelle A-2} \\
s_1 &= s_{1,e} \quad (70^\circ C) = 0.9543 \frac{kJ}{kgK} \quad \text{Tabelle A-2} \\
\Rightarrow \dot{S}_{er, z} &= 0.234 \frac{kJ}{K}
\end{align*}

``````latex


\begin{equation*}
\text{d)} \quad \frac{dE}{dt} = \dot{m}_1 \cdot \left( u_1 + \frac{p_1 v_1}{c^2} \right) - \dot{m}_2 \cdot \left( u_2 + \frac{p_2 v_2}{c^2} \right) + \dot{Q}_{R,12} = 0
\end{equation*}

\begin{equation*}
dE = \Delta U = \dot{m}_2 \left( h_1 - h_2 \right) + \dot{Q}_{R,12}
\end{equation*}

\begin{equation*}
h_1 (100^\circ C) = h_{u,1} + x \cdot \left( h_{ug} - h_{u,1} \right)
\end{equation*}

\begin{equation*}
\frac{T_{AB}}{\Delta t} = 415.04 + 0.005 \left( 2257.0 \right) = 430.325 \frac{kJ}{kg}
\end{equation*}

\begin{equation*}
h_2 (70^\circ C) = h_{u,2} + x \cdot \left( h_{ug} - h_{u,2} \right)
\end{equation*}

\begin{equation*}
\frac{T_{AB}}{\Delta t} = 232.55 + 0.005 \left( 2339.8 \right) = 304.64 \frac{kJ}{kg}
\end{equation*}

\begin{equation*}
\Delta U = \dot{m}_{12} \left( h_{u,2} - h_{u,1} \right) \dot{m}_{12} \left( u_2 - u_1 \right)
\end{equation*}

\begin{equation*}
u_2 (70^\circ C) = u_{u,2} + x \cdot \left( u_{ug} - u_{u,2} \right)
\end{equation*}

\begin{equation*}
\frac{T_{AB}}{\Delta t} = 232.55 + 0.005 \left( 2466.8 - 292.85 \right) = 303.533 \frac{kJ}{kg}
\end{equation*}

\begin{equation*}
u_1 (100^\circ C) = u_{u,1} + x \cdot \left( u_{ug} - u_{u,1} \right)
\end{equation*}

\begin{equation*}
\frac{T_{AB}}{\Delta t} = 415.04 + 0.005 \left( 2506.5 - 418.34 \right) = 423.837 \frac{kJ}{kg}
\end{equation*}

\begin{equation*}
\dot{m}_{12} u_2 + \dot{m}_{12} u_2 = \dot{m}_{12} \left( h_1 - h_2 \right) - \dot{Q}_R
\end{equation*}

\begin{equation*}
\Delta m_{12} \left( u_2 + h_2 - h_1 \right) = \dot{m}_{12} \left( u_1 - u_2 \right) - \dot{Q}_R
\end{equation*}

\begin{equation*}
\Delta m_{12} = \dot{m}_{12} \frac{u_1 - u_2 + \frac{\dot{Q}_R}{\dot{m}_{12}}}{u_2 + h_2 - h_1}
\end{equation*}

\begin{equation*}
= \boxed{3859.02 \, \text{kg}}
\end{equation*}

\begin{equation*}
\left( \dot{Q}_R = 35 \cdot 1000 \, \text{kJ} \right)
\end{equation*}

``````latex


\section*{ex.1}

\begin{equation*}
e) \quad \frac{dS}{dt} = \sum_i \left( \dot{m}_i s_i + \frac{\dot{Q}}{T} \right) - \dot{S}_{cr,2}
\end{equation*}

\begin{equation*}
\Delta S_{12} = \int \dot{m}_{12} (s_2 - s_1) - \frac{\dot{Q}_{12}}{T} = \dot{S}_{cr,2}
\end{equation*}

``````latex


