
``````latex


\section*{Aufgabe 3}

\subsection*{a)}

\[
\dot{m}_{1} = \frac{m \dot{V}_{3}}{A} = \frac{m^3 \dot{V}_{3}}{A} \cdot \rho \cdot v
\]

\[
A = \pi \left( \frac{d}{2} \right)^2 = \pi \left( \frac{7,85 \cdot 10^{-3}}{2} \right)^2
\]

\[
= 32 \, \text{kg} \cdot \frac{9,81 \, \text{N}}{\text{kg}} \cdot \frac{1}{7,85 \cdot 10^{-3} \, \text{m}^2} + 0,1 \, \text{kg} \cdot \frac{9,81 \, \text{N}}{\text{kg}} \cdot \frac{1}{7,85 \cdot 10^{-3} \, \text{m}^2} + 1,85 \, \frac{\text{N}}{\text{m}^2}
\]

\[
= 0,3977 \, \text{bar} + 1 \, \text{bar} = 1,3977 \, \text{bar}
\]

\subsection*{b)}

Der Druck \( P_{1,2} = P_{1,1} \) weil die Masse auf den Massen immer gleich ist.

\subsection*{c)}

\[
1 \, \text{HS} : \Delta U_{g} = Q - W \quad , \quad Q = \Delta U_{g} + W
\]

\[
W = \int_{V_{1}}^{V_{2}} P_{1,3} \, dV = P_{1,3} \cdot (V_{2} - V_{1}) \cdot P_{1,3}
\]

\[
\Delta U_{g} = m_{g} \cdot (U_{2} - U_{1}) = m_{g} \cdot (T_{2} - T_{1}) \cdot c_{v}
\]

\[
\text{für } V_{2} : V_{2} = \frac{m_{g} \cdot R \cdot T_{2}}{P_{1,3}} = \frac{3,9787 \cdot 10^{-3} \, \text{kg} \cdot 8,314 \, \frac{\text{J}}{\text{mol K}} \cdot 273,15 \, \text{K}}{1,3187 \cdot 10^{5} \, \frac{\text{N}}{\text{m}^2}} \cdot \frac{50 \, \text{kg}}{\text{kmol}}
\]

\[
= 1,708 \cdot 10^{-3} \, \text{m}^3
\]

\[
W = \cancel{\frac{3,9787 \cdot 10^{-3} \, \text{kg}}{1,708 \cdot 3,195 \cdot 10^{-3} \, \text{m}^3}} \cdot 1,3187 \cdot 10^{5} \, \frac{\text{N}}{\text{m}^2} = -0,2812 \, \text{kJ} = -0,2827 \, \text{J}
\]

\[
\Delta U_{g} = 3,9787 \cdot 10^{-3} \, \text{kg} \cdot (273,15 \, \text{K} - 773,15 \, \text{K}) \cdot 0,653 \, \frac{\text{kJ}}{\text{kg K}} = -1,0920 \, \text{kJ}
\]

\[
Q = \Delta U_{g} + W = -1,3662 \, \text{kJ} \quad \text{Die vom Gas abgegebene Wärme.}
\]

\[
Q_{12} = +1,3662 \, \text{J}
\]

``````latex

\section*{d)}

\[
T_{x_2} = 90^\circ C
\]

\textbf{1HS:}
\[
\Delta U_{x_1 BW} = Q - W = (7,36c\dot{2} - 0,2852) \, kJ = 7,0748 \, kJ
\]

\[
\Delta U_{x_2} = m_{BW} (u_2 - u_1)
\]

\[
u_2 = \frac{1 - x_2}{v_f (0,0931 \, c)} + \frac{x_2}{v_f (0,201 \, c)}
\]

\[
u_1 = v_f (0^\circ C) (1 - x_1) + v_f (0^\circ C) x_1, \quad x_1 = 0,16
\]

\[
m_{BW} (u_2 - u_1) = x_2 (u_f (T_x) - u_f (T_1)) + u_f (T_1) - u_1 = \Delta u_{x_2}
\]

\[
x_2 = \frac{\Delta u_{x_2} + u_f (T_1) - u_f (T_x)}{u_f (T_x) - u_f (T_1)}
\]

\[
x = \frac{7,0748 \, kJ}{0,1 \, kg} = \frac{(-0,085 \, \frac{kJ}{kg}) \cdot 0,1 + (-333,652 \, \frac{kJ}{kg}) \cdot 0,6 - (-0,053 \, \frac{kJ}{kg})}{-333,652 \, \frac{kJ}{kg} - (-0,053 \, \frac{kJ}{kg})}
\]

\[
= 0,575
\]

``````latex


