
``````latex


1. 
\begin{align*}
\dot{m} &= 0,3 \frac{\text{kg}}{\text{s}} \\
T_{\text{ein}} &= 70^\circ \text{C} \\
x_p &= 0,005
\end{align*}

\begin{align*}
\dot{Q}_R
\end{align*}

a) 
\begin{align*}
0 &= \dot{m} \cdot h_{\text{ein}} - \dot{m} \cdot h_{\text{aus}} + 100 \text{kW} - \dot{Q}_{\text{aus}} - \dot{W} \\
\dot{Q}_{\text{aus}} &= \dot{m} \cdot h_{\text{ein}} - \dot{m} \cdot h_{\text{aus}} + \dot{Q}_R
\end{align*}

\text{TAB A2}
\begin{align*}
h_{\text{ein}} &= h_f (70^\circ \text{C}) = 292,88 \frac{\text{kJ}}{\text{kg}} \\
h_{\text{aus}} &= h_f (100^\circ \text{C}) = 419,64 \frac{\text{kJ}}{\text{kg}} \\
\dot{m}_{\text{ein}} &= 0,3 \frac{\text{kg}}{\text{s}} \\
\dot{m}_{\text{aus}} &= 0,3 \frac{\text{kg}}{\text{s}} - \dot{m}_{\text{ein}}
\end{align*}

\begin{align*}
\Rightarrow \dot{Q}_{\text{aus}} &= \dot{m} (h_{\text{ein}} - h_{\text{aus}}) + 100 \text{kW} \\
\dot{Q}_{\text{aus}} &= 62,182 \text{kW}
\end{align*}

b) 
\begin{align*}
\text{Exergiebilanz um Kühlflüssigkeit} \\
0 &= \dot{E}_{\text{str}} + \dot{E}_{\text{q}} - \dot{W} - \dot{E}_{\text{umw}}
\end{align*}

c) 
\begin{align*}
T_{\text{KF}} &= 285 \text{K} \\
\text{ZBS} \\
0 &= \dot{m} (s_e - s_a) + \frac{\dot{Q}_{\text{aus}}}{T_{\text{KF}}} - \dot{s}_{\text{cz}}
\end{align*}

\begin{align*}
\dot{s}_{\text{cz}} &= \frac{\dot{Q}_{\text{aus}}}{T_{\text{KF}}} \\
\dot{s}_{\text{cz}} &= \frac{62,182 \text{kW}}{285 \text{K}} \\
\dot{s}_{\text{cz}} &= 0,2107 \frac{\text{kW}}{\text{K}} - \dot{s}_{\text{cz}}
\end{align*}

``````latex


\section*{a) Halboffenes System}

\begin{align*}
    M_2 U_2 - M_1 U_1 &= \Delta M \cdot h_{\text{ein}} + Q - CW \\
    M_1 &= M_{\text{ges}} \\
    Q &= Q_{\text{aus}} = 835 \text{MJ} \\
    M_2 &= m_{\text{ges}} + m_B \\
    (m_g + m_B) U_2 - m_g U_1 &= \Delta M \cdot h_{\text{ein}} + (-Q_{\text{aus}}) \\
    m_g U_2 + m_B U_2 - m_g U_1 &= \Delta m h + (x) \\
    \Delta m \left( \frac{U_2 - h_{\text{ein}}}{U_2 - h_{\text{ein}}} \right) &= m_g U_1 + (x) \\
    \Delta m &= \frac{M_{\text{ges}} h_{\text{ein}} + Q}{U_2 - h_{\text{ein}}}
\end{align*}

\begin{align*}
    h_{\text{ein}} &= h_f(100^\circ) - h_f(20^\circ) \\
    h_{\text{ein}} &= h_f(20^\circ) = 83.36 \frac{\text{kJ}}{\text{kg}}
\end{align*}

\begin{align*}
    M_{\text{ges}} &= 5755 \text{kg}
\end{align*}

\begin{align*}
    \Delta m &= \frac{5755 \text{kg} \cdot 418.94 \frac{\text{kJ}}{\text{kg}} - 835 \cdot 10^3 \text{kJ}}{292.35 - 83.36}
\end{align*}

\begin{align*}
    \Delta m &= 11368.9 \text{kg}
\end{align*}

\section*{e) Halboffen}

\begin{align*}
    M_{S2} - M_{S1} &= \Delta M \cdot S_{\text{ein}} + \frac{Q_{\text{ein}}}{T} - S_{\text{ez}} \\
    S_{\text{ez}} &= M_{S2} - M_{S1} + \Delta M \cdot S_{\text{ein}} - \frac{Q_{\text{ein}}}{T}
\end{align*}

\begin{align*}
    S_{\text{ez}} &= 1012.428 \text{kJ}
\end{align*}

\begin{align*}
    M_2 &= m_1 + m_2 = 9355 \text{kg} \\
    \Delta M_2 &= 3600 \\
    M_2 &= M_1 + S_2 \\
    M_1 &= M_A \\
    S_2 &= S_p(70^\circ) = 0.9549 \frac{\text{kJ}}{\text{kg}} \\
    S_1 &= S_p(100^\circ) + x \left( S_f(100^\circ) - S_p(100^\circ) \right) \\
    \Delta 2 &= 1.3063 + x \left( 7.3540 - 1.3063 \right) \\
    S_2 &= 4.339 \frac{\text{kJ}}{\text{kg}} \\
    S_{\text{ein}} &= S_p(70^\circ) = 0.2966 \\
    Q &= 35 \cdot 10^3 \text{kJ} \\
    T &= 255 K
\end{align*}

``````latex


