
``````latex


\section*{Aufgabe 1}

\subsection*{a)}

\begin{equation*}
O = \dot{m}_{ein} (h_{ein} - h_{aus}) + \dot{Q}_R - \dot{Q}_{aw} - \dot{W}^0
\end{equation*}

\begin{equation*}
\dot{m}_{ein} = \dot{m}_{aus} = \dot{m}
\end{equation*}

station√§rer Fallprozess

\begin{equation*}
\Rightarrow \dot{Q}_{aw} = \dot{m} (h_{ein} - h_{aus}) + \dot{Q}_R
\end{equation*}

\begin{equation*}
\dot{Q}_{aw} = 0,3 \frac{\text{kg}}{\text{s}} (293,88 \frac{\text{kJ}}{\text{kg}} - 930,12 \frac{\text{kJ}}{\text{kg}}) + 100 \text{kW} = \underline{58,86 \text{kW}}
\end{equation*}

\begin{equation*}
h_{ein} = h_f \left( 70^\circ \text{C} \right) = 292,88 \frac{\text{kJ}}{\text{kg}}
\end{equation*}

\begin{equation*}
X_D = \frac{h_{aus} - h_f}{h_g - h_f} \quad \text{bei} \quad T = 100^\circ \text{C}
\end{equation*}

\begin{equation*}
\Rightarrow h_{aus} = h_f + X_D (h_g - h_f) = 419,06 \frac{\text{kJ}}{\text{kg}} + 0,005 (2631,3 - 419,06) \frac{\text{kJ}}{\text{kg}} = 930,12 \frac{\text{kJ}}{\text{kg}}
\end{equation*}

\subsection*{b)}

\begin{equation*}
\overline{T}_{KF} = \frac{T_{KF,ein} + T_{KF,aus}}{2} = \frac{288,15 \text{K} + 298,15 \text{K}}{2} = \underline{293,15 \text{K}}
\end{equation*}

\subsection*{c)}

\textbf{Entropiebilanz:}

\begin{equation*}
0 = \dot{m} (s_{ein} - s_{aus}) + \frac{\dot{Q}_R}{T_{Trenn,1}} - \frac{\dot{Q}_{aw}}{T_{KF}} + \dot{S}_{erz}
\end{equation*}

\begin{equation*}
\Rightarrow \dot{S}_{erz} = \frac{\dot{Q}_{aw}}{T_{KF}} + \dot{m} \left( s_{ein} - s_{aus,ein} \right) - \frac{\dot{Q}_R}{T_{Trenn,1}}
\end{equation*}

\begin{equation*}
s_{aus} = s_f + X_D (s_g - s_f) = 1,3069 \frac{\text{kJ}}{\text{kg} \cdot \text{K}} + 0,005 (7,3589 - 1,3069) \frac{\text{kJ}}{\text{kg} \cdot \text{K}} = 1,3374 \frac{\text{kJ}}{\text{kg} \cdot \text{K}}
\end{equation*}

``````latex


\section*{Student Solution}

\subsection*{a)}

\[
S_{\text{en}} = S_f(T=70^\circ C) = 0{,}9549 \frac{\text{kJ}}{\text{kg K}}
\]

\[
\dot{S}_{\text{ev}} = \frac{58{,}86 \text{kW}}{293{,}15 \text{K}} + 0{,}3 \frac{\text{kg}}{\text{s}} \left(1{,}3379 \frac{\text{kJ}}{\text{kg K}} - 0{,}9549 \frac{\text{kJ}}{\text{kg K}}\right) = \frac{100 \text{kW}}{371{,}15 \text{K}}
\]

\[
= 0{,}096 \frac{\text{kW}}{\text{K}}
\]

\subsection*{d)}

\textbf{Energiebilanz halboffenes System}

\[
0 = \Delta \dot{m}_{12} \left[ h_{A1} - h_{A2} \right] - Q_{\text{aus},12}
\]

\[
\Rightarrow \Delta \dot{m}_{12} = \frac{Q_{\text{aus},12}}{h_{A1} - h_{A2}}
\]

\[
h_{A1} = h_f(70^\circ C) = 293{,}78 \frac{\text{kJ}}{\text{kg}}
\]

\[
h_{A2} = h_f(70^\circ C) + x_D \left( h_g(70^\circ C) - h_f(70^\circ C) \right)
\]

\[
= 293{,}78 \frac{\text{kJ}}{\text{kg}} + 0{,}005 \left( 2662{,}8 \frac{\text{kJ}}{\text{kg}} - 293{,}78 \frac{\text{kJ}}{\text{kg}} \right) = 304{,}65 \frac{\text{kJ}}{\text{kg}}
\]

\subsection*{e)}

\[
\Delta S_{12} = S_2 - S_1 = h_{A2} s_2 - h_{A1} s_1 = \Delta \dot{m}_{12} \Delta s_{12}
\]

\textbf{(halboffenes System)}

\[
S_1 = S_f(20^\circ C) = 0{,}2966 \frac{\text{kJ}}{\text{kg K}}
\]

\[
S_2 = S_f(70^\circ C) + x_D \left( S_g(70^\circ C) - S_f(70^\circ C) \right)
\]

\[
= 0{,}9549 \frac{\text{kJ}}{\text{kg K}} + 0{,}005 \left( 7{,}7353 \frac{\text{kJ}}{\text{kg K}} - 0{,}9549 \frac{\text{kJ}}{\text{kg K}} \right)
\]

\[
= 0{,}9889 \frac{\text{kJ}}{\text{kg K}}
\]

\[
\Delta S_{12} = 3600 \frac{\text{kg}}{\text{h}} \cdot (0{,}9889 - 0{,}2966) \frac{\text{kJ}}{\text{kg K}} = 2492{,}29 \frac{\text{kJ}}{\text{K}}
\]

``````latex


