
``````latex


\section*{Aufgabe 1}

\subsection*{a)}
\begin{align*}
    h_{\text{ein}} &= 292.98 \frac{\text{kJ}}{\text{kg}} \quad \text{(A-2)} \\
    h_{\text{aus}} &= 419.04 \frac{\text{kJ}}{\text{kg}} \quad \text{(1+2)}
\end{align*}

Energiebilanz:
\begin{align*}
    0 &= \dot{m} (h_{\text{ein}} - h_{\text{aus}}) + \dot{Q} - \dot{W} \quad \text{(0, isotherm)} \\
    \dot{Q} &= \dot{m} (h_{\text{aus}} - h_{\text{ein}}) = 37.818 \text{kW} \\
    Q_{\text{aus}} &= \dot{Q} - \dot{Q} = \underline{62.182 \text{kW}}
\end{align*}

\subsection*{b)}
\begin{align*}
    T_{\text{KF}} &= \frac{\int_{s_e}^{s_a} T dS}{s_a - s_e} \\
    \int T dS &= \Delta U \quad \text{Aus Tabelle (Differential, dm isobare)} \\
    s_{a} - s_{e} &= c_{if} \ln \left( \frac{T_e}{T_a} \right) \\
    T_{\text{KF}} &= \frac{T_e - T_a}{\ln \left( \frac{T_e}{T_a} \right)} = \underline{293.122 \text{K}}
\end{align*}

\subsection*{c)}
``````latex


\begin{itemize}
    \item[d)] $m_2 u_2 - m_4 u_4 = \Delta m h_{ein} + Q_{2 \rightarrow 4} = 0$
    
    \[
    (m_1 + \Delta m) u_2 - m_1 u_1 = \Delta m h_{ein}
    \]
    
    \[
    u_2 = 292.35 \frac{\text{kJ}}{\text{kg}} \quad \text{(A-2)}
    \]
    
    \[
    u_1 = 918.99 \frac{\text{kJ}}{\text{kg}} \quad (2566.5 \frac{\text{kJ}}{\text{kg}} - 918.99 \frac{\text{kJ}}{\text{kg}}) = 929.3778 \frac{\text{kJ}}{\text{kg}}
    \]
    
    \[
    h_{ein} = 83.06 \frac{\text{kJ}}{\text{kg}} \quad \text{(A-2)}
    \]
    
    \[
    \Delta m_{ein} = \frac{m_4 u_4 - m_2 u_2}{u_2 - h_{ein}} = \cancel{\frac{0}{0}} = 3756.889 \, \text{kg}
    \]
    
    \item[e)] $\Delta S = m_2 s_2 - m_1 s_1$
    
    \[
    s_1 = 1.3069 \frac{\text{kJ}}{\text{kg K}} + x_0 (7.3550 \frac{\text{kJ}}{\text{kg K}} - 1.3069 \frac{\text{kJ}}{\text{kg K}}) = 1.337 \frac{\text{kJ}}{\text{kg K}}
    \]
    
    \[
    s_2 = 0.359 \frac{\text{kJ}}{\text{kg K}} \quad \text{(A-2)}
    \]
    
    \[
    \Delta S = (m_1 + \Delta m_2) s_2 - m_1 s_1 = \cancel{\frac{0}{0}} = 1388.921 \frac{\text{kJ}}{\text{K}}
    \]
    
    \[
    \text{(Es könnte sein, dass die Lösung falsch ist.)}
    \]
    
\end{itemize}

``````latex


