
``````latex


\section*{Thermodynamik 1 HS23}

\subsection*{1.}
\textbf{Energiebilanz Reaktor:}

\begin{itemize}
    \item[a)] 
    \begin{equation}
    \frac{dE}{dt} = \dot{m} (h_{\text{ein}} - h_{\text{aus}}) + \dot{Q} - \dot{W}^{\text{o}}
    \end{equation}
    \begin{equation}
    \dot{Q} = \dot{m} (h_{\text{aus}} - h_{\text{ein}})
    \end{equation}
    \begin{equation}
    = 0
    \end{equation}
    \begin{equation}
    h_{\text{aus}} = 449.09 \frac{\text{kJ}}{\text{kg}} \quad h_{\text{ein}} = 292.88 \frac{\text{kJ}}{\text{kg}}
    \end{equation}
    \begin{equation}
    T = 293.12 \text{K}
    \end{equation}
    
    \item[b)] 
    \begin{equation}
    \frac{Q}{T} = \int_{s_1}^{s_2} T dS = \frac{h_2 - h_1 + V(p_2 - p_1)}{T} = C \left( \frac{T_2 - T_1}{T} \right)
    \end{equation}
    \begin{equation}
    = C \ln \left( \frac{T_2}{T_1} \right)
    \end{equation}
    \begin{equation}
    = c \ln \left( \frac{T_2}{T_1} \right)
    \end{equation}
    
    \item[c)] 
    \begin{equation}
    \frac{dS}{dt} = \sum \frac{\dot{Q}_i}{T} + S_{\text{erz}}
    \end{equation}
    \begin{equation}
    S_{\text{erz}} = - \frac{\dot{Q}}{T} = \frac{65 \text{kW}}{293.12 \text{K}} = 0.2218 \frac{\text{kJ}}{\text{K} \cdot \text{s}} = S_{\text{erz}}
    \end{equation}
    
    \item[d)] 
    \begin{equation}
    \frac{dE}{dt} = 0
    \end{equation}
    \begin{equation}
    Q = m_{\text{ges},1} \left( h_{\text{ges}}(70^\circ \text{C}) - h(100^\circ \text{C}) \right) + m_{12} \left( h(70^\circ \text{C}) - h(20^\circ \text{C}) \right)
    \end{equation}
    \begin{equation}
    m_{12} = - m_{\text{ges},1} \frac{h(70^\circ \text{C}) - h(100^\circ \text{C})}{h(70^\circ \text{C}) - h(20^\circ \text{C})} = - 8.755 \frac{\text{kJ}}{\text{kg}} \frac{292.88 \frac{\text{kJ}}{\text{kg}} - 419.09 \frac{\text{kJ}}{\text{kg}}}{292.88 \frac{\text{kJ}}{\text{kg}} - 83.96 \frac{\text{kJ}}{\text{kg}}} = 3970 \text{kg} = \Delta m_{12}
    \end{equation}
    
    \item[e)] 
    \textbf{halboffenes System:}
    \begin{equation}
    \Delta S = m_{s2} - m_{s1}
    \end{equation}
    \begin{equation}
    = \left( m_{\text{ges},1} + \Delta m_{12} \right) s(70^\circ \text{C}) - m_{\text{ges},1} s(100^\circ \text{C})
    \end{```latex


