
``````latex


\section*{Thermodynamik I - Sessionpr√ºfung HS 23}

\subsection*{1.a}
\begin{equation*}
\frac{dE}{dt} = \sum_i \dot{m}_i (h_i(t) + \frac{v_i^2(t)}{2} + p_i v_i(t)) - \sum_j \dot{m}_j (h_j(t) + \frac{v_j^2(t)}{2} + p_j v_j(t)) + \sum_j \dot{Q}_j - \sum_n \dot{W}_n
\end{equation*}

\begin{equation*}
0 = \dot{m}_{in} (h_e - h_a) + \dot{G}_z - \dot{Q}_{aus}
\end{equation*}

\begin{equation*}
\dot{Q}_{aus} = \dot{m}_{in} (h_e - h_a) - \dot{G}_z
\end{equation*}

\begin{equation*}
h_e = h_i (70^\circ C) \rightarrow AZ
\end{equation*}
\begin{equation*}
= 292.88 \frac{kJ}{kg}
\end{equation*}

\begin{equation*}
h_a = h_i (0^\circ C) \rightarrow AZ
\end{equation*}
\begin{equation*}
= 41.5 \frac{kJ}{kg}
\end{equation*}

\begin{equation*}
\dot{Q}_{aus} = 0.3 \frac{kg}{s} \cdot (292.88 \frac{kJ}{kg} - 41.5 \frac{kJ}{kg}) + 100 kW
\end{equation*}

\begin{equation*}
\dot{Q}_{aus} = 62.182 kW
\end{equation*}

\subsection*{b}
\begin{equation*}
T_{wir} = \frac{\int_{s_1}^{s_2} T \cdot ds}{s_2 - s_1}
\end{equation*}

\begin{equation*}
T_{wir, am} = 15^\circ C
\end{equation*}

\begin{equation*}
T_{wir, aus} = 25^\circ C
\end{equation*}

\begin{equation*}
s_2 = s (285.15 K) \rightarrow AZ
\end{equation*}
\begin{equation*}
= s (15^\circ C)
\end{equation*}
\begin{equation*}
= 0.2245 \frac{kJ}{kgK}
\end{equation*}

\begin{equation*}
s_2 = s (298 K) \rightarrow AZ
\end{equation*}
\begin{equation*}
= s (25^\circ C)
\end{equation*}
\begin{equation*}
= 0.36494 \frac{kJ}{kgK}
\end{equation*}

``````latex


\section*{1.C}
\begin{equation*}
0 = \dot{m} (se - sa) + \sum_{j} \dot{Q}_j + \dot{S}_{gen}
\end{equation*}

\begin{equation*}
\dot{S}_{gen} = - \dot{m} (se - sa) - \frac{\dot{Q}_{oven}}{T_{ref}}
\end{equation*}

\section*{d}
\begin{equation*}
(m_{gas} \cdot c_{m2}) \cdot (T_{outlet2}) = m_{gas} \cdot c_{m2} \cdot T_{outlet} + \dot{m}_{gas} \cdot T_{in}
\end{equation*}

\begin{equation*}
0 = m_{gas} \cdot c_{m2} \cdot (T_{outlet2} - T_{in}) = m_{gas} \cdot c_{m2} \cdot T_{outlet} - m_{gas} \cdot c_{m2} \cdot T_{outlet2}
\end{equation*}

\begin{equation*}
m_{gas} = \frac{\dot{m}_{gas} \cdot (T_{outlet2} - T_{outlet})}{T_{outlet} - T_{in}}
\end{equation*}

\begin{equation*}
= 57.55 \, \text{kg} \cdot \frac{400^\circ C - 70^\circ C}{80^\circ C - 20^\circ C}
\end{equation*}

\begin{equation*}
m_{gas} = 3453 \, \text{kg}
\end{equation*}

\section*{e}
\begin{equation*}
\dot{S}_{in} = (\dot{m}_{in} (S_{sa}) + \frac{\dot{Q}_{oven}}{T_{in}} - \frac{\dot{Q}_{oven}}{T_{oven}}) + S_{L}
\end{equation*}

``````latex


