
``````latex


\section*{Aufgabe 1}

\subsection*{a)}

\text{ges.:} \quad \dot{Q}_{aus}

\text{Stationärer Fließprozess:}
\[
0 = \dot{m} (h_e - h_a) + \frac{\omega_e^2 - \omega_a^2}{2} + g(z_e - z_a) + \sum \dot{Q}_j - \sum \dot{W}_k
\]

\[
\Rightarrow 0 = \dot{m} (h_e - h_a) + \sum \dot{Q}_j
\]

\[
0 = \dot{m} (h_e - h_a) + \dot{Q}_k - \dot{Q}_{aus}
\]

\[
\Rightarrow \dot{Q}_{aus} = \dot{m} (h_e - h_a) + \dot{Q}_k
\]

\[
= \dot{m} (22,98 \frac{\text{kJ}}{\text{kg}} - 419,04 \frac{\text{kJ}}{\text{kg}}) + \dot{Q}_k
\]

\[
= 0,3 \frac{\text{kg}}{\text{s}} (22,98 \frac{\text{kJ}}{\text{kg}} - 419,04 \frac{\text{kJ}}{\text{kg}}) + 100 \text{kW}
\]

\[
= 62,182 \frac{\text{kJ}}{\text{s}} = 62,182 \text{kW}
\]

\text{Werte für } h_e, h_a \text{ kommen aus Tabelle 42!}

\subsection*{b)}

\[
\overline{T} = \int_{e}^{a} T ds \cdot \frac{1}{s_a - s_e}
\]

\[
= \frac{T_{K, \text{aus}} \cdot s_{aus} - T_{K, \text{ein}} \cdot s_{ein}}{s_{aus} - s_{ein}}
\]

``````latex


\section*{c) (mit Lösungsgrößen: $\overline{T}_{KF} = 295 K$)}

\[
0 = \dot{m}(s_e - s_a) + \sum_i \left( \frac{\dot{Q}_i}{T_i} \right) + \dot{S}_{erz}
\]

\[
s_e = 0{,}9549 \frac{kJ}{kg \cdot K}
\]
\[
s_a = 1{,}3069 \frac{kJ}{kg \cdot K} \quad \text{Tabelle 4.2}
\]

\[
\Rightarrow \dot{S}_{erz} = \dot{m}(s_a - s_e) + \dot{Q}_{aus} \cdot \frac{1}{T_{KF}} = 
\]

\[
= 0{,}3 \frac{kg}{s} \left( 1{,}3069 \frac{kJ}{kg \cdot K} - 0{,}9549 \frac{kJ}{kg \cdot K} \right) + \frac{62{,}182 kW}{295 K}
\]

\[
= 0{,}316 \frac{kJ}{K \cdot s}
\]

\section*{d) Energieerhaltung:}

\[
\frac{dE}{dt} = \sum_i \dot{m}_i(t) h_i(t) + \dot{m}_e(t) h_e(t) + \sum_i \dot{Q}_i(t) - \sum_i \dot{W}_i(t)
\]

\[
Q_{R,12} = \Delta m_{12} (h_{20^\circ C} - h_{70^\circ C}) + m_{gu,1} (h_e - h_{40^\circ C})
\]

\subsection*{, wobei}

\[
h_{20^\circ C} = 83{,}96 \frac{kJ}{kg}
\]

\[
h_{70^\circ C} = 292{,}98 \frac{kJ}{kg}
\]

\[
h_e = \# (119{,}04 + x_d \cdot 0{,}2257) \frac{kJ}{kg}
\]

\[
= 430{,}325 \frac{kJ}{kg}
\]

\[
\text{Tabelle 4.2}
\]

``````latex


\section*{Fortsetzung 1c)}

\begin{equation*}
\Delta m_{12} = \frac{Q_{R,12} - m_{gen,1} (h_{e} - h_{20^{\circ}C})}{h_{20^{\circ}C} - h_{70^{\circ}C}}
\end{equation*}

\begin{equation*}
= 36,14 \, \text{kg}
\end{equation*}

\section*{e)}

\begin{equation*}
\frac{dS}{dt} = \sum_{i} \dot{m}_{i}(t) s_{i}(t) + \int_{6}^{a} \frac{\dot{Q}}{T_{a}} + \dot{S}_{\text{gen}}
\end{equation*}

\begin{equation*}
\Rightarrow \Delta S = \sum_{i} \Delta m_{i} \cdot s_{i} + \int_{G}^{a} \frac{Q}{T_{a}} + S_{\text{gen}}
\end{equation*}

\begin{equation*}
\Rightarrow \Delta S = \Delta m_{12} \left( s_{20^{\circ}C} - s_{70^{\circ}C} \right) + m_{\text{gen,1}} \left( s_{100^{\circ}C} - s_{70^{\circ}C} \right) + S_{\text{env}}
\end{equation*}

\begin{equation*}
\Rightarrow s_{20^{\circ}C} = 0,2966 \, \frac{\text{kJ}}{\text{kg} \cdot \text{K}}
\end{equation*}

\begin{equation*}
s_{70^{\circ}C} = 0,8549 \, \frac{\text{kJ}}{\text{kg} \cdot \text{K}}
\end{equation*}

\begin{equation*}
s_{100^{\circ}C} = \left( 1,3069 + x_{i} \left( 7,3549 - 1,3069 \right) \right) \frac{\text{kJ}}{\text{kg} \cdot \text{K}}
\end{equation*}

\begin{equation*}
= 1,33714
\end{equation*}

\begin{equation*}
S_{\text{env}} = 0 \quad (\text{adiabat})
\end{equation*}

\section*{H2S: Tabelle A-2}

``````latex


