
``````latex


\section*{Aufgabe 1}

\subsection*{a)}
\begin{align*}
h &= h_f + x_0 \cdot (h_g - h_f) = h_f + x_0 \cdot h_{fg} = 419.44 \, \text{kJ/kg} + 0.005 \times 2277.0 \, \text{kJ/kg} \\
&= 430.325 \, \text{kJ/kg}
\end{align*}

\[
\dot{Q}_{\text{aus}} = \dot{m}_{\text{aus}} \, h = 0.3 \, \text{kg/s} \cdot 430.325 \, \text{kJ/kg} = 129.1 \, \text{kW}
\]

\subsection*{b)}
\[
C = \text{Const.} \Rightarrow S(T = 298.15 \, \text{K}) - S(T = 298.15 \, \text{K}) = \int_{T_1}^{T_2} \frac{1}{T} \, dT = C \cdot \ln \left( \frac{T_2}{T_1} \right)
\]

\[
\overline{T}_{\text{KF}} = \frac{\int_{S_a}^{S_e} T \, ds}{S_a - S_e} = \frac{T_{aSa} - T_{eSe}}{C \cdot \ln \left( \frac{298.15 \, \text{K}}{298.15 \, \text{K}} \right)} = \left[ \ldots \right] \approx 298 \, \text{K}
\]

\subsection*{c)}
\[
\dot{S}_{\text{ext}}(t) = -\dot{m} \left[ S_e - S_a \right] - \frac{\dot{Q}_{\text{aus}}}{\overline{T}_{\text{KF}}}
\]

\[
= -0.3 \, \text{kg/s} \cdot \left( C \cdot \ln \left( \frac{T_e}{T_p} \right) \right) - \frac{65 \, \text{kW}}{298 \, \text{K}}
\]

\[
=
\]

\subsection*{d)}
\begin{align*}
U_i &= (1 - x_0) \, m_{\text{ges},i} \, h_f + x_0 \, m_{\text{ges},i} \, h_g + \int \dot{Q} \, dt - \int \dot{W} \, dt \\
&= (1 - 0.005) \cdot 375 \, \text{kg} \cdot
\end{align*}

``````latex


