
``````latex


1. a) \quad 0 = \dot{m}_{ein} \left( h_{ein} \right) - \dot{m}_{aus} h_{aus} + \dot{Q} - \dot{W} + \dot{Q}_R

\[
h_{ein} = h_f \left( 70^\circ C \right) = 252.38 \frac{kJ}{kg}
\]

\[
h_{aus} = h_f \left( 100^\circ C \right) = 419.04 \frac{kJ}{kg}
\]

\[
\dot{Q}_{aus} = \dot{m}_{aus} h_{aus} - \dot{m}_{ein} h_{ein} = \frac{\dot{Q}_R}{\dot{m}_{ein} \left( h_{aus} - h_{ein} \right)} - \dot{Q}_R
\]

\[
\dot{Q}_{aus} = -62.18 \, kW
\]

b) \quad \overline{T} = \frac{\int_{s_A}^{s_E} T ds}{s_A - s_E}

\[
dH = T ds + v dp \quad \text{weil isobar}
\]

\[
\overline{T} = \frac{h_2 - h_1}{s_2 - s_1} = \frac{\Delta \left( T_2 - T_1 \right) + v \left( p_2 - p_1 \right)}{\ln \left( \frac{T_2}{T_1} \right)}
\]

\[
\overline{T} = \frac{T_2 - T_1}{\ln \left( \frac{T_2}{T_1} \right)} = 233.12 \, K
\]

c) \quad 0 = \frac{\dot{Q}_{aus}}{\overline{T}} - \frac{\dot{Q}_{aus}}{T} + \dot{S}_{irr,2}

\[
\dot{S}_{irr,2} = \frac{\dot{Q}_{aus}}{\overline{T}} \neq \frac{\dot{Q}_{aus}}{T_{ex}} = 0.045 \, \frac{kW}{K}
\]

``````latex

d) \quad m_2 u_2 - m_1 u_1 = \Delta m_2 (h_{ein}) + \dot{Q}_{zu} \quad \text{Energie Austausch gleich}

\[
\Delta m_2 = m_2 u_2 - m_1 u_1 - \dot{Q}_{zu}
\]

\[
u_1 = u_f (100^\circ C) + x_D (u_g (100^\circ C) - u_f (100^\circ C)) = 429.38 \frac{kJ}{kg}
\]

\[
h_{ein} (20^\circ C) = u_f (20^\circ C) = 83.35 \frac{kJ}{kg}
\]

\[
u_2 (70^\circ C) = u_f (70^\circ C) = 232.35 \frac{kJ}{kg}
\]

\[
\Delta m_2 = m_2 - m_1
\]

\[
m_2 u_2 - m_1 u_1 = (m_2 - m_1) h_{ein} + \dot{Q}_{zu}
\]

\[
m_2 = \frac{m_1 u_1 - \dot{Q}_{zu}}{u_2 - h_{ein}}
\]

\[
m_2 = 5511.72 \, \text{kg}
\]

\[
\Delta m_2 = \frac{40.8 + 8.2}{2} = 3576.72 \, \text{kg}
\]

e) \quad m_2 s_2 - m_1 s_1 = \Delta S_{m_2}

\[
s_2 = s_f (70^\circ C) = 0.954 \frac{kJ}{kgK}
\]

\[
s_1 = s_f (100^\circ C) + x_D (s_g (100^\circ C) - s_f (100^\circ C)) = 1.33714 \frac{kJ}{kgK}
\]

\[
\Delta S = 1387.5 \frac{kJ}{kgK}
\]

``````latex


