
``````latex


1) \quad \dot{Q}_{ges} = \dot{Q}_{aus}

\[
0 = \dot{m}_{in} (h_{ein} - h_{aus}) + \dot{Q}_{aus} - \dot{W}^{\prime \prime}
\]

\[
0 = \dot{m} (h_{2} - h_{1}) + \dot{Q}_{aus}
\]

\[
0 = \dot{m} (h_{p}(T_{e}) - h(100^{\circ})) + \dot{Q}_{aus}
\]

\[
\dot{Q}_{aus} = 0.2 \frac{\text{kJ}}{\text{s}} (252.58 \frac{\text{kJ}}{\text{kg}} - 436.34 \frac{\text{kJ}}{\text{kg}})
\]

\[
\dot{Q}_{aus} = -41.21 \frac{\text{kJ}}{\text{W}}
\]

\[
h_{p}(T_{e}) = 252.58 \frac{\text{kJ}}{\text{kg}}
\]

\[
h(100^{\circ} \text{C}) = h_{fg} \cdot 1.01 \frac{\text{kJ}}{\text{kg}} + 0.005 (2257.0 \frac{\text{kJ}}{\text{kg}})
\]

\[
= 436.34 \frac{\text{kJ}}{\text{kg}}
\]

b) \quad \dot{s} = \frac{\dot{Q}}{T_{KF}}

\[
\bar{T} = \frac{\int_{s_{a}}^{s_{e}} T ds}{s_{a} - s_{e}}
\]

\[
\text{ideale Fl√ºssigkeit} \Rightarrow ds = \frac{c^{\text{fl}}}{T} dT
\]

\[
\Rightarrow T ds = c^{\text{fl}} dT \Rightarrow \int T ds = c^{\text{fl}} (T_{aus} - T_{ein})
\]

\[
s_{a} - s_{e} = c^{\text{fl}} \ln \left( \frac{T_{aus}}{T_{ein}} \right)
\]

\[
\bar{T} = \frac{T_{aus} - T_{ein}}{\ln \left( \frac{T_{aus}}{T_{ein}} \right)} = \frac{(295.15 - 258.15) \text{K}}{\ln \left( \frac{295.15}{258.15} \right)} \approx 9.66 \text{K}
\]

c) \quad 0 = \frac{\dot{Q}_{i}}{T_{KF}} + \dot{s}_{ez} \Rightarrow \dot{s}_{ez} = \frac{\dot{Q}_{aus}}{T_{KF}} = \frac{41.21 \frac{\text{kJ}}{\text{s}}}{295 \text{K}} = 0.720 \frac{\text{kJ}}{\text{K}}

d)

``````latex


