**Determine \( \dot{Q}_{\text{out}} \):**  

The problem begins with the energy balance for a steady-state flow process:  
\[
0 = \dot{m}_{\text{KF}} \left( h_{\text{out}} - h_{\text{in}} \right) + \sum \dot{Q}_{\text{in}} - \sum \dot{W}_{\text{in}}
\]  
Here, it is noted that \( p_{\text{KF,out}} = p_{\text{KF,in}} \), and \( \Delta \dot{W}_{\text{in}} = 0 \), simplifying the equation.  

The energy balance reduces to:  
\[
0 = \dot{m}_{\text{KF}} \left( h_{\text{out}} - h_{\text{in}} \right) + \dot{Q}_{\text{out}}
\]  

Rearranging for \( \dot{Q}_{\text{out}} \):  
\[
\dot{Q}_{\text{out}} = \dot{m}_{\text{KF}} \left( h_{\text{out}} - h_{\text{in}} \right)
\]  

The enthalpy difference \( h_{\text{out}} - h_{\text{in}} \) is expressed as:  
\[
h_{\text{out}} - h_{\text{in}} = \int_{T_{\text{in}}}^{T_{\text{out}}} c_p \, dT + v \cdot (p_2 - p_1)
\]  

It is noted that \( p_2 - p_1 = 0 \) because there is no pressure loss (\( p_{\text{KF,out}} = p_{\text{KF,in}} \)).  

Thus, the enthalpy difference simplifies to:  
\[
h_{\text{out}} - h_{\text{in}} = c_p \left( T_{\text{out}} - T_{\text{in}} \right)
\]  

Substituting the temperature difference:  
\[
h_{\text{out}} - h_{\text{in}} = c_p \cdot (10 \, \text{K})
\]  

The calculation for \( \dot{Q}_{\text{out}} \) is left incomplete.