The entropy change \( \Delta S \) is calculated using the formula:  
\[
\Delta S = S_2 \cdot m_2 - m_1 \cdot S_1
\]  
where \( x = 0.005 \).  

The entropy \( S_1 \) is given as:  
\[
S_1 = x \cdot S_g + (1 - x) \cdot S_f = 1.33714 \, \frac{\text{kJ}}{\text{kg路K}}
\]  
Here, \( S_g = 7.5549 \, \frac{\text{kJ}}{\text{kg路K}} \) (from Table A-2) and \( S_f = 1.3369 \, \frac{\text{kJ}}{\text{kg路K}} \).  

For \( S_2 \), at \( T = 70^\circ\text{C} \) and \( x_2 = 0 \):  
\[
S_2 = x \cdot S_g + (1 - x) \cdot S_f(70^\circ\text{C})
\]  
where \( S_f(70^\circ\text{C}) = 0.9549 \, \frac{\text{kJ}}{\text{kg路K}} \) (from Table A-2).  

The total mass \( m_2 \) is calculated as:  
\[
m_2 = 5755 \, \text{kg} + 3600 \, \text{kg} = 9355 \, \text{kg}
\]  

Finally, the entropy change is:  
\[
\Delta S = 1235.83 \, \text{kJ}
\]  

This value is underlined in the solution.