**Entropy change from state 1 to state 2:**  
The entropy change is given by:  
\[
\Delta S = m_2 s_2 - m_1 s_1 - \left( \Delta m_{12} s_{\text{in}} \right) - \frac{Q_{\text{out,12}}}{T} + \dot{S}_{\text{gen}}
\]  

**Specific entropy calculations:**  
\[
s_2 = s_f(70^\circ\text{C}) + x_0 \cdot \left( s_g(70^\circ\text{C}) - s_f(70^\circ\text{C}) \right)
\]  
\[
s_1 = s_f(100^\circ\text{C}) + x_0 \cdot \left( s_g(100^\circ\text{C}) - s_f(100^\circ\text{C}) \right)
\]  

**Mass relationship:**  
\[
m_2 = m_1 + \Delta m_{12}
\]