The entropy change is calculated as:  
\[
m_2 s_2 - m_1 s_1 = \Delta m_{12} s_{\text{in}} + \frac{Q}{T} - S_{\text{out}}
\]  

For state 2:  
\[
s_2 = s_l(70^\circ\text{C}) = 0.3548 \, \frac{\text{kJ}}{\text{kg·K}}
\]  
For state 1:  
\[
s_1 = s_l(100^\circ\text{C}) + x_1 \cdot \left( s_g(100^\circ\text{C}) - s_l(100^\circ\text{C}) \right) = 1.35741 \, \frac{\text{kJ}}{\text{kg·K}}
\]  
For the incoming mass:  
\[
s_{\text{in}} = s_l(20^\circ\text{C}) = 0.2866 \, \frac{\text{kJ}}{\text{kg·K}}
\]  

Entropy change:  
\[
\Delta S_{12} = 162.8 \, \frac{\text{kJ}}{\text{K}}
\]