The equation for entropy generation is written as:  
\[
0 = \dot{m} \left( s_0 - s_6 \right) + \frac{\dot{Q}_B}{T_B} + \dot{S}_{\text{gen}}
\]  

The entropy change \( s_{\text{gen}} \) is calculated using the following expression:  
\[
s_{\text{gen}} = s_6 - s_0 - \frac{q_B}{T_B} = c_p \ln \left( \frac{T_6}{T_0} \right) - \frac{q_B}{T_B}
\]  

The numerical result is:  
\[
s_{\text{gen}} = -625.73 \, \frac{\text{J}}{\text{kgÂ·K}}
\]  

A note is added indicating that the sign should be positive.  

The exergy destruction is calculated as:  
\[
ex_{\text{dest}} = s_{\text{gen}} \cdot T_0 = -152.144 \, \frac{\text{kJ}}{\text{kg}}
\]  

This result is underlined for emphasis.