The mass-specific increase in flow exergy is calculated as:  
\[
ex_{\text{flow},6} = h_6 - h_0 - T_0 (s_6 - s_0) + \frac{1}{2} w_6^2
\]  
\[
ex_{\text{flow},0} = h_0 - h_0 - T_0 (s_0 - s_0) + \frac{1}{2} w_0^2
\]  
The difference is:  
\[
\Delta ex_{\text{flow},06} = ex_{\text{flow},6} - ex_{\text{flow},0} = h_6 - h_0 - T_0 (s_6 - s_0) + \frac{1}{2} w_6^2 - \frac{1}{2} w_0^2
\]  
Using \( h_6 - h_0 = c_p (T_6 - T_0) \) and \( s_6 - s_0 = c_p \ln \left( \frac{T_6}{T_0} \right) \), the expression becomes:  
\[
\Delta ex_{\text{flow},06} = c_p (T_6 - T_0) - T_0 \left( c_p \ln \left( \frac{T_6}{T_0} \right) \right) + \frac{w_6^2 - w_0^2}{2}
\]  
Substituting the values:  
\[
\Delta ex_{\text{flow},06} = 120.8 \, \frac{\text{kJ}}{\text{kg}}
\]