The energy balance equation is written as:  
\[
0 = \dot{m}_{\text{aus}} \left[ h_{\text{ein}} - h_{\text{aus}} \right] + \dot{Q}_{\text{aus}}
\]  

The heat flow is expressed as:  
\[
\dot{Q} = \dot{m}_{\text{aus}} \left[ h_{\text{aus}} + h_{\text{ein}} \right]
\]  

Using values from Table A-2:  
\[
h_{\text{ein}} = 292.98 \, \frac{\text{kJ}}{\text{kg}}, \quad h_{\text{aus}} = 449.01 \, \frac{\text{kJ}}{\text{kg}}
\]  

Substituting into the equation:  
\[
\dot{Q} = \dot{m} \left[ 449.01 + 292.98 \right]
\]  
\[
\dot{Q} = -371.87 \, \text{kJ}
\]  

---

The energy balance equation is written as:  
\[
\Delta E = m_2 u_2 - m_1 u_1 = \Delta m_{12} \left[ h_1 \right] + Q_{\text{out}}
\]  

The change in mass flow is expressed as:  
\[
\Delta m_{12} = m_2 u_2 - m_1 u_1 - Q_{\text{out}}
\]