The energy balance for the ice-water mixture is expressed as:  
\[
U_{2,\text{EW}} - U_{1,\text{EW}} = Q_{12}
\]  
Expanding the equation:  
\[
Q_{12} = m_{\text{EW}} \left( x_2 u_{\text{fus}} + (1 - x_2) u_{\text{liq}} \right) - m_{\text{EW}} \left( x_1 u_{\text{fus}} + (1 - x_1) u_{\text{liq}} \right)
\]  
Simplifying further:  
\[
Q_{12} = x_1 \left( u_{\text{fus}} - u_{\text{liq}} \right) + x_2 \left( u_{\text{liq}} - u_{\text{fus}} \right)
\]  
Crossed-out terms are ignored. The equation simplifies to:  
\[
Q_{12} = m_{\text{EW}} \left( u_{\text{liq}} - u_{\text{fus}} \right) + x_1 u_{\text{liq}}
\]  
Final state temperature is noted as:  
\[
T = 0^\circ\text{C}
\]  

No diagrams or figures are present on this page.

The equation for energy balance is written as:  
\[
U_{2,\text{EW}} - U_{1,\text{EW}} = -Q_{12} = m_{\text{EW}} \left( x_2 u_L + (1 - x_2) u_S \right) - m_{\text{EW}} \left( x_1 u_L + (1 - x_1) u_S \right)
\]  

Rearranging terms:  
\[
-\frac{Q_{12}}{m_{\text{EW}}} = x_2 (u_L - u_S) + u_S - x_1 (u_L - u_S) - u_S
\]  
\[
= (x_2 - x_1)(u_L - u_S)
\]  

Solving for \( x_2 \):  
\[
x_2 = -\frac{Q_{12}}{m_{\text{EW}} (u_L - u_S)} + x_1
\]  

Substituting values:  
\[
x_2 = 0.574
\]  

No diagrams or additional figures are present on the page.