The differential change in enthalpy \( dH \) is expressed as:  
\[
dH = T \, dS + V \, dp \quad \text{(since \( dp \) does not change, this simplifies to)}
\]  
\[
dH = T \, dS
\]  
Integrating \( dH \), we have:  
\[
\int dH = \int T \, dS
\]  
The enthalpy change is calculated as:  
\[
\bar{T} = \frac{\dot{Q}_h}{S_{\text{aus}} - S_{\text{ein}}} = c_p \ln \left( \frac{T_{\text{aus}}^{\text{KF}}}{T_{\text{ein}}^{\text{KF}}} \right)
\]  
Substituting values:  
\[
\ln \left( \frac{T_{\text{aus}}^{\text{KF}}}{T_{\text{ein}}^{\text{KF}}} \right) = \ln \left( \frac{298.15}{288.15} \right) = 2.93 \, \text{kJ}
\]

---