The entropy change is calculated using the equation:  
\[
\Delta S = m_2 s_2 - m_1 s_1
\]  

The following relationships and values are used:  
\[
m_2 = m_1 + \Delta m_{12} = 9255 \, \text{kg}
\]  
\[
m_1 = 5755 \, \text{kg}
\]  
\[
s_1 = s_f(100^\circ\text{C}) = 1.3069 \, \frac{\text{kJ}}{\text{kg·K}}
\]  
\[
s_2 = s_f(70^\circ\text{C}) = 0.9549 \, \frac{\text{kJ}}{\text{kg·K}}
\]  
These values are taken from Table A2.  

Substituting into the entropy change equation:  
\[
\Delta S = 9255 \cdot 0.9549 - 5755 \cdot 1.3069
\]  
\[
\Delta S \approx 1376.39 \, \frac{\text{kJ}}{\text{K}}
\]