The entropy balance equation is written as:  
\[
\frac{dS}{dt} = \dot{m}(s_1 - s_2) + \frac{\dot{Q}}{T} + \dot{S}_{\text{gen}}
\]  

The entropy change (\( \Delta S_{12} \)) is expressed as:  
\[
\Delta S_{12} = \Delta m_{12}(s_1 - s_2) + \frac{\dot{Q}}{T} + \dot{S}_{\text{gen}}
\]  

Simplifying further:  
\[
\Delta S_{12} = \Delta m_{12}(s_1 - s_2)
\]  

The entropy difference (\( s_1 - s_2 \)) is calculated as:  
\[
s_1 - s_2 = \int_{T_2}^{T_1} \frac{C}{T} \, dT = C \ln\left(\frac{T_1}{T_2}\right)
\]