The steady-state entropy balance is expressed as:  
\[
0 = \dot{m} (s_e - s_a) + \frac{\dot{Q}_{\text{aus}}}{T_{\text{KF}}} + \dot{S}_{\text{erz}}
\]  
Rearranging for \( \dot{S}_{\text{erz}} \):  
\[
\dot{S}_{\text{erz}} = \dot{m} (s_a - s_e) - \frac{\dot{Q}_{\text{aus}}}{T_{\text{KF}}}
\]  

The entropy difference \( s_a - s_e \) is calculated as:  
\[
s_a - s_e = \int_{T_{\text{in}}}^{T_{\text{out}}} c \frac{1}{T} \, dT = c \ln \left( \frac{T_{\text{out}}}{T_{\text{in}}} \right)
\]  
Substituting the given temperatures:  
\[
s_a - s_e = c \ln \left( \frac{298.15}{288.15} \right)
\]