The mass change \(\Delta m_{12}\) is calculated using the energy balance:  
\[
m_2 u_2 - m_1 u_1 = \Delta m_{12}(h_m) + \dot{Q}_{\text{out},12}
\]  
Rearranging for \( m_2 \):  
\[
m_2 = m_1 + \Delta m_{12}
\]  

No further numerical values are provided for calculation.

The energy balance equation is written as:  
\[
m_1 u_1 + m_2 u_2 - \Delta m_{12} h_i = Q_{\text{out},12} + Q_{\text{in},12}
\]  
Rearranging for \( \Delta m_{12} \):  
\[
\Delta m_{12} (h_2 - h_i) = Q_{\text{out},12} + m_1 u_1 - m_2 u_2
\]  
\[
\Delta m_{12} = \frac{Q_{\text{out},12} + m_1 u_1 - m_2 u_2}{h_2 - h_i}
\]  
Substituting values:  
\[
\Delta m_{12} = \frac{35 \, \text{MJ} + 5755 \, \text{kg} \cdot 0.5549 \, \frac{\text{kJ}}{\text{kg}} - 262.95 \, \frac{\text{kJ}}{\text{kg}}}{8.96 \, \frac{\text{kJ}}{\text{kg}} - 0.005 \cdot (2506.5 - 8.96) \, \frac{\text{kJ}}{\text{kg}}}
\]  
Result:  
\[
\Delta m_{12} = -3982.82 \, \text{kg}
\]  

---