The entropy change \( \Delta S \) is calculated using:  
\[
\Delta S = \Sigma m_2 s_2 - m_1 s_1
\]  

For \( m_2 = 5755 \, \text{kg} \):  
\[
s_1 = s_f + x (s_{fg}) \quad \text{at } 100^\circ\text{C} \quad \text{(from Table A-2)}
\]  
\[
s_1 = 1.337 \, \text{kJ/kg·K}
\]  

For \( s_2 \):  
\[
s_2 = s_f \quad \text{at } 70^\circ\text{C} \quad \text{(from Table A-2)}
\]  
\[
s_2 = 0.9549 \, \text{kJ/kg·K}
\]  

Substituting into the entropy equation:  
\[
\Delta S = m_2 s_2 - m_1 s_1
\]  
\[
\Delta S = 5755 \cdot 0.9549 - 5755 \cdot 1.337
\]  
\[
\Delta S = 1238.6 \, \text{kJ/K}
\]