The goal is to calculate \( \dot{Q}_{\text{out}} \).  

The energy balance equation is written as:  
\[
Q = \dot{m} (h_{\text{in}} - h_{\text{out}}) + \dot{Q}_R + \dot{Q}_{\text{out}}
\]  
Rearranging for \( \dot{Q}_{\text{out}} \):  
\[
-\dot{Q}_{\text{out}} = \dot{m} (h_{\text{in}} - h_{\text{out}}) + \dot{Q}_R
\]  
\[
\dot{Q}_{\text{out}} = \dot{m} (h_{\text{out}} - h_{\text{in}}) - \dot{Q}_R
\]  

Using the given values:  
\[
h_{\text{in}} = 292.98 \, \frac{\text{kJ}}{\text{kg}}, \quad h_{\text{out}} = 419.04 \, \frac{\text{kJ}}{\text{kg}}
\]  
\[
\dot{m} = 0.3 \, \frac{\text{kg}}{\text{s}}, \quad \dot{Q}_R = 100 \, \frac{\text{kJ}}{\text{s}}
\]  

Substituting:  
\[
\dot{Q}_{\text{out}} = 0.3 \, \frac{\text{kg}}{\text{s}} (419.04 \, \frac{\text{kJ}}{\text{kg}} - 292.98 \, \frac{\text{kJ}}{\text{kg}}) - 100 \, \frac{\text{kJ}}{\text{s}}
\]  
\[
\dot{Q}_{\text{out}} = -62.16 \, \frac{\text{kJ}}{\text{s}}
\]  

The mass flow rate removes \( \dot{Q}_{\text{out}} = 62.16 \, \frac{\text{kJ}}{\text{s}} \).  

---