The entropy change \( \Delta S \) is calculated as follows:  

\[
\Delta S = m_2 s_2 - m_1 s_1
\]

For \( s_1 \):  
\[
s_1 = s_f(100^\circ\text{C}) + x \cdot \left( s_g(100^\circ\text{C}) - s_f(100^\circ\text{C}) \right)
\]
\[
= 7.3605 \, \frac{\text{kJ}}{\text{kg·K}} + 0.005 \cdot \left( 7.3754 - 7.3605 \right) \, \frac{\text{kJ}}{\text{kg·K}}
\]
\[
= 7.337 \, \frac{\text{kJ}}{\text{kg·K}}
\]

For \( s_2 \):  
\[
s_2 = s_f(70^\circ\text{C}) + x \cdot \left( s_g(70^\circ\text{C}) - s_f(70^\circ\text{C}) \right)
\]
\[
= 0.9589 \, \frac{\text{kJ}}{\text{kg·K}} + 0.005 \cdot \left( 2.7851 - 0.9589 \right) \, \frac{\text{kJ}}{\text{kg·K}}
\]
\[
= 0.9683 \, \frac{\text{kJ}}{\text{kg·K}}
\]

Finally, \( \Delta S \) is computed:  
\[
\Delta S = \left( 5755 \, \text{kg} - 3600 \, \text{kg} \right) \cdot 0.9589 \, \frac{\text{kJ}}{\text{kg·K}} - 52.85 \, \text{kg} \cdot 7.337 \, \frac{\text{kJ}}{\text{kg·K}}
\]
\[
= 5563.4 \, \text{kW}
\]  

No diagrams or figures are present on this page.