Using the energy balance equation:  
\[
m_2 u_2 - m_1 u_1 = \Delta m h + Q - W_0
\]  
Given:  
\[
m_2 = 5755 \, \text{kg} - \Delta m
\]  
\[
m_1 = 5755 \, \text{kg}
\]  

For \( u_1 \) at \( 100^\circ\text{C} \):  
\[
u_1 = u_f(100^\circ\text{C}) + x(u_{fg}(100^\circ\text{C}))
\]  
\[
u_1 = 429.38 \, \frac{\text{kJ}}{\text{kg}} + 0.005 \left(2506.5 \, \frac{\text{kJ}}{\text{kg}}\right)
\]  
\[
u_1 = 429.38 \, \frac{\text{kJ}}{\text{kg}} + 12.53 \, \frac{\text{kJ}}{\text{kg}}
\]  
\[
u_1 = 441.91 \, \frac{\text{kJ}}{\text{kg}}
\]  

For \( u_2 \) at \( 70^\circ\text{C} \):  
\[
u_2 = u_f(70^\circ\text{C}) + x(u_{fg}(70^\circ\text{C}))
\]  
\[
u_2 = 303.83 \, \frac{\text{kJ}}{\text{kg}}
\]  

For \( h \) at \( 20^\circ\text{C} \):  
\[
h = h_f(20^\circ\text{C})
\]  
\[
h = 83.96 \, \frac{\text{kJ}}{\text{kg}}
\]  

Substituting into the energy balance equation:  
\[
(5755 \, \text{kg} - \Delta m) \cdot 303.83 \, \frac{\text{kJ}}{\text{kg}} - 5755 \, \text{kg} \cdot 429.38 \, \frac{\text{kJ}}{\text{kg}} = \Delta m \cdot 83.96 \, \frac{\text{kJ}}{\text{kg}} - 35 \, \text{MJ}
\]  

Solving for \( \Delta m \):  
\[
\Delta m = 1.7723 \, \text{kg}
\]  
\[
\Delta m = 1773 \, \text{kg}
\]