The specific flow exergy at state 6, \( e_{x,\text{sir},6} \), is determined using the following equation:  
\[
e_{x,\text{sir},6} = h_6 - h_0 - T_0 \cdot (s_6 - s_0) + \text{KE} + \text{PE}
\]  
Here, \( h_6 \) is given as \( h_6 = h(T_6, p_6 = 0.191 \, \text{bar}) \), and \( T_6 = 340 \, \text{K} \).  

The equation expands to:  
\[
e_{x,\text{sir},6} = c_p^{\text{ig}} \cdot (T_6 - T_0) - T_0 \cdot \left( c_p \cdot \ln\left(\frac{T_6}{T_0}\right) - R \cdot \ln\left(\frac{p_6}{p_0}\right) \right) + \text{KE}
\]  
Where \( R = c_p - c_v = \frac{c_p}{\kappa} \).  

Substituting values:  
\[
e_{x,\text{sir},6} = 97.43 \, \frac{\text{kJ}}{\text{kg}} - 82.01 \, \frac{\text{kJ}}{\text{kg}} + \frac{w_6^2}{2} \cdot \frac{1}{\text{kg}}
\]  
\[
e_{x,\text{sir},6} = 125.47 \, \frac{\text{kJ}}{\text{kg}}
\]  

The specific flow exergy at state 0, \( e_{x,\text{sir},0} \), is calculated as:  
\[
e_{x,\text{sir},0} = h_0 - h_0 - T_0 \cdot (s_0 - s_0) + \text{KE} + \text{PE}
\]  
This simplifies to:  
\[
e_{x,\text{sir},0} = \text{KE} = \frac{w_0^2}{2} = 80 \, \frac{\text{kJ}}{\text{kg}}
\]  

The change in specific flow exergy, \( \Delta e_{x,\text{sir}} \), is:  
\[
\Delta e_{x,\text{sir}} = e_{x,\text{sir},6} - e_{x,\text{sir},0}
\]  
\[
\Delta e_{x,\text{sir}} = 105.47 \, \frac{\text{kJ}}{\text{kg}}
\]  

---