The entropy destruction \( \Delta ex_{st} \) is calculated using the following equation:  
\[
0 = \dot{m} (h_e - h_a - T_0 (s_e - s_a)) + \frac{w_e^2}{2} - \frac{w_a^2}{2} = -\Delta ex_{st}
\]  
Given values:  
\[
T_0 = 243.15 \, \text{K}, \quad T_6 = 340 \, \text{K}
\]  
The enthalpy difference \( h_0 - h_e \) is expressed as:  
\[
h_0 - h_e = c_p (T_0 - T_6) = 1.006 \, \frac{\text{kJ}}{\text{kg·K}} \cdot (96.85 \, \text{K}) = 97.43 \, \frac{\text{kJ}}{\text{kg}}
\]  
The entropy difference \( s_e - s_d \) is expressed as:  
\[
s_e - s_d = c_p \ln \left( \frac{T_0}{T_6} \right) - R \ln \left( \frac{p_0}{p_6} \right)
\]  
Simplifying:  
\[
s_e - s_d = c_p \ln \left( \frac{T_0}{T_6} \right) = 1.006 \, \frac{\text{kJ}}{\text{kg·K}} \cdot \ln \left( \frac{243.15}{340} \right) = -0.933 \, \frac{\text{kJ}}{\text{kg·K}}
\]  
Finally, the entropy destruction is calculated as:  
\[
\Delta ex_{st} = -\dot{m} \left[ c_p (h_0 - h_e) - T_0 \left( c_p \ln \left( \frac{T_0}{T_6} \right) + \frac{w_e^2}{2} - \frac{w_a^2}{2} \right) \right]
\]  

---