The internal energy \( u \) is expressed as:  

\[
u = u_f + x \cdot (u_s - u_f)
\]

Rearranging to solve for \( x_2 \):  

\[
\frac{u - u_f}{u_s - u_f} = x_2
\]

Given values:  

\[
u_s = -333.442 \, \frac{\text{kJ}}{\text{kg}}, \quad u_f = -0.033 \, \frac{\text{kJ}}{\text{kg}}
\]

Using the energy balance:  

\[
\Delta U = m \cdot (u_2 - u_1)
\]

Where \( u_2 = u \):  

\[
u_2 = u_f + x_i \cdot (u_s - u_f)
\]

Substituting:  

\[
u_1 = u(0^\circ\text{C})
\]

\[
u_1 = -0.033 + 0.6 \cdot (-333.458 + 0.033)
\]

\[
u_1 = -200.0828 \, \frac{\text{kJ}}{\text{kg}}
\]

Calculating \( \Delta U \):  

\[
\Delta U = -200.0828 \, \frac{\text{kJ}}{\text{kg}} - (-185.0828 \, \frac{\text{kJ}}{\text{kg}})
\]

\[
\Delta U = -185.0828 \, \frac{\text{kJ}}{\text{kg}}
\]

Solving for \( x_2 \):  

\[
x_2 = \frac{-185.0828 \, \frac{\text{kJ}}{\text{kg}} + 0.033 \, \frac{\text{kJ}}{\text{kg}}}{-333.442 \, \frac{\text{kJ}}{\text{kg}} + 0.033 \, \frac{\text{kJ}}{\text{kg}}}
\]

\[
x_2 = 0.555
\]