Entropy change:  
\[
\Delta S = m_2 \cdot s_2 - m_1 \cdot s_1
\]  
Substituting:  
\[
\Delta S = (m_1 + \Delta m_{12}) \cdot s_2 - m_1 \cdot s_1
\]  

Final result:  
\[
\Delta S_{12} = 1387.22 \, \frac{\text{kJ}}{\text{K}}
\]  

From Table A2:  
\[
s_2 = s_f(70^\circ\text{C}) = 0.954 \, \frac{\text{kJ}}{\text{kg路K}}
\]  
\[
s_1 = s_f(100^\circ\text{C}) + x_D \cdot (s_g(100^\circ\text{C}) - s_f(100^\circ\text{C}))
\]  
\[
s_1 = 1.306 \, \frac{\text{kJ}}{\text{kg路K}} + 7.3749 \, \frac{\text{kJ}}{\text{kg路K}}
\]  
\[
s_1 = 1.33714 \, \frac{\text{kJ}}{\text{kg路K}}
\]