The entropy at state 1 is calculated as:  
\[
s_1 = s_1(x = 0.005, 100^\circ\text{C}) = s_f(100^\circ\text{C}) + x \cdot (s_g(100^\circ\text{C}) - s_f(100^\circ\text{C}))
\]  
Using Table A-2:  
\[
s_1 = 1.33714 \, \text{kJ/(kg·K)}
\]  

The entropy at state 2 is calculated as:  
\[
s_2 = s_2(x = 0, 70^\circ\text{C}) = s_f(70^\circ\text{C}) = 0.9548 \, \text{kJ/(kg·K)}
\]  

The entropy change is given by:  
\[
\Delta S_{12} = m_2 s_2 - m_1 s_1
\]  
Substituting values:  
\[
\Delta S_{12} = (\Delta m_{12} + m_1) \cdot s_2 - m_1 \cdot s_1 = 13947.198 \, \text{kJ/K}
\]