The energy balance equation is written as:  
\[
0 = \dot{m} \left( h_5 - h_6 + \frac{w_5^2 - w_6^2}{2} \right) + \dot{Q} - \dot{W}
\]  

The velocity \( w_6 \) is derived using the following steps:  
\[
w_6 = \sqrt{\left( \xi_5 v_5 e_5 + c \Delta x \right)}  
\]  
\[
w_6 = \sqrt{\frac{1}{\dot{m}} \left( r \beta v_6 - \beta v_5 \right)}  
\]  
\[
w_6 = \sqrt{\frac{R \left( T_6 - T_5 \right)}{\gamma - 1}} = \sqrt{\frac{\bar{R} \left( T_6 - T_5 \right)}{\gamma - 1}}
\]  

Substituting values:  
\[
w_6 = \sqrt{\frac{2 \cdot \dot{Q} \left( 273.15 - 30.4 - 43794 \right)}{\gamma - 1}} = 47.875 \, \text{m/s}
\]  

Additional equations:  
\[
\dot{W} = \dot{m} \left( h_5 - h_6 \right) = \dot{m} \left( \frac{w_5^2 - w_6^2}{2} \right)
\]  
\[
w_6 = \sqrt{2 \left( \dot{W} - \dot{m} \left( h_5 - h_6 \right) \right)}
\]  
\[
h_5 - h_6 = c_p \left( T_5 - T_6 \right)
\]  

---