The energy balance for determining the mass \( \Delta m \) is expressed as:  
\[
m_2 u_2 - m_1 u_1 = \Delta m h(x=0, 20^\circ\text{C}) - Q_{\text{out},12}
\]  
Rearranging:  
\[
m_1 \left(u_2 - u_1\right) + \Delta m u(x=0, 20^\circ\text{C}) = \Delta m h(x=0, 20^\circ\text{C}) - Q_{\text{out},12}
\]  
Substituting and solving for \( \Delta m \):  
\[
\Delta m = \frac{m_1 \left(u_2(x=0, 70^\circ\text{C}) - u_1(x=0, 100^\circ\text{C})\right) + Q_{\text{out},12}}{h(x=0, 20^\circ\text{C}) - u(x=0, 20^\circ\text{C})}
\]  

---