It is stated that \( m_1 = m_2 \) and \( p_1 = p_2 \) because the same "weight" is exerted by the piston.  

An isentropic polytropic process is assumed:  
\[
T_2 = T_1 \left( \frac{V_1}{V_2} \right)^{\gamma - 1}
\]  
Using the ideal gas law:  
\[
p_2 \cdot v_2 = R \cdot T_2 \quad \Rightarrow \quad v_2 = \frac{R \cdot T_2}{p_2}
\]  
Substituting into the temperature equation:  
\[
T_2 = T_1 \left( \frac{V_1}{\frac{R \cdot T_2}{p_2}} \right)^{\gamma - 1} = T_1 \cdot \frac{R \cdot T_2}{V_1 \cdot p_2}
\]  

This concludes the derivation for \( T_2 \).