The entropy change \( \Delta S_{12} \) is calculated using the formula:  
\[
\Delta S_{12} = m_{2} s_{2} - m_{1} s_{1}
\]  
where:  
- \( m_{1} = 5755 \, \text{kg} \)  
- \( m_{2} = m_{1} + \Delta m_{12} = 9355 \, \text{kg} \)  

To calculate \( s_{1} \):  
\[
s_{1} = s_f + x \cdot (s_g - s_f)
\]  
Substituting values:  
\[
s_{1} = 1.3069 \, \frac{\text{kJ}}{\text{kg·K}} + 0.005 \cdot (7.3553 - 1.3069) \, \frac{\text{kJ}}{\text{kg·K}}
\]  
\[
s_{1} = 1.337 \, \frac{\text{kJ}}{\text{kg·K}}
\]  

To calculate \( s_{2} \):  
\[
s_{2} = s_f + x \cdot (s_g - s_f)
\]  
Substituting values:  
\[
s_{2} = 0.9549 + 0.005 \cdot (7.3553 - 0.9549) \, \frac{\text{kJ}}{\text{kg·K}}
\]  
\[
s_{2} = 0.9839 \, \frac{\text{kJ}}{\text{kg·K}}
\]  

Finally, substituting into the entropy change formula:  
\[
\Delta S_{12} = 9355 \, \text{kg} \cdot 0.9839 \, \frac{\text{kJ}}{\text{kg·K}} - 5755 \, \text{kg} \cdot 1.337 \, \frac{\text{kJ}}{\text{kg·K}}
\]  

---