Energy balance:  
\[
m_2 u_2 - m_1 u_1 = (m_2 - m_1) h_{\text{ein}} + \dot{Q}_{R,12} \cdot t = 0
\]

From Table A2:  
\[
u_2 = u_1 (T = 100^\circ\text{C}, x = 0.005) = 418.94 + 0.005 \cdot (2505.5 - 418.94) = 429.3878 \, \frac{\text{kJ}}{\text{kg}}
\]

The mass \( m_2 \) is defined as:  
\[
m_2 = m_1 + \Delta m
\]

Substituting into the energy balance:  
\[
(m_1 + \Delta m) u_2 - m_1 u_1 = \Delta m h_{\text{ein}} + \dot{Q}_{R,12}
\]

Rearranging for \( \Delta m \):  
\[
\Delta m (h_{\text{ein}} - u_2) = m_1 u_2 - m_1 u_1 - \dot{Q}_{R,12}
\]

Finally:  
\[
\Delta m = \frac{m_1 (u_2 - u_1) - \dot{Q}_{R,12}}{h_{\text{ein}} - u_2}
\]

---