The entropy change is calculated using the equation:  
\[
\Delta S = m_2 s_2 - m_1 s_1 = \Delta m_{12} s_{\text{in}} + \frac{Q_R - Q_{\text{out}}}{T} + \dot{S}_{\text{gen}}
\]  
The entropy at state 2 is expressed as:  
\[
S_{12} = (m_1 + \Delta m_{12}) s_2 - m_1 s_1
\]  
The entropy at state 1 is calculated as:  
\[
s_1 = s_f(100^\circ\text{C}) + x_D \cdot \left(s_g(100^\circ\text{C}) - s_f(100^\circ\text{C})\right) = 1.33774 \, \frac{\text{kJ}}{\text{kg·K}}
\]  
Where:  
\[
s_f(100^\circ\text{C}) = 1.306 \, \frac{\text{kJ}}{\text{kg·K}}, \quad s_g(100^\circ\text{C}) = 7.358 \, \frac{\text{kJ}}{\text{kg·K}}
\]  
The entropy at state 2 is:  
\[
s_2 = s_f(70^\circ\text{C}) = 0.9589 \, \frac{\text{kJ}}{\text{kg·K}}
\]  
Finally, the total entropy change is:  
\[
S_{12} = 7237.85 \, \frac{\text{kJ}}{\text{kg·K}}
\]