The entropy change is calculated using the following entropy balance equation:  

\[
\Delta S = m_2 s_2 - m_1 s_1
\]

The entropy at state 1 (\(s_1\)) is given by:  
\[
s_1 = (TAB-A2) = s_f(100^\circ\text{C}) + x_D \left(s_g(100^\circ\text{C}) - s_f(100^\circ\text{C})\right) = 1.33 + 14 \, \frac{\text{kJ}}{\text{kg·K}}
\]

The entropy at state 2 (\(s_2\)) is calculated as:  
\[
s_2 = (TAB-A2) = s_f(70^\circ\text{C}) = 0.9549 \, \frac{\text{kJ}}{\text{kg·K}}
\]

The total entropy change (\(\Delta S\)) is then:  
\[
\Delta S = \left(m_1 + \Delta m_{12}\right) s_2 - m_1 s_1 = 1237.85 \, \frac{\text{kJ}}{\text{K}}
\]