The energy balance equation is written as:  
\[
\frac{dE_{\text{tot}}}{dt} = \sum \dot{m}_i h_i - \sum \dot{Q} - \sum \dot{W}
\]  
From this, the change in internal energy (\( \Delta U \)) is expressed as:  
\[
\Delta U = \Delta m \cdot h_{\text{ein,12}} - Q_{R,12}
\]  
The mass balance is given as:  
\[
m_{\text{tot,2}} - m_{\text{tot,1}} = \Delta m = m_{\text{tot,2}} - m_{\text{tot,1}}
\]  
Substituting into the energy balance:  
\[
\Delta m \cdot h_{\text{ein,12}} - Q_{R,12} = m_{\text{tot,2}} \cdot u_2 - m_{\text{tot,1}} \cdot u_1
\]  
Rearranging terms:  
\[
\Delta m \cdot (u_2 - h_{\text{ein,12}}) = Q_{R,12} + m_{\text{tot,1}} \cdot u_1 - m_{\text{tot,2}} \cdot u_2
\]  
Finally, solving for \( \Delta m \):  
\[
\Delta m = 3301.94 \, \text{kg}
\]  

Additional notes:  
The total mass \( m_{\text{tot}} \) is defined as:  
\[
m_{\text{tot}} = \Delta m + m_1
\]  

Values from Table A-2:  
\[
u_2 = u_f(70^\circ\text{C}) = 232.55 \, \text{kJ/kg}
\]  
\[
u_1 = u_f(100^\circ\text{C}) = 448.94 \, \text{kJ/kg}
\]  
\[
h_{\text{ein,12}} = h_f(20^\circ\text{C}) = 83.96 \, \text{kJ/kg}
\]  

---