The entropy change is calculated using the following equation:  
\[
\Delta s_{\text{str}} = h_0 - h_6 - T_0(s_6 - s_0) + \Delta \text{ke}
\]  
where \( \Delta \text{ke} \) represents the change in kinetic energy:  
\[
\Delta \text{ke} = \frac{w_6^2 - w_0^2}{2}
\]  

Assumptions:  
- No potential energy is considered.  
- The process is stationary and adiabatic.  

Values used:  
- \( h_0 = 244.6 \, \frac{\text{kJ}}{\text{kg}} \)  
- \( h_6 = 342.04 \, \frac{\text{kJ}}{\text{kg}} \)  
- \( T_0 = 243.75 \, \text{K} \)  

Entropy difference:  
\[
s_0 - s_6 = c_p \ln \left( \frac{T_0}{T_6} \right) = -0.33722 \, \frac{\text{kJ}}{\text{kgÂ·K}}
\]  
\[
T_0(s_0 - s_6) = -82 \, \frac{\text{kJ}}{\text{kg}}
\]  

Kinetic energy change:  
\[
\Delta \text{ke} = \frac{200^2 - 520^2}{2} = -770.05 \, \frac{\text{kJ}}{\text{kg}}
\]  

Final calculation:  
\[
\Delta s_{\text{str}} = 244.6 - 342.04 - 82 - 770.05 = -725.46 \, \frac{\text{kJ}}{\text{kg}}
\]  

---