The exergy destruction rate is expressed as:  
\[
\frac{dE_{\text{ex,dest}}}{dt} = \dot{E}_{\text{ex,in}} - \dot{E}_{\text{ex,out}}
\]  
The change in exergy destruction is:  
\[
\Delta ex_{\text{dest}} = ex_{\text{in}} - ex_{\text{out}}
\]  
Substituting:  
\[
\Delta ex_{\text{dest}} = \left( 1 - \frac{T_0}{T_G} \right) \dot{q} - ex_{\text{reversible}}
\]  
Where:  
\[
ex_{\text{reversible}} = \left( 1 - \frac{T_0}{T_G} \right) \dot{q}
\]  
The final value is:  
\[
ex_{\text{reversible}} = 809.1 \, \text{kJ/kg}
\]