From the energy balance:  
\[
0 = \dot{m} \left[ h_e - h_a + \frac{(w_e^2 - w_a^2)}{2} \right] + \sum_j \dot{Q}_j - \sum_n \dot{W}_{\text{en}} = 0.
\]  
Assuming \( \dot{W}_t = 0 \), \( q = 1195 \, \text{kJ/kg} \), and \( w_e = w_{\text{air}} = 200 \, \text{m/s} \), the equation simplifies:  
\[
\frac{(w_e^2 - w_a^2)}{2} = h_a - h_e - q.
\]  
This can be expressed as:  
\[
h_a - h_e = c_p (T_a - T_e) - q.
\]  

For the isentropic process from state 5 to state 6:  
\[
T_6 = T_5 \cdot \left( \frac{p_6}{p_5} \right)^{\frac{\kappa - 1}{\kappa}}.
\]  
Substituting values:  
\[
T_6 = T_5 \cdot 0.76 = 0.76 \cdot 431.9 \, \text{K} = 328.07 \, \text{K}.
\]

The equation for the outlet velocity \( w_6 \) is derived using the energy balance:  
\[
\frac{w_5^2 - w_6^2}{2} = c_p \, (T_6 - T_5)
\]  
Substituting the given values:  
\[
c_p = 1.006 \, \text{kJ/kg·K}, \quad T_5 = 431.91 \, \text{K}, \quad T_6 = 328.07 \, \text{K}
\]  
\[
\frac{w_5^2 - w_6^2}{2} = 1.006 \, \text{kJ/kg·K} \cdot (328.07 - 431.91) \, \text{K}
\]  
\[
= -104.45 \, \text{kJ/kg}
\]  
Rearranging to solve for \( w_6 \):  
\[
w_6 = \sqrt{2 \cdot (-104.45 \, \text{kJ/kg}) + w_5^2}
\]  
Substituting \( w_5 = 220 \, \text{m/s} \):  
\[
w_6 = \sqrt{2 \cdot (-104.45 \, \text{kJ/kg}) + (220 \, \text{m/s})^2}
\]  
\[
w_6 = 510 \, \text{m/s}
\]