The entropy change is calculated using:  
\[
\Delta S = m_2 \cdot s_2 - m_1 \cdot s_1
\]  

From the table:  
\[
m_1 = 5755 \, \text{kg}
\]  
\[
m_2 = \Delta m + m_1 = 9224.9 \, \text{kg}
\]  
\[
s_2(70^\circ\text{C}) = 0.95649 \, \frac{\text{kJ}}{\text{kg·K}}
\]  
\[
s_1(100^\circ\text{C}) = 1.3061 \, \frac{\text{kJ}}{\text{kg·K}}
\]  

Substituting these values:  
\[
\Delta S = 9224.9 \cdot 0.95649 - 5755 \cdot 1.3061 = 16329.6 \, \frac{\text{kJ}}{\text{K}}
\]  

Converting to MJ:  
\[
\Delta S = 16.33 \, \text{MJ}
\]  

Final result:  
\[
\Delta S = 16.33 \, \text{MJ}
\]