The energy balance equation is written as:  
\[
\Delta E = m \cdot h_{\text{ein}} + Q_e - Q_{\text{aus}} - U_2
\]  

Rearranging for the mass change:  
\[
m_2 \cdot U_2 - m_1 \cdot U_1 = m \cdot h_{\text{ein}}
\]  
where \( m_2 = m_1 + \Delta m \).  

Substituting \( m_2 \) into the equation:  
\[
m_2 \cdot U_2 + \Delta m \cdot U_2 - m_1 \cdot U_1 = m \cdot h_{\text{ein}}
\]  

Rearranging further:  
\[
\Delta m \cdot h_{\text{ein}} = m_2 \cdot U_2 - m_1 \cdot U_1 = m_1 \cdot (U_2 - U_1)
\]  

Solving for \( \Delta m \):  
\[
\Delta m = \frac{m_1 \cdot (U_2 - U_1)}{h_{\text{ein}} - U_2}
\]  

Using the given values from the table:  
\[
U_2 = U_2(70^\circ\text{C}) = 292.95 \, \frac{\text{kJ}}{\text{kg}}
\]  
\[
U_1 = U_1(100^\circ\text{C}) = 418.54 \, \frac{\text{kJ}}{\text{kg}}
\]  
\[
h_{\text{ein}} = h_{\text{p}}(20^\circ\text{C}) = 83.96 \, \frac{\text{kJ}}{\text{kg}}
\]  
\[
m_1 = 5755 \, \text{kg}
\]  

Substituting these values:  
\[
\Delta m = \frac{5755 \cdot (292.95 - 418.54)}{83.96 - 292.95} = 3469.9 \, \text{kg}
\]  

Final result:  
\[
\Delta m_{12} = 3469.9 \, \text{kg}
\]  

---