The equation for the energy balance is written as:  
\[
-2 \left( h_e - h_a \right) = \omega_e^2 - \omega_a^2
\]  

The expression for \(\omega_a^2\) is derived as:  
\[
\omega_a^2 = \omega_5^2 + 2 \cdot c_{p,\text{air}} \cdot \left( T_5 - T_6 \right)
\]  

Rearranging for \(\omega_a\):  
\[
\omega_a = \sqrt{\omega_5^2 + 2 \cdot c_{p,\text{air}} \cdot \left( T_5 - T_6 \right)}
\]  

The calculated value for \(\omega_a\) is:  
\[
\omega_a = 220.47 \, \text{m/s}
\]  

No further content is provided for part c).