The entropy change \( \Delta S \) is derived using the entropy balance equation:  
\[
\frac{dS}{dt} = \sum_i \dot{m}_i(t) \cdot s_i(t) + \int_G \frac{\dot{Q}}{T_G} + \dot{S}_{\text{gen}}
\]  
This simplifies to:  
\[
\Delta S = \sum_i \Delta m_i \cdot s_i + \int_G \frac{Q}{T_G} + S_{\text{gen}}
\]  
Substituting the terms for this problem:  
\[
\Delta S = \Delta m_{12} \cdot (s_{20^\circ\text{C}} - s_{70^\circ\text{C}}) + m_{\text{gen},1} \cdot (s_{100^\circ\text{C}} - s_{70^\circ\text{C}}) + S_{\text{gen}}
\]  

Values used:  
\[
s_{20^\circ\text{C}} = 0.2966 \, \frac{\text{kJ}}{\text{kg路K}}, \quad s_{70^\circ\text{C}} = 0.9549 \, \frac{\text{kJ}}{\text{kg路K}}
\]  
\[
s_{100^\circ\text{C}} = 1.3069 + x_D \cdot (7.3549 - 1.3069) \, \frac{\text{kJ}}{\text{kg路K}}
\]  
Resulting in:  
\[
s_{100^\circ\text{C}} = 1.33714 \, \frac{\text{kJ}}{\text{kg路K}}
\]  

Since the system is adiabatic:  
\[
S_{\text{gen}} = 0
\]  

Reference for values: Table A-2.