Section d)

Sought: \( e_{3, \text{verl}} \) (verl stands for lost)

Exergy balance from state (1) to state (2) since it is adiabatic:

\[
\frac{dE_X}{dt} = \sum \dot{m} e_{\text{str}} + \sum \dot{E}_X - \sum \dot{W} - \rho_0 \frac{dV}{dt} - E_{3, \text{verl}} \quad \Bigg| \dot{m}
\]

This implies:

\[
C = e_{\text{str}} - W - e_{3, \text{verl}}
\]

From which we derive:

\[
e_{3, \text{verl}} = e_{\text{str}} - W
\]

Energy equation from state (1) to state (2):

\[
0 = \dot{m} (ri + kei + pei) + \sum \dot{Q} - \sum \dot{W}
\]