The equations are as follows:

1. \( e_{x,st,s} = h_6 - h_0 - T_0 \cdot (s_6 - s_0) + ke_6 + pe_6 \)

2. \( e_{x,st,0} = h_s - h_0 - T_0 \cdot (s_s - s_0) + ke_s + pe_s \)

3. \( \Delta e_{x,st} = h_6 - h_s - T_0 \cdot (s_6 - s_s) + ke_6 - ke_s \)

4. This equation simplifies to:
   \( = C_p \cdot (T_6 - T_0) - T_0 \cdot (C_p \cdot \ln \left( \frac{T_6}{T_0} \right) - R \cdot \ln \left( \frac{p_6}{p_0} \right)) + \frac{w_6^2}{2} - \frac{w_s^2}{2} \)

5. Substituting values, it becomes:
   \( = 1.006 \frac{kJ}{kgK} \cdot (328.07K - 243.15K) - 243.15K \cdot 1.006 \frac{kJ}{kgK} \cdot \ln \left( \frac{328.07K}{243.15K} \right) \)

6. Adding kinetic energy terms:
   \( + \frac{(50.25 \frac{m}{s})^2}{2} - \frac{(200 \frac{m}{s})^2}{2} \)

7. The final result is:
   \( = 120.808 \frac{kJ}{kg} \)