The equations are as follows:

1. The exergy change for a component \( e_{x,st,c} \) is given by \( e_{x,st,c} = h_c - h_0 - T_c(s_6 - s_c) + \frac{\omega_c^2}{2} \).

2. After canceling out terms, the equation simplifies to \( e_{x,st,c} = 0 \).

3. The change in exergy \( \Delta e_{x,st} \) also simplifies to zero after canceling out terms.

4. The gas constant \( R \) is calculated as \( R = c_p - c_v \) and further simplified to \( R = c_p - \frac{c_p}{\kappa} = 0.2874 \frac{\text{kJ}}{\text{kg K}} \).

5. The initial exergy state \( e_{x,st,0} \) is given by \( e_{x,st,0} = \frac{1}{2} \omega_0^2 \).

6. The change in exergy \( \Delta e_{x,st} \) is calculated as \( \Delta e_{x,st} = h_6 - h_0 - T_c(s_6 - s_0) + \frac{\omega_6^2}{2} - \frac{\omega_0^2}{2} \).

7. This is further expanded to \( \Delta e_{x,st} = c_{p,luft}(T_6 - T_0) - T_0 \left( c_{p,luft} \ln \left( \frac{T_6}{T_0} \right) - R \ln \left( \frac{p_6}{p_0} \right) \right) + \frac{\omega_6^2}{2} - \frac{\omega_0^2}{2} \).

8. The final result is \( \Delta e_{x,st} = 120.81 \frac{\text{kJ}}{\text{kg}} \) after calculating the individual terms as \( 85.43 \frac{\text{kJ}}{\text{kg}} - 73.276 \frac{\text{kJ}}{\text{kg}} + 108.65 \frac{\text{kJ}}{\text{kg}} \).