The expressions are as follows:

1. \( x_{E2} = \frac{u_{E2} - u_f}{u_g - u_f} \) translates to "x sub E2 equals the fraction with numerator u sub E2 minus u sub f and denominator u sub g minus u sub f."

2. \( u_{Q,E2} = u_{a,E1} + \frac{Q_{12}}{m_{\text{EW}}} \) translates to "u sub Q, E2 equals u sub a, E1 plus the fraction with numerator Q sub 12 and denominator m sub EW."

3. \( u_{E1} = u_{E1} + x u \Rightarrow (1-x) u_f + x u_{\text{ext}} \) translates to "u sub E1 equals u sub E1 plus x times u implies (1 minus x) times u sub f plus x times u sub ext."