The equations and expressions provided are as follows:

1. The equation \( m_2 u_2 - m_1 u_1 = \Delta m_{12} u_{12} + Q_R \).

2. The values for \( m_1 \) and \( m_2 \) are given as:
   - \( m_1 = 5755 \, \text{kg} \)
   - \( m_2 = 5755 + \Delta m \)

3. The expression for \( u_2 \) is defined as:
   - \( u_2 = u_f + x (u_g - u_f) \)

4. The specific value for \( u_2 \) at \( 1000 \, \text{C} \) is calculated as:
   - \( u_2 (1000 \, \text{C}) = 478.94 + 0.005 \left( 2506.5 - 478.94 \right) \)
   - This results in \( u_2 = 429.3778 \frac{kJ}{kg} \)

5. Another expression for \( u_2 \) at \( 70 \, \text{C} \) is:
   - \( u_2 = u_f + x u_f (70 \, \text{C}) = 292.95 \frac{kJ}{kg} \)

6. The value for \( h_{12} \) at \( 20 \, \text{C} \) and \( x = 0 \) is:
   - \( h_{12} = h (20 \, \text{C}, x = 0) = 83.95 \)

7. The equation derived from the initial equation is:
   - \( (m_1 + \Delta m) u_2 - m_1 u_1 = \Delta m u_{12} + Q_R \)

8. The expression for \( \Delta m \) is derived as:
   - \( \Delta m (u_{12} - u_2) = -m_1 u_1 + m_1 u_2 - Q_R \)
   - \( \Delta m = \frac{-m_1 u_1 + m_1 u_2 - Q_R}{u_{12} - u_2} \)

9. Continuing, the value for \( \Delta m \) is calculated as:
   - \( \Delta m = - \frac{5775 (429.377) + 5775 (292.95) - 35 \cdot 10^3}{83.95 - 292.95} \)
   - This results in \( \Delta m = 3937 \, \text{kg} \)