The equation for \( Q_{A2} \) is given by:
\[ Q_{A2} = x_{Eis2} \cdot m_{EW} \cdot (v_{w2} - v_{Eis2}) + x_{Eis1} \cdot m_{EW} \cdot (v_{w1} - v_{Eis1}) + (1 - x_{Eis2}) \cdot m_{EW} \cdot (v_{w2} - v_{Eis2}) + (1 - x_{Eis1}) \cdot m_{EW} \cdot (v_{w1} - v_{Eis1}) + m_{g} \cdot (v_{g2} - v_{g1}) \]

The equation simplifies to:
\[ Q_{A2} = x_{Eis2} \frac{m_{EW} v_{w2}}{v_{Eis2}} + (1 - x_{Eis2}) \frac{m_{EW} v_{w2}}{v_{Eis2}} + m_{g} \cdot v_{g2} - x_{Eis1} \frac{m_{EW} v_{w1}}{v_{Eis1}} - (1 - x_{Eis1}) \frac{m_{EW} v_{w1}}{v_{Eis1}} - m_{g} \cdot v_{g1} \]

The values for constants are:
\[ m_{EW} = 0.1 \, \text{kg} \]
\[ v_{Eis1,2} = v_{solid} (0.033 \frac{\text{kJ}}{\text{kg}}) = -333.442 \frac{\text{kJ}}{\text{kg}} \]
\[ v_{w2} = v_{liquid} (0.003 \frac{\text{kJ}}{\text{kg}}) = -0.033 \frac{\text{kJ}}{\text{kg}} \]
\[ v_{Eis1} = v_{solid} (0.1) = -333.455 \frac{\text{kJ}}{\text{kg}} \]
\[ v_{w1} = v_{liquid} (0.2) = -0.045 \frac{\text{kJ}}{\text{kg}} \]

The equation involving \( x_{Eis} \) is:
\[ x_{Eis} (m_{EW} (v_{w2} - v_{Eis2})) = m_{EW} v_{w2} - x_{Eis} m_{EW} v_{Eis2} + (1 - x_{Eis}) m_{EW} v_{w1} + m_{g} (v_{g2} - v_{g1}) = c_{v} m_{g} (T_{2} - T_{1}) \]

The value of \( x_{Eis} \) is calculated as:
\[ x_{Eis} = \frac{0.1 \, \text{kg} \cdot (-0.033 \frac{\text{kJ}}{\text{kg}}) + 0.6 \cdot 0.1 \, \text{kg} \cdot (-333.455 \frac{\text{kJ}}{\text{kg}}) - (1 - 0.6) \cdot 0.1 \, \text{kg} \cdot (-0.045 \frac{\text{kJ}}{\text{kg}})}{0.1 \, \text{kg} \cdot (-0.033 + 333.442) \frac{\text{kJ}}{\text{kg}}} + \frac{0.033 \frac{\text{kJ}}{\text{kg}} - 0.003 \cdot 0.1 \, \text{kg} (279.173 \text{k} - 773.15 \text{k})}{0.1 \, \text{kg} \cdot (-0.033 + 333.442) \frac{\text{kJ}}{\text{kg}}} \]

The equation for \( Q_{A2} \) continues as:
\[ Q_{A2} = x_{2} m_{EW} v_{Eis2} - x_{2} m_{EW} v_{Eis2} + m_{EW} \]