c)
The expression for \( e_{x,str}^m \) is given by the equation:
\[ e_{x,str}^m = \left[ h_0 - h_0 - T_0 (s - s_0) + \frac{v_0^2}{2} \right] \]

The expression for \( e_{x,str,6} \) is given by the equation:
\[ e_{x,str,6} = \left[ h_6 - h_0 - T_0 (s_6 - s_0) + \frac{v_6^2}{2} \right] \]

The expression for \( e_{x,str,0} \) is given by the equation:
\[ e_{x,str,0} = \left[ h_0 - h_0 - T_0 (s_0 - s_0) + \frac{v_0^2}{2} \right] \]
which simplifies to:
\[ e_{x,str,0} = \frac{v_0^2}{2} = 20000 \frac{m^2}{s^2} \]

2. a1
The expression for \( \dot{E}_{x,\text{verL}} \) is given by the equation:
\[ \dot{E}_{x,\text{verL}} = \dot{m} \left[ h_e - h_a - T_0 (s_e - s_a) + s \Delta e \right] + \sum_i \left( \eta_i \frac{T_0}{T_i} \right) \dot{Q}_i = e_{x,\text{verL in}} \]

The equation simplifies to:
\[ 0 = \dot{m} \left[ h_e - h_a + s \Delta e \right] + \sum_j \dot{Q}_j \]

From which it follows that:
\[ \dot{E}_{x,\text{verL}} = \dot{m} \left[ - T_0 (s_e - s_a) \right] + \sum_i \left( \eta_i - \frac{T_0}{T_i} \right) \dot{Q}_i - \sum_j \dot{Q}_j \]
which simplifies to:
\[ \dot{E}_{x,\text{verL}} = e_{x,\text{verL in}} \]

Finally, the expression for \( e_{x,\text{verL}} \) is given by:
\[ e_{x,\text{verL}} = - T_0 (s_e - s_a) + \frac{1}{\dot{m}} \sum_i \left( \eta_i - \frac{T_0}{T_i} \right) \dot{Q}_i - \frac{1}{\dot{m}} \sum_j \dot{Q}_j \]