The expression for \( s_{ex} \) is given by:
\( s_{ex} = (C_p (T_5 - T_0) - T_0 (C_p \ln \frac{T_5}{T_0}) - R \ln \frac{P_5}{P_0}) + \frac{w_6^2}{2} - \frac{u_0^2}{2} \)

Another expression for \( s_{ex} \) is:
\( s_{ex} = \sqrt{(288 \frac{u}{u_s})} \)

Equation (1) states:
\( \text{exer1} = \text{exQ} - \Delta \text{exS} \frac{v_{00} u_{S}}{u_{S}} \)

The expression for \( \text{exQ} \) is:
\( \text{exQ} = \left(1 - \frac{T_0}{1298K}\right) q_B \)

This simplifies to:
\( = 969.58 \frac{u_{S}}{u_{S}} \)

Finally, the expression for \( \text{exer1} \) is:
\( \text{exer1} = 969.58 \frac{u_{S}}{u_{S}} \)