\( \dot{Q}_{in} \) (crossed out)  
\( \dot{m} \cdot (h_6 - h_5 - T_0 \cdot (s_6 - s_5) + \Delta k_e) \)  

\( T_0 = 243.15 \, \text{K} \)  

\( \Delta ex_{str} = \dot{m} \cdot (h_e - h_s) \)  
\( \dot{m} \cdot (h_6 - h_0 - T_0 \cdot (s_6 - s_0) + k_e_6) - \dot{m} \cdot (h_s - h_0 - T_0 \cdot (s_s - s_0) + k_e_s) \)  

\( = \dot{m} \cdot (h_e - h_s - T_0 \cdot (s_6 - s_s) + \frac{w_6^2 - w_s^2}{2}) \)  

\( h_e - h_s = \int c_p \, dT = 1.006 \cdot (328.07 + (crossed out)243.15) = 85.43 \, \frac{\text{kJ}}{\text{kg}} \)  

\( s_6 - s_s = \int \frac{c_p}{T} \, dT - R \ln \left( \frac{p_6}{p_0} \right) \)  

\( = 1.006 \cdot \ln \left( \frac{328.07}{243.15} \right) - 1.725 \, \frac{\text{kJ}}{\text{kg·K}} \cdot \ln \left( \frac{4}{1} \right) \)  

\( = 0.301 \, \frac{\text{kJ}}{\text{kg·K}} \)  

\( \Delta ex_{str} = m_{ges} \cdot (85.43 \, \frac{\text{kJ}}{\text{kg}} - 243.15 \, \frac{\text{kJ}}{\text{kg}} \cdot 0.301 \, \frac{\text{kJ}}{\text{kg·K}}) = m_{ges} \cdot (24659.122 \, \frac{\text{kJ}}{\text{kg}}) \)  

\( e_x = 24659.122 \, \frac{\text{kJ}}{\text{kg}} \)