\( m_2 \cdot u_2 - m_1 \cdot u_1 = \Delta m_{12} \cdot h_{ein} + Q_{R,12} \)  
\( \Rightarrow m_2 = m_1 + \Delta m_{12} \)  
\( Q_{R,12} = m_1 (u_2 - u_1) + \Delta m_{12} (h_{ein} - u_2) \)  
\( u_2 = u_f (70^\circ C) = 292.95 \, \frac{kJ}{kg} \)  
\( u_1 = u_f (100^\circ C) + x_D (u_g (100^\circ C) - u_f (100^\circ C)) = 418.94 \, \frac{kJ}{kg} + 0.005 (2506.5 - 418.94) \, \frac{kJ}{kg} = 429.37 \, \frac{kJ}{kg} \)  
\( h_{ein} = h_f (20^\circ C) = 83.96 \, \frac{kJ}{kg} \)  
\( \Delta m_{12} = \frac{35,000kJ - 5755kg \cdot (292.95 - 429.37) \, \frac{kJ}{kg}}{292.95 - 83.96 \, \frac{kJ}{kg}} = 332.4 \, \frac{kg}{K} \)