T_0 = -30°C = 243.15 K  

p_0 V_0 = R T_0 → V_0 = R T_0 / p_0  

R = c_p - c_v = c_p^(1 - κ) - c_v^(1 - κ) = 0.287429 kJ/kg·K  

V_0 = 3.65908 m^3/kg  

T_6 / T_0 = (k - 1) → T_6 = T_0^(k / k - 1)  

T_6 = V_0 / V_6  

T_6 = R T_6 / p_6  

T_6 = R / (p_6 · V_0)  

T_6 = R / (p_6 · V_0)^(k - 1)  

T_6 = R / (p_6 · V_0)^(k).

\( T_6 / T_5 = (p_6 / p_5)^{(k-1)/k} \)  
\( \Rightarrow T_6 = T_5 \cdot (p_6 / p_5)^{(k-1)/k} = 328.0747 \, \text{K} \)  

\( S_5 = S_6 \)  

\( 0 = \dot{m}_{\text{gas}} \left[ h_5 - h_6 + \frac{w_5^2 - w_6^2}{2} \right] - \dot{W}_{\text{turbine}} \)