\( \frac{dE_x}{dt} = \sum \dot{E}_{x,str,i} + \sum \dot{E}_{x,Q,j} - \sum \dot{W}_n - \dot{E}_{x,verl} \)  

Adiabatic: \( \dot{E}_{x,Q,j} = 0 \)  

\( 0 = \sum \dot{E}_{x,str,i} + \dot{E}_{x,QD} - \dot{E}_{x,verl} \)  

\( \dot{e}_{x,verl} = h_6 - h_0 - T_0(s_6 - s_0) + ke + \left(1 - \frac{T_0}{T_B}\right) q_B \)  

\( \dot{e}_{x,verl} = \Delta e_{x,str} + \left(1 - \frac{T_0}{T_B}\right) q_B \)  

\( T_0 = -30^\circ C \)  
\( T_B = 1289 \, \text{K} \)  
\( q_B = 100 \, \text{kJ/kg} \)  

---

Thus:  
\( \dot{e}_{x,verl} = 100 \, \text{kJ/kg} + \left(1 - \frac{273.15 - 30}{1289}\right) 1195 = 1069.58 \, \text{kJ} \)