\( p_{g,1} \), \( m_g \)  

\( p_{g,1} \cdot A = m_g \cdot g + m_{EW} \cdot g + p_{amb} \cdot A \)  
\( p_{g,1} = \frac{1}{A} (m_g + m_{EW}) \cdot g + p_{amb} \)  
\( = 110003.6 \, \text{N/m}^2 \)  

\( A = \pi \cdot 0.1^2 \)  
\( p_{amb} = 100000 \, \text{N/m}^2 \)  

\( m = \frac{p \cdot V}{R \cdot T} = 0.0027 \, \text{kg} \)  

\( T = 273.15 \, \text{K} \)  
\( R = \frac{8.314}{50} = 0.16628 \, \text{kJ/kg·K} \)  
\( = 166.28 \, \text{J/kg·K} \)  

\( V = 3.14 \cdot 10^{-3} \, \text{m}^3 \)  

---