\( M_2 \cdot S_2 - M_1 \cdot S_1 = \Delta M_{12} \cdot S_{in} + \frac{Q_{out}}{T_{ein}} - \frac{Q_{out}}{T_{aus}} + S_{erz} \)  

\( S_2 = S_f(70^\circ C) = 0.9549 \, \text{kJ/kg路K} \)  

\( S_1 = S_f(100^\circ C) + x_D \cdot (S_g(100^\circ C) - S_f(100^\circ C)) = 1.33714 \, \text{kJ/kg路K} \)  

\( S_{in} = S_f(20^\circ C) = 0.296 \, \text{kJ/kg路K} \)  

\( T_{ein} = T_{rev} = \frac{Q_{rev}}{S_2 - S_{in}} = \frac{Q_{out}}{S_2 - S_{in}} = \frac{35,450,000 \, \text{kJ}}{(0.954 - 1.33714) \, \text{kJ/kg路K}} \)  

\( T_{aus} = 285 \, \text{K} \, \text{(from b)} \)  

\( S_{erz} = M_1 \cdot S_1 - M_2 \cdot S_2 - \Delta M_{12} \cdot S_{in} - \frac{Q_{out}}{T_{ein}} + \frac{Q_{out}}{T_{aus}} \)