\( w_6 = 520 \, \text{m/s} \)  
\( T_6 = 340 \, \text{K} \)  

\( \Delta ex_{str} = ex_{str,6} - ex_{str,0} \)  

\( ex_{str,6} = h_6 - h_0 - T_u (s_6 - s_0) + \frac{w_6^2}{2} \)  
\( ex_{str,0} = h_0 - h_u - T_u (s_0 - s_u) + \frac{w_0^2}{2} \)  

\( \Delta ex_{str} = h_6 - h_0 - T_u (s_6 - s_0) + \frac{w_6^2 - w_0^2}{2} \)  

\( T_u = T_0 = 243.15 \, \text{K} \)  

\( h_6 - h_0 = c_{p,\text{Luft}} \cdot (T_6 - T_0) \, \text{(Tables 1G)} \)  
\( s_6 - s_0 = c_{p,\text{Luft}} \cdot \ln \left( \frac{T_6}{T_0} \right) - R \cdot \ln \left( \frac{p_6}{p_0} \right) \, \text{(eq. 20.1)} \)  

\( \Delta ex_{str} = c_{p,\text{Luft}} \cdot \left[ (T_6 - T_0) - T_u \cdot \ln \left( \frac{T_6}{T_0} \right) \right] + \frac{w_6^2 - w_0^2}{2} \)  

\( \Delta ex_{str} = 1.006 \, \text{kJ/kgÂ·K} \cdot \left[ (340 - 243.15) - 243.15 \cdot \ln \left( \frac{340}{243.15} \right) \right] + \frac{520^2 - 200^2}{2} \)  

\( \Delta ex_{str} = -725.42 \, \text{kJ/kg} + 125.62 \, \text{kJ/kg} \)  

\( \Delta ex_{str} = \underline{\underline{-849.96 \, \text{kJ/kg}}} \)  

---