\( \overline{T}_{\text{KF}} = \frac{\int_{S_2}^{S_1} T \, \text{d}s}{S_2 - S_1} = \frac{q_{12,\text{rev}}}{S_2 - S_1} = \frac{h_2 - h_1}{S_2 - S_1} \)  

i.p.: \( h_2 - h_1 = \int_{T_a}^{T_2} c^{\text{li}} \, \text{d}T + v^{\text{li}} \cdot (p_2 - p_0) = c^{\text{li}} \cdot (T_2 - T_1) \)  

\( S_2 - S_1 = c^{\text{li}} \cdot \ln \left( \frac{T_2}{T_1} \right) \)  

\( \overline{T}_{\text{KF}} = \frac{T_2 - T_1}{\ln \left( \frac{T_2}{T_1} \right)} = \frac{238.15 - 288.15}{\ln \left( \frac{238.15}{288.15} \right)} = 293.12 \, \text{K} \)