\[
\Delta ex_{str} = e_{t, str, 6} - e_{t, str, 0}
\]  
\[
\Delta ex_{str} = (h_6 - h_0 - T_0(s_6 - s_0) + te + pe) \Rightarrow (h_6 - h_0 - T_0(s_6 - s_0) + te + pe)
\]  
\[
\Delta ex_{str} = h_6 - h_0 - T_0(s_6 - s_0) + te + pe
\]  
\[
= c_p(T_6 - T_0) - T_0(c_p \ln \frac{T_6}{T_0} - R \ln \frac{p_6}{p_0}) - \frac{w_6^2 - w_0^2}{2}
\]  
\[
= 1.006 \, \frac{\text{kJ}}{\text{kg·K}} \cdot (328.07 \, \text{K} - 243.15 \, \text{K}) - 243.15 \, \text{K} \cdot (1.006 \, \frac{\text{kJ}}{\text{kg·K}} \ln \frac{328.07}{243.15} - R \ln \frac{0.45}{0.191}) - \frac{220^2}{2} - \frac{200^2}{2}
\]  
\[
\Delta ex_{str} = NO.66 \, \frac{\text{kJ}}{\text{kg}}
\]