\( m_1 = 5755 \, \text{kg} \)  
\( x_1 = 0.005 \)  
\( T_1 = 100^\circ \text{C} \)  
\( T_{\text{in}} = 20^\circ \text{C} \)  

\( m_2 = m_1 + \Delta m \)  
\( \Delta m \)  
\( T_2 = 70^\circ \text{C} \)  

\( m_2 u_2 - m_1 u_1 = \dot{m}_{\text{ein}} + Q_{\text{aus,12}} \)  

A-2 @ \( 100^\circ \text{C} \):  
\( u_1 = u_f(100^\circ \text{C}) + x_D \left( h_g(100^\circ \text{C}) - h_f(100^\circ \text{C}) \right) \)  
\( = 418.99 \, \text{kJ/kg} + 0.005 \left( 2506.5 \, \text{kJ/kg} - 418.99 \, \text{kJ/kg} \right) \)  
\( = 429.38 \, \text{kJ/kg} \)  

@ \( 70^\circ \text{C} \):  
\( u_2 = 202.95 \, \text{kJ/kg} + 0.005 \left( 2496.9 \, \text{kJ/kg} - 202.95 \, \text{kJ/kg} \right) \)  
\( = 303.83 \, \text{kJ/kg} \)  

\( h_{\text{ein}} @ 20^\circ \text{C} \):  
\( h_{\text{ein}} = h_f(20^\circ \text{C}) + x_D \left( h_g(20^\circ \text{C}) - h_f(20^\circ \text{C}) \right) \)  
\( = 79.77 \, \text{kJ/kg} + 0.005 \left( 2536.2 \, \text{kJ/kg} - 79.77 \, \text{kJ/kg} \right) \)  
\( = 87.08 \, \text{kJ/kg} \)  

\( m_2 u_2 - m_1 u_1 + \Delta m u_{\text{ein}} - \Delta m h_{\text{ein}} = Q_{\text{aus}} \)  

\( \Delta m = \frac{Q_{\text{aus}} + (\dot{m}_{\text{ein}} (u_{\text{ein}} - u_2))}{u_2 - h_{\text{ein}}} \)  

\( \Delta m = 3495 \, \text{kg} \)