\( \dot{m}_{\text{ges}} ex_{\text{str},6} - ex_{\text{str},0} \)  

\( ex_{\text{str},6} = h_6 - h_0 - T_0 (s_6 - s_0) + \frac{1}{2} w_6^2 \)  
\( ex_{\text{str},0} = h_0 - h_0 - T_0 (s_0 - s_0) + \frac{1}{2} w_0^2 \)  

\( \Delta ex_{\text{str},06} = ex_{\text{str},6} - ex_{\text{str},0} = h_6 - h_0 - T_0 s_6 + T_0 s_0 + \frac{1}{2} w_6^2 - \frac{1}{2} w_0^2 \)  
\( = c_p (T_6 - T_0) = -T_0 (s_6 - s_0) \)  

\( \Delta ex_{\text{str},06} = c_p (T_6 - T_0) - T_0 \left( c_p \ln \left( \frac{T_6}{T_0} \right) \right) + \frac{w_6^2 - w_0^2}{2} - R_u \ln \left( \frac{p_6}{p_0} \right) \)  

\( = 120.8 \, \frac{\text{kJ}}{\text{kg}} \)