\( w_6, T_6 \)  
Balance equation:  
\( 0 = \dot{m}_{ges} (h_5 - h_6 + \frac{1}{2} (w_5^2 - w_6^2)) + \dot{Q}^0 - \dot{W}^c \)  

\( \frac{1}{2} (w_5^2 - w_6^2) = h_6 - h_5 \)  

\( h_6 = c_p (T_6 - T_5) \)  

\( \rightarrow w_6^2 = 2 (h_5 - h_6) - w_5^2 \)  

\( h_5 = c_p (T_5 - T_6) \)  

\( \rightarrow w_6 = \sqrt{2 c_p (T_5 - T_6) - w_5^2} \)  

\( T_6 = T_5 \left( \frac{p_6}{p_5} \right)^{\frac{\kappa - 1}{\kappa}} = 431.9 \, \text{K} \)  

\( p_6 = 0.491 \, \text{bar} \)  
\( p_5 = 0.5 \, \text{bar} \)  

---