\( p_{g,1} = \frac{m_K \cdot g + m_{EW} \cdot g + p_{amb} \cdot A}{A} \)  

\( p_{g,1} = \frac{m_K + m_{EW} \cdot g}{A} + p_{amb} \)  

\( p_{g,1} = \frac{0.764 + 32 \cdot 9.81 \, \text{m/s}^2 + 1.05 \, \text{N/m}^2}{\pi \cdot (0.1 \, \text{m})^2} \)  

\( p_{g,1} = 1.40 \, \text{bar} \)  

\( p \cdot V = m \cdot R \cdot T \Rightarrow m = \frac{p \cdot V}{R \cdot T} \cdot M_g \)  

\( m = \frac{7.4 \cdot 10^2 \, \text{Pa} \cdot 3.14 \cdot 10^{-3} \, \text{m}^3}{8.31 \, \text{kJ/(kmolÂ·K)} \cdot 773.15 \, \text{K}} \cdot 50 \, \text{kg/kmol} \)  

\( m = 3.66 \, \text{g} \)