\( t_{ice,2} = t_{ice,1} = 0.003^\circ C \)  

\( \Rightarrow \Delta E = E_2 - E_1 = Q_{12} = 1500 \, J \)  

\( \Delta u_{12} = \frac{1500 \, J}{m} = u_2 - u_1 = m \cdot \left( \frac{(x_2 \cdot u_{2,ice} + (1 - x_2) \cdot u_{2,flüssig}) - (x_1 \cdot u_{1,ice} + (1 - x_1) \cdot u_{1,flüssig})}{x_1 \cdot u_{1,ice} + (1 - x_1) \cdot u_{1,flüssig}} \right) \)  

\( \Rightarrow x_2 = \frac{\Delta u_{12}}{m} + \left( x_1 \cdot u_{1,ice} + (1 - x_1) \cdot u_{1,flüssig} \right) - u_{2,flüssig} \)  

\( x_2 = \frac{\Delta u_{12}}{m} + \left( x_1 \cdot u_{1,ice} + (1 - x_1) \cdot u_{1,flüssig} \right) - u_{2,flüssig} \) divided by \( u_{2,ice} - u_{2,flüssig} \)  

\( x_2 = 0.555 \)