Determine \( \dot{Q}_{\text{out}} \):  
\( O = \dot{m} [h_e - h_a] + \sum \dot{Q}_i \)  

\( \Rightarrow \dot{m} [h_a - h_e] - \dot{Q}_R = \dot{Q}_{\text{out}} = 0.3 \, \text{kg/s} [h_2 - h_n] - 100 \, \text{kW} \)  

\( h_n^{A-2} = 2626.8 \, \text{kJ/kg}, \, h_2^{A-2} = 2676.4 \, \text{kJ/kg}, \, h_{n,f} = 252.9 \, \text{kJ/kg}, \, h_{2,f} = 415.04 \, \text{kJ/kg} \)  

\( h_n = h_{n,f} + x(h_{n,g}) \)  

\( h_n = 304.65 \, \text{kJ/kg}, \, h_2 = 436.33 \, \text{kJ/kg} \)  

\( \dot{Q}_{\text{out}} = -62.3 \, \text{kW} \)  

---