\( exstr6 - exstr0 \)  

\( exstr6 - exstr0 = he - ha - T0 (se - sa) + \Delta ke \)  

\( he = cp (T0 - T6) - T0 (cp \ln \frac{T0}{T6}) - R \ln \frac{p0}{p6} + \Delta ke \)  

\( cp = 1.006 \)  

\( 243.15 - 526.918 - 243.15 (1.006 \ln \frac{526.918}{243.15}) - R \ln \frac{p0}{p6} + \Delta ke \)  

\( R = 0.287 \, \text{kJ/kg·K} \)  

\( 285.47 \, \text{kJ/kg} - T0 (0.778 \, \text{kJ/kg·K}) + \frac{(489.449)^2}{2} - \frac{(200)^2}{2} \)  

\( 285 + 96.299 \, \text{kJ/kg} + 99750.16 \, \text{J} \)  

\( \Delta exstr = 196079.16 \, \text{J} \)