\( \dot{m}_{in} = 0.3 \, \text{kg/s} \)  
\( m_{ges} = 5755 \, \text{kg} \)  

\( 0 = \dot{m} (h_{ein} - h_{aus}) + \dot{Q}_R + \dot{Q}_{aus} - \dot{W}^0 \)  

\( \dot{Q}_{aus} = -\dot{Q}_R + \dot{m} (h_{aus} - h_{ein}) \)  

\( h_{ein} = h_f(70^\circ \text{C}) + 0.005 \, (h_{fg}(70^\circ \text{C}) - h_f(70^\circ \text{C})) = 304.65 \, \text{kJ/kg} \)  

\( h_{aus} = h_f(100^\circ \text{C}) + 0.005 \, (h_{fg}(100^\circ \text{C}) - h_f(100^\circ \text{C})) = 430.825 \, \text{kJ/kg} \)  

\( \Rightarrow \dot{Q}_{aus} = -62.2972 \, \text{kJ/s} = -62.3 \, \text{kW} \)  

---