\( ex_{verl} = T_0 \dot{S}_{erz} \)  

\( 0 = in (s_0 - s_1) + \frac{\dot{Q}}{T} + \dot{S}_{erz} \)  

Adiabatic process  

\( \dot{S}_{erz} = s_1 - s_0 + \frac{\dot{q}}{T} \)  

\( \dot{S}_{erz} = c_p \ln \left( \frac{T_c}{T_0} \right) - R \ln \left( \frac{p_c}{p_0} \right) \)  

\( ex_{verl} = T_0 c_p \ln \left( \frac{T_c}{T_0} \right) \)  

\( T_0 = 243.15 \, K \)  

\( ex_{verl} = 243.15 \, K \cdot 1.006 \, \frac{kJ}{kg \cdot K} \cdot \ln \left( \frac{343.0 \, K}{243.15 \, K} \right) = 82.009 \, \frac{kJ}{kg} \)