\(\Delta ex_{str} = [h_0 - h_6 - T_0 (s_0 - s_6) + \frac{w_0^2 - w_6^2}{2}] + (1 - \frac{T_0}{T_B}) \cdot \frac{\dot{Q}_B}{\dot{m}_K} \)  
Ideal Gas:  

\( h_0 - h_6 = c_p \cdot (T_0 - T_6) = 1.006 \, \text{kJ/kg·K} \cdot (-30^\circ \text{C} - 328 \, \text{K} + 273.15 \, \text{K}) \)  
\(\Rightarrow h_0 - h_6 = -85.46 \, \text{kJ/kg} \)  

\( T_0 (s_0 - s_6) = T_0 \cdot c_p \cdot \ln \left( \frac{T_0}{T_6} \right) - R \cdot \ln \left( \frac{p_6}{p_0} \right) \)  
\( c_p = \text{const}, R = \text{const} \)  
\(\Rightarrow T_0 (s_0 - s_6) = 243.15 \, \text{K} \cdot 1.006 \, \text{kJ/kg·K} \cdot \ln \left( \frac{243.15 \, \text{K}}{328 \, \text{K}} \right) \)  
\(\Rightarrow T_0 (s_0 - s_6) = -73.3 \, \text{kJ/kg} \)  

\(\frac{w_0^2 - w_6^2}{2} = \frac{200^2 \, \text{m}^2/\text{s}^2 - 507.24^2 \, \text{m}^2/\text{s}^2}{2} \)  
\(\Rightarrow \frac{w_0^2 - w_6^2}{2} = -108.65 \, \text{kJ/kg} \)  

\((1 - \frac{T_0}{T_B}) \cdot \frac{\dot{Q}_B}{\dot{m}_K} = (1 - \frac{243.15 \, \text{K}}{1289 \, \text{K}}) \cdot 1195 \, \text{kJ/kg} \)  
\(\Rightarrow (1 - \frac{T_0}{T_B}) \cdot \frac{\dot{Q}_B}{\dot{m}_K} = 906.95 \, \text{kJ/kg} \)  

\(\Delta ex_{str} = -85.46 + 73.3 - 108.65 + 906.95 \)  
\(\Rightarrow \Delta ex_{str} = 786.14 \, \text{kJ/kg} \)  

\(\Rightarrow \Delta ex_{str} = -\Delta ex_{str} = -786.14 \, \text{kJ/kg} \)