Reversible adiabatic = isentropic  

First law of thermodynamics:  
0 = m (h_e + w_e squared divided by 2 - h_a - w_a squared divided by 2) + ΣQ - ΣW  

This simplifies to:  
h_e + w_e squared divided by 2 = h_a + w_a squared divided by 2  

Isentropic: \( n = 1.4 \)  

\( T_2 \) divided by \( T_1 \) = \( (P_2 \) divided by \( P_1)^{(n-1)/n} \)  

This leads to:  
\( T_2 = T_1 (P_2 \) divided by \( P_1)^{(n-1)/n} \)  

\( T_6 = T_5 (P_0 \) divided by \( P_5)^{(n-1)/n} = 328.07 \, K \)  

\( h_e - h_a = w_a \)  

\( h_e - h_a + w_e squared divided by 2 = w_a squared divided by 2 \)  

\( w_a = \sqrt{2 (h_e - h_a) + w_e squared} \)  

\( h_e - h_a = h_s - h_6 \)  

\( h_e - h_a = c_p^{\circ} (T_a - T_2) = 1.006 \, kJ/kgK (431.9 \, K - 328.07 \, K) \)  

\( w_a = \)