\( p_{EW} = \frac{F_c}{A} + p_{amb} \)  
\( m_g = \frac{p \cdot V}{R \cdot T} = \frac{23.9 \cdot 10^5 \, \text{Pa}}{0.000785} = 127979.6 \, \text{Pa} = 1.36 \, \text{bar} \)  

\( T_{EW} = 0^\circ C \)  

\( U_A = m_{eis} \cdot U_{FE} + m_w \cdot U_{FL} = 0.075 \cdot -333.448 + 0.062 \cdot -0.0366 = -1755.05 \)  

\( m_{eis} = 0.6 \cdot m_{EW} \)  
\( m_{EW} = m_{eis} + m_w = 0.6 \cdot m_w = 0.1 \cdot 1.6 = 0.062 \, \text{kg} \)  

\( m_{eis} = 0.6 \cdot 0.062 = 0.0375 \, \text{kg} \)  

\( U_{FE} = U(16a) + \frac{1}{1.3} \cdot \left( \frac{U(1.4) - U(1)}{1.4 - 1.3} \right) = -333.448 \)  

\( U_{FL} = U(16a) + \frac{1}{1.3} \cdot \left( \frac{U(1.4) - U(1)}{1.4 - 1.3} \right) = -0.033 \cdot 8 \cdot (0.012) = -0.0366 \)  

\( \Delta E = \Delta U = Q = 1366.29 = (m_{eis,2} \cdot U_{FE} + m_w,12 \cdot U_{FL}) \)  

\( Q - U_A = m_{eis} \cdot U_{FE} + (0.1 - m_{eis}) \cdot U_{FL} \)  
\( Q - U_A - 0.1 \cdot U_{FL} = m_{eis} \cdot (U_{FE} - U_{FL}) \)  

\( m_w = 0.1 - m_{eis} \)  
\( x = \frac{m_{eis}}{m_{EW}} \)