\( \dot{ex}_{\text{str}} = m \cdot \left[ h_6 - h_0 - T_0 \cdot (s_6 - s_0) + \frac{(w_6^2 - w_0^2)}{2} \right] \)  

\( h_6 - h_0 = h_6 - h_5 + h_5 - h_0 = c_p \cdot (T_6 - T_5) + R \cdot T_0 \cdot \ln \left( \frac{p_5}{p_0} \right) \)  

\( s_6 - s_0 = s_6 - s_5 + s_5 - s_0 = c_p \cdot \ln \left( \frac{T_6}{T_5} \right) - R \cdot \ln \left( \frac{p_5}{p_0} \right) \)  

\( R = c_p - c_v = c_p - \frac{c_p}{\kappa} = c_p \cdot \left( 1 - \frac{1}{\kappa} \right) = 0.287 \)  

\( \dot{ex}_{\text{str}} = 11.10 \, \text{kJ} \)