An equation is written:  
dE/dt = 0  

The equation is crossed out and replaced with:  
0 = ṁ (h_in + k_ein - h_aus - k_eaus) + Q̇_B  

This is further rewritten as:  
0 = ṁ (w_ein squared divided by 2 minus w_aus squared divided by 2 + Q̇_B + h_ein - h_aus)  

The equation is simplified:  
w_aus squared divided by 2 = w_ein squared divided by 2 + 2 cp (T_6 - T_1)  

T_6:  
s_aus = s_e  
s_5 - s_6 = cp ln(T_5 divided by T_6) - R ln(p_5 divided by p_6) = 0  

ln(T_5 divided by T_1) = R divided by cp ln(p_5 divided by p_6)  

T_5 divided by T_6 = (p_5 divided by p_0) raised to the power of R divided by cp  

T_6 = T_5 (p_0 divided by p_5) raised to the power of kappa minus 1 divided by kappa  

T_6 = 431.9 K multiplied by (0.191 bar divided by 0.5 bar) raised to the power of 0.4 divided by 1.4 = 328.07 K  

w_aus = square root of (w_ein squared divided by 2 + 2 cp (T_6 - T_1)) = 206.36 m/s  

---