\( T_6 = T_5 \left( \frac{p_6}{p_5} \right)^{\frac{n-1}{n}} \)  
\( T_6 = T_5 \left( \frac{p_6}{p_5} \right)^{\frac{n-1}{n}} \)  
\( T_6 = 328.07 \, K \)  

\( \dot{Q} = 0 \)  
\( \dot{W} = 0 \)  

\( 0 = \dot{m} \left( h_5 - h_6 + \frac{w_5^2 - w_6^2}{2} \right) \)  

\( -\frac{w_6^2}{2} = h_5 - h_6 - W_{56} \)  

\( W_6 = \sqrt{2 \left( h_5 - h_6 - W_{56} \right) - w_5^2} \)  

\( W_6 = 2 c_p (T_5 - T_6) - 2 h_{56} + \frac{w_5^2}{2} \)  

\( W_6 = 2299 \)  

\( W_{56} = \frac{R (T_5 - T_6)}{1 - n} \)  
\( W_{56} = -79.6 \, kJ \)  

\( n = 1.4 \)  

\( R = c_p - c_v \)  
\( R = c_p \left( 1 - \frac{1}{k} \right) = 0.2874 \, kJ/kgK \)