\( \dot{Q}_{aus} = 65 \, \text{kW} \)  

\( \overline{T}_{KF} = \frac{\dot{Q}_{aus}}{S_{aus} - S_{ein}} \)  

\( T \cdot dS = dU - p \cdot dV = dH \)  
\( dH = U + p \cdot dV \)  

\( \overline{T}_{KF} = \frac{S_{aus} - S_{ein}}{S_{aus} - S_{ein}} = \frac{h_{aus} - h_{ein}}{S_{aus} - S_{ein}} = C \cdot (T_{aus} - T_{ein}) \)  

\( \overline{T}_{KF} = \frac{(T_{aus} - T_{ein})}{\mu \cdot \ln \left( \frac{T_2}{T_1} \right)} = \frac{T_{aus} - T_{ein}}{\ln \left( \frac{T_2}{T_1} \right)} = 293.1226 \, \text{K} \)