\( h_1 = h_4, x_4 = 0, p_4 = 8 \, \text{bar} \)  
\( h_2 = h_4 = 93.62 \, \text{kJ/kg} \, \text{A11} \)  

\( x_1 = ??? \)  
\( h_1 = h_f + x(h_g - h_f) \)  
â†’ \( h_1 - h_f \)  
\( h_g - h_f = x_1 = \frac{46}{0.1647} \)  

\( h_g @ 92^\circ \text{C} \, \text{A10} \)  
\( h_g = 254.03 - 251.80 (9 - 8) + 251.80 = 252.34 \, \text{kJ/kg} \)  

\( h_f @ 92^\circ \text{C} \, \text{A10} \)  
\( h_f = 66.18 - 60.73 (9 - 8) + 60.73 = 62.093 \, \text{kJ/kg} \)  

\( x_1 = \frac{h_1 - h_f}{h_g - h_f} = x_1 = 0.1647 \)