\( x_{Eis} = \frac{Q - Q_F}{m_g - Q_F} \)  
= \( \frac{u_2 - u_F}{m_g - u_F} \)  
= \( \frac{-185.090 \, \text{kJ} + 333.458 \, \text{kJ}}{-333.458 + 0.0945} \)  

**Zustand 1:**  
0.06 kg Eis  
0.09 kg Wasser  

\( u_1 = -333.458 \, \frac{\text{kJ}}{\text{kg}} \cdot 0.06 \, \text{kg} - 0.0945 \, \frac{\text{kJ}}{\text{kg}} \cdot 0.09 \, \text{kg} \)  
= -20.009 kJ  

\( Q_{12} = \Delta U = u_2 - u_1 \)  
\( u_2 = Q_{12} + u_1 = -185.090 - 20.0097 \)  
= -185.090 kJ  

\( u_2 = \frac{u_m}{m} = -185.090 \, \frac{\text{kJ}}{\text{kg}} \)  

\( X = \frac{u_2 - u_{Wasser}}{u_{Eis}} \)  
= \( \frac{-185.090 + 0.0945}{-333.458 + 0.0945} \)  
= 0.555