\( m_{EW} = m_{W2} + m_{E2} \)  
\( m_{E2} = m_{EW} - m_{W2} \)  

\( m_{W1} U_{2,W} + m_{E1} U_{2,E} = m_{W2} U_{2,W} + m_{E2} U_{2,E} \)  
\( = Q_{12} \)  

\( m_{W1} = 0.4 \, m_{EW} = 0.04 \, \text{kg} \)  
\( m_{E1} = 0.6 \, m_{EW} = 0.06 \, \text{kg} \)  

\( U_{2,W} = -0.045 \, \text{kJ/g} = U_{2,W} \)  
\( U_{2,E} = 333.458 \, \text{kJ/g} = U_{12,E} \)  

\( m_{W2} U_{2,W} + (m_{EW} - m_{W2}) U_{2,E} \)  
\( = m_{W1} U_{W1} + m_{E1} U_{E1} + Q_{12} \)  

\( m_{W2} (U_{2,W} - U_{2,E}) = m_{W1} U_{W1} + m_{E1} U_{E1} + Q_{12} - m_{EW} U_{2,E} \)  

\( m_{W2} = 0.044483 \, \text{kg} \)  
\( m_{E2} = 0.0556 \, \text{kg} \)  

\( x_{E2} = 0.555 \)