\( p_{g,1} = p_{amb} + \frac{32 \, \text{kg} \cdot 5.51 \, \text{m/s}^2}{\pi \cdot (0.1 \, \text{m})^2} + \frac{0.1 \, \text{kg} \cdot 5.81 \, \text{m/s}^2}{\pi \cdot (0.1 \, \text{m})^2} \)  

\( m_g = \frac{p_g \cdot V}{R \cdot T} = \frac{p_{g,1} \cdot V_{g,1}}{R \cdot T_{g,1}} \)  

\( m_g = \frac{\text{(expression crossed out)}}{\text{(expression crossed out)}} = 44.37 \, \text{kg} \)  

\( p_{g,1} = 1.4 \, \text{bar} \)  

\( m_{g,s} = 0.003242 \, \text{kg/s} \)  

\( m_s = 3.92 \, \text{s} \)  

---