The equation for \( w_6 \):  
\( h_6 = h_5 - \frac{w_6^2}{2} \quad \text{and} \quad h_5 = h_6 + \frac{w_6^2}{2} \)  
\( w_6 = \sqrt{2 \cdot \left( h_5 - h_6 \right) + w_5^2} \)  
\( w_6 = \sqrt{2 \cdot \left( c_p \cdot \left( T_5 - T_6 \right) \right) + w_5^2} \)  
\( w_6 = \sqrt{2 \cdot \left( 1.006 \cdot \left( 431.9 - 83.79 \right) \cdot \frac{1 \, \text{kJ}}{1 \, \text{kg} \cdot \text{K}} \right) + 220^2} \)  
\( w_6 = \sqrt{2 \cdot \left( 1.006 \cdot 348.11 \cdot \frac{1 \, \text{kJ}}{1 \, \text{kg} \cdot \text{K}} \right) + 220^2} \)  
\( w_6 = \sqrt{2 \cdot 350.27 + 220^2} \)  
\( w_6 = \sqrt{700.54 + 48400} \)  
\( w_6 = \sqrt{49100.54} \)  
\( w_6 = 320.78 \, \text{m/s} \)