\( T_{g,2} = 90^\circ \text{C} \)  

LHS:  
\( \Delta U_{12,\text{EW}} = Q - W = (7.36 \, \text{kJ} - 0.2852 \, \text{kJ}) \, \text{kJ} = 7.052 \, \text{kJ} \)  

\( \Delta U_{12} = m_{\text{EW}} (u_2 - u_1) \)  

\( u_2 = x_2 \, u_f(0^\circ \text{C}) + (1 - x_2) \, u_f(0^\circ \text{C}) \)  

\( u_1 = u_f(0^\circ \text{C}) (1 - x_1) + u_f(0^\circ \text{C}) x_1 \), \( x_1 = 0.6 \)  

\( m_{\text{EW}} (u_2 - u_1) = x_2 (u_f(T_1) - u_f(T_2)) + u_f(T_2) - u_f(T_1) = \Delta U_{12} \)  

\( x_2 = \frac{\Delta U_{12} + u_1 - u_f(T_2)}{u_f(T_1) - u_f(T_2)} \)  

\( x = \frac{7.052 \, \text{kJ}}{0.1 \, \text{kg}} - (0.085 \, \text{kJ/kg}) \, 0.6 \, (-333.552 \, \text{kJ/kg}) - (-0.053 \, \text{kJ/kg}) \)  

\( x = \frac{-333.452 \, \text{kJ/kg} - (-0.053 \, \text{kJ/kg})}{(-333.552 \, \text{kJ/kg})} \)  

\( = 0.575 \)