Reversible adiabatic isentropic equation:  
\( p_6 = p_5 \)  

\( \frac{T_6}{T_5} = \left( \frac{p_6}{p_5} \right)^{\frac{n-1}{n}} \)  

\( T_6 = T_5 \cdot \left( \frac{p_6}{p_5} \right)^{\frac{n-1}{n}} \)  

\( T_6 = 431.3 \, \text{K} \cdot \left( \frac{0.831}{0.5} \right)^{\frac{0.4}{1.4}} = 328.07 \, \text{K} = T_6 \)  

---

Steady-state balance:  
\( 0 = \dot{m} \cdot \left[ h_e - h_a + \frac{w_e^2}{2} - \frac{w_a^2}{2} \right] \)  

Adiabatic: \( \dot{Q} = 0 \)  

\( (h_5 - h_6) = c_p \cdot (T_5 - T_6) = 1.006 \, \text{kJ/kgÂ·K} \cdot (431.3 \, \text{K} - 328.07 \, \text{K}) = 104.45 \, \text{kJ/kg} \)  

\( w_a = \sqrt{\frac{104.45 \, \text{kJ/kg}}{2} + (220 \, \text{m/s})^2} \)  

\( w_a = 390.96 \, \text{m/s} \)