\( e_{x,str} = (h_6 - h_0 - T_0 (s_6 - s_0) + \frac{w_6^2}{2}) \)  

\( c_v = c_p - \frac{R}{M} \)  
\( R = \frac{\bar{R}}{M} = 288.982 \, \frac{\text{J}}{\text{kg·K}} \)  
\( c_v = 715.01 \, \frac{\text{J}}{\text{kg·K}} \)  

\( s_6 - s_0 = \int_{T_0}^{T_6} \frac{c_p}{T} \, dT - R \cdot \ln \left( \frac{p_6}{p_0} \right) \)  
\( s_6 - s_0 = c_p \left( \ln(T_6) - \ln(T_0) \right) - R \cdot \ln \left( \frac{p_6}{p_0} \right) \)  

\( s_6 - s_0 = 301.361 \, \frac{\text{J}}{\text{kg·K}} \)  

\( e_{x,str} = 156239.168 \, \frac{\text{J}}{\text{kg}} \)