\( ex_{verl} = T_0 \cdot \dot{S}_{erz} \)  

\( \dot{S}_{erz} = S_6 - S_5 \)  

\( S_6 = S(431.9 \, \text{K}) \cdot c \)  

\( S_5 = S(250 \, \text{K}) \cdot c \)  

\( S_6 = S(431.9 \, \text{K}) - S(250 \, \text{K}) \cdot c \)  

\( = S(250 \, \text{K}) \cdot 5.10 - S(250 \, \text{K}) - S(431.9 \, \text{K}) \cdot c \)  

\( = \)  

\( S_6 = 1.494 \, \text{kJ/kg路K} \quad \rightarrow \text{in 2c calculated/interpolated} \)  

\( S_5 = 1.752 \, \text{kJ/kg路K} \quad \rightarrow \text{in 2c calculated/interpolated} \)  

\( ex_{verl} = T_0 \cdot (S_6 - S_5) \)  

\( = 283.15 \, \text{K} \cdot (1.494 \, \text{kJ/kg路K} - 1.752 \, \text{kJ/kg路K}) \)  

\( ex_{verl} = -73.126 \, \text{kJ/kg} \)  

\( \underline{ex_{verl} = -73.126 \, \text{kJ/kg}} \)