a) Given: \( \dot{Q}_{out} \)  

Stationary flow process:  
0 = \( \dot{m}_{in} \cdot (h_e - h_a) + \frac{w_e^2 - w_a^2}{2} + g \cdot (z_e - z_a) + \sum \dot{Q}_j - \sum \dot{W}_j \)  

<< 0 = \( \dot{m}_{in} \cdot (h_e - h_a) + \sum \dot{Q}_j \)  

0 = \( \dot{m}_{in} \cdot (h_e - h_a) + \dot{Q}_R - \dot{Q}_{out} \)  

=> \( \dot{Q}_{out} = \dot{m}_{in} \cdot (h_e - h_a) + \dot{Q}_R \)  
= \( \dot{m}_{in} \cdot (292.98 \, \text{kJ/kg} - 419.04 \, \text{kJ/kg}) + \dot{Q}_R \)  
= \( 0.3 \, \text{kg/s} \cdot (292.98 \, \text{kJ/kg} - 419.04 \, \text{kJ/kg}) + 100 \, \text{kW} \)  
= \( 62.182 \, \text{kJ/s} = 62.182 \, \text{kW} \)  

Values for \( h_f \) come from Table A2!