m_EW (u_2 - u_1) + m_g (u_2 - u_1) = Q̇ = 0  

p_g = p_EW  

u_2EW = u_f = -333.638 kilojoules per kilogram + (0.05 kilograms per kilogram × 333.638 kilojoules per kilogram) = -333.61 kilojoules per kilogram  

m_g (u_2 - u_1) = m_g c_V (T_2 - T_1) = -1.082 kilojoules  

u_2EW = u_f + m_g (u_2 - u_1) / m_EW = -122.55 kilojoules per kilogram  

p_2EW = p_1EW = 1.48 bar  

T_1EW = T_2EW  

x = u_2EW + 333.638 kilojoules per kilogram / (-0.05 kilograms per kilogram + 333.638 kilojoules per kilogram) = 0.632