\( \dot{S}_{\text{erz}} = ? \)  

\[ 
\text{[steady-state]} \quad 0 = \dot{m}_{\text{in}} (s_e - s_a) + \dot{m}_{\text{aus}} (s_e - s_a) + \frac{\dot{Q}_{\text{aus}}}{\bar{T}_{\text{KW}}} + \dot{S}_{\text{erz}} 
\]  

\[ 
\dot{S}_{\text{erz}} = 2 \dot{m}_{\text{in}} (s_a - s_e) - \frac{\dot{Q}_{\text{aus}}}{\bar{T}_{\text{KW}}} 
\]  

\[ 
\dot{S}_{\text{erz}} = 2 \cdot 0.3 \, \text{kg/s} \cdot (0.36 - 0.2265) \, \text{kJ/kg·K} - \frac{65 \, \text{kW}}{293 \, \text{K}} 
\]  

\[ 
\dot{S}_{\text{erz}} = -0.356 \, \text{kW/K} 
\]  

Additional notes:  
\( s_a = s_g (15^\circ \text{C}) = 0.2265 \, \text{kJ/kg·K} \)  
\( s_e = s_g (25^\circ \text{C}) = 0.36 \, \text{kJ/kg·K} \)  
\( \frac{\dot{Q}_{\text{aus}}}{\bar{T}} = \text{heat removed} \)