\( \Delta S_{12} = m_2 \cdot (S_2 - S_1) \rightarrow S_1 = S_f(100^\circ \text{C}) + x_D \cdot (S_g(100^\circ \text{C}) - S_f(100^\circ \text{C})) \)  
\( S_f = 3.306 \, \frac{\text{kJ}}{\text{kg·K}} + 0.005 \cdot (7.3589 - 3.306) \, \frac{\text{kJ}}{\text{kg·K}} = 1.3374 \, \frac{\text{kJ}}{\text{kg·K}} \)  
\( S_2 = S_f(20^\circ \text{C}) = 0.3549 \, \frac{\text{kJ}}{\text{kg·K}} \)  
\( m_2 = m_{gas} = m_{ges} + \Delta m_{12} = 5755 \, \text{kg} + 3600 \, \text{kg} = 9355 \, \text{kg} \)  
\( \Delta S_{12} = 9355 \, \text{kg} \cdot (0.5549 \, \frac{\text{kJ}}{\text{kg·K}} - 1.3374 \, \frac{\text{kJ}}{\text{kg·K}}) = -3575 \, \frac{\text{kJ}}{\text{K}} \)