\( m_2 \cdot u_2 - m_1 \cdot u_1 = \Delta m_{12} \cdot h_{ein} + Q_{R,12} \)  
\( \rightarrow m_2 \cdot u_2 = m_1 \cdot u_1 + Q_{R,12} - \Delta m_{12} \cdot h_{ein} \)  
\( u_2 = u_f(70^\circ \text{C}) = 292.95 \, \frac{\text{kJ}}{\text{kg}} \)  
\( u_1 = u_f(100^\circ \text{C}) + x_D \cdot (u_g(100^\circ \text{C}) - u_f(100^\circ \text{C})) = 419.34 \, \frac{\text{kJ}}{\text{kg}} \)  
\( h_{ein} = h_f(20^\circ \text{C}) = 83.96 \, \frac{\text{kJ}}{\text{kg}} \)  
\( \Delta m_{12} = \frac{Q_{R,12} - m_1 \cdot (u_2 - u_1)}{h_{ein}} = \frac{35,000 \, \text{kJ} - 5755 \, \text{kg} \cdot (292.95 - 419.34) \, \frac{\text{kJ}}{\text{kg}}}{83.96 \, \frac{\text{kJ}}{\text{kg}}} = 332.4 \, \text{kg} \)