\( 0 = \dot{m}(S_{ein} - S_{aus}) + Z \frac{\dot{Q}}{T} + \dot{S}_{erz} \).  
\( -\dot{S}_{erz} = \dot{m}(S_{ein} - S_{aus}) - \frac{\dot{Q}_{R}}{T_{R}} + \frac{\dot{Q}_{aus}}{T_{KF}} \).  

\( T = T_{R} \):  
\( S_{ein} = S_{f}(@70^\circ \text{C}) \cdot x_{D} = 0.988 \, \text{kJ/kg路K} \).  
\( S_{aus} = S_{f}(@100^\circ \text{C}/x_{D}) = 1.3371 \, \text{kJ/kg路K} \).  

\( S_{ein} - S_{aus} = S_{f}@70^\circ \text{C} - S_{f}@100^\circ \text{C} = 0.95479 - 1.3069 = -0.06 \, \text{kJ/kg路K} \).  

\( \dot{S}_{erz} = 0 = \dot{m}(S_{ein} - S_{aus}) + \frac{\dot{Q}}{T} + \dot{S}_{erz} \).  
\( \dot{S}_{erz} = \dot{m}(S_{ein} - S_{aus}) - \frac{\dot{Q}_{R}}{T_{R}} + \frac{\dot{Q}_{aus}}{T_{KF}} \).  
\( \dot{S}_{erz} = 0.057 \, \text{kJ/kg路K} \).