\( \dot{S}_{erz} \)  
\( 0 = \dot{m} [S_e - S_a] + \sum \frac{\dot{Q}}{T} + \dot{S}_{erz} \)  
\( \dot{S}_{erz} = \dot{m} [S_a - S_e] - \sum \frac{\dot{Q}}{T} \)  

\( S_e = S = 0.9549 \, \text{kJ/kgK} \, \text{(A-2)} \)  
\( S_a = 1.3069 \, \text{kJ/kgK} \, \text{(A-2)} \)  

\( \dot{S}_{erz} = 0.3 \, \text{kg/s} \cdot \left[ 1.3069 - 0.9549 \right] + \frac{\dot{Q}_R}{T} \)  
\( \dot{S}_{erz} = 0.3 \, \text{kg/s} \cdot \left[ 1.3069 - 0.9549 \right] + \frac{100 \, \text{kW}}{295 \, \text{K}} \)  
\( \dot{S}_{erz} = 0.326 \, \text{kg/s} \cdot \text{kJ/kgK} \)

---