\( m_2 s_2 - m_1 s_1 = \Delta m_{12} s_{in} + \frac{Q_{out}}{T_{out}} - \frac{Q_{out}}{T_{mean}} + S_{erz} \)  

\( s_2 = s_f(70^\circ C) = 0.9549 \, \text{kJ/kg路K} \)  

\( s_1 = s_f(100^\circ C) + x_D (s_g(100^\circ C) - s_f(100^\circ C)) = 1.33714 \, \text{kJ/kg路K} \)  

\( s_{in} = s_f(20^\circ C) = 0.296 \, \text{kJ/kg路K} \)  

\( T_{mean} = \frac{q_{rev}}{s_2 - s_{in}} = \frac{q_{rev}}{s_2 - s_{in}} = \frac{Q_{out}}{s_2 - s_{in}} = \frac{35,450,000 \, \text{kJ}}{(0.954 - 1.33714) \, \text{kJ/kg路K}} \)  

\( T_{out} = 285 \, \text{K} \, \text{(from b)} \)  

\( S_{erz} = m_1 s_1 - m_2 s_2 - \Delta m_{12} s_{in} - \frac{Q_{out}}{T_{in}} + \frac{Q_{out}}{T_{mean}} \)