\( h_6 - h_0 = \int c_p \, dt = c_p (T_5 - T_0) = 1.006 \, \text{kJ/kgK} \, (431.9 \, \text{K} - 258.0 \, \text{K}) = 174.15 \, \text{kJ/kg} \)

\( w_6 = \sqrt{2(h_6 - h_0)} + w_5^2 \)  
\( w_6 = \sqrt{2 \cdot 104.45 \cdot 10^3 \, \text{J/kg} \, (200 \, \text{m/s})^2} = 498.80 \, \text{m/s} \)

\( e_{K,spezifisch} - e_{x,str,0} = \frac{1}{2} w_6^2 - T_0 (s_6 - s_0) + k_e,6 - k_e,0 \)

\( h_6 - h_0 = c_p (T_6 - T_0) = 1.006 \, \text{kJ/kgK} \, (328.0 \, \text{K} - 243.15 \, \text{K}) = 85.43 \, \text{kJ/kg} \)

\( s_6 - s_0 = c_p \ln \left( \frac{T_6}{T_0} \right) - R \ln \left( \frac{p_6}{p_0} \right) \)  
\( s_6 - s_0 = 1.006 \, \text{kJ/kgK} \ln \left( \frac{328.0}{243.15} \right) - 0.30 \, \text{kJ/kgK} \)

\( \Delta e_{x,str} = k_e,0 = \frac{1}{2} w_0^2 \)

\( \Delta e_{x,str} = 85.43 \, \text{kJ/kg} - 243.15 \, \text{K} (0.3 \, \text{kJ/kgK}) + \left( \frac{498.80 \, \text{m/s} - (200 \, \text{m/s})^2}{2} \right) \)

\( = 146.63 \, \text{kJ/kg} \)

---