Exergy loss \( ex_{verl} \):  

Exergy balance equation:  
\[
\frac{d ex_{str}}{dt} = \sum \dot{ex}_{str} + \sum \dot{Q} \cdot \left(1 - \frac{T_0}{T}\right) - \sum \dot{W} - \rho \cdot \frac{\partial ex_{str}}{\partial t} - ex_{verl} \cdot \dot{m}
\]  

Simplified for steady-state and adiabatic conditions:  
\[
C = ex_{str} - W - ex_{verl}
\]  

Rearranging:  
\[
ex_{verl} = ex_{str} - W
\]  

Energy balance equation:  
\[
0 = \dot{m} \cdot \left(h + \frac{w^2}{2} + \text{potential energy}\right) + \sum \dot{Q} - \sum \dot{W}
\]