\( m_2 \cdot s_2 - m_1 \cdot s_1 = \Delta m_{12} \cdot s_\text{ein} + \frac{Q}{T} + S_{erz} \)  

\( \Delta S_{12} = m_2 \cdot s_2 - m_1 \cdot s_1 - \Delta m_{12} \cdot s_\text{ein} \)  

State 2:  
\( s_2 = s_\text{f}(70^\circ \text{C}) = 0.3548 \, \frac{\text{kJ}}{\text{kg·K}} \)  

State 1:  
\( s_1 = s_\text{f}(100^\circ \text{C}) + x_1 \cdot (s_\text{fg}(100^\circ \text{C}) - s_\text{f}(100^\circ \text{C})) = 1.35741 \, \frac{\text{kJ}}{\text{kg·K}} \)  

\( s_\text{ein} = s_\text{f}(20^\circ \text{C}) = 0.2966 \, \frac{\text{kJ}}{\text{kg·K}} \)  

\( \Delta S_{12} = 162.8 \, \frac{\text{kJ}}{\text{K}} \)