\( T_{KF} = \frac{\int T \, dS}{S_{out} - S_{in}} \)  

\( S = c_p \cdot \ln \left( \frac{T}{T_e} \right) \)  
\( T = T_e \cdot e^{\frac{S - S_e}{c_p}} \)  

Further derivations and equations are shown, including:  
\( T_{KF} = T_e \cdot e^{\frac{S_e}{c_p}} \cdot \int e^{\frac{-S}{c_p}} \, dS \)  
\( = T_e \cdot e^{\frac{S_e}{c_p}} \cdot \frac{e^{\frac{-S}{c_p}}}{c_p \cdot \ln \left( \frac{T_{out}}{T_{in}} \right)} \)  

\( S - S_e = c_p \cdot \ln \left( \frac{T}{T_e} \right) \)  
\( T = T_e \cdot e^{\frac{S - S_e}{c_p}} \)  

Final expression is left incomplete with an underline.