\( x_{\text{Ice},2} = \frac{m_{\text{Ice}}}{m_{\text{EW}}} \)  

\( m_{\text{tot}} = 0.1 \, \text{kg} \)  

\( \Delta U + h = 0 \)  

\( \Delta U_1 = \Delta U_2 \)  

\( \Delta U_1 = 3.16 \times 4.78 + U_{1,h} = U_{2,h} \)  

\( -83.442 - \Delta q + U_{\text{EW}} = U_{\text{EW}} \)  

\( Q_{12} = -3.16 \times 4.78 + 1 - 0.645 + 0.6(-333.185 + 0.645) = -546.56 \, \text{kJ} \)  

\( U_{\text{EW}} - U_{Ice} \)  

\( U_{\text{Ice}} - U_{Ice} \)  

From Table 1:  

\( x_{\text{Ice},2} = \frac{-546.56 + 0.083}{-333.442 + 0.083} = \)  

\( \Delta U \rightarrow \Delta U_{12} = G_{12} + h_{12} \)  

\( \Delta U_{12} = \frac{1500 \, \text{J}}{m} \rightarrow U_2 = \frac{1500}{m} + U_1 \)  

\( U_2 = U_{\text{FL}} + x_2(U_{\text{fg}} - U_{\text{FL}}) \)  

\( U_1 = -0.645 + 0.6(-333.185 + 0.645) = -200.083 \)  

\( x_2 = \frac{Q_{12} + U_1 - U_{\text{FL}}}{U_{\text{fg}} - U_{\text{FL}}} = \frac{-1500 \, \text{J}}{0.1 \, \text{kg}} - 200.083 + 0.645}{-333.442 + 0.645} \)  

\( \rightarrow x_{\text{Ice},2} \neq 1 \, \text{(higher than 0.6 since temperature rises)} \)