\( T_1 = 100^\circ \text{C} \rightarrow \Delta T = 30 \, \text{K} \)  
\( Q_R = Q_{out} = 35 \, \text{MJ} \)  
\( u_f(100^\circ \text{C}) = 419.94 \, \text{kJ/kg} \)  
\( u_g(100^\circ \text{C}) = 2506.5 \, \text{kJ/kg} \)  

\( x_D = 0.005 \rightarrow m_{D} = x_D \cdot m_{total} = 28.775 \, \text{kg} \)  

\( c_p = u_f + 0.005 \cdot (u_g - u_f) = 420.3788 \, \text{kJ/kg} \)  

\( u_2 = u_f(70^\circ \text{C}) = 293.25 \, \text{kJ/kg} \)  
\( u_3 = 93.95 \, \text{kJ/kg} \)  

\( \rightarrow \Delta m \)  

\( -m_{total} \cdot u_1 + u_3 \cdot m_{gas} + u_g \cdot m_D = Q_{out} \)  

\( m_{gas} + \Delta m \cdot u_2 = m_{gas} \cdot u_1 - \Delta m \cdot u_3 = Q_{out} \)  

\( Q_{out} = m_{gas} \cdot u_2 + m_{gas} \cdot u_1 = \Delta m \cdot (u_2 - u_3) \)  

\( \Delta m = \frac{Q_{out} - m_{gas} \cdot u_2 + m_{gas} \cdot u_1}{u_2 - u_3} \)  

\( \Delta m = \frac{35 \, \text{MJ}}{293.25 - 93.95} = 358.9106 \, \text{kg} \)  

---