The equation for \( h_a \):  
\( h_a = \int_{T_0}^{T_6} c_p \, \text{dT} \)  

Simplified:  
\( h_a = c_p \cdot (T_6 - T_0) \)  

Substituting values:  
\( h_a = 1.006 \cdot (328.07 - (-30)) \)  

Result:  
\( h_a = \text{value not calculated on the page} \)

\( e_{x,str,6} = h_6 - h_0 - T_0 \cdot (s_6 - s_0) + \frac{w_6^2 - w_0^2}{2} \)  
\( e_{x,str,6} = h_6 - h_0 - T_0 \cdot (s_6 - s_0) + \frac{w_6^2}{2} \)  
\( h_6 - h_0 = \int c_p \, dT = c_p \cdot (T_6 - T_0) \)  
\( T_0 = 243.15 \, \text{K} \)  

\( s_6 - s_0 = \int \frac{c_p}{T} \, dT - R \cdot \ln \left( \frac{p_6}{p_0} \right) = 90 \cdot \ln \left( \frac{p_6}{p_0} \right) - 90 \cdot \ln \left( \frac{p_0}{p_6} \right) - 0 \)  

\( e_{x,str,6} = 133.6 - \frac{w_6^2}{2} \)  

\( s_0 (243.15 \, \text{K}) = s_0 (293.07 \, \text{K}) - \frac{90 \cdot (330 \, \text{K} - 293 \, \text{K})}{5 \, \text{K}} \)  
\( s_0 (243.15 \, \text{K}) = s_0 (293.07 \, \text{K}) - 2 \cdot \frac{90}{5} \)