First law of thermodynamics:  
ΔE = Σm_i (h_i + ke_i + pe_i) + ΣQ̇ - ΣẆ_in  

→ ΔE = m_total Δu + Δke + Δpe  
→ Δu = m_total (u_2 - u_1) = Δm_12 h_in + Q_R12  

u_1 from Table A-2: u_1 = u_f (T_1) + x_D (m_D / m_total) u_fg (T_1)  
u_1 = 429.384 kJ/kg  

u_2 from Table A-2: u_2 = 292.95 kJ/kg

Write: \( h_{in} \) as TAB-A2: \( h_{in} = 83.896 \, \text{kJ/kg} \)  

\[
\rightarrow m_{ges,1} (u_2 - u_1) + \Delta m_{12} u_2 = \Delta m_{12} h_{in} + Q_{R,12}
\]  

\[
\rightarrow \Delta m_{12} = \frac{m_{ges,1} (u_2 - u_1) - Q_{R,12}}{h_{in} - u_2}
\]  

\[
= 3923.45 \, \text{kg}
\]  

---