\( p_{g,1} \), \( m_g \)  

\( p_{g,1} = p_0 + \frac{F_{mew}}{A} + \frac{F_{mew}}{A} = p_0 + \left( \frac{32 \, \text{kg} \cdot 9.81 \, \text{m/s}^2 + 0.1 \, \text{kg} \cdot 5.81 \, \text{m/s}^2}{\pi \left( \frac{D}{2} \right)^2} \right) \)  

\( p_{g,1} = 1.10054 \, \text{bar} \)  

\( pV = mRT \rightarrow m_g = \frac{p_{g,1} V_{g,1}}{R T_{g,1}} = \frac{1.4 \, \text{bar} \cdot 3.14 \cdot 10^{-3} \, \text{m}^3}{8.31 \, \text{J/molÂ·K} \cdot 773.15 \, \text{K}} \)  

\( m_g = 0.00342 \, \text{kg} = 3.42 \, \text{g} \)  

---