\( t_{ice,2} = t_{ice,1} = 0.003^\circ C \)  

\( \Delta E = E_2 - E_1 = Q_{12} = 1500 \, J \)  

\( \Delta u_{12} = \frac{1500 \, J}{m} = m \cdot (u_2 - u_1) = m \cdot \left[ (x_2 \cdot u_{2,ice} + (1 - x_2) \cdot u_{2,flüssig}) - (x_1 \cdot u_{1,ice} + (1 - x_1) \cdot u_{1,flüssig}) \right] \)  

\( \Delta u_{12} = \frac{\Delta u_{12}}{m} + (x_1 \cdot u_{1,ice} + (1 - x_1) \cdot u_{1,flüssig}) = x_2 \cdot u_{2,ice} + (1 - x_2) \cdot u_{2,flüssig} \)  

\( x_2 = \frac{\Delta u_{12}}{m} + (x_1 \cdot u_{1,ice} + (1 - x_1) \cdot u_{1,flüssig}) - u_{2,flüssig} \)  
\( \div (u_{2,ice} - u_{2,flüssig}) \)  

\( x_2 = 0.555 \)