\( \Delta ex_{\text{str}} = \dot{m} \left[ h - h_0 - T_0 (s - s_0) + k_e + p_e^0 \right] \)  

\( ex_{\text{str},6} = h_6 - h_0 - T_0 (s_6 - s_0) + \frac{w_6^2}{2} \)  
\( ex_{\text{str},0} = h_0 - h_0 - T_0 (s_0 - s_0) + \frac{w_0^2}{2} \)  

\( \Delta ex_{\text{str}} = h_6 - h_0 - T_0 (s_6 - s_0) + \frac{w_6^2}{2} - \frac{w_0^2}{2} \)  

\( h_6 - h_0 = c_p (T_6 - T_0) \)  
\( s_6 - s_0 = c_p \ln \frac{T_6}{T_0} - R \ln \frac{p_6}{p_0} \)  

\( \Delta ex_{\text{str}} = c_p (T_6 - T_0) - T_0 \left[ c_p \ln \frac{T_6}{T_0} - R \ln \frac{p_6}{p_0} \right] + \frac{w_6^2 - w_0^2}{2} \)  

\( \Delta ex_{\text{str}} = c_p (T_6 - T_0) - c_p T_0 \ln \frac{T_6}{T_0} + c_p T_0 \ln \frac{p_6}{p_0} + \frac{w_6^2 - w_0^2}{2} \)  

\( = 1.006 \, \frac{\text{kJ}}{\text{kgÂ·K}} \left[ (340 \, \text{K} - (-30 + 273.15) \, \text{K}) - (-30 + 273.15) \, \text{K} \ln \frac{340}{-30 + 273.15} \right] + \frac{510^2 - 220^2}{2} \)  

\( = 110.65 + 42.18 \, \frac{\text{kJ}}{\text{kg}} = 110.1 \, \text{MJ/kg} \)