\( \Delta ex_{str} = [h_0 - h_6 - T_0 \cdot (s_0 - s_6) + \frac{w_0^2 - w_6^2}{2}] + (1 - \frac{T_0}{T_B}) \cdot q_B - ex_{verl} \)  

Ideal gas:  
\( h_0 - h_6 = c_p \cdot (T_0 - T_6) = 1.006 \, \text{kJ/kgÂ·K} \cdot (-30^\circ \text{C} - 328 \, \text{K} + 273.15 \, \text{K}) \)  
\( = -85.46 \, \text{kJ/kg} \)  

\( T_0 \cdot (s_0 - s_6) = T_0 \cdot c_p \cdot \ln(\frac{T_0}{T_6}) - R \cdot \ln(\frac{p_0}{p_6}) \)  
\( = -73.3 \, \text{kJ/kg} \)  

\( \Delta ke = \frac{200 \, \text{m/s}^2 - 507.24 \, \text{m/s}^2}{2} = -108.65 \, \text{kJ/kg} \)  

\( (1 - \frac{T_0}{T_B}) \cdot q_B = (1 - \frac{243.15 \, \text{K}}{1289 \, \text{K}}) \cdot 1195 \, \text{kJ/kg} = 806.95 \, \text{kJ/kg} \)  

\( \Delta ex_{str,06} = -85.46 \, \text{kJ/kg} + 73.3 \, \text{kJ/kg} - 108.65 \, \text{kJ/kg} + 806.95 \, \text{kJ/kg} = 681.69 \, \text{kJ/kg} \)  

\( \Delta ex_{str} = -\Delta ex_{str,06} = -681 \, \text{kJ/kg} \)