Reversible adiabatic = isentropic  
First law of thermodynamics:  
0 = \( \dot{m} (h_e + w_e^2 / 2 - h_a - w_a^2 / 2) + \dot{Q} - \dot{W} \)  
\( \dot{Q} = 0 \), \( \dot{W} = 0 \)  

Thus:  
\( h_e + w_e^2 / 2 = h_a + w_a^2 / 2 \)  

Isentropic: \( n = 1.4 \)  

\( T_2 / T_1 = (P_2 / P_1)^{(n-1)/n} \)  
Thus:  
\( T_2 = T_1 (P_2 / P_1)^{(n-1)/n} \)  

\( T_6 = T_5 (P_0 / P_5)^{(n-1)/n} = 328.07 \, \text{K} \)  

\( h_e - h_a = w_a \)  
\( h_e - h_a + w_e^2 / 2 = w_a^2 / 2 \)  
\( w_a = \sqrt{2(h_e - h_a) + w_e^2} \)  

\( h_e - h_a = h_s - h_6 = c_p^{\text{air}} (T_a - T_2) = 1.006 \, \text{kJ/kgK} (431.9 \, \text{K} - 328.07 \, \text{K}) \)  

\( w_a = \)