\( \dot{E}_{\text{verl}} = -\Delta \dot{E}_{\text{str}} + \left( 1 - \frac{T_0}{T_B} \right) \dot{Q}_B \)  

\( \dot{Q}_B = 1195 \, \frac{\text{kJ}}{\text{kg}} \cdot \dot{m}_K \)  
\( \dot{E}_{\text{verl}} = -\Delta \dot{E}_{\text{str}} + \left( 1 - \frac{243.15 \, \text{K}}{1289 \, \text{K}} \right) \cdot \dot{m}_K \)  

\( \dot{E}_{\text{verl}} = -100 \, \frac{\text{kJ}}{\text{kg}} + 0.129 \, \dot{m}_{\text{ges}} \)  

Boxed equations:  
\( \dot{m}_K + \dot{m}_M = \dot{m}_{\text{ges}} \)  
\( \dot{m}_M = 5.293 \, \dot{m}_K \)  
\( \dot{m}_K + 5.293 \, \dot{m}_K = \dot{m}_{\text{ges}} \)  
\( 6.293 \, \dot{m}_K = \dot{m}_{\text{ges}} \)  
\( \dot{m}_K = \frac{1}{6.293} \, \dot{m}_{\text{ges}} \)