\( \Delta ex_{\text{str}} = (h_6 - h_0) - T_0 (s_6 - s_0) \)  
\( \Delta ex_{\text{str}} = c_p^{\text{ig}} (T_6 - T_0) - T_0 \left( c_p^{\text{ig}} \ln \left( \frac{T_6}{T_0} \right) - R \ln \left( \frac{p_6}{p_0} \right) \right) \)  
\( R = 287 \, \frac{\text{J}}{\text{kg路K}} \)  

\( \Delta ex_{\text{str}} = 1.006 \, \frac{\text{kJ}}{\text{kg路K}} (328 \, \text{K} - 243.15 \, \text{K}) - 243.15 \, \text{K} \left( 1.006 \, \frac{\text{kJ}}{\text{kg路K}} \ln \left( \frac{328 \, \text{K}}{243.15 \, \text{K}} \right) - 287 \, \frac{\text{J}}{\text{kg路K}} \ln \left( \frac{p_6}{p_0} \right) \right) \)  

\( \Delta ex_{\text{str}} = 12.74 \, \frac{\text{kJ}}{\text{kg}} \)