\( \Delta ex_{str} = ex_{str,6} - ex_{str,0} \)  
\( \Delta ex_{str} = h_e - h_a - T_0 (s_e - s_a) + \Delta e \)  
\( = h_0 - h_6 - T_0 (s_0 - s_6) + (w_e^2 - w_6^2)/2 \)  

\( h_0 - h_6 = c_p (T_0 - T_6) \)  

\( s_0 - s_6 = - \left( c_p \ln \left( \frac{T_6}{T_0} \right) - R \ln \left( \frac{p_6}{p_0} \right) \right) \)  

\( = - c_p \ln \left( \frac{T_6}{T_0} \right) \)  

\( w_e^2 - w_6^2 = (w_{Luft})^2 / 2 - (w_6)^2 / 2 \)  

\( T_0 = -30^\circ \text{C} = 243.15 \, \text{K} \)  

\( ex_{str} = c_p (T_0 - T_6) - T_0 \left( - c_p \ln \left( \frac{T_6}{T_0} \right) + \frac{(w_e)^2}{2} - \frac{w_6^2}{2} \right) \)  

\( = 1.006 \, \text{kJ/kgK} (243.15 \, \text{K} - 320.0254 \, \text{K}) + 243.15 \, \text{K} \cdot (1.006 \, \text{kJ/kgK} \ln \left( \frac{320.0254}{243.15} \right) + \frac{(200)^2}{2} - \frac{(507.243)^2}{2}) \)  

\( = \) [Expression crossed out]

\( ex_{str} = h_6 - h_0 - T_0 \cdot (s_6 - s_0) + \frac{w_6^2}{2} - \frac{w_0^2}{2} \)  
\( = c_p \cdot (T_6 - T_0) - T_0 \cdot \ln \left( \frac{T_6}{T_0} \right) + \frac{w_6^2}{2} - \frac{w_0^2}{2} \)  
\( = 120.805 \, \frac{\text{kJ}}{\text{kg}} \)