Given:  
\( c_p = 1.006 \, \text{kJ/kgÂ·K} \), \( n = \kappa = 1.4 \)  

\( p_e = p_0 = 0.191 \, \text{bar} = 19.1 \, \text{kPa} \)  
\( w_5 = 220 \, \text{m/s} \), \( p_5 = 0.5 \, \text{bar} \), \( T_5 = 431.9 \, \text{K} \)  

To determine \( T_6 \) using the adiabatic coefficient:  
\( \frac{T_c}{T_5} = \left( \frac{p_c}{p_5} \right)^{\frac{n-1}{n}} \implies T_c = T_5 \cdot \left( \frac{p_c}{p_5} \right)^{\frac{0.4}{1.4}} \)  

\( T_c = 431.9 \, \text{K} \cdot \left( \frac{0.191 \, \text{bar}}{0.5 \, \text{bar}} \right)^{\frac{0.4}{1.4}} = 328.07 \, \text{K} \)  

---

\( w_6 \): Steady flow process in an adiabatic reversible nozzle:  
\( 0 = \dot{m} \left[ h_5 - h_6 + \frac{(w_5)^2 - (w_6)^2}{2} + p_e \cdot v_e + q_e - w_e \right] \)  
\( 0 = h_5 - h_6 + \frac{w_5^2 - w_6^2}{2} \)  

Using \( h_5 - h_6 = c_p \cdot \Delta T = c_p \cdot (T_5 - T_6) \):  
\( c_p \cdot (T_5 - T_6) = \frac{w_5^2 - w_6^2}{2} \)  

Rearranging:  
\( c_p \cdot (T_5 - T_6) + \frac{w_5^2}{2} = \frac{w_6^2}{2} \)  
\( w_6^2 = 2 \cdot c_p \cdot (T_5 - T_6) + w_5^2 \)  

Substituting values:  
\( w_6 = \sqrt{2 \cdot 1.006 \cdot (431.9 - 328.1) + 220^2} \, \text{m/s} \)  

\( w_6 \approx 507.2 \, \text{m/s} \)  

(Note: A crossed-out calculation is ignored.)