\( m_{\text{gas}} (u_2, \text{Eis} - u_1, \text{Gas}) = -Q \)  

\( u_1, \text{Gas} = u_{\text{flüssig}} (1 \, \text{bar}) + x_{\text{Eis}} \cdot (u_{\text{fest}} (1 \, \text{bar}) - u_{\text{flüssig}} (1 \, \text{bar})) \)  

\( u_{\text{flüssig}} (1 \, \text{bar}) = -0.045 \, \text{kJ/kg} \)  
\( u_{\text{fest}} (1 \, \text{bar}) = 333.458 \, \text{kJ/kg} \)  

\( m_{\text{gas}} \cdot u_2, \text{Eis} = -18.875 \, \text{kJ} \)  

\( u_2, \text{Eis} = -188.75 \, \text{kJ/kg} \)  

\( x_2, \text{Eis} = \frac{u_2, \text{Eis} - u_{\text{flüssig}} (1 \, \text{bar})}{u_{\text{fest}} (1 \, \text{bar}) - u_{\text{flüssig}} (1 \, \text{bar})} = 0.566 \)