\( T_{KF} = \frac{T_2 - T_A}{\ln \frac{T_aus - T_ein}{T_2 - T_A}} = \frac{T_{aus} - T_{ein}}{\ln \frac{T_2 - T_A}{T_2 - T_A}} = 85.227^\circ C \)  

\( T_{KF} = 358.377 \, \text{K} \)  

\( s_{aus} (x = 0, 100^\circ C) = s_f = 1.3069 \, \text{kJ/kg·K} \)  

\( s_{ein} (x = 0, 70^\circ C) = s_f = 0.9549 \, \text{kJ/kg·K} \)  

---

\( T_{KF} = \frac{T_{KF,aus} - T_{KF,ein}}{S_{aus} - S_{ein}} = \frac{T_{KF,aus} - T_{KF,ein}}{\ln\left(\frac{T_2}{T_1}\right)} = 293.121 \, \text{K} \)  

\( S_{aus} - S_{ein} = \ln\left(\frac{T_2}{T_1}\right) \)