\( s_5 - s_6 \)  
\( s(T = 431.9 \, \text{K}) = \)  

\( s_6 - s_5 = 0 = s^\circ(T_6) - s^\circ(T_5) - R \cdot \ln\left(\frac{p_6}{p_5}\right) \)  

\( s^\circ(T_6) = s^\circ(T_5) + R \cdot \ln\left(\frac{p_6}{p_5}\right) \)  

\( s^\circ(T_5 = 431.9 \, \text{K}) = 21.06533 \, \text{kJ/kg·K} \)  

\( \text{TAB A-22} \)  

\( = 21.06977 \, \text{kJ/kg·K} \)  

\( s^\circ(T_6) = s^\circ(T_5) \)  

\( s^\circ(T_6) = 21.06977 \, \text{kJ/kg·K} + \frac{8.314 \, \text{kJ/kmol·K}}{28.97 \, \text{kg/kmol}} \cdot \ln\left(\frac{0.15}{0.1}\right) \)  

\( = 1.79364 \, \text{kJ/kg·K} \)  

\( T_6(s^\circ(T_6)) = 325 \, \text{K} + \frac{(330 - 325) \, \text{K}}{(1.7936 - 1.78249) \, \text{kJ/kg·K}} \cdot (1.7936 - 1.78241) \, \text{kJ/kg·K} \)  

\( = 328.62 \, \text{K} \)