\( e_{x,str,6} - e_{x,str,0} = (h_6 - h_0 - T_0(s_6 - s_0) + \frac{w_6^2}{2}) - (h_5 - h_0 - T_0(s_5 - s_0) + \frac{w_5^2}{2}) \)  
= \( \int c_p dT - T_0 \int \frac{c_p}{T} dt - R \ln \left(\frac{p_6}{p_5}\right) + \frac{w_6^2 - w_5^2}{2} \)  

\( R = c_p - c_v = \frac{c_p}{c_p - c_p \kappa} = 0.287492 \, \text{kJ/kgÂ·K} \)  

\( T_0 = 293.15 \, \text{K} \)  

\( \Delta e_{x,str} = c_p(T_6 - T_5) - T_0 c_p \ln \left(\frac{T_6}{T_5}\right) - T_0 R \ln \left(\frac{p_6}{p_5}\right) + \frac{w_6^2 - w_5^2}{2} \)  
= \( -109.95 - 67.26 - 67.255 + 174.437 \)  
= \( -167.97 \, \text{kJ/kg} \)