\( m_2 u_2 - m_1 u_1 = \Delta m_{12} h_{12} + Q_R \)  
\( m_1 = 5755 \, \text{kg} \)  
\( m_2 = 5755 + \Delta m \)  

\( u_2 = u_f + x (u_g - u_f) \)  
\( u_2 (100^\circ \text{C}) = 478.94 + 0.005 (2506.5 - 478.94) \)  
\( = 429.3778 \, \frac{\text{kJ}}{\text{kg}} \)  

\( u_1 = u_f \, \text{at} \, 70^\circ \text{C} = 292.95 \, \frac{\text{kJ}}{\text{kg}} \)  
\( h_{12} = h (20^\circ, x = 0) = 83.95 \)  

\( \Rightarrow (m_1 + \Delta m) u_2 - m_1 u_1 = \Delta m h_{12} + Q_R \)  
\( \Delta m (h_{12} - u_2) = -m_1 u_1 + m_1 u_2 - Q_R \)  
\( \Delta m = \frac{-m_1 u_1 + m_1 u_2 - Q_R}{h_{12} - u_2} \)

Delta m equals negative 5755 times (429.377) plus 5755 times (292.95) minus 35 times 10 to the power of 6, divided by (83.95 minus 292.95).  
Equals 3937 kilograms.