\( \Delta E = \Delta U = \dot{m} \cdot (u_1 - u_2) \)  
\( u_1 = x_D \cdot x \cdot u_g(100^\circ \text{C}) + (1 - x) \cdot u_f(100^\circ \text{C}) \)  
\( u_2 = u_f(70^\circ \text{C}) \)  
\( \rightarrow u_1 = 0.005 \cdot 2506.5 + 0.995 \cdot 418.91 \, \left( \frac{\text{kJ}}{\text{kg}} \right) = 429.38 \, \left( \frac{\text{kJ}}{\text{kg}} \right) \)  
\( u_2 = 292.35 \, \left( \frac{\text{kJ}}{\text{kg}} \right) \)  
\( \rightarrow \Delta E = 5755 \cdot (429.38 - 292.35) = 784432.45 \, \text{J} = 785.0 \, \text{MJ} \)  

\( \Delta E = \Delta m \cdot c_{\text{wasser}} \cdot \Delta T \)  
\( \Delta E = (m_{\text{total}} - m_D) \cdot c_w \cdot \Delta T \)  
\( m_{\text{total}} = \frac{\Delta E}{c_w \cdot \Delta T} + m_D \, , \, c_w = 4.22 \)  
\( m_{\text{total}} = \frac{785000 \, \text{J}}{4.22 \, \text{kJ/kgÂ·K} \cdot 30} + 5755 = 11475 \, \text{kg} \)  
\( \Delta m = 11475 - 5755 = 3720 \, \text{kg} \)