\( \dot{Q}_{aus} = 65 \, \text{kW} \)  

\( \frac{1}{T_{KF}} = \frac{s_{aus} - s_{ein}}{s_{aus} - s_{ein}} \)  

\( T \cdot ds = dU - p \cdot dV = dH \)  
\( dH = dU + p \cdot dV \)  

\( \frac{1}{T_{KF}} = \frac{s_{aus} - s_{ein}}{s_{aus} - s_{ein}} = \frac{h_{aus} - h_{ein}}{s_{aus} - s_{ein}} = C \cdot (T_{aus} - T_{ein}) \)  

\( \frac{1}{T_{KF}} = \frac{(T_{aus} - T_{ein})}{\mu \cdot \ln \left( \frac{T_2}{T_1} \right)} = \frac{T_{aus} - T_{ein}}{\ln \left( \frac{T_{2}}{T_{1}} \right)} = 293.1226 \, \text{K} \)