\( \Delta S = m_2 s_2 - m_1 s_1 = \Delta m_{12} s_{in} + \frac{Q_R - Q_{out}}{T} + \dot{S}_{erz} \)  

\( S_{12} = (m_1 + \Delta m_{12}) S_2 - m_1 S_1 \)  

\( S_1 = S_f (100^\circ \text{C}) + x_D \cdot \big(S_g (100^\circ \text{C}) - S_f (100^\circ \text{C})\big) = 1.33774 \, \frac{\text{kJ}}{\text{kg·K}} \)  
\( S_g (100^\circ \text{C}) = 7.35849 \, \frac{\text{kJ}}{\text{kg·K}} \)  
\( S_f (100^\circ \text{C}) = 1.30649 \, \frac{\text{kJ}}{\text{kg·K}} \)  

\( S_2 = S_f (70^\circ \text{C}) = 0.95889 \, \frac{\text{kJ}}{\text{kg·K}} \)  

\( S_{12} = 7237.85 \, \frac{\text{kJ}}{\text{kg·K}} \)