\( x_{Eis} = \frac{u_2 - u_f}{u_f - u_f} \)  
\( = \frac{u_2 - u_f}{u_f - u_f} = -185.090 \, \text{kJ} + 333.458 \, \text{kJ} \)  

**Zustand 1:**  
0.06 kg Eis  
0.04 kg Wasser  

\( u_n = -333.458 \, \frac{\text{kJ}}{\text{kg}} \cdot 0.06 \, \text{kg} - 0.045 \, \frac{\text{kJ}}{\text{kg}} \cdot 0.04 \, \text{kg} = -20.009 \, \text{kJ} \)  

\( Q_{12} = \Delta U = u_2 - u_1 \)  
\( u_2 = Q_{12} + u_1 = -185.090 - 20.0097 = -185.090 \, \text{kJ} \)  

\( u_2 = \frac{u_m}{m} = -185.090 \, \frac{\text{kJ}}{\text{kg}} \)  

\( X = \frac{u_2 - u_{f, Wasser}}{u_{Fest} - u_{Fl√ºssig}} = \frac{-185.090 + 0.045}{-333.458 + 0.045} = 0.555 \)