\( w_6^2 \), \( T_6^2 \), \( p_0 = 0.191 \, \text{bar} \)  

\( O = \dot{m}_{\text{ges}} (h_5 - h_6 + \frac{1}{2} m w_5^2 - \frac{1}{2} m w_6^2) \)  
\( \dot{m}_{\text{ges}} \to O = i_{\text{ges}} \)  

\( h_5 = h (437.9 \, \text{K}, 0.5 \, \text{bar}) = A - 22 \)  
\( A = 490 \), \( C = 431.9 \times 10^3 \), \( B = 490 \), \( D = 441.61 \times 10^3 \)  
\( D - C = 433.364.2 = 433.369.10^3 \, \text{J/kg} \)  

\( h_6 = h (0.491 \, \text{bar}, 328.07 \, \text{K}) = \)  
\( \frac{T_6}{T_5} = \frac{p_6}{p_5}^{n-1/n} \)  
\( T_5 = 437.9 \, \text{K} \), \( T_6 = 328.07 \, \text{K} \)  

\( A = 325 \), \( C = 32.37 \times 10^3 \), \( D = 330.34 \times 10^3 \)  
\( C + 320 - 325 \), \( D - C = 328.398.92 \, \text{J/kg} \)  

\( w_6^2 = \frac{1}{2} m w_5^2 - \frac{1}{2} m w_6^2 \to w_6^2 = \frac{2}{m} (h_5 - h_6) + w_5^2 \)  
\( w_6 = \sqrt{\frac{1}{2} (h_5 - h_6) + w_5^2} = \frac{m = 1}{m} + w_5^2 = 508.26 \, \text{m/s} \)