\( m_2 u_2 - m_1 u_1 = \Delta m_{12} h_2 - h_1 \)  

\( m_2 u_2 - m_1 u_1 = \Delta m_{12} (h_2 - h_1) \)  

\( m_1 = 5755 \, \text{kg} \)  

\( m_2 = m_1 + \Delta m_{12} \)  

\( u_2 = x u_g + (1 - x) u_f = 429.32 \, \text{kJ/kg} \)  

\( u_g = 2506.5 \, \text{kJ/kg} \)  

\( u_f = 429.84 \, \text{kJ/kg} \)  

(from Table A-2)  

\( x = 0.005 \)  

\( u_2 = h_{fg}(70^\circ \text{C}) = 2333.8 \, \text{kJ/kg} \)  

(from Table A-2)  

(because of volume change)  

\( h_1 = h_{fg}(20^\circ \text{C}) = 2454.1 \, \text{kJ/kg} \)  

(from Table A-2)  

\( h_2 = h_{fg}(70^\circ \text{C}) = 2333.8 \, \text{kJ/kg} \)  

(from Table A-2)  

\( (m_1 + \Delta m_{12}) u_2 - m_1 u_1 = \Delta m_{12} (h_2 - h_1) \)  

\( \Delta m_{12} (u_2 - h_2 + h_1) = m_1 u_1 - u_2 m_1 \)  

\( \Delta m_{12} = \frac{-m_1 u_1 + m_1 u_2}{u_2 - h_2 + h_1} \)  

\( \Delta m_{12} = \frac{m_1 (u_2 + u_1)}{h_1 - h_2} \)  

\( \Delta m_{12} = 4468.31 \, \text{kg} \)