\( Q_{12} = x_{Eis,2} \cdot m_{EW} \cdot (u_{W,2} - u_{Eis,2}) + (1 - x_{Eis,2}) \cdot m_{EW} \cdot (u_{W,2} - u_{W,1}) - m_g \cdot (u_{g,2} - u_{g,1}) \)  

Given:  
\( m_{EW} = 0.1 \, \text{kg} \)  
\( u_{Eis,2} = u_{\text{fest}} (0^\circ \text{C}) = -333.442 \, \text{kJ/kg} \)  
\( u_{W,2} = u_{\text{flüssig}} (0^\circ \text{C}) = -0.033 \, \text{kJ/kg} \)  
\( u_{Eis,1} = u_{\text{fest}} (0^\circ \text{C}) = -333.455 \, \text{kJ/kg} \)  
\( u_{W,1} = u_{\text{flüssig}} (0^\circ \text{C}) = -0.045 \, \text{kJ/kg} \)