Delta E equals Delta U equals m 2 times u 2 minus m 1 times u 1 equals Delta m 12 times h in,12 minus Q out,12.  

Delta m 12 equals m 2 times u 2 minus m 1 times u 1 plus Q out,12 divided by h in,12.

\((m_1 + \Delta m_{12}) U_2 - m_1 U_1 = \Delta m_{12} \, h_{ein,12} - Q_{aus,12}\)  

\(\Delta m_{12} (U_2 - h_{ein,12}) = m_1 U_1 - m_1 U_2 - Q_{aus,12}\)  

\(\Delta m_{12} = \frac{m_1 U_1 - m_1 U_2 - Q_{aus,12}}{U_2 - h_{ein,12}}\), \(m_1 = m_{ges,1} = 5755 \, \text{kg}\)  

\(h_{ein,12} = h(20^\circ \text{C}, x = 0) = h_f(20^\circ \text{C}) = 83.36 \, \text{kJ/kg} \, \text{(A-2)}\)  

\(U_1 = U(100^\circ \text{C}, x = 0) = u_f(100^\circ \text{C}) = 418.94 \, \text{kJ/kg} \, \text{(A-2)}\)  

\(U_2 = U(70^\circ \text{C}, x = 0) = u_f(70^\circ \text{C}) = 282.95 \, \text{kJ/kg} \, \text{(A-2)}\)  

\(\Delta U_{12} = U_1 = U(100^\circ \text{C}, x = 0.005) - U_f(100^\circ \text{C}) + x \, (U_g(100^\circ \text{C}) - U_f(100^\circ \text{C}))\)  

\(\Delta U_{12} = 429.38 \, \text{kJ/kg} \, \text{(A-2)}\)  

\(\Delta m_{12} = 3588.4 \, \text{kg}\)