\( ex_{str,6} - ex_{str,0} = \dot{m} (h_6 - h_0 - T_0 (s_6 - s_0) + \frac{ke}{\dot{m}} ) \)  

\( h_6 - h_0 = c_p (T_6 - T_0) = 1.006 \, \text{kJ/kgÂ·K} (328.07 - 243.15) = 85.43 \, \text{kJ/kg} \)  

\( T_0 (s_6 - s_0) = 243.15 \, \text{K} \left( c_p \ln \left( \frac{T_6}{T_0} \right) - R \ln \left( \frac{p_6}{p_0} \right) \right) \)  

\( = 243.15 \, \text{K} \left( 1.006 \ln \left( \frac{328.07}{243.15} \right) \right) = 73.27 \, \text{kJ} \)  

\( \Delta ex_{str,6} = \dot{m} (85.43 - 73.27) \)  

\( ke = \frac{w_6^2}{2} = \frac{50.2^2}{2} = 1285.13 \, \text{W} \)  

Total \( \Delta ex_{str,1 \to 6} = (85.43 + 73.27 + 1285.13) \, \text{kW} \)  

\( = 140.82 \, \text{kW} = \Delta ex \)  

---