The following equations and calculations are written:  

Steady-state process:  
\( 0 = \dot{m} (h_e - h_a + \frac{w_e^2 - w_a^2}{2}) + Q - W \)  

Adiabatic:  
\( Q = 0 \)  

Rearranged:  
\( h_e - h_a = c_p (T_e - T_a) = \frac{w_e^2}{2} \)  

\( h_e - h_a = \int c_p dT = c_p (T_e - T_a) \)  

Adiabatic:  
\( \frac{T_6}{T_5} = (\frac{p_6}{p_5})^{\frac{\kappa - 1}{\kappa}} \)  

\( T_6 = 431.9 \, \text{K} \cdot (0.191 / 0.5)^{0.4 / 1.4} = 323.075 \, \text{K} \)  

\( w_6^2 = 2 [c_p (T_2 - T_1) + \frac{w_e^2}{2}] = 257.28 \, \text{m/s}^2 \)  

\( w_6 = 507.24 \, \text{m/s} \)