The equation for \( w_6 \) is written as:  
\( w_6 = 2 \)  

The equation for \( T_6 \) is written as:  
\( T_6 = T_5 \cdot \left( \frac{p_6}{p_5} \right)^{\frac{n-1}{n}} \)  

Substituting values:  
\( T_6 = 431.69 \cdot \left( \frac{0.101}{0.5} \right)^{\frac{0.4}{1.4}} \)  

The calculation yields:  
\( T_6 = 328.075 \, \text{K} \)  

The result is boxed.  

An additional equation is written for \( w_6 \):  
\( w_6 = \dot{m} \cdot \left( h_5 - h_6 + \frac{w_5^2}{2} - \frac{w_6^2}{2} \right) \)