\( T_{g,2} = 0^\circ \text{C} \)  

First law:  
\( \Delta U_{12,\text{EW}} = Q - W = (7.36 \, \text{kJ} - 0.2852 \, \text{kJ}) \, \text{kJ} = 7.052 \, \text{kJ} \)  

\( \Delta U_{12} = m_{\text{EW}} \cdot (u_2 - u_1) \)  

\( u_2 = x_2 \cdot u_f(0^\circ \text{C}) + (1 - x_2) \cdot u_i(0^\circ \text{C}) \)  

\( u_1 = u_i(0^\circ \text{C}) \cdot (1 - x_1) + u_f(0^\circ \text{C}) \cdot x_1 \), \( x_1 = 0.6 \)  

\( m_{\text{EW}} \cdot (u_2 - u_1) = x_2 \cdot (u_f(T_i) - u_i(T_i)) + u_i(T_i) - u_1 = \Delta U_{12} \)  

\( x_2 = \frac{\Delta U_{12} + u_1 - u_i(T_i)}{u_f(T_i) - u_i(T_i)} \)  

\( x = \frac{7.052 \, \text{kJ}}{0.1 \, \text{kg}} \cdot \frac{(-0.085 \, \text{kJ/kg})}{(-333.552 \, \text{kJ/kg}) \cdot 0.6 - (-0.053 \, \text{kJ/kg})} \)  

\( x = \frac{-333.452 \, \text{kJ/kg} - (-0.053 \, \text{kJ/kg})} \)  

\( = 0.575 \)