\( \dot{e}_{x,str} \frac{d}{dt} = \dot{e}_{x,str,in} + \dot{e}_{x,str,out} - \left[ \dot{m} \frac{e_0 \Delta u(t)}{dt} \right] = \dot{e}_{x,verl} \)  

\( \Rightarrow \dot{e}_{x,verl} = e_{x,str,0} + e_{x,str,Q} \)  

\( e_{x,str,Q} = \frac{\dot{E}_{x,Q}}{\dot{m}} = \frac{1}{\dot{m}_K} \left( 1 - \frac{T_0}{T} \right) \cdot \dot{Q} = \left( 1 - \frac{T_0}{T} \right) q \cdot y \)  

\( q = 1195 \, \text{kJ/kg} \)  
\( T = 1289 \, \text{K} \)  

\( y = \dot{m}_M / \dot{m}_K \)  
\( \dot{m}_M = \dot{m}_K + 5.293 \cdot \dot{m}_K \)  
\( \dot{m}_M / \dot{m}_K = 6.293 \)  

\( e_{x,str,Q} = 116.605 \, \text{kJ/kg} + \frac{869.58 \cdot 1}{6.293} \, \text{kJ/kg} \)  

\( = 270.62 \, \text{kJ/kg} \)