\( \Delta E = -|Q_{12}| - W_{12}^{\circ} \), as it is isochoric.

\( m_{EW} (u_{2,EW} - u_{1,EW}) = -Q_{12} \)

At \( 0^\circ \text{C} \): \( u_{EW} = u_{\text{flüssig}} + x_{A} (u_{\text{Eis}} - u_{\text{flüssig}}) \)

\( u_{\text{flüssig}} (0^\circ \text{C}) = -0.045 \, \frac{\text{kJ}}{\text{kg}} \)

\( u_{\text{Eis}} (0^\circ \text{C}) = -333.45 \, \frac{\text{kJ}}{\text{kg}} \)

\( u_{EW} = -209.08 \, \frac{\text{kJ}}{\text{kg}} \)

At \( 0^\circ \text{C} \): \( u_{2,EW} = u_{\text{flüssig}} + x_{2} (u_{\text{Eis}} - u_{\text{flüssig}}) \)

\( T_{EW,2} = T_{g,2} \)

\( u_{\text{flüssig}} (0.003^\circ \text{C}) = -0.033 \, \frac{\text{kJ}}{\text{kg}} \)

\( u_{\text{Eis}} (0.003^\circ \text{C}) = -333.44 \, \frac{\text{kJ}}{\text{kg}} \)

\( -\frac{Q_{12}}{m_{EW}} + u_{1,EW} = u_{2,EW} \)

\( u_{EW} = u_{\text{flüssig}} + x_{2} (u_{\text{Eis}} - u_{\text{flüssig}}) \)

\( x_{2} = \frac{Q_{12}}{m_{EW}} + u_{1,EW} - u_{\text{flüssig}} \)

\( u_{\text{Eis}} (0.003^\circ \text{C}) = -333.44 \, \frac{\text{kJ}}{\text{kg}} \)

\( E = \text{Fest} \), \( F = \text{Flüssig} \)