Given: \( \dot{Q}_{out} \)  

Steady-state flow process:  
0 = \( \dot{m}_{in} \cdot (h_e - h_a) + \frac{w_e^2 - w_a^2}{2} - g \cdot (z_e - z_a) + \sum \dot{Q}_j - \sum \dot{W}_j \)  

\( \Rightarrow \) 0 = \( \dot{m}_{in} \cdot (h_e - h_a) + \sum \dot{Q}_j \)  

\( \Rightarrow \) 0 = \( \dot{m}_{in} \cdot (h_e - h_a) + \( \dot{Q}_R \) - \( \dot{Q}_{out} \)  

\( \Rightarrow \dot{Q}_{out} = \dot{m}_{in} \cdot (h_e - h_a) + \( \dot{Q}_R \)  

\( = \dot{m}_{in} \cdot (292.98 \, \text{kJ/kg} - 419.04 \, \text{kJ/kg}) + 100 \, \text{kW} \)  

\( = 0.3 \, \text{kg/s} \cdot (292.98 \, \text{kJ/kg} - 419.04 \, \text{kJ/kg}) + 100 \, \text{kW} \)  

\( = 62.182 \, \text{kJ/s} = 62.182 \, \text{kW} \)  

Values for \( h_f \) come from Table A2!