\( m_{EW} (u_2 - u_1) + m_g (u_2 - u_1) = Q_{12} - W_{12} = 0 \)  

\( p_g = p_{EW} \)  

\( u_{1,EW} = u_{f} - 333.638 \, \text{kJ/kg} + x \cdot (-0.05 \, \text{kJ/kg} + 333.638 \, \text{kJ/kg}) = -133.641 \, \text{kJ/kg} \)  

\( m_g (u_2 - u_1) = m_g c_V (T_2 - T_1) = -1.082 \, \text{kJ} \)  

\( u_{2,EW} = u_{f} + \frac{-m_g (u_2 - u_1)}{m_{EW}} = -122.55 \, \text{kJ/kg} \)  

\( p_{2,EW} = p_{1,EW} = 1.48 \, \text{bar} \)  

\( T_{1,EW} = T_{2,EW} \)  

\( x = \frac{u_{2,EW} + 333.638 \, \text{kJ/kg}}{-0.05 \, \text{kJ/kg} + 333.638 \, \text{kJ/kg}} = 0.632 \)