\( m_2 \, u_2 - m_1 \, u_1 = \Delta m_2 \, (h_{ein}) + Q_{R} \)  
\( Q_{R} = Q_{out} \, \text{(energy balance)} \)  

\( \Delta m_2 = m_2 \, u_2 - m_1 \, u_1 - Q_{R} \)  

\( u_1 = u_f(100^\circ \text{C}) + x_D \, (u_g(100^\circ \text{C}) - u_f(100^\circ \text{C})) = 429.38 \, \text{kJ/kg} \)  

\( h_{ein}(20^\circ \text{C}) = h_f(20^\circ \text{C}) = 83.35 \, \text{kJ/kg} \)  

\( u_2(70^\circ \text{C}) = u_f(70^\circ \text{C}) = 232.35 \, \text{kJ/kg} \)  

\( \Delta m_2 = m_2 - m_1 \)  

\( m_2 \, u_2 - m_1 \, u_1 = (m_2 - m_1) \, h_{ein} + Q_{R} \)  

\( m_2 = m_1 \, u_1 - m_{ein} \, h_{ein} \)  

\( m_2 = \frac{Q_{R}}{u_2 - h_{ein}} \)  

\( m_2 = 5511.72 \, \text{kg} \)  

\( \Delta m_2 = 5511.72 - 5755 = 376.72 \, \text{kg} \)  

---