Equations and calculations are written:  

\( 0 = \dot{m}_{65} \left[ h_5 - h_6 + \frac{(w_5^2 - w_6^2)}{2} \right] + \dot{Q}_{56} + \dot{W}_{56} \)  

\( 0 = \dot{m}_{65} \left[ h_0 - h_6 + \frac{(w_5^2 - w_6^2)}{2} \right] + \dot{Q}_{0} - \dot{W}_{0} \)  

\( h_0 - h_6 = c_p (T_0 - T_6) \)  

\( \frac{T_1}{T_5} = \left( \frac{p_0}{p_5} \right)^{\frac{\kappa - 1}{\kappa}} \Rightarrow T_6 = T_1 \left( \frac{p_0}{p_5} \right)^{\frac{\kappa - 1}{\kappa}} = 431.51 K \left( \frac{0.191 \, \text{bar}}{0.5 \, \text{bar}} \right)^{\frac{0.4}{1.4}} = 325.07 K = T_6 \)  

\( \Rightarrow p_2 c_p (T_0 - T_6) + \frac{(w_2^2 - w_6^2)}{2} = 0 \)  

\( \Rightarrow 2 c_p (T_0 - T_6) - w_0^2 = -w_0^2 \)  

\( \Rightarrow \sqrt{w_0^2 + 2 c_p (T_0 - T_6)} = w_0 \)  

\( \Rightarrow w_0 = \sqrt{200^2 - 2 \cdot 1.006 \, \text{kJ/kgÂ·K} \cdot (243.15 - 325.07)} = 453.19 \, \text{m/s} \)  

The final result is underlined: \( w_0 = 453.19 \, \text{m/s} \).

Zero equals mass flow rate multiplied by the difference in stream exergy minus the exergy loss.  

Zero equals the difference in stream exergy minus the exergy loss.  

Exergy loss equals:  
\[ 122.21 \, \text{kJ/kg} \]