TASK 1d  
Energy balance for an open system:  
\[
\Delta E = m_2 \cdot u_2 - m_1 \cdot u_1 = \Delta m_{12} \cdot h_{12} + Q_{R,12} - Q_{\text{out},12}
\]  
(Note: \( Q_{R,12} - Q_{\text{out},12} \) is crossed out in the equation.)  

Definitions:  
\[
m_2 = m_{\text{ges},1} + \Delta m_{12}, \quad m_1 = m_{\text{ges},1}
\]  

From Table A2:  
\[
u_2 = u_f(70^\circ\text{C}) = 292.95 \, \frac{\text{kJ}}{\text{kg}}
\]  
\[
u_f(100^\circ\text{C}) = 418.94 \, \frac{\text{kJ}}{\text{kg}}, \quad u_g(100^\circ\text{C}) = 2506.5 \, \frac{\text{kJ}}{\text{kg}}
\]  
\[
h_{12} = h_f(20^\circ\text{C}) = 83.96 \, \frac{\text{kJ}}{\text{kg}}
\]  

For \( u_1 \):  
\[
u_1 = u_f + x_D \cdot (u_g - u_f) = 429.36 \, \frac{\text{kJ}}{\text{kg}}
\]  

Energy balance equation:  
\[
(m_1 + \Delta m_{12}) \cdot u_2 - m_1 \cdot u_1 = \Delta m_{12} \cdot h_{12}
\]  
Rearranging:  
\[
\Delta m_{12} \cdot (u_2 - h_{12}) = m_1 \cdot u_1 - m_1 \cdot u_2
\]  
Solving for \( \Delta m_{12} \):  
\[
\Delta m_{12} = \frac{m_1 \cdot u_1 - m_1 \cdot u_2}{u_2 - h_{12}}
\]  

Final result:  
\[
\Delta m_{12} = 3756.43 \, \text{kg}
\]  

---

TASK 1e  
Entropy change:  
\[
\Delta S = m_2 \cdot s_2 - m_1 \cdot s_1
\]  
Substituting:  
\[
\Delta S = (m_1 + \Delta m_{12}) \cdot s_2 - m_1 \cdot s_1
\]  

Final result:  
\[
\Delta S_{12} = 1387.22 \, \frac{\text{kJ}}{\text{K}}
\]  

From Table A2:  
\[
s_2 = s_f(70^\circ\text{C}) = 0.954 \, \frac{\text{kJ}}{\text{kg路K}}
\]  
\[
s_1 = s_f(100^\circ\text{C}) + x_D \cdot (s_g(100^\circ\text{C}) - s_f(100^\circ\text{C}))
\]  
\[
s_1 = 1.306 \, \frac{\text{kJ}}{\text{kg路K}} + 7.3749 \, \frac{\text{kJ}}{\text{kg路K}}
\]  
\[
s_1 = 1.33714 \, \frac{\text{kJ}}{\text{kg路K}}
\]