TASK 2c  
The change in flow exergy is expressed as:  
\[
\Delta ex_{\text{str}} = \left( h_6 - h_0 - T_0(s_6 - s_0) + \Delta e \right)
\]  
Substituting the values:  
\[
= \left( h_6 - h_0 - T_0(s_6 - s_0) + \Delta e \right)
\]  
With further substitutions and simplifications:  
\[
= \left( c_p \ln\left(\frac{T_6}{T_0}\right) - R \ln\left(\frac{p_6}{p_0}\right) + \frac{w_6^2}{2} - \frac{w_0^2}{2} \right)
\]  
Numerical calculation yields:  
\[
12547.75 \, \frac{\text{J}}{\text{kg}} = 12.547 \, \frac{\text{kJ}}{\text{kg}}
\]  

TASK 2d  
The exergy destruction is calculated using the equation:  
\[
0 = \Delta ex_{\text{str}} + \sum \left(1 - \frac{T_c}{T_0}\right) \dot{Q} - \dot{W}_{\text{in}} - \dot{e}_{\text{x,in}}
\]  
Breaking down the terms:  
\[
-e_{\text{x,in}} = \Delta ex_{\text{str}} - \frac{\dot{W}_{\text{in}}}{\dot{m}_K}
\]  
The specific exergy destruction is expressed as:  
\[
e_{\text{x,in}} = T_0 \cdot \dot{S}_{\text{gen}} = T_0 \left(s_a - s_e\right) = T_0 \left(s_6 - s_0\right)
\]  
Substituting the values:  
\[
= T_0 \left(c_p \ln\left(\frac{T_0}{T_5}\right) - R \ln\left(\frac{p_0}{p_5}\right)\right)
\]  
Numerical calculation yields:  
\[
15421.75 \, \frac{\text{J}}{\text{kg}} = 15.422 \, \frac{\text{kJ}}{\text{kg}}
\]  