TASK 1a  
The first law of thermodynamics is applied:  
\[
\dot{Q}_{\text{out}} = \dot{m} (h_e - h_a) + \dot{Q}_R
\]  

The enthalpy values are determined:  
\[
h_e = h(T = 100^\circ\text{C}) = h_fg(T = 100^\circ\text{C}) + h_a
\]  
\[
h_a = h(T = 70^\circ\text{C}) = h_fg(T = 70^\circ\text{C}) + h_a
\]  

From Table A2:  
\[
h_e = 2333.845 \, \frac{\text{kJ}}{\text{kg}}
\]  
\[
h_a = 2252 \, \frac{\text{kJ}}{\text{kg}}
\]  

Substituting into the equation:  
\[
\dot{Q}_{\text{out}} = 0.3 \cdot (2252 - 2333.8) + 100 \, \text{kW} = 70.36 \, \text{kW}
\]  

TASK 1b  
Continuing with \( \dot{Q}_{\text{out}} = 65 \, \text{kW} \):  

The entropy change is calculated:  
\[
\Delta S = S_e - S_a = \frac{\dot{Q}_{\text{out}}}{T_j}
\]  

The thermodynamic mean temperature \( T_j \) is determined:  
\[
T_j = \frac{\int T \, dS}{S_e - S_a} = \frac{S_e \cdot T_e - S_a \cdot T_a}{S_e - S_a}
\]  

The entropy values are expressed:  
\[
S_e - S_a = \int_{T_a}^{T_e} \frac{c}{T} \, dT = \ln(T_e) - \ln(T_a)
\]  

Final expressions for entropy difference are left incomplete.