TASK 2c  
The mass-specific increase in flow exergy \( \Delta ex_{\text{flow}} \) is calculated using the following equation:  
\[
\Delta ex_{\text{flow}} = (h_6 - h_0) - T_0 (s_6 - s_0) + \frac{w_6^2 - w_0^2}{2}
\]

The enthalpy difference \( h_6 - h_0 \) is given by:  
\[
h_6 - h_0 = c_{p,\text{air}} (T_6 - T_0) = 1.006 \, \frac{\text{kJ}}{\text{kg·K}} (328.16 - 243.15) = 85.4597 \, \frac{\text{kJ}}{\text{kg}}
\]

The entropy difference \( T_0 (s_6 - s_0) \) is calculated as:  
\[
T_0 (s_6 - s_0) = T_0 \left( c_{p,\text{air}} \ln \left( \frac{T_6}{T_0} \right) - R \ln \left( \frac{p_6}{p_0} \right) \right)
\]
Since \( p_6 = p_0 \), the pressure term vanishes, and the equation simplifies to:  
\[
T_0 (s_6 - s_0) = 243.15 \, \text{K} \cdot \frac{1.006 \, \text{kJ}}{\text{kg·K}} \ln \left( \frac{328.1}{243.15} \right) = 73.2946 \, \frac{\text{kJ}}{\text{kg}}
\]

The kinetic energy term \( \frac{w_6^2 - w_0^2}{2} \) is calculated as:  
\[
\frac{w_6^2 - w_0^2}{2} = \frac{507.1^2 \, \frac{\text{m}^2}{\text{s}^2} - 200^2 \, \frac{\text{m}^2}{\text{s}^2}}{2} = \frac{108620.85 \, \frac{\text{J}}{\text{kg}}}{2} = 108.621 \, \frac{\text{kJ}}{\text{kg}}
\]

Combining all terms:  
\[
\Delta ex_{\text{flow}} = 85.4597 \, \frac{\text{kJ}}{\text{kg}} - 73.2946 \, \frac{\text{kJ}}{\text{kg}} + 108.621 \, \frac{\text{kJ}}{\text{kg}} = 120.786 \, \frac{\text{kJ}}{\text{kg}}
\]

---

TASK 2d  
The mass-specific exergy destruction \( ex_{\text{dest}} \) is calculated using the exergy balance for a stationary system:  
\[
0 = (h_{\text{in}} - h_{\text{out}}) - T_0 (s_{\text{in}} - s_{\text{out}}) + Q_{\text{in}} + \left( 1 - \frac{T_0}{T_B} \right) Q_B - W_{\text{rev}} - ex_{\text{dest}}
\]
Rearranging:  
\[
ex_{\text{dest}} = -\Delta ex_{\text{flow}} + \left( 1 - \frac{T_0}{T_B} \right) Q_B
\]

Substituting values:  
\[
ex_{\text{dest}} = -120.786 \, \frac{\text{kJ}}{\text{kg}} + \left( 1 - \frac{243.15 \, \text{K}}{1289 \, \text{K}} \right) \cdot 1195 \, \frac{\text{kJ}}{\text{kg}}
\]

Simplifying:  
\[
ex_{\text{dest}} = -120.786 \, \frac{\text{kJ}}{\text{kg}} + \left( 1 - 0.1887 \right) \cdot 1195 \, \frac{\text{kJ}}{\text{kg}}
\]
\[
ex_{\text{dest}} = -120.786 \, \frac{\text{kJ}}{\text{kg}} + 0.8113 \cdot 1195 \, \frac{\text{kJ}}{\text{kg}}
\]
\[
ex_{\text{dest}} = -120.786 \, \frac{\text{kJ}}{\text{kg}} + 968.796 \, \frac{\text{kJ}}{\text{kg}} = 848.796 \, \frac{\text{kJ}}{\text{kg}}
\]